@prefix rdfs: <http://www.w3.org/2000/01/rdf-schema#> .
@prefix xsd: <http://www.w3.org/2001/XMLSchema#> .
@prefix owl: <http://www.w3.org/2002/07/owl#> .
@prefix rdf: <http://www.w3.org/1999/02/22-rdf-syntax-ns#> .
@prefix dct: <http://purl.org/dc/terms/> .
@prefix prov: <http://www.w3.org/ns/prov#> .
@prefix : <http://purl.org/ontology/edu/eso/> .

<http://purl.org/ontology/edu/eso/eso.ttl> rdf:type owl:Ontology ;
    dct:creator "Sabbir M. Rashid"^^xsd:string ;
    dct:contributor "Deborah L. McGuiness"^^xsd:string ;
    dct:created "2017-05-15T12:00:00"^^xsd:dateTime ;
    dct:modified "2018-05-31T12:00:00"^^xsd:dateTime ;
    dct:description "Education Standards Ontology based on the Common Core Standards"^^xsd:string ;
    dct:title "Education Standards Ontology"^^xsd:string ;
    dct:license <http://www.apache.org/licenses/LICENSE-2.0> , <http://www.corestandards.org/public-license/> ;
    owl:versionIRI <http://purl.org/ontology/edu/eso/0.9> ;
    prov:wasQuotedFrom <http://www.corestandards.org/> .

:CCSS.ELA-Literacy rdf:type owl:Class ;
    rdfs:label "English Language Arts Standards"^^xsd:string ;
    prov:wasQuotedFrom <http://www.corestandards.org/ELA-Literacy/> .

:CCSS.ELA-Literacy.introduction rdf:type owl:Class ;
    rdfs:subClassOf :CCSS.ELA-Literacy ;
    rdfs:label "Introduction"^^xsd:string ;
    prov:wasQuotedFrom <http://www.corestandards.org/ELA-Literacy/introduction/> .

:CCSS.ELA-Literacy.introduction.how-to-read-the-standards rdf:type owl:Class ;
    rdfs:subClassOf :CCSS.ELA-Literacy.introduction ;
    prov:wasQuotedFrom <http://www.corestandards.org/ELA-Literacy/introduction/how-to-read-the-standards/> ;
    rdfs:label "English Language Arts Standards - Introduction - How to Read the Standards"^^xsd:string ;
    rdfs:comment "The Standards comprise three main sections: a comprehensive K-5 section and two content area-specific sections for grades 6-12, one for ELA and one for history/social studies, science, and technical subjects. Three appendices accompany the main document."^^xsd:string .

:CCSS.ELA-Literacy.introduction.key-design-consideration rdf:type owl:Class ;
    rdfs:subClassOf :CCSS.ELA-Literacy.introduction ;
    prov:wasQuotedFrom <http://www.corestandards.org/ELA-Literacy/introduction/key-design-consideration/> ;
    rdfs:label "English Language Arts Standards - Introduction - Key Design Consideration"^^xsd:string ;
    rdfs:comment "The CCR standards anchor the document and define general, cross-disciplinary literacy expectations that must be met for students to be prepared to enter college and workforce training programs ready to succeed. The K-12 grade-specific standards define end-of-year expectations and a cumulative progression designed to enable students to meet college and career readiness expectations no later than the end of high school. The CCR and high school (grades 9-12) standards work in tandem to define the college and career readiness line-the former providing broad standards, the latter providing additional specificity. Hence, both should be considered when developing college and career readiness assessments."^^xsd:string .

:CCSS.ELA-Literacy.introduction.students-who-are-college-and-career-ready-in-reading-writing-speaking-listening-language rdf:type owl:Class ;
    rdfs:subClassOf :CCSS.ELA-Literacy.introduction ;
    prov:wasQuotedFrom <http://www.corestandards.org/ELA-Literacy/introduction/students-who-are-college-and-career-ready-in-reading-writing-speaking-listening-language/> ;
    rdfs:label "English Language Arts Standards - Introduction - Students Who are College and Career Ready in Reading, Writing, Speaking, Listening, & Language"^^xsd:string ;
    rdfs:comment "The descriptions that follow are not standards themselves but instead offer a portrait of students who meet the standards set out in this document. As students advance through the grades and master the standards in reading, writing, speaking, listening, and language, they are able to exhibit with increasing fullness and regularity these capacities of the literate individual."^^xsd:string .

:CCSS.ELA-Literacy.CCRA rdf:type owl:Class ;
    rdfs:subClassOf :CCSS.ELA-Literacy ;
    rdfs:label "Anchor Standards"^^xsd:string ;
    prov:wasQuotedFrom <http://www.corestandards.org/ELA-Literacy/CCRA/> .

:CCSS.ELA-Literacy.CCRA.L rdf:type owl:Class ;
    rdfs:subClassOf :CCSS.ELA-Literacy.CCRA ;
    prov:wasQuotedFrom <http://www.corestandards.org/ELA-Literacy/CCRA/L/> ;
    rdfs:label "English Language Arts Standards - Anchor Standards - College and Career Readiness Anchor Standards for Language"^^xsd:string ;
    rdfs:comment "The K-12 standards on the following pages define what students should understand and be able to do by the end of each grade. They correspond to the College and Career Readiness (CCR) anchor standards below by number. The CCR and grade-specific standards are necessary complements-the former providing broad standards, the latter providing additional specificity-that together define the skills and understandings that all students must demonstrate."^^xsd:string .

:CCSS.ELA-Literacy.CCRA.R rdf:type owl:Class ;
    rdfs:subClassOf :CCSS.ELA-Literacy.CCRA ;
    prov:wasQuotedFrom <http://www.corestandards.org/ELA-Literacy/CCRA/R/> ;
    rdfs:label "English Language Arts Standards - Anchor Standards - College and Career Readiness Anchor Standards for Reading"^^xsd:string ;
    rdfs:comment "The K-12 standards on the following pages define what students should understand and be able to do by the end of each grade. They correspond to the College and Career Readiness (CCR) anchor standards below by number. The CCR and grade-specific standards are necessary complements-the former providing broad standards, the latter providing additional specificity-that together define the skills and understandings that all students must demonstrate."^^xsd:string .

:CCSS.ELA-Literacy.CCRA.SL rdf:type owl:Class ;
    rdfs:subClassOf :CCSS.ELA-Literacy.CCRA ;
    prov:wasQuotedFrom <http://www.corestandards.org/ELA-Literacy/CCRA/SL/> ;
    rdfs:label "English Language Arts Standards - Anchor Standards - College and Career Readiness Anchor Standards for Speaking and Listening"^^xsd:string ;
    rdfs:comment "The K-12 standards on the following pages define what students should understand and be able to do by the end of each grade. They correspond to the College and Career Readiness (CCR) anchor standards below by number. The CCR and grade-specific standards are necessary complements-the former providing broad standards, the latter providing additional specificity-that together define the skills and understandings that all students must demonstrate. "^^xsd:string .

:CCSS.ELA-Literacy.CCRA.W rdf:type owl:Class ;
    rdfs:subClassOf :CCSS.ELA-Literacy.CCRA ;
    prov:wasQuotedFrom <http://www.corestandards.org/ELA-Literacy/CCRA/W/> ;
    rdfs:label "English Language Arts Standards - Anchor Standards - College and Career Readiness Anchor Standards for Writing "^^xsd:string ;
    rdfs:comment "The K-12 standards on the following pages define what students should understand and be able to do by the end of each grade. They correspond to the College and Career Readiness (CCR) anchor standards below by number. The CCR and grade-specific standards are necessary complements-the former providing broad standards, the latter providing additional specificity-that together define the skills and understandings that all students must demonstrate."^^xsd:string .

:CCSS.ELA-Literacy.RL rdf:type owl:Class ;
    rdfs:subClassOf :CCSS.ELA-Literacy ;
    rdfs:label "Reading: Literature"^^xsd:string ;
    prov:wasQuotedFrom <http://www.corestandards.org/ELA-Literacy/RL/> .

:CCSS.ELA-Literacy.RL.introduction-for-k-5 rdf:type owl:Class ;
    rdfs:subClassOf :CCSS.ELA-Literacy.RL ;
    prov:wasQuotedFrom <http://www.corestandards.org/ELA-Literacy/RL/introduction-for-k-5/> ;
    rdfs:label "English Language Arts Standards - Reading: Literature - Introduction for K-5"^^xsd:string ;
    rdfs:comment "The following standards offer a focus for instruction each year and help ensure that students gain adequate exposure to a range of texts and tasks. Rigor is also infused through the requirement that students read increasingly complex texts through the grades. Students advancing through the grades are expected to meet each year-s grade-specific standards and retain or further develop skills and understandings mastered in preceding grades."^^xsd:string .

:CCSS.ELA-Literacy.RL.introduction-for-6-12 rdf:type owl:Class ;
    rdfs:subClassOf :CCSS.ELA-Literacy.RL ;
    prov:wasQuotedFrom <http://www.corestandards.org/ELA-Literacy/RL/introduction-for-6-12/> ;
    rdfs:label "English Language Arts Standards - Reading: Literature - Introduction for 6-12"^^xsd:string ;
    rdfs:comment "The following standards offer a focus for instruction each year and help ensure that students gain adequate exposure to a range of texts and tasks. Rigor is also infused through the requirement that students read increasingly complex texts through the grades. Students advancing through the grades are expected to meet each year-s grade-specific standards and retain or further develop skills and understandings mastered in preceding grades."^^xsd:string .

:CCSS.ELA-Literacy.RL.K rdf:type owl:Class ;
    rdfs:subClassOf :CCSS.ELA-Literacy.RL ;
    prov:wasQuotedFrom <http://www.corestandards.org/ELA-Literacy/RL/K/> ;
    rdfs:label "English Language Arts Standards - Reading: Literature - Kindergarten"^^xsd:string .

:CCSS.ELA-Literacy.RL.1 rdf:type owl:Class ;
    rdfs:subClassOf :CCSS.ELA-Literacy.RL ;
    prov:wasQuotedFrom <http://www.corestandards.org/ELA-Literacy/RL/1/> ;
    rdfs:label "English Language Arts Standards - Reading: Literature - Grade 1"^^xsd:string .

:CCSS.ELA-Literacy.RL.2 rdf:type owl:Class ;
    rdfs:subClassOf :CCSS.ELA-Literacy.RL ;
    prov:wasQuotedFrom <http://www.corestandards.org/ELA-Literacy/RL/2/> ;
    rdfs:label "English Language Arts Standards - Reading: Literature - Grade 2"^^xsd:string .

:CCSS.ELA-Literacy.RL.3 rdf:type owl:Class ;
    rdfs:subClassOf :CCSS.ELA-Literacy.RL ;
    prov:wasQuotedFrom <http://www.corestandards.org/ELA-Literacy/RL/3/> ;
    rdfs:label "English Language Arts Standards - Reading: Literature - Grade 3"^^xsd:string .

:CCSS.ELA-Literacy.RL.4 rdf:type owl:Class ;
    rdfs:subClassOf :CCSS.ELA-Literacy.RL ;
    prov:wasQuotedFrom <http://www.corestandards.org/ELA-Literacy/RL/4/> ;
    rdfs:label "English Language Arts Standards - Reading: Literature - Grade 4"^^xsd:string .

:CCSS.ELA-Literacy.RL.5 rdf:type owl:Class ;
    rdfs:subClassOf :CCSS.ELA-Literacy.RL ;
    prov:wasQuotedFrom <http://www.corestandards.org/ELA-Literacy/RL/5/> ;
    rdfs:label "English Language Arts Standards - Reading: Literature - Grade 5"^^xsd:string .

:CCSS.ELA-Literacy.RL.6 rdf:type owl:Class ;
    rdfs:subClassOf :CCSS.ELA-Literacy.RL ;
    prov:wasQuotedFrom <http://www.corestandards.org/ELA-Literacy/RL/6/> ;
    rdfs:label "English Language Arts Standards - Reading: Literature - Grade 6"^^xsd:string .

:CCSS.ELA-Literacy.RL.7 rdf:type owl:Class ;
    rdfs:subClassOf :CCSS.ELA-Literacy.RL ;
    prov:wasQuotedFrom <http://www.corestandards.org/ELA-Literacy/RL/7/> ;
    rdfs:label "English Language Arts Standards - Reading: Literature - Grade 7"^^xsd:string .

:CCSS.ELA-Literacy.RL.8 rdf:type owl:Class ;
    rdfs:subClassOf :CCSS.ELA-Literacy.RL ;
    prov:wasQuotedFrom <http://www.corestandards.org/ELA-Literacy/RL/8/> ;
    rdfs:label "English Language Arts Standards - Reading: Literature - Grade 8"^^xsd:string .

:CCSS.ELA-Literacy.RL.9-10 rdf:type owl:Class ;
    rdfs:subClassOf :CCSS.ELA-Literacy.RL ;
    prov:wasQuotedFrom <http://www.corestandards.org/ELA-Literacy/RL/9-10/> ;
    rdfs:label "English Language Arts Standards - Reading: Literature - Grade 9-10"^^xsd:string .

:CCSS.ELA-Literacy.RL.11-12 rdf:type owl:Class ;
    rdfs:subClassOf :CCSS.ELA-Literacy.RL ;
    prov:wasQuotedFrom <http://www.corestandards.org/ELA-Literacy/RL/11-12/> ;
    rdfs:label "English Language Arts Standards - Reading: Literature - Grade 11-12"^^xsd:string .

:CCSS.ELA-Literacy.RI rdf:type owl:Class ;
    rdfs:subClassOf :CCSS.ELA-Literacy ;
    rdfs:label "Reading: Informational Text"^^xsd:string ;
    prov:wasQuotedFrom <http://www.corestandards.org/ELA-Literacy/RI/> .

:CCSS.ELA-Literacy.RI.introduction-for-6-12 rdf:type owl:Class ;
    rdfs:subClassOf :CCSS.ELA-Literacy.RI ;
    prov:wasQuotedFrom <http://www.corestandards.org/ELA-Literacy/RI/introduction-for-6-12/> ;
    rdfs:label "English Language Arts Standards - Reading: Informational Text - Introduction for 6-12"^^xsd:string ;
    rdfs:comment "The CCR anchor standards and high school grade-specific standards work in tandem to define college and career readiness expectations-the former providing broad standards, the latter providing additional specificity."^^xsd:string .

:CCSS.ELA-Literacy.RI.K rdf:type owl:Class ;
    rdfs:subClassOf :CCSS.ELA-Literacy.RI ;
    prov:wasQuotedFrom <http://www.corestandards.org/ELA-Literacy/RI/K/> ;
    rdfs:label "English Language Arts Standards - Reading: Informational Text - Kindergarten"^^xsd:string .

:CCSS.ELA-Literacy.RI.1 rdf:type owl:Class ;
    rdfs:subClassOf :CCSS.ELA-Literacy.RI ;
    prov:wasQuotedFrom <http://www.corestandards.org/ELA-Literacy/RI/1/> ;
    rdfs:label "English Language Arts Standards - Reading: Informational Text - Grade 1"^^xsd:string .

:CCSS.ELA-Literacy.RI.2 rdf:type owl:Class ;
    rdfs:subClassOf :CCSS.ELA-Literacy.RI ;
    prov:wasQuotedFrom <http://www.corestandards.org/ELA-Literacy/RI/2/> ;
    rdfs:label "English Language Arts Standards - Reading: Informational Text - Grade 2"^^xsd:string .

:CCSS.ELA-Literacy.RI.3 rdf:type owl:Class ;
    rdfs:subClassOf :CCSS.ELA-Literacy.RI ;
    prov:wasQuotedFrom <http://www.corestandards.org/ELA-Literacy/RI/3/> ;
    rdfs:label "English Language Arts Standards - Reading: Informational Text - Grade 3"^^xsd:string .

:CCSS.ELA-Literacy.RI.4 rdf:type owl:Class ;
    rdfs:subClassOf :CCSS.ELA-Literacy.RI ;
    prov:wasQuotedFrom <http://www.corestandards.org/ELA-Literacy/RI/4/> ;
    rdfs:label "English Language Arts Standards - Reading: Informational Text - Grade 4"^^xsd:string .

:CCSS.ELA-Literacy.RI.5 rdf:type owl:Class ;
    rdfs:subClassOf :CCSS.ELA-Literacy.RI ;
    prov:wasQuotedFrom <http://www.corestandards.org/ELA-Literacy/RI/5/> ;
    rdfs:label "English Language Arts Standards - Reading: Informational Text - Grade 5"^^xsd:string .

:CCSS.ELA-Literacy.RI.6 rdf:type owl:Class ;
    rdfs:subClassOf :CCSS.ELA-Literacy.RI ;
    prov:wasQuotedFrom <http://www.corestandards.org/ELA-Literacy/RI/6/> ;
    rdfs:label "English Language Arts Standards - Reading: Informational Text - Grade 6"^^xsd:string .

:CCSS.ELA-Literacy.RI.7 rdf:type owl:Class ;
    rdfs:subClassOf :CCSS.ELA-Literacy.RI ;
    prov:wasQuotedFrom <http://www.corestandards.org/ELA-Literacy/RI/7/> ;
    rdfs:label "English Language Arts Standards - Reading: Informational Text - Grade 7"^^xsd:string .

:CCSS.ELA-Literacy.RI.8 rdf:type owl:Class ;
    rdfs:subClassOf :CCSS.ELA-Literacy.RI ;
    prov:wasQuotedFrom <http://www.corestandards.org/ELA-Literacy/RI/8/> ;
    rdfs:label "English Language Arts Standards - Reading: Informational Text - Grade 8"^^xsd:string .

:CCSS.ELA-Literacy.RI.9-10 rdf:type owl:Class ;
    rdfs:subClassOf :CCSS.ELA-Literacy.RI ;
    prov:wasQuotedFrom <http://www.corestandards.org/ELA-Literacy/RI/9-10/> ;
    rdfs:label "English Language Arts Standards - Reading: Informational Text - Grade 9-10"^^xsd:string .

:CCSS.ELA-Literacy.RI.11-12 rdf:type owl:Class ;
    rdfs:subClassOf :CCSS.ELA-Literacy.RI ;
    prov:wasQuotedFrom <http://www.corestandards.org/ELA-Literacy/RI/11-12/> ;
    rdfs:label "English Language Arts Standards - Reading: Informational Text - Grade 11-12"^^xsd:string .

:CCSS.ELA-Literacy.RF rdf:type owl:Class ;
    rdfs:subClassOf :CCSS.ELA-Literacy ;
    rdfs:label "Reading: Foundational Skills"^^xsd:string ;
    prov:wasQuotedFrom <http://www.corestandards.org/ELA-Literacy/RF/> .

:CCSS.ELA-Literacy.RF.introduction rdf:type owl:Class ;
    rdfs:subClassOf :CCSS.ELA-Literacy.RF ;
    prov:wasQuotedFrom <http://www.corestandards.org/ELA-Literacy/RF/introduction/> ;
    rdfs:label "English Language Arts Standards - Reading: Foundational Skills - Introduction for K-5"^^xsd:string ;
    rdfs:comment "These standards are directed toward fostering students- understanding and working knowledge of concepts of print, the alphabetic principle, and other basic conventions of the English writing system. These foundational skills are not an end in and of themselves; rather, they are necessary and important components of an effective, comprehensive reading program designed to develop proficient readers with the capacity to comprehend texts across a range of types and disciplines. Instruction should be differentiated: good readers will need much less practice with these concepts than struggling readers will. The point is to teach students what they need to learn and not what they already know-to discern when particular children or activities warrant more or less attention.-"^^xsd:string .

:CCSS.ELA-Literacy.RF.K rdf:type owl:Class ;
    rdfs:subClassOf :CCSS.ELA-Literacy.RF ;
    prov:wasQuotedFrom <http://www.corestandards.org/ELA-Literacy/RF/K/> ;
    rdfs:label "English Language Arts Standards - Reading: Foundational Skills - Kindergarten"^^xsd:string .

:CCSS.ELA-Literacy.RF.1 rdf:type owl:Class ;
    rdfs:subClassOf :CCSS.ELA-Literacy.RF ;
    prov:wasQuotedFrom <http://www.corestandards.org/ELA-Literacy/RF/1/> ;
    rdfs:label "English Language Arts Standards - Reading: Foundational Skills - Grade 1"^^xsd:string .

:CCSS.ELA-Literacy.RF.2 rdf:type owl:Class ;
    rdfs:subClassOf :CCSS.ELA-Literacy.RF ;
    prov:wasQuotedFrom <http://www.corestandards.org/ELA-Literacy/RF/2/> ;
    rdfs:label "English Language Arts Standards - Reading: Foundational Skills - Grade 2"^^xsd:string .

:CCSS.ELA-Literacy.RF.3 rdf:type owl:Class ;
    rdfs:subClassOf :CCSS.ELA-Literacy.RF ;
    prov:wasQuotedFrom <http://www.corestandards.org/ELA-Literacy/RF/3/> ;
    rdfs:label "English Language Arts Standards - Reading: Foundational Skills - Grade 3"^^xsd:string .

:CCSS.ELA-Literacy.RF.4 rdf:type owl:Class ;
    rdfs:subClassOf :CCSS.ELA-Literacy.RF ;
    prov:wasQuotedFrom <http://www.corestandards.org/ELA-Literacy/RF/4/> ;
    rdfs:label "English Language Arts Standards - Reading: Foundational Skills - Grade 4"^^xsd:string .

:CCSS.ELA-Literacy.RF.5 rdf:type owl:Class ;
    rdfs:subClassOf :CCSS.ELA-Literacy.RF ;
    prov:wasQuotedFrom <http://www.corestandards.org/ELA-Literacy/RF/5/> ;
    rdfs:label "English Language Arts Standards - Reading: Foundational Skills - Grade 5"^^xsd:string .

:CCSS.ELA-Literacy.W rdf:type owl:Class ;
    rdfs:subClassOf :CCSS.ELA-Literacy ;
    rdfs:label "Writing"^^xsd:string ;
    prov:wasQuotedFrom <http://www.corestandards.org/ELA-Literacy/W/> .

:CCSS.ELA-Literacy.W.introduction rdf:type owl:Class ;
    rdfs:subClassOf :CCSS.ELA-Literacy.W ;
    prov:wasQuotedFrom <http://www.corestandards.org/ELA-Literacy/W/introduction/> ;
    rdfs:label "English Language Arts Standards - Writing - Introduction"^^xsd:string ;
    rdfs:comment "The following standards for K-5 offer a focus for instruction each year to help ensure that students gain adequate mastery of a range of skills and applications. Each year in their writing, students should demonstrate increasing sophistication in all aspects of language use, from vocabulary and syntax to the development and organization of ideas, and they should address increasingly demanding content and sources. Students advancing through the grades are expected to meet each year-s grade-specific standards and retain or further develop skills and understandings mastered in preceding grades. The expected growth in student writing ability is reflected both in the standards themselves and in the collection of annotated student writing samples in Appendix C."^^xsd:string .

:CCSS.ELA-Literacy.W.introduction-for-6-12 rdf:type owl:Class ;
    rdfs:subClassOf :CCSS.ELA-Literacy.W ;
    prov:wasQuotedFrom <http://www.corestandards.org/ELA-Literacy/W/introduction-for-6-12/> ;
    rdfs:label "English Language Arts Standards - Writing - Introduction for 6-12"^^xsd:string ;
    rdfs:comment "The following standards for grades 6-12 offer a focus for instruction each year to help ensure that students gain adequate mastery of a range of skills and applications. Each year in their writing, students should demonstrate increasing sophistication in all aspects of language use, from vocabulary and syntax to the development and organization of ideas, and they should address increasingly demanding content and sources. Students advancing through the grades are expected to meet each year-s grade-specific standards and retain or further develop skills and understandings mastered in preceding grades. The expected growth in student writing ability is reflected both in the standards themselves and in the collection of annotated student writing samples in Appendix C."^^xsd:string .

:CCSS.ELA-Literacy.W.K rdf:type owl:Class ;
    rdfs:subClassOf :CCSS.ELA-Literacy.W ;
    prov:wasQuotedFrom <http://www.corestandards.org/ELA-Literacy/W/K/> ;
    rdfs:label "English Language Arts Standards - Writing - Kindergarten"^^xsd:string .

:CCSS.ELA-Literacy.W.1 rdf:type owl:Class ;
    rdfs:subClassOf :CCSS.ELA-Literacy.W ;
    prov:wasQuotedFrom <http://www.corestandards.org/ELA-Literacy/W/1/> ;
    rdfs:label "English Language Arts Standards - Writing - Grade 1"^^xsd:string .

:CCSS.ELA-Literacy.W.2 rdf:type owl:Class ;
    rdfs:subClassOf :CCSS.ELA-Literacy.W ;
    prov:wasQuotedFrom <http://www.corestandards.org/ELA-Literacy/W/2/> ;
    rdfs:label "English Language Arts Standards - Writing - Grade 2"^^xsd:string .

:CCSS.ELA-Literacy.W.3 rdf:type owl:Class ;
    rdfs:subClassOf :CCSS.ELA-Literacy.W ;
    prov:wasQuotedFrom <http://www.corestandards.org/ELA-Literacy/W/3/> ;
    rdfs:label "English Language Arts Standards - Writing - Grade 3"^^xsd:string .

:CCSS.ELA-Literacy.W.4 rdf:type owl:Class ;
    rdfs:subClassOf :CCSS.ELA-Literacy.W ;
    prov:wasQuotedFrom <http://www.corestandards.org/ELA-Literacy/W/4/> ;
    rdfs:label "English Language Arts Standards - Writing - Grade 4"^^xsd:string .

:CCSS.ELA-Literacy.W.5 rdf:type owl:Class ;
    rdfs:subClassOf :CCSS.ELA-Literacy.W ;
    prov:wasQuotedFrom <http://www.corestandards.org/ELA-Literacy/W/5/> ;
    rdfs:label "English Language Arts Standards - Writing - Grade 5"^^xsd:string .

:CCSS.ELA-Literacy.W.6 rdf:type owl:Class ;
    rdfs:subClassOf :CCSS.ELA-Literacy.W ;
    prov:wasQuotedFrom <http://www.corestandards.org/ELA-Literacy/W/6/> ;
    rdfs:label "English Language Arts Standards - Writing - Grade 6"^^xsd:string .

:CCSS.ELA-Literacy.W.7 rdf:type owl:Class ;
    rdfs:subClassOf :CCSS.ELA-Literacy.W ;
    prov:wasQuotedFrom <http://www.corestandards.org/ELA-Literacy/W/7/> ;
    rdfs:label "English Language Arts Standards - Writing - Grade 7"^^xsd:string .

:CCSS.ELA-Literacy.W.8 rdf:type owl:Class ;
    rdfs:subClassOf :CCSS.ELA-Literacy.W ;
    prov:wasQuotedFrom <http://www.corestandards.org/ELA-Literacy/W/8/> ;
    rdfs:label "English Language Arts Standards - Writing - Grade 8"^^xsd:string .

:CCSS.ELA-Literacy.W.9-10 rdf:type owl:Class ;
    rdfs:subClassOf :CCSS.ELA-Literacy.W ;
    prov:wasQuotedFrom <http://www.corestandards.org/ELA-Literacy/W/9-10/> ;
    rdfs:label "English Language Arts Standards - Writing - Grade 9-10"^^xsd:string .

:CCSS.ELA-Literacy.W.11-12 rdf:type owl:Class ;
    rdfs:subClassOf :CCSS.ELA-Literacy.W ;
    prov:wasQuotedFrom <http://www.corestandards.org/ELA-Literacy/W/11-12/> ;
    rdfs:label "English Language Arts Standards - Writing - Grade 11-12"^^xsd:string .

:CCSS.ELA-Literacy.SL rdf:type owl:Class ;
    rdfs:subClassOf :CCSS.ELA-Literacy ;
    rdfs:label "Speaking & Listening"^^xsd:string ;
    prov:wasQuotedFrom <http://www.corestandards.org/ELA-Literacy/SL/> .

:CCSS.ELA-Literacy.SL.introduction rdf:type owl:Class ;
    rdfs:subClassOf :CCSS.ELA-Literacy.SL ;
    prov:wasQuotedFrom <http://www.corestandards.org/ELA-Literacy/SL/introduction/> ;
    rdfs:label "English Language Arts Standards - Speaking & Listening - Introduction"^^xsd:string ;
    rdfs:comment "The following standards for K-5 offer a focus for instruction each year to help ensure that students gain adequate mastery of a range of skills and applications. Students advancing through the grades are expected to meet each year-s grade-specific standards and retain or further develop skills and understandings mastered in preceding grades."^^xsd:string .

:CCSS.ELA-Literacy.SL.introduction-for-6-12 rdf:type owl:Class ;
    rdfs:subClassOf :CCSS.ELA-Literacy.SL ;
    prov:wasQuotedFrom <http://www.corestandards.org/ELA-Literacy/SL/introduction-for-6-12/> ;
    rdfs:label "English Language Arts Standards - Speaking & Listening - Introduction for 6-12"^^xsd:string ;
    rdfs:comment "The following standards for grades 6-12 offer a focus for instruction in each year to help ensure that students gain adequate mastery of a range of skills and applications. Students advancing through the grades are expected to meet each year-s grade-specific standards and retain or further develop skills and understandings mastered in preceding grades."^^xsd:string .

:CCSS.ELA-Literacy.SL.K rdf:type owl:Class ;
    rdfs:subClassOf :CCSS.ELA-Literacy.SL ;
    prov:wasQuotedFrom <http://www.corestandards.org/ELA-Literacy/SL/K/> ;
    rdfs:label "English Language Arts Standards - Speaking & Listening - Kindergarten"^^xsd:string .

:CCSS.ELA-Literacy.SL.1 rdf:type owl:Class ;
    rdfs:subClassOf :CCSS.ELA-Literacy.SL ;
    prov:wasQuotedFrom <http://www.corestandards.org/ELA-Literacy/SL/1/> ;
    rdfs:label "English Language Arts Standards - Speaking & Listening - Grade 1"^^xsd:string .

:CCSS.ELA-Literacy.SL.2 rdf:type owl:Class ;
    rdfs:subClassOf :CCSS.ELA-Literacy.SL ;
    prov:wasQuotedFrom <http://www.corestandards.org/ELA-Literacy/SL/2/> ;
    rdfs:label "English Language Arts Standards - Speaking & Listening - Grade 2"^^xsd:string .

:CCSS.ELA-Literacy.SL.3 rdf:type owl:Class ;
    rdfs:subClassOf :CCSS.ELA-Literacy.SL ;
    prov:wasQuotedFrom <http://www.corestandards.org/ELA-Literacy/SL/3/> ;
    rdfs:label "English Language Arts Standards - Speaking & Listening - Grade 3"^^xsd:string .

:CCSS.ELA-Literacy.SL.4 rdf:type owl:Class ;
    rdfs:subClassOf :CCSS.ELA-Literacy.SL ;
    prov:wasQuotedFrom <http://www.corestandards.org/ELA-Literacy/SL/4/> ;
    rdfs:label "English Language Arts Standards - Speaking & Listening - Grade 4"^^xsd:string .

:CCSS.ELA-Literacy.SL.5 rdf:type owl:Class ;
    rdfs:subClassOf :CCSS.ELA-Literacy.SL ;
    prov:wasQuotedFrom <http://www.corestandards.org/ELA-Literacy/SL/5/> ;
    rdfs:label "English Language Arts Standards - Speaking & Listening - Grade 5"^^xsd:string .

:CCSS.ELA-Literacy.SL.6 rdf:type owl:Class ;
    rdfs:subClassOf :CCSS.ELA-Literacy.SL ;
    prov:wasQuotedFrom <http://www.corestandards.org/ELA-Literacy/SL/6/> ;
    rdfs:label "English Language Arts Standards - Speaking & Listening - Grade 6"^^xsd:string .

:CCSS.ELA-Literacy.SL.7 rdf:type owl:Class ;
    rdfs:subClassOf :CCSS.ELA-Literacy.SL ;
    prov:wasQuotedFrom <http://www.corestandards.org/ELA-Literacy/SL/7/> ;
    rdfs:label "English Language Arts Standards - Speaking & Listening - Grade 7"^^xsd:string .

:CCSS.ELA-Literacy.SL.8 rdf:type owl:Class ;
    rdfs:subClassOf :CCSS.ELA-Literacy.SL ;
    prov:wasQuotedFrom <http://www.corestandards.org/ELA-Literacy/SL/8/> ;
    rdfs:label "English Language Arts Standards - Speaking & Listening - Grade 8"^^xsd:string .

:CCSS.ELA-Literacy.SL.9-10 rdf:type owl:Class ;
    rdfs:subClassOf :CCSS.ELA-Literacy.SL ;
    prov:wasQuotedFrom <http://www.corestandards.org/ELA-Literacy/SL/9-10/> ;
    rdfs:label "English Language Arts Standards - Speaking & Listening - Grade 9-10"^^xsd:string .

:CCSS.ELA-Literacy.SL.11-12 rdf:type owl:Class ;
    rdfs:subClassOf :CCSS.ELA-Literacy.SL ;
    prov:wasQuotedFrom <http://www.corestandards.org/ELA-Literacy/SL/11-12/> ;
    rdfs:label "English Language Arts Standards - Speaking & Listening - Grade 11-12"^^xsd:string .

:CCSS.ELA-Literacy.L rdf:type owl:Class ;
    rdfs:subClassOf :CCSS.ELA-Literacy ;
    rdfs:label "Language"^^xsd:string ;
    prov:wasQuotedFrom <http://www.corestandards.org/ELA-Literacy/L/> .

:CCSS.ELA-Literacy.L.introduction-for-k-5 rdf:type owl:Class ;
    rdfs:subClassOf :CCSS.ELA-Literacy.L ;
    prov:wasQuotedFrom <http://www.corestandards.org/ELA-Literacy/L/introduction-for-k-5/> ;
    rdfs:label "English Language Arts Standards - Language - Introduction for K-5"^^xsd:string ;
    rdfs:comment "The following standards for grades K-5 offer a focus for instruction each year to help ensure that students gain adequate mastery of a range of skills and applications. Students advancing through the grades are expected to meet each year-s grade-specific standards and retain or further develop skills and understandings mastered in preceding grades. Beginning in grade 3, skills and understandings that are particularly likely to require continued attention in higher grades as they are applied to increasingly sophisticated writing and speaking are marked with an asterisk (*)."^^xsd:string .

:CCSS.ELA-Literacy.L.introduction-for-6-12 rdf:type owl:Class ;
    rdfs:subClassOf :CCSS.ELA-Literacy.L ;
    prov:wasQuotedFrom <http://www.corestandards.org/ELA-Literacy/L/introduction-for-6-12/> ;
    rdfs:label "English Language Arts Standards - Language - Introduction for 6-12"^^xsd:string ;
    rdfs:comment "The following standards for grades 6-12 offer a focus for instruction each year to help ensure that students gain adequate mastery of a range of skills and applications. Students advancing through the grades are expected to meet each year-s grade-specific standards and retain or further develop skills and understandings mastered in preceding grades. Beginning in grade 3, skills and understandings that are particularly likely to require continued attention in higher grades as they are applied to increasingly sophisticated writing and speaking are marked with an asterisk (*)."^^xsd:string .

:CCSS.ELA-Literacy.L.K rdf:type owl:Class ;
    rdfs:subClassOf :CCSS.ELA-Literacy.L ;
    prov:wasQuotedFrom <http://www.corestandards.org/ELA-Literacy/L/K/> ;
    rdfs:label "English Language Arts Standards - Language - Kindergarten"^^xsd:string .

:CCSS.ELA-Literacy.L.1 rdf:type owl:Class ;
    rdfs:subClassOf :CCSS.ELA-Literacy.L ;
    prov:wasQuotedFrom <http://www.corestandards.org/ELA-Literacy/L/1/> ;
    rdfs:label "English Language Arts Standards - Language - Grade 1"^^xsd:string .

:CCSS.ELA-Literacy.L.2 rdf:type owl:Class ;
    rdfs:subClassOf :CCSS.ELA-Literacy.L ;
    prov:wasQuotedFrom <http://www.corestandards.org/ELA-Literacy/L/2/> ;
    rdfs:label "English Language Arts Standards - Language - Grade 2"^^xsd:string .

:CCSS.ELA-Literacy.L.3 rdf:type owl:Class ;
    rdfs:subClassOf :CCSS.ELA-Literacy.L ;
    prov:wasQuotedFrom <http://www.corestandards.org/ELA-Literacy/L/3/> ;
    rdfs:label "English Language Arts Standards - Language - Grade 3"^^xsd:string .

:CCSS.ELA-Literacy.L.4 rdf:type owl:Class ;
    rdfs:subClassOf :CCSS.ELA-Literacy.L ;
    prov:wasQuotedFrom <http://www.corestandards.org/ELA-Literacy/L/4/> ;
    rdfs:label "English Language Arts Standards - Language - Grade 4"^^xsd:string .

:CCSS.ELA-Literacy.L.5 rdf:type owl:Class ;
    rdfs:subClassOf :CCSS.ELA-Literacy.L ;
    prov:wasQuotedFrom <http://www.corestandards.org/ELA-Literacy/L/5/> ;
    rdfs:label "English Language Arts Standards - Language - Grade 5"^^xsd:string .

:CCSS.ELA-Literacy.L.6 rdf:type owl:Class ;
    rdfs:subClassOf :CCSS.ELA-Literacy.L ;
    prov:wasQuotedFrom <http://www.corestandards.org/ELA-Literacy/L/6/> ;
    rdfs:label "English Language Arts Standards - Language - Grade 6"^^xsd:string .

:CCSS.ELA-Literacy.L.7 rdf:type owl:Class ;
    rdfs:subClassOf :CCSS.ELA-Literacy.L ;
    prov:wasQuotedFrom <http://www.corestandards.org/ELA-Literacy/L/7/> ;
    rdfs:label "English Language Arts Standards - Language - Grade 7"^^xsd:string .

:CCSS.ELA-Literacy.L.8 rdf:type owl:Class ;
    rdfs:subClassOf :CCSS.ELA-Literacy.L ;
    prov:wasQuotedFrom <http://www.corestandards.org/ELA-Literacy/L/8/> ;
    rdfs:label "English Language Arts Standards - Language - Grade 8"^^xsd:string .

:CCSS.ELA-Literacy.L.9-10 rdf:type owl:Class ;
    rdfs:subClassOf :CCSS.ELA-Literacy.L ;
    prov:wasQuotedFrom <http://www.corestandards.org/ELA-Literacy/L/9-10/> ;
    rdfs:label "English Language Arts Standards - Language - Grade 9-10"^^xsd:string .

:CCSS.ELA-Literacy.L.11-12 rdf:type owl:Class ;
    rdfs:subClassOf :CCSS.ELA-Literacy.L ;
    prov:wasQuotedFrom <http://www.corestandards.org/ELA-Literacy/L/11-12/> ;
    rdfs:label "English Language Arts Standards - Language - Grade 11-12"^^xsd:string .

:CCSS.ELA-Literacy.L.language-progressive-skills rdf:type owl:Class ;
    rdfs:subClassOf :CCSS.ELA-Literacy.L ;
    prov:wasQuotedFrom <http://www.corestandards.org/ELA-Literacy/L/language-progressive-skills/> ;
    rdfs:label "English Language Arts Standards - Language - Language Progressive Skills"^^xsd:string ;
    rdfs:comment "The following skills, marked with an asterisk (*) in Language standards 1-3, are particularly likely to require continued attention in higher grades as they are applied to increasingly sophisticated writing and speaking."^^xsd:string .

:CCSS.ELA-Literacy.standard-10-range-quality-complexity rdf:type owl:Class ;
    rdfs:subClassOf :CCSS.ELA-Literacy ;
    rdfs:label "Standard 10: Range, Quality, & Complexity"^^xsd:string ;
    prov:wasQuotedFrom <http://www.corestandards.org/ELA-Literacy/standard-10-range-quality-complexity/> .

:CCSS.ELA-Literacy.standard-10-range-quality-complexity.measuring-text-complexity-three-factors rdf:type owl:Class ;
    rdfs:subClassOf :CCSS.ELA-Literacy.standard-10-range-quality-complexity ;
    prov:wasQuotedFrom <http://www.corestandards.org/ELA-Literacy/standard-10-range-quality-complexity/measuring-text-complexity-three-factors/> ;
    rdfs:label "English Language Arts Standards - Standard 10: Range, Quality, & Complexity - Measuring Text Complexity: Three Factors"^^xsd:string .

:CCSS.ELA-Literacy.standard-10-range-quality-complexity.range-of-text-types-for-612 rdf:type owl:Class ;
    rdfs:subClassOf :CCSS.ELA-Literacy.standard-10-range-quality-complexity ;
    prov:wasQuotedFrom <http://www.corestandards.org/ELA-Literacy/standard-10-range-quality-complexity/range-of-text-types-for-612/> ;
    rdfs:label "English Language Arts Standards - Standard 10: Range, Quality, & Complexity - Range of Text Types for 6-12"^^xsd:string ;
    rdfs:comment "Students in grades 6-12 apply the Reading standards to the following range of text types, with texts selected from a broad range of cultures and periods."^^xsd:string .

:CCSS.ELA-Literacy.standard-10-range-quality-complexity.range-of-text-types-for-k-5 rdf:type owl:Class ;
    rdfs:subClassOf :CCSS.ELA-Literacy.standard-10-range-quality-complexity ;
    prov:wasQuotedFrom <http://www.corestandards.org/ELA-Literacy/standard-10-range-quality-complexity/range-of-text-types-for-k-5/> ;
    rdfs:label "English Language Arts Standards - Standard 10: Range, Quality, & Complexity - Range of Text Types for K-5"^^xsd:string ;
    rdfs:comment "Students in K-5 apply the Reading standards to the following range of text types, with texts selected from a broad range of cultures and periods."^^xsd:string .

:CCSS.ELA-Literacy.standard-10-range-quality-complexity.staying-on-topic-within-a-grade-across-grades rdf:type owl:Class ;
    rdfs:subClassOf :CCSS.ELA-Literacy.standard-10-range-quality-complexity ;
    prov:wasQuotedFrom <http://www.corestandards.org/ELA-Literacy/standard-10-range-quality-complexity/staying-on-topic-within-a-grade-across-grades/> ;
    rdfs:label "English Language Arts Standards - Standard 10: Range, Quality, & Complexity - Staying on Topic Within a Grade & Across Grades"^^xsd:string ;
    rdfs:comment "Building knowledge systematically in English language arts is like giving children various pieces of a puzzle in each grade that, over time, will form one big picture. At a curricular or instructional level, texts-within and across grade levels-need to be selected around topics or themes that systematically develop the knowledge base of students. Within a grade level, there should be an adequate number of titles on a single topic that would allow children to study that topic for a sustained period. The knowledge children have learned about particular topics in early grade levels should then be expanded and developed in subsequent grade levels to ensure an increasingly deeper understanding of these topics. Children in the upper elementary grades will generally be expected to read these texts independently and reflect on them in writing. However, children in the early grades (particularly K-2) should participate in rich, structured conversations with an adult in response to the written texts that are read aloud, orally comparing and contrasting as well as analyzing and synthesizing, in the manner called for by the Standards."^^xsd:string .

:CCSS.ELA-Literacy.standard-10-range-quality-complexity.texts-illustrating-the-complexity-quality-range-of-student-reading-6-12 rdf:type owl:Class ;
    rdfs:subClassOf :CCSS.ELA-Literacy.standard-10-range-quality-complexity ;
    prov:wasQuotedFrom <http://www.corestandards.org/ELA-Literacy/standard-10-range-quality-complexity/texts-illustrating-the-complexity-quality-range-of-student-reading-6-12/> ;
    rdfs:label "English Language Arts Standards - Standard 10: Range, Quality, & Complexity - Texts Illustrating the Complexity, Quality, & Range of Student Reading 6-12"^^xsd:string ;
    rdfs:comment "Given space limitations, the illustrative texts listed above are meant only to show individual titles that are representative of a range of topics and genres. (See Appendix B for excerpts of these and other texts illustrative of grades 6-12 text complexity, quality, and range.) At a curricular or instructional level, within and across grade levels, texts need to be selected around topics or themes that generate knowledge and allow students to study those topics or themes in depth."^^xsd:string .

:CCSS.ELA-Literacy.standard-10-range-quality-complexity.texts-illustrating-the-complexity-quality-range-of-student-reading-k5 rdf:type owl:Class ;
    rdfs:subClassOf :CCSS.ELA-Literacy.standard-10-range-quality-complexity ;
    prov:wasQuotedFrom <http://www.corestandards.org/ELA-Literacy/standard-10-range-quality-complexity/texts-illustrating-the-complexity-quality-range-of-student-reading-k5/> ;
    rdfs:label "English Language Arts Standards - Standard 10: Range, Quality, & Complexity - Texts Illustrating the Complexity, Quality, & Range of Student Reading K-5"^^xsd:string ;
    rdfs:comment "Given space limitations, the illustrative texts listed above are meant only to show individual titles that are representative of a wide range of topics and genres. (See Appendix B for excerpts of these and other texts illustrative of K-5 text complexity, quality, and range.) At a curricular or instructional level, within and across grade levels, texts need to be selected around topics or themes that generate knowledge and allow students to study those topics or themes in depth. On the next page is an example of progressions of texts building knowledge across grade levels."^^xsd:string .

:CCSS.ELA-Literacy.WHST rdf:type owl:Class ;
    rdfs:subClassOf :CCSS.ELA-Literacy ;
    rdfs:label "Writing"^^xsd:string ;
    prov:wasQuotedFrom <http://www.corestandards.org/ELA-Literacy/WHST/> .

:CCSS.ELA-Literacy.WHST.introduction rdf:type owl:Class ;
    rdfs:subClassOf :CCSS.ELA-Literacy.WHST ;
    prov:wasQuotedFrom <http://www.corestandards.org/ELA-Literacy/WHST/introduction/> ;
    rdfs:label "English Language Arts Standards - Writing - Introduction"^^xsd:string ;
    rdfs:comment "The standards below begin at grade 6; standards for K-5 writing in history/social studies, science, and technical subjects are integrated into the K-5 Writing standards. The CCR anchor standards and high school standards in literacy work in tandem to define college and career readiness expectations-the former providing broad standards, the latter providing additional specificity."^^xsd:string .

:CCSS.ELA-Literacy.WHST.6-8 rdf:type owl:Class ;
    rdfs:subClassOf :CCSS.ELA-Literacy.WHST ;
    prov:wasQuotedFrom <http://www.corestandards.org/ELA-Literacy/WHST/6-8/> ;
    rdfs:label "English Language Arts Standards - Writing - Grade 6-8"^^xsd:string .

:CCSS.ELA-Literacy.WHST.9-10 rdf:type owl:Class ;
    rdfs:subClassOf :CCSS.ELA-Literacy.WHST ;
    prov:wasQuotedFrom <http://www.corestandards.org/ELA-Literacy/WHST/9-10/> ;
    rdfs:label "English Language Arts Standards - Writing - Grade 9-10"^^xsd:string .

:CCSS.ELA-Literacy.WHST.11-12 rdf:type owl:Class ;
    rdfs:subClassOf :CCSS.ELA-Literacy.WHST ;
    prov:wasQuotedFrom <http://www.corestandards.org/ELA-Literacy/WHST/11-12/> ;
    rdfs:label "English Language Arts Standards - Writing - Grade 11-12"^^xsd:string .

:CCSS.ELA-Literacy.CCRA rdf:type owl:Class ;
    rdfs:subClassOf :CCSS.ELA-Literacy ;
    rdfs:label "College and Career Readiness Anchor"^^xsd:string ;
    prov:wasQuotedFrom <http://www.corestandards.org/ELA-Literacy/CCRA/> .

:CCSS.ELA-Literacy.CCRA.R rdf:type owl:Class ;
    rdfs:label "College and Career Readiness Anchor for Reading"^^xsd:string ;
    prov:wasQuotedFrom <http://www.corestandards.org/ELA-Literacy/CCRA/R/> ;
    rdfs:subClassOf :CCSS.ELA-Literacy.CCRA .

:CCSS.ELA-Literacy.CCRA.R.1 rdf:type owl:Class ;
    prov:wasQuotedFrom <http://www.corestandards.org/ELA-Literacy/CCRA/R/1/> ;
    rdfs:subClassOf :CCSS.ELA-Literacy.CCRA.R ;
    rdfs:comment "Read closely to determine what the text says explicitly and to make logical inferences from it; cite specific textual evidence when writing or speaking to support conclusions drawn from the text."^^xsd:string .

:CCSS.ELA-Literacy.CCRA.R.2 rdf:type owl:Class ;
    prov:wasQuotedFrom <http://www.corestandards.org/ELA-Literacy/CCRA/R/2/> ;
    rdfs:subClassOf :CCSS.ELA-Literacy.CCRA.R ;
    rdfs:comment "Determine central ideas or themes of a text and analyze their development; summarize the key supporting details and ideas."^^xsd:string .

:CCSS.ELA-Literacy.CCRA.R.3 rdf:type owl:Class ;
    prov:wasQuotedFrom <http://www.corestandards.org/ELA-Literacy/CCRA/R/3/> ;
    rdfs:subClassOf :CCSS.ELA-Literacy.CCRA.R ;
    rdfs:comment "Analyze how and why individuals, events, or ideas develop and interact over the course of a text."^^xsd:string .

:CCSS.ELA-Literacy.CCRA.R.4 rdf:type owl:Class ;
    prov:wasQuotedFrom <http://www.corestandards.org/ELA-Literacy/CCRA/R/4/> ;
    rdfs:subClassOf :CCSS.ELA-Literacy.CCRA.R ;
    rdfs:comment "Interpret words and phrases as they are used in a text, including determining technical, connotative, and figurative meanings, and analyze how specific word choices shape meaning or tone."^^xsd:string .

:CCSS.ELA-Literacy.CCRA.R.5 rdf:type owl:Class ;
    prov:wasQuotedFrom <http://www.corestandards.org/ELA-Literacy/CCRA/R/5/> ;
    rdfs:subClassOf :CCSS.ELA-Literacy.CCRA.R ;
    rdfs:comment "Analyze the structure of texts, including how specific sentences, paragraphs, and larger portions of the text (e.g., a section, chapter, scene, or stanza) relate to each other and the whole."^^xsd:string .

:CCSS.ELA-Literacy.CCRA.R.6 rdf:type owl:Class ;
    prov:wasQuotedFrom <http://www.corestandards.org/ELA-Literacy/CCRA/R/6/> ;
    rdfs:subClassOf :CCSS.ELA-Literacy.CCRA.R ;
    rdfs:comment "Assess how point of view or purpose shapes the content and style of a text."^^xsd:string .

:CCSS.ELA-Literacy.CCRA.R.7 rdf:type owl:Class ;
    prov:wasQuotedFrom <http://www.corestandards.org/ELA-Literacy/CCRA/R/7/> ;
    rdfs:subClassOf :CCSS.ELA-Literacy.CCRA.R ;
    rdfs:comment "Integrate and evaluate content presented in diverse media and formats, including visually and quantitatively, as well as in words.1"^^xsd:string .

:CCSS.ELA-Literacy.CCRA.R.8 rdf:type owl:Class ;
    prov:wasQuotedFrom <http://www.corestandards.org/ELA-Literacy/CCRA/R/8/> ;
    rdfs:subClassOf :CCSS.ELA-Literacy.CCRA.R ;
    rdfs:comment "Delineate and evaluate the argument and specific claims in a text, including the validity of the reasoning as well as the relevance and sufficiency of the evidence."^^xsd:string .

:CCSS.ELA-Literacy.CCRA.R.9 rdf:type owl:Class ;
    prov:wasQuotedFrom <http://www.corestandards.org/ELA-Literacy/CCRA/R/9/> ;
    rdfs:subClassOf :CCSS.ELA-Literacy.CCRA.R ;
    rdfs:comment "Analyze how two or more texts address similar themes or topics in order to build knowledge or to compare the approaches the authors take."^^xsd:string .

:CCSS.ELA-Literacy.CCRA.R.10 rdf:type owl:Class ;
    prov:wasQuotedFrom <http://www.corestandards.org/ELA-Literacy/CCRA/R/10/> ;
    rdfs:subClassOf :CCSS.ELA-Literacy.CCRA.R ;
    rdfs:comment "Read and comprehend complex literary and informational texts independently and proficiently."^^xsd:string .

:CCSS.ELA-Literacy.CCRA.W rdf:type owl:Class ;
    rdfs:label "College and Career Readiness Anchor for Writing"^^xsd:string ;
    prov:wasQuotedFrom <http://www.corestandards.org/ELA-Literacy/CCRA/W/> ;
    rdfs:subClassOf :CCSS.ELA-Literacy.CCRA .

:CCSS.ELA-Literacy.CCRA.W.1 rdf:type owl:Class ;
    prov:wasQuotedFrom <http://www.corestandards.org/ELA-Literacy/CCRA/W/1/> ;
    rdfs:subClassOf :CCSS.ELA-Literacy.CCRA.W ;
    rdfs:comment "Write arguments to support claims in an analysis of substantive topics or texts using valid reasoning and relevant and sufficient evidence. "^^xsd:string .

:CCSS.ELA-Literacy.CCRA.W.2 rdf:type owl:Class ;
    prov:wasQuotedFrom <http://www.corestandards.org/ELA-Literacy/CCRA/W/2/> ;
    rdfs:subClassOf :CCSS.ELA-Literacy.CCRA.W ;
    rdfs:comment "Write informative/explanatory texts to examine and convey complex ideas and information clearly and accurately through the effective selection, organization, and analysis of content."^^xsd:string .

:CCSS.ELA-Literacy.CCRA.W.3 rdf:type owl:Class ;
    prov:wasQuotedFrom <http://www.corestandards.org/ELA-Literacy/CCRA/W/3/> ;
    rdfs:subClassOf :CCSS.ELA-Literacy.CCRA.W ;
    rdfs:comment "Write narratives to develop real or imagined experiences or events using effective technique, well-chosen details and well-structured event sequences."^^xsd:string .

:CCSS.ELA-Literacy.CCRA.W.4 rdf:type owl:Class ;
    prov:wasQuotedFrom <http://www.corestandards.org/ELA-Literacy/CCRA/W/4/> ;
    rdfs:subClassOf :CCSS.ELA-Literacy.CCRA.W ;
    rdfs:comment "Produce clear and coherent writing in which the development, organization, and style are appropriate to task, purpose, and audience."^^xsd:string .

:CCSS.ELA-Literacy.CCRA.W.5 rdf:type owl:Class ;
    prov:wasQuotedFrom <http://www.corestandards.org/ELA-Literacy/CCRA/W/5/> ;
    rdfs:subClassOf :CCSS.ELA-Literacy.CCRA.W ;
    rdfs:comment "Develop and strengthen writing as needed by planning, revising, editing, rewriting, or trying a new approach."^^xsd:string .

:CCSS.ELA-Literacy.CCRA.W.6 rdf:type owl:Class ;
    prov:wasQuotedFrom <http://www.corestandards.org/ELA-Literacy/CCRA/W/6/> ;
    rdfs:subClassOf :CCSS.ELA-Literacy.CCRA.W ;
    rdfs:comment "Use technology, including the Internet, to produce and publish writing and to interact and collaborate with others."^^xsd:string .

:CCSS.ELA-Literacy.CCRA.W.7 rdf:type owl:Class ;
    prov:wasQuotedFrom <http://www.corestandards.org/ELA-Literacy/CCRA/W/7/> ;
    rdfs:subClassOf :CCSS.ELA-Literacy.CCRA.W ;
    rdfs:comment "Conduct short as well as more sustained research projects based on focused questions, demonstrating understanding of the subject under investigation."^^xsd:string .

:CCSS.ELA-Literacy.CCRA.W.8 rdf:type owl:Class ;
    prov:wasQuotedFrom <http://www.corestandards.org/ELA-Literacy/CCRA/W/8/> ;
    rdfs:subClassOf :CCSS.ELA-Literacy.CCRA.W ;
    rdfs:comment "Gather relevant information from multiple print and digital sources, assess the credibility and accuracy of each source, and integrate the information while avoiding plagiarism."^^xsd:string .

:CCSS.ELA-Literacy.CCRA.W.9 rdf:type owl:Class ;
    prov:wasQuotedFrom <http://www.corestandards.org/ELA-Literacy/CCRA/W/9/> ;
    rdfs:subClassOf :CCSS.ELA-Literacy.CCRA.W ;
    rdfs:comment "Draw evidence from literary or informational texts to support analysis, reflection, and research."^^xsd:string .

:CCSS.ELA-Literacy.CCRA.W.10 rdf:type owl:Class ;
    prov:wasQuotedFrom <http://www.corestandards.org/ELA-Literacy/CCRA/W/10/> ;
    rdfs:subClassOf :CCSS.ELA-Literacy.CCRA.W ;
    rdfs:comment "Write routinely over extended time frames (time for research, reflection, and revision) and shorter time frames (a single sitting or a day or two) for a range of tasks, purposes, and audiences."^^xsd:string .

:CCSS.ELA-Literacy.CCRA.SL rdf:type owl:Class ;
    rdfs:label "College and Career Readiness Anchor for Speaking and Listening"^^xsd:string ;
    prov:wasQuotedFrom <http://www.corestandards.org/ELA-Literacy/CCRA/SL/> ;
    rdfs:subClassOf :CCSS.ELA-Literacy.CCRA .

:CCSS.ELA-Literacy.CCRA.SL.1 rdf:type owl:Class ;
    prov:wasQuotedFrom <http://www.corestandards.org/ELA-Literacy/CCRA/SL/1/> ;
    rdfs:subClassOf :CCSS.ELA-Literacy.CCRA.SL ;
    rdfs:comment "Prepare for and participate effectively in a range of conversations and collaborations with diverse partners, building on others' ideas and expressing their own clearly and persuasively."^^xsd:string .

:CCSS.ELA-Literacy.CCRA.SL.2 rdf:type owl:Class ;
    prov:wasQuotedFrom <http://www.corestandards.org/ELA-Literacy/CCRA/SL/2/> ;
    rdfs:subClassOf :CCSS.ELA-Literacy.CCRA.SL ;
    rdfs:comment "Integrate and evaluate information presented in diverse media and formats, including visually, quantitatively, and orally."^^xsd:string .

:CCSS.ELA-Literacy.CCRA.SL.3 rdf:type owl:Class ;
    prov:wasQuotedFrom <http://www.corestandards.org/ELA-Literacy/CCRA/SL/3/> ;
    rdfs:subClassOf :CCSS.ELA-Literacy.CCRA.SL ;
    rdfs:comment "Evaluate a speaker's point of view, reasoning, and use of evidence and rhetoric."^^xsd:string .

:CCSS.ELA-Literacy.CCRA.SL.4 rdf:type owl:Class ;
    prov:wasQuotedFrom <http://www.corestandards.org/ELA-Literacy/CCRA/SL/4/> ;
    rdfs:subClassOf :CCSS.ELA-Literacy.CCRA.SL ;
    rdfs:comment "Present information, findings, and supporting evidence such that listeners can follow the line of reasoning and the organization, development, and style are appropriate to task, purpose, and audience."^^xsd:string .

:CCSS.ELA-Literacy.CCRA.SL.5 rdf:type owl:Class ;
    prov:wasQuotedFrom <http://www.corestandards.org/ELA-Literacy/CCRA/SL/5/> ;
    rdfs:subClassOf :CCSS.ELA-Literacy.CCRA.SL ;
    rdfs:comment "Make strategic use of digital media and visual displays of data to express information and enhance understanding of presentations."^^xsd:string .

:CCSS.ELA-Literacy.CCRA.SL.6 rdf:type owl:Class ;
    prov:wasQuotedFrom <http://www.corestandards.org/ELA-Literacy/CCRA/SL/6/> ;
    rdfs:subClassOf :CCSS.ELA-Literacy.CCRA.SL ;
    rdfs:comment "Adapt speech to a variety of contexts and communicative tasks, demonstrating command of formal English when indicated or appropriate."^^xsd:string .

:CCSS.ELA-Literacy.CCRA.L rdf:type owl:Class ;
    rdfs:label "College and Career Readiness Anchor for Language"^^xsd:string ;
    prov:wasQuotedFrom <http://www.corestandards.org/ELA-Literacy/CCRA/L/> ;
    rdfs:subClassOf :CCSS.ELA-Literacy.CCRA .

:CCSS.ELA-Literacy.CCRA.L.1 rdf:type owl:Class ;
    prov:wasQuotedFrom <http://www.corestandards.org/ELA-Literacy/CCRA/L/1/> ;
    rdfs:subClassOf :CCSS.ELA-Literacy.CCRA.L ;
    rdfs:comment "Demonstrate command of the conventions of standard English grammar and usage when writing or speaking."^^xsd:string .

:CCSS.ELA-Literacy.CCRA.L.2 rdf:type owl:Class ;
    prov:wasQuotedFrom <http://www.corestandards.org/ELA-Literacy/CCRA/L/2/> ;
    rdfs:subClassOf :CCSS.ELA-Literacy.CCRA.L ;
    rdfs:comment "Demonstrate command of the conventions of standard English capitalization, punctuation, and spelling when writing."^^xsd:string .

:CCSS.ELA-Literacy.CCRA.L.3 rdf:type owl:Class ;
    prov:wasQuotedFrom <http://www.corestandards.org/ELA-Literacy/CCRA/L/3/> ;
    rdfs:subClassOf :CCSS.ELA-Literacy.CCRA.L ;
    rdfs:comment "Apply knowledge of language to understand how language functions in different contexts, to make effective choices for meaning or style, and to comprehend more fully when reading or listening. "^^xsd:string .

:CCSS.ELA-Literacy.CCRA.L.4 rdf:type owl:Class ;
    prov:wasQuotedFrom <http://www.corestandards.org/ELA-Literacy/CCRA/L/4/> ;
    rdfs:subClassOf :CCSS.ELA-Literacy.CCRA.L ;
    rdfs:comment "Determine or clarify the meaning of unknown and multiple-meaning words and phrases by using context clues, analyzing meaningful word parts, and consulting general and specialized reference materials, as appropriate."^^xsd:string .

:CCSS.ELA-Literacy.CCRA.L.5 rdf:type owl:Class ;
    prov:wasQuotedFrom <http://www.corestandards.org/ELA-Literacy/CCRA/L/5/> ;
    rdfs:subClassOf :CCSS.ELA-Literacy.CCRA.L ;
    rdfs:comment "Demonstrate understanding of figurative language, word relationships, and nuances in word meanings."^^xsd:string .

:CCSS.ELA-Literacy.CCRA.L.6 rdf:type owl:Class ;
    prov:wasQuotedFrom <http://www.corestandards.org/ELA-Literacy/CCRA/L/6/> ;
    rdfs:subClassOf :CCSS.ELA-Literacy.CCRA.L ;
    rdfs:comment "Acquire and use accurately a range of general academic and domain-specific words and phrases sufficient for reading, writing, speaking, and listening at the college and career readiness level; demonstrate independence in gathering vocabulary knowledge when encountering an unknown term important to comprehension or expression."^^xsd:string .

:CCSS.ELA-Literacy.RL.K rdf:type owl:Class ;
    prov:wasQuotedFrom <http://www.corestandards.org/ELA-Literacy/RL/K/> ;
    rdfs:subClassOf :CCSS.ELA-Literacy.RL .

:CCSS.ELA-Literacy.RL.K.1 rdf:type owl:Class ;
    prov:wasQuotedFrom <http://www.corestandards.org/ELA-Literacy/RL/K/1/> ;
    rdfs:subClassOf :CCSS.ELA-Literacy.RL.K ;
    rdfs:comment "With prompting and support, ask and answer questions about key details in a text."^^xsd:string .

:CCSS.ELA-Literacy.RL.K.2 rdf:type owl:Class ;
    prov:wasQuotedFrom <http://www.corestandards.org/ELA-Literacy/RL/K/2/> ;
    rdfs:subClassOf :CCSS.ELA-Literacy.RL.K ;
    rdfs:comment "With prompting and support, retell familiar stories, including key details."^^xsd:string .

:CCSS.ELA-Literacy.RL.K.3 rdf:type owl:Class ;
    prov:wasQuotedFrom <http://www.corestandards.org/ELA-Literacy/RL/K/3/> ;
    rdfs:subClassOf :CCSS.ELA-Literacy.RL.K ;
    rdfs:comment "With prompting and support, identify characters, settings, and major events in a story."^^xsd:string .

:CCSS.ELA-Literacy.RL.K.4 rdf:type owl:Class ;
    prov:wasQuotedFrom <http://www.corestandards.org/ELA-Literacy/RL/K/4/> ;
    rdfs:subClassOf :CCSS.ELA-Literacy.RL.K ;
    rdfs:comment "Ask and answer questions about unknown words in a text."^^xsd:string .

:CCSS.ELA-Literacy.RL.K.5 rdf:type owl:Class ;
    prov:wasQuotedFrom <http://www.corestandards.org/ELA-Literacy/RL/K/5/> ;
    rdfs:subClassOf :CCSS.ELA-Literacy.RL.K ;
    rdfs:comment "Recognize common types of texts (e.g., storybooks, poems)."^^xsd:string .

:CCSS.ELA-Literacy.RL.K.6 rdf:type owl:Class ;
    prov:wasQuotedFrom <http://www.corestandards.org/ELA-Literacy/RL/K/6/> ;
    rdfs:subClassOf :CCSS.ELA-Literacy.RL.K ;
    rdfs:comment "With prompting and support, name the author and illustrator of a story and define the role of each in telling the story."^^xsd:string .

:CCSS.ELA-Literacy.RL.K.7 rdf:type owl:Class ;
    prov:wasQuotedFrom <http://www.corestandards.org/ELA-Literacy/RL/K/7/> ;
    rdfs:subClassOf :CCSS.ELA-Literacy.RL.K ;
    rdfs:comment "With prompting and support, describe the relationship between illustrations and the story in which they appear (e.g., what moment in a story an illustration depicts)."^^xsd:string .

:CCSS.ELA-Literacy.RL.K.8 rdf:type owl:Class ;
    prov:wasQuotedFrom <http://www.corestandards.org/ELA-Literacy/RL/K/8/> ;
    rdfs:subClassOf :CCSS.ELA-Literacy.RL.K ;
    rdfs:comment "(RL.K.8 not applicable to literature)"^^xsd:string .

:CCSS.ELA-Literacy.RL.K.9 rdf:type owl:Class ;
    prov:wasQuotedFrom <http://www.corestandards.org/ELA-Literacy/RL/K/9/> ;
    rdfs:subClassOf :CCSS.ELA-Literacy.RL.K ;
    rdfs:comment "With prompting and support, compare and contrast the adventures and experiences of characters in familiar stories."^^xsd:string .

:CCSS.ELA-Literacy.RL.K.10 rdf:type owl:Class ;
    prov:wasQuotedFrom <http://www.corestandards.org/ELA-Literacy/RL/K/10/> ;
    rdfs:subClassOf :CCSS.ELA-Literacy.RL.K ;
    rdfs:comment "Actively engage in group reading activities with purpose and understanding."^^xsd:string .

:CCSS.ELA-Literacy.RL.1 rdf:type owl:Class ;
    prov:wasQuotedFrom <http://www.corestandards.org/ELA-Literacy/RL/1/> ;
    rdfs:subClassOf :CCSS.ELA-Literacy.RL .

:CCSS.ELA-Literacy.RL.1.1 rdf:type owl:Class ;
    prov:wasQuotedFrom <http://www.corestandards.org/ELA-Literacy/RL/1/1/> ;
    rdfs:subClassOf :CCSS.ELA-Literacy.RL.1 ;
    rdfs:comment "Ask and answer questions about key details in a text."^^xsd:string .

:CCSS.ELA-Literacy.RL.1.2 rdf:type owl:Class ;
    prov:wasQuotedFrom <http://www.corestandards.org/ELA-Literacy/RL/1/2/> ;
    rdfs:subClassOf :CCSS.ELA-Literacy.RL.1 ;
    rdfs:comment "Retell stories, including key details, and demonstrate understanding of their central message or lesson."^^xsd:string .

:CCSS.ELA-Literacy.RL.1.3 rdf:type owl:Class ;
    prov:wasQuotedFrom <http://www.corestandards.org/ELA-Literacy/RL/1/3/> ;
    rdfs:subClassOf :CCSS.ELA-Literacy.RL.1 ;
    rdfs:comment "Describe characters, settings, and major events in a story, using key details."^^xsd:string .

:CCSS.ELA-Literacy.RL.1.4 rdf:type owl:Class ;
    prov:wasQuotedFrom <http://www.corestandards.org/ELA-Literacy/RL/1/4/> ;
    rdfs:subClassOf :CCSS.ELA-Literacy.RL.1 ;
    rdfs:comment "Identify words and phrases in stories or poems that suggest feelings or appeal to the senses."^^xsd:string .

:CCSS.ELA-Literacy.RL.1.5 rdf:type owl:Class ;
    prov:wasQuotedFrom <http://www.corestandards.org/ELA-Literacy/RL/1/5/> ;
    rdfs:subClassOf :CCSS.ELA-Literacy.RL.1 ;
    rdfs:comment "Explain major differences between books that tell stories and books that give information, drawing on a wide reading of a range of text types."^^xsd:string .

:CCSS.ELA-Literacy.RL.1.6 rdf:type owl:Class ;
    prov:wasQuotedFrom <http://www.corestandards.org/ELA-Literacy/RL/1/6/> ;
    rdfs:subClassOf :CCSS.ELA-Literacy.RL.1 ;
    rdfs:comment "Identify who is telling the story at various points in a text."^^xsd:string .

:CCSS.ELA-Literacy.RL.1.7 rdf:type owl:Class ;
    prov:wasQuotedFrom <http://www.corestandards.org/ELA-Literacy/RL/1/7/> ;
    rdfs:subClassOf :CCSS.ELA-Literacy.RL.1 ;
    rdfs:comment "Use illustrations and details in a story to describe its characters, setting, or events."^^xsd:string .

:CCSS.ELA-Literacy.RL.1.8 rdf:type owl:Class ;
    prov:wasQuotedFrom <http://www.corestandards.org/ELA-Literacy/RL/1/8/> ;
    rdfs:subClassOf :CCSS.ELA-Literacy.RL.1 ;
    rdfs:comment "(RL.1.8 not applicable to literature)"^^xsd:string .

:CCSS.ELA-Literacy.RL.1.9 rdf:type owl:Class ;
    prov:wasQuotedFrom <http://www.corestandards.org/ELA-Literacy/RL/1/9/> ;
    rdfs:subClassOf :CCSS.ELA-Literacy.RL.1 ;
    rdfs:comment "Compare and contrast the adventures and experiences of characters in stories."^^xsd:string .

:CCSS.ELA-Literacy.RL.1.10 rdf:type owl:Class ;
    prov:wasQuotedFrom <http://www.corestandards.org/ELA-Literacy/RL/1/10/> ;
    rdfs:subClassOf :CCSS.ELA-Literacy.RL.1 ;
    rdfs:comment "With prompting and support, read prose and poetry of appropriate complexity for grade 1."^^xsd:string .

:CCSS.ELA-Literacy.RL.2 rdf:type owl:Class ;
    prov:wasQuotedFrom <http://www.corestandards.org/ELA-Literacy/RL/2/> ;
    rdfs:subClassOf :CCSS.ELA-Literacy.RL .

:CCSS.ELA-Literacy.RL.2.1 rdf:type owl:Class ;
    prov:wasQuotedFrom <http://www.corestandards.org/ELA-Literacy/RL/2/1/> ;
    rdfs:subClassOf :CCSS.ELA-Literacy.RL.2 ;
    rdfs:comment "Ask and answer such questions as who, what, where, when, why, and how to demonstrate understanding of key details in a text."^^xsd:string .

:CCSS.ELA-Literacy.RL.2.2 rdf:type owl:Class ;
    prov:wasQuotedFrom <http://www.corestandards.org/ELA-Literacy/RL/2/2/> ;
    rdfs:subClassOf :CCSS.ELA-Literacy.RL.2 ;
    rdfs:comment "Recount stories, including fables and folktales from diverse cultures, and determine their central message, lesson, or moral."^^xsd:string .

:CCSS.ELA-Literacy.RL.2.3 rdf:type owl:Class ;
    prov:wasQuotedFrom <http://www.corestandards.org/ELA-Literacy/RL/2/3/> ;
    rdfs:subClassOf :CCSS.ELA-Literacy.RL.2 ;
    rdfs:comment "Describe how characters in a story respond to major events and challenges."^^xsd:string .

:CCSS.ELA-Literacy.RL.2.4 rdf:type owl:Class ;
    prov:wasQuotedFrom <http://www.corestandards.org/ELA-Literacy/RL/2/4/> ;
    rdfs:subClassOf :CCSS.ELA-Literacy.RL.2 ;
    rdfs:comment "Describe how words and phrases (e.g., regular beats, alliteration, rhymes, repeated lines) supply rhythm and meaning in a story, poem, or song."^^xsd:string .

:CCSS.ELA-Literacy.RL.2.5 rdf:type owl:Class ;
    prov:wasQuotedFrom <http://www.corestandards.org/ELA-Literacy/RL/2/5/> ;
    rdfs:subClassOf :CCSS.ELA-Literacy.RL.2 ;
    rdfs:comment "Describe the overall structure of a story, including describing how the beginning introduces the story and the ending concludes the action."^^xsd:string .

:CCSS.ELA-Literacy.RL.2.6 rdf:type owl:Class ;
    prov:wasQuotedFrom <http://www.corestandards.org/ELA-Literacy/RL/2/6/> ;
    rdfs:subClassOf :CCSS.ELA-Literacy.RL.2 ;
    rdfs:comment "Acknowledge differences in the points of view of characters, including by speaking in a different voice for each character when reading dialogue aloud."^^xsd:string .

:CCSS.ELA-Literacy.RL.2.7 rdf:type owl:Class ;
    prov:wasQuotedFrom <http://www.corestandards.org/ELA-Literacy/RL/2/7/> ;
    rdfs:subClassOf :CCSS.ELA-Literacy.RL.2 ;
    rdfs:comment "Use information gained from the illustrations and words in a print or digital text to demonstrate understanding of its characters, setting, or plot."^^xsd:string .

:CCSS.ELA-Literacy.RL.2.8 rdf:type owl:Class ;
    prov:wasQuotedFrom <http://www.corestandards.org/ELA-Literacy/RL/2/8/> ;
    rdfs:subClassOf :CCSS.ELA-Literacy.RL.2 ;
    rdfs:comment "(RL.2.8 not applicable to literature)"^^xsd:string .

:CCSS.ELA-Literacy.RL.2.9 rdf:type owl:Class ;
    prov:wasQuotedFrom <http://www.corestandards.org/ELA-Literacy/RL/2/9/> ;
    rdfs:subClassOf :CCSS.ELA-Literacy.RL.2 ;
    rdfs:comment "Compare and contrast two or more versions of the same story (e.g., Cinderella stories) by different authors or from different cultures."^^xsd:string .

:CCSS.ELA-Literacy.RL.2.10 rdf:type owl:Class ;
    prov:wasQuotedFrom <http://www.corestandards.org/ELA-Literacy/RL/2/10/> ;
    rdfs:subClassOf :CCSS.ELA-Literacy.RL.2 ;
    rdfs:comment "By the end of the year, read and comprehend literature, including stories and poetry, in the grades 2-3 text complexity band proficiently, with scaffolding as needed at the high end of the range."^^xsd:string .

:CCSS.ELA-Literacy.RL.3 rdf:type owl:Class ;
    prov:wasQuotedFrom <http://www.corestandards.org/ELA-Literacy/RL/3/> ;
    rdfs:subClassOf :CCSS.ELA-Literacy.RL .

:CCSS.ELA-Literacy.RL.3.1 rdf:type owl:Class ;
    prov:wasQuotedFrom <http://www.corestandards.org/ELA-Literacy/RL/3/1/> ;
    rdfs:subClassOf :CCSS.ELA-Literacy.RL.3 ;
    rdfs:comment "Ask and answer questions to demonstrate understanding of a text, referring explicitly to the text as the basis for the answers."^^xsd:string .

:CCSS.ELA-Literacy.RL.3.2 rdf:type owl:Class ;
    prov:wasQuotedFrom <http://www.corestandards.org/ELA-Literacy/RL/3/2/> ;
    rdfs:subClassOf :CCSS.ELA-Literacy.RL.3 ;
    rdfs:comment "Recount stories, including fables, folktales, and myths from diverse cultures; determine the central message, lesson, or moral and explain how it is conveyed through key details in the text."^^xsd:string .

:CCSS.ELA-Literacy.RL.3.3 rdf:type owl:Class ;
    prov:wasQuotedFrom <http://www.corestandards.org/ELA-Literacy/RL/3/3/> ;
    rdfs:subClassOf :CCSS.ELA-Literacy.RL.3 ;
    rdfs:comment "Describe characters in a story (e.g., their traits, motivations, or feelings) and explain how their actions contribute to the sequence of events"^^xsd:string .

:CCSS.ELA-Literacy.RL.3.4 rdf:type owl:Class ;
    prov:wasQuotedFrom <http://www.corestandards.org/ELA-Literacy/RL/3/4/> ;
    rdfs:subClassOf :CCSS.ELA-Literacy.RL.3 ;
    rdfs:comment "Determine the meaning of words and phrases as they are used in a text, distinguishing literal from nonliteral language."^^xsd:string .

:CCSS.ELA-Literacy.RL.3.5 rdf:type owl:Class ;
    prov:wasQuotedFrom <http://www.corestandards.org/ELA-Literacy/RL/3/5/> ;
    rdfs:subClassOf :CCSS.ELA-Literacy.RL.3 ;
    rdfs:comment "Refer to parts of stories, dramas, and poems when writing or speaking about a text, using terms such as chapter, scene, and stanza; describe how each successive part builds on earlier sections."^^xsd:string .

:CCSS.ELA-Literacy.RL.3.6 rdf:type owl:Class ;
    prov:wasQuotedFrom <http://www.corestandards.org/ELA-Literacy/RL/3/6/> ;
    rdfs:subClassOf :CCSS.ELA-Literacy.RL.3 ;
    rdfs:comment "Distinguish their own point of view from that of the narrator or those of the characters."^^xsd:string .

:CCSS.ELA-Literacy.RL.3.7 rdf:type owl:Class ;
    prov:wasQuotedFrom <http://www.corestandards.org/ELA-Literacy/RL/3/7/> ;
    rdfs:subClassOf :CCSS.ELA-Literacy.RL.3 ;
    rdfs:comment "Explain how specific aspects of a text's illustrations contribute to what is conveyed by the words in a story (e.g., create mood, emphasize aspects of a character or setting)"^^xsd:string .

:CCSS.ELA-Literacy.RL.3.8 rdf:type owl:Class ;
    prov:wasQuotedFrom <http://www.corestandards.org/ELA-Literacy/RL/3/8/> ;
    rdfs:subClassOf :CCSS.ELA-Literacy.RL.3 ;
    rdfs:comment "(RL.3.8 not applicable to literature)"^^xsd:string .

:CCSS.ELA-Literacy.RL.3.9 rdf:type owl:Class ;
    prov:wasQuotedFrom <http://www.corestandards.org/ELA-Literacy/RL/3/9/> ;
    rdfs:subClassOf :CCSS.ELA-Literacy.RL.3 ;
    rdfs:comment "Compare and contrast the themes, settings, and plots of stories written by the same author about the same or similar characters (e.g., in books from a series)"^^xsd:string .

:CCSS.ELA-Literacy.RL.3.10 rdf:type owl:Class ;
    prov:wasQuotedFrom <http://www.corestandards.org/ELA-Literacy/RL/3/10/> ;
    rdfs:subClassOf :CCSS.ELA-Literacy.RL.3 ;
    rdfs:comment "By the end of the year, read and comprehend literature, including stories, dramas, and poetry, at the high end of the grades 2-3 text complexity band independently and proficiently."^^xsd:string .

:CCSS.ELA-Literacy.RL.4 rdf:type owl:Class ;
    prov:wasQuotedFrom <http://www.corestandards.org/ELA-Literacy/RL/4/> ;
    rdfs:subClassOf :CCSS.ELA-Literacy.RL .

:CCSS.ELA-Literacy.RL.4.1 rdf:type owl:Class ;
    prov:wasQuotedFrom <http://www.corestandards.org/ELA-Literacy/RL/4/1/> ;
    rdfs:subClassOf :CCSS.ELA-Literacy.RL.4 ;
    rdfs:comment "Refer to details and examples in a text when explaining what the text says explicitly and when drawing inferences from the text."^^xsd:string .

:CCSS.ELA-Literacy.RL.4.2 rdf:type owl:Class ;
    prov:wasQuotedFrom <http://www.corestandards.org/ELA-Literacy/RL/4/2/> ;
    rdfs:subClassOf :CCSS.ELA-Literacy.RL.4 ;
    rdfs:comment "Determine a theme of a story, drama, or poem from details in the text; summarize the text."^^xsd:string .

:CCSS.ELA-Literacy.RL.4.3 rdf:type owl:Class ;
    prov:wasQuotedFrom <http://www.corestandards.org/ELA-Literacy/RL/4/3/> ;
    rdfs:subClassOf :CCSS.ELA-Literacy.RL.4 ;
    rdfs:comment "Describe in depth a character, setting, or event in a story or drama, drawing on specific details in the text (e.g., a character's thoughts, words, or actions)."^^xsd:string .

:CCSS.ELA-Literacy.RL.4.4 rdf:type owl:Class ;
    prov:wasQuotedFrom <http://www.corestandards.org/ELA-Literacy/RL/4/4/> ;
    rdfs:subClassOf :CCSS.ELA-Literacy.RL.4 ;
    rdfs:comment "Determine the meaning of words and phrases as they are used in a text, including those that allude to significant characters found in mythology (e.g., Herculean)."^^xsd:string .

:CCSS.ELA-Literacy.RL.4.5 rdf:type owl:Class ;
    prov:wasQuotedFrom <http://www.corestandards.org/ELA-Literacy/RL/4/5/> ;
    rdfs:subClassOf :CCSS.ELA-Literacy.RL.4 ;
    rdfs:comment "Explain major differences between poems, drama, and prose, and refer to the structural elements of poems (e.g., verse, rhythm, meter) and drama (e.g., casts of characters, settings, descriptions, dialogue, stage directions) when writing or speaking about a text."^^xsd:string .

:CCSS.ELA-Literacy.RL.4.6 rdf:type owl:Class ;
    prov:wasQuotedFrom <http://www.corestandards.org/ELA-Literacy/RL/4/6/> ;
    rdfs:subClassOf :CCSS.ELA-Literacy.RL.4 ;
    rdfs:comment "Compare and contrast the point of view from which different stories are narrated, including the difference between first- and third-person narrations."^^xsd:string .

:CCSS.ELA-Literacy.RL.4.7 rdf:type owl:Class ;
    prov:wasQuotedFrom <http://www.corestandards.org/ELA-Literacy/RL/4/7/> ;
    rdfs:subClassOf :CCSS.ELA-Literacy.RL.4 ;
    rdfs:comment "Make connections between the text of a story or drama and a visual or oral presentation of the text, identifying where each version reflects specific descriptions and directions in the text."^^xsd:string .

:CCSS.ELA-Literacy.RL.4.8 rdf:type owl:Class ;
    prov:wasQuotedFrom <http://www.corestandards.org/ELA-Literacy/RL/4/8/> ;
    rdfs:subClassOf :CCSS.ELA-Literacy.RL.4 ;
    rdfs:comment "(RL.4.8 not applicable to literature)"^^xsd:string .

:CCSS.ELA-Literacy.RL.4.9 rdf:type owl:Class ;
    prov:wasQuotedFrom <http://www.corestandards.org/ELA-Literacy/RL/4/9/> ;
    rdfs:subClassOf :CCSS.ELA-Literacy.RL.4 ;
    rdfs:comment "Compare and contrast the treatment of similar themes and topics (e.g., opposition of good and evil) and patterns of events (e.g., the quest) in stories, myths, and traditional literature from different cultures."^^xsd:string .

:CCSS.ELA-Literacy.RL.4.10 rdf:type owl:Class ;
    prov:wasQuotedFrom <http://www.corestandards.org/ELA-Literacy/RL/4/10/> ;
    rdfs:subClassOf :CCSS.ELA-Literacy.RL.4 ;
    rdfs:comment "By the end of the year, read and comprehend literature, including stories, dramas, and poetry, in the grades 4-5 text complexity band proficiently, with scaffolding as needed at the high end of the range."^^xsd:string .

:CCSS.ELA-Literacy.RL.5 rdf:type owl:Class ;
    prov:wasQuotedFrom <http://www.corestandards.org/ELA-Literacy/RL/5/> ;
    rdfs:subClassOf :CCSS.ELA-Literacy.RL .

:CCSS.ELA-Literacy.RL.5.1 rdf:type owl:Class ;
    prov:wasQuotedFrom <http://www.corestandards.org/ELA-Literacy/RL/5/1/> ;
    rdfs:subClassOf :CCSS.ELA-Literacy.RL.5 ;
    rdfs:comment "Quote accurately from a text when explaining what the text says explicitly and when drawing inferences from the text."^^xsd:string .

:CCSS.ELA-Literacy.RL.5.2 rdf:type owl:Class ;
    prov:wasQuotedFrom <http://www.corestandards.org/ELA-Literacy/RL/5/2/> ;
    rdfs:subClassOf :CCSS.ELA-Literacy.RL.5 ;
    rdfs:comment "Determine a theme of a story, drama, or poem from details in the text, including how characters in a story or drama respond to challenges or how the speaker in a poem reflects upon a topic; summarize the text."^^xsd:string .

:CCSS.ELA-Literacy.RL.5.3 rdf:type owl:Class ;
    prov:wasQuotedFrom <http://www.corestandards.org/ELA-Literacy/RL/5/3/> ;
    rdfs:subClassOf :CCSS.ELA-Literacy.RL.5 ;
    rdfs:comment "Compare and contrast two or more characters, settings, or events in a story or drama, drawing on specific details in the text (e.g., how characters interact)."^^xsd:string .

:CCSS.ELA-Literacy.RL.5.4 rdf:type owl:Class ;
    prov:wasQuotedFrom <http://www.corestandards.org/ELA-Literacy/RL/5/4/> ;
    rdfs:subClassOf :CCSS.ELA-Literacy.RL.5 ;
    rdfs:comment "Determine the meaning of words and phrases as they are used in a text, including figurative language such as metaphors and similes."^^xsd:string .

:CCSS.ELA-Literacy.RL.5.5 rdf:type owl:Class ;
    prov:wasQuotedFrom <http://www.corestandards.org/ELA-Literacy/RL/5/5/> ;
    rdfs:subClassOf :CCSS.ELA-Literacy.RL.5 ;
    rdfs:comment "Explain how a series of chapters, scenes, or stanzas fits together to provide the overall structure of a particular story, drama, or poem."^^xsd:string .

:CCSS.ELA-Literacy.RL.5.6 rdf:type owl:Class ;
    prov:wasQuotedFrom <http://www.corestandards.org/ELA-Literacy/RL/5/6/> ;
    rdfs:subClassOf :CCSS.ELA-Literacy.RL.5 ;
    rdfs:comment "Describe how a narrator's or speaker's point of view influences how events are described."^^xsd:string .

:CCSS.ELA-Literacy.RL.5.7 rdf:type owl:Class ;
    prov:wasQuotedFrom <http://www.corestandards.org/ELA-Literacy/RL/5/7/> ;
    rdfs:subClassOf :CCSS.ELA-Literacy.RL.5 ;
    rdfs:comment "Analyze how visual and multimedia elements contribute to the meaning, tone, or beauty of a text (e.g., graphic novel, multimedia presentation of fiction, folktale, myth, poem)."^^xsd:string .

:CCSS.ELA-Literacy.RL.5.8 rdf:type owl:Class ;
    prov:wasQuotedFrom <http://www.corestandards.org/ELA-Literacy/RL/5/8/> ;
    rdfs:subClassOf :CCSS.ELA-Literacy.RL.5 ;
    rdfs:comment "(RL.5.8 not applicable to literature)"^^xsd:string .

:CCSS.ELA-Literacy.RL.5.9 rdf:type owl:Class ;
    prov:wasQuotedFrom <http://www.corestandards.org/ELA-Literacy/RL/5/9/> ;
    rdfs:subClassOf :CCSS.ELA-Literacy.RL.5 ;
    rdfs:comment "Compare and contrast stories in the same genre (e.g., mysteries and adventure stories) on their approaches to similar themes and topics."^^xsd:string .

:CCSS.ELA-Literacy.RL.5.10 rdf:type owl:Class ;
    prov:wasQuotedFrom <http://www.corestandards.org/ELA-Literacy/RL/5/10/> ;
    rdfs:subClassOf :CCSS.ELA-Literacy.RL.5 ;
    rdfs:comment "By the end of the year, read and comprehend literature, including stories, dramas, and poetry, at the high end of the grades 4-5 text complexity band independently and proficiently."^^xsd:string .

:CCSS.ELA-Literacy.RL.6 rdf:type owl:Class ;
    prov:wasQuotedFrom <http://www.corestandards.org/ELA-Literacy/RL/6/> ;
    rdfs:subClassOf :CCSS.ELA-Literacy.RL .

:CCSS.ELA-Literacy.RL.6.1 rdf:type owl:Class ;
    prov:wasQuotedFrom <http://www.corestandards.org/ELA-Literacy/RL/6/1/> ;
    rdfs:subClassOf :CCSS.ELA-Literacy.RL.6 ;
    rdfs:comment "Cite textual evidence to support analysis of what the text says explicitly as well as inferences drawn from the text."^^xsd:string .

:CCSS.ELA-Literacy.RL.6.2 rdf:type owl:Class ;
    prov:wasQuotedFrom <http://www.corestandards.org/ELA-Literacy/RL/6/2/> ;
    rdfs:subClassOf :CCSS.ELA-Literacy.RL.6 ;
    rdfs:comment "Determine a theme or central idea of a text and how it is conveyed through particular details; provide a summary of the text distinct from personal opinions or judgments."^^xsd:string .

:CCSS.ELA-Literacy.RL.6.3 rdf:type owl:Class ;
    prov:wasQuotedFrom <http://www.corestandards.org/ELA-Literacy/RL/6/3/> ;
    rdfs:subClassOf :CCSS.ELA-Literacy.RL.6 ;
    rdfs:comment "Describe how a particular story's or drama's plot unfolds in a series of episodes as well as how the characters respond or change as the plot moves toward a resolution."^^xsd:string .

:CCSS.ELA-Literacy.RL.6.4 rdf:type owl:Class ;
    prov:wasQuotedFrom <http://www.corestandards.org/ELA-Literacy/RL/6/4/> ;
    rdfs:subClassOf :CCSS.ELA-Literacy.RL.6 ;
    rdfs:comment "Determine the meaning of words and phrases as they are used in a text, including figurative and connotative meanings; analyze the impact of a specific word choice on meaning and tone"^^xsd:string .

:CCSS.ELA-Literacy.RL.6.5 rdf:type owl:Class ;
    prov:wasQuotedFrom <http://www.corestandards.org/ELA-Literacy/RL/6/5/> ;
    rdfs:subClassOf :CCSS.ELA-Literacy.RL.6 ;
    rdfs:comment "Analyze how a particular sentence, chapter, scene, or stanza fits into the overall structure of a text and contributes to the development of the theme, setting, or plot."^^xsd:string .

:CCSS.ELA-Literacy.RL.6.6 rdf:type owl:Class ;
    prov:wasQuotedFrom <http://www.corestandards.org/ELA-Literacy/RL/6/6/> ;
    rdfs:subClassOf :CCSS.ELA-Literacy.RL.6 ;
    rdfs:comment "Explain how an author develops the point of view of the narrator or speaker in a text."^^xsd:string .

:CCSS.ELA-Literacy.RL.6.7 rdf:type owl:Class ;
    prov:wasQuotedFrom <http://www.corestandards.org/ELA-Literacy/RL/6/7/> ;
    rdfs:subClassOf :CCSS.ELA-Literacy.RL.6 ;
    rdfs:comment "Compare and contrast the experience of reading a story, drama, or poem to listening to or viewing an audio, video, or live version of the text, including contrasting what they 'see' and 'hear' when reading the text to what they perceive when they listen or watch."^^xsd:string .

:CCSS.ELA-Literacy.RL.6.8 rdf:type owl:Class ;
    prov:wasQuotedFrom <http://www.corestandards.org/ELA-Literacy/RL/6/8/> ;
    rdfs:subClassOf :CCSS.ELA-Literacy.RL.6 ;
    rdfs:comment "(RL.6.8 not applicable to literature)"^^xsd:string .

:CCSS.ELA-Literacy.RL.6.9 rdf:type owl:Class ;
    prov:wasQuotedFrom <http://www.corestandards.org/ELA-Literacy/RL/6/9/> ;
    rdfs:subClassOf :CCSS.ELA-Literacy.RL.6 ;
    rdfs:comment "Compare and contrast texts in different forms or genres (e.g., stories and poems; historical novels and fantasy stories) in terms of their approaches to similar themes and topics."^^xsd:string .

:CCSS.ELA-Literacy.RL.6.10 rdf:type owl:Class ;
    prov:wasQuotedFrom <http://www.corestandards.org/ELA-Literacy/RL/6/10/> ;
    rdfs:subClassOf :CCSS.ELA-Literacy.RL.6 ;
    rdfs:comment " By the end of the year, read and comprehend literature, including stories, dramas, and poems, in the grades 6-8 text complexity band proficiently, with scaffolding as needed at the high end of the range."^^xsd:string .

:CCSS.ELA-Literacy.RL.7 rdf:type owl:Class ;
    prov:wasQuotedFrom <http://www.corestandards.org/ELA-Literacy/RL/7/> ;
    rdfs:subClassOf :CCSS.ELA-Literacy.RL .

:CCSS.ELA-Literacy.RL.7.1 rdf:type owl:Class ;
    prov:wasQuotedFrom <http://www.corestandards.org/ELA-Literacy/RL/7/1/> ;
    rdfs:subClassOf :CCSS.ELA-Literacy.RL.7 ;
    rdfs:comment "Cite several pieces of textual evidence to support analysis of what the text says explicitly as well as inferences drawn from the text."^^xsd:string .

:CCSS.ELA-Literacy.RL.7.2 rdf:type owl:Class ;
    prov:wasQuotedFrom <http://www.corestandards.org/ELA-Literacy/RL/7/2/> ;
    rdfs:subClassOf :CCSS.ELA-Literacy.RL.7 ;
    rdfs:comment "Determine a theme or central idea of a text and analyze its development over the course of the text; provide an objective summary of the text."^^xsd:string .

:CCSS.ELA-Literacy.RL.7.3 rdf:type owl:Class ;
    prov:wasQuotedFrom <http://www.corestandards.org/ELA-Literacy/RL/7/3/> ;
    rdfs:subClassOf :CCSS.ELA-Literacy.RL.7 ;
    rdfs:comment "Analyze how particular elements of a story or drama interact (e.g., how setting shapes the characters or plot)."^^xsd:string .

:CCSS.ELA-Literacy.RL.7.4 rdf:type owl:Class ;
    prov:wasQuotedFrom <http://www.corestandards.org/ELA-Literacy/RL/7/4/> ;
    rdfs:subClassOf :CCSS.ELA-Literacy.RL.7 ;
    rdfs:comment "Determine the meaning of words and phrases as they are used in a text, including figurative and connotative meanings; analyze the impact of rhymes and other repetitions of sounds (e.g., alliteration) on a specific verse or stanza of a poem or section of a story or drama."^^xsd:string .

:CCSS.ELA-Literacy.RL.7.5 rdf:type owl:Class ;
    prov:wasQuotedFrom <http://www.corestandards.org/ELA-Literacy/RL/7/5/> ;
    rdfs:subClassOf :CCSS.ELA-Literacy.RL.7 ;
    rdfs:comment "Analyze how a drama's or poem's form or structure (e.g., soliloquy, sonnet) contributes to its meaning"^^xsd:string .

:CCSS.ELA-Literacy.RL.7.6 rdf:type owl:Class ;
    prov:wasQuotedFrom <http://www.corestandards.org/ELA-Literacy/RL/7/6/> ;
    rdfs:subClassOf :CCSS.ELA-Literacy.RL.7 ;
    rdfs:comment "Analyze how an author develops and contrasts the points of view of different characters or narrators in a text."^^xsd:string .

:CCSS.ELA-Literacy.RL.7.7 rdf:type owl:Class ;
    prov:wasQuotedFrom <http://www.corestandards.org/ELA-Literacy/RL/7/7/> ;
    rdfs:subClassOf :CCSS.ELA-Literacy.RL.7 ;
    rdfs:comment "Compare and contrast a written story, drama, or poem to its audio, filmed, staged, or multimedia version, analyzing the effects of techniques unique to each medium (e.g., lighting, sound, color, or camera focus and angles in a film)."^^xsd:string .

:CCSS.ELA-Literacy.RL.7.8 rdf:type owl:Class ;
    prov:wasQuotedFrom <http://www.corestandards.org/ELA-Literacy/RL/7/8/> ;
    rdfs:subClassOf :CCSS.ELA-Literacy.RL.7 ;
    rdfs:comment "(RL.7.8 not applicable to literature)"^^xsd:string .

:CCSS.ELA-Literacy.RL.7.9 rdf:type owl:Class ;
    prov:wasQuotedFrom <http://www.corestandards.org/ELA-Literacy/RL/7/9/> ;
    rdfs:subClassOf :CCSS.ELA-Literacy.RL.7 ;
    rdfs:comment "Compare and contrast a fictional portrayal of a time, place, or character and a historical account of the same period as a means of understanding how authors of fiction use or alter history."^^xsd:string .

:CCSS.ELA-Literacy.RL.7.10 rdf:type owl:Class ;
    prov:wasQuotedFrom <http://www.corestandards.org/ELA-Literacy/RL/7/10/> ;
    rdfs:subClassOf :CCSS.ELA-Literacy.RL.7 ;
    rdfs:comment "By the end of the year, read and comprehend literature, including stories, dramas, and poems, in the grades 6-8 text complexity band proficiently, with scaffolding as needed at the high end of the range."^^xsd:string .

:CCSS.ELA-Literacy.RL.8 rdf:type owl:Class ;
    prov:wasQuotedFrom <http://www.corestandards.org/ELA-Literacy/RL/8/> ;
    rdfs:subClassOf :CCSS.ELA-Literacy.RL .

:CCSS.ELA-Literacy.RL.8.1 rdf:type owl:Class ;
    prov:wasQuotedFrom <http://www.corestandards.org/ELA-Literacy/RL/8/1/> ;
    rdfs:subClassOf :CCSS.ELA-Literacy.RL.8 ;
    rdfs:comment "Cite the textual evidence that most strongly supports an analysis of what the text says explicitly as well as inferences drawn from the text."^^xsd:string .

:CCSS.ELA-Literacy.RL.8.2 rdf:type owl:Class ;
    prov:wasQuotedFrom <http://www.corestandards.org/ELA-Literacy/RL/8/2/> ;
    rdfs:subClassOf :CCSS.ELA-Literacy.RL.8 ;
    rdfs:comment "Determine a theme or central idea of a text and analyze its development over the course of the text, including its relationship to the characters, setting, and plot; provide an objective summary of the text."^^xsd:string .

:CCSS.ELA-Literacy.RL.8.3 rdf:type owl:Class ;
    prov:wasQuotedFrom <http://www.corestandards.org/ELA-Literacy/RL/8/3/> ;
    rdfs:subClassOf :CCSS.ELA-Literacy.RL.8 ;
    rdfs:comment "Analyze how particular lines of dialogue or incidents in a story or drama propel the action, reveal aspects of a character, or provoke a decision."^^xsd:string .

:CCSS.ELA-Literacy.RL.8.4 rdf:type owl:Class ;
    prov:wasQuotedFrom <http://www.corestandards.org/ELA-Literacy/RL/8/4/> ;
    rdfs:subClassOf :CCSS.ELA-Literacy.RL.8 ;
    rdfs:comment "Determine the meaning of words and phrases as they are used in a text, including figurative and connotative meanings; analyze the impact of specific word choices on meaning and tone, including analogies or allusions to other texts."^^xsd:string .

:CCSS.ELA-Literacy.RL.8.5 rdf:type owl:Class ;
    prov:wasQuotedFrom <http://www.corestandards.org/ELA-Literacy/RL/8/5/> ;
    rdfs:subClassOf :CCSS.ELA-Literacy.RL.8 ;
    rdfs:comment "Compare and contrast the structure of two or more texts and analyze how the differing structure of each text contributes to its meaning and style."^^xsd:string .

:CCSS.ELA-Literacy.RL.8.6 rdf:type owl:Class ;
    prov:wasQuotedFrom <http://www.corestandards.org/ELA-Literacy/RL/8/6/> ;
    rdfs:subClassOf :CCSS.ELA-Literacy.RL.8 ;
    rdfs:comment "Analyze how differences in the points of view of the characters and the audience or reader (e.g., created through the use of dramatic irony) create such effects as suspense or humor."^^xsd:string .

:CCSS.ELA-Literacy.RL.8.7 rdf:type owl:Class ;
    prov:wasQuotedFrom <http://www.corestandards.org/ELA-Literacy/RL/8/7/> ;
    rdfs:subClassOf :CCSS.ELA-Literacy.RL.8 ;
    rdfs:comment "Analyze the extent to which a filmed or live production of a story or drama stays faithful to or departs from the text or script, evaluating the choices made by the director or actors."^^xsd:string .

:CCSS.ELA-Literacy.RL.8.8 rdf:type owl:Class ;
    prov:wasQuotedFrom <http://www.corestandards.org/ELA-Literacy/RL/8/8/> ;
    rdfs:subClassOf :CCSS.ELA-Literacy.RL.8 ;
    rdfs:comment "(RL.8.8 not applicable to literature)"^^xsd:string .

:CCSS.ELA-Literacy.RL.8.9 rdf:type owl:Class ;
    prov:wasQuotedFrom <http://www.corestandards.org/ELA-Literacy/RL/8/9/> ;
    rdfs:subClassOf :CCSS.ELA-Literacy.RL.8 ;
    rdfs:comment "Analyze how a modern work of fiction draws on themes, patterns of events, or character types from myths, traditional stories, or religious works such as the Bible, including describing how the material is rendered new."^^xsd:string .

:CCSS.ELA-Literacy.RL.8.10 rdf:type owl:Class ;
    prov:wasQuotedFrom <http://www.corestandards.org/ELA-Literacy/RL/8/10/> ;
    rdfs:subClassOf :CCSS.ELA-Literacy.RL.8 ;
    rdfs:comment "By the end of the year, read and comprehend literature, including stories, dramas, and poems, at the high end of grades 6-8 text complexity band independently and proficiently."^^xsd:string .

:CCSS.ELA-Literacy.RL.9-10 rdf:type owl:Class ;
    prov:wasQuotedFrom <http://www.corestandards.org/ELA-Literacy/RL/9-10/> ;
    rdfs:subClassOf :CCSS.ELA-Literacy.RL .

:CCSS.ELA-Literacy.RL.9-10.1 rdf:type owl:Class ;
    prov:wasQuotedFrom <http://www.corestandards.org/ELA-Literacy/RL/9-10/1/> ;
    rdfs:subClassOf :CCSS.ELA-Literacy.RL.9-10 ;
    rdfs:comment "Cite strong and thorough textual evidence to support analysis of what the text says explicitly as well as inferences drawn from the text."^^xsd:string .

:CCSS.ELA-Literacy.RL.9-10.2 rdf:type owl:Class ;
    prov:wasQuotedFrom <http://www.corestandards.org/ELA-Literacy/RL/9-10/2/> ;
    rdfs:subClassOf :CCSS.ELA-Literacy.RL.9-10 ;
    rdfs:comment "Determine a theme or central idea of a text and analyze in detail its development over the course of the text, including how it emerges and is shaped and refined by specific details; provide an objective summary of the text."^^xsd:string .

:CCSS.ELA-Literacy.RL.9-10.3 rdf:type owl:Class ;
    prov:wasQuotedFrom <http://www.corestandards.org/ELA-Literacy/RL/9-10/3/> ;
    rdfs:subClassOf :CCSS.ELA-Literacy.RL.9-10 ;
    rdfs:comment "Analyze how complex characters (e.g., those with multiple or conflicting motivations) develop over the course of a text, interact with other characters, and advance the plot or develop the theme."^^xsd:string .

:CCSS.ELA-Literacy.RL.9-10.4 rdf:type owl:Class ;
    prov:wasQuotedFrom <http://www.corestandards.org/ELA-Literacy/RL/9-10/4/> ;
    rdfs:subClassOf :CCSS.ELA-Literacy.RL.9-10 ;
    rdfs:comment "Determine the meaning of words and phrases as they are used in the text, including figurative and connotative meanings; analyze the cumulative impact of specific word choices on meaning and tone (e.g., how the language evokes a sense of time and place; how it sets a formal or informal tone)."^^xsd:string .

:CCSS.ELA-Literacy.RL.9-10.5 rdf:type owl:Class ;
    prov:wasQuotedFrom <http://www.corestandards.org/ELA-Literacy/RL/9-10/5/> ;
    rdfs:subClassOf :CCSS.ELA-Literacy.RL.9-10 ;
    rdfs:comment "Analyze how an author's choices concerning how to structure a text, order events within it (e.g., parallel plots), and manipulate time (e.g., pacing, flashbacks) create such effects as mystery, tension, or surprise."^^xsd:string .

:CCSS.ELA-Literacy.RL.9-10.6 rdf:type owl:Class ;
    prov:wasQuotedFrom <http://www.corestandards.org/ELA-Literacy/RL/9-10/6/> ;
    rdfs:subClassOf :CCSS.ELA-Literacy.RL.9-10 ;
    rdfs:comment "Analyze a particular point of view or cultural experience reflected in a work of literature from outside the United States, drawing on a wide reading of world literature. "^^xsd:string .

:CCSS.ELA-Literacy.RL.9-10.7 rdf:type owl:Class ;
    prov:wasQuotedFrom <http://www.corestandards.org/ELA-Literacy/RL/9-10/7/> ;
    rdfs:subClassOf :CCSS.ELA-Literacy.RL.9-10 ;
    rdfs:comment "Analyze the representation of a subject or a key scene in two different artistic mediums, including what is emphasized or absent in each treatment (e.g., Auden's 'Muse des Beaux Arts' and Breughel's Landscape with the Fall of Icarus)."^^xsd:string .

:CCSS.ELA-Literacy.RL.9-10.8 rdf:type owl:Class ;
    prov:wasQuotedFrom <http://www.corestandards.org/ELA-Literacy/RL/9-10/8/> ;
    rdfs:subClassOf :CCSS.ELA-Literacy.RL.9-10 ;
    rdfs:comment "(RL.9-10.8 not applicable to literature)"^^xsd:string .

:CCSS.ELA-Literacy.RL.9-10.9 rdf:type owl:Class ;
    prov:wasQuotedFrom <http://www.corestandards.org/ELA-Literacy/RL/9-10/9/> ;
    rdfs:subClassOf :CCSS.ELA-Literacy.RL.9-10 ;
    rdfs:comment "Analyze how an author draws on and transforms source material in a specific work (e.g., how Shakespeare treats a theme or topic from Ovid or the Bible or how a later author draws on a play by Shakespeare)."^^xsd:string .

:CCSS.ELA-Literacy.RL.9-10.10 rdf:type owl:Class ;
    prov:wasQuotedFrom <http://www.corestandards.org/ELA-Literacy/RL/9-10/10/> ;
    rdfs:subClassOf :CCSS.ELA-Literacy.RL.9-10 ;
    rdfs:comment "By the end of grade 9, read and comprehend literature, including stories, dramas, and poems, in the grades 9-10 text complexity band proficiently, with scaffolding as needed at the high end of the range.
By the end of grade 10, read and comprehend literature, including stories, dramas, and poems, at the high end of the grades 9-10 text complexity band independently and proficiently."^^xsd:string .

:CCSS.ELA-Literacy.RL.11-12 rdf:type owl:Class ;
    prov:wasQuotedFrom <http://www.corestandards.org/ELA-Literacy/RL/11-12/> ;
    rdfs:subClassOf :CCSS.ELA-Literacy.RL .

:CCSS.ELA-Literacy.RL.11-12.1 rdf:type owl:Class ;
    prov:wasQuotedFrom <http://www.corestandards.org/ELA-Literacy/RL/11-12/1/> ;
    rdfs:subClassOf :CCSS.ELA-Literacy.RL.11-12 ;
    rdfs:comment "Cite strong and thorough textual evidence to support analysis of what the text says explicitly as well as inferences drawn from the text, including determining where the text leaves matters uncertain."^^xsd:string .

:CCSS.ELA-Literacy.RL.11-12.2 rdf:type owl:Class ;
    prov:wasQuotedFrom <http://www.corestandards.org/ELA-Literacy/RL/11-12/2/> ;
    rdfs:subClassOf :CCSS.ELA-Literacy.RL.11-12 ;
    rdfs:comment "Determine two or more themes or central ideas of a text and analyze their development over the course of the text, including how they interact and build on one another to produce a complex account; provide an objective summary of the text."^^xsd:string .

:CCSS.ELA-Literacy.RL.11-12.3 rdf:type owl:Class ;
    prov:wasQuotedFrom <http://www.corestandards.org/ELA-Literacy/RL/11-12/3/> ;
    rdfs:subClassOf :CCSS.ELA-Literacy.RL.11-12 ;
    rdfs:comment "Analyze the impact of the author's choices regarding how to develop and relate elements of a story or drama (e.g., where a story is set, how the action is ordered, how the characters are introduced and developed)."^^xsd:string .

:CCSS.ELA-Literacy.RL.11-12.4 rdf:type owl:Class ;
    prov:wasQuotedFrom <http://www.corestandards.org/ELA-Literacy/RL/11-12/4/> ;
    rdfs:subClassOf :CCSS.ELA-Literacy.RL.11-12 ;
    rdfs:comment "Determine the meaning of words and phrases as they are used in the text, including figurative and connotative meanings; analyze the impact of specific word choices on meaning and tone, including words with multiple meanings or language that is particularly fresh, engaging, or beautiful. (Include Shakespeare as well as other authors.)"^^xsd:string .

:CCSS.ELA-Literacy.RL.11-12.5 rdf:type owl:Class ;
    prov:wasQuotedFrom <http://www.corestandards.org/ELA-Literacy/RL/11-12/5/> ;
    rdfs:subClassOf :CCSS.ELA-Literacy.RL.11-12 ;
    rdfs:comment "Analyze how an author's choices concerning how to structure specific parts of a text (e.g., the choice of where to begin or end a story, the choice to provide a comedic or tragic resolution) contribute to its overall structure and meaning as well as its aesthetic impact."^^xsd:string .

:CCSS.ELA-Literacy.RL.11-12.6 rdf:type owl:Class ;
    prov:wasQuotedFrom <http://www.corestandards.org/ELA-Literacy/RL/11-12/6/> ;
    rdfs:subClassOf :CCSS.ELA-Literacy.RL.11-12 ;
    rdfs:comment "Analyze a case in which grasping a point of view requires distinguishing what is directly stated in a text from what is really meant (e.g., satire, sarcasm, irony, or understatement). "^^xsd:string .

:CCSS.ELA-Literacy.RL.11-12.7 rdf:type owl:Class ;
    prov:wasQuotedFrom <http://www.corestandards.org/ELA-Literacy/RL/11-12/7/> ;
    rdfs:subClassOf :CCSS.ELA-Literacy.RL.11-12 ;
    rdfs:comment "Analyze multiple interpretations of a story, drama, or poem (e.g., recorded or live production of a play or recorded novel or poetry), evaluating how each version interprets the source text. (Include at least one play by Shakespeare and one play by an American dramatist.)"^^xsd:string .

:CCSS.ELA-Literacy.RL.11-12.8 rdf:type owl:Class ;
    prov:wasQuotedFrom <http://www.corestandards.org/ELA-Literacy/RL/11-12/8/> ;
    rdfs:subClassOf :CCSS.ELA-Literacy.RL.11-12 ;
    rdfs:comment "(RL.11-12.8 not applicable to literature)"^^xsd:string .

:CCSS.ELA-Literacy.RL.11-12.9 rdf:type owl:Class ;
    prov:wasQuotedFrom <http://www.corestandards.org/ELA-Literacy/RL/11-12/9/> ;
    rdfs:subClassOf :CCSS.ELA-Literacy.RL.11-12 ;
    rdfs:comment "Demonstrate knowledge of eighteenth-, nineteenth- and early-twentieth-century foundational works of American literature, including how two or more texts from the same period treat similar themes or topics."^^xsd:string .

:CCSS.ELA-Literacy.RL.11-12.10 rdf:type owl:Class ;
    prov:wasQuotedFrom <http://www.corestandards.org/ELA-Literacy/RL/11-12/10/> ;
    rdfs:subClassOf :CCSS.ELA-Literacy.RL.11-12 ;
    rdfs:comment "By the end of grade 11, read and comprehend literature, including stories, dramas, and poems, in the grades 11-CCR text complexity band proficiently, with scaffolding as needed at the high end of the range.
By the end of grade 12, read and comprehend literature, including stories, dramas, and poems, at the high end of the grades 11-CCR text complexity band independently and proficiently."^^xsd:string .

:CCSS.ELA-Literacy.RI.K.1 rdf:type owl:Class ;
    prov:wasQuotedFrom <http://www.corestandards.org/ELA-Literacy/RI/K/1/> ;
    rdfs:subClassOf :CCSS.ELA-Literacy.RI.K ;
    rdfs:comment "With prompting and support, ask and answer questions about key details in a text."^^xsd:string .

:CCSS.ELA-Literacy.RI.K.2 rdf:type owl:Class ;
    prov:wasQuotedFrom <http://www.corestandards.org/ELA-Literacy/RI/K/2/> ;
    rdfs:subClassOf :CCSS.ELA-Literacy.RI.K ;
    rdfs:comment "With prompting and support, identify the main topic and retell key details of a text."^^xsd:string .

:CCSS.ELA-Literacy.RI.K.3 rdf:type owl:Class ;
    prov:wasQuotedFrom <http://www.corestandards.org/ELA-Literacy/RI/K/3/> ;
    rdfs:subClassOf :CCSS.ELA-Literacy.RI.K ;
    rdfs:comment "With prompting and support, describe the connection between two individuals, events, ideas, or pieces of information in a text."^^xsd:string .

:CCSS.ELA-Literacy.RI.K.4 rdf:type owl:Class ;
    prov:wasQuotedFrom <http://www.corestandards.org/ELA-Literacy/RI/K/4/> ;
    rdfs:subClassOf :CCSS.ELA-Literacy.RI.K ;
    rdfs:comment "With prompting and support, ask and answer questions about unknown words in a text."^^xsd:string .

:CCSS.ELA-Literacy.RI.K.5 rdf:type owl:Class ;
    prov:wasQuotedFrom <http://www.corestandards.org/ELA-Literacy/RI/K/5/> ;
    rdfs:subClassOf :CCSS.ELA-Literacy.RI.K ;
    rdfs:comment "Identify the front cover, back cover, and title page of a book."^^xsd:string .

:CCSS.ELA-Literacy.RI.K.6 rdf:type owl:Class ;
    prov:wasQuotedFrom <http://www.corestandards.org/ELA-Literacy/RI/K/6/> ;
    rdfs:subClassOf :CCSS.ELA-Literacy.RI.K ;
    rdfs:comment "Name the author and illustrator of a text and define the role of each in presenting the ideas or information in a text."^^xsd:string .

:CCSS.ELA-Literacy.RI.K.7 rdf:type owl:Class ;
    prov:wasQuotedFrom <http://www.corestandards.org/ELA-Literacy/RI/K/7/> ;
    rdfs:subClassOf :CCSS.ELA-Literacy.RI.K ;
    rdfs:comment "With prompting and support, describe the relationship between illustrations and the text in which they appear (e.g., what person, place, thing, or idea in the text an illustration depicts)."^^xsd:string .

:CCSS.ELA-Literacy.RI.K.8 rdf:type owl:Class ;
    prov:wasQuotedFrom <http://www.corestandards.org/ELA-Literacy/RI/K/8/> ;
    rdfs:subClassOf :CCSS.ELA-Literacy.RI.K ;
    rdfs:comment "With prompting and support, identify the reasons an author gives to support points in a text."^^xsd:string .

:CCSS.ELA-Literacy.RI.K.9 rdf:type owl:Class ;
    prov:wasQuotedFrom <http://www.corestandards.org/ELA-Literacy/RI/K/9/> ;
    rdfs:subClassOf :CCSS.ELA-Literacy.RI.K ;
    rdfs:comment "With prompting and support, identify basic similarities in and differences between two texts on the same topic (e.g., in illustrations, descriptions, or procedures)."^^xsd:string .

:CCSS.ELA-Literacy.RI.K.10 rdf:type owl:Class ;
    prov:wasQuotedFrom <http://www.corestandards.org/ELA-Literacy/RI/K/10/> ;
    rdfs:subClassOf :CCSS.ELA-Literacy.RI.K ;
    rdfs:comment "Actively engage in group reading activities with purpose and understanding."^^xsd:string .

:CCSS.ELA-Literacy.RI.1.1 rdf:type owl:Class ;
    prov:wasQuotedFrom <http://www.corestandards.org/ELA-Literacy/RI/1/1/> ;
    rdfs:subClassOf :CCSS.ELA-Literacy.RI.1 ;
    rdfs:comment "Ask and answer questions about key details in a text."^^xsd:string .

:CCSS.ELA-Literacy.RI.1.2 rdf:type owl:Class ;
    prov:wasQuotedFrom <http://www.corestandards.org/ELA-Literacy/RI/1/2/> ;
    rdfs:subClassOf :CCSS.ELA-Literacy.RI.1 ;
    rdfs:comment "Identify the main topic and retell key details of a text."^^xsd:string .

:CCSS.ELA-Literacy.RI.1.3 rdf:type owl:Class ;
    prov:wasQuotedFrom <http://www.corestandards.org/ELA-Literacy/RI/1/3/> ;
    rdfs:subClassOf :CCSS.ELA-Literacy.RI.1 ;
    rdfs:comment "Describe the connection between two individuals, events, ideas, or pieces of information in a text."^^xsd:string .

:CCSS.ELA-Literacy.RI.1.4 rdf:type owl:Class ;
    prov:wasQuotedFrom <http://www.corestandards.org/ELA-Literacy/RI/1/4/> ;
    rdfs:subClassOf :CCSS.ELA-Literacy.RI.1 ;
    rdfs:comment "Ask and answer questions to help determine or clarify the meaning of words and phrases in a text."^^xsd:string .

:CCSS.ELA-Literacy.RI.1.5 rdf:type owl:Class ;
    prov:wasQuotedFrom <http://www.corestandards.org/ELA-Literacy/RI/1/5/> ;
    rdfs:subClassOf :CCSS.ELA-Literacy.RI.1 ;
    rdfs:comment "Know and use various text features (e.g., headings, tables of contents, glossaries, electronic menus, icons) to locate key facts or information in a text."^^xsd:string .

:CCSS.ELA-Literacy.RI.1.6 rdf:type owl:Class ;
    prov:wasQuotedFrom <http://www.corestandards.org/ELA-Literacy/RI/1/6/> ;
    rdfs:subClassOf :CCSS.ELA-Literacy.RI.1 ;
    rdfs:comment "Distinguish between information provided by pictures or other illustrations and information provided by the words in a text."^^xsd:string .

:CCSS.ELA-Literacy.RI.1.7 rdf:type owl:Class ;
    prov:wasQuotedFrom <http://www.corestandards.org/ELA-Literacy/RI/1/7/> ;
    rdfs:subClassOf :CCSS.ELA-Literacy.RI.1 ;
    rdfs:comment "Use the illustrations and details in a text to describe its key ideas."^^xsd:string .

:CCSS.ELA-Literacy.RI.1.8 rdf:type owl:Class ;
    prov:wasQuotedFrom <http://www.corestandards.org/ELA-Literacy/RI/1/8/> ;
    rdfs:subClassOf :CCSS.ELA-Literacy.RI.1 ;
    rdfs:comment "Identify the reasons an author gives to support points in a text."^^xsd:string .

:CCSS.ELA-Literacy.RI.1.9 rdf:type owl:Class ;
    prov:wasQuotedFrom <http://www.corestandards.org/ELA-Literacy/RI/1/9/> ;
    rdfs:subClassOf :CCSS.ELA-Literacy.RI.1 ;
    rdfs:comment "Identify basic similarities in and differences between two texts on the same topic (e.g., in illustrations, descriptions, or procedures)."^^xsd:string .

:CCSS.ELA-Literacy.RI.1.10 rdf:type owl:Class ;
    prov:wasQuotedFrom <http://www.corestandards.org/ELA-Literacy/RI/1/10/> ;
    rdfs:subClassOf :CCSS.ELA-Literacy.RI.1 ;
    rdfs:comment "With prompting and support, read informational texts appropriately complex for grade 1."^^xsd:string .

:CCSS.ELA-Literacy.RI.2.1 rdf:type owl:Class ;
    prov:wasQuotedFrom <http://www.corestandards.org/ELA-Literacy/RI/2/1/> ;
    rdfs:subClassOf :CCSS.ELA-Literacy.RI.2 ;
    rdfs:comment "Ask and answer such questions as who, what, where, when, why, and how to demonstrate understanding of key details in a text."^^xsd:string .

:CCSS.ELA-Literacy.RI.2.2 rdf:type owl:Class ;
    prov:wasQuotedFrom <http://www.corestandards.org/ELA-Literacy/RI/2/2/> ;
    rdfs:subClassOf :CCSS.ELA-Literacy.RI.2 ;
    rdfs:comment "Identify the main topic of a multiparagraph text as well as the focus of specific paragraphs within the text."^^xsd:string .

:CCSS.ELA-Literacy.RI.2.3 rdf:type owl:Class ;
    prov:wasQuotedFrom <http://www.corestandards.org/ELA-Literacy/RI/2/3/> ;
    rdfs:subClassOf :CCSS.ELA-Literacy.RI.2 ;
    rdfs:comment "Describe the connection between a series of historical events, scientific ideas or concepts, or steps in technical procedures in a text."^^xsd:string .

:CCSS.ELA-Literacy.RI.2.4 rdf:type owl:Class ;
    prov:wasQuotedFrom <http://www.corestandards.org/ELA-Literacy/RI/2/4/> ;
    rdfs:subClassOf :CCSS.ELA-Literacy.RI.2 ;
    rdfs:comment "Determine the meaning of words and phrases in a text relevant to a grade 2 topic or subject area."^^xsd:string .

:CCSS.ELA-Literacy.RI.2.5 rdf:type owl:Class ;
    prov:wasQuotedFrom <http://www.corestandards.org/ELA-Literacy/RI/2/5/> ;
    rdfs:subClassOf :CCSS.ELA-Literacy.RI.2 ;
    rdfs:comment "Know and use various text features (e.g., captions, bold print, subheadings, glossaries, indexes, electronic menus, icons) to locate key facts or information in a text efficiently."^^xsd:string .

:CCSS.ELA-Literacy.RI.2.6 rdf:type owl:Class ;
    prov:wasQuotedFrom <http://www.corestandards.org/ELA-Literacy/RI/2/6/> ;
    rdfs:subClassOf :CCSS.ELA-Literacy.RI.2 ;
    rdfs:comment "Identify the main purpose of a text, including what the author wants to answer, explain, or describe."^^xsd:string .

:CCSS.ELA-Literacy.RI.2.7 rdf:type owl:Class ;
    prov:wasQuotedFrom <http://www.corestandards.org/ELA-Literacy/RI/2/7/> ;
    rdfs:subClassOf :CCSS.ELA-Literacy.RI.2 ;
    rdfs:comment "Explain how specific images (e.g., a diagram showing how a machine works) contribute to and clarify a text."^^xsd:string .

:CCSS.ELA-Literacy.RI.2.8 rdf:type owl:Class ;
    prov:wasQuotedFrom <http://www.corestandards.org/ELA-Literacy/RI/2/8/> ;
    rdfs:subClassOf :CCSS.ELA-Literacy.RI.2 ;
    rdfs:comment "Describe how reasons support specific points the author makes in a text."^^xsd:string .

:CCSS.ELA-Literacy.RI.2.9 rdf:type owl:Class ;
    prov:wasQuotedFrom <http://www.corestandards.org/ELA-Literacy/RI/2/9/> ;
    rdfs:subClassOf :CCSS.ELA-Literacy.RI.2 ;
    rdfs:comment "Compare and contrast the most important points presented by two texts on the same topic."^^xsd:string .

:CCSS.ELA-Literacy.RI.2.10 rdf:type owl:Class ;
    prov:wasQuotedFrom <http://www.corestandards.org/ELA-Literacy/RI/2/10/> ;
    rdfs:subClassOf :CCSS.ELA-Literacy.RI.2 ;
    rdfs:comment "By the end of year, read and comprehend informational texts, including history/social studies, science, and technical texts, in the grades 2-3 text complexity band proficiently, with scaffolding as needed at the high end of the range."^^xsd:string .

:CCSS.ELA-Literacy.RI.3.1 rdf:type owl:Class ;
    prov:wasQuotedFrom <http://www.corestandards.org/ELA-Literacy/RI/3/1/> ;
    rdfs:subClassOf :CCSS.ELA-Literacy.RI.3 ;
    rdfs:comment "Ask and answer questions to demonstrate understanding of a text, referring explicitly to the text as the basis for the answers."^^xsd:string .

:CCSS.ELA-Literacy.RI.3.2 rdf:type owl:Class ;
    prov:wasQuotedFrom <http://www.corestandards.org/ELA-Literacy/RI/3/2/> ;
    rdfs:subClassOf :CCSS.ELA-Literacy.RI.3 ;
    rdfs:comment "Determine the main idea of a text; recount the key details and explain how they support the main idea."^^xsd:string .

:CCSS.ELA-Literacy.RI.3.3 rdf:type owl:Class ;
    prov:wasQuotedFrom <http://www.corestandards.org/ELA-Literacy/RI/3/3/> ;
    rdfs:subClassOf :CCSS.ELA-Literacy.RI.3 ;
    rdfs:comment "Describe the relationship between a series of historical events, scientific ideas or concepts, or steps in technical procedures in a text, using language that pertains to time, sequence, and cause/effect."^^xsd:string .

:CCSS.ELA-Literacy.RI.3.4 rdf:type owl:Class ;
    prov:wasQuotedFrom <http://www.corestandards.org/ELA-Literacy/RI/3/4/> ;
    rdfs:subClassOf :CCSS.ELA-Literacy.RI.3 ;
    rdfs:comment "Determine the meaning of general academic and domain-specific words and phrases in a text relevant to a grade 3 topic or subject area."^^xsd:string .

:CCSS.ELA-Literacy.RI.3.5 rdf:type owl:Class ;
    prov:wasQuotedFrom <http://www.corestandards.org/ELA-Literacy/RI/3/5/> ;
    rdfs:subClassOf :CCSS.ELA-Literacy.RI.3 ;
    rdfs:comment "Use text features and search tools (e.g., key words, sidebars, hyperlinks) to locate information relevant to a given topic efficiently."^^xsd:string .

:CCSS.ELA-Literacy.RI.3.6 rdf:type owl:Class ;
    prov:wasQuotedFrom <http://www.corestandards.org/ELA-Literacy/RI/3/6/> ;
    rdfs:subClassOf :CCSS.ELA-Literacy.RI.3 ;
    rdfs:comment "Distinguish their own point of view from that of the author of a text."^^xsd:string .

:CCSS.ELA-Literacy.RI.3.7 rdf:type owl:Class ;
    prov:wasQuotedFrom <http://www.corestandards.org/ELA-Literacy/RI/3/7/> ;
    rdfs:subClassOf :CCSS.ELA-Literacy.RI.3 ;
    rdfs:comment "Use information gained from illustrations (e.g., maps, photographs) and the words in a text to demonstrate understanding of the text (e.g., where, when, why, and how key events occur)."^^xsd:string .

:CCSS.ELA-Literacy.RI.3.8 rdf:type owl:Class ;
    prov:wasQuotedFrom <http://www.corestandards.org/ELA-Literacy/RI/3/8/> ;
    rdfs:subClassOf :CCSS.ELA-Literacy.RI.3 ;
    rdfs:comment "Describe the logical connection between particular sentences and paragraphs in a text (e.g., comparison, cause/effect, first/second/third in a sequence)."^^xsd:string .

:CCSS.ELA-Literacy.RI.3.9 rdf:type owl:Class ;
    prov:wasQuotedFrom <http://www.corestandards.org/ELA-Literacy/RI/3/9/> ;
    rdfs:subClassOf :CCSS.ELA-Literacy.RI.3 ;
    rdfs:comment "Compare and contrast the most important points and key details presented in two texts on the same topic."^^xsd:string .

:CCSS.ELA-Literacy.RI.3.10 rdf:type owl:Class ;
    prov:wasQuotedFrom <http://www.corestandards.org/ELA-Literacy/RI/3/10/> ;
    rdfs:subClassOf :CCSS.ELA-Literacy.RI.3 ;
    rdfs:comment "By the end of the year, read and comprehend informational texts, including history/social studies, science, and technical texts, at the high end of the grades 2-3 text complexity band independently and proficiently."^^xsd:string .

:CCSS.ELA-Literacy.RI.4.1 rdf:type owl:Class ;
    prov:wasQuotedFrom <http://www.corestandards.org/ELA-Literacy/RI/4/1/> ;
    rdfs:subClassOf :CCSS.ELA-Literacy.RI.4 ;
    rdfs:comment "Refer to details and examples in a text when explaining what the text says explicitly and when drawing inferences from the text."^^xsd:string .

:CCSS.ELA-Literacy.RI.4.2 rdf:type owl:Class ;
    prov:wasQuotedFrom <http://www.corestandards.org/ELA-Literacy/RI/4/2/> ;
    rdfs:subClassOf :CCSS.ELA-Literacy.RI.4 ;
    rdfs:comment "Determine the main idea of a text and explain how it is supported by key details; summarize the text."^^xsd:string .

:CCSS.ELA-Literacy.RI.4.3 rdf:type owl:Class ;
    prov:wasQuotedFrom <http://www.corestandards.org/ELA-Literacy/RI/4/3/> ;
    rdfs:subClassOf :CCSS.ELA-Literacy.RI.4 ;
    rdfs:comment "Explain events, procedures, ideas, or concepts in a historical, scientific, or technical text, including what happened and why, based on specific information in the text."^^xsd:string .

:CCSS.ELA-Literacy.RI.4.4 rdf:type owl:Class ;
    prov:wasQuotedFrom <http://www.corestandards.org/ELA-Literacy/RI/4/4/> ;
    rdfs:subClassOf :CCSS.ELA-Literacy.RI.4 ;
    rdfs:comment "Determine the meaning of general academic and domain-specific words or phrases in a text relevant to a grade 4 topic or subject area."^^xsd:string .

:CCSS.ELA-Literacy.RI.4.5 rdf:type owl:Class ;
    prov:wasQuotedFrom <http://www.corestandards.org/ELA-Literacy/RI/4/5/> ;
    rdfs:subClassOf :CCSS.ELA-Literacy.RI.4 ;
    rdfs:comment "Describe the overall structure (e.g., chronology, comparison, cause/effect, problem/solution) of events, ideas, concepts, or information in a text or part of a text."^^xsd:string .

:CCSS.ELA-Literacy.RI.4.6 rdf:type owl:Class ;
    prov:wasQuotedFrom <http://www.corestandards.org/ELA-Literacy/RI/4/6/> ;
    rdfs:subClassOf :CCSS.ELA-Literacy.RI.4 ;
    rdfs:comment "Compare and contrast a firsthand and secondhand account of the same event or topic; describe the differences in focus and the information provided."^^xsd:string .

:CCSS.ELA-Literacy.RI.4.7 rdf:type owl:Class ;
    prov:wasQuotedFrom <http://www.corestandards.org/ELA-Literacy/RI/4/7/> ;
    rdfs:subClassOf :CCSS.ELA-Literacy.RI.4 ;
    rdfs:comment "Interpret information presented visually, orally, or quantitatively (e.g., in charts, graphs, diagrams, time lines, animations, or interactive elements on Web pages) and explain how the information contributes to an understanding of the text in which it appears."^^xsd:string .

:CCSS.ELA-Literacy.RI.4.8 rdf:type owl:Class ;
    prov:wasQuotedFrom <http://www.corestandards.org/ELA-Literacy/RI/4/8/> ;
    rdfs:subClassOf :CCSS.ELA-Literacy.RI.4 ;
    rdfs:comment "Explain how an author uses reasons and evidence to support particular points in a text."^^xsd:string .

:CCSS.ELA-Literacy.RI.4.9 rdf:type owl:Class ;
    prov:wasQuotedFrom <http://www.corestandards.org/ELA-Literacy/RI/4/9/> ;
    rdfs:subClassOf :CCSS.ELA-Literacy.RI.4 ;
    rdfs:comment "Integrate information from two texts on the same topic in order to write or speak about the subject knowledgeably."^^xsd:string .

:CCSS.ELA-Literacy.RI.4.10 rdf:type owl:Class ;
    prov:wasQuotedFrom <http://www.corestandards.org/ELA-Literacy/RI/4/10/> ;
    rdfs:subClassOf :CCSS.ELA-Literacy.RI.4 ;
    rdfs:comment "By the end of year, read and comprehend informational texts, including history/social studies, science, and technical texts, in the grades 4-5 text complexity band proficiently, with scaffolding as needed at the high end of the range."^^xsd:string .

:CCSS.ELA-Literacy.RI.5.1 rdf:type owl:Class ;
    prov:wasQuotedFrom <http://www.corestandards.org/ELA-Literacy/RI/5/1/> ;
    rdfs:subClassOf :CCSS.ELA-Literacy.RI.5 ;
    rdfs:comment "Quote accurately from a text when explaining what the text says explicitly and when drawing inferences from the text."^^xsd:string .

:CCSS.ELA-Literacy.RI.5.2 rdf:type owl:Class ;
    prov:wasQuotedFrom <http://www.corestandards.org/ELA-Literacy/RI/5/2/> ;
    rdfs:subClassOf :CCSS.ELA-Literacy.RI.5 ;
    rdfs:comment "Determine two or more main ideas of a text and explain how they are supported by key details; summarize the text."^^xsd:string .

:CCSS.ELA-Literacy.RI.5.3 rdf:type owl:Class ;
    prov:wasQuotedFrom <http://www.corestandards.org/ELA-Literacy/RI/5/3/> ;
    rdfs:subClassOf :CCSS.ELA-Literacy.RI.5 ;
    rdfs:comment "Explain the relationships or interactions between two or more individuals, events, ideas, or concepts in a historical, scientific, or technical text based on specific information in the text."^^xsd:string .

:CCSS.ELA-Literacy.RI.5.4 rdf:type owl:Class ;
    prov:wasQuotedFrom <http://www.corestandards.org/ELA-Literacy/RI/5/4/> ;
    rdfs:subClassOf :CCSS.ELA-Literacy.RI.5 ;
    rdfs:comment "Determine the meaning of general academic and domain-specific words and phrases in a text relevant to a grade 5 topic or subject area."^^xsd:string .

:CCSS.ELA-Literacy.RI.5.5 rdf:type owl:Class ;
    prov:wasQuotedFrom <http://www.corestandards.org/ELA-Literacy/RI/5/5/> ;
    rdfs:subClassOf :CCSS.ELA-Literacy.RI.5 ;
    rdfs:comment "Compare and contrast the overall structure (e.g., chronology, comparison, cause/effect, problem/solution) of events, ideas, concepts, or information in two or more texts."^^xsd:string .

:CCSS.ELA-Literacy.RI.5.6 rdf:type owl:Class ;
    prov:wasQuotedFrom <http://www.corestandards.org/ELA-Literacy/RI/5/6/> ;
    rdfs:subClassOf :CCSS.ELA-Literacy.RI.5 ;
    rdfs:comment "Analyze multiple accounts of the same event or topic, noting important similarities and differences in the point of view they represent."^^xsd:string .

:CCSS.ELA-Literacy.RI.5.7 rdf:type owl:Class ;
    prov:wasQuotedFrom <http://www.corestandards.org/ELA-Literacy/RI/5/7/> ;
    rdfs:subClassOf :CCSS.ELA-Literacy.RI.5 ;
    rdfs:comment "Draw on information from multiple print or digital sources, demonstrating the ability to locate an answer to a question quickly or to solve a problem efficiently."^^xsd:string .

:CCSS.ELA-Literacy.RI.5.8 rdf:type owl:Class ;
    prov:wasQuotedFrom <http://www.corestandards.org/ELA-Literacy/RI/5/8/> ;
    rdfs:subClassOf :CCSS.ELA-Literacy.RI.5 ;
    rdfs:comment "Explain how an author uses reasons and evidence to support particular points in a text, identifying which reasons and evidence support which point(s)."^^xsd:string .

:CCSS.ELA-Literacy.RI.5.9 rdf:type owl:Class ;
    prov:wasQuotedFrom <http://www.corestandards.org/ELA-Literacy/RI/5/9/> ;
    rdfs:subClassOf :CCSS.ELA-Literacy.RI.5 ;
    rdfs:comment "Integrate information from several texts on the same topic in order to write or speak about the subject knowledgeably."^^xsd:string .

:CCSS.ELA-Literacy.RI.5.10 rdf:type owl:Class ;
    prov:wasQuotedFrom <http://www.corestandards.org/ELA-Literacy/RI/5/10/> ;
    rdfs:subClassOf :CCSS.ELA-Literacy.RI.5 ;
    rdfs:comment "By the end of the year, read and comprehend informational texts, including history/social studies, science, and technical texts, at the high end of the grades 4-5 text complexity band independently and proficiently."^^xsd:string .

:CCSS.ELA-Literacy.RI.6.1 rdf:type owl:Class ;
    prov:wasQuotedFrom <http://www.corestandards.org/ELA-Literacy/RI/6/1/> ;
    rdfs:subClassOf :CCSS.ELA-Literacy.RI.6 ;
    rdfs:comment "Cite textual evidence to support analysis of what the text says explicitly as well as inferences drawn from the text."^^xsd:string .

:CCSS.ELA-Literacy.RI.6.2 rdf:type owl:Class ;
    prov:wasQuotedFrom <http://www.corestandards.org/ELA-Literacy/RI/6/2/> ;
    rdfs:subClassOf :CCSS.ELA-Literacy.RI.6 ;
    rdfs:comment "Determine a central idea of a text and how it is conveyed through particular details; provide a summary of the text distinct from personal opinions or judgments."^^xsd:string .

:CCSS.ELA-Literacy.RI.6.3 rdf:type owl:Class ;
    prov:wasQuotedFrom <http://www.corestandards.org/ELA-Literacy/RI/6/3/> ;
    rdfs:subClassOf :CCSS.ELA-Literacy.RI.6 ;
    rdfs:comment "Analyze in detail how a key individual, event, or idea is introduced, illustrated, and elaborated in a text (e.g., through examples or anecdotes)."^^xsd:string .

:CCSS.ELA-Literacy.RI.6.4 rdf:type owl:Class ;
    prov:wasQuotedFrom <http://www.corestandards.org/ELA-Literacy/RI/6/4/> ;
    rdfs:subClassOf :CCSS.ELA-Literacy.RI.6 ;
    rdfs:comment "Determine the meaning of words and phrases as they are used in a text, including figurative, connotative, and technical meanings."^^xsd:string .

:CCSS.ELA-Literacy.RI.6.5 rdf:type owl:Class ;
    prov:wasQuotedFrom <http://www.corestandards.org/ELA-Literacy/RI/6/5/> ;
    rdfs:subClassOf :CCSS.ELA-Literacy.RI.6 ;
    rdfs:comment "Analyze how a particular sentence, paragraph, chapter, or section fits into the overall structure of a text and contributes to the development of the ideas."^^xsd:string .

:CCSS.ELA-Literacy.RI.6.6 rdf:type owl:Class ;
    prov:wasQuotedFrom <http://www.corestandards.org/ELA-Literacy/RI/6/6/> ;
    rdfs:subClassOf :CCSS.ELA-Literacy.RI.6 ;
    rdfs:comment "Determine an author's point of view or purpose in a text and explain how it is conveyed in the text."^^xsd:string .

:CCSS.ELA-Literacy.RI.6.7 rdf:type owl:Class ;
    prov:wasQuotedFrom <http://www.corestandards.org/ELA-Literacy/RI/6/7/> ;
    rdfs:subClassOf :CCSS.ELA-Literacy.RI.6 ;
    rdfs:comment "Integrate information presented in different media or formats (e.g., visually, quantitatively) as well as in words to develop a coherent understanding of a topic or issue."^^xsd:string .

:CCSS.ELA-Literacy.RI.6.8 rdf:type owl:Class ;
    prov:wasQuotedFrom <http://www.corestandards.org/ELA-Literacy/RI/6/8/> ;
    rdfs:subClassOf :CCSS.ELA-Literacy.RI.6 ;
    rdfs:comment "Trace and evaluate the argument and specific claims in a text, distinguishing claims that are supported by reasons and evidence from claims that are not."^^xsd:string .

:CCSS.ELA-Literacy.RI.6.9 rdf:type owl:Class ;
    prov:wasQuotedFrom <http://www.corestandards.org/ELA-Literacy/RI/6/9/> ;
    rdfs:subClassOf :CCSS.ELA-Literacy.RI.6 ;
    rdfs:comment "Compare and contrast one author's presentation of events with that of another (e.g., a memoir written by and a biography on the same person)."^^xsd:string .

:CCSS.ELA-Literacy.RI.6.10 rdf:type owl:Class ;
    prov:wasQuotedFrom <http://www.corestandards.org/ELA-Literacy/RI/6/10/> ;
    rdfs:subClassOf :CCSS.ELA-Literacy.RI.6 ;
    rdfs:comment "By the end of the year, read and comprehend literary nonfiction in the grades 6-8 text complexity band proficiently, with scaffolding as needed at the high end of the range."^^xsd:string .

:CCSS.ELA-Literacy.RI.7.1 rdf:type owl:Class ;
    prov:wasQuotedFrom <http://www.corestandards.org/ELA-Literacy/RI/7/1/> ;
    rdfs:subClassOf :CCSS.ELA-Literacy.RI.7 ;
    rdfs:comment "Cite several pieces of textual evidence to support analysis of what the text says explicitly as well as inferences drawn from the text."^^xsd:string .

:CCSS.ELA-Literacy.RI.7.2 rdf:type owl:Class ;
    prov:wasQuotedFrom <http://www.corestandards.org/ELA-Literacy/RI/7/2/> ;
    rdfs:subClassOf :CCSS.ELA-Literacy.RI.7 ;
    rdfs:comment "Determine two or more central ideas in a text and analyze their development over the course of the text; provide an objective summary of the text."^^xsd:string .

:CCSS.ELA-Literacy.RI.7.3 rdf:type owl:Class ;
    prov:wasQuotedFrom <http://www.corestandards.org/ELA-Literacy/RI/7/3/> ;
    rdfs:subClassOf :CCSS.ELA-Literacy.RI.7 ;
    rdfs:comment "Analyze the interactions between individuals, events, and ideas in a text (e.g., how ideas influence individuals or events, or how individuals influence ideas or events)."^^xsd:string .

:CCSS.ELA-Literacy.RI.7.4 rdf:type owl:Class ;
    prov:wasQuotedFrom <http://www.corestandards.org/ELA-Literacy/RI/7/4/> ;
    rdfs:subClassOf :CCSS.ELA-Literacy.RI.7 ;
    rdfs:comment "Determine the meaning of words and phrases as they are used in a text, including figurative, connotative, and technical meanings; analyze the impact of a specific word choice on meaning and tone."^^xsd:string .

:CCSS.ELA-Literacy.RI.7.5 rdf:type owl:Class ;
    prov:wasQuotedFrom <http://www.corestandards.org/ELA-Literacy/RI/7/5/> ;
    rdfs:subClassOf :CCSS.ELA-Literacy.RI.7 ;
    rdfs:comment "Analyze the structure an author uses to organize a text, including how the major sections contribute to the whole and to the development of the ideas."^^xsd:string .

:CCSS.ELA-Literacy.RI.7.6 rdf:type owl:Class ;
    prov:wasQuotedFrom <http://www.corestandards.org/ELA-Literacy/RI/7/6/> ;
    rdfs:subClassOf :CCSS.ELA-Literacy.RI.7 ;
    rdfs:comment "Determine an author's point of view or purpose in a text and analyze how the author distinguishes his or her position from that of others."^^xsd:string .

:CCSS.ELA-Literacy.RI.7.7 rdf:type owl:Class ;
    prov:wasQuotedFrom <http://www.corestandards.org/ELA-Literacy/RI/7/7/> ;
    rdfs:subClassOf :CCSS.ELA-Literacy.RI.7 ;
    rdfs:comment "Compare and contrast a text to an audio, video, or multimedia version of the text, analyzing each medium's portrayal of the subject (e.g., how the delivery of a speech affects the impact of the words)."^^xsd:string .

:CCSS.ELA-Literacy.RI.7.8 rdf:type owl:Class ;
    prov:wasQuotedFrom <http://www.corestandards.org/ELA-Literacy/RI/7/8/> ;
    rdfs:subClassOf :CCSS.ELA-Literacy.RI.7 ;
    rdfs:comment "Trace and evaluate the argument and specific claims in a text, assessing whether the reasoning is sound and the evidence is relevant and sufficient to support the claims."^^xsd:string .

:CCSS.ELA-Literacy.RI.7.9 rdf:type owl:Class ;
    prov:wasQuotedFrom <http://www.corestandards.org/ELA-Literacy/RI/7/9/> ;
    rdfs:subClassOf :CCSS.ELA-Literacy.RI.7 ;
    rdfs:comment "Analyze how two or more authors writing about the same topic shape their presentations of key information by emphasizing different evidence or advancing different interpretations of facts."^^xsd:string .

:CCSS.ELA-Literacy.RI.7.10 rdf:type owl:Class ;
    prov:wasQuotedFrom <http://www.corestandards.org/ELA-Literacy/RI/7/10/> ;
    rdfs:subClassOf :CCSS.ELA-Literacy.RI.7 ;
    rdfs:comment "By the end of the year, read and comprehend literary nonfiction in the grades 6-8 text complexity band proficiently, with scaffolding as needed at the high end of the range."^^xsd:string .

:CCSS.ELA-Literacy.RI.8.1 rdf:type owl:Class ;
    prov:wasQuotedFrom <http://www.corestandards.org/ELA-Literacy/RI/8/1/> ;
    rdfs:subClassOf :CCSS.ELA-Literacy.RI.8 ;
    rdfs:comment "Cite the textual evidence that most strongly supports an analysis of what the text says explicitly as well as inferences drawn from the text."^^xsd:string .

:CCSS.ELA-Literacy.RI.8.2 rdf:type owl:Class ;
    prov:wasQuotedFrom <http://www.corestandards.org/ELA-Literacy/RI/8/2/> ;
    rdfs:subClassOf :CCSS.ELA-Literacy.RI.8 ;
    rdfs:comment "Determine a central idea of a text and analyze its development over the course of the text, including its relationship to supporting ideas; provide an objective summary of the text."^^xsd:string .

:CCSS.ELA-Literacy.RI.8.3 rdf:type owl:Class ;
    prov:wasQuotedFrom <http://www.corestandards.org/ELA-Literacy/RI/8/3/> ;
    rdfs:subClassOf :CCSS.ELA-Literacy.RI.8 ;
    rdfs:comment "Analyze how a text makes connections among and distinctions between individuals, ideas, or events (e.g., through comparisons, analogies, or categories)."^^xsd:string .

:CCSS.ELA-Literacy.RI.8.4 rdf:type owl:Class ;
    prov:wasQuotedFrom <http://www.corestandards.org/ELA-Literacy/RI/8/4/> ;
    rdfs:subClassOf :CCSS.ELA-Literacy.RI.8 ;
    rdfs:comment "Determine the meaning of words and phrases as they are used in a text, including figurative, connotative, and technical meanings; analyze the impact of specific word choices on meaning and tone, including analogies or allusions to other texts."^^xsd:string .

:CCSS.ELA-Literacy.RI.8.5 rdf:type owl:Class ;
    prov:wasQuotedFrom <http://www.corestandards.org/ELA-Literacy/RI/8/5/> ;
    rdfs:subClassOf :CCSS.ELA-Literacy.RI.8 ;
    rdfs:comment "Analyze in detail the structure of a specific paragraph in a text, including the role of particular sentences in developing and refining a key concept."^^xsd:string .

:CCSS.ELA-Literacy.RI.8.6 rdf:type owl:Class ;
    prov:wasQuotedFrom <http://www.corestandards.org/ELA-Literacy/RI/8/6/> ;
    rdfs:subClassOf :CCSS.ELA-Literacy.RI.8 ;
    rdfs:comment "Determine an author's point of view or purpose in a text and analyze how the author acknowledges and responds to conflicting evidence or viewpoints. "^^xsd:string .

:CCSS.ELA-Literacy.RI.8.7 rdf:type owl:Class ;
    prov:wasQuotedFrom <http://www.corestandards.org/ELA-Literacy/RI/8/7/> ;
    rdfs:subClassOf :CCSS.ELA-Literacy.RI.8 ;
    rdfs:comment "Evaluate the advantages and disadvantages of using different mediums (e.g., print or digital text, video, multimedia) to present a particular topic or idea."^^xsd:string .

:CCSS.ELA-Literacy.RI.8.8 rdf:type owl:Class ;
    prov:wasQuotedFrom <http://www.corestandards.org/ELA-Literacy/RI/8/8/> ;
    rdfs:subClassOf :CCSS.ELA-Literacy.RI.8 ;
    rdfs:comment "Delineate and evaluate the argument and specific claims in a text, assessing whether the reasoning is sound and the evidence is relevant and sufficient; recognize when irrelevant evidence is introduced."^^xsd:string .

:CCSS.ELA-Literacy.RI.8.9 rdf:type owl:Class ;
    prov:wasQuotedFrom <http://www.corestandards.org/ELA-Literacy/RI/8/9/> ;
    rdfs:subClassOf :CCSS.ELA-Literacy.RI.8 ;
    rdfs:comment "Analyze a case in which two or more texts provide conflicting information on the same topic and identify where the texts disagree on matters of fact or interpretation."^^xsd:string .

:CCSS.ELA-Literacy.RI.8.10 rdf:type owl:Class ;
    prov:wasQuotedFrom <http://www.corestandards.org/ELA-Literacy/RI/8/10/> ;
    rdfs:subClassOf :CCSS.ELA-Literacy.RI.8 ;
    rdfs:comment "By the end of the year, read and comprehend literary nonfiction at the high end of the grades 6-8 text complexity band independently and proficiently."^^xsd:string .

:CCSS.ELA-Literacy.RI.9-10.1 rdf:type owl:Class ;
    prov:wasQuotedFrom <http://www.corestandards.org/ELA-Literacy/RI/9-10/1/> ;
    rdfs:subClassOf :CCSS.ELA-Literacy.RI.9-10 ;
    rdfs:comment "Cite strong and thorough textual evidence to support analysis of what the text says explicitly as well as inferences drawn from the text."^^xsd:string .

:CCSS.ELA-Literacy.RI.9-10.2 rdf:type owl:Class ;
    prov:wasQuotedFrom <http://www.corestandards.org/ELA-Literacy/RI/9-10/2/> ;
    rdfs:subClassOf :CCSS.ELA-Literacy.RI.9-10 ;
    rdfs:comment "Determine a central idea of a text and analyze its development over the course of the text, including how it emerges and is shaped and refined by specific details; provide an objective summary of the text."^^xsd:string .

:CCSS.ELA-Literacy.RI.9-10.3 rdf:type owl:Class ;
    prov:wasQuotedFrom <http://www.corestandards.org/ELA-Literacy/RI/9-10/3/> ;
    rdfs:subClassOf :CCSS.ELA-Literacy.RI.9-10 ;
    rdfs:comment "Analyze how the author unfolds an analysis or series of ideas or events, including the order in which the points are made, how they are introduced and developed, and the connections that are drawn between them."^^xsd:string .

:CCSS.ELA-Literacy.RI.9-10.4 rdf:type owl:Class ;
    prov:wasQuotedFrom <http://www.corestandards.org/ELA-Literacy/RI/9-10/4/> ;
    rdfs:subClassOf :CCSS.ELA-Literacy.RI.9-10 ;
    rdfs:comment "Determine the meaning of words and phrases as they are used in a text, including figurative, connotative, and technical meanings; analyze the cumulative impact of specific word choices on meaning and tone (e.g., how the language of a court opinion differs from that of a newspaper)."^^xsd:string .

:CCSS.ELA-Literacy.RI.9-10.5 rdf:type owl:Class ;
    prov:wasQuotedFrom <http://www.corestandards.org/ELA-Literacy/RI/9-10/5/> ;
    rdfs:subClassOf :CCSS.ELA-Literacy.RI.9-10 ;
    rdfs:comment "Analyze in detail how an author's ideas or claims are developed and refined by particular sentences, paragraphs, or larger portions of a text (e.g., a section or chapter)."^^xsd:string .

:CCSS.ELA-Literacy.RI.9-10.6 rdf:type owl:Class ;
    prov:wasQuotedFrom <http://www.corestandards.org/ELA-Literacy/RI/9-10/6/> ;
    rdfs:subClassOf :CCSS.ELA-Literacy.RI.9-10 ;
    rdfs:comment "Determine an author's point of view or purpose in a text and analyze how an author uses rhetoric to advance that point of view or purpose."^^xsd:string .

:CCSS.ELA-Literacy.RI.9-10.7 rdf:type owl:Class ;
    prov:wasQuotedFrom <http://www.corestandards.org/ELA-Literacy/RI/9-10/7/> ;
    rdfs:subClassOf :CCSS.ELA-Literacy.RI.9-10 ;
    rdfs:comment "Analyze various accounts of a subject told in different mediums (e.g., a person's life story in both print and multimedia), determining which details are emphasized in each account."^^xsd:string .

:CCSS.ELA-Literacy.RI.9-10.8 rdf:type owl:Class ;
    prov:wasQuotedFrom <http://www.corestandards.org/ELA-Literacy/RI/9-10/8/> ;
    rdfs:subClassOf :CCSS.ELA-Literacy.RI.9-10 ;
    rdfs:comment "Delineate and evaluate the argument and specific claims in a text, assessing whether the reasoning is valid and the evidence is relevant and sufficient; identify false statements and fallacious reasoning."^^xsd:string .

:CCSS.ELA-Literacy.RI.9-10.9 rdf:type owl:Class ;
    prov:wasQuotedFrom <http://www.corestandards.org/ELA-Literacy/RI/9-10/9/> ;
    rdfs:subClassOf :CCSS.ELA-Literacy.RI.9-10 ;
    rdfs:comment "Analyze seminal U.S. documents of historical and literary significance (e.g., Washington's Farewell Address, the Gettysburg Address, Roosevelt's Four Freedoms speech, King's 'Letter from Birmingham Jail'), including how they address related themes and concepts."^^xsd:string .

:CCSS.ELA-Literacy.RI.9-10.10 rdf:type owl:Class ;
    prov:wasQuotedFrom <http://www.corestandards.org/ELA-Literacy/RI/9-10/10/> ;
    rdfs:subClassOf :CCSS.ELA-Literacy.RI.9-10 ;
    rdfs:comment "By the end of grade 9, read and comprehend literary nonfiction in the grades 9-10 text complexity band proficiently, with scaffolding as needed at the high end of the range.

By the end of grade 10, read and comprehend literary nonfiction at the high end of the grades 9-10 text complexity band independently and proficiently."^^xsd:string .

:CCSS.ELA-Literacy.RI.11-12.1 rdf:type owl:Class ;
    prov:wasQuotedFrom <http://www.corestandards.org/ELA-Literacy/RI/11-12/1/> ;
    rdfs:subClassOf :CCSS.ELA-Literacy.RI.11-12 ;
    rdfs:comment "Cite strong and thorough textual evidence to support analysis of what the text says explicitly as well as inferences drawn from the text, including determining where the text leaves matters uncertain."^^xsd:string .

:CCSS.ELA-Literacy.RI.11-12.2 rdf:type owl:Class ;
    prov:wasQuotedFrom <http://www.corestandards.org/ELA-Literacy/RI/11-12/2/> ;
    rdfs:subClassOf :CCSS.ELA-Literacy.RI.11-12 ;
    rdfs:comment "Determine two or more central ideas of a text and analyze their development over the course of the text, including how they interact and build on one another to provide a complex analysis; provide an objective summary of the text."^^xsd:string .

:CCSS.ELA-Literacy.RI.11-12.3 rdf:type owl:Class ;
    prov:wasQuotedFrom <http://www.corestandards.org/ELA-Literacy/RI/11-12/3/> ;
    rdfs:subClassOf :CCSS.ELA-Literacy.RI.11-12 ;
    rdfs:comment "Analyze a complex set of ideas or sequence of events and explain how specific individuals, ideas, or events interact and develop over the course of the text."^^xsd:string .

:CCSS.ELA-Literacy.RI.11-12.4 rdf:type owl:Class ;
    prov:wasQuotedFrom <http://www.corestandards.org/ELA-Literacy/RI/11-12/4/> ;
    rdfs:subClassOf :CCSS.ELA-Literacy.RI.11-12 ;
    rdfs:comment "Determine the meaning of words and phrases as they are used in a text, including figurative, connotative, and technical meanings; analyze how an author uses and refines the meaning of a key term or terms over the course of a text (e.g., how Madison defines faction in Federalist No. 10)."^^xsd:string .

:CCSS.ELA-Literacy.RI.11-12.5 rdf:type owl:Class ;
    prov:wasQuotedFrom <http://www.corestandards.org/ELA-Literacy/RI/11-12/5/> ;
    rdfs:subClassOf :CCSS.ELA-Literacy.RI.11-12 ;
    rdfs:comment "Analyze and evaluate the effectiveness of the structure an author uses in his or her exposition or argument, including whether the structure makes points clear, convincing, and engaging."^^xsd:string .

:CCSS.ELA-Literacy.RI.11-12.6 rdf:type owl:Class ;
    prov:wasQuotedFrom <http://www.corestandards.org/ELA-Literacy/RI/11-12/6/> ;
    rdfs:subClassOf :CCSS.ELA-Literacy.RI.11-12 ;
    rdfs:comment "Determine an author's point of view or purpose in a text in which the rhetoric is particularly effective, analyzing how style and content contribute to the power, persuasiveness or beauty of the text. "^^xsd:string .

:CCSS.ELA-Literacy.RI.11-12.7 rdf:type owl:Class ;
    prov:wasQuotedFrom <http://www.corestandards.org/ELA-Literacy/RI/11-12/7/> ;
    rdfs:subClassOf :CCSS.ELA-Literacy.RI.11-12 ;
    rdfs:comment "Integrate and evaluate multiple sources of information presented in different media or formats (e.g., visually, quantitatively) as well as in words in order to address a question or solve a problem."^^xsd:string .

:CCSS.ELA-Literacy.RI.11-12.8 rdf:type owl:Class ;
    prov:wasQuotedFrom <http://www.corestandards.org/ELA-Literacy/RI/11-12/8/> ;
    rdfs:subClassOf :CCSS.ELA-Literacy.RI.11-12 ;
    rdfs:comment "Delineate and evaluate the reasoning in seminal U.S. texts, including the application of constitutional principles and use of legal reasoning (e.g., in U.S. Supreme Court majority opinions and dissents) and the premises, purposes, and arguments in works of public advocacy (e.g., The Federalist, presidential addresses)."^^xsd:string .

:CCSS.ELA-Literacy.RI.11-12.9 rdf:type owl:Class ;
    prov:wasQuotedFrom <http://www.corestandards.org/ELA-Literacy/RI/11-12/9/> ;
    rdfs:subClassOf :CCSS.ELA-Literacy.RI.11-12 ;
    rdfs:comment "Analyze seventeenth-, eighteenth-, and nineteenth-century foundational U.S. documents of historical and literary significance (including The Declaration of Independence, the Preamble to the Constitution, the Bill of Rights, and Lincoln's Second Inaugural Address) for their themes, purposes, and rhetorical features."^^xsd:string .

:CCSS.ELA-Literacy.RI.11-12.10 rdf:type owl:Class ;
    prov:wasQuotedFrom <http://www.corestandards.org/ELA-Literacy/RI/11-12/10/> ;
    rdfs:subClassOf :CCSS.ELA-Literacy.RI.11-12 ;
    rdfs:comment "By the end of grade 11, read and comprehend literary nonfiction in the grades 11-CCR text complexity band proficiently, with scaffolding as needed at the high end of the range.
By the end of grade 12, read and comprehend literary nonfiction at the high end of the grades 11-CCR text complexity band independently and proficiently."^^xsd:string .

:CCSS.ELA-Literacy.RF.K.1 rdf:type owl:Class ;
    prov:wasQuotedFrom <http://www.corestandards.org/ELA-Literacy/RF/K/1/> ;
    rdfs:subClassOf :CCSS.ELA-Literacy.RF.K ;
    rdfs:comment "Demonstrate understanding of the organization and basic features of print."^^xsd:string .

:CCSS.ELA-Literacy.RF.K.1.a rdf:type owl:Class ;
    prov:wasQuotedFrom <http://www.corestandards.org/ELA-Literacy/RF/K/1/a/> ;
    rdfs:subClassOf :CCSS.ELA-Literacy.RF.K.1 ;
    rdfs:comment "Follow words from left to right, top to bottom, and page by page."^^xsd:string .

:CCSS.ELA-Literacy.RF.K.1.b rdf:type owl:Class ;
    prov:wasQuotedFrom <http://www.corestandards.org/ELA-Literacy/RF/K/1/b/> ;
    rdfs:subClassOf :CCSS.ELA-Literacy.RF.K.1 ;
    rdfs:comment "Recognize that spoken words are represented in written language by specific sequences of letters."^^xsd:string .

:CCSS.ELA-Literacy.RF.K.1.c rdf:type owl:Class ;
    prov:wasQuotedFrom <http://www.corestandards.org/ELA-Literacy/RF/K/1/c/> ;
    rdfs:subClassOf :CCSS.ELA-Literacy.RF.K.1 ;
    rdfs:comment "Understand that words are separated by spaces in print."^^xsd:string .

:CCSS.ELA-Literacy.RF.K.1.d rdf:type owl:Class ;
    prov:wasQuotedFrom <http://www.corestandards.org/ELA-Literacy/RF/K/1/d/> ;
    rdfs:subClassOf :CCSS.ELA-Literacy.RF.K.1 ;
    rdfs:comment "Recognize and name all upper- and lowercase letters of the alphabet."^^xsd:string .

:CCSS.ELA-Literacy.RF.K.2 rdf:type owl:Class ;
    prov:wasQuotedFrom <http://www.corestandards.org/ELA-Literacy/RF/K/2/> ;
    rdfs:subClassOf :CCSS.ELA-Literacy.RF.K ;
    rdfs:comment "Demonstrate understanding of spoken words, syllables, and sounds (phonemes)."^^xsd:string .

:CCSS.ELA-Literacy.RF.K.2.a rdf:type owl:Class ;
    prov:wasQuotedFrom <http://www.corestandards.org/ELA-Literacy/RF/K/2/a/> ;
    rdfs:subClassOf :CCSS.ELA-Literacy.RF.K.2 ;
    rdfs:comment "Recognize and produce rhyming words."^^xsd:string .

:CCSS.ELA-Literacy.RF.K.2.b rdf:type owl:Class ;
    prov:wasQuotedFrom <http://www.corestandards.org/ELA-Literacy/RF/K/2/b/> ;
    rdfs:subClassOf :CCSS.ELA-Literacy.RF.K.2 ;
    rdfs:comment "Count, pronounce, blend, and segment syllables in spoken words."^^xsd:string .

:CCSS.ELA-Literacy.RF.K.2.c rdf:type owl:Class ;
    prov:wasQuotedFrom <http://www.corestandards.org/ELA-Literacy/RF/K/2/c/> ;
    rdfs:subClassOf :CCSS.ELA-Literacy.RF.K.2 ;
    rdfs:comment "Blend and segment onsets and rimes of single-syllable spoken words."^^xsd:string .

:CCSS.ELA-Literacy.RF.K.2.d rdf:type owl:Class ;
    prov:wasQuotedFrom <http://www.corestandards.org/ELA-Literacy/RF/K/2/d/> ;
    rdfs:subClassOf :CCSS.ELA-Literacy.RF.K.2 ;
    rdfs:comment "Isolate and pronounce the initial, medial vowel, and final sounds (phonemes) in three-phoneme (consonant-vowel-consonant, or CVC) words.1 (This does not include CVCs ending with /l/, /r/, or /x/.)"^^xsd:string .

:CCSS.ELA-Literacy.RF.K.2.e rdf:type owl:Class ;
    prov:wasQuotedFrom <http://www.corestandards.org/ELA-Literacy/RF/K/2/e/> ;
    rdfs:subClassOf :CCSS.ELA-Literacy.RF.K.2 ;
    rdfs:comment "Add or substitute individual sounds (phonemes) in simple, one-syllable words to make new words."^^xsd:string .

:CCSS.ELA-Literacy.RF.K.3 rdf:type owl:Class ;
    prov:wasQuotedFrom <http://www.corestandards.org/ELA-Literacy/RF/K/3/> ;
    rdfs:subClassOf :CCSS.ELA-Literacy.RF.K ;
    rdfs:comment "Know and apply grade-level phonics and word analysis skills in decoding words."^^xsd:string .

:CCSS.ELA-Literacy.RF.K.3.a rdf:type owl:Class ;
    prov:wasQuotedFrom <http://www.corestandards.org/ELA-Literacy/RF/K/3/a/> ;
    rdfs:subClassOf :CCSS.ELA-Literacy.RF.K.3 ;
    rdfs:comment "Demonstrate basic knowledge of one-to-one letter-sound correspondences by producing the primary sound or many of the most frequent sounds for each consonant."^^xsd:string .

:CCSS.ELA-Literacy.RF.K.3.b rdf:type owl:Class ;
    prov:wasQuotedFrom <http://www.corestandards.org/ELA-Literacy/RF/K/3/b/> ;
    rdfs:subClassOf :CCSS.ELA-Literacy.RF.K.3 ;
    rdfs:comment "Associate the long and short sounds with the common spellings (graphemes) for the five major vowels.
"^^xsd:string .

:CCSS.ELA-Literacy.RF.K.3.c rdf:type owl:Class ;
    prov:wasQuotedFrom <http://www.corestandards.org/ELA-Literacy/RF/K/3/c/> ;
    rdfs:subClassOf :CCSS.ELA-Literacy.RF.K.3 ;
    rdfs:comment "Read common high-frequency words by sight (e.g., the, of, to, you, she, my, is, are, do, does)."^^xsd:string .

:CCSS.ELA-Literacy.RF.K.3.d rdf:type owl:Class ;
    prov:wasQuotedFrom <http://www.corestandards.org/ELA-Literacy/RF/K/3/d/> ;
    rdfs:subClassOf :CCSS.ELA-Literacy.RF.K.3 ;
    rdfs:comment "Distinguish between similarly spelled words by identifying the sounds of the letters that differ."^^xsd:string .

:CCSS.ELA-Literacy.RF.K.4 rdf:type owl:Class ;
    prov:wasQuotedFrom <http://www.corestandards.org/ELA-Literacy/RF/K/4/> ;
    rdfs:subClassOf :CCSS.ELA-Literacy.RF.K ;
    rdfs:comment "Read emergent-reader texts with purpose and understanding."^^xsd:string .

:CCSS.ELA-Literacy.RF.1.1 rdf:type owl:Class ;
    prov:wasQuotedFrom <http://www.corestandards.org/ELA-Literacy/RF/1/1/> ;
    rdfs:subClassOf :CCSS.ELA-Literacy.RF.1 ;
    rdfs:comment "Demonstrate understanding of the organization and basic features of print."^^xsd:string .

:CCSS.ELA-Literacy.RF.1.1.a rdf:type owl:Class ;
    prov:wasQuotedFrom <http://www.corestandards.org/ELA-Literacy/RF/1/1/a/> ;
    rdfs:subClassOf :CCSS.ELA-Literacy.RF.1.1 ;
    rdfs:comment "Recognize the distinguishing features of a sentence (e.g., first word, capitalization, ending punctuation)."^^xsd:string .

:CCSS.ELA-Literacy.RF.1.2 rdf:type owl:Class ;
    prov:wasQuotedFrom <http://www.corestandards.org/ELA-Literacy/RF/1/2/> ;
    rdfs:subClassOf :CCSS.ELA-Literacy.RF.1 ;
    rdfs:comment "Demonstrate understanding of spoken words, syllables, and sounds (phonemes)."^^xsd:string .

:CCSS.ELA-Literacy.RF.1.2.a rdf:type owl:Class ;
    prov:wasQuotedFrom <http://www.corestandards.org/ELA-Literacy/RF/1/2/a/> ;
    rdfs:subClassOf :CCSS.ELA-Literacy.RF.1.2 ;
    rdfs:comment "Distinguish long from short vowel sounds in spoken single-syllable words."^^xsd:string .

:CCSS.ELA-Literacy.RF.1.2.b rdf:type owl:Class ;
    prov:wasQuotedFrom <http://www.corestandards.org/ELA-Literacy/RF/1/2/b/> ;
    rdfs:subClassOf :CCSS.ELA-Literacy.RF.1.2 ;
    rdfs:comment "Orally produce single-syllable words by blending sounds (phonemes), including consonant blends."^^xsd:string .

:CCSS.ELA-Literacy.RF.1.2.c rdf:type owl:Class ;
    prov:wasQuotedFrom <http://www.corestandards.org/ELA-Literacy/RF/1/2/c/> ;
    rdfs:subClassOf :CCSS.ELA-Literacy.RF.1.2 ;
    rdfs:comment "Isolate and pronounce initial, medial vowel, and final sounds (phonemes) in spoken single-syllable words."^^xsd:string .

:CCSS.ELA-Literacy.RF.1.2.d rdf:type owl:Class ;
    prov:wasQuotedFrom <http://www.corestandards.org/ELA-Literacy/RF/1/2/d/> ;
    rdfs:subClassOf :CCSS.ELA-Literacy.RF.1.2 ;
    rdfs:comment "Segment spoken single-syllable words into their complete sequence of individual sounds (phonemes)."^^xsd:string .

:CCSS.ELA-Literacy.RF.1.3 rdf:type owl:Class ;
    prov:wasQuotedFrom <http://www.corestandards.org/ELA-Literacy/RF/1/3/> ;
    rdfs:subClassOf :CCSS.ELA-Literacy.RF.1 ;
    rdfs:comment "Know and apply grade-level phonics and word analysis skills in decoding words."^^xsd:string .

:CCSS.ELA-Literacy.RF.1.3.a rdf:type owl:Class ;
    prov:wasQuotedFrom <http://www.corestandards.org/ELA-Literacy/RF/1/3/a/> ;
    rdfs:subClassOf :CCSS.ELA-Literacy.RF.1.3 ;
    rdfs:comment "Know the spelling-sound correspondences for common consonant digraphs."^^xsd:string .

:CCSS.ELA-Literacy.RF.1.3.b rdf:type owl:Class ;
    prov:wasQuotedFrom <http://www.corestandards.org/ELA-Literacy/RF/1/3/b/> ;
    rdfs:subClassOf :CCSS.ELA-Literacy.RF.1.3 ;
    rdfs:comment "Decode regularly spelled one-syllable words."^^xsd:string .

:CCSS.ELA-Literacy.RF.1.3.c rdf:type owl:Class ;
    prov:wasQuotedFrom <http://www.corestandards.org/ELA-Literacy/RF/1/3/c/> ;
    rdfs:subClassOf :CCSS.ELA-Literacy.RF.1.3 ;
    rdfs:comment "Know final -e and common vowel team conventions for representing long vowel sounds."^^xsd:string .

:CCSS.ELA-Literacy.RF.1.3.d rdf:type owl:Class ;
    prov:wasQuotedFrom <http://www.corestandards.org/ELA-Literacy/RF/1/3/d/> ;
    rdfs:subClassOf :CCSS.ELA-Literacy.RF.1.3 ;
    rdfs:comment "Use knowledge that every syllable must have a vowel sound to determine the number of syllables in a printed word."^^xsd:string .

:CCSS.ELA-Literacy.RF.1.3.e rdf:type owl:Class ;
    prov:wasQuotedFrom <http://www.corestandards.org/ELA-Literacy/RF/1/3/e/> ;
    rdfs:subClassOf :CCSS.ELA-Literacy.RF.1.3 ;
    rdfs:comment "Decode two-syllable words following basic patterns by breaking the words into syllables."^^xsd:string .

:CCSS.ELA-Literacy.RF.1.3.f rdf:type owl:Class ;
    prov:wasQuotedFrom <http://www.corestandards.org/ELA-Literacy/RF/1/3/f/> ;
    rdfs:subClassOf :CCSS.ELA-Literacy.RF.1.3 ;
    rdfs:comment "Read words with inflectional endings."^^xsd:string .

:CCSS.ELA-Literacy.RF.1.3.g rdf:type owl:Class ;
    prov:wasQuotedFrom <http://www.corestandards.org/ELA-Literacy/RF/1/3/g/> ;
    rdfs:subClassOf :CCSS.ELA-Literacy.RF.1.3 ;
    rdfs:comment "Recognize and read grade-appropriate irregularly spelled words."^^xsd:string .

:CCSS.ELA-Literacy.RF.1.4 rdf:type owl:Class ;
    prov:wasQuotedFrom <http://www.corestandards.org/ELA-Literacy/RF/1/4/> ;
    rdfs:subClassOf :CCSS.ELA-Literacy.RF.1 ;
    rdfs:comment "Read with sufficient accuracy and fluency to support comprehension."^^xsd:string .

:CCSS.ELA-Literacy.RF.1.4.a rdf:type owl:Class ;
    prov:wasQuotedFrom <http://www.corestandards.org/ELA-Literacy/RF/1/4/a/> ;
    rdfs:subClassOf :CCSS.ELA-Literacy.RF.1.4 ;
    rdfs:comment "Read grade-level text with purpose and understanding."^^xsd:string .

:CCSS.ELA-Literacy.RF.1.4.b rdf:type owl:Class ;
    prov:wasQuotedFrom <http://www.corestandards.org/ELA-Literacy/RF/1/4/b/> ;
    rdfs:subClassOf :CCSS.ELA-Literacy.RF.1.4 ;
    rdfs:comment "Read grade-level text orally with accuracy, appropriate rate, and expression on successive readings."^^xsd:string .

:CCSS.ELA-Literacy.RF.1.4.c rdf:type owl:Class ;
    prov:wasQuotedFrom <http://www.corestandards.org/ELA-Literacy/RF/1/4/c/> ;
    rdfs:subClassOf :CCSS.ELA-Literacy.RF.1.4 ;
    rdfs:comment "Use context to confirm or self-correct word recognition and understanding, rereading as necessary."^^xsd:string .

:CCSS.ELA-Literacy.RF.2.3 rdf:type owl:Class ;
    prov:wasQuotedFrom <http://www.corestandards.org/ELA-Literacy/RF/2/3/> ;
    rdfs:subClassOf :CCSS.ELA-Literacy.RF.2 ;
    rdfs:comment "Know and apply grade-level phonics and word analysis skills in decoding words."^^xsd:string .

:CCSS.ELA-Literacy.RF.2.3.a rdf:type owl:Class ;
    prov:wasQuotedFrom <http://www.corestandards.org/ELA-Literacy/RF/2/3/a/> ;
    rdfs:subClassOf :CCSS.ELA-Literacy.RF.2.3 ;
    rdfs:comment "Distinguish long and short vowels when reading regularly spelled one-syllable words."^^xsd:string .

:CCSS.ELA-Literacy.RF.2.3.b rdf:type owl:Class ;
    prov:wasQuotedFrom <http://www.corestandards.org/ELA-Literacy/RF/2/3/b/> ;
    rdfs:subClassOf :CCSS.ELA-Literacy.RF.2.3 ;
    rdfs:comment "Know spelling-sound correspondences for additional common vowel teams."^^xsd:string .

:CCSS.ELA-Literacy.RF.2.3.c rdf:type owl:Class ;
    prov:wasQuotedFrom <http://www.corestandards.org/ELA-Literacy/RF/2/3/c/> ;
    rdfs:subClassOf :CCSS.ELA-Literacy.RF.2.3 ;
    rdfs:comment "Decode regularly spelled two-syllable words with long vowels."^^xsd:string .

:CCSS.ELA-Literacy.RF.2.3.d rdf:type owl:Class ;
    prov:wasQuotedFrom <http://www.corestandards.org/ELA-Literacy/RF/2/3/d/> ;
    rdfs:subClassOf :CCSS.ELA-Literacy.RF.2.3 ;
    rdfs:comment "Decode words with common prefixes and suffixes."^^xsd:string .

:CCSS.ELA-Literacy.RF.2.3.e rdf:type owl:Class ;
    prov:wasQuotedFrom <http://www.corestandards.org/ELA-Literacy/RF/2/3/e/> ;
    rdfs:subClassOf :CCSS.ELA-Literacy.RF.2.3 ;
    rdfs:comment "Identify words with inconsistent but common spelling-sound correspondences."^^xsd:string .

:CCSS.ELA-Literacy.RF.2.3.f rdf:type owl:Class ;
    prov:wasQuotedFrom <http://www.corestandards.org/ELA-Literacy/RF/2/3/f/> ;
    rdfs:subClassOf :CCSS.ELA-Literacy.RF.2.3 ;
    rdfs:comment "Recognize and read grade-appropriate irregularly spelled words."^^xsd:string .

:CCSS.ELA-Literacy.RF.2.4 rdf:type owl:Class ;
    prov:wasQuotedFrom <http://www.corestandards.org/ELA-Literacy/RF/2/4/> ;
    rdfs:subClassOf :CCSS.ELA-Literacy.RF.2 ;
    rdfs:comment "Read with sufficient accuracy and fluency to support comprehension."^^xsd:string .

:CCSS.ELA-Literacy.RF.2.4.a rdf:type owl:Class ;
    prov:wasQuotedFrom <http://www.corestandards.org/ELA-Literacy/RF/2/4/a/> ;
    rdfs:subClassOf :CCSS.ELA-Literacy.RF.2.4 ;
    rdfs:comment "Read grade-level text with purpose and understanding."^^xsd:string .

:CCSS.ELA-Literacy.RF.2.4.b rdf:type owl:Class ;
    prov:wasQuotedFrom <http://www.corestandards.org/ELA-Literacy/RF/2/4/b/> ;
    rdfs:subClassOf :CCSS.ELA-Literacy.RF.2.4 ;
    rdfs:comment "Read grade-level text orally with accuracy, appropriate rate, and expression on successive readings."^^xsd:string .

:CCSS.ELA-Literacy.RF.2.4.c rdf:type owl:Class ;
    prov:wasQuotedFrom <http://www.corestandards.org/ELA-Literacy/RF/2/4/c/> ;
    rdfs:subClassOf :CCSS.ELA-Literacy.RF.2.4 ;
    rdfs:comment "Use context to confirm or self-correct word recognition and understanding, rereading as necessary."^^xsd:string .

:CCSS.ELA-Literacy.RF.3.3 rdf:type owl:Class ;
    prov:wasQuotedFrom <http://www.corestandards.org/ELA-Literacy/RF/3/3/> ;
    rdfs:subClassOf :CCSS.ELA-Literacy.RF.3 ;
    rdfs:comment "Know and apply grade-level phonics and word analysis skills in decoding words."^^xsd:string .

:CCSS.ELA-Literacy.RF.3.3.a rdf:type owl:Class ;
    prov:wasQuotedFrom <http://www.corestandards.org/ELA-Literacy/RF/3/3/a/> ;
    rdfs:subClassOf :CCSS.ELA-Literacy.RF.3.3 ;
    rdfs:comment "Identify and know the meaning of the most common prefixes and derivational suffixes."^^xsd:string .

:CCSS.ELA-Literacy.RF.3.3.b rdf:type owl:Class ;
    prov:wasQuotedFrom <http://www.corestandards.org/ELA-Literacy/RF/3/3/b/> ;
    rdfs:subClassOf :CCSS.ELA-Literacy.RF.3.3 ;
    rdfs:comment "Decode words with common Latin suffixes."^^xsd:string .

:CCSS.ELA-Literacy.RF.3.3.c rdf:type owl:Class ;
    prov:wasQuotedFrom <http://www.corestandards.org/ELA-Literacy/RF/3/3/c/> ;
    rdfs:subClassOf :CCSS.ELA-Literacy.RF.3.3 ;
    rdfs:comment "Decode multisyllable words."^^xsd:string .

:CCSS.ELA-Literacy.RF.3.3.d rdf:type owl:Class ;
    prov:wasQuotedFrom <http://www.corestandards.org/ELA-Literacy/RF/3/3/d/> ;
    rdfs:subClassOf :CCSS.ELA-Literacy.RF.3.3 ;
    rdfs:comment "Read grade-appropriate irregularly spelled words."^^xsd:string .

:CCSS.ELA-Literacy.RF.3.4 rdf:type owl:Class ;
    prov:wasQuotedFrom <http://www.corestandards.org/ELA-Literacy/RF/3/4/> ;
    rdfs:subClassOf :CCSS.ELA-Literacy.RF.3 ;
    rdfs:comment "Read with sufficient accuracy and fluency to support comprehension."^^xsd:string .

:CCSS.ELA-Literacy.RF.3.4.a rdf:type owl:Class ;
    prov:wasQuotedFrom <http://www.corestandards.org/ELA-Literacy/RF/3/4/a/> ;
    rdfs:subClassOf :CCSS.ELA-Literacy.RF.3.4 ;
    rdfs:comment "Read grade-level text with purpose and understanding."^^xsd:string .

:CCSS.ELA-Literacy.RF.3.4.b rdf:type owl:Class ;
    prov:wasQuotedFrom <http://www.corestandards.org/ELA-Literacy/RF/3/4/b/> ;
    rdfs:subClassOf :CCSS.ELA-Literacy.RF.3.4 ;
    rdfs:comment "Read grade-level prose and poetry orally with accuracy, appropriate rate, and expression on successive readings."^^xsd:string .

:CCSS.ELA-Literacy.RF.3.4.c rdf:type owl:Class ;
    prov:wasQuotedFrom <http://www.corestandards.org/ELA-Literacy/RF/3/4/c/> ;
    rdfs:subClassOf :CCSS.ELA-Literacy.RF.3.4 ;
    rdfs:comment "Use context to confirm or self-correct word recognition and understanding, rereading as necessary."^^xsd:string .

:CCSS.ELA-Literacy.RF.4.3 rdf:type owl:Class ;
    prov:wasQuotedFrom <http://www.corestandards.org/ELA-Literacy/RF/4/3/> ;
    rdfs:subClassOf :CCSS.ELA-Literacy.RF.4 ;
    rdfs:comment "Know and apply grade-level phonics and word analysis skills in decoding words."^^xsd:string .

:CCSS.ELA-Literacy.RF.4.3.a rdf:type owl:Class ;
    prov:wasQuotedFrom <http://www.corestandards.org/ELA-Literacy/RF/4/3/a/> ;
    rdfs:subClassOf :CCSS.ELA-Literacy.RF.4.3 ;
    rdfs:comment "Use combined knowledge of all letter-sound correspondences, syllabication patterns, and morphology (e.g., roots and affixes) to read accurately unfamiliar multisyllabic words in context and out of context."^^xsd:string .

:CCSS.ELA-Literacy.RF.4.4 rdf:type owl:Class ;
    prov:wasQuotedFrom <http://www.corestandards.org/ELA-Literacy/RF/4/4/> ;
    rdfs:subClassOf :CCSS.ELA-Literacy.RF.4 ;
    rdfs:comment "Read with sufficient accuracy and fluency to support comprehension."^^xsd:string .

:CCSS.ELA-Literacy.RF.4.4.a rdf:type owl:Class ;
    prov:wasQuotedFrom <http://www.corestandards.org/ELA-Literacy/RF/4/4/a/> ;
    rdfs:subClassOf :CCSS.ELA-Literacy.RF.4.4 ;
    rdfs:comment "Read grade-level text with purpose and understanding."^^xsd:string .

:CCSS.ELA-Literacy.RF.4.4.b rdf:type owl:Class ;
    prov:wasQuotedFrom <http://www.corestandards.org/ELA-Literacy/RF/4/4/b/> ;
    rdfs:subClassOf :CCSS.ELA-Literacy.RF.4.4 ;
    rdfs:comment "Read grade-level prose and poetry orally with accuracy, appropriate rate, and expression on successive readings."^^xsd:string .

:CCSS.ELA-Literacy.RF.4.4.c rdf:type owl:Class ;
    prov:wasQuotedFrom <http://www.corestandards.org/ELA-Literacy/RF/4/4/c/> ;
    rdfs:subClassOf :CCSS.ELA-Literacy.RF.4.4 ;
    rdfs:comment "Use context to confirm or self-correct word recognition and understanding, rereading as necessary."^^xsd:string .

:CCSS.ELA-Literacy.RF.5.3 rdf:type owl:Class ;
    prov:wasQuotedFrom <http://www.corestandards.org/ELA-Literacy/RF/5/3/> ;
    rdfs:subClassOf :CCSS.ELA-Literacy.RF.5 ;
    rdfs:comment "Know and apply grade-level phonics and word analysis skills in decoding words."^^xsd:string .

:CCSS.ELA-Literacy.RF.5.3.a rdf:type owl:Class ;
    prov:wasQuotedFrom <http://www.corestandards.org/ELA-Literacy/RF/5/3/a/> ;
    rdfs:subClassOf :CCSS.ELA-Literacy.RF.5.3 ;
    rdfs:comment "Use combined knowledge of all letter-sound correspondences, syllabication patterns, and morphology (e.g., roots and affixes) to read accurately unfamiliar multisyllabic words in context and out of context."^^xsd:string .

:CCSS.ELA-Literacy.RF.5.4 rdf:type owl:Class ;
    prov:wasQuotedFrom <http://www.corestandards.org/ELA-Literacy/RF/5/4/> ;
    rdfs:subClassOf :CCSS.ELA-Literacy.RF.5 ;
    rdfs:comment "Read with sufficient accuracy and fluency to support comprehension."^^xsd:string .

:CCSS.ELA-Literacy.RF.5.4.a rdf:type owl:Class ;
    prov:wasQuotedFrom <http://www.corestandards.org/ELA-Literacy/RF/5/4/a/> ;
    rdfs:subClassOf :CCSS.ELA-Literacy.RF.5.4 ;
    rdfs:comment "Read grade-level text with purpose and understanding."^^xsd:string .

:CCSS.ELA-Literacy.RF.5.4.b rdf:type owl:Class ;
    prov:wasQuotedFrom <http://www.corestandards.org/ELA-Literacy/RF/5/4/b/> ;
    rdfs:subClassOf :CCSS.ELA-Literacy.RF.5.4 ;
    rdfs:comment "Read grade-level prose and poetry orally with accuracy, appropriate rate, and expression on successive readings."^^xsd:string .

:CCSS.ELA-Literacy.RF.5.4.c rdf:type owl:Class ;
    prov:wasQuotedFrom <http://www.corestandards.org/ELA-Literacy/RF/5/4/c/> ;
    rdfs:subClassOf :CCSS.ELA-Literacy.RF.5.4 ;
    rdfs:comment "Use context to confirm or self-correct word recognition and understanding, rereading as necessary."^^xsd:string .

:CCSS.ELA-Literacy.W.K.1 rdf:type owl:Class ;
    prov:wasQuotedFrom <http://www.corestandards.org/ELA-Literacy/W/K/1/> ;
    rdfs:subClassOf :CCSS.ELA-Literacy.W.K ;
    rdfs:comment "Use a combination of drawing, dictating, and writing to compose opinion pieces in which they tell a reader the topic or the name of the book they are writing about and state an opinion or preference about the topic or book (e.g., My favorite book is...)."^^xsd:string .

:CCSS.ELA-Literacy.W.K.2 rdf:type owl:Class ;
    prov:wasQuotedFrom <http://www.corestandards.org/ELA-Literacy/W/K/2/> ;
    rdfs:subClassOf :CCSS.ELA-Literacy.W.K ;
    rdfs:comment "Use a combination of drawing, dictating, and writing to compose informative/explanatory texts in which they name what they are writing about and supply some information about the topic."^^xsd:string .

:CCSS.ELA-Literacy.W.K.3 rdf:type owl:Class ;
    prov:wasQuotedFrom <http://www.corestandards.org/ELA-Literacy/W/K/3/> ;
    rdfs:subClassOf :CCSS.ELA-Literacy.W.K ;
    rdfs:comment "Use a combination of drawing, dictating, and writing to narrate a single event or several loosely linked events, tell about the events in the order in which they occurred, and provide a reaction to what happened."^^xsd:string .

:CCSS.ELA-Literacy.W.K.4 rdf:type owl:Class ;
    prov:wasQuotedFrom <http://www.corestandards.org/ELA-Literacy/W/K/4/> ;
    rdfs:subClassOf :CCSS.ELA-Literacy.W.K ;
    rdfs:comment "(W.K.4 begins in grade 3)"^^xsd:string .

:CCSS.ELA-Literacy.W.K.5 rdf:type owl:Class ;
    prov:wasQuotedFrom <http://www.corestandards.org/ELA-Literacy/W/K/5/> ;
    rdfs:subClassOf :CCSS.ELA-Literacy.W.K ;
    rdfs:comment "With guidance and support from adults, respond to questions and suggestions from peers and add details to strengthen writing as needed."^^xsd:string .

:CCSS.ELA-Literacy.W.K.6 rdf:type owl:Class ;
    prov:wasQuotedFrom <http://www.corestandards.org/ELA-Literacy/W/K/6/> ;
    rdfs:subClassOf :CCSS.ELA-Literacy.W.K ;
    rdfs:comment "With guidance and support from adults, explore a variety of digital tools to produce and publish writing, including in collaboration with peers."^^xsd:string .

:CCSS.ELA-Literacy.W.K.7 rdf:type owl:Class ;
    prov:wasQuotedFrom <http://www.corestandards.org/ELA-Literacy/W/K/7/> ;
    rdfs:subClassOf :CCSS.ELA-Literacy.W.K ;
    rdfs:comment "Participate in shared research and writing projects (e.g., explore a number of books by a favorite author and express opinions about them)."^^xsd:string .

:CCSS.ELA-Literacy.W.K.8 rdf:type owl:Class ;
    prov:wasQuotedFrom <http://www.corestandards.org/ELA-Literacy/W/K/8/> ;
    rdfs:subClassOf :CCSS.ELA-Literacy.W.K ;
    rdfs:comment "With guidance and support from adults, recall information from experiences or gather information from provided sources to answer a question."^^xsd:string .

:CCSS.ELA-Literacy.W.K.9 rdf:type owl:Class ;
    prov:wasQuotedFrom <http://www.corestandards.org/ELA-Literacy/W/K/9/> ;
    rdfs:subClassOf :CCSS.ELA-Literacy.W.K ;
    rdfs:comment "(W.K.9 begins in grade 4)"^^xsd:string .

:CCSS.ELA-Literacy.W.K.10 rdf:type owl:Class ;
    prov:wasQuotedFrom <http://www.corestandards.org/ELA-Literacy/W/K/10/> ;
    rdfs:subClassOf :CCSS.ELA-Literacy.W.K ;
    rdfs:comment "(W.K.10 begins in grade 3)"^^xsd:string .

:CCSS.ELA-Literacy.W.1.1 rdf:type owl:Class ;
    prov:wasQuotedFrom <http://www.corestandards.org/ELA-Literacy/W/1/1/> ;
    rdfs:subClassOf :CCSS.ELA-Literacy.W.1 ;
    rdfs:comment "Write opinion pieces in which they introduce the topic or name the book they are writing about, state an opinion, supply a reason for the opinion, and provide some sense of closure."^^xsd:string .

:CCSS.ELA-Literacy.W.1.2 rdf:type owl:Class ;
    prov:wasQuotedFrom <http://www.corestandards.org/ELA-Literacy/W/1/2/> ;
    rdfs:subClassOf :CCSS.ELA-Literacy.W.1 ;
    rdfs:comment "Write informative/explanatory texts in which they name a topic, supply some facts about the topic, and provide some sense of closure."^^xsd:string .

:CCSS.ELA-Literacy.W.1.3 rdf:type owl:Class ;
    prov:wasQuotedFrom <http://www.corestandards.org/ELA-Literacy/W/1/3/> ;
    rdfs:subClassOf :CCSS.ELA-Literacy.W.1 ;
    rdfs:comment "Write narratives in which they recount two or more appropriately sequenced events, include some details regarding what happened, use temporal words to signal event order, and provide some sense of closure."^^xsd:string .

:CCSS.ELA-Literacy.W.1.4 rdf:type owl:Class ;
    prov:wasQuotedFrom <http://www.corestandards.org/ELA-Literacy/W/1/4/> ;
    rdfs:subClassOf :CCSS.ELA-Literacy.W.1 ;
    rdfs:comment "(W.1.4 begins in grade 3)"^^xsd:string .

:CCSS.ELA-Literacy.W.1.5 rdf:type owl:Class ;
    prov:wasQuotedFrom <http://www.corestandards.org/ELA-Literacy/W/1/5/> ;
    rdfs:subClassOf :CCSS.ELA-Literacy.W.1 ;
    rdfs:comment "With guidance and support from adults, focus on a topic, respond to questions and suggestions from peers, and add details to strengthen writing as needed."^^xsd:string .

:CCSS.ELA-Literacy.W.1.6 rdf:type owl:Class ;
    prov:wasQuotedFrom <http://www.corestandards.org/ELA-Literacy/W/1/6/> ;
    rdfs:subClassOf :CCSS.ELA-Literacy.W.1 ;
    rdfs:comment "With guidance and support from adults, use a variety of digital tools to produce and publish writing, including in collaboration with peers."^^xsd:string .

:CCSS.ELA-Literacy.W.1.7 rdf:type owl:Class ;
    prov:wasQuotedFrom <http://www.corestandards.org/ELA-Literacy/W/1/7/> ;
    rdfs:subClassOf :CCSS.ELA-Literacy.W.1 ;
    rdfs:comment "Participate in shared research and writing projects (e.g., explore a number of 'how-to' books on a given topic and use them to write a sequence of instructions)."^^xsd:string .

:CCSS.ELA-Literacy.W.1.8 rdf:type owl:Class ;
    prov:wasQuotedFrom <http://www.corestandards.org/ELA-Literacy/W/1/8/> ;
    rdfs:subClassOf :CCSS.ELA-Literacy.W.1 ;
    rdfs:comment "With guidance and support from adults, recall information from experiences or gather information from provided sources to answer a question."^^xsd:string .

:CCSS.ELA-Literacy.W.1.9 rdf:type owl:Class ;
    prov:wasQuotedFrom <http://www.corestandards.org/ELA-Literacy/W/1/9/> ;
    rdfs:subClassOf :CCSS.ELA-Literacy.W.1 ;
    rdfs:comment "(W.1.9 begins in grade 4)"^^xsd:string .

:CCSS.ELA-Literacy.W.1.10 rdf:type owl:Class ;
    prov:wasQuotedFrom <http://www.corestandards.org/ELA-Literacy/W/1/10/> ;
    rdfs:subClassOf :CCSS.ELA-Literacy.W.1 ;
    rdfs:comment "(W.1.10 begins in grade 3)"^^xsd:string .

:CCSS.ELA-Literacy.W.2.1 rdf:type owl:Class ;
    prov:wasQuotedFrom <http://www.corestandards.org/ELA-Literacy/W/2/1/> ;
    rdfs:subClassOf :CCSS.ELA-Literacy.W.2 ;
    rdfs:comment "Write opinion pieces in which they introduce the topic or book they are writing about, state an opinion, supply reasons that support the opinion, use linking words (e.g., because, and, also) to connect opinion and reasons, and provide a concluding statement or section."^^xsd:string .

:CCSS.ELA-Literacy.W.2.2 rdf:type owl:Class ;
    prov:wasQuotedFrom <http://www.corestandards.org/ELA-Literacy/W/2/2/> ;
    rdfs:subClassOf :CCSS.ELA-Literacy.W.2 ;
    rdfs:comment "Write informative/explanatory texts in which they introduce a topic, use facts and definitions to develop points, and provide a concluding statement or section."^^xsd:string .

:CCSS.ELA-Literacy.W.2.3 rdf:type owl:Class ;
    prov:wasQuotedFrom <http://www.corestandards.org/ELA-Literacy/W/2/3/> ;
    rdfs:subClassOf :CCSS.ELA-Literacy.W.2 ;
    rdfs:comment "Write narratives in which they recount a well-elaborated event or short sequence of events, include details to describe actions, thoughts, and feelings, use temporal words to signal event order, and provide a sense of closure."^^xsd:string .

:CCSS.ELA-Literacy.W.2.4 rdf:type owl:Class ;
    prov:wasQuotedFrom <http://www.corestandards.org/ELA-Literacy/W/2/4/> ;
    rdfs:subClassOf :CCSS.ELA-Literacy.W.2 ;
    rdfs:comment "(W.2.4 begins in grade 3)"^^xsd:string .

:CCSS.ELA-Literacy.W.2.5 rdf:type owl:Class ;
    prov:wasQuotedFrom <http://www.corestandards.org/ELA-Literacy/W/2/5/> ;
    rdfs:subClassOf :CCSS.ELA-Literacy.W.2 ;
    rdfs:comment "With guidance and support from adults and peers, focus on a topic and strengthen writing as needed by revising and editing."^^xsd:string .

:CCSS.ELA-Literacy.W.2.6 rdf:type owl:Class ;
    prov:wasQuotedFrom <http://www.corestandards.org/ELA-Literacy/W/2/6/> ;
    rdfs:subClassOf :CCSS.ELA-Literacy.W.2 ;
    rdfs:comment "With guidance and support from adults, use a variety of digital tools to produce and publish writing, including in collaboration with peers."^^xsd:string .

:CCSS.ELA-Literacy.W.2.7 rdf:type owl:Class ;
    prov:wasQuotedFrom <http://www.corestandards.org/ELA-Literacy/W/2/7/> ;
    rdfs:subClassOf :CCSS.ELA-Literacy.W.2 ;
    rdfs:comment "Participate in shared research and writing projects (e.g., read a number of books on a single topic to produce a report; record science observations)."^^xsd:string .

:CCSS.ELA-Literacy.W.2.8 rdf:type owl:Class ;
    prov:wasQuotedFrom <http://www.corestandards.org/ELA-Literacy/W/2/8/> ;
    rdfs:subClassOf :CCSS.ELA-Literacy.W.2 ;
    rdfs:comment "Recall information from experiences or gather information from provided sources to answer a question."^^xsd:string .

:CCSS.ELA-Literacy.W.2.9 rdf:type owl:Class ;
    prov:wasQuotedFrom <http://www.corestandards.org/ELA-Literacy/W/2/9/> ;
    rdfs:subClassOf :CCSS.ELA-Literacy.W.2 ;
    rdfs:comment "(W.2.9 begins in grade 4)"^^xsd:string .

:CCSS.ELA-Literacy.W.2.10 rdf:type owl:Class ;
    prov:wasQuotedFrom <http://www.corestandards.org/ELA-Literacy/W/2/10/> ;
    rdfs:subClassOf :CCSS.ELA-Literacy.W.2 ;
    rdfs:comment "(W.2.10 begins in grade 3)"^^xsd:string .

:CCSS.ELA-Literacy.W.3.1 rdf:type owl:Class ;
    prov:wasQuotedFrom <http://www.corestandards.org/ELA-Literacy/W/3/1/> ;
    rdfs:subClassOf :CCSS.ELA-Literacy.W.3 ;
    rdfs:comment "Write opinion pieces on topics or texts, supporting a point of view with reasons."^^xsd:string .

:CCSS.ELA-Literacy.W.3.1.a rdf:type owl:Class ;
    prov:wasQuotedFrom <http://www.corestandards.org/ELA-Literacy/W/3/1/a/> ;
    rdfs:subClassOf :CCSS.ELA-Literacy.W.3.1 ;
    rdfs:comment "Introduce the topic or text they are writing about, state an opinion, and create an organizational structure that lists reasons."^^xsd:string .

:CCSS.ELA-Literacy.W.3.1.b rdf:type owl:Class ;
    prov:wasQuotedFrom <http://www.corestandards.org/ELA-Literacy/W/3/1/b/> ;
    rdfs:subClassOf :CCSS.ELA-Literacy.W.3.1 ;
    rdfs:comment "Provide reasons that support the opinion."^^xsd:string .

:CCSS.ELA-Literacy.W.3.1.c rdf:type owl:Class ;
    prov:wasQuotedFrom <http://www.corestandards.org/ELA-Literacy/W/3/1/c/> ;
    rdfs:subClassOf :CCSS.ELA-Literacy.W.3.1 ;
    rdfs:comment "Use linking words and phrases (e.g., because, therefore, since, for example) to connect opinion and reasons."^^xsd:string .

:CCSS.ELA-Literacy.W.3.1.d rdf:type owl:Class ;
    prov:wasQuotedFrom <http://www.corestandards.org/ELA-Literacy/W/3/1/d/> ;
    rdfs:subClassOf :CCSS.ELA-Literacy.W.3.1 ;
    rdfs:comment "Provide a concluding statement or section."^^xsd:string .

:CCSS.ELA-Literacy.W.3.2 rdf:type owl:Class ;
    prov:wasQuotedFrom <http://www.corestandards.org/ELA-Literacy/W/3/2/> ;
    rdfs:subClassOf :CCSS.ELA-Literacy.W.3 ;
    rdfs:comment "Write informative/explanatory texts to examine a topic and convey ideas and information clearly."^^xsd:string .

:CCSS.ELA-Literacy.W.3.2.a rdf:type owl:Class ;
    prov:wasQuotedFrom <http://www.corestandards.org/ELA-Literacy/W/3/2/a/> ;
    rdfs:subClassOf :CCSS.ELA-Literacy.W.3.2 ;
    rdfs:comment "Introduce a topic and group related information together; include illustrations when useful to aiding comprehension."^^xsd:string .

:CCSS.ELA-Literacy.W.3.2.b rdf:type owl:Class ;
    prov:wasQuotedFrom <http://www.corestandards.org/ELA-Literacy/W/3/2/b/> ;
    rdfs:subClassOf :CCSS.ELA-Literacy.W.3.2 ;
    rdfs:comment "Develop the topic with facts, definitions, and details."^^xsd:string .

:CCSS.ELA-Literacy.W.3.2.c rdf:type owl:Class ;
    prov:wasQuotedFrom <http://www.corestandards.org/ELA-Literacy/W/3/2/c/> ;
    rdfs:subClassOf :CCSS.ELA-Literacy.W.3.2 ;
    rdfs:comment "Use linking words and phrases (e.g., also, another, and, more, but) to connect ideas within categories of information."^^xsd:string .

:CCSS.ELA-Literacy.W.3.2.d rdf:type owl:Class ;
    prov:wasQuotedFrom <http://www.corestandards.org/ELA-Literacy/W/3/2/d/> ;
    rdfs:subClassOf :CCSS.ELA-Literacy.W.3.2 ;
    rdfs:comment "Provide a concluding statement or section."^^xsd:string .

:CCSS.ELA-Literacy.W.3.3 rdf:type owl:Class ;
    prov:wasQuotedFrom <http://www.corestandards.org/ELA-Literacy/W/3/3/> ;
    rdfs:subClassOf :CCSS.ELA-Literacy.W.3 ;
    rdfs:comment "Write narratives to develop real or imagined experiences or events using effective technique, descriptive details, and clear event sequences."^^xsd:string .

:CCSS.ELA-Literacy.W.3.3.a rdf:type owl:Class ;
    prov:wasQuotedFrom <http://www.corestandards.org/ELA-Literacy/W/3/3/a/> ;
    rdfs:subClassOf :CCSS.ELA-Literacy.W.3.3 ;
    rdfs:comment "Establish a situation and introduce a narrator and/or characters; organize an event sequence that unfolds naturally."^^xsd:string .

:CCSS.ELA-Literacy.W.3.3.b rdf:type owl:Class ;
    prov:wasQuotedFrom <http://www.corestandards.org/ELA-Literacy/W/3/3/b/> ;
    rdfs:subClassOf :CCSS.ELA-Literacy.W.3.3 ;
    rdfs:comment "Use dialogue and descriptions of actions, thoughts, and feelings to develop experiences and events or show the response of characters to situations."^^xsd:string .

:CCSS.ELA-Literacy.W.3.3.c rdf:type owl:Class ;
    prov:wasQuotedFrom <http://www.corestandards.org/ELA-Literacy/W/3/3/c/> ;
    rdfs:subClassOf :CCSS.ELA-Literacy.W.3.3 ;
    rdfs:comment "Use temporal words and phrases to signal event order."^^xsd:string .

:CCSS.ELA-Literacy.W.3.3.d rdf:type owl:Class ;
    prov:wasQuotedFrom <http://www.corestandards.org/ELA-Literacy/W/3/3/d/> ;
    rdfs:subClassOf :CCSS.ELA-Literacy.W.3.3 ;
    rdfs:comment "Provide a sense of closure."^^xsd:string .

:CCSS.ELA-Literacy.W.3.4 rdf:type owl:Class ;
    prov:wasQuotedFrom <http://www.corestandards.org/ELA-Literacy/W/3/4/> ;
    rdfs:subClassOf :CCSS.ELA-Literacy.W.3 ;
    rdfs:comment "With guidance and support from adults, produce writing in which the development and organization are appropriate to task and purpose. (Grade-specific expectations for writing types are defined in standards 1-3 above.)"^^xsd:string .

:CCSS.ELA-Literacy.W.3.5 rdf:type owl:Class ;
    prov:wasQuotedFrom <http://www.corestandards.org/ELA-Literacy/W/3/5/> ;
    rdfs:subClassOf :CCSS.ELA-Literacy.W.3 ;
    rdfs:comment "With guidance and support from peers and adults, develop and strengthen writing as needed by planning, revising, and editing. (Editing for conventions should demonstrate command of Language standards 1-3 up to and including grade 3 .)"^^xsd:string .

:CCSS.ELA-Literacy.W.3.6 rdf:type owl:Class ;
    prov:wasQuotedFrom <http://www.corestandards.org/ELA-Literacy/W/3/6/> ;
    rdfs:subClassOf :CCSS.ELA-Literacy.W.3 ;
    rdfs:comment "With guidance and support from adults, use technology to produce and publish writing (using keyboarding skills) as well as to interact and collaborate with others."^^xsd:string .

:CCSS.ELA-Literacy.W.3.7 rdf:type owl:Class ;
    prov:wasQuotedFrom <http://www.corestandards.org/ELA-Literacy/W/3/7/> ;
    rdfs:subClassOf :CCSS.ELA-Literacy.W.3 ;
    rdfs:comment "Conduct short research projects that build knowledge about a topic."^^xsd:string .

:CCSS.ELA-Literacy.W.3.8 rdf:type owl:Class ;
    prov:wasQuotedFrom <http://www.corestandards.org/ELA-Literacy/W/3/8/> ;
    rdfs:subClassOf :CCSS.ELA-Literacy.W.3 ;
    rdfs:comment "Recall information from experiences or gather information from print and digital sources; take brief notes on sources and sort evidence into provided categories."^^xsd:string .

:CCSS.ELA-Literacy.W.3.9 rdf:type owl:Class ;
    prov:wasQuotedFrom <http://www.corestandards.org/ELA-Literacy/W/3/9/> ;
    rdfs:subClassOf :CCSS.ELA-Literacy.W.3 ;
    rdfs:comment "(W.3.9 begins in grade 4)"^^xsd:string .

:CCSS.ELA-Literacy.W.3.10 rdf:type owl:Class ;
    prov:wasQuotedFrom <http://www.corestandards.org/ELA-Literacy/W/3/10/> ;
    rdfs:subClassOf :CCSS.ELA-Literacy.W.3 ;
    rdfs:comment "Write routinely over extended time frames (time for research, reflection, and revision) and shorter time frames (a single sitting or a day or two) for a range of discipline-specific tasks, purposes, and audiences."^^xsd:string .

:CCSS.ELA-Literacy.W.4.1 rdf:type owl:Class ;
    prov:wasQuotedFrom <http://www.corestandards.org/ELA-Literacy/W/4/1/> ;
    rdfs:subClassOf :CCSS.ELA-Literacy.W.4 ;
    rdfs:comment "Write opinion pieces on topics or texts, supporting a point of view with reasons and information."^^xsd:string .

:CCSS.ELA-Literacy.W.4.1.a rdf:type owl:Class ;
    prov:wasQuotedFrom <http://www.corestandards.org/ELA-Literacy/W/4/1/a/> ;
    rdfs:subClassOf :CCSS.ELA-Literacy.W.4.1 ;
    rdfs:comment "Introduce a topic or text clearly, state an opinion, and create an organizational structure in which related ideas are grouped to support the writer's purpose."^^xsd:string .

:CCSS.ELA-Literacy.W.4.1.b rdf:type owl:Class ;
    prov:wasQuotedFrom <http://www.corestandards.org/ELA-Literacy/W/4/1/b/> ;
    rdfs:subClassOf :CCSS.ELA-Literacy.W.4.1 ;
    rdfs:comment "Provide reasons that are supported by facts and details."^^xsd:string .

:CCSS.ELA-Literacy.W.4.1.c rdf:type owl:Class ;
    prov:wasQuotedFrom <http://www.corestandards.org/ELA-Literacy/W/4/1/c/> ;
    rdfs:subClassOf :CCSS.ELA-Literacy.W.4.1 ;
    rdfs:comment "Link opinion and reasons using words and phrases (e.g., for instance, in order to, in addition)."^^xsd:string .

:CCSS.ELA-Literacy.W.4.1.d rdf:type owl:Class ;
    prov:wasQuotedFrom <http://www.corestandards.org/ELA-Literacy/W/4/1/d/> ;
    rdfs:subClassOf :CCSS.ELA-Literacy.W.4.1 ;
    rdfs:comment "Provide a concluding statement or section related to the opinion presented."^^xsd:string .

:CCSS.ELA-Literacy.W.4.2 rdf:type owl:Class ;
    prov:wasQuotedFrom <http://www.corestandards.org/ELA-Literacy/W/4/2/> ;
    rdfs:subClassOf :CCSS.ELA-Literacy.W.4 ;
    rdfs:comment "Write informative/explanatory texts to examine a topic and convey ideas and information clearly."^^xsd:string .

:CCSS.ELA-Literacy.W.4.2.a rdf:type owl:Class ;
    prov:wasQuotedFrom <http://www.corestandards.org/ELA-Literacy/W/4/2/a/> ;
    rdfs:subClassOf :CCSS.ELA-Literacy.W.4.2 ;
    rdfs:comment "Introduce a topic clearly and group related information in paragraphs and sections; include formatting (e.g., headings), illustrations, and multimedia when useful to aiding comprehension."^^xsd:string .

:CCSS.ELA-Literacy.W.4.2.b rdf:type owl:Class ;
    prov:wasQuotedFrom <http://www.corestandards.org/ELA-Literacy/W/4/2/b/> ;
    rdfs:subClassOf :CCSS.ELA-Literacy.W.4.2 ;
    rdfs:comment "Develop the topic with facts, definitions, concrete details, quotations, or other information and examples related to the topic."^^xsd:string .

:CCSS.ELA-Literacy.W.4.2.c rdf:type owl:Class ;
    prov:wasQuotedFrom <http://www.corestandards.org/ELA-Literacy/W/4/2/c/> ;
    rdfs:subClassOf :CCSS.ELA-Literacy.W.4.2 ;
    rdfs:comment "Link ideas within categories of information using words and phrases (e.g., another, for example, also, because)."^^xsd:string .

:CCSS.ELA-Literacy.W.4.2.d rdf:type owl:Class ;
    prov:wasQuotedFrom <http://www.corestandards.org/ELA-Literacy/W/4/2/d/> ;
    rdfs:subClassOf :CCSS.ELA-Literacy.W.4.2 ;
    rdfs:comment "Use precise language and domain-specific vocabulary to inform about or explain the topic."^^xsd:string .

:CCSS.ELA-Literacy.W.4.2.e rdf:type owl:Class ;
    prov:wasQuotedFrom <http://www.corestandards.org/ELA-Literacy/W/4/2/e/> ;
    rdfs:subClassOf :CCSS.ELA-Literacy.W.4.2 ;
    rdfs:comment "Provide a concluding statement or section related to the information or explanation presented."^^xsd:string .

:CCSS.ELA-Literacy.W.4.3 rdf:type owl:Class ;
    prov:wasQuotedFrom <http://www.corestandards.org/ELA-Literacy/W/4/3/> ;
    rdfs:subClassOf :CCSS.ELA-Literacy.W.4 ;
    rdfs:comment "Write narratives to develop real or imagined experiences or events using effective technique, descriptive details, and clear event sequences."^^xsd:string .

:CCSS.ELA-Literacy.W.4.3.a rdf:type owl:Class ;
    prov:wasQuotedFrom <http://www.corestandards.org/ELA-Literacy/W/4/3/a/> ;
    rdfs:subClassOf :CCSS.ELA-Literacy.W.4.3 ;
    rdfs:comment "Orient the reader by establishing a situation and introducing a narrator and/or characters; organize an event sequence that unfolds naturally."^^xsd:string .

:CCSS.ELA-Literacy.W.4.3.b rdf:type owl:Class ;
    prov:wasQuotedFrom <http://www.corestandards.org/ELA-Literacy/W/4/3/b/> ;
    rdfs:subClassOf :CCSS.ELA-Literacy.W.4.3 ;
    rdfs:comment "Use dialogue and description to develop experiences and events or show the responses of characters to situations."^^xsd:string .

:CCSS.ELA-Literacy.W.4.3.c rdf:type owl:Class ;
    prov:wasQuotedFrom <http://www.corestandards.org/ELA-Literacy/W/4/3/c/> ;
    rdfs:subClassOf :CCSS.ELA-Literacy.W.4.3 ;
    rdfs:comment "Use a variety of transitional words and phrases to manage the sequence of events."^^xsd:string .

:CCSS.ELA-Literacy.W.4.3.d rdf:type owl:Class ;
    prov:wasQuotedFrom <http://www.corestandards.org/ELA-Literacy/W/4/3/d/> ;
    rdfs:subClassOf :CCSS.ELA-Literacy.W.4.3 ;
    rdfs:comment "Use concrete words and phrases and sensory details to convey experiences and events precisely."^^xsd:string .

:CCSS.ELA-Literacy.W.4.3.e rdf:type owl:Class ;
    prov:wasQuotedFrom <http://www.corestandards.org/ELA-Literacy/W/4/3/e/> ;
    rdfs:subClassOf :CCSS.ELA-Literacy.W.4.3 ;
    rdfs:comment "Provide a conclusion that follows from the narrated experiences or events."^^xsd:string .

:CCSS.ELA-Literacy.W.4.4 rdf:type owl:Class ;
    prov:wasQuotedFrom <http://www.corestandards.org/ELA-Literacy/W/4/4/> ;
    rdfs:subClassOf :CCSS.ELA-Literacy.W.4 ;
    rdfs:comment "Produce clear and coherent writing in which the development and organization are appropriate to task, purpose, and audience. (Grade-specific expectations for writing types are defined in standards 1-3 above.)"^^xsd:string .

:CCSS.ELA-Literacy.W.4.5 rdf:type owl:Class ;
    prov:wasQuotedFrom <http://www.corestandards.org/ELA-Literacy/W/4/5/> ;
    rdfs:subClassOf :CCSS.ELA-Literacy.W.4 ;
    rdfs:comment "With guidance and support from peers and adults, develop and strengthen writing as needed by planning, revising, and editing. (Editing for conventions should demonstrate command of Language standards 1-3 up to and including grade 4 .)"^^xsd:string .

:CCSS.ELA-Literacy.W.4.6 rdf:type owl:Class ;
    prov:wasQuotedFrom <http://www.corestandards.org/ELA-Literacy/W/4/6/> ;
    rdfs:subClassOf :CCSS.ELA-Literacy.W.4 ;
    rdfs:comment "With some guidance and support from adults, use technology, including the Internet, to produce and publish writing as well as to interact and collaborate with others; demonstrate sufficient command of keyboarding skills to type a minimum of one page in a single sitting."^^xsd:string .

:CCSS.ELA-Literacy.W.4.7 rdf:type owl:Class ;
    prov:wasQuotedFrom <http://www.corestandards.org/ELA-Literacy/W/4/7/> ;
    rdfs:subClassOf :CCSS.ELA-Literacy.W.4 ;
    rdfs:comment "Conduct short research projects that build knowledge through investigation of different aspects of a topic."^^xsd:string .

:CCSS.ELA-Literacy.W.4.8 rdf:type owl:Class ;
    prov:wasQuotedFrom <http://www.corestandards.org/ELA-Literacy/W/4/8/> ;
    rdfs:subClassOf :CCSS.ELA-Literacy.W.4 ;
    rdfs:comment "Recall relevant information from experiences or gather relevant information from print and digital sources; take notes and categorize information, and provide a list of sources."^^xsd:string .

:CCSS.ELA-Literacy.W.4.9 rdf:type owl:Class ;
    prov:wasQuotedFrom <http://www.corestandards.org/ELA-Literacy/W/4/9/> ;
    rdfs:subClassOf :CCSS.ELA-Literacy.W.4 ;
    rdfs:comment "Draw evidence from literary or informational texts to support analysis, reflection, and research."^^xsd:string .

:CCSS.ELA-Literacy.W.4.9.a rdf:type owl:Class ;
    prov:wasQuotedFrom <http://www.corestandards.org/ELA-Literacy/W/4/9/a/> ;
    rdfs:subClassOf :CCSS.ELA-Literacy.W.4.9 ;
    rdfs:comment "Apply grade 4 Reading standards to literature (e.g., 'Describe in depth a character, setting, or event in a story or drama, drawing on specific details in the text [e.g., a character's thoughts, words, or actions].')."^^xsd:string .

:CCSS.ELA-Literacy.W.4.9.b rdf:type owl:Class ;
    prov:wasQuotedFrom <http://www.corestandards.org/ELA-Literacy/W/4/9/b/> ;
    rdfs:subClassOf :CCSS.ELA-Literacy.W.4.9 ;
    rdfs:comment "Apply grade 4 Reading standards to informational texts (e.g., 'Explain how an author uses reasons and evidence to support particular points in a text')."^^xsd:string .

:CCSS.ELA-Literacy.W.4.10 rdf:type owl:Class ;
    prov:wasQuotedFrom <http://www.corestandards.org/ELA-Literacy/W/4/10/> ;
    rdfs:subClassOf :CCSS.ELA-Literacy.W.4 ;
    rdfs:comment "Write routinely over extended time frames (time for research, reflection, and revision) and shorter time frames (a single sitting or a day or two) for a range of discipline-specific tasks, purposes, and audiences."^^xsd:string .

:CCSS.ELA-Literacy.W.5.1 rdf:type owl:Class ;
    prov:wasQuotedFrom <http://www.corestandards.org/ELA-Literacy/W/5/1/> ;
    rdfs:subClassOf :CCSS.ELA-Literacy.W.5 ;
    rdfs:comment "Write opinion pieces on topics or texts, supporting a point of view with reasons and information."^^xsd:string .

:CCSS.ELA-Literacy.W.5.1.a rdf:type owl:Class ;
    prov:wasQuotedFrom <http://www.corestandards.org/ELA-Literacy/W/5/1/a/> ;
    rdfs:subClassOf :CCSS.ELA-Literacy.W.5.1 ;
    rdfs:comment "Introduce a topic or text clearly, state an opinion, and create an organizational structure in which ideas are logically grouped to support the writer's purpose."^^xsd:string .

:CCSS.ELA-Literacy.W.5.1.b rdf:type owl:Class ;
    prov:wasQuotedFrom <http://www.corestandards.org/ELA-Literacy/W/5/1/b/> ;
    rdfs:subClassOf :CCSS.ELA-Literacy.W.5.1 ;
    rdfs:comment "Provide logically ordered reasons that are supported by facts and details."^^xsd:string .

:CCSS.ELA-Literacy.W.5.1.c rdf:type owl:Class ;
    prov:wasQuotedFrom <http://www.corestandards.org/ELA-Literacy/W/5/1/c/> ;
    rdfs:subClassOf :CCSS.ELA-Literacy.W.5.1 ;
    rdfs:comment "Link opinion and reasons using words, phrases, and clauses (e.g., consequently, specifically)."^^xsd:string .

:CCSS.ELA-Literacy.W.5.1.d rdf:type owl:Class ;
    prov:wasQuotedFrom <http://www.corestandards.org/ELA-Literacy/W/5/1/d/> ;
    rdfs:subClassOf :CCSS.ELA-Literacy.W.5.1 ;
    rdfs:comment "Provide a concluding statement or section related to the opinion presented."^^xsd:string .

:CCSS.ELA-Literacy.W.5.2 rdf:type owl:Class ;
    prov:wasQuotedFrom <http://www.corestandards.org/ELA-Literacy/W/5/2/> ;
    rdfs:subClassOf :CCSS.ELA-Literacy.W.5 ;
    rdfs:comment "Write informative/explanatory texts to examine a topic and convey ideas and information clearly."^^xsd:string .

:CCSS.ELA-Literacy.W.5.2.a rdf:type owl:Class ;
    prov:wasQuotedFrom <http://www.corestandards.org/ELA-Literacy/W/5/2/a/> ;
    rdfs:subClassOf :CCSS.ELA-Literacy.W.5.2 ;
    rdfs:comment "Introduce a topic clearly, provide a general observation and focus, and group related information logically; include formatting (e.g., headings), illustrations, and multimedia when useful to aiding comprehension."^^xsd:string .

:CCSS.ELA-Literacy.W.5.2.b rdf:type owl:Class ;
    prov:wasQuotedFrom <http://www.corestandards.org/ELA-Literacy/W/5/2/b/> ;
    rdfs:subClassOf :CCSS.ELA-Literacy.W.5.2 ;
    rdfs:comment "Develop the topic with facts, definitions, concrete details, quotations, or other information and examples related to the topic."^^xsd:string .

:CCSS.ELA-Literacy.W.5.2.c rdf:type owl:Class ;
    prov:wasQuotedFrom <http://www.corestandards.org/ELA-Literacy/W/5/2/c/> ;
    rdfs:subClassOf :CCSS.ELA-Literacy.W.5.2 ;
    rdfs:comment "Link ideas within and across categories of information using words, phrases, and clauses (e.g., in contrast, especially)."^^xsd:string .

:CCSS.ELA-Literacy.W.5.2.d rdf:type owl:Class ;
    prov:wasQuotedFrom <http://www.corestandards.org/ELA-Literacy/W/5/2/d/> ;
    rdfs:subClassOf :CCSS.ELA-Literacy.W.5.2 ;
    rdfs:comment "Use precise language and domain-specific vocabulary to inform about or explain the topic."^^xsd:string .

:CCSS.ELA-Literacy.W.5.2.e rdf:type owl:Class ;
    prov:wasQuotedFrom <http://www.corestandards.org/ELA-Literacy/W/5/2/e/> ;
    rdfs:subClassOf :CCSS.ELA-Literacy.W.5.2 ;
    rdfs:comment "Provide a concluding statement or section related to the information or explanation presented."^^xsd:string .

:CCSS.ELA-Literacy.W.5.3 rdf:type owl:Class ;
    prov:wasQuotedFrom <http://www.corestandards.org/ELA-Literacy/W/5/3/> ;
    rdfs:subClassOf :CCSS.ELA-Literacy.W.5 ;
    rdfs:comment "Write narratives to develop real or imagined experiences or events using effective technique, descriptive details, and clear event sequences."^^xsd:string .

:CCSS.ELA-Literacy.W.5.3.a rdf:type owl:Class ;
    prov:wasQuotedFrom <http://www.corestandards.org/ELA-Literacy/W/5/3/a/> ;
    rdfs:subClassOf :CCSS.ELA-Literacy.W.5.3 ;
    rdfs:comment "Orient the reader by establishing a situation and introducing a narrator and/or characters; organize an event sequence that unfolds naturally."^^xsd:string .

:CCSS.ELA-Literacy.W.5.3.b rdf:type owl:Class ;
    prov:wasQuotedFrom <http://www.corestandards.org/ELA-Literacy/W/5/3/b/> ;
    rdfs:subClassOf :CCSS.ELA-Literacy.W.5.3 ;
    rdfs:comment "Use narrative techniques, such as dialogue, description, and pacing, to develop experiences and events or show the responses of characters to situations."^^xsd:string .

:CCSS.ELA-Literacy.W.5.3.c rdf:type owl:Class ;
    prov:wasQuotedFrom <http://www.corestandards.org/ELA-Literacy/W/5/3/c/> ;
    rdfs:subClassOf :CCSS.ELA-Literacy.W.5.3 ;
    rdfs:comment "Use a variety of transitional words, phrases, and clauses to manage the sequence of events."^^xsd:string .

:CCSS.ELA-Literacy.W.5.3.d rdf:type owl:Class ;
    prov:wasQuotedFrom <http://www.corestandards.org/ELA-Literacy/W/5/3/d/> ;
    rdfs:subClassOf :CCSS.ELA-Literacy.W.5.3 ;
    rdfs:comment "Use concrete words and phrases and sensory details to convey experiences and events precisely."^^xsd:string .

:CCSS.ELA-Literacy.W.5.3.e rdf:type owl:Class ;
    prov:wasQuotedFrom <http://www.corestandards.org/ELA-Literacy/W/5/3/e/> ;
    rdfs:subClassOf :CCSS.ELA-Literacy.W.5.3 ;
    rdfs:comment "Provide a conclusion that follows from the narrated experiences or events."^^xsd:string .

:CCSS.ELA-Literacy.W.5.4 rdf:type owl:Class ;
    prov:wasQuotedFrom <http://www.corestandards.org/ELA-Literacy/W/5/4/> ;
    rdfs:subClassOf :CCSS.ELA-Literacy.W.5 ;
    rdfs:comment "Produce clear and coherent writing in which the development and organization are appropriate to task, purpose, and audience. (Grade-specific expectations for writing types are defined in standards 1-3 above.)"^^xsd:string .

:CCSS.ELA-Literacy.W.5.5 rdf:type owl:Class ;
    prov:wasQuotedFrom <http://www.corestandards.org/ELA-Literacy/W/5/5/> ;
    rdfs:subClassOf :CCSS.ELA-Literacy.W.5 ;
    rdfs:comment "With guidance and support from peers and adults, develop and strengthen writing as needed by planning, revising, editing, rewriting, or trying a new approach. (Editing for conventions should demonstrate command of Language standards 1-3 up to and including grade 5 .)"^^xsd:string .

:CCSS.ELA-Literacy.W.5.6 rdf:type owl:Class ;
    prov:wasQuotedFrom <http://www.corestandards.org/ELA-Literacy/W/5/6/> ;
    rdfs:subClassOf :CCSS.ELA-Literacy.W.5 ;
    rdfs:comment "With some guidance and support from adults, use technology, including the Internet, to produce and publish writing as well as to interact and collaborate with others; demonstrate sufficient command of keyboarding skills to type a minimum of two pages in a single sitting."^^xsd:string .

:CCSS.ELA-Literacy.W.5.7 rdf:type owl:Class ;
    prov:wasQuotedFrom <http://www.corestandards.org/ELA-Literacy/W/5/7/> ;
    rdfs:subClassOf :CCSS.ELA-Literacy.W.5 ;
    rdfs:comment "Conduct short research projects that use several sources to build knowledge through investigation of different aspects of a topic."^^xsd:string .

:CCSS.ELA-Literacy.W.5.8 rdf:type owl:Class ;
    prov:wasQuotedFrom <http://www.corestandards.org/ELA-Literacy/W/5/8/> ;
    rdfs:subClassOf :CCSS.ELA-Literacy.W.5 ;
    rdfs:comment "Recall relevant information from experiences or gather relevant information from print and digital sources; summarize or paraphrase information in notes and finished work, and provide a list of sources."^^xsd:string .

:CCSS.ELA-Literacy.W.5.9 rdf:type owl:Class ;
    prov:wasQuotedFrom <http://www.corestandards.org/ELA-Literacy/W/5/9/> ;
    rdfs:subClassOf :CCSS.ELA-Literacy.W.5 ;
    rdfs:comment "Draw evidence from literary or informational texts to support analysis, reflection, and research."^^xsd:string .

:CCSS.ELA-Literacy.W.5.9.a rdf:type owl:Class ;
    prov:wasQuotedFrom <http://www.corestandards.org/ELA-Literacy/W/5/9/a/> ;
    rdfs:subClassOf :CCSS.ELA-Literacy.W.5.9 ;
    rdfs:comment "Apply grade 5 Reading standards to literature (e.g., 'Compare and contrast two or more characters, settings, or events in a story or a drama, drawing on specific details in the text [e.g., how characters interact]')."^^xsd:string .

:CCSS.ELA-Literacy.W.5.9.b rdf:type owl:Class ;
    prov:wasQuotedFrom <http://www.corestandards.org/ELA-Literacy/W/5/9/b/> ;
    rdfs:subClassOf :CCSS.ELA-Literacy.W.5.9 ;
    rdfs:comment "Apply grade 5 Reading standards to informational texts (e.g., 'Explain how an author uses reasons and evidence to support particular points in a text, identifying which reasons and evidence support which point[s]'')."^^xsd:string .

:CCSS.ELA-Literacy.W.5.10 rdf:type owl:Class ;
    prov:wasQuotedFrom <http://www.corestandards.org/ELA-Literacy/W/5/10/> ;
    rdfs:subClassOf :CCSS.ELA-Literacy.W.5 ;
    rdfs:comment "Write routinely over extended time frames (time for research, reflection, and revision) and shorter time frames (a single sitting or a day or two) for a range of discipline-specific tasks, purposes, and audiences."^^xsd:string .

:CCSS.ELA-Literacy.W.6.1 rdf:type owl:Class ;
    prov:wasQuotedFrom <http://www.corestandards.org/ELA-Literacy/W/6/1/> ;
    rdfs:subClassOf :CCSS.ELA-Literacy.W.6 ;
    rdfs:comment "Write arguments to support claims with clear reasons and relevant evidence."^^xsd:string .

:CCSS.ELA-Literacy.W.6.1.a rdf:type owl:Class ;
    prov:wasQuotedFrom <http://www.corestandards.org/ELA-Literacy/W/6/1/a/> ;
    rdfs:subClassOf :CCSS.ELA-Literacy.W.6.1 ;
    rdfs:comment "Introduce claim(s) and organize the reasons and evidence clearly."^^xsd:string .

:CCSS.ELA-Literacy.W.6.1.b rdf:type owl:Class ;
    prov:wasQuotedFrom <http://www.corestandards.org/ELA-Literacy/W/6/1/b/> ;
    rdfs:subClassOf :CCSS.ELA-Literacy.W.6.1 ;
    rdfs:comment "Support claim(s) with clear reasons and relevant evidence, using credible sources and demonstrating an understanding of the topic or text."^^xsd:string .

:CCSS.ELA-Literacy.W.6.1.c rdf:type owl:Class ;
    prov:wasQuotedFrom <http://www.corestandards.org/ELA-Literacy/W/6/1/c/> ;
    rdfs:subClassOf :CCSS.ELA-Literacy.W.6.1 ;
    rdfs:comment "Use words, phrases, and clauses to clarify the relationships among claim(s) and reasons."^^xsd:string .

:CCSS.ELA-Literacy.W.6.1.d rdf:type owl:Class ;
    prov:wasQuotedFrom <http://www.corestandards.org/ELA-Literacy/W/6/1/d/> ;
    rdfs:subClassOf :CCSS.ELA-Literacy.W.6.1 ;
    rdfs:comment "Establish and maintain a formal style."^^xsd:string .

:CCSS.ELA-Literacy.W.6.1.e rdf:type owl:Class ;
    prov:wasQuotedFrom <http://www.corestandards.org/ELA-Literacy/W/6/1/e/> ;
    rdfs:subClassOf :CCSS.ELA-Literacy.W.6.1 ;
    rdfs:comment "Provide a concluding statement or section that follows from the argument presented."^^xsd:string .

:CCSS.ELA-Literacy.W.6.2 rdf:type owl:Class ;
    prov:wasQuotedFrom <http://www.corestandards.org/ELA-Literacy/W/6/2/> ;
    rdfs:subClassOf :CCSS.ELA-Literacy.W.6 ;
    rdfs:comment "Write informative/explanatory texts to examine a topic and convey ideas, concepts, and information through the selection, organization, and analysis of relevant content."^^xsd:string .

:CCSS.ELA-Literacy.W.6.2.a rdf:type owl:Class ;
    prov:wasQuotedFrom <http://www.corestandards.org/ELA-Literacy/W/6/2/a/> ;
    rdfs:subClassOf :CCSS.ELA-Literacy.W.6.2 ;
    rdfs:comment "Introduce a topic; organize ideas, concepts, and information, using strategies such as definition, classification, comparison/contrast, and cause/effect; include formatting (e.g., headings), graphics (e.g., charts, tables), and multimedia when useful to aiding comprehension."^^xsd:string .

:CCSS.ELA-Literacy.W.6.2.b rdf:type owl:Class ;
    prov:wasQuotedFrom <http://www.corestandards.org/ELA-Literacy/W/6/2/b/> ;
    rdfs:subClassOf :CCSS.ELA-Literacy.W.6.2 ;
    rdfs:comment "Develop the topic with relevant facts, definitions, concrete details, quotations, or other information and examples."^^xsd:string .

:CCSS.ELA-Literacy.W.6.2.c rdf:type owl:Class ;
    prov:wasQuotedFrom <http://www.corestandards.org/ELA-Literacy/W/6/2/c/> ;
    rdfs:subClassOf :CCSS.ELA-Literacy.W.6.2 ;
    rdfs:comment "Use appropriate transitions to clarify the relationships among ideas and concepts."^^xsd:string .

:CCSS.ELA-Literacy.W.6.2.d rdf:type owl:Class ;
    prov:wasQuotedFrom <http://www.corestandards.org/ELA-Literacy/W/6/2/d/> ;
    rdfs:subClassOf :CCSS.ELA-Literacy.W.6.2 ;
    rdfs:comment "Use precise language and domain-specific vocabulary to inform about or explain the topic."^^xsd:string .

:CCSS.ELA-Literacy.W.6.2.e rdf:type owl:Class ;
    prov:wasQuotedFrom <http://www.corestandards.org/ELA-Literacy/W/6/2/e/> ;
    rdfs:subClassOf :CCSS.ELA-Literacy.W.6.2 ;
    rdfs:comment "Establish and maintain a formal style."^^xsd:string .

:CCSS.ELA-Literacy.W.6.2.f rdf:type owl:Class ;
    prov:wasQuotedFrom <http://www.corestandards.org/ELA-Literacy/W/6/2/f/> ;
    rdfs:subClassOf :CCSS.ELA-Literacy.W.6.2 ;
    rdfs:comment "Provide a concluding statement or section that follows from the information or explanation presented."^^xsd:string .

:CCSS.ELA-Literacy.W.6.3 rdf:type owl:Class ;
    prov:wasQuotedFrom <http://www.corestandards.org/ELA-Literacy/W/6/3/> ;
    rdfs:subClassOf :CCSS.ELA-Literacy.W.6 ;
    rdfs:comment "Write narratives to develop real or imagined experiences or events using effective technique, relevant descriptive details, and well-structured event sequences."^^xsd:string .

:CCSS.ELA-Literacy.W.6.3.a rdf:type owl:Class ;
    prov:wasQuotedFrom <http://www.corestandards.org/ELA-Literacy/W/6/3/a/> ;
    rdfs:subClassOf :CCSS.ELA-Literacy.W.6.3 ;
    rdfs:comment "Engage and orient the reader by establishing a context and introducing a narrator and/or characters; organize an event sequence that unfolds naturally and logically."^^xsd:string .

:CCSS.ELA-Literacy.W.6.3.b rdf:type owl:Class ;
    prov:wasQuotedFrom <http://www.corestandards.org/ELA-Literacy/W/6/3/b/> ;
    rdfs:subClassOf :CCSS.ELA-Literacy.W.6.3 ;
    rdfs:comment "Use narrative techniques, such as dialogue, pacing, and description, to develop experiences, events, and/or characters."^^xsd:string .

:CCSS.ELA-Literacy.W.6.3.c rdf:type owl:Class ;
    prov:wasQuotedFrom <http://www.corestandards.org/ELA-Literacy/W/6/3/c/> ;
    rdfs:subClassOf :CCSS.ELA-Literacy.W.6.3 ;
    rdfs:comment "Use a variety of transition words, phrases, and clauses to convey sequence and signal shifts from one time frame or setting to another."^^xsd:string .

:CCSS.ELA-Literacy.W.6.3.d rdf:type owl:Class ;
    prov:wasQuotedFrom <http://www.corestandards.org/ELA-Literacy/W/6/3/d/> ;
    rdfs:subClassOf :CCSS.ELA-Literacy.W.6.3 ;
    rdfs:comment "Use precise words and phrases, relevant descriptive details, and sensory language to convey experiences and events."^^xsd:string .

:CCSS.ELA-Literacy.W.6.3.e rdf:type owl:Class ;
    prov:wasQuotedFrom <http://www.corestandards.org/ELA-Literacy/W/6/3/e/> ;
    rdfs:subClassOf :CCSS.ELA-Literacy.W.6.3 ;
    rdfs:comment "Provide a conclusion that follows from the narrated experiences or events."^^xsd:string .

:CCSS.ELA-Literacy.W.6.4 rdf:type owl:Class ;
    prov:wasQuotedFrom <http://www.corestandards.org/ELA-Literacy/W/6/4/> ;
    rdfs:subClassOf :CCSS.ELA-Literacy.W.6 ;
    rdfs:comment "Produce clear and coherent writing in which the development, organization, and style are appropriate to task, purpose, and audience. (Grade-specific expectations for writing types are defined in standards 1-3 above.)"^^xsd:string .

:CCSS.ELA-Literacy.W.6.5 rdf:type owl:Class ;
    prov:wasQuotedFrom <http://www.corestandards.org/ELA-Literacy/W/6/5/> ;
    rdfs:subClassOf :CCSS.ELA-Literacy.W.6 ;
    rdfs:comment "With some guidance and support from peers and adults, develop and strengthen writing as needed by planning, revising, editing, rewriting, or trying a new approach. (Editing for conventions should demonstrate command of Language standards 1-3 up to and including grade 6 .)"^^xsd:string .

:CCSS.ELA-Literacy.W.6.6 rdf:type owl:Class ;
    prov:wasQuotedFrom <http://www.corestandards.org/ELA-Literacy/W/6/6/> ;
    rdfs:subClassOf :CCSS.ELA-Literacy.W.6 ;
    rdfs:comment "Use technology, including the Internet, to produce and publish writing as well as to interact and collaborate with others; demonstrate sufficient command of keyboarding skills to type a minimum of three pages in a single sitting."^^xsd:string .

:CCSS.ELA-Literacy.W.6.7 rdf:type owl:Class ;
    prov:wasQuotedFrom <http://www.corestandards.org/ELA-Literacy/W/6/7/> ;
    rdfs:subClassOf :CCSS.ELA-Literacy.W.6 ;
    rdfs:comment "Conduct short research projects to answer a question, drawing on several sources and refocusing the inquiry when appropriate."^^xsd:string .

:CCSS.ELA-Literacy.W.6.8 rdf:type owl:Class ;
    prov:wasQuotedFrom <http://www.corestandards.org/ELA-Literacy/W/6/8/> ;
    rdfs:subClassOf :CCSS.ELA-Literacy.W.6 ;
    rdfs:comment "Gather relevant information from multiple print and digital sources; assess the credibility of each source; and quote or paraphrase the data and conclusions of others while avoiding plagiarism and providing basic bibliographic information for sources."^^xsd:string .

:CCSS.ELA-Literacy.W.6.9 rdf:type owl:Class ;
    prov:wasQuotedFrom <http://www.corestandards.org/ELA-Literacy/W/6/9/> ;
    rdfs:subClassOf :CCSS.ELA-Literacy.W.6 ;
    rdfs:comment "Draw evidence from literary or informational texts to support analysis, reflection, and research."^^xsd:string .

:CCSS.ELA-Literacy.W.6.9.a rdf:type owl:Class ;
    prov:wasQuotedFrom <http://www.corestandards.org/ELA-Literacy/W/6/9/a/> ;
    rdfs:subClassOf :CCSS.ELA-Literacy.W.6.9 ;
    rdfs:comment "Apply grade 6 Reading standards to literature (e.g., 'Compare and contrast texts in different forms or genres [e.g., stories and poems; historical novels and fantasy stories] in terms of their approaches to similar themes and topics')."^^xsd:string .

:CCSS.ELA-Literacy.W.6.9.b rdf:type owl:Class ;
    prov:wasQuotedFrom <http://www.corestandards.org/ELA-Literacy/W/6/9/b/> ;
    rdfs:subClassOf :CCSS.ELA-Literacy.W.6.9 ;
    rdfs:comment "Apply grade 6 Reading standards to literary nonfiction (e.g., 'Trace and evaluate the argument and specific claims in a text, distinguishing claims that are supported by reasons and evidence from claims that are not')."^^xsd:string .

:CCSS.ELA-Literacy.W.6.10 rdf:type owl:Class ;
    prov:wasQuotedFrom <http://www.corestandards.org/ELA-Literacy/W/6/10/> ;
    rdfs:subClassOf :CCSS.ELA-Literacy.W.6 ;
    rdfs:comment "Write routinely over extended time frames (time for research, reflection, and revision) and shorter time frames (a single sitting or a day or two) for a range of discipline-specific tasks, purposes, and audiences."^^xsd:string .

:CCSS.ELA-Literacy.W.7.1 rdf:type owl:Class ;
    prov:wasQuotedFrom <http://www.corestandards.org/ELA-Literacy/W/7/1/> ;
    rdfs:subClassOf :CCSS.ELA-Literacy.W.7 ;
    rdfs:comment "Write arguments to support claims with clear reasons and relevant evidence."^^xsd:string .

:CCSS.ELA-Literacy.W.7.1.a rdf:type owl:Class ;
    prov:wasQuotedFrom <http://www.corestandards.org/ELA-Literacy/W/7/1/a/> ;
    rdfs:subClassOf :CCSS.ELA-Literacy.W.7.1 ;
    rdfs:comment "Introduce claim(s), acknowledge alternate or opposing claims, and organize the reasons and evidence logically."^^xsd:string .

:CCSS.ELA-Literacy.W.7.1.b rdf:type owl:Class ;
    prov:wasQuotedFrom <http://www.corestandards.org/ELA-Literacy/W/7/1/b/> ;
    rdfs:subClassOf :CCSS.ELA-Literacy.W.7.1 ;
    rdfs:comment "Support claim(s) with logical reasoning and relevant evidence, using accurate, credible sources and demonstrating an understanding of the topic or text."^^xsd:string .

:CCSS.ELA-Literacy.W.7.1.c rdf:type owl:Class ;
    prov:wasQuotedFrom <http://www.corestandards.org/ELA-Literacy/W/7/1/c/> ;
    rdfs:subClassOf :CCSS.ELA-Literacy.W.7.1 ;
    rdfs:comment "Use words, phrases, and clauses to create cohesion and clarify the relationships among claim(s), reasons, and evidence."^^xsd:string .

:CCSS.ELA-Literacy.W.7.1.d rdf:type owl:Class ;
    prov:wasQuotedFrom <http://www.corestandards.org/ELA-Literacy/W/7/1/d/> ;
    rdfs:subClassOf :CCSS.ELA-Literacy.W.7.1 ;
    rdfs:comment "Establish and maintain a formal style."^^xsd:string .

:CCSS.ELA-Literacy.W.7.1.e rdf:type owl:Class ;
    prov:wasQuotedFrom <http://www.corestandards.org/ELA-Literacy/W/7/1/e/> ;
    rdfs:subClassOf :CCSS.ELA-Literacy.W.7.1 ;
    rdfs:comment "Provide a concluding statement or section that follows from and supports the argument presented."^^xsd:string .

:CCSS.ELA-Literacy.W.7.2 rdf:type owl:Class ;
    prov:wasQuotedFrom <http://www.corestandards.org/ELA-Literacy/W/7/2/> ;
    rdfs:subClassOf :CCSS.ELA-Literacy.W.7 ;
    rdfs:comment "Write informative/explanatory texts to examine a topic and convey ideas, concepts, and information through the selection, organization, and analysis of relevant content."^^xsd:string .

:CCSS.ELA-Literacy.W.7.2.a rdf:type owl:Class ;
    prov:wasQuotedFrom <http://www.corestandards.org/ELA-Literacy/W/7/2/a/> ;
    rdfs:subClassOf :CCSS.ELA-Literacy.W.7.2 ;
    rdfs:comment "Introduce a topic clearly, previewing what is to follow; organize ideas, concepts, and information, using strategies such as definition, classification, comparison/contrast, and cause/effect; include formatting (e.g., headings), graphics (e.g., charts, tables), and multimedia when useful to aiding comprehension."^^xsd:string .

:CCSS.ELA-Literacy.W.7.2.b rdf:type owl:Class ;
    prov:wasQuotedFrom <http://www.corestandards.org/ELA-Literacy/W/7/2/b/> ;
    rdfs:subClassOf :CCSS.ELA-Literacy.W.7.2 ;
    rdfs:comment "Develop the topic with relevant facts, definitions, concrete details, quotations, or other information and examples."^^xsd:string .

:CCSS.ELA-Literacy.W.7.2.c rdf:type owl:Class ;
    prov:wasQuotedFrom <http://www.corestandards.org/ELA-Literacy/W/7/2/c/> ;
    rdfs:subClassOf :CCSS.ELA-Literacy.W.7.2 ;
    rdfs:comment "Use appropriate transitions to create cohesion and clarify the relationships among ideas and concepts."^^xsd:string .

:CCSS.ELA-Literacy.W.7.2.d rdf:type owl:Class ;
    prov:wasQuotedFrom <http://www.corestandards.org/ELA-Literacy/W/7/2/d/> ;
    rdfs:subClassOf :CCSS.ELA-Literacy.W.7.2 ;
    rdfs:comment "Use precise language and domain-specific vocabulary to inform about or explain the topic."^^xsd:string .

:CCSS.ELA-Literacy.W.7.2.e rdf:type owl:Class ;
    prov:wasQuotedFrom <http://www.corestandards.org/ELA-Literacy/W/7/2/e/> ;
    rdfs:subClassOf :CCSS.ELA-Literacy.W.7.2 ;
    rdfs:comment "Establish and maintain a formal style."^^xsd:string .

:CCSS.ELA-Literacy.W.7.2.f rdf:type owl:Class ;
    prov:wasQuotedFrom <http://www.corestandards.org/ELA-Literacy/W/7/2/f/> ;
    rdfs:subClassOf :CCSS.ELA-Literacy.W.7.2 ;
    rdfs:comment "Provide a concluding statement or section that follows from and supports the information or explanation presented."^^xsd:string .

:CCSS.ELA-Literacy.W.7.3 rdf:type owl:Class ;
    prov:wasQuotedFrom <http://www.corestandards.org/ELA-Literacy/W/7/3/> ;
    rdfs:subClassOf :CCSS.ELA-Literacy.W.7 ;
    rdfs:comment "Write narratives to develop real or imagined experiences or events using effective technique, relevant descriptive details, and well-structured event sequences."^^xsd:string .

:CCSS.ELA-Literacy.W.7.3.a rdf:type owl:Class ;
    prov:wasQuotedFrom <http://www.corestandards.org/ELA-Literacy/W/7/3/a/> ;
    rdfs:subClassOf :CCSS.ELA-Literacy.W.7.3 ;
    rdfs:comment "Engage and orient the reader by establishing a context and point of view and introducing a narrator and/or characters; organize an event sequence that unfolds naturally and logically."^^xsd:string .

:CCSS.ELA-Literacy.W.7.3.b rdf:type owl:Class ;
    prov:wasQuotedFrom <http://www.corestandards.org/ELA-Literacy/W/7/3/b/> ;
    rdfs:subClassOf :CCSS.ELA-Literacy.W.7.3 ;
    rdfs:comment "Use narrative techniques, such as dialogue, pacing, and description, to develop experiences, events, and/or characters."^^xsd:string .

:CCSS.ELA-Literacy.W.7.3.c rdf:type owl:Class ;
    prov:wasQuotedFrom <http://www.corestandards.org/ELA-Literacy/W/7/3/c/> ;
    rdfs:subClassOf :CCSS.ELA-Literacy.W.7.3 ;
    rdfs:comment "Use a variety of transition words, phrases, and clauses to convey sequence and signal shifts from one time frame or setting to another."^^xsd:string .

:CCSS.ELA-Literacy.W.7.3.d rdf:type owl:Class ;
    prov:wasQuotedFrom <http://www.corestandards.org/ELA-Literacy/W/7/3/d/> ;
    rdfs:subClassOf :CCSS.ELA-Literacy.W.7.3 ;
    rdfs:comment "Use precise words and phrases, relevant descriptive details, and sensory language to capture the action and convey experiences and events."^^xsd:string .

:CCSS.ELA-Literacy.W.7.3.e rdf:type owl:Class ;
    prov:wasQuotedFrom <http://www.corestandards.org/ELA-Literacy/W/7/3/e/> ;
    rdfs:subClassOf :CCSS.ELA-Literacy.W.7.3 ;
    rdfs:comment "Provide a conclusion that follows from and reflects on the narrated experiences or events."^^xsd:string .

:CCSS.ELA-Literacy.W.7.4 rdf:type owl:Class ;
    prov:wasQuotedFrom <http://www.corestandards.org/ELA-Literacy/W/7/4/> ;
    rdfs:subClassOf :CCSS.ELA-Literacy.W.7 ;
    rdfs:comment "Produce clear and coherent writing in which the development, organization, and style are appropriate to task, purpose, and audience. (Grade-specific expectations for writing types are defined in standards 1-3 above.)"^^xsd:string .

:CCSS.ELA-Literacy.W.7.5 rdf:type owl:Class ;
    prov:wasQuotedFrom <http://www.corestandards.org/ELA-Literacy/W/7/5/> ;
    rdfs:subClassOf :CCSS.ELA-Literacy.W.7 ;
    rdfs:comment "With some guidance and support from peers and adults, develop and strengthen writing as needed by planning, revising, editing, rewriting, or trying a new approach, focusing on how well purpose and audience have been addressed. (Editing for conventions should demonstrate command of Language standards 1-3 up to and including grade 7 .)"^^xsd:string .

:CCSS.ELA-Literacy.W.7.6 rdf:type owl:Class ;
    prov:wasQuotedFrom <http://www.corestandards.org/ELA-Literacy/W/7/6/> ;
    rdfs:subClassOf :CCSS.ELA-Literacy.W.7 ;
    rdfs:comment "Use technology, including the Internet, to produce and publish writing and link to and cite sources as well as to interact and collaborate with others, including linking to and citing sources."^^xsd:string .

:CCSS.ELA-Literacy.W.7.7 rdf:type owl:Class ;
    prov:wasQuotedFrom <http://www.corestandards.org/ELA-Literacy/W/7/7/> ;
    rdfs:subClassOf :CCSS.ELA-Literacy.W.7 ;
    rdfs:comment "Conduct short research projects to answer a question, drawing on several sources and generating additional related, focused questions for further research and investigation."^^xsd:string .

:CCSS.ELA-Literacy.W.7.8 rdf:type owl:Class ;
    prov:wasQuotedFrom <http://www.corestandards.org/ELA-Literacy/W/7/8/> ;
    rdfs:subClassOf :CCSS.ELA-Literacy.W.7 ;
    rdfs:comment "Gather relevant information from multiple print and digital sources, using search terms effectively; assess the credibility and accuracy of each source; and quote or paraphrase the data and conclusions of others while avoiding plagiarism and following a standard format for citation."^^xsd:string .

:CCSS.ELA-Literacy.W.7.9 rdf:type owl:Class ;
    prov:wasQuotedFrom <http://www.corestandards.org/ELA-Literacy/W/7/9/> ;
    rdfs:subClassOf :CCSS.ELA-Literacy.W.7 ;
    rdfs:comment "Draw evidence from literary or informational texts to support analysis, reflection, and research."^^xsd:string .

:CCSS.ELA-Literacy.W.7.9.a rdf:type owl:Class ;
    prov:wasQuotedFrom <http://www.corestandards.org/ELA-Literacy/W/7/9/a/> ;
    rdfs:subClassOf :CCSS.ELA-Literacy.W.7.9 ;
    rdfs:comment "Apply grade 7 Reading standards to literature (e.g., 'Compare and contrast a fictional portrayal of a time, place, or character and a historical account of the same period as a means of understanding how authors of fiction use or alter history')."^^xsd:string .

:CCSS.ELA-Literacy.W.7.9.b rdf:type owl:Class ;
    prov:wasQuotedFrom <http://www.corestandards.org/ELA-Literacy/W/7/9/b/> ;
    rdfs:subClassOf :CCSS.ELA-Literacy.W.7.9 ;
    rdfs:comment "Apply grade 7 Reading standards to literary nonfiction (e.g. 'Trace and evaluate the argument and specific claims in a text, assessing whether the reasoning is sound and the evidence is relevant and sufficient to support the claims')."^^xsd:string .

:CCSS.ELA-Literacy.W.7.10 rdf:type owl:Class ;
    prov:wasQuotedFrom <http://www.corestandards.org/ELA-Literacy/W/7/10/> ;
    rdfs:subClassOf :CCSS.ELA-Literacy.W.7 ;
    rdfs:comment "Write routinely over extended time frames (time for research, reflection, and revision) and shorter time frames (a single sitting or a day or two) for a range of discipline-specific tasks, purposes, and audiences."^^xsd:string .

:CCSS.ELA-Literacy.W.8.1 rdf:type owl:Class ;
    prov:wasQuotedFrom <http://www.corestandards.org/ELA-Literacy/W/8/1/> ;
    rdfs:subClassOf :CCSS.ELA-Literacy.W.8 ;
    rdfs:comment "Write arguments to support claims with clear reasons and relevant evidence"^^xsd:string .

:CCSS.ELA-Literacy.W.8.1.a rdf:type owl:Class ;
    prov:wasQuotedFrom <http://www.corestandards.org/ELA-Literacy/W/8/1/a/> ;
    rdfs:subClassOf :CCSS.ELA-Literacy.W.8.1 ;
    rdfs:comment "Introduce claim(s), acknowledge and distinguish the claim(s) from alternate or opposing claims, and organize the reasons and evidence logically."^^xsd:string .

:CCSS.ELA-Literacy.W.8.1.b rdf:type owl:Class ;
    prov:wasQuotedFrom <http://www.corestandards.org/ELA-Literacy/W/8/1/b/> ;
    rdfs:subClassOf :CCSS.ELA-Literacy.W.8.1 ;
    rdfs:comment "Support claim(s) with logical reasoning and relevant evidence, using accurate, credible sources and demonstrating an understanding of the topic or text."^^xsd:string .

:CCSS.ELA-Literacy.W.8.1.c rdf:type owl:Class ;
    prov:wasQuotedFrom <http://www.corestandards.org/ELA-Literacy/W/8/1/c/> ;
    rdfs:subClassOf :CCSS.ELA-Literacy.W.8.1 ;
    rdfs:comment "Use words, phrases, and clauses to create cohesion and clarify the relationships among claim(s), counterclaims, reasons, and evidence."^^xsd:string .

:CCSS.ELA-Literacy.W.8.1.d rdf:type owl:Class ;
    prov:wasQuotedFrom <http://www.corestandards.org/ELA-Literacy/W/8/1/d/> ;
    rdfs:subClassOf :CCSS.ELA-Literacy.W.8.1 ;
    rdfs:comment "Establish and maintain a formal style."^^xsd:string .

:CCSS.ELA-Literacy.W.8.1.e rdf:type owl:Class ;
    prov:wasQuotedFrom <http://www.corestandards.org/ELA-Literacy/W/8/1/e/> ;
    rdfs:subClassOf :CCSS.ELA-Literacy.W.8.1 ;
    rdfs:comment "Provide a concluding statement or section that follows from and supports the argument presented."^^xsd:string .

:CCSS.ELA-Literacy.W.8.2 rdf:type owl:Class ;
    prov:wasQuotedFrom <http://www.corestandards.org/ELA-Literacy/W/8/2/> ;
    rdfs:subClassOf :CCSS.ELA-Literacy.W.8 ;
    rdfs:comment "Write informative/explanatory texts to examine a topic and convey ideas, concepts, and information through the selection, organization, and analysis of relevant content."^^xsd:string .

:CCSS.ELA-Literacy.W.8.2.a rdf:type owl:Class ;
    prov:wasQuotedFrom <http://www.corestandards.org/ELA-Literacy/W/8/2/a/> ;
    rdfs:subClassOf :CCSS.ELA-Literacy.W.8.2 ;
    rdfs:comment "Introduce a topic clearly, previewing what is to follow; organize ideas, concepts, and information into broader categories; include formatting (e.g., headings), graphics (e.g., charts, tables), and multimedia when useful to aiding comprehension."^^xsd:string .

:CCSS.ELA-Literacy.W.8.2.b rdf:type owl:Class ;
    prov:wasQuotedFrom <http://www.corestandards.org/ELA-Literacy/W/8/2/b/> ;
    rdfs:subClassOf :CCSS.ELA-Literacy.W.8.2 ;
    rdfs:comment "Develop the topic with relevant, well-chosen facts, definitions, concrete details, quotations, or other information and examples."^^xsd:string .

:CCSS.ELA-Literacy.W.8.2.c rdf:type owl:Class ;
    prov:wasQuotedFrom <http://www.corestandards.org/ELA-Literacy/W/8/2/c/> ;
    rdfs:subClassOf :CCSS.ELA-Literacy.W.8.2 ;
    rdfs:comment "Use appropriate and varied transitions to create cohesion and clarify the relationships among ideas and concepts."^^xsd:string .

:CCSS.ELA-Literacy.W.8.2.d rdf:type owl:Class ;
    prov:wasQuotedFrom <http://www.corestandards.org/ELA-Literacy/W/8/2/d/> ;
    rdfs:subClassOf :CCSS.ELA-Literacy.W.8.2 ;
    rdfs:comment "Use precise language and domain-specific vocabulary to inform about or explain the topic."^^xsd:string .

:CCSS.ELA-Literacy.W.8.2.e rdf:type owl:Class ;
    prov:wasQuotedFrom <http://www.corestandards.org/ELA-Literacy/W/8/2/e/> ;
    rdfs:subClassOf :CCSS.ELA-Literacy.W.8.2 ;
    rdfs:comment "Establish and maintain a formal style."^^xsd:string .

:CCSS.ELA-Literacy.W.8.2.f rdf:type owl:Class ;
    prov:wasQuotedFrom <http://www.corestandards.org/ELA-Literacy/W/8/2/f/> ;
    rdfs:subClassOf :CCSS.ELA-Literacy.W.8.2 ;
    rdfs:comment "Provide a concluding statement or section that follows from and supports the information or explanation presented."^^xsd:string .

:CCSS.ELA-Literacy.W.8.3 rdf:type owl:Class ;
    prov:wasQuotedFrom <http://www.corestandards.org/ELA-Literacy/W/8/3/> ;
    rdfs:subClassOf :CCSS.ELA-Literacy.W.8 ;
    rdfs:comment "Write narratives to develop real or imagined experiences or events using effective technique, relevant descriptive details, and well-structured event sequences."^^xsd:string .

:CCSS.ELA-Literacy.W.8.3.a rdf:type owl:Class ;
    prov:wasQuotedFrom <http://www.corestandards.org/ELA-Literacy/W/8/3/a/> ;
    rdfs:subClassOf :CCSS.ELA-Literacy.W.8.3 ;
    rdfs:comment "Engage and orient the reader by establishing a context and point of view and introducing a narrator and/or characters; organize an event sequence that unfolds naturally and logically."^^xsd:string .

:CCSS.ELA-Literacy.W.8.3.b rdf:type owl:Class ;
    prov:wasQuotedFrom <http://www.corestandards.org/ELA-Literacy/W/8/3/b/> ;
    rdfs:subClassOf :CCSS.ELA-Literacy.W.8.3 ;
    rdfs:comment "Use narrative techniques, such as dialogue, pacing, description, and reflection, to develop experiences, events, and/or characters."^^xsd:string .

:CCSS.ELA-Literacy.W.8.3.c rdf:type owl:Class ;
    prov:wasQuotedFrom <http://www.corestandards.org/ELA-Literacy/W/8/3/c/> ;
    rdfs:subClassOf :CCSS.ELA-Literacy.W.8.3 ;
    rdfs:comment "Use a variety of transition words, phrases, and clauses to convey sequence, signal shifts from one time frame or setting to another, and show the relationships among experiences and events."^^xsd:string .

:CCSS.ELA-Literacy.W.8.3.d rdf:type owl:Class ;
    prov:wasQuotedFrom <http://www.corestandards.org/ELA-Literacy/W/8/3/d/> ;
    rdfs:subClassOf :CCSS.ELA-Literacy.W.8.3 ;
    rdfs:comment "Use precise words and phrases, relevant descriptive details, and sensory language to capture the action and convey experiences and events."^^xsd:string .

:CCSS.ELA-Literacy.W.8.3.e rdf:type owl:Class ;
    prov:wasQuotedFrom <http://www.corestandards.org/ELA-Literacy/W/8/3/e/> ;
    rdfs:subClassOf :CCSS.ELA-Literacy.W.8.3 ;
    rdfs:comment "Provide a conclusion that follows from and reflects on the narrated experiences or events."^^xsd:string .

:CCSS.ELA-Literacy.W.8.4 rdf:type owl:Class ;
    prov:wasQuotedFrom <http://www.corestandards.org/ELA-Literacy/W/8/4/> ;
    rdfs:subClassOf :CCSS.ELA-Literacy.W.8 ;
    rdfs:comment "Produce clear and coherent writing in which the development, organization, and style are appropriate to task, purpose, and audience. (Grade-specific expectations for writing types are defined in standards 1-3 above.)"^^xsd:string .

:CCSS.ELA-Literacy.W.8.5 rdf:type owl:Class ;
    prov:wasQuotedFrom <http://www.corestandards.org/ELA-Literacy/W/8/5/> ;
    rdfs:subClassOf :CCSS.ELA-Literacy.W.8 ;
    rdfs:comment "With some guidance and support from peers and adults, develop and strengthen writing as needed by planning, revising, editing, rewriting, or trying a new approach, focusing on how well purpose and audience have been addressed. (Editing for conventions should demonstrate command of Language standards 1-3 up to and including grade 8 .)"^^xsd:string .

:CCSS.ELA-Literacy.W.8.6 rdf:type owl:Class ;
    prov:wasQuotedFrom <http://www.corestandards.org/ELA-Literacy/W/8/6/> ;
    rdfs:subClassOf :CCSS.ELA-Literacy.W.8 ;
    rdfs:comment "Use technology, including the Internet, to produce and publish writing and present the relationships between information and ideas efficiently as well as to interact and collaborate with others."^^xsd:string .

:CCSS.ELA-Literacy.W.8.7 rdf:type owl:Class ;
    prov:wasQuotedFrom <http://www.corestandards.org/ELA-Literacy/W/8/7/> ;
    rdfs:subClassOf :CCSS.ELA-Literacy.W.8 ;
    rdfs:comment "Conduct short research projects to answer a question (including a self-generated question), drawing on several sources and generating additional related, focused questions that allow for multiple avenues of exploration."^^xsd:string .

:CCSS.ELA-Literacy.W.8.8 rdf:type owl:Class ;
    prov:wasQuotedFrom <http://www.corestandards.org/ELA-Literacy/W/8/8/> ;
    rdfs:subClassOf :CCSS.ELA-Literacy.W.8 ;
    rdfs:comment "Gather relevant information from multiple print and digital sources, using search terms effectively; assess the credibility and accuracy of each source; and quote or paraphrase the data and conclusions of others while avoiding plagiarism and following a standard format for citation."^^xsd:string .

:CCSS.ELA-Literacy.W.8.9 rdf:type owl:Class ;
    prov:wasQuotedFrom <http://www.corestandards.org/ELA-Literacy/W/8/9/> ;
    rdfs:subClassOf :CCSS.ELA-Literacy.W.8 ;
    rdfs:comment "Draw evidence from literary or informational texts to support analysis, reflection, and research."^^xsd:string .

:CCSS.ELA-Literacy.W.8.9.a rdf:type owl:Class ;
    prov:wasQuotedFrom <http://www.corestandards.org/ELA-Literacy/W/8/9/a/> ;
    rdfs:subClassOf :CCSS.ELA-Literacy.W.8.9 ;
    rdfs:comment "Apply grade 8 Reading standards to literature (e.g., 'Analyze how a modern work of fiction draws on themes, patterns of events, or character types from myths, traditional stories, or religious works such as the Bible, including describing how the material is rendered new')."^^xsd:string .

:CCSS.ELA-Literacy.W.8.9.b rdf:type owl:Class ;
    prov:wasQuotedFrom <http://www.corestandards.org/ELA-Literacy/W/8/9/b/> ;
    rdfs:subClassOf :CCSS.ELA-Literacy.W.8.9 ;
    rdfs:comment "Apply grade 8 Reading standards to literary nonfiction (e.g., 'Delineate and evaluate the argument and specific claims in a text, assessing whether the reasoning is sound and the evidence is relevant and sufficient; recognize when irrelevant evidence is introduced')."^^xsd:string .

:CCSS.ELA-Literacy.W.8.10 rdf:type owl:Class ;
    prov:wasQuotedFrom <http://www.corestandards.org/ELA-Literacy/W/8/10/> ;
    rdfs:subClassOf :CCSS.ELA-Literacy.W.8 ;
    rdfs:comment "Write routinely over extended time frames (time for research, reflection, and revision) and shorter time frames (a single sitting or a day or two) for a range of discipline-specific tasks, purposes, and audiences."^^xsd:string .

:CCSS.ELA-Literacy.W.9-10.1 rdf:type owl:Class ;
    prov:wasQuotedFrom <http://www.corestandards.org/ELA-Literacy/W/9-10/1/> ;
    rdfs:subClassOf :CCSS.ELA-Literacy.W.9-10 ;
    rdfs:comment "Write arguments to support claims in an analysis of substantive topics or texts, using valid reasoning and relevant and sufficient evidence."^^xsd:string .

:CCSS.ELA-Literacy.W.9-10.1.a rdf:type owl:Class ;
    prov:wasQuotedFrom <http://www.corestandards.org/ELA-Literacy/W/9-10/1/a/> ;
    rdfs:subClassOf :CCSS.ELA-Literacy.W.9-10.1 ;
    rdfs:comment "Introduce precise claim(s), distinguish the claim(s) from alternate or opposing claims, and create an organization that establishes clear relationships among claim(s), counterclaims, reasons, and evidence."^^xsd:string .

:CCSS.ELA-Literacy.W.9-10.1.b rdf:type owl:Class ;
    prov:wasQuotedFrom <http://www.corestandards.org/ELA-Literacy/W/9-10/1/b/> ;
    rdfs:subClassOf :CCSS.ELA-Literacy.W.9-10.1 ;
    rdfs:comment "Develop claim(s) and counterclaims fairly, supplying evidence for each while pointing out the strengths and limitations of both in a manner that anticipates the audience's knowledge level and concerns."^^xsd:string .

:CCSS.ELA-Literacy.W.9-10.1.c rdf:type owl:Class ;
    prov:wasQuotedFrom <http://www.corestandards.org/ELA-Literacy/W/9-10/1/c/> ;
    rdfs:subClassOf :CCSS.ELA-Literacy.W.9-10.1 ;
    rdfs:comment "Use words, phrases, and clauses to link the major sections of the text, create cohesion, and clarify the relationships between claim(s) and reasons, between reasons and evidence, and between claim(s) and counterclaims."^^xsd:string .

:CCSS.ELA-Literacy.W.9-10.1.d rdf:type owl:Class ;
    prov:wasQuotedFrom <http://www.corestandards.org/ELA-Literacy/W/9-10/1/d/> ;
    rdfs:subClassOf :CCSS.ELA-Literacy.W.9-10.1 ;
    rdfs:comment "Establish and maintain a formal style and objective tone while attending to the norms and conventions of the discipline in which they are writing."^^xsd:string .

:CCSS.ELA-Literacy.W.9-10.1.e rdf:type owl:Class ;
    prov:wasQuotedFrom <http://www.corestandards.org/ELA-Literacy/W/9-10/1/e/> ;
    rdfs:subClassOf :CCSS.ELA-Literacy.W.9-10.1 ;
    rdfs:comment "Provide a concluding statement or section that follows from and supports the argument presented."^^xsd:string .

:CCSS.ELA-Literacy.W.9-10.2 rdf:type owl:Class ;
    prov:wasQuotedFrom <http://www.corestandards.org/ELA-Literacy/W/9-10/2/> ;
    rdfs:subClassOf :CCSS.ELA-Literacy.W.9-10 ;
    rdfs:comment "Write informative/explanatory texts to examine and convey complex ideas, concepts, and information clearly and accurately through the effective selection, organization, and analysis of content."^^xsd:string .

:CCSS.ELA-Literacy.W.9-10.2.a rdf:type owl:Class ;
    prov:wasQuotedFrom <http://www.corestandards.org/ELA-Literacy/W/9-10/2/a/> ;
    rdfs:subClassOf :CCSS.ELA-Literacy.W.9-10.2 ;
    rdfs:comment "Introduce a topic; organize complex ideas, concepts, and information to make important connections and distinctions; include formatting (e.g., headings), graphics (e.g., figures, tables), and multimedia when useful to aiding comprehension."^^xsd:string .

:CCSS.ELA-Literacy.W.9-10.2.b rdf:type owl:Class ;
    prov:wasQuotedFrom <http://www.corestandards.org/ELA-Literacy/W/9-10/2/b/> ;
    rdfs:subClassOf :CCSS.ELA-Literacy.W.9-10.2 ;
    rdfs:comment "Develop the topic with well-chosen, relevant, and sufficient facts, extended definitions, concrete details, quotations, or other information and examples appropriate to the audience's knowledge of the topic."^^xsd:string .

:CCSS.ELA-Literacy.W.9-10.2.c rdf:type owl:Class ;
    prov:wasQuotedFrom <http://www.corestandards.org/ELA-Literacy/W/9-10/2/c/> ;
    rdfs:subClassOf :CCSS.ELA-Literacy.W.9-10.2 ;
    rdfs:comment "Use appropriate and varied transitions to link the major sections of the text, create cohesion, and clarify the relationships among complex ideas and concepts."^^xsd:string .

:CCSS.ELA-Literacy.W.9-10.2.d rdf:type owl:Class ;
    prov:wasQuotedFrom <http://www.corestandards.org/ELA-Literacy/W/9-10/2/d/> ;
    rdfs:subClassOf :CCSS.ELA-Literacy.W.9-10.2 ;
    rdfs:comment "Use precise language and domain-specific vocabulary to manage the complexity of the topic."^^xsd:string .

:CCSS.ELA-Literacy.W.9-10.2.e rdf:type owl:Class ;
    prov:wasQuotedFrom <http://www.corestandards.org/ELA-Literacy/W/9-10/2/e/> ;
    rdfs:subClassOf :CCSS.ELA-Literacy.W.9-10.2 ;
    rdfs:comment "Establish and maintain a formal style and objective tone while attending to the norms and conventions of the discipline in which they are writing."^^xsd:string .

:CCSS.ELA-Literacy.W.9-10.2.f rdf:type owl:Class ;
    prov:wasQuotedFrom <http://www.corestandards.org/ELA-Literacy/W/9-10/2/f/> ;
    rdfs:subClassOf :CCSS.ELA-Literacy.W.9-10.2 ;
    rdfs:comment "Provide a concluding statement or section that follows from and supports the information or explanation presented (e.g., articulating implications or the significance of the topic)."^^xsd:string .

:CCSS.ELA-Literacy.W.9-10.3 rdf:type owl:Class ;
    prov:wasQuotedFrom <http://www.corestandards.org/ELA-Literacy/W/9-10/3/> ;
    rdfs:subClassOf :CCSS.ELA-Literacy.W.9-10 ;
    rdfs:comment "Write narratives to develop real or imagined experiences or events using effective technique, well-chosen details, and well-structured event sequences."^^xsd:string .

:CCSS.ELA-Literacy.W.9-10.3.a rdf:type owl:Class ;
    prov:wasQuotedFrom <http://www.corestandards.org/ELA-Literacy/W/9-10/3/a/> ;
    rdfs:subClassOf :CCSS.ELA-Literacy.W.9-10.3 ;
    rdfs:comment "Engage and orient the reader by setting out a problem, situation, or observation, establishing one or multiple point(s) of view, and introducing a narrator and/or characters; create a smooth progression of experiences or events."^^xsd:string .

:CCSS.ELA-Literacy.W.9-10.3.b rdf:type owl:Class ;
    prov:wasQuotedFrom <http://www.corestandards.org/ELA-Literacy/W/9-10/3/b/> ;
    rdfs:subClassOf :CCSS.ELA-Literacy.W.9-10.3 ;
    rdfs:comment "Use narrative techniques, such as dialogue, pacing, description, reflection, and multiple plot lines, to develop experiences, events, and/or characters."^^xsd:string .

:CCSS.ELA-Literacy.W.9-10.3.c rdf:type owl:Class ;
    prov:wasQuotedFrom <http://www.corestandards.org/ELA-Literacy/W/9-10/3/c/> ;
    rdfs:subClassOf :CCSS.ELA-Literacy.W.9-10.3 ;
    rdfs:comment "Use a variety of techniques to sequence events so that they build on one another to create a coherent whole."^^xsd:string .

:CCSS.ELA-Literacy.W.9-10.3.d rdf:type owl:Class ;
    prov:wasQuotedFrom <http://www.corestandards.org/ELA-Literacy/W/9-10/3/d/> ;
    rdfs:subClassOf :CCSS.ELA-Literacy.W.9-10.3 ;
    rdfs:comment "Use precise words and phrases, telling details, and sensory language to convey a vivid picture of the experiences, events, setting, and/or characters."^^xsd:string .

:CCSS.ELA-Literacy.W.9-10.3.e rdf:type owl:Class ;
    prov:wasQuotedFrom <http://www.corestandards.org/ELA-Literacy/W/9-10/3/e/> ;
    rdfs:subClassOf :CCSS.ELA-Literacy.W.9-10.3 ;
    rdfs:comment "Provide a conclusion that follows from and reflects on what is experienced, observed, or resolved over the course of the narrative."^^xsd:string .

:CCSS.ELA-Literacy.W.9-10.4 rdf:type owl:Class ;
    prov:wasQuotedFrom <http://www.corestandards.org/ELA-Literacy/W/9-10/4/> ;
    rdfs:subClassOf :CCSS.ELA-Literacy.W.9-10 ;
    rdfs:comment "Produce clear and coherent writing in which the development, organization, and style are appropriate to task, purpose, and audience. (Grade-specific expectations for writing types are defined in standards 1-3 above.)"^^xsd:string .

:CCSS.ELA-Literacy.W.9-10.5 rdf:type owl:Class ;
    prov:wasQuotedFrom <http://www.corestandards.org/ELA-Literacy/W/9-10/5/> ;
    rdfs:subClassOf :CCSS.ELA-Literacy.W.9-10 ;
    rdfs:comment "Develop and strengthen writing as needed by planning, revising, editing, rewriting, or trying a new approach, focusing on addressing what is most significant for a specific purpose and audience. (Editing for conventions should demonstrate command of Language standards 1-3 up to and including grades 9-10 .)"^^xsd:string .

:CCSS.ELA-Literacy.W.9-10.6 rdf:type owl:Class ;
    prov:wasQuotedFrom <http://www.corestandards.org/ELA-Literacy/W/9-10/6/> ;
    rdfs:subClassOf :CCSS.ELA-Literacy.W.9-10 ;
    rdfs:comment "Use technology, including the Internet, to produce, publish, and update individual or shared writing products, taking advantage of technology's capacity to link to other information and to display information flexibly and dynamically."^^xsd:string .

:CCSS.ELA-Literacy.W.9-10.7 rdf:type owl:Class ;
    prov:wasQuotedFrom <http://www.corestandards.org/ELA-Literacy/W/9-10/7/> ;
    rdfs:subClassOf :CCSS.ELA-Literacy.W.9-10 ;
    rdfs:comment "Conduct short as well as more sustained research projects to answer a question (including a self-generated question) or solve a problem; narrow or broaden the inquiry when appropriate; synthesize multiple sources on the subject, demonstrating understanding of the subject under investigation."^^xsd:string .

:CCSS.ELA-Literacy.W.9-10.8 rdf:type owl:Class ;
    prov:wasQuotedFrom <http://www.corestandards.org/ELA-Literacy/W/9-10/8/> ;
    rdfs:subClassOf :CCSS.ELA-Literacy.W.9-10 ;
    rdfs:comment "Gather relevant information from multiple authoritative print and digital sources, using advanced searches effectively; assess the usefulness of each source in answering the research question; integrate information into the text selectively to maintain the flow of ideas, avoiding plagiarism and following a standard format for citation."^^xsd:string .

:CCSS.ELA-Literacy.W.9-10.9 rdf:type owl:Class ;
    prov:wasQuotedFrom <http://www.corestandards.org/ELA-Literacy/W/9-10/9/> ;
    rdfs:subClassOf :CCSS.ELA-Literacy.W.9-10 ;
    rdfs:comment "Draw evidence from literary or informational texts to support analysis, reflection, and research."^^xsd:string .

:CCSS.ELA-Literacy.W.9-10.9.a rdf:type owl:Class ;
    prov:wasQuotedFrom <http://www.corestandards.org/ELA-Literacy/W/9-10/9/a/> ;
    rdfs:subClassOf :CCSS.ELA-Literacy.W.9-10.9 ;
    rdfs:comment "Apply grades 9-10 Reading standards to literature (e.g., 'Analyze how an author draws on and transforms source material in a specific work [e.g., how Shakespeare treats a theme or topic from Ovid or the Bible or how a later author draws on a play by Shakespeare]')."^^xsd:string .

:CCSS.ELA-Literacy.W.9-10.9.b rdf:type owl:Class ;
    prov:wasQuotedFrom <http://www.corestandards.org/ELA-Literacy/W/9-10/9/b/> ;
    rdfs:subClassOf :CCSS.ELA-Literacy.W.9-10.9 ;
    rdfs:comment "Apply grades 9-10 Reading standards to literary nonfiction (e.g., 'Delineate and evaluate the argument and specific claims in a text, assessing whether the reasoning is valid and the evidence is relevant and sufficient; identify false statements and fallacious reasoning')."^^xsd:string .

:CCSS.ELA-Literacy.W.9-10.10 rdf:type owl:Class ;
    prov:wasQuotedFrom <http://www.corestandards.org/ELA-Literacy/W/9-10/10/> ;
    rdfs:subClassOf :CCSS.ELA-Literacy.W.9-10 ;
    rdfs:comment "Write routinely over extended time frames (time for research, reflection, and revision) and shorter time frames (a single sitting or a day or two) for a range of tasks, purposes, and audiences."^^xsd:string .

:CCSS.ELA-Literacy.W.11-12.1 rdf:type owl:Class ;
    prov:wasQuotedFrom <http://www.corestandards.org/ELA-Literacy/W/11-12/1/> ;
    rdfs:subClassOf :CCSS.ELA-Literacy.W.11-12 ;
    rdfs:comment "Write arguments to support claims in an analysis of substantive topics or texts, using valid reasoning and relevant and sufficient evidence."^^xsd:string .

:CCSS.ELA-Literacy.W.11-12.1.a rdf:type owl:Class ;
    prov:wasQuotedFrom <http://www.corestandards.org/ELA-Literacy/W/11-12/1/a/> ;
    rdfs:subClassOf :CCSS.ELA-Literacy.W.11-12.1 ;
    rdfs:comment "Introduce precise, knowledgeable claim(s), establish the significance of the claim(s), distinguish the claim(s) from alternate or opposing claims, and create an organization that logically sequences claim(s), counterclaims, reasons, and evidence."^^xsd:string .

:CCSS.ELA-Literacy.W.11-12.1.b rdf:type owl:Class ;
    prov:wasQuotedFrom <http://www.corestandards.org/ELA-Literacy/W/11-12/1/b/> ;
    rdfs:subClassOf :CCSS.ELA-Literacy.W.11-12.1 ;
    rdfs:comment "Develop claim(s) and counterclaims fairly and thoroughly, supplying the most relevant evidence for each while pointing out the strengths and limitations of both in a manner that anticipates the audience's knowledge level, concerns, values, and possible biases."^^xsd:string .

:CCSS.ELA-Literacy.W.11-12.1.c rdf:type owl:Class ;
    prov:wasQuotedFrom <http://www.corestandards.org/ELA-Literacy/W/11-12/1/c/> ;
    rdfs:subClassOf :CCSS.ELA-Literacy.W.11-12.1 ;
    rdfs:comment "Use words, phrases, and clauses as well as varied syntax to link the major sections of the text, create cohesion, and clarify the relationships between claim(s) and reasons, between reasons and evidence, and between claim(s) and counterclaims."^^xsd:string .

:CCSS.ELA-Literacy.W.11-12.1.d rdf:type owl:Class ;
    prov:wasQuotedFrom <http://www.corestandards.org/ELA-Literacy/W/11-12/1/d/> ;
    rdfs:subClassOf :CCSS.ELA-Literacy.W.11-12.1 ;
    rdfs:comment "Establish and maintain a formal style and objective tone while attending to the norms and conventions of the discipline in which they are writing."^^xsd:string .

:CCSS.ELA-Literacy.W.11-12.1.e rdf:type owl:Class ;
    prov:wasQuotedFrom <http://www.corestandards.org/ELA-Literacy/W/11-12/1/e/> ;
    rdfs:subClassOf :CCSS.ELA-Literacy.W.11-12.1 ;
    rdfs:comment "Provide a concluding statement or section that follows from and supports the argument presented."^^xsd:string .

:CCSS.ELA-Literacy.W.11-12.2 rdf:type owl:Class ;
    prov:wasQuotedFrom <http://www.corestandards.org/ELA-Literacy/W/11-12/2/> ;
    rdfs:subClassOf :CCSS.ELA-Literacy.W.11-12 ;
    rdfs:comment "Write informative/explanatory texts to examine and convey complex ideas, concepts, and information clearly and accurately through the effective selection, organization, and analysis of content."^^xsd:string .

:CCSS.ELA-Literacy.W.11-12.2.a rdf:type owl:Class ;
    prov:wasQuotedFrom <http://www.corestandards.org/ELA-Literacy/W/11-12/2/a/> ;
    rdfs:subClassOf :CCSS.ELA-Literacy.W.11-12.2 ;
    rdfs:comment "Introduce a topic; organize complex ideas, concepts, and information so that each new element builds on that which precedes it to create a unified whole; include formatting (e.g., headings), graphics (e.g., figures, tables), and multimedia when useful to aiding comprehension."^^xsd:string .

:CCSS.ELA-Literacy.W.11-12.2.b rdf:type owl:Class ;
    prov:wasQuotedFrom <http://www.corestandards.org/ELA-Literacy/W/11-12/2/b/> ;
    rdfs:subClassOf :CCSS.ELA-Literacy.W.11-12.2 ;
    rdfs:comment "Develop the topic thoroughly by selecting the most significant and relevant facts, extended definitions, concrete details, quotations, or other information and examples appropriate to the audience's knowledge of the topic."^^xsd:string .

:CCSS.ELA-Literacy.W.11-12.2.c rdf:type owl:Class ;
    prov:wasQuotedFrom <http://www.corestandards.org/ELA-Literacy/W/11-12/2/c/> ;
    rdfs:subClassOf :CCSS.ELA-Literacy.W.11-12.2 ;
    rdfs:comment "Use appropriate and varied transitions and syntax to link the major sections of the text, create cohesion, and clarify the relationships among complex ideas and concepts."^^xsd:string .

:CCSS.ELA-Literacy.W.11-12.2.d rdf:type owl:Class ;
    prov:wasQuotedFrom <http://www.corestandards.org/ELA-Literacy/W/11-12/2/d/> ;
    rdfs:subClassOf :CCSS.ELA-Literacy.W.11-12.2 ;
    rdfs:comment "Use precise language, domain-specific vocabulary, and techniques such as metaphor, simile, and analogy to manage the complexity of the topic."^^xsd:string .

:CCSS.ELA-Literacy.W.11-12.2.e rdf:type owl:Class ;
    prov:wasQuotedFrom <http://www.corestandards.org/ELA-Literacy/W/11-12/2/e/> ;
    rdfs:subClassOf :CCSS.ELA-Literacy.W.11-12.2 ;
    rdfs:comment "Establish and maintain a formal style and objective tone while attending to the norms and conventions of the discipline in which they are writing."^^xsd:string .

:CCSS.ELA-Literacy.W.11-12.2.f rdf:type owl:Class ;
    prov:wasQuotedFrom <http://www.corestandards.org/ELA-Literacy/W/11-12/2/f/> ;
    rdfs:subClassOf :CCSS.ELA-Literacy.W.11-12.2 ;
    rdfs:comment "Provide a concluding statement or section that follows from and supports the information or explanation presented (e.g., articulating implications or the significance of the topic)."^^xsd:string .

:CCSS.ELA-Literacy.W.11-12.3 rdf:type owl:Class ;
    prov:wasQuotedFrom <http://www.corestandards.org/ELA-Literacy/W/11-12/3/> ;
    rdfs:subClassOf :CCSS.ELA-Literacy.W.11-12 ;
    rdfs:comment "Write narratives to develop real or imagined experiences or events using effective technique, well-chosen details, and well-structured event sequences."^^xsd:string .

:CCSS.ELA-Literacy.W.11-12.3.a rdf:type owl:Class ;
    prov:wasQuotedFrom <http://www.corestandards.org/ELA-Literacy/W/11-12/3/a/> ;
    rdfs:subClassOf :CCSS.ELA-Literacy.W.11-12.3 ;
    rdfs:comment "Engage and orient the reader by setting out a problem, situation, or observation and its significance, establishing one or multiple point(s) of view, and introducing a narrator and/or characters; create a smooth progression of experiences or events."^^xsd:string .

:CCSS.ELA-Literacy.W.11-12.3.b rdf:type owl:Class ;
    prov:wasQuotedFrom <http://www.corestandards.org/ELA-Literacy/W/11-12/3/b/> ;
    rdfs:subClassOf :CCSS.ELA-Literacy.W.11-12.3 ;
    rdfs:comment "Use narrative techniques, such as dialogue, pacing, description, reflection, and multiple plot lines, to develop experiences, events, and/or characters."^^xsd:string .

:CCSS.ELA-Literacy.W.11-12.3.c rdf:type owl:Class ;
    prov:wasQuotedFrom <http://www.corestandards.org/ELA-Literacy/W/11-12/3/c/> ;
    rdfs:subClassOf :CCSS.ELA-Literacy.W.11-12.3 ;
    rdfs:comment "Use a variety of techniques to sequence events so that they build on one another to create a coherent whole and build toward a particular tone and outcome (e.g., a sense of mystery, suspense, growth, or resolution)."^^xsd:string .

:CCSS.ELA-Literacy.W.11-12.3.d rdf:type owl:Class ;
    prov:wasQuotedFrom <http://www.corestandards.org/ELA-Literacy/W/11-12/3/d/> ;
    rdfs:subClassOf :CCSS.ELA-Literacy.W.11-12.3 ;
    rdfs:comment "Use precise words and phrases, telling details, and sensory language to convey a vivid picture of the experiences, events, setting, and/or characters."^^xsd:string .

:CCSS.ELA-Literacy.W.11-12.3.e rdf:type owl:Class ;
    prov:wasQuotedFrom <http://www.corestandards.org/ELA-Literacy/W/11-12/3/e/> ;
    rdfs:subClassOf :CCSS.ELA-Literacy.W.11-12.3 ;
    rdfs:comment "Provide a conclusion that follows from and reflects on what is experienced, observed, or resolved over the course of the narrative."^^xsd:string .

:CCSS.ELA-Literacy.W.11-12.4 rdf:type owl:Class ;
    prov:wasQuotedFrom <http://www.corestandards.org/ELA-Literacy/W/11-12/4/> ;
    rdfs:subClassOf :CCSS.ELA-Literacy.W.11-12 ;
    rdfs:comment "Produce clear and coherent writing in which the development, organization, and style are appropriate to task, purpose, and audience. (Grade-specific expectations for writing types are defined in standards 1-3 above.)"^^xsd:string .

:CCSS.ELA-Literacy.W.11-12.5 rdf:type owl:Class ;
    prov:wasQuotedFrom <http://www.corestandards.org/ELA-Literacy/W/11-12/5/> ;
    rdfs:subClassOf :CCSS.ELA-Literacy.W.11-12 ;
    rdfs:comment "Develop and strengthen writing as needed by planning, revising, editing, rewriting, or trying a new approach, focusing on addressing what is most significant for a specific purpose and audience. (Editing for conventions should demonstrate command of Language standards 1-3 up to and including grades 11-12 .)"^^xsd:string .

:CCSS.ELA-Literacy.W.11-12.6 rdf:type owl:Class ;
    prov:wasQuotedFrom <http://www.corestandards.org/ELA-Literacy/W/11-12/6/> ;
    rdfs:subClassOf :CCSS.ELA-Literacy.W.11-12 ;
    rdfs:comment "Use technology, including the Internet, to produce, publish, and update individual or shared writing products in response to ongoing feedback, including new arguments or information."^^xsd:string .

:CCSS.ELA-Literacy.W.11-12.7 rdf:type owl:Class ;
    prov:wasQuotedFrom <http://www.corestandards.org/ELA-Literacy/W/11-12/7/> ;
    rdfs:subClassOf :CCSS.ELA-Literacy.W.11-12 ;
    rdfs:comment "Conduct short as well as more sustained research projects to answer a question (including a self-generated question) or solve a problem; narrow or broaden the inquiry when appropriate; synthesize multiple sources on the subject, demonstrating understanding of the subject under investigation."^^xsd:string .

:CCSS.ELA-Literacy.W.11-12.8 rdf:type owl:Class ;
    prov:wasQuotedFrom <http://www.corestandards.org/ELA-Literacy/W/11-12/8/> ;
    rdfs:subClassOf :CCSS.ELA-Literacy.W.11-12 ;
    rdfs:comment "Gather relevant information from multiple authoritative print and digital sources, using advanced searches effectively; assess the strengths and limitations of each source in terms of the task, purpose, and audience; integrate information into the text selectively to maintain the flow of ideas, avoiding plagiarism and overreliance on any one source and following a standard format for citation."^^xsd:string .

:CCSS.ELA-Literacy.W.11-12.9 rdf:type owl:Class ;
    prov:wasQuotedFrom <http://www.corestandards.org/ELA-Literacy/W/11-12/9/> ;
    rdfs:subClassOf :CCSS.ELA-Literacy.W.11-12 ;
    rdfs:comment "Draw evidence from literary or informational texts to support analysis, reflection, and research."^^xsd:string .

:CCSS.ELA-Literacy.W.11-12.9.a rdf:type owl:Class ;
    prov:wasQuotedFrom <http://www.corestandards.org/ELA-Literacy/W/11-12/9/a/> ;
    rdfs:subClassOf :CCSS.ELA-Literacy.W.11-12.9 ;
    rdfs:comment "Apply grades 11-12 Reading standards to literature (e.g., 'Demonstrate knowledge of eighteenth-, nineteenth- and early-twentieth-century foundational works of American literature, including how two or more texts from the same period treat similar themes or topics')."^^xsd:string .

:CCSS.ELA-Literacy.W.11-12.9.b rdf:type owl:Class ;
    prov:wasQuotedFrom <http://www.corestandards.org/ELA-Literacy/W/11-12/9/b/> ;
    rdfs:subClassOf :CCSS.ELA-Literacy.W.11-12.9 ;
    rdfs:comment "Apply grades 11-12 Reading standards to literary nonfiction (e.g., 'Delineate and evaluate the reasoning in seminal U.S. texts, including the application of constitutional principles and use of legal reasoning [e.g., in U.S. Supreme Court Case majority opinions and dissents] and the premises, purposes, and arguments in works of public advocacy [e.g., The Federalist, presidential addresses]')."^^xsd:string .

:CCSS.ELA-Literacy.W.11-12.10 rdf:type owl:Class ;
    prov:wasQuotedFrom <http://www.corestandards.org/ELA-Literacy/W/11-12/10/> ;
    rdfs:subClassOf :CCSS.ELA-Literacy.W.11-12 ;
    rdfs:comment "Write routinely over extended time frames (time for research, reflection, and revision) and shorter time frames (a single sitting or a day or two) for a range of tasks, purposes, and audiences."^^xsd:string .

:CCSS.ELA-Literacy.SL.K.1 rdf:type owl:Class ;
    prov:wasQuotedFrom <http://www.corestandards.org/ELA-Literacy/SL/K/1/> ;
    rdfs:subClassOf :CCSS.ELA-Literacy.SL.K ;
    rdfs:comment "Participate in collaborative conversations with diverse partners about kindergarten topics and texts with peers and adults in small and larger groups."^^xsd:string .

:CCSS.ELA-Literacy.SL.K.1.a rdf:type owl:Class ;
    prov:wasQuotedFrom <http://www.corestandards.org/ELA-Literacy/SL/K/1/a/> ;
    rdfs:subClassOf :CCSS.ELA-Literacy.SL.K.1 ;
    rdfs:comment "Follow agreed-upon rules for discussions (e.g., listening to others and taking turns speaking about the topics and texts under discussion)."^^xsd:string .

:CCSS.ELA-Literacy.SL.K.1.b rdf:type owl:Class ;
    prov:wasQuotedFrom <http://www.corestandards.org/ELA-Literacy/SL/K/1/b/> ;
    rdfs:subClassOf :CCSS.ELA-Literacy.SL.K.1 ;
    rdfs:comment "Continue a conversation through multiple exchanges."^^xsd:string .

:CCSS.ELA-Literacy.SL.K.2 rdf:type owl:Class ;
    prov:wasQuotedFrom <http://www.corestandards.org/ELA-Literacy/SL/K/2/> ;
    rdfs:subClassOf :CCSS.ELA-Literacy.SL.K ;
    rdfs:comment "Confirm understanding of a text read aloud or information presented orally or through other media by asking and answering questions about key details and requesting clarification if something is not understood."^^xsd:string .

:CCSS.ELA-Literacy.SL.K.3 rdf:type owl:Class ;
    prov:wasQuotedFrom <http://www.corestandards.org/ELA-Literacy/SL/K/3/> ;
    rdfs:subClassOf :CCSS.ELA-Literacy.SL.K ;
    rdfs:comment "Ask and answer questions in order to seek help, get information, or clarify something that is not understood."^^xsd:string .

:CCSS.ELA-Literacy.SL.K.4 rdf:type owl:Class ;
    prov:wasQuotedFrom <http://www.corestandards.org/ELA-Literacy/SL/K/4/> ;
    rdfs:subClassOf :CCSS.ELA-Literacy.SL.K ;
    rdfs:comment "Describe familiar people, places, things, and events and, with prompting and support, provide additional detail."^^xsd:string .

:CCSS.ELA-Literacy.SL.K.5 rdf:type owl:Class ;
    prov:wasQuotedFrom <http://www.corestandards.org/ELA-Literacy/SL/K/5/> ;
    rdfs:subClassOf :CCSS.ELA-Literacy.SL.K ;
    rdfs:comment "Add drawings or other visual displays to descriptions as desired to provide additional detail."^^xsd:string .

:CCSS.ELA-Literacy.SL.K.6 rdf:type owl:Class ;
    prov:wasQuotedFrom <http://www.corestandards.org/ELA-Literacy/SL/K/6/> ;
    rdfs:subClassOf :CCSS.ELA-Literacy.SL.K ;
    rdfs:comment "Speak audibly and express thoughts, feelings, and ideas clearly."^^xsd:string .

:CCSS.ELA-Literacy.SL.1.1 rdf:type owl:Class ;
    prov:wasQuotedFrom <http://www.corestandards.org/ELA-Literacy/SL/1/1/> ;
    rdfs:subClassOf :CCSS.ELA-Literacy.SL.1 ;
    rdfs:comment "Participate in collaborative conversations with diverse partners about grade 1 topics and texts with peers and adults in small and larger groups."^^xsd:string .

:CCSS.ELA-Literacy.SL.1.1.a rdf:type owl:Class ;
    prov:wasQuotedFrom <http://www.corestandards.org/ELA-Literacy/SL/1/1/a/> ;
    rdfs:subClassOf :CCSS.ELA-Literacy.SL.1.1 ;
    rdfs:comment "Follow agreed-upon rules for discussions (e.g., listening to others with care, speaking one at a time about the topics and texts under discussion)."^^xsd:string .

:CCSS.ELA-Literacy.SL.1.1.b rdf:type owl:Class ;
    prov:wasQuotedFrom <http://www.corestandards.org/ELA-Literacy/SL/1/1/b/> ;
    rdfs:subClassOf :CCSS.ELA-Literacy.SL.1.1 ;
    rdfs:comment "Build on others' talk in conversations by responding to the comments of others through multiple exchanges."^^xsd:string .

:CCSS.ELA-Literacy.SL.1.1.c rdf:type owl:Class ;
    prov:wasQuotedFrom <http://www.corestandards.org/ELA-Literacy/SL/1/1/c/> ;
    rdfs:subClassOf :CCSS.ELA-Literacy.SL.1.1 ;
    rdfs:comment "Ask questions to clear up any confusion about the topics and texts under discussion."^^xsd:string .

:CCSS.ELA-Literacy.SL.1.2 rdf:type owl:Class ;
    prov:wasQuotedFrom <http://www.corestandards.org/ELA-Literacy/SL/1/2/> ;
    rdfs:subClassOf :CCSS.ELA-Literacy.SL.1 ;
    rdfs:comment "Ask and answer questions about key details in a text read aloud or information presented orally or through other media."^^xsd:string .

:CCSS.ELA-Literacy.SL.1.3 rdf:type owl:Class ;
    prov:wasQuotedFrom <http://www.corestandards.org/ELA-Literacy/SL/1/3/> ;
    rdfs:subClassOf :CCSS.ELA-Literacy.SL.1 ;
    rdfs:comment "Ask and answer questions about what a speaker says in order to gather additional information or clarify something that is not understood."^^xsd:string .

:CCSS.ELA-Literacy.SL.1.4 rdf:type owl:Class ;
    prov:wasQuotedFrom <http://www.corestandards.org/ELA-Literacy/SL/1/4/> ;
    rdfs:subClassOf :CCSS.ELA-Literacy.SL.1 ;
    rdfs:comment "Describe people, places, things, and events with relevant details, expressing ideas and feelings clearly."^^xsd:string .

:CCSS.ELA-Literacy.SL.1.5 rdf:type owl:Class ;
    prov:wasQuotedFrom <http://www.corestandards.org/ELA-Literacy/SL/1/5/> ;
    rdfs:subClassOf :CCSS.ELA-Literacy.SL.1 ;
    rdfs:comment "Add drawings or other visual displays to descriptions when appropriate to clarify ideas, thoughts, and feelings."^^xsd:string .

:CCSS.ELA-Literacy.SL.1.6 rdf:type owl:Class ;
    prov:wasQuotedFrom <http://www.corestandards.org/ELA-Literacy/SL/1/6/> ;
    rdfs:subClassOf :CCSS.ELA-Literacy.SL.1 ;
    rdfs:comment "Produce complete sentences when appropriate to task and situation. (See grade 1 Language standards 1 and 3  for specific expectations.)"^^xsd:string .

:CCSS.ELA-Literacy.SL.2.1 rdf:type owl:Class ;
    prov:wasQuotedFrom <http://www.corestandards.org/ELA-Literacy/SL/2/1/> ;
    rdfs:subClassOf :CCSS.ELA-Literacy.SL.2 ;
    rdfs:comment "Participate in collaborative conversations with diverse partners about grade 2 topics and texts with peers and adults in small and larger groups."^^xsd:string .

:CCSS.ELA-Literacy.SL.2.1.a rdf:type owl:Class ;
    prov:wasQuotedFrom <http://www.corestandards.org/ELA-Literacy/SL/2/1/a/> ;
    rdfs:subClassOf :CCSS.ELA-Literacy.SL.2.1 ;
    rdfs:comment "Follow agreed-upon rules for discussions (e.g., gaining the floor in respectful ways, listening to others with care, speaking one at a time about the topics and texts under discussion)."^^xsd:string .

:CCSS.ELA-Literacy.SL.2.1.b rdf:type owl:Class ;
    prov:wasQuotedFrom <http://www.corestandards.org/ELA-Literacy/SL/2/1/b/> ;
    rdfs:subClassOf :CCSS.ELA-Literacy.SL.2.1 ;
    rdfs:comment "Build on others' talk in conversations by linking their comments to the remarks of others."^^xsd:string .

:CCSS.ELA-Literacy.SL.2.1.c rdf:type owl:Class ;
    prov:wasQuotedFrom <http://www.corestandards.org/ELA-Literacy/SL/2/1/c/> ;
    rdfs:subClassOf :CCSS.ELA-Literacy.SL.2.1 ;
    rdfs:comment "Ask for clarification and further explanation as needed about the topics and texts under discussion."^^xsd:string .

:CCSS.ELA-Literacy.SL.2.2 rdf:type owl:Class ;
    prov:wasQuotedFrom <http://www.corestandards.org/ELA-Literacy/SL/2/2/> ;
    rdfs:subClassOf :CCSS.ELA-Literacy.SL.2 ;
    rdfs:comment "Recount or describe key ideas or details from a text read aloud or information presented orally or through other media."^^xsd:string .

:CCSS.ELA-Literacy.SL.2.3 rdf:type owl:Class ;
    prov:wasQuotedFrom <http://www.corestandards.org/ELA-Literacy/SL/2/3/> ;
    rdfs:subClassOf :CCSS.ELA-Literacy.SL.2 ;
    rdfs:comment "Ask and answer questions about what a speaker says in order to clarify comprehension, gather additional information, or deepen understanding of a topic or issue."^^xsd:string .

:CCSS.ELA-Literacy.SL.2.4 rdf:type owl:Class ;
    prov:wasQuotedFrom <http://www.corestandards.org/ELA-Literacy/SL/2/4/> ;
    rdfs:subClassOf :CCSS.ELA-Literacy.SL.2 ;
    rdfs:comment "Tell a story or recount an experience with appropriate facts and relevant, descriptive details, speaking audibly in coherent sentences."^^xsd:string .

:CCSS.ELA-Literacy.SL.2.5 rdf:type owl:Class ;
    prov:wasQuotedFrom <http://www.corestandards.org/ELA-Literacy/SL/2/5/> ;
    rdfs:subClassOf :CCSS.ELA-Literacy.SL.2 ;
    rdfs:comment "Create audio recordings of stories or poems; add drawings or other visual displays to stories or recounts of experiences when appropriate to clarify ideas, thoughts, and feelings."^^xsd:string .

:CCSS.ELA-Literacy.SL.2.6 rdf:type owl:Class ;
    prov:wasQuotedFrom <http://www.corestandards.org/ELA-Literacy/SL/2/6/> ;
    rdfs:subClassOf :CCSS.ELA-Literacy.SL.2 ;
    rdfs:comment "Produce complete sentences when appropriate to task and situation in order to provide requested detail or clarification. (See grade 2 Language standards 1 and 3  for specific expectations.)"^^xsd:string .

:CCSS.ELA-Literacy.SL.3.1 rdf:type owl:Class ;
    prov:wasQuotedFrom <http://www.corestandards.org/ELA-Literacy/SL/3/1/> ;
    rdfs:subClassOf :CCSS.ELA-Literacy.SL.3 ;
    rdfs:comment "Engage effectively in a range of collaborative discussions (one-on-one, in groups, and teacher-led) with diverse partners on grade 3 topics and texts, building on others' ideas and expressing their own clearly."^^xsd:string .

:CCSS.ELA-Literacy.SL.3.1.a rdf:type owl:Class ;
    prov:wasQuotedFrom <http://www.corestandards.org/ELA-Literacy/SL/3/1/a/> ;
    rdfs:subClassOf :CCSS.ELA-Literacy.SL.3.1 ;
    rdfs:comment "Come to discussions prepared, having read or studied required material; explicitly draw on that preparation and other information known about the topic to explore ideas under discussion."^^xsd:string .

:CCSS.ELA-Literacy.SL.3.1.b rdf:type owl:Class ;
    prov:wasQuotedFrom <http://www.corestandards.org/ELA-Literacy/SL/3/1/b/> ;
    rdfs:subClassOf :CCSS.ELA-Literacy.SL.3.1 ;
    rdfs:comment "Follow agreed-upon rules for discussions (e.g., gaining the floor in respectful ways, listening to others with care, speaking one at a time about the topics and texts under discussion)."^^xsd:string .

:CCSS.ELA-Literacy.SL.3.1.c rdf:type owl:Class ;
    prov:wasQuotedFrom <http://www.corestandards.org/ELA-Literacy/SL/3/1/c/> ;
    rdfs:subClassOf :CCSS.ELA-Literacy.SL.3.1 ;
    rdfs:comment "Ask questions to check understanding of information presented, stay on topic, and link their comments to the remarks of others."^^xsd:string .

:CCSS.ELA-Literacy.SL.3.1.d rdf:type owl:Class ;
    prov:wasQuotedFrom <http://www.corestandards.org/ELA-Literacy/SL/3/1/d/> ;
    rdfs:subClassOf :CCSS.ELA-Literacy.SL.3.1 ;
    rdfs:comment "Explain their own ideas and understanding in light of the discussion."^^xsd:string .

:CCSS.ELA-Literacy.SL.3.2 rdf:type owl:Class ;
    prov:wasQuotedFrom <http://www.corestandards.org/ELA-Literacy/SL/3/2/> ;
    rdfs:subClassOf :CCSS.ELA-Literacy.SL.3 ;
    rdfs:comment "Determine the main ideas and supporting details of a text read aloud or information presented in diverse media and formats, including visually, quantitatively, and orally."^^xsd:string .

:CCSS.ELA-Literacy.SL.3.3 rdf:type owl:Class ;
    prov:wasQuotedFrom <http://www.corestandards.org/ELA-Literacy/SL/3/3/> ;
    rdfs:subClassOf :CCSS.ELA-Literacy.SL.3 ;
    rdfs:comment "Ask and answer questions about information from a speaker, offering appropriate elaboration and detail."^^xsd:string .

:CCSS.ELA-Literacy.SL.3.4 rdf:type owl:Class ;
    prov:wasQuotedFrom <http://www.corestandards.org/ELA-Literacy/SL/3/4/> ;
    rdfs:subClassOf :CCSS.ELA-Literacy.SL.3 ;
    rdfs:comment "Report on a topic or text, tell a story, or recount an experience with appropriate facts and relevant, descriptive details, speaking clearly at an understandable pace."^^xsd:string .

:CCSS.ELA-Literacy.SL.3.5 rdf:type owl:Class ;
    prov:wasQuotedFrom <http://www.corestandards.org/ELA-Literacy/SL/3/5/> ;
    rdfs:subClassOf :CCSS.ELA-Literacy.SL.3 ;
    rdfs:comment "Create engaging audio recordings of stories or poems that demonstrate fluid reading at an understandable pace; add visual displays when appropriate to emphasize or enhance certain facts or details."^^xsd:string .

:CCSS.ELA-Literacy.SL.3.6 rdf:type owl:Class ;
    prov:wasQuotedFrom <http://www.corestandards.org/ELA-Literacy/SL/3/6/> ;
    rdfs:subClassOf :CCSS.ELA-Literacy.SL.3 ;
    rdfs:comment "Speak in complete sentences when appropriate to task and situation in order to provide requested detail or clarification. (See grade 3 Language standards 1 and 3  for specific expectations.)"^^xsd:string .

:CCSS.ELA-Literacy.SL.4.1 rdf:type owl:Class ;
    prov:wasQuotedFrom <http://www.corestandards.org/ELA-Literacy/SL/4/1/> ;
    rdfs:subClassOf :CCSS.ELA-Literacy.SL.4 ;
    rdfs:comment "Engage effectively in a range of collaborative discussions (one-on-one, in groups, and teacher-led) with diverse partners on grade 4 topics and texts, building on others' ideas and expressing their own clearly."^^xsd:string .

:CCSS.ELA-Literacy.SL.4.1.a rdf:type owl:Class ;
    prov:wasQuotedFrom <http://www.corestandards.org/ELA-Literacy/SL/4/1/a/> ;
    rdfs:subClassOf :CCSS.ELA-Literacy.SL.4.1 ;
    rdfs:comment "Come to discussions prepared, having read or studied required material; explicitly draw on that preparation and other information known about the topic to explore ideas under discussion."^^xsd:string .

:CCSS.ELA-Literacy.SL.4.1.b rdf:type owl:Class ;
    prov:wasQuotedFrom <http://www.corestandards.org/ELA-Literacy/SL/4/1/b/> ;
    rdfs:subClassOf :CCSS.ELA-Literacy.SL.4.1 ;
    rdfs:comment "Follow agreed-upon rules for discussions and carry out assigned roles."^^xsd:string .

:CCSS.ELA-Literacy.SL.4.1.c rdf:type owl:Class ;
    prov:wasQuotedFrom <http://www.corestandards.org/ELA-Literacy/SL/4/1/c/> ;
    rdfs:subClassOf :CCSS.ELA-Literacy.SL.4.1 ;
    rdfs:comment "Pose and respond to specific questions to clarify or follow up on information, and make comments that contribute to the discussion and link to the remarks of others."^^xsd:string .

:CCSS.ELA-Literacy.SL.4.1.d rdf:type owl:Class ;
    prov:wasQuotedFrom <http://www.corestandards.org/ELA-Literacy/SL/4/1/d/> ;
    rdfs:subClassOf :CCSS.ELA-Literacy.SL.4.1 ;
    rdfs:comment "Review the key ideas expressed and explain their own ideas and understanding in light of the discussion."^^xsd:string .

:CCSS.ELA-Literacy.SL.4.2 rdf:type owl:Class ;
    prov:wasQuotedFrom <http://www.corestandards.org/ELA-Literacy/SL/4/2/> ;
    rdfs:subClassOf :CCSS.ELA-Literacy.SL.4 ;
    rdfs:comment "Paraphrase portions of a text read aloud or information presented in diverse media and formats, including visually, quantitatively, and orally."^^xsd:string .

:CCSS.ELA-Literacy.SL.4.3 rdf:type owl:Class ;
    prov:wasQuotedFrom <http://www.corestandards.org/ELA-Literacy/SL/4/3/> ;
    rdfs:subClassOf :CCSS.ELA-Literacy.SL.4 ;
    rdfs:comment "Identify the reasons and evidence a speaker provides to support particular points."^^xsd:string .

:CCSS.ELA-Literacy.SL.4.4 rdf:type owl:Class ;
    prov:wasQuotedFrom <http://www.corestandards.org/ELA-Literacy/SL/4/4/> ;
    rdfs:subClassOf :CCSS.ELA-Literacy.SL.4 ;
    rdfs:comment "Report on a topic or text, tell a story, or recount an experience in an organized manner, using appropriate facts and relevant, descriptive details to support main ideas or themes; speak clearly at an understandable pace."^^xsd:string .

:CCSS.ELA-Literacy.SL.4.5 rdf:type owl:Class ;
    prov:wasQuotedFrom <http://www.corestandards.org/ELA-Literacy/SL/4/5/> ;
    rdfs:subClassOf :CCSS.ELA-Literacy.SL.4 ;
    rdfs:comment "Add audio recordings and visual displays to presentations when appropriate to enhance the development of main ideas or themes."^^xsd:string .

:CCSS.ELA-Literacy.SL.4.6 rdf:type owl:Class ;
    prov:wasQuotedFrom <http://www.corestandards.org/ELA-Literacy/SL/4/6/> ;
    rdfs:subClassOf :CCSS.ELA-Literacy.SL.4 ;
    rdfs:comment "Differentiate between contexts that call for formal English (e.g., presenting ideas) and situations where informal discourse is appropriate (e.g., small-group discussion); use formal English when appropriate to task and situation. (See grade 4 Language standards 1  for specific expectations.)"^^xsd:string .

:CCSS.ELA-Literacy.SL.5.1 rdf:type owl:Class ;
    prov:wasQuotedFrom <http://www.corestandards.org/ELA-Literacy/SL/5/1/> ;
    rdfs:subClassOf :CCSS.ELA-Literacy.SL.5 ;
    rdfs:comment "Engage effectively in a range of collaborative discussions (one-on-one, in groups, and teacher-led) with diverse partners on grade 5 topics and texts, building on others' ideas and expressing their own clearly."^^xsd:string .

:CCSS.ELA-Literacy.SL.5.1.a rdf:type owl:Class ;
    prov:wasQuotedFrom <http://www.corestandards.org/ELA-Literacy/SL/5/1/a/> ;
    rdfs:subClassOf :CCSS.ELA-Literacy.SL.5.1 ;
    rdfs:comment "Come to discussions prepared, having read or studied required material; explicitly draw on that preparation and other information known about the topic to explore ideas under discussion."^^xsd:string .

:CCSS.ELA-Literacy.SL.5.1.b rdf:type owl:Class ;
    prov:wasQuotedFrom <http://www.corestandards.org/ELA-Literacy/SL/5/1/b/> ;
    rdfs:subClassOf :CCSS.ELA-Literacy.SL.5.1 ;
    rdfs:comment "Follow agreed-upon rules for discussions and carry out assigned roles."^^xsd:string .

:CCSS.ELA-Literacy.SL.5.1.c rdf:type owl:Class ;
    prov:wasQuotedFrom <http://www.corestandards.org/ELA-Literacy/SL/5/1/c/> ;
    rdfs:subClassOf :CCSS.ELA-Literacy.SL.5.1 ;
    rdfs:comment "Pose and respond to specific questions by making comments that contribute to the discussion and elaborate on the remarks of others."^^xsd:string .

:CCSS.ELA-Literacy.SL.5.1.d rdf:type owl:Class ;
    prov:wasQuotedFrom <http://www.corestandards.org/ELA-Literacy/SL/5/1/d/> ;
    rdfs:subClassOf :CCSS.ELA-Literacy.SL.5.1 ;
    rdfs:comment "Review the key ideas expressed and draw conclusions in light of information and knowledge gained from the discussions."^^xsd:string .

:CCSS.ELA-Literacy.SL.5.2 rdf:type owl:Class ;
    prov:wasQuotedFrom <http://www.corestandards.org/ELA-Literacy/SL/5/2/> ;
    rdfs:subClassOf :CCSS.ELA-Literacy.SL.5 ;
    rdfs:comment "Summarize a written text read aloud or information presented in diverse media and formats, including visually, quantitatively, and orally."^^xsd:string .

:CCSS.ELA-Literacy.SL.5.3 rdf:type owl:Class ;
    prov:wasQuotedFrom <http://www.corestandards.org/ELA-Literacy/SL/5/3/> ;
    rdfs:subClassOf :CCSS.ELA-Literacy.SL.5 ;
    rdfs:comment "Summarize the points a speaker makes and explain how each claim is supported by reasons and evidence."^^xsd:string .

:CCSS.ELA-Literacy.SL.5.4 rdf:type owl:Class ;
    prov:wasQuotedFrom <http://www.corestandards.org/ELA-Literacy/SL/5/4/> ;
    rdfs:subClassOf :CCSS.ELA-Literacy.SL.5 ;
    rdfs:comment "Report on a topic or text or present an opinion, sequencing ideas logically and using appropriate facts and relevant, descriptive details to support main ideas or themes; speak clearly at an understandable pace."^^xsd:string .

:CCSS.ELA-Literacy.SL.5.5 rdf:type owl:Class ;
    prov:wasQuotedFrom <http://www.corestandards.org/ELA-Literacy/SL/5/5/> ;
    rdfs:subClassOf :CCSS.ELA-Literacy.SL.5 ;
    rdfs:comment "Include multimedia components (e.g., graphics, sound) and visual displays in presentations when appropriate to enhance the development of main ideas or themes."^^xsd:string .

:CCSS.ELA-Literacy.SL.5.6 rdf:type owl:Class ;
    prov:wasQuotedFrom <http://www.corestandards.org/ELA-Literacy/SL/5/6/> ;
    rdfs:subClassOf :CCSS.ELA-Literacy.SL.5 ;
    rdfs:comment "Adapt speech to a variety of contexts and tasks, using formal English when appropriate to task and situation. (See grade 5 Language standards 1 and
3  for specific expectations.)"^^xsd:string .

:CCSS.ELA-Literacy.SL.6.1 rdf:type owl:Class ;
    prov:wasQuotedFrom <http://www.corestandards.org/ELA-Literacy/SL/6/1/> ;
    rdfs:subClassOf :CCSS.ELA-Literacy.SL.6 ;
    rdfs:comment "Engage effectively in a range of collaborative discussions (one-on-one, in groups, and teacher-led) with diverse partners on grade 6 topics, texts, and issues, building on others' ideas and expressing their own clearly."^^xsd:string .

:CCSS.ELA-Literacy.SL.6.1.a rdf:type owl:Class ;
    prov:wasQuotedFrom <http://www.corestandards.org/ELA-Literacy/SL/6/1/a/> ;
    rdfs:subClassOf :CCSS.ELA-Literacy.SL.6.1 ;
    rdfs:comment "Come to discussions prepared, having read or studied required material; explicitly draw on that preparation by referring to evidence on the topic, text, or issue to probe and reflect on ideas under discussion."^^xsd:string .

:CCSS.ELA-Literacy.SL.6.1.b rdf:type owl:Class ;
    prov:wasQuotedFrom <http://www.corestandards.org/ELA-Literacy/SL/6/1/b/> ;
    rdfs:subClassOf :CCSS.ELA-Literacy.SL.6.1 ;
    rdfs:comment "Follow rules for collegial discussions, set specific goals and deadlines, and define individual roles as needed."^^xsd:string .

:CCSS.ELA-Literacy.SL.6.1.c rdf:type owl:Class ;
    prov:wasQuotedFrom <http://www.corestandards.org/ELA-Literacy/SL/6/1/c/> ;
    rdfs:subClassOf :CCSS.ELA-Literacy.SL.6.1 ;
    rdfs:comment "Pose and respond to specific questions with elaboration and detail by making comments that contribute to the topic, text, or issue under discussion."^^xsd:string .

:CCSS.ELA-Literacy.SL.6.1.d rdf:type owl:Class ;
    prov:wasQuotedFrom <http://www.corestandards.org/ELA-Literacy/SL/6/1/d/> ;
    rdfs:subClassOf :CCSS.ELA-Literacy.SL.6.1 ;
    rdfs:comment "Review the key ideas expressed and demonstrate understanding of multiple perspectives through reflection and paraphrasing."^^xsd:string .

:CCSS.ELA-Literacy.SL.6.2 rdf:type owl:Class ;
    prov:wasQuotedFrom <http://www.corestandards.org/ELA-Literacy/SL/6/2/> ;
    rdfs:subClassOf :CCSS.ELA-Literacy.SL.6 ;
    rdfs:comment "Interpret information presented in diverse media and formats (e.g., visually, quantitatively, orally) and explain how it contributes to a topic, text, or issue under study."^^xsd:string .

:CCSS.ELA-Literacy.SL.6.3 rdf:type owl:Class ;
    prov:wasQuotedFrom <http://www.corestandards.org/ELA-Literacy/SL/6/3/> ;
    rdfs:subClassOf :CCSS.ELA-Literacy.SL.6 ;
    rdfs:comment "Delineate a speaker's argument and specific claims, distinguishing claims that are supported by reasons and evidence from claims that are not."^^xsd:string .

:CCSS.ELA-Literacy.SL.6.4 rdf:type owl:Class ;
    prov:wasQuotedFrom <http://www.corestandards.org/ELA-Literacy/SL/6/4/> ;
    rdfs:subClassOf :CCSS.ELA-Literacy.SL.6 ;
    rdfs:comment "Present claims and findings, sequencing ideas logically and using pertinent descriptions, facts, and details to accentuate main ideas or themes; use appropriate eye contact, adequate volume, and clear pronunciation."^^xsd:string .

:CCSS.ELA-Literacy.SL.6.5 rdf:type owl:Class ;
    prov:wasQuotedFrom <http://www.corestandards.org/ELA-Literacy/SL/6/5/> ;
    rdfs:subClassOf :CCSS.ELA-Literacy.SL.6 ;
    rdfs:comment "Include multimedia components (e.g., graphics, images, music, sound) and visual displays in presentations to clarify information."^^xsd:string .

:CCSS.ELA-Literacy.SL.6.6 rdf:type owl:Class ;
    prov:wasQuotedFrom <http://www.corestandards.org/ELA-Literacy/SL/6/6/> ;
    rdfs:subClassOf :CCSS.ELA-Literacy.SL.6 ;
    rdfs:comment "Adapt speech to a variety of contexts and tasks, demonstrating command of formal English when indicated or appropriate. (See grade 6 Language standards 1 and 3  for specific expectations.)"^^xsd:string .

:CCSS.ELA-Literacy.SL.7.1 rdf:type owl:Class ;
    prov:wasQuotedFrom <http://www.corestandards.org/ELA-Literacy/SL/7/1/> ;
    rdfs:subClassOf :CCSS.ELA-Literacy.SL.7 ;
    rdfs:comment "Engage effectively in a range of collaborative discussions (one-on-one, in groups, and teacher-led) with diverse partners on grade 7 topics, texts, and issues, building on others' ideas and expressing their own clearly."^^xsd:string .

:CCSS.ELA-Literacy.SL.7.1.a rdf:type owl:Class ;
    prov:wasQuotedFrom <http://www.corestandards.org/ELA-Literacy/SL/7/1/a/> ;
    rdfs:subClassOf :CCSS.ELA-Literacy.SL.7.1 ;
    rdfs:comment "Come to discussions prepared, having read or researched material under study; explicitly draw on that preparation by referring to evidence on the topic, text, or issue to probe and reflect on ideas under discussion."^^xsd:string .

:CCSS.ELA-Literacy.SL.7.1.b rdf:type owl:Class ;
    prov:wasQuotedFrom <http://www.corestandards.org/ELA-Literacy/SL/7/1/b/> ;
    rdfs:subClassOf :CCSS.ELA-Literacy.SL.7.1 ;
    rdfs:comment "Follow rules for collegial discussions, track progress toward specific goals and deadlines, and define individual roles as needed."^^xsd:string .

:CCSS.ELA-Literacy.SL.7.1.c rdf:type owl:Class ;
    prov:wasQuotedFrom <http://www.corestandards.org/ELA-Literacy/SL/7/1/c/> ;
    rdfs:subClassOf :CCSS.ELA-Literacy.SL.7.1 ;
    rdfs:comment "Pose questions that elicit elaboration and respond to others' questions and comments with relevant observations and ideas that bring the discussion back on topic as needed."^^xsd:string .

:CCSS.ELA-Literacy.SL.7.1.d rdf:type owl:Class ;
    prov:wasQuotedFrom <http://www.corestandards.org/ELA-Literacy/SL/7/1/d/> ;
    rdfs:subClassOf :CCSS.ELA-Literacy.SL.7.1 ;
    rdfs:comment "Acknowledge new information expressed by others and, when warranted, modify their own views."^^xsd:string .

:CCSS.ELA-Literacy.SL.7.2 rdf:type owl:Class ;
    prov:wasQuotedFrom <http://www.corestandards.org/ELA-Literacy/SL/7/2/> ;
    rdfs:subClassOf :CCSS.ELA-Literacy.SL.7 ;
    rdfs:comment "Analyze the main ideas and supporting details presented in diverse media and formats (e.g., visually, quantitatively, orally) and explain how the ideas clarify a topic, text, or issue under study."^^xsd:string .

:CCSS.ELA-Literacy.SL.7.3 rdf:type owl:Class ;
    prov:wasQuotedFrom <http://www.corestandards.org/ELA-Literacy/SL/7/3/> ;
    rdfs:subClassOf :CCSS.ELA-Literacy.SL.7 ;
    rdfs:comment "Delineate a speaker's argument and specific claims, evaluating the soundness of the reasoning and the relevance and sufficiency of the evidence."^^xsd:string .

:CCSS.ELA-Literacy.SL.7.4 rdf:type owl:Class ;
    prov:wasQuotedFrom <http://www.corestandards.org/ELA-Literacy/SL/7/4/> ;
    rdfs:subClassOf :CCSS.ELA-Literacy.SL.7 ;
    rdfs:comment "Present claims and findings, emphasizing salient points in a focused, coherent manner with pertinent descriptions, facts, details, and examples; use appropriate eye contact, adequate volume, and clear pronunciation."^^xsd:string .

:CCSS.ELA-Literacy.SL.7.5 rdf:type owl:Class ;
    prov:wasQuotedFrom <http://www.corestandards.org/ELA-Literacy/SL/7/5/> ;
    rdfs:subClassOf :CCSS.ELA-Literacy.SL.7 ;
    rdfs:comment "Include multimedia components and visual displays in presentations to clarify claims and findings and emphasize salient points."^^xsd:string .

:CCSS.ELA-Literacy.SL.7.6 rdf:type owl:Class ;
    prov:wasQuotedFrom <http://www.corestandards.org/ELA-Literacy/SL/7/6/> ;
    rdfs:subClassOf :CCSS.ELA-Literacy.SL.7 ;
    rdfs:comment "Adapt speech to a variety of contexts and tasks, demonstrating command of formal English when indicated or appropriate. (See grade 7 Language standards 1 and 3  for specific expectations.)"^^xsd:string .

:CCSS.ELA-Literacy.SL.8.1 rdf:type owl:Class ;
    prov:wasQuotedFrom <http://www.corestandards.org/ELA-Literacy/SL/8/1/> ;
    rdfs:subClassOf :CCSS.ELA-Literacy.SL.8 ;
    rdfs:comment "Engage effectively in a range of collaborative discussions (one-on-one, in groups, and teacher-led) with diverse partners on grade 8 topics, texts, and issues, building on others' ideas and expressing their own clearly."^^xsd:string .

:CCSS.ELA-Literacy.SL.8.1.a rdf:type owl:Class ;
    prov:wasQuotedFrom <http://www.corestandards.org/ELA-Literacy/SL/8/1/a/> ;
    rdfs:subClassOf :CCSS.ELA-Literacy.SL.8.1 ;
    rdfs:comment "Come to discussions prepared, having read or researched material under study; explicitly draw on that preparation by referring to evidence on the topic, text, or issue to probe and reflect on ideas under discussion."^^xsd:string .

:CCSS.ELA-Literacy.SL.8.1.b rdf:type owl:Class ;
    prov:wasQuotedFrom <http://www.corestandards.org/ELA-Literacy/SL/8/1/b/> ;
    rdfs:subClassOf :CCSS.ELA-Literacy.SL.8.1 ;
    rdfs:comment "Follow rules for collegial discussions and decision-making, track progress toward specific goals and deadlines, and define individual roles as needed."^^xsd:string .

:CCSS.ELA-Literacy.SL.8.1.c rdf:type owl:Class ;
    prov:wasQuotedFrom <http://www.corestandards.org/ELA-Literacy/SL/8/1/c/> ;
    rdfs:subClassOf :CCSS.ELA-Literacy.SL.8.1 ;
    rdfs:comment "Pose questions that connect the ideas of several speakers and respond to others' questions and comments with relevant evidence, observations, and ideas."^^xsd:string .

:CCSS.ELA-Literacy.SL.8.1.d rdf:type owl:Class ;
    prov:wasQuotedFrom <http://www.corestandards.org/ELA-Literacy/SL/8/1/d/> ;
    rdfs:subClassOf :CCSS.ELA-Literacy.SL.8.1 ;
    rdfs:comment "Acknowledge new information expressed by others, and, when warranted, qualify or justify their own views in light of the evidence presented."^^xsd:string .

:CCSS.ELA-Literacy.SL.8.2 rdf:type owl:Class ;
    prov:wasQuotedFrom <http://www.corestandards.org/ELA-Literacy/SL/8/2/> ;
    rdfs:subClassOf :CCSS.ELA-Literacy.SL.8 ;
    rdfs:comment "Analyze the purpose of information presented in diverse media and formats (e.g., visually, quantitatively, orally) and evaluate the motives (e.g., social, commercial, political) behind its presentation."^^xsd:string .

:CCSS.ELA-Literacy.SL.8.3 rdf:type owl:Class ;
    prov:wasQuotedFrom <http://www.corestandards.org/ELA-Literacy/SL/8/3/> ;
    rdfs:subClassOf :CCSS.ELA-Literacy.SL.8 ;
    rdfs:comment "Delineate a speaker's argument and specific claims, evaluating the soundness of the reasoning and relevance and sufficiency of the evidence and identifying when irrelevant evidence is introduced."^^xsd:string .

:CCSS.ELA-Literacy.SL.8.4 rdf:type owl:Class ;
    prov:wasQuotedFrom <http://www.corestandards.org/ELA-Literacy/SL/8/4/> ;
    rdfs:subClassOf :CCSS.ELA-Literacy.SL.8 ;
    rdfs:comment "Present claims and findings, emphasizing salient points in a focused, coherent manner with relevant evidence, sound valid reasoning, and well-chosen details; use appropriate eye contact, adequate volume, and clear pronunciation."^^xsd:string .

:CCSS.ELA-Literacy.SL.8.5 rdf:type owl:Class ;
    prov:wasQuotedFrom <http://www.corestandards.org/ELA-Literacy/SL/8/5/> ;
    rdfs:subClassOf :CCSS.ELA-Literacy.SL.8 ;
    rdfs:comment "Integrate multimedia and visual displays into presentations to clarify information, strengthen claims and evidence, and add interest."^^xsd:string .

:CCSS.ELA-Literacy.SL.8.6 rdf:type owl:Class ;
    prov:wasQuotedFrom <http://www.corestandards.org/ELA-Literacy/SL/8/6/> ;
    rdfs:subClassOf :CCSS.ELA-Literacy.SL.8 ;
    rdfs:comment "Adapt speech to a variety of contexts and tasks, demonstrating command of formal English when indicated or appropriate. (See grade 8 Language standards 1 and 3  for specific expectations.)"^^xsd:string .

:CCSS.ELA-Literacy.SL.9-10.1 rdf:type owl:Class ;
    prov:wasQuotedFrom <http://www.corestandards.org/ELA-Literacy/SL/9-10/1/> ;
    rdfs:subClassOf :CCSS.ELA-Literacy.SL.9-10 ;
    rdfs:comment "Initiate and participate effectively in a range of collaborative discussions (one-on-one, in groups, and teacher-led) with diverse partners on grades 9-10 topics, texts, and issues, building on others' ideas and expressing their own clearly and persuasively."^^xsd:string .

:CCSS.ELA-Literacy.SL.9-10.1.a rdf:type owl:Class ;
    prov:wasQuotedFrom <http://www.corestandards.org/ELA-Literacy/SL/9-10/1/a/> ;
    rdfs:subClassOf :CCSS.ELA-Literacy.SL.9-10.1 ;
    rdfs:comment "Come to discussions prepared, having read and researched material under study; explicitly draw on that preparation by referring to evidence from texts and other research on the topic or issue to stimulate a thoughtful, well-reasoned exchange of ideas."^^xsd:string .

:CCSS.ELA-Literacy.SL.9-10.1.b rdf:type owl:Class ;
    prov:wasQuotedFrom <http://www.corestandards.org/ELA-Literacy/SL/9-10/1/b/> ;
    rdfs:subClassOf :CCSS.ELA-Literacy.SL.9-10.1 ;
    rdfs:comment "Work with peers to set rules for collegial discussions and decision-making (e.g., informal consensus, taking votes on key issues, presentation of alternate views), clear goals and deadlines, and individual roles as needed."^^xsd:string .

:CCSS.ELA-Literacy.SL.9-10.1.c rdf:type owl:Class ;
    prov:wasQuotedFrom <http://www.corestandards.org/ELA-Literacy/SL/9-10/1/c/> ;
    rdfs:subClassOf :CCSS.ELA-Literacy.SL.9-10.1 ;
    rdfs:comment "Propel conversations by posing and responding to questions that relate the current discussion to broader themes or larger ideas; actively incorporate others into the discussion; and clarify, verify, or challenge ideas and conclusions."^^xsd:string .

:CCSS.ELA-Literacy.SL.9-10.1.d rdf:type owl:Class ;
    prov:wasQuotedFrom <http://www.corestandards.org/ELA-Literacy/SL/9-10/1/d/> ;
    rdfs:subClassOf :CCSS.ELA-Literacy.SL.9-10.1 ;
    rdfs:comment "Respond thoughtfully to diverse perspectives, summarize points of agreement and disagreement, and, when warranted, qualify or justify their own views and understanding and make new connections in light of the evidence and reasoning presented."^^xsd:string .

:CCSS.ELA-Literacy.SL.9-10.2 rdf:type owl:Class ;
    prov:wasQuotedFrom <http://www.corestandards.org/ELA-Literacy/SL/9-10/2/> ;
    rdfs:subClassOf :CCSS.ELA-Literacy.SL.9-10 ;
    rdfs:comment "Integrate multiple sources of information presented in diverse media or formats (e.g., visually, quantitatively, orally) evaluating the credibility and accuracy of each source."^^xsd:string .

:CCSS.ELA-Literacy.SL.9-10.3 rdf:type owl:Class ;
    prov:wasQuotedFrom <http://www.corestandards.org/ELA-Literacy/SL/9-10/3/> ;
    rdfs:subClassOf :CCSS.ELA-Literacy.SL.9-10 ;
    rdfs:comment "Evaluate a speaker's point of view, reasoning, and use of evidence and rhetoric, identifying any fallacious reasoning or exaggerated or distorted evidence."^^xsd:string .

:CCSS.ELA-Literacy.SL.9-10.4 rdf:type owl:Class ;
    prov:wasQuotedFrom <http://www.corestandards.org/ELA-Literacy/SL/9-10/4/> ;
    rdfs:subClassOf :CCSS.ELA-Literacy.SL.9-10 ;
    rdfs:comment "Present information, findings, and supporting evidence clearly, concisely, and logically such that listeners can follow the line of reasoning and the organization, development, substance, and style are appropriate to purpose, audience, and task."^^xsd:string .

:CCSS.ELA-Literacy.SL.9-10.5 rdf:type owl:Class ;
    prov:wasQuotedFrom <http://www.corestandards.org/ELA-Literacy/SL/9-10/5/> ;
    rdfs:subClassOf :CCSS.ELA-Literacy.SL.9-10 ;
    rdfs:comment "Make strategic use of digital media (e.g., textual, graphical, audio, visual, and interactive elements) in presentations to enhance understanding of findings, reasoning, and evidence and to add interest."^^xsd:string .

:CCSS.ELA-Literacy.SL.9-10.6 rdf:type owl:Class ;
    prov:wasQuotedFrom <http://www.corestandards.org/ELA-Literacy/SL/9-10/6/> ;
    rdfs:subClassOf :CCSS.ELA-Literacy.SL.9-10 ;
    rdfs:comment "Adapt speech to a variety of contexts and tasks, demonstrating command of formal English when indicated or appropriate. (See grades 9-10 Language standards 1 and 3  for specific expectations.)"^^xsd:string .

:CCSS.ELA-Literacy.SL.11-12.1 rdf:type owl:Class ;
    prov:wasQuotedFrom <http://www.corestandards.org/ELA-Literacy/SL/11-12/1/> ;
    rdfs:subClassOf :CCSS.ELA-Literacy.SL.11-12 ;
    rdfs:comment "Initiate and participate effectively in a range of collaborative discussions (one-on-one, in groups, and teacher-led) with diverse partners on grades 11-12 topics, texts, and issues, building on others' ideas and expressing their own clearly and persuasively."^^xsd:string .

:CCSS.ELA-Literacy.SL.11-12.1.a rdf:type owl:Class ;
    prov:wasQuotedFrom <http://www.corestandards.org/ELA-Literacy/SL/11-12/1/a/> ;
    rdfs:subClassOf :CCSS.ELA-Literacy.SL.11-12.1 ;
    rdfs:comment "Come to discussions prepared, having read and researched material under study; explicitly draw on that preparation by referring to evidence from texts and other research on the topic or issue to stimulate a thoughtful, well-reasoned exchange of ideas."^^xsd:string .

:CCSS.ELA-Literacy.SL.11-12.1.b rdf:type owl:Class ;
    prov:wasQuotedFrom <http://www.corestandards.org/ELA-Literacy/SL/11-12/1/b/> ;
    rdfs:subClassOf :CCSS.ELA-Literacy.SL.11-12.1 ;
    rdfs:comment "Work with peers to promote civil, democratic discussions and decision-making, set clear goals and deadlines, and establish individual roles as needed."^^xsd:string .

:CCSS.ELA-Literacy.SL.11-12.1.c rdf:type owl:Class ;
    prov:wasQuotedFrom <http://www.corestandards.org/ELA-Literacy/SL/11-12/1/c/> ;
    rdfs:subClassOf :CCSS.ELA-Literacy.SL.11-12.1 ;
    rdfs:comment "Propel conversations by posing and responding to questions that probe reasoning and evidence; ensure a hearing for a full range of positions on a topic or issue; clarify, verify, or challenge ideas and conclusions; and promote divergent and creative perspectives."^^xsd:string .

:CCSS.ELA-Literacy.SL.11-12.1.d rdf:type owl:Class ;
    prov:wasQuotedFrom <http://www.corestandards.org/ELA-Literacy/SL/11-12/1/d/> ;
    rdfs:subClassOf :CCSS.ELA-Literacy.SL.11-12.1 ;
    rdfs:comment "Respond thoughtfully to diverse perspectives; synthesize comments, claims, and evidence made on all sides of an issue; resolve contradictions when possible; and determine what additional information or research is required to deepen the investigation or complete the task."^^xsd:string .

:CCSS.ELA-Literacy.SL.11-12.2 rdf:type owl:Class ;
    prov:wasQuotedFrom <http://www.corestandards.org/ELA-Literacy/SL/11-12/2/> ;
    rdfs:subClassOf :CCSS.ELA-Literacy.SL.11-12 ;
    rdfs:comment "Integrate multiple sources of information presented in diverse formats and media (e.g., visually, quantitatively, orally) in order to make informed decisions and solve problems, evaluating the credibility and accuracy of each source and noting any discrepancies among the data."^^xsd:string .

:CCSS.ELA-Literacy.SL.11-12.3 rdf:type owl:Class ;
    prov:wasQuotedFrom <http://www.corestandards.org/ELA-Literacy/SL/11-12/3/> ;
    rdfs:subClassOf :CCSS.ELA-Literacy.SL.11-12 ;
    rdfs:comment "Evaluate a speaker's point of view, reasoning, and use of evidence and rhetoric, assessing the stance, premises, links among ideas, word choice, points of emphasis, and tone used."^^xsd:string .

:CCSS.ELA-Literacy.SL.11-12.4 rdf:type owl:Class ;
    prov:wasQuotedFrom <http://www.corestandards.org/ELA-Literacy/SL/11-12/4/> ;
    rdfs:subClassOf :CCSS.ELA-Literacy.SL.11-12 ;
    rdfs:comment "Present information, findings, and supporting evidence, conveying a clear and distinct perspective, such that listeners can follow the line of reasoning, alternative or opposing perspectives are addressed, and the organization, development, substance, and style are appropriate to purpose, audience, and a range of formal and informal tasks."^^xsd:string .

:CCSS.ELA-Literacy.SL.11-12.5 rdf:type owl:Class ;
    prov:wasQuotedFrom <http://www.corestandards.org/ELA-Literacy/SL/11-12/5/> ;
    rdfs:subClassOf :CCSS.ELA-Literacy.SL.11-12 ;
    rdfs:comment "Make strategic use of digital media (e.g., textual, graphical, audio, visual, and interactive elements) in presentations to enhance understanding of findings, reasoning, and evidence and to add interest."^^xsd:string .

:CCSS.ELA-Literacy.SL.11-12.6 rdf:type owl:Class ;
    prov:wasQuotedFrom <http://www.corestandards.org/ELA-Literacy/SL/11-12/6/> ;
    rdfs:subClassOf :CCSS.ELA-Literacy.SL.11-12 ;
    rdfs:comment "Adapt speech to a variety of contexts and tasks, demonstrating a command of formal English when indicated or appropriate. (See grades 11-12 Language standards 1 and 3  for specific expectations.)"^^xsd:string .

:CCSS.ELA-Literacy.L.K.1 rdf:type owl:Class ;
    prov:wasQuotedFrom <http://www.corestandards.org/ELA-Literacy/L/K/1/> ;
    rdfs:subClassOf :CCSS.ELA-Literacy.L.K ;
    rdfs:comment "Demonstrate command of the conventions of standard English grammar and usage when writing or speaking."^^xsd:string .

:CCSS.ELA-Literacy.L.K.1.a rdf:type owl:Class ;
    prov:wasQuotedFrom <http://www.corestandards.org/ELA-Literacy/L/K/1/a/> ;
    rdfs:subClassOf :CCSS.ELA-Literacy.L.K.1 ;
    rdfs:comment "Print many upper- and lowercase letters."^^xsd:string .

:CCSS.ELA-Literacy.L.K.1.b rdf:type owl:Class ;
    prov:wasQuotedFrom <http://www.corestandards.org/ELA-Literacy/L/K/1/b/> ;
    rdfs:subClassOf :CCSS.ELA-Literacy.L.K.1 ;
    rdfs:comment "Use frequently occurring nouns and verbs."^^xsd:string .

:CCSS.ELA-Literacy.L.K.1.c rdf:type owl:Class ;
    prov:wasQuotedFrom <http://www.corestandards.org/ELA-Literacy/L/K/1/c/> ;
    rdfs:subClassOf :CCSS.ELA-Literacy.L.K.1 ;
    rdfs:comment "Form regular plural nouns orally by adding /s/ or /es/ (e.g., dog, dogs; wish, wishes)."^^xsd:string .

:CCSS.ELA-Literacy.L.K.1.d rdf:type owl:Class ;
    prov:wasQuotedFrom <http://www.corestandards.org/ELA-Literacy/L/K/1/d/> ;
    rdfs:subClassOf :CCSS.ELA-Literacy.L.K.1 ;
    rdfs:comment "Understand and use question words (interrogatives) (e.g., who, what, where, when, why, how)."^^xsd:string .

:CCSS.ELA-Literacy.L.K.1.e rdf:type owl:Class ;
    prov:wasQuotedFrom <http://www.corestandards.org/ELA-Literacy/L/K/1/e/> ;
    rdfs:subClassOf :CCSS.ELA-Literacy.L.K.1 ;
    rdfs:comment "Use the most frequently occurring prepositions (e.g., to, from, in, out, on, off, for, of, by, with)."^^xsd:string .

:CCSS.ELA-Literacy.L.K.1.f rdf:type owl:Class ;
    prov:wasQuotedFrom <http://www.corestandards.org/ELA-Literacy/L/K/1/f/> ;
    rdfs:subClassOf :CCSS.ELA-Literacy.L.K.1 ;
    rdfs:comment "Produce and expand complete sentences in shared language activities."^^xsd:string .

:CCSS.ELA-Literacy.L.K.2 rdf:type owl:Class ;
    prov:wasQuotedFrom <http://www.corestandards.org/ELA-Literacy/L/K/2/> ;
    rdfs:subClassOf :CCSS.ELA-Literacy.L.K ;
    rdfs:comment "Demonstrate command of the conventions of standard English capitalization, punctuation, and spelling when writing."^^xsd:string .

:CCSS.ELA-Literacy.L.K.2.a rdf:type owl:Class ;
    prov:wasQuotedFrom <http://www.corestandards.org/ELA-Literacy/L/K/2/a/> ;
    rdfs:subClassOf :CCSS.ELA-Literacy.L.K.2 ;
    rdfs:comment "Capitalize the first word in a sentence and the pronoun I"^^xsd:string .

:CCSS.ELA-Literacy.L.K.2.b rdf:type owl:Class ;
    prov:wasQuotedFrom <http://www.corestandards.org/ELA-Literacy/L/K/2/b/> ;
    rdfs:subClassOf :CCSS.ELA-Literacy.L.K.2 ;
    rdfs:comment "Recognize and name end punctuation."^^xsd:string .

:CCSS.ELA-Literacy.L.K.2.c rdf:type owl:Class ;
    prov:wasQuotedFrom <http://www.corestandards.org/ELA-Literacy/L/K/2/c/> ;
    rdfs:subClassOf :CCSS.ELA-Literacy.L.K.2 ;
    rdfs:comment "Write a letter or letters for most consonant and short-vowel sounds (phonemes)."^^xsd:string .

:CCSS.ELA-Literacy.L.K.2.d rdf:type owl:Class ;
    prov:wasQuotedFrom <http://www.corestandards.org/ELA-Literacy/L/K/2/d/> ;
    rdfs:subClassOf :CCSS.ELA-Literacy.L.K.2 ;
    rdfs:comment "Spell simple words phonetically, drawing on knowledge of sound-letter relationships."^^xsd:string .

:CCSS.ELA-Literacy.L.K.3 rdf:type owl:Class ;
    prov:wasQuotedFrom <http://www.corestandards.org/ELA-Literacy/L/K/3/> ;
    rdfs:subClassOf :CCSS.ELA-Literacy.L.K ;
    rdfs:comment "(L.K.3 begins in grade 2)"^^xsd:string .

:CCSS.ELA-Literacy.L.K.4 rdf:type owl:Class ;
    prov:wasQuotedFrom <http://www.corestandards.org/ELA-Literacy/L/K/4/> ;
    rdfs:subClassOf :CCSS.ELA-Literacy.L.K ;
    rdfs:comment "Determine or clarify the meaning of unknown and multiple-meaning words and phrases based on kindergarten reading and content."^^xsd:string .

:CCSS.ELA-Literacy.L.K.4.a rdf:type owl:Class ;
    prov:wasQuotedFrom <http://www.corestandards.org/ELA-Literacy/L/K/4/a/> ;
    rdfs:subClassOf :CCSS.ELA-Literacy.L.K.4 ;
    rdfs:comment "Identify new meanings for familiar words and apply them accurately (e.g., knowing duck is a bird and learning the verb to duck)."^^xsd:string .

:CCSS.ELA-Literacy.L.K.4.b rdf:type owl:Class ;
    prov:wasQuotedFrom <http://www.corestandards.org/ELA-Literacy/L/K/4/b/> ;
    rdfs:subClassOf :CCSS.ELA-Literacy.L.K.4 ;
    rdfs:comment "Use the most frequently occurring inflections and affixes (e.g., -ed, -s, re-, un-, pre-, -ful, -less) as a clue to the meaning of an unknown word."^^xsd:string .

:CCSS.ELA-Literacy.L.K.5 rdf:type owl:Class ;
    prov:wasQuotedFrom <http://www.corestandards.org/ELA-Literacy/L/K/5/> ;
    rdfs:subClassOf :CCSS.ELA-Literacy.L.K ;
    rdfs:comment "With guidance and support from adults, explore word relationships and nuances in word meanings."^^xsd:string .

:CCSS.ELA-Literacy.L.K.5.a rdf:type owl:Class ;
    prov:wasQuotedFrom <http://www.corestandards.org/ELA-Literacy/L/K/5/a/> ;
    rdfs:subClassOf :CCSS.ELA-Literacy.L.K.5 ;
    rdfs:comment "Sort common objects into categories (e.g., shapes, foods) to gain a sense of the concepts the categories represent."^^xsd:string .

:CCSS.ELA-Literacy.L.K.5.b rdf:type owl:Class ;
    prov:wasQuotedFrom <http://www.corestandards.org/ELA-Literacy/L/K/5/b/> ;
    rdfs:subClassOf :CCSS.ELA-Literacy.L.K.5 ;
    rdfs:comment "Demonstrate understanding of frequently occurring verbs and adjectives by relating them to their opposites (antonyms)."^^xsd:string .

:CCSS.ELA-Literacy.L.K.5.c rdf:type owl:Class ;
    prov:wasQuotedFrom <http://www.corestandards.org/ELA-Literacy/L/K/5/c/> ;
    rdfs:subClassOf :CCSS.ELA-Literacy.L.K.5 ;
    rdfs:comment "Identify real-life connections between words and their use (e.g., note places at school that are colorful)."^^xsd:string .

:CCSS.ELA-Literacy.L.K.5.d rdf:type owl:Class ;
    prov:wasQuotedFrom <http://www.corestandards.org/ELA-Literacy/L/K/5/d/> ;
    rdfs:subClassOf :CCSS.ELA-Literacy.L.K.5 ;
    rdfs:comment "Distinguish shades of meaning among verbs describing the same general action (e.g., walk, march, strut, prance) by acting out the meanings."^^xsd:string .

:CCSS.ELA-Literacy.L.K.6 rdf:type owl:Class ;
    prov:wasQuotedFrom <http://www.corestandards.org/ELA-Literacy/L/K/6/> ;
    rdfs:subClassOf :CCSS.ELA-Literacy.L.K ;
    rdfs:comment "Use words and phrases acquired through conversations, reading and being read to, and responding to texts."^^xsd:string .

:CCSS.ELA-Literacy.L.1.1 rdf:type owl:Class ;
    prov:wasQuotedFrom <http://www.corestandards.org/ELA-Literacy/L/1/1/> ;
    rdfs:subClassOf :CCSS.ELA-Literacy.L.1 ;
    rdfs:comment "Demonstrate command of the conventions of standard English grammar and usage when writing or speaking."^^xsd:string .

:CCSS.ELA-Literacy.L.1.1.a rdf:type owl:Class ;
    prov:wasQuotedFrom <http://www.corestandards.org/ELA-Literacy/L/1/1/a/> ;
    rdfs:subClassOf :CCSS.ELA-Literacy.L.1.1 ;
    rdfs:comment "Print all upper- and lowercase letters."^^xsd:string .

:CCSS.ELA-Literacy.L.1.1.b rdf:type owl:Class ;
    prov:wasQuotedFrom <http://www.corestandards.org/ELA-Literacy/L/1/1/b/> ;
    rdfs:subClassOf :CCSS.ELA-Literacy.L.1.1 ;
    rdfs:comment "Use common, proper, and possessive nouns."^^xsd:string .

:CCSS.ELA-Literacy.L.1.1.c rdf:type owl:Class ;
    prov:wasQuotedFrom <http://www.corestandards.org/ELA-Literacy/L/1/1/c/> ;
    rdfs:subClassOf :CCSS.ELA-Literacy.L.1.1 ;
    rdfs:comment "Use singular and plural nouns with matching verbs in basic sentences (e.g., He hops; We hop)."^^xsd:string .

:CCSS.ELA-Literacy.L.1.1.d rdf:type owl:Class ;
    prov:wasQuotedFrom <http://www.corestandards.org/ELA-Literacy/L/1/1/d/> ;
    rdfs:subClassOf :CCSS.ELA-Literacy.L.1.1 ;
    rdfs:comment "Use personal, possessive, and indefinite pronouns (e.g., I, me, my; they, them, their, anyone, everything)."^^xsd:string .

:CCSS.ELA-Literacy.L.1.1.e rdf:type owl:Class ;
    prov:wasQuotedFrom <http://www.corestandards.org/ELA-Literacy/L/1/1/e/> ;
    rdfs:subClassOf :CCSS.ELA-Literacy.L.1.1 ;
    rdfs:comment "Use verbs to convey a sense of past, present, and future (e.g., Yesterday I walked home; Today I walk home; Tomorrow I will walk home)."^^xsd:string .

:CCSS.ELA-Literacy.L.1.1.f rdf:type owl:Class ;
    prov:wasQuotedFrom <http://www.corestandards.org/ELA-Literacy/L/1/1/f/> ;
    rdfs:subClassOf :CCSS.ELA-Literacy.L.1.1 ;
    rdfs:comment "Use frequently occurring adjectives."^^xsd:string .

:CCSS.ELA-Literacy.L.1.1.g rdf:type owl:Class ;
    prov:wasQuotedFrom <http://www.corestandards.org/ELA-Literacy/L/1/1/g/> ;
    rdfs:subClassOf :CCSS.ELA-Literacy.L.1.1 ;
    rdfs:comment "Use frequently occurring conjunctions (e.g., and, but, or, so, because)."^^xsd:string .

:CCSS.ELA-Literacy.L.1.1.h rdf:type owl:Class ;
    prov:wasQuotedFrom <http://www.corestandards.org/ELA-Literacy/L/1/1/h/> ;
    rdfs:subClassOf :CCSS.ELA-Literacy.L.1.1 ;
    rdfs:comment "Use determiners (e.g., articles, demonstratives)."^^xsd:string .

:CCSS.ELA-Literacy.L.1.1.i rdf:type owl:Class ;
    prov:wasQuotedFrom <http://www.corestandards.org/ELA-Literacy/L/1/1/i/> ;
    rdfs:subClassOf :CCSS.ELA-Literacy.L.1.1 ;
    rdfs:comment "Use frequently occurring prepositions (e.g., during, beyond, toward)."^^xsd:string .

:CCSS.ELA-Literacy.L.1.1.j rdf:type owl:Class ;
    prov:wasQuotedFrom <http://www.corestandards.org/ELA-Literacy/L/1/1/j/> ;
    rdfs:subClassOf :CCSS.ELA-Literacy.L.1.1 ;
    rdfs:comment "Produce and expand complete simple and compound declarative, interrogative, imperative, and exclamatory sentences in response to prompts."^^xsd:string .

:CCSS.ELA-Literacy.L.1.2 rdf:type owl:Class ;
    prov:wasQuotedFrom <http://www.corestandards.org/ELA-Literacy/L/1/2/> ;
    rdfs:subClassOf :CCSS.ELA-Literacy.L.1 ;
    rdfs:comment "Demonstrate command of the conventions of standard English capitalization, punctuation, and spelling when writing."^^xsd:string .

:CCSS.ELA-Literacy.L.1.2.a rdf:type owl:Class ;
    prov:wasQuotedFrom <http://www.corestandards.org/ELA-Literacy/L/1/2/a/> ;
    rdfs:subClassOf :CCSS.ELA-Literacy.L.1.2 ;
    rdfs:comment "Capitalize dates and names of people."^^xsd:string .

:CCSS.ELA-Literacy.L.1.2.b rdf:type owl:Class ;
    prov:wasQuotedFrom <http://www.corestandards.org/ELA-Literacy/L/1/2/b/> ;
    rdfs:subClassOf :CCSS.ELA-Literacy.L.1.2 ;
    rdfs:comment "Use end punctuation for sentences."^^xsd:string .

:CCSS.ELA-Literacy.L.1.2.c rdf:type owl:Class ;
    prov:wasQuotedFrom <http://www.corestandards.org/ELA-Literacy/L/1/2/c/> ;
    rdfs:subClassOf :CCSS.ELA-Literacy.L.1.2 ;
    rdfs:comment "Use commas in dates and to separate single words in a series."^^xsd:string .

:CCSS.ELA-Literacy.L.1.2.d rdf:type owl:Class ;
    prov:wasQuotedFrom <http://www.corestandards.org/ELA-Literacy/L/1/2/d/> ;
    rdfs:subClassOf :CCSS.ELA-Literacy.L.1.2 ;
    rdfs:comment "Use conventional spelling for words with common spelling patterns and for frequently occurring irregular words."^^xsd:string .

:CCSS.ELA-Literacy.L.1.2.e rdf:type owl:Class ;
    prov:wasQuotedFrom <http://www.corestandards.org/ELA-Literacy/L/1/2/e/> ;
    rdfs:subClassOf :CCSS.ELA-Literacy.L.1.2 ;
    rdfs:comment "Spell untaught words phonetically, drawing on phonemic awareness and spelling conventions."^^xsd:string .

:CCSS.ELA-Literacy.L.1.3 rdf:type owl:Class ;
    prov:wasQuotedFrom <http://www.corestandards.org/ELA-Literacy/L/1/3/> ;
    rdfs:subClassOf :CCSS.ELA-Literacy.L.1 ;
    rdfs:comment "(L.1.3 begins in grade 2)"^^xsd:string .

:CCSS.ELA-Literacy.L.1.4 rdf:type owl:Class ;
    prov:wasQuotedFrom <http://www.corestandards.org/ELA-Literacy/L/1/4/> ;
    rdfs:subClassOf :CCSS.ELA-Literacy.L.1 ;
    rdfs:comment "Determine or clarify the meaning of unknown and multiple-meaning words and phrases based on grade 1 reading and content, choosing flexibly from an array of strategies."^^xsd:string .

:CCSS.ELA-Literacy.L.1.4.a rdf:type owl:Class ;
    prov:wasQuotedFrom <http://www.corestandards.org/ELA-Literacy/L/1/4/a/> ;
    rdfs:subClassOf :CCSS.ELA-Literacy.L.1.4 ;
    rdfs:comment "Use sentence-level context as a clue to the meaning of a word or phrase."^^xsd:string .

:CCSS.ELA-Literacy.L.1.4.b rdf:type owl:Class ;
    prov:wasQuotedFrom <http://www.corestandards.org/ELA-Literacy/L/1/4/b/> ;
    rdfs:subClassOf :CCSS.ELA-Literacy.L.1.4 ;
    rdfs:comment "Use frequently occurring affixes as a clue to the meaning of a word."^^xsd:string .

:CCSS.ELA-Literacy.L.1.4.c rdf:type owl:Class ;
    prov:wasQuotedFrom <http://www.corestandards.org/ELA-Literacy/L/1/4/c/> ;
    rdfs:subClassOf :CCSS.ELA-Literacy.L.1.4 ;
    rdfs:comment "Identify frequently occurring root words (e.g., look) and their inflectional forms (e.g., looks, looked, looking)."^^xsd:string .

:CCSS.ELA-Literacy.L.1.5 rdf:type owl:Class ;
    prov:wasQuotedFrom <http://www.corestandards.org/ELA-Literacy/L/1/5/> ;
    rdfs:subClassOf :CCSS.ELA-Literacy.L.1 ;
    rdfs:comment "With guidance and support from adults, demonstrate understanding of word relationships and nuances in word meanings."^^xsd:string .

:CCSS.ELA-Literacy.L.1.5.a rdf:type owl:Class ;
    prov:wasQuotedFrom <http://www.corestandards.org/ELA-Literacy/L/1/5/a/> ;
    rdfs:subClassOf :CCSS.ELA-Literacy.L.1.5 ;
    rdfs:comment "Sort words into categories (e.g., colors, clothing) to gain a sense of the concepts the categories represent."^^xsd:string .

:CCSS.ELA-Literacy.L.1.5.b rdf:type owl:Class ;
    prov:wasQuotedFrom <http://www.corestandards.org/ELA-Literacy/L/1/5/b/> ;
    rdfs:subClassOf :CCSS.ELA-Literacy.L.1.5 ;
    rdfs:comment "Define words by category and by one or more key attributes (e.g., a duck is a bird that swims; a tiger is a large cat with stripes)."^^xsd:string .

:CCSS.ELA-Literacy.L.1.5.c rdf:type owl:Class ;
    prov:wasQuotedFrom <http://www.corestandards.org/ELA-Literacy/L/1/5/c/> ;
    rdfs:subClassOf :CCSS.ELA-Literacy.L.1.5 ;
    rdfs:comment "Identify real-life connections between words and their use (e.g., note places at home that are cozy)."^^xsd:string .

:CCSS.ELA-Literacy.L.1.5.d rdf:type owl:Class ;
    prov:wasQuotedFrom <http://www.corestandards.org/ELA-Literacy/L/1/5/d/> ;
    rdfs:subClassOf :CCSS.ELA-Literacy.L.1.5 ;
    rdfs:comment "Distinguish shades of meaning among verbs differing in manner (e.g., look, peek, glance, stare, glare, scowl) and adjectives differing in intensity (e.g., large, gigantic) by defining or choosing them or by acting out the meanings."^^xsd:string .

:CCSS.ELA-Literacy.L.1.6 rdf:type owl:Class ;
    prov:wasQuotedFrom <http://www.corestandards.org/ELA-Literacy/L/1/6/> ;
    rdfs:subClassOf :CCSS.ELA-Literacy.L.1 ;
    rdfs:comment "Use words and phrases acquired through conversations, reading and being read to, and responding to texts, including using frequently occurring conjunctions to signal simple relationships (e.g., because)."^^xsd:string .

:CCSS.ELA-Literacy.L.2.1 rdf:type owl:Class ;
    prov:wasQuotedFrom <http://www.corestandards.org/ELA-Literacy/L/2/1/> ;
    rdfs:subClassOf :CCSS.ELA-Literacy.L.2 ;
    rdfs:comment "Demonstrate command of the conventions of standard English grammar and usage when writing or speaking."^^xsd:string .

:CCSS.ELA-Literacy.L.2.1.a rdf:type owl:Class ;
    prov:wasQuotedFrom <http://www.corestandards.org/ELA-Literacy/L/2/1/a/> ;
    rdfs:subClassOf :CCSS.ELA-Literacy.L.2.1 ;
    rdfs:comment "Use collective nouns (e.g., group)."^^xsd:string .

:CCSS.ELA-Literacy.L.2.1.b rdf:type owl:Class ;
    prov:wasQuotedFrom <http://www.corestandards.org/ELA-Literacy/L/2/1/b/> ;
    rdfs:subClassOf :CCSS.ELA-Literacy.L.2.1 ;
    rdfs:comment "Form and use frequently occurring irregular plural nouns (e.g., feet, children, teeth, mice, fish)."^^xsd:string .

:CCSS.ELA-Literacy.L.2.1.c rdf:type owl:Class ;
    prov:wasQuotedFrom <http://www.corestandards.org/ELA-Literacy/L/2/1/c/> ;
    rdfs:subClassOf :CCSS.ELA-Literacy.L.2.1 ;
    rdfs:comment "Use reflexive pronouns (e.g., myself, ourselves)."^^xsd:string .

:CCSS.ELA-Literacy.L.2.1.d rdf:type owl:Class ;
    prov:wasQuotedFrom <http://www.corestandards.org/ELA-Literacy/L/2/1/d/> ;
    rdfs:subClassOf :CCSS.ELA-Literacy.L.2.1 ;
    rdfs:comment "Form and use the past tense of frequently occurring irregular verbs (e.g., sat, hid, told)."^^xsd:string .

:CCSS.ELA-Literacy.L.2.1.e rdf:type owl:Class ;
    prov:wasQuotedFrom <http://www.corestandards.org/ELA-Literacy/L/2/1/e/> ;
    rdfs:subClassOf :CCSS.ELA-Literacy.L.2.1 ;
    rdfs:comment "Use adjectives and adverbs, and choose between them depending on what is to be modified."^^xsd:string .

:CCSS.ELA-Literacy.L.2.1.f rdf:type owl:Class ;
    prov:wasQuotedFrom <http://www.corestandards.org/ELA-Literacy/L/2/1/f/> ;
    rdfs:subClassOf :CCSS.ELA-Literacy.L.2.1 ;
    rdfs:comment "Produce, expand, and rearrange complete simple and compound sentences (e.g., The boy watched the movie; The little boy watched the movie; The action movie was watched by the little boy)."^^xsd:string .

:CCSS.ELA-Literacy.L.2.2 rdf:type owl:Class ;
    prov:wasQuotedFrom <http://www.corestandards.org/ELA-Literacy/L/2/2/> ;
    rdfs:subClassOf :CCSS.ELA-Literacy.L.2 ;
    rdfs:comment "Demonstrate command of the conventions of standard English capitalization, punctuation, and spelling when writing."^^xsd:string .

:CCSS.ELA-Literacy.L.2.2.a rdf:type owl:Class ;
    prov:wasQuotedFrom <http://www.corestandards.org/ELA-Literacy/L/2/2/a/> ;
    rdfs:subClassOf :CCSS.ELA-Literacy.L.2.2 ;
    rdfs:comment "Capitalize holidays, product names, and geographic names."^^xsd:string .

:CCSS.ELA-Literacy.L.2.2.b rdf:type owl:Class ;
    prov:wasQuotedFrom <http://www.corestandards.org/ELA-Literacy/L/2/2/b/> ;
    rdfs:subClassOf :CCSS.ELA-Literacy.L.2.2 ;
    rdfs:comment "Use commas in greetings and closings of letters."^^xsd:string .

:CCSS.ELA-Literacy.L.2.2.c rdf:type owl:Class ;
    prov:wasQuotedFrom <http://www.corestandards.org/ELA-Literacy/L/2/2/c/> ;
    rdfs:subClassOf :CCSS.ELA-Literacy.L.2.2 ;
    rdfs:comment "Use an apostrophe to form contractions and frequently occurring possessives."^^xsd:string .

:CCSS.ELA-Literacy.L.2.2.d rdf:type owl:Class ;
    prov:wasQuotedFrom <http://www.corestandards.org/ELA-Literacy/L/2/2/d/> ;
    rdfs:subClassOf :CCSS.ELA-Literacy.L.2.2 ;
    rdfs:comment "Generalize learned spelling patterns when writing words (e.g., cage  badge; boy  boil)."^^xsd:string .

:CCSS.ELA-Literacy.L.2.2.e rdf:type owl:Class ;
    prov:wasQuotedFrom <http://www.corestandards.org/ELA-Literacy/L/2/2/e/> ;
    rdfs:subClassOf :CCSS.ELA-Literacy.L.2.2 ;
    rdfs:comment "Consult reference materials, including beginning dictionaries, as needed to check and correct spellings."^^xsd:string .

:CCSS.ELA-Literacy.L.2.3 rdf:type owl:Class ;
    prov:wasQuotedFrom <http://www.corestandards.org/ELA-Literacy/L/2/3/> ;
    rdfs:subClassOf :CCSS.ELA-Literacy.L.2 ;
    rdfs:comment "Use knowledge of language and its conventions when writing, speaking, reading, or listening."^^xsd:string .

:CCSS.ELA-Literacy.L.2.3.a rdf:type owl:Class ;
    prov:wasQuotedFrom <http://www.corestandards.org/ELA-Literacy/L/2/3/a/> ;
    rdfs:subClassOf :CCSS.ELA-Literacy.L.2.3 ;
    rdfs:comment "Compare formal and informal uses of English"^^xsd:string .

:CCSS.ELA-Literacy.L.2.4 rdf:type owl:Class ;
    prov:wasQuotedFrom <http://www.corestandards.org/ELA-Literacy/L/2/4/> ;
    rdfs:subClassOf :CCSS.ELA-Literacy.L.2 ;
    rdfs:comment "Determine or clarify the meaning of unknown and multiple-meaning words and phrases based on grade 2 reading and content, choosing flexibly from an array of strategies."^^xsd:string .

:CCSS.ELA-Literacy.L.2.4.a rdf:type owl:Class ;
    prov:wasQuotedFrom <http://www.corestandards.org/ELA-Literacy/L/2/4/a/> ;
    rdfs:subClassOf :CCSS.ELA-Literacy.L.2.4 ;
    rdfs:comment "Use sentence-level context as a clue to the meaning of a word or phrase."^^xsd:string .

:CCSS.ELA-Literacy.L.2.4.b rdf:type owl:Class ;
    prov:wasQuotedFrom <http://www.corestandards.org/ELA-Literacy/L/2/4/b/> ;
    rdfs:subClassOf :CCSS.ELA-Literacy.L.2.4 ;
    rdfs:comment "Determine the meaning of the new word formed when a known prefix is added to a known word (e.g., happy/unhappy, tell/retell)."^^xsd:string .

:CCSS.ELA-Literacy.L.2.4.c rdf:type owl:Class ;
    prov:wasQuotedFrom <http://www.corestandards.org/ELA-Literacy/L/2/4/c/> ;
    rdfs:subClassOf :CCSS.ELA-Literacy.L.2.4 ;
    rdfs:comment "Use a known root word as a clue to the meaning of an unknown word with the same root (e.g., addition, additional)."^^xsd:string .

:CCSS.ELA-Literacy.L.2.4.d rdf:type owl:Class ;
    prov:wasQuotedFrom <http://www.corestandards.org/ELA-Literacy/L/2/4/d/> ;
    rdfs:subClassOf :CCSS.ELA-Literacy.L.2.4 ;
    rdfs:comment "Use knowledge of the meaning of individual words to predict the meaning of compound words (e.g., birdhouse, lighthouse, housefly; bookshelf, notebook, bookmark)."^^xsd:string .

:CCSS.ELA-Literacy.L.2.4.e rdf:type owl:Class ;
    prov:wasQuotedFrom <http://www.corestandards.org/ELA-Literacy/L/2/4/e/> ;
    rdfs:subClassOf :CCSS.ELA-Literacy.L.2.4 ;
    rdfs:comment "Use glossaries and beginning dictionaries, both print and digital, to determine or clarify the meaning of words and phrases."^^xsd:string .

:CCSS.ELA-Literacy.L.2.5 rdf:type owl:Class ;
    prov:wasQuotedFrom <http://www.corestandards.org/ELA-Literacy/L/2/5/> ;
    rdfs:subClassOf :CCSS.ELA-Literacy.L.2 ;
    rdfs:comment "Demonstrate understanding of word relationships and nuances in word meanings."^^xsd:string .

:CCSS.ELA-Literacy.L.2.5.a rdf:type owl:Class ;
    prov:wasQuotedFrom <http://www.corestandards.org/ELA-Literacy/L/2/5/a/> ;
    rdfs:subClassOf :CCSS.ELA-Literacy.L.2.5 ;
    rdfs:comment "Identify real-life connections between words and their use (e.g., describe foods that are spicy or juicy)."^^xsd:string .

:CCSS.ELA-Literacy.L.2.5.b rdf:type owl:Class ;
    prov:wasQuotedFrom <http://www.corestandards.org/ELA-Literacy/L/2/5/b/> ;
    rdfs:subClassOf :CCSS.ELA-Literacy.L.2.5 ;
    rdfs:comment "Distinguish shades of meaning among closely related verbs (e.g., toss, throw, hurl) and closely related adjectives (e.g., thin, slender, skinny, scrawny)."^^xsd:string .

:CCSS.ELA-Literacy.L.2.6 rdf:type owl:Class ;
    prov:wasQuotedFrom <http://www.corestandards.org/ELA-Literacy/L/2/6/> ;
    rdfs:subClassOf :CCSS.ELA-Literacy.L.2 ;
    rdfs:comment "Use words and phrases acquired through conversations, reading and being read to, and responding to texts, including using adjectives and adverbs to describe (e.g., When other kids are happy that makes me happy)."^^xsd:string .

:CCSS.ELA-Literacy.L.3.1 rdf:type owl:Class ;
    prov:wasQuotedFrom <http://www.corestandards.org/ELA-Literacy/L/3/1/> ;
    rdfs:subClassOf :CCSS.ELA-Literacy.L.3 ;
    rdfs:comment "Demonstrate command of the conventions of standard English grammar and usage when writing or speaking."^^xsd:string .

:CCSS.ELA-Literacy.L.3.1.a rdf:type owl:Class ;
    prov:wasQuotedFrom <http://www.corestandards.org/ELA-Literacy/L/3/1/a/> ;
    rdfs:subClassOf :CCSS.ELA-Literacy.L.3.1 ;
    rdfs:comment "Explain the function of nouns, pronouns, verbs, adjectives, and adverbs in general and their functions in particular sentences."^^xsd:string .

:CCSS.ELA-Literacy.L.3.1.b rdf:type owl:Class ;
    prov:wasQuotedFrom <http://www.corestandards.org/ELA-Literacy/L/3/1/b/> ;
    rdfs:subClassOf :CCSS.ELA-Literacy.L.3.1 ;
    rdfs:comment "Form and use regular and irregular plural nouns."^^xsd:string .

:CCSS.ELA-Literacy.L.3.1.c rdf:type owl:Class ;
    prov:wasQuotedFrom <http://www.corestandards.org/ELA-Literacy/L/3/1/c/> ;
    rdfs:subClassOf :CCSS.ELA-Literacy.L.3.1 ;
    rdfs:comment "Use abstract nouns (e.g., childhood)."^^xsd:string .

:CCSS.ELA-Literacy.L.3.1.d rdf:type owl:Class ;
    prov:wasQuotedFrom <http://www.corestandards.org/ELA-Literacy/L/3/1/d/> ;
    rdfs:subClassOf :CCSS.ELA-Literacy.L.3.1 ;
    rdfs:comment "Form and use regular and irregular verbs."^^xsd:string .

:CCSS.ELA-Literacy.L.3.1.e rdf:type owl:Class ;
    prov:wasQuotedFrom <http://www.corestandards.org/ELA-Literacy/L/3/1/e/> ;
    rdfs:subClassOf :CCSS.ELA-Literacy.L.3.1 ;
    rdfs:comment "Form and use the simple (e.g., I walked; I walk; I will walk) verb tenses."^^xsd:string .

:CCSS.ELA-Literacy.L.3.1.f rdf:type owl:Class ;
    prov:wasQuotedFrom <http://www.corestandards.org/ELA-Literacy/L/3/1/f/> ;
    rdfs:subClassOf :CCSS.ELA-Literacy.L.3.1 ;
    rdfs:comment "Ensure subject-verb and pronoun-antecedent agreement.*"^^xsd:string .

:CCSS.ELA-Literacy.L.3.1.g rdf:type owl:Class ;
    prov:wasQuotedFrom <http://www.corestandards.org/ELA-Literacy/L/3/1/g/> ;
    rdfs:subClassOf :CCSS.ELA-Literacy.L.3.1 ;
    rdfs:comment "Form and use comparative and superlative adjectives and adverbs, and choose between them depending on what is to be modified."^^xsd:string .

:CCSS.ELA-Literacy.L.3.1.h rdf:type owl:Class ;
    prov:wasQuotedFrom <http://www.corestandards.org/ELA-Literacy/L/3/1/h/> ;
    rdfs:subClassOf :CCSS.ELA-Literacy.L.3.1 ;
    rdfs:comment "Use coordinating and subordinating conjunctions."^^xsd:string .

:CCSS.ELA-Literacy.L.3.1.i rdf:type owl:Class ;
    prov:wasQuotedFrom <http://www.corestandards.org/ELA-Literacy/L/3/1/i/> ;
    rdfs:subClassOf :CCSS.ELA-Literacy.L.3.1 ;
    rdfs:comment "Produce simple, compound, and complex sentences."^^xsd:string .

:CCSS.ELA-Literacy.L.3.2 rdf:type owl:Class ;
    prov:wasQuotedFrom <http://www.corestandards.org/ELA-Literacy/L/3/2/> ;
    rdfs:subClassOf :CCSS.ELA-Literacy.L.3 ;
    rdfs:comment "Demonstrate command of the conventions of standard English capitalization, punctuation, and spelling when writing."^^xsd:string .

:CCSS.ELA-Literacy.L.3.2.a rdf:type owl:Class ;
    prov:wasQuotedFrom <http://www.corestandards.org/ELA-Literacy/L/3/2/a/> ;
    rdfs:subClassOf :CCSS.ELA-Literacy.L.3.2 ;
    rdfs:comment "Capitalize appropriate words in titles."^^xsd:string .

:CCSS.ELA-Literacy.L.3.2.b rdf:type owl:Class ;
    prov:wasQuotedFrom <http://www.corestandards.org/ELA-Literacy/L/3/2/b/> ;
    rdfs:subClassOf :CCSS.ELA-Literacy.L.3.2 ;
    rdfs:comment "Use commas in addresses."^^xsd:string .

:CCSS.ELA-Literacy.L.3.2.c rdf:type owl:Class ;
    prov:wasQuotedFrom <http://www.corestandards.org/ELA-Literacy/L/3/2/c/> ;
    rdfs:subClassOf :CCSS.ELA-Literacy.L.3.2 ;
    rdfs:comment "Use commas and quotation marks in dialogue."^^xsd:string .

:CCSS.ELA-Literacy.L.3.2.d rdf:type owl:Class ;
    prov:wasQuotedFrom <http://www.corestandards.org/ELA-Literacy/L/3/2/d/> ;
    rdfs:subClassOf :CCSS.ELA-Literacy.L.3.2 ;
    rdfs:comment "Form and use possessives."^^xsd:string .

:CCSS.ELA-Literacy.L.3.2.e rdf:type owl:Class ;
    prov:wasQuotedFrom <http://www.corestandards.org/ELA-Literacy/L/3/2/e/> ;
    rdfs:subClassOf :CCSS.ELA-Literacy.L.3.2 ;
    rdfs:comment "Use conventional spelling for high-frequency and other studied words and for adding suffixes to base words (e.g., sitting, smiled, cries, happiness)."^^xsd:string .

:CCSS.ELA-Literacy.L.3.2.f rdf:type owl:Class ;
    prov:wasQuotedFrom <http://www.corestandards.org/ELA-Literacy/L/3/2/f/> ;
    rdfs:subClassOf :CCSS.ELA-Literacy.L.3.2 ;
    rdfs:comment "Use spelling patterns and generalizations (e.g., word families, position-based spellings, syllable patterns, ending rules, meaningful word parts) in writing words."^^xsd:string .

:CCSS.ELA-Literacy.L.3.2.g rdf:type owl:Class ;
    prov:wasQuotedFrom <http://www.corestandards.org/ELA-Literacy/L/3/2/g/> ;
    rdfs:subClassOf :CCSS.ELA-Literacy.L.3.2 ;
    rdfs:comment "Consult reference materials, including beginning dictionaries, as needed to check and correct spellings."^^xsd:string .

:CCSS.ELA-Literacy.L.3.3 rdf:type owl:Class ;
    prov:wasQuotedFrom <http://www.corestandards.org/ELA-Literacy/L/3/3/> ;
    rdfs:subClassOf :CCSS.ELA-Literacy.L.3 ;
    rdfs:comment "Use knowledge of language and its conventions when writing, speaking, reading, or listening."^^xsd:string .

:CCSS.ELA-Literacy.L.3.3.a rdf:type owl:Class ;
    prov:wasQuotedFrom <http://www.corestandards.org/ELA-Literacy/L/3/3/a/> ;
    rdfs:subClassOf :CCSS.ELA-Literacy.L.3.3 ;
    rdfs:comment "Choose words and phrases for effect.*"^^xsd:string .

:CCSS.ELA-Literacy.L.3.3.b rdf:type owl:Class ;
    prov:wasQuotedFrom <http://www.corestandards.org/ELA-Literacy/L/3/3/b/> ;
    rdfs:subClassOf :CCSS.ELA-Literacy.L.3.3 ;
    rdfs:comment "Recognize and observe differences between the conventions of spoken and written standard English."^^xsd:string .

:CCSS.ELA-Literacy.L.3.4 rdf:type owl:Class ;
    prov:wasQuotedFrom <http://www.corestandards.org/ELA-Literacy/L/3/4/> ;
    rdfs:subClassOf :CCSS.ELA-Literacy.L.3 ;
    rdfs:comment "Determine or clarify the meaning of unknown and multiple-meaning word and phrases based on grade 3 reading and content, choosing flexibly from a range of strategies."^^xsd:string .

:CCSS.ELA-Literacy.L.3.4.a rdf:type owl:Class ;
    prov:wasQuotedFrom <http://www.corestandards.org/ELA-Literacy/L/3/4/a/> ;
    rdfs:subClassOf :CCSS.ELA-Literacy.L.3.4 ;
    rdfs:comment "Use sentence-level context as a clue to the meaning of a word or phrase."^^xsd:string .

:CCSS.ELA-Literacy.L.3.4.b rdf:type owl:Class ;
    prov:wasQuotedFrom <http://www.corestandards.org/ELA-Literacy/L/3/4/b/> ;
    rdfs:subClassOf :CCSS.ELA-Literacy.L.3.4 ;
    rdfs:comment "Determine the meaning of the new word formed when a known affix is added to a known word (e.g., agreeable/disagreeable, comfortable/uncomfortable, care/careless, heat/preheat)."^^xsd:string .

:CCSS.ELA-Literacy.L.3.4.c rdf:type owl:Class ;
    prov:wasQuotedFrom <http://www.corestandards.org/ELA-Literacy/L/3/4/c/> ;
    rdfs:subClassOf :CCSS.ELA-Literacy.L.3.4 ;
    rdfs:comment "Use a known root word as a clue to the meaning of an unknown word with the same root (e.g., company, companion)."^^xsd:string .

:CCSS.ELA-Literacy.L.3.4.d rdf:type owl:Class ;
    prov:wasQuotedFrom <http://www.corestandards.org/ELA-Literacy/L/3/4/d/> ;
    rdfs:subClassOf :CCSS.ELA-Literacy.L.3.4 ;
    rdfs:comment "Use glossaries or beginning dictionaries, both print and digital, to determine or clarify the precise meaning of key words and phrases."^^xsd:string .

:CCSS.ELA-Literacy.L.3.5 rdf:type owl:Class ;
    prov:wasQuotedFrom <http://www.corestandards.org/ELA-Literacy/L/3/5/> ;
    rdfs:subClassOf :CCSS.ELA-Literacy.L.3 ;
    rdfs:comment "Demonstrate understanding of figurative language, word relationships and nuances in word meanings."^^xsd:string .

:CCSS.ELA-Literacy.L.3.5.a rdf:type owl:Class ;
    prov:wasQuotedFrom <http://www.corestandards.org/ELA-Literacy/L/3/5/a/> ;
    rdfs:subClassOf :CCSS.ELA-Literacy.L.3.5 ;
    rdfs:comment "Distinguish the literal and nonliteral meanings of words and phrases in context (e.g., take steps)."^^xsd:string .

:CCSS.ELA-Literacy.L.3.5.b rdf:type owl:Class ;
    prov:wasQuotedFrom <http://www.corestandards.org/ELA-Literacy/L/3/5/b/> ;
    rdfs:subClassOf :CCSS.ELA-Literacy.L.3.5 ;
    rdfs:comment "Identify real-life connections between words and their use (e.g., describe people who are friendly or helpful)."^^xsd:string .

:CCSS.ELA-Literacy.L.3.5.c rdf:type owl:Class ;
    prov:wasQuotedFrom <http://www.corestandards.org/ELA-Literacy/L/3/5/c/> ;
    rdfs:subClassOf :CCSS.ELA-Literacy.L.3.5 ;
    rdfs:comment "Distinguish shades of meaning among related words that describe states of mind or degrees of certainty (e.g., knew, believed, suspected, heard, wondered)."^^xsd:string .

:CCSS.ELA-Literacy.L.3.6 rdf:type owl:Class ;
    prov:wasQuotedFrom <http://www.corestandards.org/ELA-Literacy/L/3/6/> ;
    rdfs:subClassOf :CCSS.ELA-Literacy.L.3 ;
    rdfs:comment "Acquire and use accurately grade-appropriate conversational, general academic, and domain-specific words and phrases, including those that signal spatial and temporal relationships (e.g., After dinner that night we went looking for them)."^^xsd:string .

:CCSS.ELA-Literacy.L.4.1 rdf:type owl:Class ;
    prov:wasQuotedFrom <http://www.corestandards.org/ELA-Literacy/L/4/1/> ;
    rdfs:subClassOf :CCSS.ELA-Literacy.L.4 ;
    rdfs:comment "Demonstrate command of the conventions of standard English grammar and usage when writing or speaking."^^xsd:string .

:CCSS.ELA-Literacy.L.4.1.a rdf:type owl:Class ;
    prov:wasQuotedFrom <http://www.corestandards.org/ELA-Literacy/L/4/1/a/> ;
    rdfs:subClassOf :CCSS.ELA-Literacy.L.4.1 ;
    rdfs:comment "Use relative pronouns (who, whose, whom, which, that) and relative adverbs (where, when, why)."^^xsd:string .

:CCSS.ELA-Literacy.L.4.1.b rdf:type owl:Class ;
    prov:wasQuotedFrom <http://www.corestandards.org/ELA-Literacy/L/4/1/b/> ;
    rdfs:subClassOf :CCSS.ELA-Literacy.L.4.1 ;
    rdfs:comment "Form and use the progressive (e.g., I was walking; I am walking; I will be walking) verb tenses."^^xsd:string .

:CCSS.ELA-Literacy.L.4.1.c rdf:type owl:Class ;
    prov:wasQuotedFrom <http://www.corestandards.org/ELA-Literacy/L/4/1/c/> ;
    rdfs:subClassOf :CCSS.ELA-Literacy.L.4.1 ;
    rdfs:comment "Use modal auxiliaries (e.g., can, may, must) to convey various conditions."^^xsd:string .

:CCSS.ELA-Literacy.L.4.1.d rdf:type owl:Class ;
    prov:wasQuotedFrom <http://www.corestandards.org/ELA-Literacy/L/4/1/d/> ;
    rdfs:subClassOf :CCSS.ELA-Literacy.L.4.1 ;
    rdfs:comment "Order adjectives within sentences according to conventional patterns (e.g., a small red bag rather than a red small bag)."^^xsd:string .

:CCSS.ELA-Literacy.L.4.1.e rdf:type owl:Class ;
    prov:wasQuotedFrom <http://www.corestandards.org/ELA-Literacy/L/4/1/e/> ;
    rdfs:subClassOf :CCSS.ELA-Literacy.L.4.1 ;
    rdfs:comment "Form and use prepositional phrases."^^xsd:string .

:CCSS.ELA-Literacy.L.4.1.f rdf:type owl:Class ;
    prov:wasQuotedFrom <http://www.corestandards.org/ELA-Literacy/L/4/1/f/> ;
    rdfs:subClassOf :CCSS.ELA-Literacy.L.4.1 ;
    rdfs:comment "Produce complete sentences, recognizing and correcting inappropriate fragments and run-ons.*"^^xsd:string .

:CCSS.ELA-Literacy.L.4.1.g rdf:type owl:Class ;
    prov:wasQuotedFrom <http://www.corestandards.org/ELA-Literacy/L/4/1/g/> ;
    rdfs:subClassOf :CCSS.ELA-Literacy.L.4.1 ;
    rdfs:comment "Correctly use frequently confused words (e.g., to, too, two; there, their).*"^^xsd:string .

:CCSS.ELA-Literacy.L.4.2 rdf:type owl:Class ;
    prov:wasQuotedFrom <http://www.corestandards.org/ELA-Literacy/L/4/2/> ;
    rdfs:subClassOf :CCSS.ELA-Literacy.L.4 ;
    rdfs:comment "Demonstrate command of the conventions of standard English capitalization, punctuation, and spelling when writing."^^xsd:string .

:CCSS.ELA-Literacy.L.4.2.a rdf:type owl:Class ;
    prov:wasQuotedFrom <http://www.corestandards.org/ELA-Literacy/L/4/2/a/> ;
    rdfs:subClassOf :CCSS.ELA-Literacy.L.4.2 ;
    rdfs:comment "Use correct capitalization."^^xsd:string .

:CCSS.ELA-Literacy.L.4.2.b rdf:type owl:Class ;
    prov:wasQuotedFrom <http://www.corestandards.org/ELA-Literacy/L/4/2/b/> ;
    rdfs:subClassOf :CCSS.ELA-Literacy.L.4.2 ;
    rdfs:comment "Use commas and quotation marks to mark direct speech and quotations from a text."^^xsd:string .

:CCSS.ELA-Literacy.L.4.2.c rdf:type owl:Class ;
    prov:wasQuotedFrom <http://www.corestandards.org/ELA-Literacy/L/4/2/c/> ;
    rdfs:subClassOf :CCSS.ELA-Literacy.L.4.2 ;
    rdfs:comment "Use a comma before a coordinating conjunction in a compound sentence."^^xsd:string .

:CCSS.ELA-Literacy.L.4.2.d rdf:type owl:Class ;
    prov:wasQuotedFrom <http://www.corestandards.org/ELA-Literacy/L/4/2/d/> ;
    rdfs:subClassOf :CCSS.ELA-Literacy.L.4.2 ;
    rdfs:comment "Spell grade-appropriate words correctly, consulting references as needed."^^xsd:string .

:CCSS.ELA-Literacy.L.4.3 rdf:type owl:Class ;
    prov:wasQuotedFrom <http://www.corestandards.org/ELA-Literacy/L/4/3/> ;
    rdfs:subClassOf :CCSS.ELA-Literacy.L.4 ;
    rdfs:comment "Use knowledge of language and its conventions when writing, speaking, reading, or listening."^^xsd:string .

:CCSS.ELA-Literacy.L.4.3.a rdf:type owl:Class ;
    prov:wasQuotedFrom <http://www.corestandards.org/ELA-Literacy/L/4/3/a/> ;
    rdfs:subClassOf :CCSS.ELA-Literacy.L.4.3 ;
    rdfs:comment "Choose words and phrases to convey ideas precisely.*"^^xsd:string .

:CCSS.ELA-Literacy.L.4.3.b rdf:type owl:Class ;
    prov:wasQuotedFrom <http://www.corestandards.org/ELA-Literacy/L/4/3/b/> ;
    rdfs:subClassOf :CCSS.ELA-Literacy.L.4.3 ;
    rdfs:comment "Choose punctuation for effect.*"^^xsd:string .

:CCSS.ELA-Literacy.L.4.3.c rdf:type owl:Class ;
    prov:wasQuotedFrom <http://www.corestandards.org/ELA-Literacy/L/4/3/c/> ;
    rdfs:subClassOf :CCSS.ELA-Literacy.L.4.3 ;
    rdfs:comment "Differentiate between contexts that call for formal English (e.g., presenting ideas) and situations where informal discourse is appropriate (e.g., small-group discussion)."^^xsd:string .

:CCSS.ELA-Literacy.L.4.4 rdf:type owl:Class ;
    prov:wasQuotedFrom <http://www.corestandards.org/ELA-Literacy/L/4/4/> ;
    rdfs:subClassOf :CCSS.ELA-Literacy.L.4 ;
    rdfs:comment "Determine or clarify the meaning of unknown and multiple-meaning words and phrases based on grade 4 reading and content, choosing flexibly from a range of strategies."^^xsd:string .

:CCSS.ELA-Literacy.L.4.4.a rdf:type owl:Class ;
    prov:wasQuotedFrom <http://www.corestandards.org/ELA-Literacy/L/4/4/a/> ;
    rdfs:subClassOf :CCSS.ELA-Literacy.L.4.4 ;
    rdfs:comment "Use context (e.g., definitions, examples, or restatements in text) as a clue to the meaning of a word or phrase."^^xsd:string .

:CCSS.ELA-Literacy.L.4.4.b rdf:type owl:Class ;
    prov:wasQuotedFrom <http://www.corestandards.org/ELA-Literacy/L/4/4/b/> ;
    rdfs:subClassOf :CCSS.ELA-Literacy.L.4.4 ;
    rdfs:comment "Use common, grade-appropriate Greek and Latin affixes and roots as clues to the meaning of a word (e.g., telegraph, photograph, autograph)."^^xsd:string .

:CCSS.ELA-Literacy.L.4.4.c rdf:type owl:Class ;
    prov:wasQuotedFrom <http://www.corestandards.org/ELA-Literacy/L/4/4/c/> ;
    rdfs:subClassOf :CCSS.ELA-Literacy.L.4.4 ;
    rdfs:comment "Consult reference materials (e.g., dictionaries, glossaries, thesauruses), both print and digital, to find the pronunciation and determine or clarify the precise meaning of key words and phrases."^^xsd:string .

:CCSS.ELA-Literacy.L.4.5 rdf:type owl:Class ;
    prov:wasQuotedFrom <http://www.corestandards.org/ELA-Literacy/L/4/5/> ;
    rdfs:subClassOf :CCSS.ELA-Literacy.L.4 ;
    rdfs:comment "Demonstrate understanding of figurative language, word relationships, and nuances in word meanings."^^xsd:string .

:CCSS.ELA-Literacy.L.4.5.a rdf:type owl:Class ;
    prov:wasQuotedFrom <http://www.corestandards.org/ELA-Literacy/L/4/5/a/> ;
    rdfs:subClassOf :CCSS.ELA-Literacy.L.4.5 ;
    rdfs:comment "Explain the meaning of simple similes and metaphors (e.g., as pretty as a picture) in context."^^xsd:string .

:CCSS.ELA-Literacy.L.4.5.b rdf:type owl:Class ;
    prov:wasQuotedFrom <http://www.corestandards.org/ELA-Literacy/L/4/5/b/> ;
    rdfs:subClassOf :CCSS.ELA-Literacy.L.4.5 ;
    rdfs:comment "Recognize and explain the meaning of common idioms, adages, and proverbs."^^xsd:string .

:CCSS.ELA-Literacy.L.4.5.c rdf:type owl:Class ;
    prov:wasQuotedFrom <http://www.corestandards.org/ELA-Literacy/L/4/5/c/> ;
    rdfs:subClassOf :CCSS.ELA-Literacy.L.4.5 ;
    rdfs:comment "Demonstrate understanding of words by relating them to their opposites (antonyms) and to words with similar but not identical meanings (synonyms). "^^xsd:string .

:CCSS.ELA-Literacy.L.4.6 rdf:type owl:Class ;
    prov:wasQuotedFrom <http://www.corestandards.org/ELA-Literacy/L/4/6/> ;
    rdfs:subClassOf :CCSS.ELA-Literacy.L.4 ;
    rdfs:comment "Acquire and use accurately grade-appropriate general academic and domain-specific words and phrases, including those that signal precise actions, emotions, or states of being (e.g., quizzed, whined, stammered) and that are basic to a particular topic (e.g., wildlife, conservation, and endangered when discussing animal preservation)."^^xsd:string .

:CCSS.ELA-Literacy.L.5.1 rdf:type owl:Class ;
    prov:wasQuotedFrom <http://www.corestandards.org/ELA-Literacy/L/5/1/> ;
    rdfs:subClassOf :CCSS.ELA-Literacy.L.5 ;
    rdfs:comment "Demonstrate command of the conventions of standard English grammar and usage when writing or speaking."^^xsd:string .

:CCSS.ELA-Literacy.L.5.1.a rdf:type owl:Class ;
    prov:wasQuotedFrom <http://www.corestandards.org/ELA-Literacy/L/5/1/a/> ;
    rdfs:subClassOf :CCSS.ELA-Literacy.L.5.1 ;
    rdfs:comment "Explain the function of conjunctions, prepositions, and interjections in general and their function in particular sentences."^^xsd:string .

:CCSS.ELA-Literacy.L.5.1.b rdf:type owl:Class ;
    prov:wasQuotedFrom <http://www.corestandards.org/ELA-Literacy/L/5/1/b/> ;
    rdfs:subClassOf :CCSS.ELA-Literacy.L.5.1 ;
    rdfs:comment "Form and use the perfect (e.g., I had walked; I have walked; I will have walked) verb tenses."^^xsd:string .

:CCSS.ELA-Literacy.L.5.1.c rdf:type owl:Class ;
    prov:wasQuotedFrom <http://www.corestandards.org/ELA-Literacy/L/5/1/c/> ;
    rdfs:subClassOf :CCSS.ELA-Literacy.L.5.1 ;
    rdfs:comment "Use verb tense to convey various times, sequences, states, and conditions."^^xsd:string .

:CCSS.ELA-Literacy.L.5.1.d rdf:type owl:Class ;
    prov:wasQuotedFrom <http://www.corestandards.org/ELA-Literacy/L/5/1/d/> ;
    rdfs:subClassOf :CCSS.ELA-Literacy.L.5.1 ;
    rdfs:comment "Recognize and correct inappropriate shifts in verb tense.*"^^xsd:string .

:CCSS.ELA-Literacy.L.5.1.e rdf:type owl:Class ;
    prov:wasQuotedFrom <http://www.corestandards.org/ELA-Literacy/L/5/1/e/> ;
    rdfs:subClassOf :CCSS.ELA-Literacy.L.5.1 ;
    rdfs:comment "Use correlative conjunctions (e.g., either/or, neither/nor)."^^xsd:string .

:CCSS.ELA-Literacy.L.5.2 rdf:type owl:Class ;
    prov:wasQuotedFrom <http://www.corestandards.org/ELA-Literacy/L/5/2/> ;
    rdfs:subClassOf :CCSS.ELA-Literacy.L.5 ;
    rdfs:comment "Demonstrate command of the conventions of standard English capitalization, punctuation, and spelling when writing."^^xsd:string .

:CCSS.ELA-Literacy.L.5.2.a rdf:type owl:Class ;
    prov:wasQuotedFrom <http://www.corestandards.org/ELA-Literacy/L/5/2/a/> ;
    rdfs:subClassOf :CCSS.ELA-Literacy.L.5.2 ;
    rdfs:comment "Use punctuation to separate items in a series.*"^^xsd:string .

:CCSS.ELA-Literacy.L.5.2.b rdf:type owl:Class ;
    prov:wasQuotedFrom <http://www.corestandards.org/ELA-Literacy/L/5/2/b/> ;
    rdfs:subClassOf :CCSS.ELA-Literacy.L.5.2 ;
    rdfs:comment "Use a comma to separate an introductory element from the rest of the sentence."^^xsd:string .

:CCSS.ELA-Literacy.L.5.2.c rdf:type owl:Class ;
    prov:wasQuotedFrom <http://www.corestandards.org/ELA-Literacy/L/5/2/c/> ;
    rdfs:subClassOf :CCSS.ELA-Literacy.L.5.2 ;
    rdfs:comment "Use a comma to set off the words yes and no (e.g., Yes, thank you), to set off a tag question from the rest of the sentence (e.g., It's true, isn't it?), and to indicate direct address (e.g., Is that you, Steve?)."^^xsd:string .

:CCSS.ELA-Literacy.L.5.2.d rdf:type owl:Class ;
    prov:wasQuotedFrom <http://www.corestandards.org/ELA-Literacy/L/5/2/d/> ;
    rdfs:subClassOf :CCSS.ELA-Literacy.L.5.2 ;
    rdfs:comment "Use underlining, quotation marks, or italics to indicate titles of works."^^xsd:string .

:CCSS.ELA-Literacy.L.5.2.e rdf:type owl:Class ;
    prov:wasQuotedFrom <http://www.corestandards.org/ELA-Literacy/L/5/2/e/> ;
    rdfs:subClassOf :CCSS.ELA-Literacy.L.5.2 ;
    rdfs:comment "Spell grade-appropriate words correctly, consulting references as needed."^^xsd:string .

:CCSS.ELA-Literacy.L.5.3 rdf:type owl:Class ;
    prov:wasQuotedFrom <http://www.corestandards.org/ELA-Literacy/L/5/3/> ;
    rdfs:subClassOf :CCSS.ELA-Literacy.L.5 ;
    rdfs:comment "Use knowledge of language and its conventions when writing, speaking, reading, or listening."^^xsd:string .

:CCSS.ELA-Literacy.L.5.3.a rdf:type owl:Class ;
    prov:wasQuotedFrom <http://www.corestandards.org/ELA-Literacy/L/5/3/a/> ;
    rdfs:subClassOf :CCSS.ELA-Literacy.L.5.3 ;
    rdfs:comment "Expand, combine, and reduce sentences for meaning, reader/listener interest, and style."^^xsd:string .

:CCSS.ELA-Literacy.L.5.3.b rdf:type owl:Class ;
    prov:wasQuotedFrom <http://www.corestandards.org/ELA-Literacy/L/5/3/b/> ;
    rdfs:subClassOf :CCSS.ELA-Literacy.L.5.3 ;
    rdfs:comment "Compare and contrast the varieties of English (e.g., dialects, registers) used in stories, dramas, or poems."^^xsd:string .

:CCSS.ELA-Literacy.L.5.4 rdf:type owl:Class ;
    prov:wasQuotedFrom <http://www.corestandards.org/ELA-Literacy/L/5/4/> ;
    rdfs:subClassOf :CCSS.ELA-Literacy.L.5 ;
    rdfs:comment "Determine or clarify the meaning of unknown and multiple-meaning words and phrases based on grade 5 reading and content, choosing flexibly from a range of strategies."^^xsd:string .

:CCSS.ELA-Literacy.L.5.4.a rdf:type owl:Class ;
    prov:wasQuotedFrom <http://www.corestandards.org/ELA-Literacy/L/5/4/a/> ;
    rdfs:subClassOf :CCSS.ELA-Literacy.L.5.4 ;
    rdfs:comment "Use context (e.g., cause/effect relationships and comparisons in text) as a clue to the meaning of a word or phrase."^^xsd:string .

:CCSS.ELA-Literacy.L.5.4.b rdf:type owl:Class ;
    prov:wasQuotedFrom <http://www.corestandards.org/ELA-Literacy/L/5/4/b/> ;
    rdfs:subClassOf :CCSS.ELA-Literacy.L.5.4 ;
    rdfs:comment "Use common, grade-appropriate Greek and Latin affixes and roots as clues to the meaning of a word (e.g., photograph, photosynthesis)."^^xsd:string .

:CCSS.ELA-Literacy.L.5.4.c rdf:type owl:Class ;
    prov:wasQuotedFrom <http://www.corestandards.org/ELA-Literacy/L/5/4/c/> ;
    rdfs:subClassOf :CCSS.ELA-Literacy.L.5.4 ;
    rdfs:comment "Consult reference materials (e.g., dictionaries, glossaries, thesauruses), both print and digital, to find the pronunciation and determine or clarify the precise meaning of key words and phrases."^^xsd:string .

:CCSS.ELA-Literacy.L.5.5 rdf:type owl:Class ;
    prov:wasQuotedFrom <http://www.corestandards.org/ELA-Literacy/L/5/5/> ;
    rdfs:subClassOf :CCSS.ELA-Literacy.L.5 ;
    rdfs:comment "Demonstrate understanding of figurative language, word relationships, and nuances in word meanings."^^xsd:string .

:CCSS.ELA-Literacy.L.5.5.a rdf:type owl:Class ;
    prov:wasQuotedFrom <http://www.corestandards.org/ELA-Literacy/L/5/5/a/> ;
    rdfs:subClassOf :CCSS.ELA-Literacy.L.5.5 ;
    rdfs:comment "Interpret figurative language, including similes and metaphors, in context."^^xsd:string .

:CCSS.ELA-Literacy.L.5.5.b rdf:type owl:Class ;
    prov:wasQuotedFrom <http://www.corestandards.org/ELA-Literacy/L/5/5/b/> ;
    rdfs:subClassOf :CCSS.ELA-Literacy.L.5.5 ;
    rdfs:comment "Recognize and explain the meaning of common idioms, adages, and proverbs."^^xsd:string .

:CCSS.ELA-Literacy.L.5.5.c rdf:type owl:Class ;
    prov:wasQuotedFrom <http://www.corestandards.org/ELA-Literacy/L/5/5/c/> ;
    rdfs:subClassOf :CCSS.ELA-Literacy.L.5.5 ;
    rdfs:comment "Use the relationship between particular words (e.g., synonyms, antonyms, homographs) to better understand each of the words."^^xsd:string .

:CCSS.ELA-Literacy.L.5.6 rdf:type owl:Class ;
    prov:wasQuotedFrom <http://www.corestandards.org/ELA-Literacy/L/5/6/> ;
    rdfs:subClassOf :CCSS.ELA-Literacy.L.5 ;
    rdfs:comment "Acquire and use accurately grade-appropriate general academic and domain-specific words and phrases, including those that signal contrast, addition, and other logical relationships (e.g., however, although, nevertheless, similarly, moreover, in addition)."^^xsd:string .

:CCSS.ELA-Literacy.L.6.1 rdf:type owl:Class ;
    prov:wasQuotedFrom <http://www.corestandards.org/ELA-Literacy/L/6/1/> ;
    rdfs:subClassOf :CCSS.ELA-Literacy.L.6 ;
    rdfs:comment "Demonstrate command of the conventions of standard English grammar and usage when writing or speaking."^^xsd:string .

:CCSS.ELA-Literacy.L.6.1.a rdf:type owl:Class ;
    prov:wasQuotedFrom <http://www.corestandards.org/ELA-Literacy/L/6/1/a/> ;
    rdfs:subClassOf :CCSS.ELA-Literacy.L.6.1 ;
    rdfs:comment "Ensure that pronouns are in the proper case (subjective, objective, possessive)."^^xsd:string .

:CCSS.ELA-Literacy.L.6.1.b rdf:type owl:Class ;
    prov:wasQuotedFrom <http://www.corestandards.org/ELA-Literacy/L/6/1/b/> ;
    rdfs:subClassOf :CCSS.ELA-Literacy.L.6.1 ;
    rdfs:comment "Use intensive pronouns (e.g., myself, ourselves)."^^xsd:string .

:CCSS.ELA-Literacy.L.6.1.c rdf:type owl:Class ;
    prov:wasQuotedFrom <http://www.corestandards.org/ELA-Literacy/L/6/1/c/> ;
    rdfs:subClassOf :CCSS.ELA-Literacy.L.6.1 ;
    rdfs:comment "Recognize and correct inappropriate shifts in pronoun number and person.*"^^xsd:string .

:CCSS.ELA-Literacy.L.6.1.d rdf:type owl:Class ;
    prov:wasQuotedFrom <http://www.corestandards.org/ELA-Literacy/L/6/1/d/> ;
    rdfs:subClassOf :CCSS.ELA-Literacy.L.6.1 ;
    rdfs:comment "Recognize and correct vague pronouns (i.e., ones with unclear or ambiguous antecedents).*"^^xsd:string .

:CCSS.ELA-Literacy.L.6.1.e rdf:type owl:Class ;
    prov:wasQuotedFrom <http://www.corestandards.org/ELA-Literacy/L/6/1/e/> ;
    rdfs:subClassOf :CCSS.ELA-Literacy.L.6.1 ;
    rdfs:comment "Recognize variations from standard English in their own and others' writing and speaking, and identify and use strategies to improve expression in conventional language.*"^^xsd:string .

:CCSS.ELA-Literacy.L.6.2 rdf:type owl:Class ;
    prov:wasQuotedFrom <http://www.corestandards.org/ELA-Literacy/L/6/2/> ;
    rdfs:subClassOf :CCSS.ELA-Literacy.L.6 ;
    rdfs:comment "Demonstrate command of the conventions of standard English capitalization, punctuation, and spelling when writing."^^xsd:string .

:CCSS.ELA-Literacy.L.6.2.a rdf:type owl:Class ;
    prov:wasQuotedFrom <http://www.corestandards.org/ELA-Literacy/L/6/2/a/> ;
    rdfs:subClassOf :CCSS.ELA-Literacy.L.6.2 ;
    rdfs:comment "Use punctuation (commas, parentheses, dashes) to set off nonrestrictive/parenthetical elements.*  "^^xsd:string .

:CCSS.ELA-Literacy.L.6.2.b rdf:type owl:Class ;
    prov:wasQuotedFrom <http://www.corestandards.org/ELA-Literacy/L/6/2/b/> ;
    rdfs:subClassOf :CCSS.ELA-Literacy.L.6.2 ;
    rdfs:comment "Spell correctly."^^xsd:string .

:CCSS.ELA-Literacy.L.6.3 rdf:type owl:Class ;
    prov:wasQuotedFrom <http://www.corestandards.org/ELA-Literacy/L/6/3/> ;
    rdfs:subClassOf :CCSS.ELA-Literacy.L.6 ;
    rdfs:comment "Use knowledge of language and its conventions when writing, speaking, reading, or listening."^^xsd:string .

:CCSS.ELA-Literacy.L.6.3.a rdf:type owl:Class ;
    prov:wasQuotedFrom <http://www.corestandards.org/ELA-Literacy/L/6/3/a/> ;
    rdfs:subClassOf :CCSS.ELA-Literacy.L.6.3 ;
    rdfs:comment "Vary sentence patterns for meaning, reader/listener interest, and style.*"^^xsd:string .

:CCSS.ELA-Literacy.L.6.3.b rdf:type owl:Class ;
    prov:wasQuotedFrom <http://www.corestandards.org/ELA-Literacy/L/6/3/b/> ;
    rdfs:subClassOf :CCSS.ELA-Literacy.L.6.3 ;
    rdfs:comment "Maintain consistency in style and tone.*"^^xsd:string .

:CCSS.ELA-Literacy.L.6.4 rdf:type owl:Class ;
    prov:wasQuotedFrom <http://www.corestandards.org/ELA-Literacy/L/6/4/> ;
    rdfs:subClassOf :CCSS.ELA-Literacy.L.6 ;
    rdfs:comment "Determine or clarify the meaning of unknown and multiple-meaning words and phrases based on grade 6 reading and content, choosing flexibly from a range of strategies."^^xsd:string .

:CCSS.ELA-Literacy.L.6.4.a rdf:type owl:Class ;
    prov:wasQuotedFrom <http://www.corestandards.org/ELA-Literacy/L/6/4/a/> ;
    rdfs:subClassOf :CCSS.ELA-Literacy.L.6.4 ;
    rdfs:comment "Use context (e.g., the overall meaning of a sentence or paragraph; a word's position or function in a sentence) as a clue to the meaning of a word or phrase."^^xsd:string .

:CCSS.ELA-Literacy.L.6.4.b rdf:type owl:Class ;
    prov:wasQuotedFrom <http://www.corestandards.org/ELA-Literacy/L/6/4/b/> ;
    rdfs:subClassOf :CCSS.ELA-Literacy.L.6.4 ;
    rdfs:comment "Use common, grade-appropriate Greek or Latin affixes and roots as clues to the meaning of a word (e.g., audience, auditory, audible)."^^xsd:string .

:CCSS.ELA-Literacy.L.6.4.c rdf:type owl:Class ;
    prov:wasQuotedFrom <http://www.corestandards.org/ELA-Literacy/L/6/4/c/> ;
    rdfs:subClassOf :CCSS.ELA-Literacy.L.6.4 ;
    rdfs:comment "Consult reference materials (e.g., dictionaries, glossaries, thesauruses), both print and digital, to find the pronunciation of a word or determine or clarify its precise meaning or its part of speech."^^xsd:string .

:CCSS.ELA-Literacy.L.6.4.d rdf:type owl:Class ;
    prov:wasQuotedFrom <http://www.corestandards.org/ELA-Literacy/L/6/4/d/> ;
    rdfs:subClassOf :CCSS.ELA-Literacy.L.6.4 ;
    rdfs:comment "Verify the preliminary determination of the meaning of a word or phrase (e.g., by checking the inferred meaning in context or in a dictionary)."^^xsd:string .

:CCSS.ELA-Literacy.L.6.5 rdf:type owl:Class ;
    prov:wasQuotedFrom <http://www.corestandards.org/ELA-Literacy/L/6/5/> ;
    rdfs:subClassOf :CCSS.ELA-Literacy.L.6 ;
    rdfs:comment "Demonstrate understanding of figurative language, word relationships, and nuances in word meanings."^^xsd:string .

:CCSS.ELA-Literacy.L.6.5.a rdf:type owl:Class ;
    prov:wasQuotedFrom <http://www.corestandards.org/ELA-Literacy/L/6/5/a/> ;
    rdfs:subClassOf :CCSS.ELA-Literacy.L.6.5 ;
    rdfs:comment "Interpret figures of speech (e.g., personification) in context."^^xsd:string .

:CCSS.ELA-Literacy.L.6.5.b rdf:type owl:Class ;
    prov:wasQuotedFrom <http://www.corestandards.org/ELA-Literacy/L/6/5/b/> ;
    rdfs:subClassOf :CCSS.ELA-Literacy.L.6.5 ;
    rdfs:comment "Use the relationship between particular words (e.g., cause/effect, part/whole, item/category) to better understand each of the words."^^xsd:string .

:CCSS.ELA-Literacy.L.6.5.c rdf:type owl:Class ;
    prov:wasQuotedFrom <http://www.corestandards.org/ELA-Literacy/L/6/5/c/> ;
    rdfs:subClassOf :CCSS.ELA-Literacy.L.6.5 ;
    rdfs:comment "Distinguish among the connotations (associations) of words with similar denotations (definitions) (e.g., stingy, scrimping, economical, unwasteful, thrifty)."^^xsd:string .

:CCSS.ELA-Literacy.L.6.6 rdf:type owl:Class ;
    prov:wasQuotedFrom <http://www.corestandards.org/ELA-Literacy/L/6/6/> ;
    rdfs:subClassOf :CCSS.ELA-Literacy.L.6 ;
    rdfs:comment "Acquire and use accurately grade-appropriate general academic and domain-specific words and phrases; gather vocabulary knowledge when considering a word or phrase important to comprehension or expression."^^xsd:string .

:CCSS.ELA-Literacy.L.7.1 rdf:type owl:Class ;
    prov:wasQuotedFrom <http://www.corestandards.org/ELA-Literacy/L/7/1/> ;
    rdfs:subClassOf :CCSS.ELA-Literacy.L.7 ;
    rdfs:comment "Demonstrate command of the conventions of standard English grammar and usage when writing or speaking."^^xsd:string .

:CCSS.ELA-Literacy.L.7.1.a rdf:type owl:Class ;
    prov:wasQuotedFrom <http://www.corestandards.org/ELA-Literacy/L/7/1/a/> ;
    rdfs:subClassOf :CCSS.ELA-Literacy.L.7.1 ;
    rdfs:comment "Explain the function of phrases and clauses in general and their function in specific sentences."^^xsd:string .

:CCSS.ELA-Literacy.L.7.1.b rdf:type owl:Class ;
    prov:wasQuotedFrom <http://www.corestandards.org/ELA-Literacy/L/7/1/b/> ;
    rdfs:subClassOf :CCSS.ELA-Literacy.L.7.1 ;
    rdfs:comment "Choose among simple, compound, complex, and compound-complex sentences to signal differing relationships among ideas."^^xsd:string .

:CCSS.ELA-Literacy.L.7.1.c rdf:type owl:Class ;
    prov:wasQuotedFrom <http://www.corestandards.org/ELA-Literacy/L/7/1/c/> ;
    rdfs:subClassOf :CCSS.ELA-Literacy.L.7.1 ;
    rdfs:comment "Place phrases and clauses within a sentence, recognizing and correcting misplaced and dangling modifiers.*"^^xsd:string .

:CCSS.ELA-Literacy.L.7.2 rdf:type owl:Class ;
    prov:wasQuotedFrom <http://www.corestandards.org/ELA-Literacy/L/7/2/> ;
    rdfs:subClassOf :CCSS.ELA-Literacy.L.7 ;
    rdfs:comment " Demonstrate command of the conventions of standard English capitalization, punctuation, and spelling when writing."^^xsd:string .

:CCSS.ELA-Literacy.L.7.2.a rdf:type owl:Class ;
    prov:wasQuotedFrom <http://www.corestandards.org/ELA-Literacy/L/7/2/a/> ;
    rdfs:subClassOf :CCSS.ELA-Literacy.L.7.2 ;
    rdfs:comment "Use a comma to separate coordinate adjectives (e.g., It was a fascinating, enjoyable movie but not He wore an old[,] green shirt)."^^xsd:string .

:CCSS.ELA-Literacy.L.7.2.b rdf:type owl:Class ;
    prov:wasQuotedFrom <http://www.corestandards.org/ELA-Literacy/L/7/2/b/> ;
    rdfs:subClassOf :CCSS.ELA-Literacy.L.7.2 ;
    rdfs:comment "Spell correctly."^^xsd:string .

:CCSS.ELA-Literacy.L.7.3 rdf:type owl:Class ;
    prov:wasQuotedFrom <http://www.corestandards.org/ELA-Literacy/L/7/3/> ;
    rdfs:subClassOf :CCSS.ELA-Literacy.L.7 ;
    rdfs:comment "Use knowledge of language and its conventions when writing, speaking, reading, or listening."^^xsd:string .

:CCSS.ELA-Literacy.L.7.3.a rdf:type owl:Class ;
    prov:wasQuotedFrom <http://www.corestandards.org/ELA-Literacy/L/7/3/a/> ;
    rdfs:subClassOf :CCSS.ELA-Literacy.L.7.3 ;
    rdfs:comment "Choose language that expresses ideas precisely and concisely, recognizing and eliminating wordiness and redundancy.*"^^xsd:string .

:CCSS.ELA-Literacy.L.7.4 rdf:type owl:Class ;
    prov:wasQuotedFrom <http://www.corestandards.org/ELA-Literacy/L/7/4/> ;
    rdfs:subClassOf :CCSS.ELA-Literacy.L.7 ;
    rdfs:comment "Determine or clarify the meaning of unknown and multiple-meaning words and phrases based on grade 7 reading and content, choosing flexibly from a range of strategies."^^xsd:string .

:CCSS.ELA-Literacy.L.7.4.a rdf:type owl:Class ;
    prov:wasQuotedFrom <http://www.corestandards.org/ELA-Literacy/L/7/4/a/> ;
    rdfs:subClassOf :CCSS.ELA-Literacy.L.7.4 ;
    rdfs:comment "Use context (e.g., the overall meaning of a sentence or paragraph; a word's position or function in a sentence) as a clue to the meaning of a word or phrase."^^xsd:string .

:CCSS.ELA-Literacy.L.7.4.b rdf:type owl:Class ;
    prov:wasQuotedFrom <http://www.corestandards.org/ELA-Literacy/L/7/4/b/> ;
    rdfs:subClassOf :CCSS.ELA-Literacy.L.7.4 ;
    rdfs:comment "Use common, grade-appropriate Greek or Latin affixes and roots as clues to the meaning of a word (e.g., belligerent, bellicose, rebel)."^^xsd:string .

:CCSS.ELA-Literacy.L.7.4.c rdf:type owl:Class ;
    prov:wasQuotedFrom <http://www.corestandards.org/ELA-Literacy/L/7/4/c/> ;
    rdfs:subClassOf :CCSS.ELA-Literacy.L.7.4 ;
    rdfs:comment "Consult general and specialized reference materials (e.g., dictionaries, glossaries, thesauruses), both print and digital, to find the pronunciation of a word or determine or clarify its precise meaning or its part of speech."^^xsd:string .

:CCSS.ELA-Literacy.L.7.4.d rdf:type owl:Class ;
    prov:wasQuotedFrom <http://www.corestandards.org/ELA-Literacy/L/7/4/d/> ;
    rdfs:subClassOf :CCSS.ELA-Literacy.L.7.4 ;
    rdfs:comment "Verify the preliminary determination of the meaning of a word or phrase (e.g., by checking the inferred meaning in context or in a dictionary)."^^xsd:string .

:CCSS.ELA-Literacy.L.7.5 rdf:type owl:Class ;
    prov:wasQuotedFrom <http://www.corestandards.org/ELA-Literacy/L/7/5/> ;
    rdfs:subClassOf :CCSS.ELA-Literacy.L.7 ;
    rdfs:comment "Demonstrate understanding of figurative language, word relationships, and nuances in word meanings."^^xsd:string .

:CCSS.ELA-Literacy.L.7.5.a rdf:type owl:Class ;
    prov:wasQuotedFrom <http://www.corestandards.org/ELA-Literacy/L/7/5/a/> ;
    rdfs:subClassOf :CCSS.ELA-Literacy.L.7.5 ;
    rdfs:comment "Interpret figures of speech (e.g., literary, biblical, and mythological allusions) in context."^^xsd:string .

:CCSS.ELA-Literacy.L.7.5.b rdf:type owl:Class ;
    prov:wasQuotedFrom <http://www.corestandards.org/ELA-Literacy/L/7/5/b/> ;
    rdfs:subClassOf :CCSS.ELA-Literacy.L.7.5 ;
    rdfs:comment "Use the relationship between particular words (e.g., synonym/antonym, analogy) to better understand each of the words."^^xsd:string .

:CCSS.ELA-Literacy.L.7.5.c rdf:type owl:Class ;
    prov:wasQuotedFrom <http://www.corestandards.org/ELA-Literacy/L/7/5/c/> ;
    rdfs:subClassOf :CCSS.ELA-Literacy.L.7.5 ;
    rdfs:comment "Distinguish among the connotations (associations) of   words with similar denotations (definitions) (e.g., refined, respectful, polite, diplomatic, condescending)."^^xsd:string .

:CCSS.ELA-Literacy.L.7.6 rdf:type owl:Class ;
    prov:wasQuotedFrom <http://www.corestandards.org/ELA-Literacy/L/7/6/> ;
    rdfs:subClassOf :CCSS.ELA-Literacy.L.7 ;
    rdfs:comment "Acquire and use accurately grade-appropriate general academic and domain-specific words and phrases; gather vocabulary knowledge when considering a word or phrase important to comprehension or expression."^^xsd:string .

:CCSS.ELA-Literacy.L.8.1 rdf:type owl:Class ;
    prov:wasQuotedFrom <http://www.corestandards.org/ELA-Literacy/L/8/1/> ;
    rdfs:subClassOf :CCSS.ELA-Literacy.L.8 ;
    rdfs:comment "Demonstrate command of the conventions of standard English grammar and usage when writing or speaking."^^xsd:string .

:CCSS.ELA-Literacy.L.8.1.a rdf:type owl:Class ;
    prov:wasQuotedFrom <http://www.corestandards.org/ELA-Literacy/L/8/1/a/> ;
    rdfs:subClassOf :CCSS.ELA-Literacy.L.8.1 ;
    rdfs:comment "Explain the function of verbals (gerunds, participles, infinitives) in general and their function in particular sentences."^^xsd:string .

:CCSS.ELA-Literacy.L.8.1.b rdf:type owl:Class ;
    prov:wasQuotedFrom <http://www.corestandards.org/ELA-Literacy/L/8/1/b/> ;
    rdfs:subClassOf :CCSS.ELA-Literacy.L.8.1 ;
    rdfs:comment "Form and use verbs in the active and passive voice."^^xsd:string .

:CCSS.ELA-Literacy.L.8.1.c rdf:type owl:Class ;
    prov:wasQuotedFrom <http://www.corestandards.org/ELA-Literacy/L/8/1/c/> ;
    rdfs:subClassOf :CCSS.ELA-Literacy.L.8.1 ;
    rdfs:comment "Form and use verbs in the indicative, imperative, interrogative, conditional, and subjunctive mood. "^^xsd:string .

:CCSS.ELA-Literacy.L.8.1.d rdf:type owl:Class ;
    prov:wasQuotedFrom <http://www.corestandards.org/ELA-Literacy/L/8/1/d/> ;
    rdfs:subClassOf :CCSS.ELA-Literacy.L.8.1 ;
    rdfs:comment "Recognize and correct inappropriate shifts in verb voice and mood.*"^^xsd:string .

:CCSS.ELA-Literacy.L.8.2 rdf:type owl:Class ;
    prov:wasQuotedFrom <http://www.corestandards.org/ELA-Literacy/L/8/2/> ;
    rdfs:subClassOf :CCSS.ELA-Literacy.L.8 ;
    rdfs:comment "Demonstrate command of the conventions of standard English capitalization, punctuation, and spelling when writing."^^xsd:string .

:CCSS.ELA-Literacy.L.8.2.a rdf:type owl:Class ;
    prov:wasQuotedFrom <http://www.corestandards.org/ELA-Literacy/L/8/2/a/> ;
    rdfs:subClassOf :CCSS.ELA-Literacy.L.8.2 ;
    rdfs:comment "Use punctuation (comma, ellipsis, dash) to indicate a pause or break."^^xsd:string .

:CCSS.ELA-Literacy.L.8.2.b rdf:type owl:Class ;
    prov:wasQuotedFrom <http://www.corestandards.org/ELA-Literacy/L/8/2/b/> ;
    rdfs:subClassOf :CCSS.ELA-Literacy.L.8.2 ;
    rdfs:comment "Use an ellipsis to indicate an omission."^^xsd:string .

:CCSS.ELA-Literacy.L.8.2.c rdf:type owl:Class ;
    prov:wasQuotedFrom <http://www.corestandards.org/ELA-Literacy/L/8/2/c/> ;
    rdfs:subClassOf :CCSS.ELA-Literacy.L.8.2 ;
    rdfs:comment "Spell correctly."^^xsd:string .

:CCSS.ELA-Literacy.L.8.3 rdf:type owl:Class ;
    prov:wasQuotedFrom <http://www.corestandards.org/ELA-Literacy/L/8/3/> ;
    rdfs:subClassOf :CCSS.ELA-Literacy.L.8 ;
    rdfs:comment "Use knowledge of language and its conventions when writing, speaking, reading, or listening."^^xsd:string .

:CCSS.ELA-Literacy.L.8.3.a rdf:type owl:Class ;
    prov:wasQuotedFrom <http://www.corestandards.org/ELA-Literacy/L/8/3/a/> ;
    rdfs:subClassOf :CCSS.ELA-Literacy.L.8.3 ;
    rdfs:comment "Use verbs in the active and passive voice and in the conditional and subjunctive mood to achieve particular effects (e.g., emphasizing the actor or the action; expressing uncertainty or describing a state contrary to fact)."^^xsd:string .

:CCSS.ELA-Literacy.L.8.4 rdf:type owl:Class ;
    prov:wasQuotedFrom <http://www.corestandards.org/ELA-Literacy/L/8/4/> ;
    rdfs:subClassOf :CCSS.ELA-Literacy.L.8 ;
    rdfs:comment "Determine or clarify the meaning of unknown and multiple-meaning words or phrases based on grade 8 reading and content, choosing flexibly from a range of strategies."^^xsd:string .

:CCSS.ELA-Literacy.L.8.4.a rdf:type owl:Class ;
    prov:wasQuotedFrom <http://www.corestandards.org/ELA-Literacy/L/8/4/a/> ;
    rdfs:subClassOf :CCSS.ELA-Literacy.L.8.4 ;
    rdfs:comment "Use context (e.g., the overall meaning of a sentence or paragraph; a word's position or function in a sentence) as a clue to the meaning of a word or phrase."^^xsd:string .

:CCSS.ELA-Literacy.L.8.4.b rdf:type owl:Class ;
    prov:wasQuotedFrom <http://www.corestandards.org/ELA-Literacy/L/8/4/b/> ;
    rdfs:subClassOf :CCSS.ELA-Literacy.L.8.4 ;
    rdfs:comment "Use common, grade-appropriate Greek or Latin affixes and roots as clues to the meaning of a word (e.g., precede, recede, secede)."^^xsd:string .

:CCSS.ELA-Literacy.L.8.4.c rdf:type owl:Class ;
    prov:wasQuotedFrom <http://www.corestandards.org/ELA-Literacy/L/8/4/c/> ;
    rdfs:subClassOf :CCSS.ELA-Literacy.L.8.4 ;
    rdfs:comment "Consult general and specialized reference materials (e.g., dictionaries, glossaries, thesauruses), both print and digital, to find the pronunciation of a word or determine or clarify its precise meaning or its part of speech."^^xsd:string .

:CCSS.ELA-Literacy.L.8.4.d rdf:type owl:Class ;
    prov:wasQuotedFrom <http://www.corestandards.org/ELA-Literacy/L/8/4/d/> ;
    rdfs:subClassOf :CCSS.ELA-Literacy.L.8.4 ;
    rdfs:comment "Verify the preliminary determination of the meaning of a word or phrase (e.g., by checking the inferred meaning in context or in a dictionary)."^^xsd:string .

:CCSS.ELA-Literacy.L.8.5 rdf:type owl:Class ;
    prov:wasQuotedFrom <http://www.corestandards.org/ELA-Literacy/L/8/5/> ;
    rdfs:subClassOf :CCSS.ELA-Literacy.L.8 ;
    rdfs:comment "Demonstrate understanding of figurative language, word relationships, and nuances in word meanings."^^xsd:string .

:CCSS.ELA-Literacy.L.8.5.a rdf:type owl:Class ;
    prov:wasQuotedFrom <http://www.corestandards.org/ELA-Literacy/L/8/5/a/> ;
    rdfs:subClassOf :CCSS.ELA-Literacy.L.8.5 ;
    rdfs:comment "Interpret figures of speech (e.g. verbal irony, puns) in context."^^xsd:string .

:CCSS.ELA-Literacy.L.8.5.b rdf:type owl:Class ;
    prov:wasQuotedFrom <http://www.corestandards.org/ELA-Literacy/L/8/5/b/> ;
    rdfs:subClassOf :CCSS.ELA-Literacy.L.8.5 ;
    rdfs:comment "Use the relationship between particular words to better understand each of the words."^^xsd:string .

:CCSS.ELA-Literacy.L.8.5.c rdf:type owl:Class ;
    prov:wasQuotedFrom <http://www.corestandards.org/ELA-Literacy/L/8/5/c/> ;
    rdfs:subClassOf :CCSS.ELA-Literacy.L.8.5 ;
    rdfs:comment "Distinguish among the connotations (associations) of words with similar denotations (definitions) (e.g., bullheaded, willful, firm, persistent, resolute)."^^xsd:string .

:CCSS.ELA-Literacy.L.8.6 rdf:type owl:Class ;
    prov:wasQuotedFrom <http://www.corestandards.org/ELA-Literacy/L/8/6/> ;
    rdfs:subClassOf :CCSS.ELA-Literacy.L.8 ;
    rdfs:comment "Acquire and use accurately grade-appropriate general academic and domain-specific words and phrases; gather vocabulary knowledge when considering a word or phrase important to comprehension or expression."^^xsd:string .

:CCSS.ELA-Literacy.L.9-10.1 rdf:type owl:Class ;
    prov:wasQuotedFrom <http://www.corestandards.org/ELA-Literacy/L/9-10/1/> ;
    rdfs:subClassOf :CCSS.ELA-Literacy.L.9-10 ;
    rdfs:comment "Demonstrate command of the conventions of standard English grammar and usage when writing or speaking."^^xsd:string .

:CCSS.ELA-Literacy.L.9-10.1.a rdf:type owl:Class ;
    prov:wasQuotedFrom <http://www.corestandards.org/ELA-Literacy/L/9-10/1/a/> ;
    rdfs:subClassOf :CCSS.ELA-Literacy.L.9-10.1 ;
    rdfs:comment "Use parallel structure.*"^^xsd:string .

:CCSS.ELA-Literacy.L.9-10.1.b rdf:type owl:Class ;
    prov:wasQuotedFrom <http://www.corestandards.org/ELA-Literacy/L/9-10/1/b/> ;
    rdfs:subClassOf :CCSS.ELA-Literacy.L.9-10.1 ;
    rdfs:comment "Use various types of phrases (noun, verb, adjectival, adverbial, participial, prepositional, absolute) and clauses (independent, dependent; noun, relative, adverbial) to convey specific meanings and add variety and interest to writing or presentations."^^xsd:string .

:CCSS.ELA-Literacy.L.9-10.2 rdf:type owl:Class ;
    prov:wasQuotedFrom <http://www.corestandards.org/ELA-Literacy/L/9-10/2/> ;
    rdfs:subClassOf :CCSS.ELA-Literacy.L.9-10 ;
    rdfs:comment "Demonstrate command of the conventions of standard English capitalization, punctuation, and spelling when writing."^^xsd:string .

:CCSS.ELA-Literacy.L.9-10.2.a rdf:type owl:Class ;
    prov:wasQuotedFrom <http://www.corestandards.org/ELA-Literacy/L/9-10/2/a/> ;
    rdfs:subClassOf :CCSS.ELA-Literacy.L.9-10.2 ;
    rdfs:comment "Use a semicolon (and perhaps a conjunctive adverb) to link two or more closely related independent clauses."^^xsd:string .

:CCSS.ELA-Literacy.L.9-10.2.b rdf:type owl:Class ;
    prov:wasQuotedFrom <http://www.corestandards.org/ELA-Literacy/L/9-10/2/b/> ;
    rdfs:subClassOf :CCSS.ELA-Literacy.L.9-10.2 ;
    rdfs:comment "Use a colon to introduce a list or quotation."^^xsd:string .

:CCSS.ELA-Literacy.L.9-10.2.c rdf:type owl:Class ;
    prov:wasQuotedFrom <http://www.corestandards.org/ELA-Literacy/L/9-10/2/c/> ;
    rdfs:subClassOf :CCSS.ELA-Literacy.L.9-10.2 ;
    rdfs:comment "Spell correctly."^^xsd:string .

:CCSS.ELA-Literacy.L.9-10.3 rdf:type owl:Class ;
    prov:wasQuotedFrom <http://www.corestandards.org/ELA-Literacy/L/9-10/3/> ;
    rdfs:subClassOf :CCSS.ELA-Literacy.L.9-10 ;
    rdfs:comment "Apply knowledge of language to understand how language functions in different contexts, to make effective choices for meaning or style, and to comprehend more fully when reading or listening."^^xsd:string .

:CCSS.ELA-Literacy.L.9-10.3.a rdf:type owl:Class ;
    prov:wasQuotedFrom <http://www.corestandards.org/ELA-Literacy/L/9-10/3/a/> ;
    rdfs:subClassOf :CCSS.ELA-Literacy.L.9-10.3 ;
    rdfs:comment "Write and edit work so that it conforms to the guidelines in a style manual (e.g., MLA Handbook, Turabian's Manual for Writers) appropriate for the discipline and writing type."^^xsd:string .

:CCSS.ELA-Literacy.L.9-10.4 rdf:type owl:Class ;
    prov:wasQuotedFrom <http://www.corestandards.org/ELA-Literacy/L/9-10/4/> ;
    rdfs:subClassOf :CCSS.ELA-Literacy.L.9-10 ;
    rdfs:comment "Determine or clarify the meaning of unknown and multiple-meaning words and phrases based on grades 9-10 reading and content, choosing flexibly from a range of strategies."^^xsd:string .

:CCSS.ELA-Literacy.L.9-10.4.a rdf:type owl:Class ;
    prov:wasQuotedFrom <http://www.corestandards.org/ELA-Literacy/L/9-10/4/a/> ;
    rdfs:subClassOf :CCSS.ELA-Literacy.L.9-10.4 ;
    rdfs:comment "Use context (e.g., the overall meaning of a sentence, paragraph, or text; a word's position or function in a sentence) as a clue to the meaning of a word or phrase."^^xsd:string .

:CCSS.ELA-Literacy.L.9-10.4.b rdf:type owl:Class ;
    prov:wasQuotedFrom <http://www.corestandards.org/ELA-Literacy/L/9-10/4/b/> ;
    rdfs:subClassOf :CCSS.ELA-Literacy.L.9-10.4 ;
    rdfs:comment "Identify and correctly use patterns of word changes that indicate different meanings or parts of speech (e.g., analyze, analysis, analytical; advocate, advocacy)."^^xsd:string .

:CCSS.ELA-Literacy.L.9-10.4.c rdf:type owl:Class ;
    prov:wasQuotedFrom <http://www.corestandards.org/ELA-Literacy/L/9-10/4/c/> ;
    rdfs:subClassOf :CCSS.ELA-Literacy.L.9-10.4 ;
    rdfs:comment "Consult general and specialized reference materials (e.g., dictionaries, glossaries, thesauruses), both print and digital, to find the pronunciation of a word or determine or clarify its precise meaning, its part of speech, or its etymology."^^xsd:string .

:CCSS.ELA-Literacy.L.9-10.4.d rdf:type owl:Class ;
    prov:wasQuotedFrom <http://www.corestandards.org/ELA-Literacy/L/9-10/4/d/> ;
    rdfs:subClassOf :CCSS.ELA-Literacy.L.9-10.4 ;
    rdfs:comment "Verify the preliminary determination of the meaning of a word or phrase (e.g., by checking the inferred meaning in context or in a dictionary)."^^xsd:string .

:CCSS.ELA-Literacy.L.9-10.5 rdf:type owl:Class ;
    prov:wasQuotedFrom <http://www.corestandards.org/ELA-Literacy/L/9-10/5/> ;
    rdfs:subClassOf :CCSS.ELA-Literacy.L.9-10 ;
    rdfs:comment "Demonstrate understanding of figurative language, word relationships, and nuances in word meanings."^^xsd:string .

:CCSS.ELA-Literacy.L.9-10.5.a rdf:type owl:Class ;
    prov:wasQuotedFrom <http://www.corestandards.org/ELA-Literacy/L/9-10/5/a/> ;
    rdfs:subClassOf :CCSS.ELA-Literacy.L.9-10.5 ;
    rdfs:comment "Interpret figures of speech (e.g., euphemism, oxymoron) in context and analyze their role in the text."^^xsd:string .

:CCSS.ELA-Literacy.L.9-10.5.b rdf:type owl:Class ;
    prov:wasQuotedFrom <http://www.corestandards.org/ELA-Literacy/L/9-10/5/b/> ;
    rdfs:subClassOf :CCSS.ELA-Literacy.L.9-10.5 ;
    rdfs:comment "Analyze nuances in the meaning of words with similar denotations."^^xsd:string .

:CCSS.ELA-Literacy.L.9-10.6 rdf:type owl:Class ;
    prov:wasQuotedFrom <http://www.corestandards.org/ELA-Literacy/L/9-10/6/> ;
    rdfs:subClassOf :CCSS.ELA-Literacy.L.9-10 ;
    rdfs:comment "Acquire and use accurately general academic and domain-specific words and phrases, sufficient for reading, writing, speaking, and listening at the college and career readiness level; demonstrate independence in gathering vocabulary knowledge when considering a word or phrase important to comprehension or expression."^^xsd:string .

:CCSS.ELA-Literacy.L.11-12.1 rdf:type owl:Class ;
    prov:wasQuotedFrom <http://www.corestandards.org/ELA-Literacy/L/11-12/1/> ;
    rdfs:subClassOf :CCSS.ELA-Literacy.L.11-12 ;
    rdfs:comment "Demonstrate command of the conventions of standard English grammar and usage when writing or speaking."^^xsd:string .

:CCSS.ELA-Literacy.L.11-12.1.a rdf:type owl:Class ;
    prov:wasQuotedFrom <http://www.corestandards.org/ELA-Literacy/L/11-12/1/a/> ;
    rdfs:subClassOf :CCSS.ELA-Literacy.L.11-12.1 ;
    rdfs:comment "Apply the understanding that usage is a matter of convention, can change over time, and is sometimes contested."^^xsd:string .

:CCSS.ELA-Literacy.L.11-12.1.b rdf:type owl:Class ;
    prov:wasQuotedFrom <http://www.corestandards.org/ELA-Literacy/L/11-12/1/b/> ;
    rdfs:subClassOf :CCSS.ELA-Literacy.L.11-12.1 ;
    rdfs:comment "Resolve issues of complex or contested usage, consulting references (e.g., Merriam-Webster's Dictionary of English Usage, Garner's Modern American Usage) as needed."^^xsd:string .

:CCSS.ELA-Literacy.L.11-12.2 rdf:type owl:Class ;
    prov:wasQuotedFrom <http://www.corestandards.org/ELA-Literacy/L/11-12/2/> ;
    rdfs:subClassOf :CCSS.ELA-Literacy.L.11-12 ;
    rdfs:comment "Demonstrate command of the conventions of standard English capitalization, punctuation, and spelling when writing."^^xsd:string .

:CCSS.ELA-Literacy.L.11-12.2.a rdf:type owl:Class ;
    prov:wasQuotedFrom <http://www.corestandards.org/ELA-Literacy/L/11-12/2/a/> ;
    rdfs:subClassOf :CCSS.ELA-Literacy.L.11-12.2 ;
    rdfs:comment "Observe hyphenation conventions."^^xsd:string .

:CCSS.ELA-Literacy.L.11-12.2.b rdf:type owl:Class ;
    prov:wasQuotedFrom <http://www.corestandards.org/ELA-Literacy/L/11-12/2/b/> ;
    rdfs:subClassOf :CCSS.ELA-Literacy.L.11-12.2 ;
    rdfs:comment "Spell correctly."^^xsd:string .

:CCSS.ELA-Literacy.L.11-12.3 rdf:type owl:Class ;
    prov:wasQuotedFrom <http://www.corestandards.org/ELA-Literacy/L/11-12/3/> ;
    rdfs:subClassOf :CCSS.ELA-Literacy.L.11-12 ;
    rdfs:comment "Apply knowledge of language to understand how language functions in different contexts, to make effective choices for meaning or style, and to comprehend more fully when reading or listening."^^xsd:string .

:CCSS.ELA-Literacy.L.11-12.3.a rdf:type owl:Class ;
    prov:wasQuotedFrom <http://www.corestandards.org/ELA-Literacy/L/11-12/3/a/> ;
    rdfs:subClassOf :CCSS.ELA-Literacy.L.11-12.3 ;
    rdfs:comment "Vary syntax for effect, consulting references (e.g., Tufte's Artful Sentences) for guidance as needed; apply an understanding of syntax to the study of complex texts when reading."^^xsd:string .

:CCSS.ELA-Literacy.L.11-12.4 rdf:type owl:Class ;
    prov:wasQuotedFrom <http://www.corestandards.org/ELA-Literacy/L/11-12/4/> ;
    rdfs:subClassOf :CCSS.ELA-Literacy.L.11-12 ;
    rdfs:comment "Determine or clarify the meaning of unknown and multiple-meaning words and phrases based on grades 11-12 reading and content, choosing flexibly from a range of strategies."^^xsd:string .

:CCSS.ELA-Literacy.L.11-12.4.a rdf:type owl:Class ;
    prov:wasQuotedFrom <http://www.corestandards.org/ELA-Literacy/L/11-12/4/a/> ;
    rdfs:subClassOf :CCSS.ELA-Literacy.L.11-12.4 ;
    rdfs:comment "Use context (e.g., the overall meaning of a sentence, paragraph, or text; a word's position or function in a sentence) as a clue to the meaning of a word or phrase."^^xsd:string .

:CCSS.ELA-Literacy.L.11-12.4.b rdf:type owl:Class ;
    prov:wasQuotedFrom <http://www.corestandards.org/ELA-Literacy/L/11-12/4/b/> ;
    rdfs:subClassOf :CCSS.ELA-Literacy.L.11-12.4 ;
    rdfs:comment "Identify and correctly use patterns of word changes that indicate different meanings or parts of speech (e.g., conceive, conception, conceivable)."^^xsd:string .

:CCSS.ELA-Literacy.L.11-12.4.c rdf:type owl:Class ;
    prov:wasQuotedFrom <http://www.corestandards.org/ELA-Literacy/L/11-12/4/c/> ;
    rdfs:subClassOf :CCSS.ELA-Literacy.L.11-12.4 ;
    rdfs:comment "Consult general and specialized reference materials (e.g., dictionaries, glossaries, thesauruses), both print and digital, to find the pronunciation of a word or determine or clarify its precise meaning, its part of speech, its etymology, or its standard usage."^^xsd:string .

:CCSS.ELA-Literacy.L.11-12.4.d rdf:type owl:Class ;
    prov:wasQuotedFrom <http://www.corestandards.org/ELA-Literacy/L/11-12/4/d/> ;
    rdfs:subClassOf :CCSS.ELA-Literacy.L.11-12.4 ;
    rdfs:comment "Verify the preliminary determination of the meaning of a word or phrase (e.g., by checking the inferred meaning in context or in a dictionary)."^^xsd:string .

:CCSS.ELA-Literacy.L.11-12.5 rdf:type owl:Class ;
    prov:wasQuotedFrom <http://www.corestandards.org/ELA-Literacy/L/11-12/5/> ;
    rdfs:subClassOf :CCSS.ELA-Literacy.L.11-12 ;
    rdfs:comment "Demonstrate understanding of figurative language, word relationships, and nuances in word meanings."^^xsd:string .

:CCSS.ELA-Literacy.L.11-12.5.a rdf:type owl:Class ;
    prov:wasQuotedFrom <http://www.corestandards.org/ELA-Literacy/L/11-12/5/a/> ;
    rdfs:subClassOf :CCSS.ELA-Literacy.L.11-12.5 ;
    rdfs:comment "Interpret figures of speech (e.g., hyperbole, paradox) in context and analyze their role in the text."^^xsd:string .

:CCSS.ELA-Literacy.L.11-12.5.b rdf:type owl:Class ;
    prov:wasQuotedFrom <http://www.corestandards.org/ELA-Literacy/L/11-12/5/b/> ;
    rdfs:subClassOf :CCSS.ELA-Literacy.L.11-12.5 ;
    rdfs:comment "Analyze nuances in the meaning of words with similar denotations."^^xsd:string .

:CCSS.ELA-Literacy.L.11-12.6 rdf:type owl:Class ;
    prov:wasQuotedFrom <http://www.corestandards.org/ELA-Literacy/L/11-12/6/> ;
    rdfs:subClassOf :CCSS.ELA-Literacy.L.11-12 ;
    rdfs:comment "Acquire and use accurately general academic and domain-specific words and phrases, sufficient for reading, writing, speaking, and listening at the college and career readiness level; demonstrate independence in gathering vocabulary knowledge when considering a word or phrase important to comprehension or expression."^^xsd:string .

:CCSS.ELA-Literacy.RH rdf:type owl:Class ;
    rdfs:subClassOf :CCSS.ELA-Literacy ;
    rdfs:label "CCSS.ELA-Literacy.RH"^^xsd:string ;
    prov:wasQuotedFrom <http://www.corestandards.org/ELA-Literacy/RH/> .

:CCSS.ELA-Literacy.RH.6-8 rdf:type owl:Class ;
    rdfs:subClassOf :CCSS.ELA-Literacy.RH ;
    rdfs:label "CCSS.ELA-Literacy.RH.6-8"^^xsd:string ;
    prov:wasQuotedFrom <http://www.corestandards.org/ELA-Literacy/RH/6-8/> .

:CCSS.ELA-Literacy.RH.6-8.1 rdf:type owl:Class ;
    prov:wasQuotedFrom <http://www.corestandards.org/ELA-Literacy/RH/6-8/1/> ;
    rdfs:subClassOf :CCSS.ELA-Literacy.RH.6-8 ;
    rdfs:comment "Cite specific textual evidence to support analysis of primary and secondary sources."^^xsd:string .

:CCSS.ELA-Literacy.RH.6-8.2 rdf:type owl:Class ;
    prov:wasQuotedFrom <http://www.corestandards.org/ELA-Literacy/RH/6-8/2/> ;
    rdfs:subClassOf :CCSS.ELA-Literacy.RH.6-8 ;
    rdfs:comment "Determine the central ideas or information of a primary or secondary source; provide an accurate summary of the source distinct from prior knowledge or opinions."^^xsd:string .

:CCSS.ELA-Literacy.RH.6-8.3 rdf:type owl:Class ;
    prov:wasQuotedFrom <http://www.corestandards.org/ELA-Literacy/RH/6-8/3/> ;
    rdfs:subClassOf :CCSS.ELA-Literacy.RH.6-8 ;
    rdfs:comment "Identify key steps in a text's description of a process related to history/social studies (e.g., how a bill becomes law, how interest rates are raised or lowered)."^^xsd:string .

:CCSS.ELA-Literacy.RH.6-8.4 rdf:type owl:Class ;
    prov:wasQuotedFrom <http://www.corestandards.org/ELA-Literacy/RH/6-8/4/> ;
    rdfs:subClassOf :CCSS.ELA-Literacy.RH.6-8 ;
    rdfs:comment "Determine the meaning of words and phrases as they are used in a text, including vocabulary specific to domains related to history/social studies."^^xsd:string .

:CCSS.ELA-Literacy.RH.6-8.5 rdf:type owl:Class ;
    prov:wasQuotedFrom <http://www.corestandards.org/ELA-Literacy/RH/6-8/5/> ;
    rdfs:subClassOf :CCSS.ELA-Literacy.RH.6-8 ;
    rdfs:comment "Describe how a text presents information (e.g., sequentially, comparatively, causally). "^^xsd:string .

:CCSS.ELA-Literacy.RH.6-8.6 rdf:type owl:Class ;
    prov:wasQuotedFrom <http://www.corestandards.org/ELA-Literacy/RH/6-8/6/> ;
    rdfs:subClassOf :CCSS.ELA-Literacy.RH.6-8 ;
    rdfs:comment "Identify aspects of a text that reveal an author's point of view or purpose (e.g., loaded language, inclusion or avoidance of particular facts)."^^xsd:string .

:CCSS.ELA-Literacy.RH.6-8.7 rdf:type owl:Class ;
    prov:wasQuotedFrom <http://www.corestandards.org/ELA-Literacy/RH/6-8/7/> ;
    rdfs:subClassOf :CCSS.ELA-Literacy.RH.6-8 ;
    rdfs:comment "Integrate visual information (e.g., in charts, graphs, photographs, videos, or maps) with other information in print and digital texts."^^xsd:string .

:CCSS.ELA-Literacy.RH.6-8.8 rdf:type owl:Class ;
    prov:wasQuotedFrom <http://www.corestandards.org/ELA-Literacy/RH/6-8/8/> ;
    rdfs:subClassOf :CCSS.ELA-Literacy.RH.6-8 ;
    rdfs:comment "Distinguish among fact, opinion, and reasoned judgment in a text."^^xsd:string .

:CCSS.ELA-Literacy.RH.6-8.9 rdf:type owl:Class ;
    prov:wasQuotedFrom <http://www.corestandards.org/ELA-Literacy/RH/6-8/9/> ;
    rdfs:subClassOf :CCSS.ELA-Literacy.RH.6-8 ;
    rdfs:comment "Analyze the relationship between a primary and secondary source on the same topic."^^xsd:string .

:CCSS.ELA-Literacy.RH.6-8.10 rdf:type owl:Class ;
    prov:wasQuotedFrom <http://www.corestandards.org/ELA-Literacy/RH/6-8/10/> ;
    rdfs:subClassOf :CCSS.ELA-Literacy.RH.6-8 ;
    rdfs:comment "By the end of grade 8, read and comprehend history/social studies texts in the grades 6-8 text complexity band independently and proficiently."^^xsd:string .

:CCSS.ELA-Literacy.RH.9-10 rdf:type owl:Class ;
    rdfs:subClassOf :CCSS.ELA-Literacy.RH ;
    rdfs:label "CCSS.ELA-Literacy.RH.9-10"^^xsd:string ;
    prov:wasQuotedFrom <http://www.corestandards.org/ELA-Literacy/RH/9-10/> .

:CCSS.ELA-Literacy.RH.9-10.1 rdf:type owl:Class ;
    prov:wasQuotedFrom <http://www.corestandards.org/ELA-Literacy/RH/9-10/1/> ;
    rdfs:subClassOf :CCSS.ELA-Literacy.RH.9-10 ;
    rdfs:comment "Cite specific textual evidence to support analysis of primary and secondary sources, attending to such features as the date and origin of the information."^^xsd:string .

:CCSS.ELA-Literacy.RH.9-10.2 rdf:type owl:Class ;
    prov:wasQuotedFrom <http://www.corestandards.org/ELA-Literacy/RH/9-10/2/> ;
    rdfs:subClassOf :CCSS.ELA-Literacy.RH.9-10 ;
    rdfs:comment "Determine the central ideas or information of a primary or secondary source; provide an accurate summary of how key events or ideas develop over the course of the text."^^xsd:string .

:CCSS.ELA-Literacy.RH.9-10.3 rdf:type owl:Class ;
    prov:wasQuotedFrom <http://www.corestandards.org/ELA-Literacy/RH/9-10/3/> ;
    rdfs:subClassOf :CCSS.ELA-Literacy.RH.9-10 ;
    rdfs:comment "Analyze in detail a series of events described in a text; determine whether earlier events caused later ones or simply preceded them. "^^xsd:string .

:CCSS.ELA-Literacy.RH.9-10.4 rdf:type owl:Class ;
    prov:wasQuotedFrom <http://www.corestandards.org/ELA-Literacy/RH/9-10/4/> ;
    rdfs:subClassOf :CCSS.ELA-Literacy.RH.9-10 ;
    rdfs:comment "Determine the meaning of words and phrases as they are used in a text, including vocabulary describing political, social, or economic aspects of history/social science."^^xsd:string .

:CCSS.ELA-Literacy.RH.9-10.5 rdf:type owl:Class ;
    prov:wasQuotedFrom <http://www.corestandards.org/ELA-Literacy/RH/9-10/5/> ;
    rdfs:subClassOf :CCSS.ELA-Literacy.RH.9-10 ;
    rdfs:comment "Analyze how a text uses structure to emphasize key points or advance an explanation or analysis."^^xsd:string .

:CCSS.ELA-Literacy.RH.9-10.6 rdf:type owl:Class ;
    prov:wasQuotedFrom <http://www.corestandards.org/ELA-Literacy/RH/9-10/6/> ;
    rdfs:subClassOf :CCSS.ELA-Literacy.RH.9-10 ;
    rdfs:comment "Compare the point of view of two or more authors for how they treat the same or similar topics, including which details they include and emphasize in their respective accounts."^^xsd:string .

:CCSS.ELA-Literacy.RH.9-10.7 rdf:type owl:Class ;
    prov:wasQuotedFrom <http://www.corestandards.org/ELA-Literacy/RH/9-10/7/> ;
    rdfs:subClassOf :CCSS.ELA-Literacy.RH.9-10 ;
    rdfs:comment "Integrate quantitative or technical analysis (e.g., charts, research data) with qualitative analysis in print or digital text."^^xsd:string .

:CCSS.ELA-Literacy.RH.9-10.8 rdf:type owl:Class ;
    prov:wasQuotedFrom <http://www.corestandards.org/ELA-Literacy/RH/9-10/8/> ;
    rdfs:subClassOf :CCSS.ELA-Literacy.RH.9-10 ;
    rdfs:comment "Assess the extent to which the reasoning and evidence in a text support the author's claims."^^xsd:string .

:CCSS.ELA-Literacy.RH.9-10.9 rdf:type owl:Class ;
    prov:wasQuotedFrom <http://www.corestandards.org/ELA-Literacy/RH/9-10/9/> ;
    rdfs:subClassOf :CCSS.ELA-Literacy.RH.9-10 ;
    rdfs:comment "Compare and contrast treatments of the same topic in several primary and secondary sources."^^xsd:string .

:CCSS.ELA-Literacy.RH.9-10.10 rdf:type owl:Class ;
    prov:wasQuotedFrom <http://www.corestandards.org/ELA-Literacy/RH/9-10/10/> ;
    rdfs:subClassOf :CCSS.ELA-Literacy.RH.9-10 ;
    rdfs:comment "By the end of grade 10, read and comprehend history/social studies texts in the grades 9-10 text complexity band independently and proficiently."^^xsd:string .

:CCSS.ELA-Literacy.RH.11-12 rdf:type owl:Class ;
    rdfs:subClassOf :CCSS.ELA-Literacy.RH ;
    rdfs:label "CCSS.ELA-Literacy.RH.11-12"^^xsd:string ;
    prov:wasQuotedFrom <http://www.corestandards.org/ELA-Literacy/RH/11-12/> .

:CCSS.ELA-Literacy.RH.11-12.1 rdf:type owl:Class ;
    prov:wasQuotedFrom <http://www.corestandards.org/ELA-Literacy/RH/11-12/1/> ;
    rdfs:subClassOf :CCSS.ELA-Literacy.RH.11-12 ;
    rdfs:comment "Cite specific textual evidence to support analysis of primary and secondary sources, connecting insights gained from specific details to an understanding of the text as a whole."^^xsd:string .

:CCSS.ELA-Literacy.RH.11-12.2 rdf:type owl:Class ;
    prov:wasQuotedFrom <http://www.corestandards.org/ELA-Literacy/RH/11-12/2/> ;
    rdfs:subClassOf :CCSS.ELA-Literacy.RH.11-12 ;
    rdfs:comment "Determine the central ideas or information of a primary or secondary source; provide an accurate summary that makes clear the relationships among the key details and ideas."^^xsd:string .

:CCSS.ELA-Literacy.RH.11-12.3 rdf:type owl:Class ;
    prov:wasQuotedFrom <http://www.corestandards.org/ELA-Literacy/RH/11-12/3/> ;
    rdfs:subClassOf :CCSS.ELA-Literacy.RH.11-12 ;
    rdfs:comment "Evaluate various explanations for actions or events and determine which explanation best accords with textual evidence, acknowledging where the text leaves matters uncertain."^^xsd:string .

:CCSS.ELA-Literacy.RH.11-12.4 rdf:type owl:Class ;
    prov:wasQuotedFrom <http://www.corestandards.org/ELA-Literacy/RH/11-12/4/> ;
    rdfs:subClassOf :CCSS.ELA-Literacy.RH.11-12 ;
    rdfs:comment "Determine the meaning of words and phrases as they are used in a text, including analyzing how an author uses and refines the meaning of a key term over the course of a text (e.g., how Madison defines faction in Federalist No. 10)."^^xsd:string .

:CCSS.ELA-Literacy.RH.11-12.5 rdf:type owl:Class ;
    prov:wasQuotedFrom <http://www.corestandards.org/ELA-Literacy/RH/11-12/5/> ;
    rdfs:subClassOf :CCSS.ELA-Literacy.RH.11-12 ;
    rdfs:comment "Analyze in detail how a complex primary source is structured, including how key sentences, paragraphs, and larger portions of the text contribute to the whole.  "^^xsd:string .

:CCSS.ELA-Literacy.RH.11-12.6 rdf:type owl:Class ;
    prov:wasQuotedFrom <http://www.corestandards.org/ELA-Literacy/RH/11-12/6/> ;
    rdfs:subClassOf :CCSS.ELA-Literacy.RH.11-12 ;
    rdfs:comment "Evaluate authors' differing points of view on the same historical event or issue by assessing the authors' claims, reasoning, and evidence."^^xsd:string .

:CCSS.ELA-Literacy.RH.11-12.7 rdf:type owl:Class ;
    prov:wasQuotedFrom <http://www.corestandards.org/ELA-Literacy/RH/11-12/7/> ;
    rdfs:subClassOf :CCSS.ELA-Literacy.RH.11-12 ;
    rdfs:comment "Integrate and evaluate multiple sources of information presented in diverse formats and media (e.g., visually, quantitatively, as well as in words) in order to address a question or solve a problem."^^xsd:string .

:CCSS.ELA-Literacy.RH.11-12.8 rdf:type owl:Class ;
    prov:wasQuotedFrom <http://www.corestandards.org/ELA-Literacy/RH/11-12/8/> ;
    rdfs:subClassOf :CCSS.ELA-Literacy.RH.11-12 ;
    rdfs:comment "Evaluate an author's premises, claims, and evidence by corroborating or challenging them with other information. "^^xsd:string .

:CCSS.ELA-Literacy.RH.11-12.9 rdf:type owl:Class ;
    prov:wasQuotedFrom <http://www.corestandards.org/ELA-Literacy/RH/11-12/9/> ;
    rdfs:subClassOf :CCSS.ELA-Literacy.RH.11-12 ;
    rdfs:comment "Integrate information from diverse sources, both primary and secondary, into a coherent understanding of an idea or event, noting discrepancies among sources."^^xsd:string .

:CCSS.ELA-Literacy.RH.11-12.10 rdf:type owl:Class ;
    prov:wasQuotedFrom <http://www.corestandards.org/ELA-Literacy/RH/11-12/10/> ;
    rdfs:subClassOf :CCSS.ELA-Literacy.RH.11-12 ;
    rdfs:comment "By the end of grade 12, read and comprehend history/social studies texts in the grades 11-CCR text complexity band independently and proficiently."^^xsd:string .

:CCSS.ELA-Literacy.RST rdf:type owl:Class ;
    rdfs:subClassOf :CCSS.ELA-Literacy ;
    rdfs:label "CCSS.ELA-Literacy.RST"^^xsd:string ;
    prov:wasQuotedFrom <http://www.corestandards.org/ELA-Literacy/RST/> .

:CCSS.ELA-Literacy.RST.6-8 rdf:type owl:Class ;
    rdfs:subClassOf :CCSS.ELA-Literacy.RST ;
    rdfs:label "CCSS.ELA-Literacy.RST.6-8"^^xsd:string ;
    prov:wasQuotedFrom <http://www.corestandards.org/ELA-Literacy/RST/6-8/> .

:CCSS.ELA-Literacy.RST.6-8.1 rdf:type owl:Class ;
    prov:wasQuotedFrom <http://www.corestandards.org/ELA-Literacy/RST/6-8/1/> ;
    rdfs:subClassOf :CCSS.ELA-Literacy.RST.6-8 ;
    rdfs:comment "Cite specific textual evidence to support analysis of science and technical texts."^^xsd:string .

:CCSS.ELA-Literacy.RST.6-8.2 rdf:type owl:Class ;
    prov:wasQuotedFrom <http://www.corestandards.org/ELA-Literacy/RST/6-8/2/> ;
    rdfs:subClassOf :CCSS.ELA-Literacy.RST.6-8 ;
    rdfs:comment "Determine the central ideas or conclusions of a text; provide an accurate summary of the text distinct from prior knowledge or opinions."^^xsd:string .

:CCSS.ELA-Literacy.RST.6-8.3 rdf:type owl:Class ;
    prov:wasQuotedFrom <http://www.corestandards.org/ELA-Literacy/RST/6-8/3/> ;
    rdfs:subClassOf :CCSS.ELA-Literacy.RST.6-8 ;
    rdfs:comment "Follow precisely a multistep procedure when carrying out experiments, taking measurements, or performing technical tasks."^^xsd:string .

:CCSS.ELA-Literacy.RST.6-8.4 rdf:type owl:Class ;
    prov:wasQuotedFrom <http://www.corestandards.org/ELA-Literacy/RST/6-8/4/> ;
    rdfs:subClassOf :CCSS.ELA-Literacy.RST.6-8 ;
    rdfs:comment "Determine the meaning of symbols, key terms, and other domain-specific words and phrases as they are used in a specific scientific or technical context relevant to grades 6-8 texts and topics."^^xsd:string .

:CCSS.ELA-Literacy.RST.6-8.5 rdf:type owl:Class ;
    prov:wasQuotedFrom <http://www.corestandards.org/ELA-Literacy/RST/6-8/5/> ;
    rdfs:subClassOf :CCSS.ELA-Literacy.RST.6-8 ;
    rdfs:comment "Analyze the structure an author uses to organize a text, including how the major sections contribute to the whole and to an understanding of the topic."^^xsd:string .

:CCSS.ELA-Literacy.RST.6-8.6 rdf:type owl:Class ;
    prov:wasQuotedFrom <http://www.corestandards.org/ELA-Literacy/RST/6-8/6/> ;
    rdfs:subClassOf :CCSS.ELA-Literacy.RST.6-8 ;
    rdfs:comment "Analyze the author's purpose in providing an explanation, describing a procedure, or discussing an experiment in a text."^^xsd:string .

:CCSS.ELA-Literacy.RST.6-8.7 rdf:type owl:Class ;
    prov:wasQuotedFrom <http://www.corestandards.org/ELA-Literacy/RST/6-8/7/> ;
    rdfs:subClassOf :CCSS.ELA-Literacy.RST.6-8 ;
    rdfs:comment "Integrate quantitative or technical information expressed in words in a text with a version of that information expressed visually (e.g., in a flowchart, diagram, model, graph, or table)."^^xsd:string .

:CCSS.ELA-Literacy.RST.6-8.8 rdf:type owl:Class ;
    prov:wasQuotedFrom <http://www.corestandards.org/ELA-Literacy/RST/6-8/8/> ;
    rdfs:subClassOf :CCSS.ELA-Literacy.RST.6-8 ;
    rdfs:comment "Distinguish among facts, reasoned judgment based on research findings, and speculation in a text."^^xsd:string .

:CCSS.ELA-Literacy.RST.6-8.9 rdf:type owl:Class ;
    prov:wasQuotedFrom <http://www.corestandards.org/ELA-Literacy/RST/6-8/9/> ;
    rdfs:subClassOf :CCSS.ELA-Literacy.RST.6-8 ;
    rdfs:comment "Compare and contrast the information gained from experiments, simulations, video, or multimedia sources with that gained from reading a text on the same topic."^^xsd:string .

:CCSS.ELA-Literacy.RST.6-8.10 rdf:type owl:Class ;
    prov:wasQuotedFrom <http://www.corestandards.org/ELA-Literacy/RST/6-8/10/> ;
    rdfs:subClassOf :CCSS.ELA-Literacy.RST.6-8 ;
    rdfs:comment "By the end of grade 8, read and comprehend science/technical texts in the grades 6-8 text complexity band independently and proficiently."^^xsd:string .

:CCSS.ELA-Literacy.RST.9-10 rdf:type owl:Class ;
    rdfs:subClassOf :CCSS.ELA-Literacy.RST ;
    rdfs:label "CCSS.ELA-Literacy.RST.9-10"^^xsd:string ;
    prov:wasQuotedFrom <http://www.corestandards.org/ELA-Literacy/RST/9-10/> .

:CCSS.ELA-Literacy.RST.9-10.1 rdf:type owl:Class ;
    prov:wasQuotedFrom <http://www.corestandards.org/ELA-Literacy/RST/9-10/1/> ;
    rdfs:subClassOf :CCSS.ELA-Literacy.RST.9-10 ;
    rdfs:comment "Cite specific textual evidence to support analysis of science and technical texts, attending to the precise details of explanations or descriptions."^^xsd:string .

:CCSS.ELA-Literacy.RST.9-10.2 rdf:type owl:Class ;
    prov:wasQuotedFrom <http://www.corestandards.org/ELA-Literacy/RST/9-10/2/> ;
    rdfs:subClassOf :CCSS.ELA-Literacy.RST.9-10 ;
    rdfs:comment "Determine the central ideas or conclusions of a text; trace the text's explanation or depiction of a complex process, phenomenon, or concept; provide an accurate summary of the text."^^xsd:string .

:CCSS.ELA-Literacy.RST.9-10.3 rdf:type owl:Class ;
    prov:wasQuotedFrom <http://www.corestandards.org/ELA-Literacy/RST/9-10/3/> ;
    rdfs:subClassOf :CCSS.ELA-Literacy.RST.9-10 ;
    rdfs:comment "Follow precisely a complex multistep procedure when carrying out experiments, taking measurements, or performing technical tasks, attending to special cases or exceptions defined in the text. "^^xsd:string .

:CCSS.ELA-Literacy.RST.9-10.4 rdf:type owl:Class ;
    prov:wasQuotedFrom <http://www.corestandards.org/ELA-Literacy/RST/9-10/4/> ;
    rdfs:subClassOf :CCSS.ELA-Literacy.RST.9-10 ;
    rdfs:comment "Determine the meaning of symbols, key terms, and other domain-specific words and phrases as they are used in a specific scientific or technical context relevant to grades 9-10 texts and topics."^^xsd:string .

:CCSS.ELA-Literacy.RST.9-10.5 rdf:type owl:Class ;
    prov:wasQuotedFrom <http://www.corestandards.org/ELA-Literacy/RST/9-10/5/> ;
    rdfs:subClassOf :CCSS.ELA-Literacy.RST.9-10 ;
    rdfs:comment "Analyze the structure of the relationships among concepts in a text, including relationships among key terms (e.g., force, friction, reaction force, energy)."^^xsd:string .

:CCSS.ELA-Literacy.RST.9-10.6 rdf:type owl:Class ;
    prov:wasQuotedFrom <http://www.corestandards.org/ELA-Literacy/RST/9-10/6/> ;
    rdfs:subClassOf :CCSS.ELA-Literacy.RST.9-10 ;
    rdfs:comment "Analyze the author's purpose in providing an explanation, describing a procedure, or discussing an experiment in a text, defining the question the author seeks to address."^^xsd:string .

:CCSS.ELA-Literacy.RST.9-10.7 rdf:type owl:Class ;
    prov:wasQuotedFrom <http://www.corestandards.org/ELA-Literacy/RST/9-10/7/> ;
    rdfs:subClassOf :CCSS.ELA-Literacy.RST.9-10 ;
    rdfs:comment "Translate quantitative or technical information expressed in words in a text into visual form (e.g., a table or chart) and translate information expressed visually or mathematically (e.g., in an equation) into words."^^xsd:string .

:CCSS.ELA-Literacy.RST.9-10.8 rdf:type owl:Class ;
    prov:wasQuotedFrom <http://www.corestandards.org/ELA-Literacy/RST/9-10/8/> ;
    rdfs:subClassOf :CCSS.ELA-Literacy.RST.9-10 ;
    rdfs:comment "Assess the extent to which the reasoning and evidence in a text support the author's claim or a recommendation for solving a scientific or technical problem."^^xsd:string .

:CCSS.ELA-Literacy.RST.9-10.9 rdf:type owl:Class ;
    prov:wasQuotedFrom <http://www.corestandards.org/ELA-Literacy/RST/9-10/9/> ;
    rdfs:subClassOf :CCSS.ELA-Literacy.RST.9-10 ;
    rdfs:comment "Compare and contrast findings presented in a text to those from other sources (including their own experiments), noting when the findings support or contradict previous explanations or accounts."^^xsd:string .

:CCSS.ELA-Literacy.RST.9-10.10 rdf:type owl:Class ;
    prov:wasQuotedFrom <http://www.corestandards.org/ELA-Literacy/RST/9-10/10/> ;
    rdfs:subClassOf :CCSS.ELA-Literacy.RST.9-10 ;
    rdfs:comment "By the end of grade 10, read and comprehend science/technical texts in the grades 9-10 text complexity band independently and proficiently."^^xsd:string .

:CCSS.ELA-Literacy.RST.11-12 rdf:type owl:Class ;
    rdfs:subClassOf :CCSS.ELA-Literacy.RST ;
    rdfs:label "CCSS.ELA-Literacy.RST.11-12"^^xsd:string ;
    prov:wasQuotedFrom <http://www.corestandards.org/ELA-Literacy/RST/11-12/> .

:CCSS.ELA-Literacy.RST.11-12.1 rdf:type owl:Class ;
    prov:wasQuotedFrom <http://www.corestandards.org/ELA-Literacy/RST/11-12/1/> ;
    rdfs:subClassOf :CCSS.ELA-Literacy.RST.11-12 ;
    rdfs:comment "Cite specific textual evidence to support analysis of science and technical texts, attending to important distinctions the author makes and to any gaps or inconsistencies in the account."^^xsd:string .

:CCSS.ELA-Literacy.RST.11-12.2 rdf:type owl:Class ;
    prov:wasQuotedFrom <http://www.corestandards.org/ELA-Literacy/RST/11-12/2/> ;
    rdfs:subClassOf :CCSS.ELA-Literacy.RST.11-12 ;
    rdfs:comment "Determine the central ideas or conclusions of a text; summarize complex concepts, processes, or information presented in a text by paraphrasing them in simpler but still accurate terms."^^xsd:string .

:CCSS.ELA-Literacy.RST.11-12.3 rdf:type owl:Class ;
    prov:wasQuotedFrom <http://www.corestandards.org/ELA-Literacy/RST/11-12/3/> ;
    rdfs:subClassOf :CCSS.ELA-Literacy.RST.11-12 ;
    rdfs:comment "Follow precisely a complex multistep procedure when carrying out experiments, taking measurements, or performing technical tasks; analyze the specific results based on explanations in the text."^^xsd:string .

:CCSS.ELA-Literacy.RST.11-12.4 rdf:type owl:Class ;
    prov:wasQuotedFrom <http://www.corestandards.org/ELA-Literacy/RST/11-12/4/> ;
    rdfs:subClassOf :CCSS.ELA-Literacy.RST.11-12 ;
    rdfs:comment "Determine the meaning of symbols, key terms, and other domain-specific words and phrases as they are used in a specific scientific or technical context relevant to grades 11-12 texts and topics."^^xsd:string .

:CCSS.ELA-Literacy.RST.11-12.5 rdf:type owl:Class ;
    prov:wasQuotedFrom <http://www.corestandards.org/ELA-Literacy/RST/11-12/5/> ;
    rdfs:subClassOf :CCSS.ELA-Literacy.RST.11-12 ;
    rdfs:comment "Analyze how the text structures information or ideas into categories or hierarchies, demonstrating understanding of the information or ideas."^^xsd:string .

:CCSS.ELA-Literacy.RST.11-12.6 rdf:type owl:Class ;
    prov:wasQuotedFrom <http://www.corestandards.org/ELA-Literacy/RST/11-12/6/> ;
    rdfs:subClassOf :CCSS.ELA-Literacy.RST.11-12 ;
    rdfs:comment "Analyze the author's purpose in providing an explanation, describing a procedure, or discussing an experiment in a text, identifying important issues that remain unresolved."^^xsd:string .

:CCSS.ELA-Literacy.RST.11-12.7 rdf:type owl:Class ;
    prov:wasQuotedFrom <http://www.corestandards.org/ELA-Literacy/RST/11-12/7/> ;
    rdfs:subClassOf :CCSS.ELA-Literacy.RST.11-12 ;
    rdfs:comment "Integrate and evaluate multiple sources of information presented in diverse formats and media (e.g., quantitative data, video, multimedia) in order to address a question or solve a problem."^^xsd:string .

:CCSS.ELA-Literacy.RST.11-12.8 rdf:type owl:Class ;
    prov:wasQuotedFrom <http://www.corestandards.org/ELA-Literacy/RST/11-12/8/> ;
    rdfs:subClassOf :CCSS.ELA-Literacy.RST.11-12 ;
    rdfs:comment "Evaluate the hypotheses, data, analysis, and conclusions in a science or technical text, verifying the data when possible and corroborating or challenging conclusions with other sources of information."^^xsd:string .

:CCSS.ELA-Literacy.RST.11-12.9 rdf:type owl:Class ;
    prov:wasQuotedFrom <http://www.corestandards.org/ELA-Literacy/RST/11-12/9/> ;
    rdfs:subClassOf :CCSS.ELA-Literacy.RST.11-12 ;
    rdfs:comment "Synthesize information from a range of sources (e.g., texts, experiments, simulations) into a coherent understanding of a process, phenomenon, or concept, resolving conflicting information when possible."^^xsd:string .

:CCSS.ELA-Literacy.RST.11-12.10 rdf:type owl:Class ;
    prov:wasQuotedFrom <http://www.corestandards.org/ELA-Literacy/RST/11-12/10/> ;
    rdfs:subClassOf :CCSS.ELA-Literacy.RST.11-12 ;
    rdfs:comment "By the end of grade 12, read and comprehend science/technical texts in the grades 11-CCR text complexity band independently and proficiently."^^xsd:string .

:CCSS.ELA-Literacy.WHST.6-8 rdf:type owl:Class ;
    prov:wasQuotedFrom <http://www.corestandards.org/ELA-Literacy/WHST/6-8/> ;
    rdfs:subClassOf :CCSS.ELA-Literacy.WHST .

:CCSS.ELA-Literacy.WHST.6-8.1 rdf:type owl:Class ;
    prov:wasQuotedFrom <http://www.corestandards.org/ELA-Literacy/WHST/6-8/1/> ;
    rdfs:subClassOf :CCSS.ELA-Literacy.WHST.6-8 ;
    rdfs:comment "Write arguments focused on discipline-specific content."^^xsd:string .

:CCSS.ELA-Literacy.WHST.6-8.1.a rdf:type owl:Class ;
    prov:wasQuotedFrom <http://www.corestandards.org/ELA-Literacy/WHST/6-8/1/a/> ;
    rdfs:subClassOf :CCSS.ELA-Literacy.WHST.6-8.1 ;
    rdfs:comment "Introduce claim(s) about a topic or issue, acknowledge and distinguish the claim(s) from alternate or opposing claims, and organize the reasons and evidence logically."^^xsd:string .

:CCSS.ELA-Literacy.WHST.6-8.1.b rdf:type owl:Class ;
    prov:wasQuotedFrom <http://www.corestandards.org/ELA-Literacy/WHST/6-8/1/b/> ;
    rdfs:subClassOf :CCSS.ELA-Literacy.WHST.6-8.1 ;
    rdfs:comment "Support claim(s) with logical reasoning and relevant, accurate data and evidence that demonstrate an understanding of the topic or text, using credible sources."^^xsd:string .

:CCSS.ELA-Literacy.WHST.6-8.1.c rdf:type owl:Class ;
    prov:wasQuotedFrom <http://www.corestandards.org/ELA-Literacy/WHST/6-8/1/c/> ;
    rdfs:subClassOf :CCSS.ELA-Literacy.WHST.6-8.1 ;
    rdfs:comment "Use words, phrases, and clauses to create cohesion and clarify the relationships among claim(s), counterclaims, reasons, and evidence."^^xsd:string .

:CCSS.ELA-Literacy.WHST.6-8.1.d rdf:type owl:Class ;
    prov:wasQuotedFrom <http://www.corestandards.org/ELA-Literacy/WHST/6-8/1/d/> ;
    rdfs:subClassOf :CCSS.ELA-Literacy.WHST.6-8.1 ;
    rdfs:comment "Establish and maintain a formal style."^^xsd:string .

:CCSS.ELA-Literacy.WHST.6-8.1.e rdf:type owl:Class ;
    prov:wasQuotedFrom <http://www.corestandards.org/ELA-Literacy/WHST/6-8/1/e/> ;
    rdfs:subClassOf :CCSS.ELA-Literacy.WHST.6-8.1 ;
    rdfs:comment "Provide a concluding statement or section that follows from and supports the argument presented."^^xsd:string .

:CCSS.ELA-Literacy.WHST.6-8.2 rdf:type owl:Class ;
    prov:wasQuotedFrom <http://www.corestandards.org/ELA-Literacy/WHST/6-8/2/> ;
    rdfs:subClassOf :CCSS.ELA-Literacy.WHST.6-8 ;
    rdfs:comment "Write informative/explanatory texts, including the narration of historical events, scientific procedures/ experiments, or technical processes."^^xsd:string .

:CCSS.ELA-Literacy.WHST.6-8.2.a rdf:type owl:Class ;
    prov:wasQuotedFrom <http://www.corestandards.org/ELA-Literacy/WHST/6-8/2/a/> ;
    rdfs:subClassOf :CCSS.ELA-Literacy.WHST.6-8.2 ;
    rdfs:comment "Introduce a topic clearly, previewing what is to follow; organize ideas, concepts, and information into broader categories as appropriate to achieving purpose; include formatting (e.g., headings), graphics (e.g., charts, tables), and multimedia when useful to aiding comprehension."^^xsd:string .

:CCSS.ELA-Literacy.WHST.6-8.2.b rdf:type owl:Class ;
    prov:wasQuotedFrom <http://www.corestandards.org/ELA-Literacy/WHST/6-8/2/b/> ;
    rdfs:subClassOf :CCSS.ELA-Literacy.WHST.6-8.2 ;
    rdfs:comment "Develop the topic with relevant, well-chosen facts, definitions, concrete details, quotations, or other information and examples."^^xsd:string .

:CCSS.ELA-Literacy.WHST.6-8.2.c rdf:type owl:Class ;
    prov:wasQuotedFrom <http://www.corestandards.org/ELA-Literacy/WHST/6-8/2/c/> ;
    rdfs:subClassOf :CCSS.ELA-Literacy.WHST.6-8.2 ;
    rdfs:comment "Use appropriate and varied transitions to create cohesion and clarify the relationships among ideas and concepts."^^xsd:string .

:CCSS.ELA-Literacy.WHST.6-8.2.d rdf:type owl:Class ;
    prov:wasQuotedFrom <http://www.corestandards.org/ELA-Literacy/WHST/6-8/2/d/> ;
    rdfs:subClassOf :CCSS.ELA-Literacy.WHST.6-8.2 ;
    rdfs:comment "Use precise language and domain-specific vocabulary to inform about or explain the topic."^^xsd:string .

:CCSS.ELA-Literacy.WHST.6-8.2.e rdf:type owl:Class ;
    prov:wasQuotedFrom <http://www.corestandards.org/ELA-Literacy/WHST/6-8/2/e/> ;
    rdfs:subClassOf :CCSS.ELA-Literacy.WHST.6-8.2 ;
    rdfs:comment "Establish and maintain a formal style and objective tone."^^xsd:string .

:CCSS.ELA-Literacy.WHST.6-8.2.f rdf:type owl:Class ;
    prov:wasQuotedFrom <http://www.corestandards.org/ELA-Literacy/WHST/6-8/2/f/> ;
    rdfs:subClassOf :CCSS.ELA-Literacy.WHST.6-8.2 ;
    rdfs:comment "Provide a concluding statement or section that follows from and supports the information or explanation presented."^^xsd:string .

:CCSS.ELA-Literacy.WHST.6-8.3 rdf:type owl:Class ;
    prov:wasQuotedFrom <http://www.corestandards.org/ELA-Literacy/WHST/6-8/3/> ;
    rdfs:subClassOf :CCSS.ELA-Literacy.WHST.6-8 ;
    rdfs:comment "(See note; not applicable as a separate requirement)"^^xsd:string .

:CCSS.ELA-Literacy.WHST.6-8.4 rdf:type owl:Class ;
    prov:wasQuotedFrom <http://www.corestandards.org/ELA-Literacy/WHST/6-8/4/> ;
    rdfs:subClassOf :CCSS.ELA-Literacy.WHST.6-8 ;
    rdfs:comment "Produce clear and coherent writing in which the development, organization, and style are appropriate to task, purpose, and audience."^^xsd:string .

:CCSS.ELA-Literacy.WHST.6-8.5 rdf:type owl:Class ;
    prov:wasQuotedFrom <http://www.corestandards.org/ELA-Literacy/WHST/6-8/5/> ;
    rdfs:subClassOf :CCSS.ELA-Literacy.WHST.6-8 ;
    rdfs:comment "With some guidance and support from peers and adults, develop and strengthen writing as needed by planning, revising, editing, rewriting, or trying a new approach, focusing on how well purpose and audience have been addressed."^^xsd:string .

:CCSS.ELA-Literacy.WHST.6-8.6 rdf:type owl:Class ;
    prov:wasQuotedFrom <http://www.corestandards.org/ELA-Literacy/WHST/6-8/6/> ;
    rdfs:subClassOf :CCSS.ELA-Literacy.WHST.6-8 ;
    rdfs:comment "Use technology, including the Internet, to produce and publish writing and present the relationships between information and ideas clearly and efficiently."^^xsd:string .

:CCSS.ELA-Literacy.WHST.6-8.7 rdf:type owl:Class ;
    prov:wasQuotedFrom <http://www.corestandards.org/ELA-Literacy/WHST/6-8/7/> ;
    rdfs:subClassOf :CCSS.ELA-Literacy.WHST.6-8 ;
    rdfs:comment "Conduct short research projects to answer a question (including a self-generated question), drawing on several sources and generating additional related, focused questions that allow for multiple avenues of exploration."^^xsd:string .

:CCSS.ELA-Literacy.WHST.6-8.8 rdf:type owl:Class ;
    prov:wasQuotedFrom <http://www.corestandards.org/ELA-Literacy/WHST/6-8/8/> ;
    rdfs:subClassOf :CCSS.ELA-Literacy.WHST.6-8 ;
    rdfs:comment "Gather relevant information from multiple print and digital sources, using search terms effectively; assess the credibility and accuracy of each source; and quote or paraphrase the data and conclusions of others while avoiding plagiarism and following a standard format for citation."^^xsd:string .

:CCSS.ELA-Literacy.WHST.6-8.9 rdf:type owl:Class ;
    prov:wasQuotedFrom <http://www.corestandards.org/ELA-Literacy/WHST/6-8/9/> ;
    rdfs:subClassOf :CCSS.ELA-Literacy.WHST.6-8 ;
    rdfs:comment "Draw evidence from informational texts to support analysis, reflection, and research."^^xsd:string .

:CCSS.ELA-Literacy.WHST.6-8.10 rdf:type owl:Class ;
    prov:wasQuotedFrom <http://www.corestandards.org/ELA-Literacy/WHST/6-8/10/> ;
    rdfs:subClassOf :CCSS.ELA-Literacy.WHST.6-8 ;
    rdfs:comment "Write routinely over extended time frames (time for reflection and revision) and shorter time frames (a single sitting or a day or two) for a range of discipline-specific tasks, purposes, and audiences."^^xsd:string .

:CCSS.ELA-Literacy.WHST.9-10 rdf:type owl:Class ;
    prov:wasQuotedFrom <http://www.corestandards.org/ELA-Literacy/WHST/9-10/> ;
    rdfs:subClassOf :CCSS.ELA-Literacy.WHST .

:CCSS.ELA-Literacy.WHST.9-10.1 rdf:type owl:Class ;
    prov:wasQuotedFrom <http://www.corestandards.org/ELA-Literacy/WHST/9-10/1/> ;
    rdfs:subClassOf :CCSS.ELA-Literacy.WHST.9-10 ;
    rdfs:comment "Write arguments focused on discipline-specific content."^^xsd:string .

:CCSS.ELA-Literacy.WHST.9-10.1.a rdf:type owl:Class ;
    prov:wasQuotedFrom <http://www.corestandards.org/ELA-Literacy/WHST/9-10/1/a/> ;
    rdfs:subClassOf :CCSS.ELA-Literacy.WHST.9-10.1 ;
    rdfs:comment "Introduce precise claim(s), distinguish the claim(s) from alternate or opposing claims, and create an organization that establishes clear relationships among the claim(s), counterclaims, reasons, and evidence."^^xsd:string .

:CCSS.ELA-Literacy.WHST.9-10.1.b rdf:type owl:Class ;
    prov:wasQuotedFrom <http://www.corestandards.org/ELA-Literacy/WHST/9-10/1/b/> ;
    rdfs:subClassOf :CCSS.ELA-Literacy.WHST.9-10.1 ;
    rdfs:comment "Develop claim(s) and counterclaims fairly, supplying data and evidence for each while pointing out the strengths and limitations of both claim(s) and counterclaims in a discipline-appropriate form and in a manner that anticipates the audience's knowledge level and concerns."^^xsd:string .

:CCSS.ELA-Literacy.WHST.9-10.1.c rdf:type owl:Class ;
    prov:wasQuotedFrom <http://www.corestandards.org/ELA-Literacy/WHST/9-10/1/c/> ;
    rdfs:subClassOf :CCSS.ELA-Literacy.WHST.9-10.1 ;
    rdfs:comment "Use words, phrases, and clauses to link the major sections of the text, create cohesion, and clarify the relationships between claim(s) and reasons, between reasons and evidence, and between claim(s) and counterclaims."^^xsd:string .

:CCSS.ELA-Literacy.WHST.9-10.1.d rdf:type owl:Class ;
    prov:wasQuotedFrom <http://www.corestandards.org/ELA-Literacy/WHST/9-10/1/d/> ;
    rdfs:subClassOf :CCSS.ELA-Literacy.WHST.9-10.1 ;
    rdfs:comment "Establish and maintain a formal style and objective tone while attending to the norms and conventions of the discipline in which they are writing."^^xsd:string .

:CCSS.ELA-Literacy.WHST.9-10.1.e rdf:type owl:Class ;
    prov:wasQuotedFrom <http://www.corestandards.org/ELA-Literacy/WHST/9-10/1/e/> ;
    rdfs:subClassOf :CCSS.ELA-Literacy.WHST.9-10.1 ;
    rdfs:comment "Provide a concluding statement or section that follows from or supports the argument presented."^^xsd:string .

:CCSS.ELA-Literacy.WHST.9-10.2 rdf:type owl:Class ;
    prov:wasQuotedFrom <http://www.corestandards.org/ELA-Literacy/WHST/9-10/2/> ;
    rdfs:subClassOf :CCSS.ELA-Literacy.WHST.9-10 ;
    rdfs:comment "Write informative/explanatory texts, including the narration of historical events, scientific procedures/ experiments, or technical processes."^^xsd:string .

:CCSS.ELA-Literacy.WHST.9-10.2.a rdf:type owl:Class ;
    prov:wasQuotedFrom <http://www.corestandards.org/ELA-Literacy/WHST/9-10/2/a/> ;
    rdfs:subClassOf :CCSS.ELA-Literacy.WHST.9-10.2 ;
    rdfs:comment "Introduce a topic and organize ideas, concepts, and information to make important connections and distinctions; include formatting (e.g., headings), graphics (e.g., figures, tables), and multimedia when useful to aiding comprehension."^^xsd:string .

:CCSS.ELA-Literacy.WHST.9-10.2.b rdf:type owl:Class ;
    prov:wasQuotedFrom <http://www.corestandards.org/ELA-Literacy/WHST/9-10/2/b/> ;
    rdfs:subClassOf :CCSS.ELA-Literacy.WHST.9-10.2 ;
    rdfs:comment "Develop the topic with well-chosen, relevant, and sufficient facts, extended definitions, concrete details, quotations, or other information and examples appropriate to the audience's knowledge of the topic."^^xsd:string .

:CCSS.ELA-Literacy.WHST.9-10.2.c rdf:type owl:Class ;
    prov:wasQuotedFrom <http://www.corestandards.org/ELA-Literacy/WHST/9-10/2/c/> ;
    rdfs:subClassOf :CCSS.ELA-Literacy.WHST.9-10.2 ;
    rdfs:comment "Use varied transitions and sentence structures to link the major sections of the text, create cohesion, and clarify the relationships among ideas and concepts."^^xsd:string .

:CCSS.ELA-Literacy.WHST.9-10.2.d rdf:type owl:Class ;
    prov:wasQuotedFrom <http://www.corestandards.org/ELA-Literacy/WHST/9-10/2/d/> ;
    rdfs:subClassOf :CCSS.ELA-Literacy.WHST.9-10.2 ;
    rdfs:comment "Use precise language and domain-specific vocabulary to manage the complexity of the topic and convey a style appropriate to the discipline and context as well as to the expertise of likely readers."^^xsd:string .

:CCSS.ELA-Literacy.WHST.9-10.2.e rdf:type owl:Class ;
    prov:wasQuotedFrom <http://www.corestandards.org/ELA-Literacy/WHST/9-10/2/e/> ;
    rdfs:subClassOf :CCSS.ELA-Literacy.WHST.9-10.2 ;
    rdfs:comment "Establish and maintain a formal style and objective tone while attending to the norms and conventions of the discipline in which they are writing."^^xsd:string .

:CCSS.ELA-Literacy.WHST.9-10.2.f rdf:type owl:Class ;
    prov:wasQuotedFrom <http://www.corestandards.org/ELA-Literacy/WHST/9-10/2/f/> ;
    rdfs:subClassOf :CCSS.ELA-Literacy.WHST.9-10.2 ;
    rdfs:comment "Provide a concluding statement or section that follows from and supports the information or explanation presented (e.g., articulating implications or the significance of the topic)."^^xsd:string .

:CCSS.ELA-Literacy.WHST.9-10.3 rdf:type owl:Class ;
    prov:wasQuotedFrom <http://www.corestandards.org/ELA-Literacy/WHST/9-10/3/> ;
    rdfs:subClassOf :CCSS.ELA-Literacy.WHST.9-10 ;
    rdfs:comment "(See note; not applicable as a separate requirement)"^^xsd:string .

:CCSS.ELA-Literacy.WHST.9-10.4 rdf:type owl:Class ;
    prov:wasQuotedFrom <http://www.corestandards.org/ELA-Literacy/WHST/9-10/4/> ;
    rdfs:subClassOf :CCSS.ELA-Literacy.WHST.9-10 ;
    rdfs:comment "Produce clear and coherent writing in which the development, organization, and style are appropriate to task, purpose, and audience."^^xsd:string .

:CCSS.ELA-Literacy.WHST.9-10.5 rdf:type owl:Class ;
    prov:wasQuotedFrom <http://www.corestandards.org/ELA-Literacy/WHST/9-10/5/> ;
    rdfs:subClassOf :CCSS.ELA-Literacy.WHST.9-10 ;
    rdfs:comment "Develop and strengthen writing as needed by planning, revising, editing, rewriting, or trying a new approach, focusing on addressing what is most significant for a specific purpose and audience."^^xsd:string .

:CCSS.ELA-Literacy.WHST.9-10.6 rdf:type owl:Class ;
    prov:wasQuotedFrom <http://www.corestandards.org/ELA-Literacy/WHST/9-10/6/> ;
    rdfs:subClassOf :CCSS.ELA-Literacy.WHST.9-10 ;
    rdfs:comment "Use technology, including the Internet, to produce, publish, and update individual or shared writing products, taking advantage of technology's capacity to link to other information and to display information flexibly and dynamically."^^xsd:string .

:CCSS.ELA-Literacy.WHST.9-10.7 rdf:type owl:Class ;
    prov:wasQuotedFrom <http://www.corestandards.org/ELA-Literacy/WHST/9-10/7/> ;
    rdfs:subClassOf :CCSS.ELA-Literacy.WHST.9-10 ;
    rdfs:comment "Conduct short as well as more sustained research projects to answer a question (including a self-generated question) or solve a problem; narrow or broaden the inquiry when appropriate; synthesize multiple sources on the subject, demonstrating understanding of the subject under investigation."^^xsd:string .

:CCSS.ELA-Literacy.WHST.9-10.8 rdf:type owl:Class ;
    prov:wasQuotedFrom <http://www.corestandards.org/ELA-Literacy/WHST/9-10/8/> ;
    rdfs:subClassOf :CCSS.ELA-Literacy.WHST.9-10 ;
    rdfs:comment "Gather relevant information from multiple authoritative print and digital sources, using advanced searches effectively; assess the usefulness of each source in answering the research question; integrate information into the text selectively to maintain the flow of ideas, avoiding plagiarism and following a standard format for citation."^^xsd:string .

:CCSS.ELA-Literacy.WHST.9-10.9 rdf:type owl:Class ;
    prov:wasQuotedFrom <http://www.corestandards.org/ELA-Literacy/WHST/9-10/9/> ;
    rdfs:subClassOf :CCSS.ELA-Literacy.WHST.9-10 ;
    rdfs:comment "Draw evidence from informational texts to support analysis, reflection, and research."^^xsd:string .

:CCSS.ELA-Literacy.WHST.9-10.10 rdf:type owl:Class ;
    prov:wasQuotedFrom <http://www.corestandards.org/ELA-Literacy/WHST/9-10/10/> ;
    rdfs:subClassOf :CCSS.ELA-Literacy.WHST.9-10 ;
    rdfs:comment "Write routinely over extended time frames (time for reflection and revision) and shorter time frames (a single sitting or a day or two) for a range of discipline-specific tasks, purposes, and audiences."^^xsd:string .

:CCSS.ELA-Literacy.WHST.11-12 rdf:type owl:Class ;
    prov:wasQuotedFrom <http://www.corestandards.org/ELA-Literacy/WHST/11-12/> ;
    rdfs:subClassOf :CCSS.ELA-Literacy.WHST .

:CCSS.ELA-Literacy.WHST.11-12.1 rdf:type owl:Class ;
    prov:wasQuotedFrom <http://www.corestandards.org/ELA-Literacy/WHST/11-12/1/> ;
    rdfs:subClassOf :CCSS.ELA-Literacy.WHST.11-12 ;
    rdfs:comment "Write arguments focused on discipline-specific content."^^xsd:string .

:CCSS.ELA-Literacy.WHST.11-12.1.a rdf:type owl:Class ;
    prov:wasQuotedFrom <http://www.corestandards.org/ELA-Literacy/WHST/11-12/1/a/> ;
    rdfs:subClassOf :CCSS.ELA-Literacy.WHST.11-12.1 ;
    rdfs:comment "Introduce precise, knowledgeable claim(s), establish the significance of the claim(s), distinguish the claim(s) from alternate or opposing claims, and create an organization that logically sequences the claim(s), counterclaims, reasons, and evidence."^^xsd:string .

:CCSS.ELA-Literacy.WHST.11-12.1.b rdf:type owl:Class ;
    prov:wasQuotedFrom <http://www.corestandards.org/ELA-Literacy/WHST/11-12/1/b/> ;
    rdfs:subClassOf :CCSS.ELA-Literacy.WHST.11-12.1 ;
    rdfs:comment "Develop claim(s) and counterclaims fairly and thoroughly, supplying the most relevant data and evidence for each while pointing out the strengths and limitations of both claim(s) and counterclaims in a discipline-appropriate form that anticipates the audience's knowledge level, concerns, values, and possible biases."^^xsd:string .

:CCSS.ELA-Literacy.WHST.11-12.1.c rdf:type owl:Class ;
    prov:wasQuotedFrom <http://www.corestandards.org/ELA-Literacy/WHST/11-12/1/c/> ;
    rdfs:subClassOf :CCSS.ELA-Literacy.WHST.11-12.1 ;
    rdfs:comment "Use words, phrases, and clauses as well as varied syntax to link the major sections of the text, create cohesion, and clarify the relationships between claim(s) and reasons, between reasons and evidence, and between claim(s) and counterclaims."^^xsd:string .

:CCSS.ELA-Literacy.WHST.11-12.1.d rdf:type owl:Class ;
    prov:wasQuotedFrom <http://www.corestandards.org/ELA-Literacy/WHST/11-12/1/d/> ;
    rdfs:subClassOf :CCSS.ELA-Literacy.WHST.11-12.1 ;
    rdfs:comment "Establish and maintain a formal style and objective tone while attending to the norms and conventions of the discipline in which they are writing."^^xsd:string .

:CCSS.ELA-Literacy.WHST.11-12.1.e rdf:type owl:Class ;
    prov:wasQuotedFrom <http://www.corestandards.org/ELA-Literacy/WHST/11-12/1/e/> ;
    rdfs:subClassOf :CCSS.ELA-Literacy.WHST.11-12.1 ;
    rdfs:comment "Provide a concluding statement or section that follows from or supports the argument presented."^^xsd:string .

:CCSS.ELA-Literacy.WHST.11-12.2 rdf:type owl:Class ;
    prov:wasQuotedFrom <http://www.corestandards.org/ELA-Literacy/WHST/11-12/2/> ;
    rdfs:subClassOf :CCSS.ELA-Literacy.WHST.11-12 ;
    rdfs:comment "Write informative/explanatory texts, including the narration of historical events, scientific procedures/experiments, or technical processes."^^xsd:string .

:CCSS.ELA-Literacy.WHST.11-12.2.a rdf:type owl:Class ;
    prov:wasQuotedFrom <http://www.corestandards.org/ELA-Literacy/WHST/11-12/2/a/> ;
    rdfs:subClassOf :CCSS.ELA-Literacy.WHST.11-12.2 ;
    rdfs:comment "Introduce a topic and organize complex ideas, concepts, and information so that each new element builds on that which precedes it to create a unified whole; include formatting (e.g., headings), graphics (e.g., figures, tables), and multimedia when useful to aiding comprehension."^^xsd:string .

:CCSS.ELA-Literacy.WHST.11-12.2.b rdf:type owl:Class ;
    prov:wasQuotedFrom <http://www.corestandards.org/ELA-Literacy/WHST/11-12/2/b/> ;
    rdfs:subClassOf :CCSS.ELA-Literacy.WHST.11-12.2 ;
    rdfs:comment "Develop the topic thoroughly by selecting the most significant and relevant facts, extended definitions, concrete details, quotations, or other information and examples appropriate to the audience's knowledge of the topic."^^xsd:string .

:CCSS.ELA-Literacy.WHST.11-12.2.c rdf:type owl:Class ;
    prov:wasQuotedFrom <http://www.corestandards.org/ELA-Literacy/WHST/11-12/2/c/> ;
    rdfs:subClassOf :CCSS.ELA-Literacy.WHST.11-12.2 ;
    rdfs:comment "Use varied transitions and sentence structures to link the major sections of the text, create cohesion, and clarify the relationships among complex ideas and concepts."^^xsd:string .

:CCSS.ELA-Literacy.WHST.11-12.2.d rdf:type owl:Class ;
    prov:wasQuotedFrom <http://www.corestandards.org/ELA-Literacy/WHST/11-12/2/d/> ;
    rdfs:subClassOf :CCSS.ELA-Literacy.WHST.11-12.2 ;
    rdfs:comment "Use precise language, domain-specific vocabulary and techniques such as metaphor, simile, and analogy to manage the complexity of the topic; convey a knowledgeable stance in a style that responds to the discipline and context as well as to the expertise of likely readers."^^xsd:string .

:CCSS.ELA-Literacy.WHST.11-12.2.e rdf:type owl:Class ;
    prov:wasQuotedFrom <http://www.corestandards.org/ELA-Literacy/WHST/11-12/2/e/> ;
    rdfs:subClassOf :CCSS.ELA-Literacy.WHST.11-12.2 ;
    rdfs:comment "Provide a concluding statement or section that follows from and supports the information or explanation provided (e.g., articulating implications or the significance of the topic)."^^xsd:string .

:CCSS.ELA-Literacy.WHST.11-12.3 rdf:type owl:Class ;
    prov:wasQuotedFrom <http://www.corestandards.org/ELA-Literacy/WHST/11-12/3/> ;
    rdfs:subClassOf :CCSS.ELA-Literacy.WHST.11-12 ;
    rdfs:comment "(See note; not applicable as a separate requirement)"^^xsd:string .

:CCSS.ELA-Literacy.WHST.11-12.4 rdf:type owl:Class ;
    prov:wasQuotedFrom <http://www.corestandards.org/ELA-Literacy/WHST/11-12/4/> ;
    rdfs:subClassOf :CCSS.ELA-Literacy.WHST.11-12 ;
    rdfs:comment "Produce clear and coherent writing in which the development, organization, and style are appropriate to task, purpose, and audience."^^xsd:string .

:CCSS.ELA-Literacy.WHST.11-12.5 rdf:type owl:Class ;
    prov:wasQuotedFrom <http://www.corestandards.org/ELA-Literacy/WHST/11-12/5/> ;
    rdfs:subClassOf :CCSS.ELA-Literacy.WHST.11-12 ;
    rdfs:comment "Develop and strengthen writing as needed by planning, revising, editing, rewriting, or trying a new approach, focusing on addressing what is most significant for a specific purpose and audience."^^xsd:string .

:CCSS.ELA-Literacy.WHST.11-12.6 rdf:type owl:Class ;
    prov:wasQuotedFrom <http://www.corestandards.org/ELA-Literacy/WHST/11-12/6/> ;
    rdfs:subClassOf :CCSS.ELA-Literacy.WHST.11-12 ;
    rdfs:comment "Use technology, including the Internet, to produce, publish, and update individual or shared writing products in response to ongoing feedback, including new arguments or information."^^xsd:string .

:CCSS.ELA-Literacy.WHST.11-12.7 rdf:type owl:Class ;
    prov:wasQuotedFrom <http://www.corestandards.org/ELA-Literacy/WHST/11-12/7/> ;
    rdfs:subClassOf :CCSS.ELA-Literacy.WHST.11-12 ;
    rdfs:comment "Conduct short as well as more sustained research projects to answer a question (including a self-generated question) or solve a problem; narrow or broaden the inquiry when appropriate; synthesize multiple sources on the subject, demonstrating understanding of the subject under investigation."^^xsd:string .

:CCSS.ELA-Literacy.WHST.11-12.8 rdf:type owl:Class ;
    prov:wasQuotedFrom <http://www.corestandards.org/ELA-Literacy/WHST/11-12/8/> ;
    rdfs:subClassOf :CCSS.ELA-Literacy.WHST.11-12 ;
    rdfs:comment "Gather relevant information from multiple authoritative print and digital sources, using advanced searches effectively; assess the strengths and limitations of each source in terms of the specific task, purpose, and audience; integrate information into the text selectively to maintain the flow of ideas, avoiding plagiarism and overreliance on any one source and following a standard format for citation."^^xsd:string .

:CCSS.ELA-Literacy.WHST.11-12.9 rdf:type owl:Class ;
    prov:wasQuotedFrom <http://www.corestandards.org/ELA-Literacy/WHST/11-12/9/> ;
    rdfs:subClassOf :CCSS.ELA-Literacy.WHST.11-12 ;
    rdfs:comment "Draw evidence from informational texts to support analysis, reflection, and research."^^xsd:string .

:CCSS.ELA-Literacy.WHST.11-12.10 rdf:type owl:Class ;
    prov:wasQuotedFrom <http://www.corestandards.org/ELA-Literacy/WHST/11-12/10/> ;
    rdfs:subClassOf :CCSS.ELA-Literacy.WHST.11-12 ;
    rdfs:comment "Write routinely over extended time frames (time for reflection and revision) and shorter time frames (a single sitting or a day or two) for a range of discipline-specific tasks, purposes, and audiences."^^xsd:string .

:CCSS.Math rdf:type owl:Class ;
    rdfs:label "Mathematics Standards"^^xsd:string ;
    prov:wasQuotedFrom <http://www.corestandards.org/Math/> .

:CCSS.Math.Practice rdf:type owl:Class ;
    rdfs:subClassOf :CCSS.Math ;
    rdfs:label "Standards for Mathematical Practice"^^xsd:string ;
    prov:wasQuotedFrom <http://www.corestandards.org/Math/Practice/> .

:CCSS.Math.Practice.MP1 rdf:type owl:Class ;
    rdfs:subClassOf :CCSS.Math.Practice ;
    prov:wasQuotedFrom <http://www.corestandards.org/Math/Practice/MP1/> ;
    rdfs:label "Standards for Mathematical Practice - Make sense of problems and persevere in solving them."^^xsd:string ;
    rdfs:comment "Mathematically proficient students start by explaining to themselves the meaning of a problem and looking for entry points to its solution. They analyze givens, constraints, relationships, and goals. They make conjectures about the form and meaning of the solution and plan a solution pathway rather than simply jumping into a solution attempt. They consider analogous problems, and try special cases and simpler forms of the original problem in order to gain insight into its solution. They monitor and evaluate their progress and change course if necessary. Older students might, depending on the context of the problem, transform algebraic expressions or change the viewing window on their graphing calculator to get the information they need. Mathematically proficient students can explain correspondences between equations, verbal descriptions, tables, and graphs or draw diagrams of important features and relationships, graph data, and search for regularity or trends. Younger students might rely on using concrete objects or pictures to help conceptualize and solve a problem. Mathematically proficient students check their answers to problems using a different method, and they continually ask themselves, -Does this make sense?- They can understand the approaches of others to solving complex problems and identify correspondences between different approaches."^^xsd:string .

:CCSS.Math.Practice.MP2 rdf:type owl:Class ;
    rdfs:subClassOf :CCSS.Math.Practice ;
    prov:wasQuotedFrom <http://www.corestandards.org/Math/Practice/MP2/> ;
    rdfs:label "Standards for Mathematical Practice - Reason abstractly and quantitatively."^^xsd:string ;
    rdfs:comment "Mathematically proficient students make sense of quantities and their relationships in problem situations. They bring two complementary abilities to bear on problems involving quantitative relationships: the ability to decontextualize-to abstract a given situation and represent it symbolically and manipulate the representing symbols as if they have a life of their own, without necessarily attending to their referents-and the ability to contextualize, to pause as needed during the manipulation process in order to probe into the referents for the symbols involved. Quantitative reasoning entails habits of creating a coherent representation of the problem at hand; considering the units involved; attending to the meaning of quantities, not just how to compute them; and knowing and flexibly using different properties of operations and objects."^^xsd:string .

:CCSS.Math.Practice.MP3 rdf:type owl:Class ;
    rdfs:subClassOf :CCSS.Math.Practice ;
    prov:wasQuotedFrom <http://www.corestandards.org/Math/Practice/MP3/> ;
    rdfs:label "Standards for Mathematical Practice - Construct viable arguments and critique the reasoning of others."^^xsd:string ;
    rdfs:comment "Mathematically proficient students understand and use stated assumptions, definitions, and previously established results in constructing arguments. They make conjectures and build a logical progression of statements to explore the truth of their conjectures. They are able to analyze situations by breaking them into cases, and can recognize and use counterexamples. They justify their conclusions, communicate them to others, and respond to the arguments of others. They reason inductively about data, making plausible arguments that take into account the context from which the data arose. Mathematically proficient students are also able to compare the effectiveness of two plausible arguments, distinguish correct logic or reasoning from that which is flawed, and-if there is a flaw in an argument-explain what it is. Elementary students can construct arguments using concrete referents such as objects, drawings, diagrams, and actions. Such arguments can make sense and be correct, even though they are not generalized or made formal until later grades. Later, students learn to determine domains to which an argument applies. Students at all grades can listen or read the arguments of others, decide whether they make sense, and ask useful questions to clarify or improve the arguments."^^xsd:string .

:CCSS.Math.Practice.MP4 rdf:type owl:Class ;
    rdfs:subClassOf :CCSS.Math.Practice ;
    prov:wasQuotedFrom <http://www.corestandards.org/Math/Practice/MP4/> ;
    rdfs:label "Standards for Mathematical Practice - Model with mathematics."^^xsd:string ;
    rdfs:comment "Mathematically proficient students can apply the mathematics they know to solve problems arising in everyday life, society, and the workplace. In early grades, this might be as simple as writing an addition equation to describe a situation. In middle grades, a student might apply proportional reasoning to plan a school event or analyze a problem in the community. By high school, a student might use geometry to solve a design problem or use a function to describe how one quantity of interest depends on another. Mathematically proficient students who can apply what they know are comfortable making assumptions and approximations to simplify a complicated situation, realizing that these may need revision later. They are able to identify important quantities in a practical situation and map their relationships using such tools as diagrams, two-way tables, graphs, flowcharts and formulas. They can analyze those relationships mathematically to draw conclusions. They routinely interpret their mathematical results in the context of the situation and reflect on whether the results make sense, possibly improving the model if it has not served its purpose."^^xsd:string .

:CCSS.Math.Practice.MP5 rdf:type owl:Class ;
    rdfs:subClassOf :CCSS.Math.Practice ;
    prov:wasQuotedFrom <http://www.corestandards.org/Math/Practice/MP5/> ;
    rdfs:label "Standards for Mathematical Practice - Use appropriate tools strategically."^^xsd:string ;
    rdfs:comment "Mathematically proficient students consider the available tools when solving a mathematical problem. These tools might include pencil and paper, concrete models, a ruler, a protractor, a calculator, a spreadsheet, a computer algebra system, a statistical package, or dynamic geometry software. Proficient students are sufficiently familiar with tools appropriate for their grade or course to make sound decisions about when each of these tools might be helpful, recognizing both the insight to be gained and their limitations. For example, mathematically proficient high school students analyze graphs of functions and solutions generated using a graphing calculator. They detect possible errors by strategically using estimation and other mathematical knowledge. When making mathematical models, they know that technology can enable them to visualize the results of varying assumptions, explore consequences, and compare predictions with data. Mathematically proficient students at various grade levels are able to identify relevant external mathematical resources, such as digital content located on a website, and use them to pose or solve problems. They are able to use technological tools to explore and deepen their understanding of concepts."^^xsd:string .

:CCSS.Math.Practice.MP6 rdf:type owl:Class ;
    rdfs:subClassOf :CCSS.Math.Practice ;
    prov:wasQuotedFrom <http://www.corestandards.org/Math/Practice/MP6/> ;
    rdfs:label "Standards for Mathematical Practice - Attend to precision."^^xsd:string ;
    rdfs:comment "Mathematically proficient students try to communicate precisely to others. They try to use clear definitions in discussion with others and in their own reasoning. They state the meaning of the symbols they choose, including using the equal sign consistently and appropriately. They are careful about specifying units of measure, and labeling axes to clarify the correspondence with quantities in a problem. They calculate accurately and efficiently, express numerical answers with a degree of precision appropriate for the problem context. In the elementary grades, students give carefully formulated explanations to each other. By the time they reach high school they have learned to examine claims and make explicit use of definitions."^^xsd:string .

:CCSS.Math.Practice.MP7 rdf:type owl:Class ;
    rdfs:subClassOf :CCSS.Math.Practice ;
    prov:wasQuotedFrom <http://www.corestandards.org/Math/Practice/MP7/> ;
    rdfs:label "Standards for Mathematical Practice - Look for and make use of structure."^^xsd:string ;
    rdfs:comment "Mathematically proficient students look closely to discern a pattern or structure. Young students, for example, might notice that three and seven more is the same amount as seven and three more, or they may sort a collection of shapes according to how many sides the shapes have. Later, students will see 7 - 8 equals the well remembered 7 - 5 + 7 - 3, in preparation for learning about the distributive property. In the expression x2 + 9x + 14, older students can see the 14 as 2 - 7 and the 9 as 2 + 7. They recognize the significance of an existing line in a geometric figure and can use the strategy of drawing an auxiliary line for solving problems. They also can step back for an overview and shift perspective. They can see complicated things, such as some algebraic expressions, as single objects or as being composed of several objects. For example, they can see 5 - 3(x - y)2 as 5 minus a positive number times a square and use that to realize that its value cannot be more than 5 for any real numbers x and y."^^xsd:string .

:CCSS.Math.Practice.MP8 rdf:type owl:Class ;
    rdfs:subClassOf :CCSS.Math.Practice ;
    prov:wasQuotedFrom <http://www.corestandards.org/Math/Practice/MP8/> ;
    rdfs:label "Standards for Mathematical Practice - Look for and express regularity in repeated reasoning."^^xsd:string ;
    rdfs:comment "Mathematically proficient students notice if calculations are repeated, and look both for general methods and for shortcuts. Upper elementary students might notice when dividing 25 by 11 that they are repeating the same calculations over and over again, and conclude they have a repeating decimal. By paying attention to the calculation of slope as they repeatedly check whether points are on the line through (1, 2) with slope 3, middle school students might abstract the equation (y - 2)/(x - 1) = 3. Noticing the regularity in the way terms cancel when expanding (x - 1)(x + 1), (x - 1)(x2 + x + 1), and (x - 1)(x3 + x2 + x + 1) might lead them to the general formula for the sum of a geometric series. As they work to solve a problem, mathematically proficient students maintain oversight of the process, while attending to the details. They continually evaluate the reasonableness of their intermediate results."^^xsd:string .

:CCSS.Math.Content rdf:type owl:Class ;
    rdfs:subClassOf :CCSS.Math ;
    rdfs:label "Standards for Mathematical Content"^^xsd:string ;
    prov:wasQuotedFrom <http://www.corestandards.org/Math/Content/> .

:CCSS.Math.Content.K rdf:type owl:Class ;
    rdfs:subClassOf :CCSS.Math.Content ;
    rdfs:label "Standards for Mathematical Content"^^xsd:string ;
    prov:wasQuotedFrom <http://www.corestandards.org/Math/Content/K/> .

:CCSS.Math.Content.K.CC rdf:type owl:Class ;
    rdfs:subClassOf :CCSS.Math.Content.K ;
    rdfs:label "Counting & Cardinality"^^xsd:string ;
    prov:wasQuotedFrom <http://www.corestandards.org/Math/Content/K/CC/> .

:CCSS.Math.Content.K.CC.A rdf:type owl:Class ;
    rdfs:subClassOf :CCSS.Math.Content.K.CC ;
    rdfs:label "Counting & Cardinality"^^xsd:string ;
    prov:wasQuotedFrom <http://www.corestandards.org/Math/Content/K/CC/> .

:CCSS.Math.Content.K.CC.A.1 rdf:type owl:Class ;
    rdfs:subClassOf :CCSS.Math.Content.K.CC.A ;
    prov:wasQuotedFrom <http://www.corestandards.org/Math/Content/K/CC/1/> ;
    rdfs:label "English Language Arts Standards - Anchor Standards - College and Career Readiness Anchor Standards for Language - 1"^^xsd:string ;
    rdfs:comment "Demonstrate command of the conventions of standard English grammar and usage when writing or speaking."^^xsd:string .

:CCSS.Math.Content.K.CC.A.2 rdf:type owl:Class ;
    rdfs:subClassOf :CCSS.Math.Content.K.CC.A ;
    prov:wasQuotedFrom <http://www.corestandards.org/Math/Content/K/CC/2/> ;
    rdfs:label "English Language Arts Standards - Anchor Standards - College and Career Readiness Anchor Standards for Language - 2"^^xsd:string ;
    rdfs:comment "Demonstrate command of the conventions of standard English capitalization, punctuation, and spelling when writing."^^xsd:string .

:CCSS.Math.Content.K.CC.A.3 rdf:type owl:Class ;
    rdfs:subClassOf :CCSS.Math.Content.K.CC.A ;
    prov:wasQuotedFrom <http://www.corestandards.org/Math/Content/K/CC/3/> ;
    rdfs:label "English Language Arts Standards - Anchor Standards - College and Career Readiness Anchor Standards for Language - 3"^^xsd:string ;
    rdfs:comment "Apply knowledge of language to understand how language functions in different contexts, to make effective choices for meaning or style, and to comprehend more fully when reading or listening. "^^xsd:string .

:CCSS.Math.Content.K.CC.B rdf:type owl:Class ;
    rdfs:subClassOf :CCSS.Math.Content.K.CC ;
    rdfs:label "Counting & Cardinality"^^xsd:string ;
    prov:wasQuotedFrom <http://www.corestandards.org/Math/Content/K/CC/> .

:CCSS.Math.Content.K.CC.B.4 rdf:type owl:Class ;
    rdfs:subClassOf :CCSS.Math.Content.K.CC.B ;
    prov:wasQuotedFrom <http://www.corestandards.org/Math/Content/K/CC/4/> ;
    rdfs:label "English Language Arts Standards - Anchor Standards - College and Career Readiness Anchor Standards for Language - 4"^^xsd:string ;
    rdfs:comment "Determine or clarify the meaning of unknown and multiple-meaning words and phrases by using context clues, analyzing meaningful word parts, and consulting general and specialized reference materials, as appropriate."^^xsd:string .

:CCSS.Math.Content.K.CC.B.5 rdf:type owl:Class ;
    rdfs:subClassOf :CCSS.Math.Content.K.CC.B ;
    prov:wasQuotedFrom <http://www.corestandards.org/Math/Content/K/CC/5/> ;
    rdfs:label "English Language Arts Standards - Anchor Standards - College and Career Readiness Anchor Standards for Language - 5"^^xsd:string ;
    rdfs:comment "Demonstrate understanding of figurative language, word relationships, and nuances in word meanings."^^xsd:string .

:CCSS.Math.Content.K.CC.C rdf:type owl:Class ;
    rdfs:subClassOf :CCSS.Math.Content.K.CC ;
    rdfs:label "Counting & Cardinality"^^xsd:string ;
    prov:wasQuotedFrom <http://www.corestandards.org/Math/Content/K/CC/> .

:CCSS.Math.Content.K.CC.C.6 rdf:type owl:Class ;
    rdfs:subClassOf :CCSS.Math.Content.K.CC.C ;
    prov:wasQuotedFrom <http://www.corestandards.org/Math/Content/K/CC/6/> ;
    rdfs:label "English Language Arts Standards - Anchor Standards - College and Career Readiness Anchor Standards for Language - 6"^^xsd:string ;
    rdfs:comment "Acquire and use accurately a range of general academic and domain-specific words and phrases sufficient for reading, writing, speaking, and listening at the college and career readiness level; demonstrate independence in gathering vocabulary knowledge when encountering an unknown term important to comprehension or expression."^^xsd:string .

:CCSS.Math.Content.K.CC.C.7 rdf:type owl:Class ;
    rdfs:subClassOf :CCSS.Math.Content.K.CC.C ;
    prov:wasQuotedFrom <http://www.corestandards.org/Math/Content/K/CC/7/> ;
    rdfs:label "English Language Arts Standards - Anchor Standards - College and Career Readiness Anchor Standards for Reading - 7"^^xsd:string ;
    rdfs:comment "Integrate and evaluate content presented in diverse media and formats, including visually and quantitatively, as well as in words.1"^^xsd:string .

:CCSS.Math.Content.K.CC.B.4.a rdf:type owl:Class ;
    rdfs:subClassOf :CCSS.Math.Content.K.CC.B.4 ;
    prov:wasQuotedFrom <http://www.corestandards.org/Math/Content/K/CC/a/> .

:CCSS.Math.Content.K.CC.B.4.b rdf:type owl:Class ;
    rdfs:subClassOf :CCSS.Math.Content.K.CC.B.4 ;
    prov:wasQuotedFrom <http://www.corestandards.org/Math/Content/K/CC/b/> .

:CCSS.Math.Content.K.CC.B.4.c rdf:type owl:Class ;
    rdfs:subClassOf :CCSS.Math.Content.K.CC.B.4 ;
    prov:wasQuotedFrom <http://www.corestandards.org/Math/Content/K/CC/c/> .

:CCSS.Math.Content.K.OA rdf:type owl:Class ;
    rdfs:subClassOf :CCSS.Math.Content.K ;
    rdfs:label "Operations & Algebraic Thinking"^^xsd:string ;
    prov:wasQuotedFrom <http://www.corestandards.org/Math/Content/K/OA/> .

:CCSS.Math.Content.K.OA.A rdf:type owl:Class ;
    rdfs:subClassOf :CCSS.Math.Content.K.OA ;
    rdfs:label "Operations & Algebraic Thinking"^^xsd:string ;
    prov:wasQuotedFrom <http://www.corestandards.org/Math/Content/K/OA/> .

:CCSS.Math.Content.K.OA.A.1 rdf:type owl:Class ;
    rdfs:subClassOf :CCSS.Math.Content.K.OA.A ;
    prov:wasQuotedFrom <http://www.corestandards.org/Math/Content/K/OA/1/> ;
    rdfs:label "English Language Arts Standards - Anchor Standards - College and Career Readiness Anchor Standards for Language - 1"^^xsd:string ;
    rdfs:comment "Demonstrate command of the conventions of standard English grammar and usage when writing or speaking."^^xsd:string .

:CCSS.Math.Content.K.OA.A.2 rdf:type owl:Class ;
    rdfs:subClassOf :CCSS.Math.Content.K.OA.A ;
    prov:wasQuotedFrom <http://www.corestandards.org/Math/Content/K/OA/2/> ;
    rdfs:label "English Language Arts Standards - Anchor Standards - College and Career Readiness Anchor Standards for Language - 2"^^xsd:string ;
    rdfs:comment "Demonstrate command of the conventions of standard English capitalization, punctuation, and spelling when writing."^^xsd:string .

:CCSS.Math.Content.K.OA.A.3 rdf:type owl:Class ;
    rdfs:subClassOf :CCSS.Math.Content.K.OA.A ;
    prov:wasQuotedFrom <http://www.corestandards.org/Math/Content/K/OA/3/> ;
    rdfs:label "English Language Arts Standards - Anchor Standards - College and Career Readiness Anchor Standards for Language - 3"^^xsd:string ;
    rdfs:comment "Apply knowledge of language to understand how language functions in different contexts, to make effective choices for meaning or style, and to comprehend more fully when reading or listening. "^^xsd:string .

:CCSS.Math.Content.K.OA.A.4 rdf:type owl:Class ;
    rdfs:subClassOf :CCSS.Math.Content.K.OA.A ;
    prov:wasQuotedFrom <http://www.corestandards.org/Math/Content/K/OA/4/> ;
    rdfs:label "English Language Arts Standards - Anchor Standards - College and Career Readiness Anchor Standards for Language - 4"^^xsd:string ;
    rdfs:comment "Determine or clarify the meaning of unknown and multiple-meaning words and phrases by using context clues, analyzing meaningful word parts, and consulting general and specialized reference materials, as appropriate."^^xsd:string .

:CCSS.Math.Content.K.OA.A.5 rdf:type owl:Class ;
    rdfs:subClassOf :CCSS.Math.Content.K.OA.A ;
    prov:wasQuotedFrom <http://www.corestandards.org/Math/Content/K/OA/5/> ;
    rdfs:label "English Language Arts Standards - Anchor Standards - College and Career Readiness Anchor Standards for Language - 5"^^xsd:string ;
    rdfs:comment "Demonstrate understanding of figurative language, word relationships, and nuances in word meanings."^^xsd:string .

:CCSS.Math.Content.K.NBT rdf:type owl:Class ;
    rdfs:subClassOf :CCSS.Math.Content.K ;
    rdfs:label "Number & Operations in Base Ten"^^xsd:string ;
    prov:wasQuotedFrom <http://www.corestandards.org/Math/Content/K/NBT/> .

:CCSS.Math.Content.K.NBT.A rdf:type owl:Class ;
    rdfs:subClassOf :CCSS.Math.Content.K.NBT ;
    rdfs:label "Number & Operations in Base Ten"^^xsd:string ;
    prov:wasQuotedFrom <http://www.corestandards.org/Math/Content/K/NBT/> .

:CCSS.Math.Content.K.NBT.A.1 rdf:type owl:Class ;
    rdfs:subClassOf :CCSS.Math.Content.K.NBT.A ;
    prov:wasQuotedFrom <http://www.corestandards.org/Math/Content/K/NBT/1/> ;
    rdfs:label "English Language Arts Standards - Anchor Standards - College and Career Readiness Anchor Standards for Language - 1"^^xsd:string ;
    rdfs:comment "Demonstrate command of the conventions of standard English grammar and usage when writing or speaking."^^xsd:string .

:CCSS.Math.Content.K.MD rdf:type owl:Class ;
    rdfs:subClassOf :CCSS.Math.Content.K ;
    rdfs:label "Measurement & Data"^^xsd:string ;
    prov:wasQuotedFrom <http://www.corestandards.org/Math/Content/K/MD/> .

:CCSS.Math.Content.K.MD.A rdf:type owl:Class ;
    rdfs:subClassOf :CCSS.Math.Content.K.MD ;
    rdfs:label "Measurement & Data"^^xsd:string ;
    prov:wasQuotedFrom <http://www.corestandards.org/Math/Content/K/MD/> .

:CCSS.Math.Content.K.MD.A.1 rdf:type owl:Class ;
    rdfs:subClassOf :CCSS.Math.Content.K.MD.A ;
    prov:wasQuotedFrom <http://www.corestandards.org/Math/Content/K/MD/1/> ;
    rdfs:label "English Language Arts Standards - Anchor Standards - College and Career Readiness Anchor Standards for Language - 1"^^xsd:string ;
    rdfs:comment "Demonstrate command of the conventions of standard English grammar and usage when writing or speaking."^^xsd:string .

:CCSS.Math.Content.K.MD.A.2 rdf:type owl:Class ;
    rdfs:subClassOf :CCSS.Math.Content.K.MD.A ;
    prov:wasQuotedFrom <http://www.corestandards.org/Math/Content/K/MD/2/> ;
    rdfs:label "English Language Arts Standards - Anchor Standards - College and Career Readiness Anchor Standards for Language - 2"^^xsd:string ;
    rdfs:comment "Demonstrate command of the conventions of standard English capitalization, punctuation, and spelling when writing."^^xsd:string .

:CCSS.Math.Content.K.MD.B rdf:type owl:Class ;
    rdfs:subClassOf :CCSS.Math.Content.K.MD ;
    rdfs:label "Measurement & Data"^^xsd:string ;
    prov:wasQuotedFrom <http://www.corestandards.org/Math/Content/K/MD/> .

:CCSS.Math.Content.K.MD.B.3 rdf:type owl:Class ;
    rdfs:subClassOf :CCSS.Math.Content.K.MD.B ;
    prov:wasQuotedFrom <http://www.corestandards.org/Math/Content/K/MD/3/> ;
    rdfs:label "English Language Arts Standards - Anchor Standards - College and Career Readiness Anchor Standards for Language - 3"^^xsd:string ;
    rdfs:comment "Apply knowledge of language to understand how language functions in different contexts, to make effective choices for meaning or style, and to comprehend more fully when reading or listening. "^^xsd:string .

:CCSS.Math.Content.K.G rdf:type owl:Class ;
    rdfs:subClassOf :CCSS.Math.Content.K ;
    rdfs:label "Geometry"^^xsd:string ;
    prov:wasQuotedFrom <http://www.corestandards.org/Math/Content/K/G/> .

:CCSS.Math.Content.K.G.A rdf:type owl:Class ;
    rdfs:subClassOf :CCSS.Math.Content.K.G ;
    rdfs:label "Geometry"^^xsd:string ;
    prov:wasQuotedFrom <http://www.corestandards.org/Math/Content/K/G/> .

:CCSS.Math.Content.K.G.A.1 rdf:type owl:Class ;
    rdfs:subClassOf :CCSS.Math.Content.K.G.A ;
    prov:wasQuotedFrom <http://www.corestandards.org/Math/Content/K/G/1/> ;
    rdfs:label "English Language Arts Standards - Anchor Standards - College and Career Readiness Anchor Standards for Language - 1"^^xsd:string ;
    rdfs:comment "Demonstrate command of the conventions of standard English grammar and usage when writing or speaking."^^xsd:string .

:CCSS.Math.Content.K.G.A.2 rdf:type owl:Class ;
    rdfs:subClassOf :CCSS.Math.Content.K.G.A ;
    prov:wasQuotedFrom <http://www.corestandards.org/Math/Content/K/G/2/> ;
    rdfs:label "English Language Arts Standards - Anchor Standards - College and Career Readiness Anchor Standards for Language - 2"^^xsd:string ;
    rdfs:comment "Demonstrate command of the conventions of standard English capitalization, punctuation, and spelling when writing."^^xsd:string .

:CCSS.Math.Content.K.G.A.3 rdf:type owl:Class ;
    rdfs:subClassOf :CCSS.Math.Content.K.G.A ;
    prov:wasQuotedFrom <http://www.corestandards.org/Math/Content/K/G/3/> ;
    rdfs:label "English Language Arts Standards - Anchor Standards - College and Career Readiness Anchor Standards for Language - 3"^^xsd:string ;
    rdfs:comment "Apply knowledge of language to understand how language functions in different contexts, to make effective choices for meaning or style, and to comprehend more fully when reading or listening. "^^xsd:string .

:CCSS.Math.Content.K.G.B rdf:type owl:Class ;
    rdfs:subClassOf :CCSS.Math.Content.K.G ;
    rdfs:label "Geometry"^^xsd:string ;
    prov:wasQuotedFrom <http://www.corestandards.org/Math/Content/K/G/> .

:CCSS.Math.Content.K.G.B.4 rdf:type owl:Class ;
    rdfs:subClassOf :CCSS.Math.Content.K.G.B ;
    prov:wasQuotedFrom <http://www.corestandards.org/Math/Content/K/G/4/> ;
    rdfs:label "English Language Arts Standards - Anchor Standards - College and Career Readiness Anchor Standards for Language - 4"^^xsd:string ;
    rdfs:comment "Determine or clarify the meaning of unknown and multiple-meaning words and phrases by using context clues, analyzing meaningful word parts, and consulting general and specialized reference materials, as appropriate."^^xsd:string .

:CCSS.Math.Content.K.G.B.5 rdf:type owl:Class ;
    rdfs:subClassOf :CCSS.Math.Content.K.G.B ;
    prov:wasQuotedFrom <http://www.corestandards.org/Math/Content/K/G/5/> ;
    rdfs:label "English Language Arts Standards - Anchor Standards - College and Career Readiness Anchor Standards for Language - 5"^^xsd:string ;
    rdfs:comment "Demonstrate understanding of figurative language, word relationships, and nuances in word meanings."^^xsd:string .

:CCSS.Math.Content.K.G.B.6 rdf:type owl:Class ;
    rdfs:subClassOf :CCSS.Math.Content.K.G.B ;
    prov:wasQuotedFrom <http://www.corestandards.org/Math/Content/K/G/6/> ;
    rdfs:label "English Language Arts Standards - Anchor Standards - College and Career Readiness Anchor Standards for Language - 6"^^xsd:string ;
    rdfs:comment "Acquire and use accurately a range of general academic and domain-specific words and phrases sufficient for reading, writing, speaking, and listening at the college and career readiness level; demonstrate independence in gathering vocabulary knowledge when encountering an unknown term important to comprehension or expression."^^xsd:string .

:CCSS.Math.Content.1 rdf:type owl:Class ;
    rdfs:subClassOf :CCSS.Math.Content ;
    prov:wasQuotedFrom <http://www.corestandards.org/Math/Content/1/> .

:CCSS.Math.Content.1.OA rdf:type owl:Class ;
    rdfs:subClassOf :CCSS.Math.Content.1 ;
    rdfs:label "Geometry"^^xsd:string ;
    prov:wasQuotedFrom <http://www.corestandards.org/Math/Content/1/OA/> .

:CCSS.Math.Content.1.OA.A rdf:type owl:Class ;
    rdfs:subClassOf :CCSS.Math.Content.1.OA ;
    rdfs:label "Operations & Algebraic Thinking"^^xsd:string ;
    prov:wasQuotedFrom <http://www.corestandards.org/Math/Content/1/OA/> .

:CCSS.Math.Content.1.OA.A.1 rdf:type owl:Class ;
    rdfs:subClassOf :CCSS.Math.Content.1.OA.A ;
    prov:wasQuotedFrom <http://www.corestandards.org/Math/Content/1/OA/1/> ;
    rdfs:label "English Language Arts Standards - Anchor Standards - College and Career Readiness Anchor Standards for Language - 1"^^xsd:string ;
    rdfs:comment "Demonstrate command of the conventions of standard English grammar and usage when writing or speaking."^^xsd:string .

:CCSS.Math.Content.1.OA.A.2 rdf:type owl:Class ;
    rdfs:subClassOf :CCSS.Math.Content.1.OA.A ;
    prov:wasQuotedFrom <http://www.corestandards.org/Math/Content/1/OA/2/> ;
    rdfs:label "English Language Arts Standards - Anchor Standards - College and Career Readiness Anchor Standards for Language - 2"^^xsd:string ;
    rdfs:comment "Demonstrate command of the conventions of standard English capitalization, punctuation, and spelling when writing."^^xsd:string .

:CCSS.Math.Content.1.OA.B rdf:type owl:Class ;
    rdfs:subClassOf :CCSS.Math.Content.1.OA ;
    rdfs:label "Operations & Algebraic Thinking"^^xsd:string ;
    prov:wasQuotedFrom <http://www.corestandards.org/Math/Content/1/OA/> .

:CCSS.Math.Content.1.OA.B.3 rdf:type owl:Class ;
    rdfs:subClassOf :CCSS.Math.Content.1.OA.B ;
    prov:wasQuotedFrom <http://www.corestandards.org/Math/Content/1/OA/3/> ;
    rdfs:label "English Language Arts Standards - Anchor Standards - College and Career Readiness Anchor Standards for Language - 3"^^xsd:string ;
    rdfs:comment "Apply knowledge of language to understand how language functions in different contexts, to make effective choices for meaning or style, and to comprehend more fully when reading or listening. "^^xsd:string .

:CCSS.Math.Content.1.OA.B.4 rdf:type owl:Class ;
    rdfs:subClassOf :CCSS.Math.Content.1.OA.B ;
    prov:wasQuotedFrom <http://www.corestandards.org/Math/Content/1/OA/4/> ;
    rdfs:label "English Language Arts Standards - Anchor Standards - College and Career Readiness Anchor Standards for Language - 4"^^xsd:string ;
    rdfs:comment "Determine or clarify the meaning of unknown and multiple-meaning words and phrases by using context clues, analyzing meaningful word parts, and consulting general and specialized reference materials, as appropriate."^^xsd:string .

:CCSS.Math.Content.1.OA.C rdf:type owl:Class ;
    rdfs:subClassOf :CCSS.Math.Content.1.OA ;
    rdfs:label "Operations & Algebraic Thinking"^^xsd:string ;
    prov:wasQuotedFrom <http://www.corestandards.org/Math/Content/1/OA/> .

:CCSS.Math.Content.1.OA.C.5 rdf:type owl:Class ;
    rdfs:subClassOf :CCSS.Math.Content.1.OA.C ;
    prov:wasQuotedFrom <http://www.corestandards.org/Math/Content/1/OA/5/> ;
    rdfs:label "English Language Arts Standards - Anchor Standards - College and Career Readiness Anchor Standards for Language - 5"^^xsd:string ;
    rdfs:comment "Demonstrate understanding of figurative language, word relationships, and nuances in word meanings."^^xsd:string .

:CCSS.Math.Content.1.OA.C.6 rdf:type owl:Class ;
    rdfs:subClassOf :CCSS.Math.Content.1.OA.C ;
    prov:wasQuotedFrom <http://www.corestandards.org/Math/Content/1/OA/6/> ;
    rdfs:label "English Language Arts Standards - Anchor Standards - College and Career Readiness Anchor Standards for Language - 6"^^xsd:string ;
    rdfs:comment "Acquire and use accurately a range of general academic and domain-specific words and phrases sufficient for reading, writing, speaking, and listening at the college and career readiness level; demonstrate independence in gathering vocabulary knowledge when encountering an unknown term important to comprehension or expression."^^xsd:string .

:CCSS.Math.Content.1.OA.D rdf:type owl:Class ;
    rdfs:subClassOf :CCSS.Math.Content.1.OA ;
    rdfs:label "Operations & Algebraic Thinking"^^xsd:string ;
    prov:wasQuotedFrom <http://www.corestandards.org/Math/Content/1/OA/> .

:CCSS.Math.Content.1.OA.D.7 rdf:type owl:Class ;
    rdfs:subClassOf :CCSS.Math.Content.1.OA.D ;
    prov:wasQuotedFrom <http://www.corestandards.org/Math/Content/1/OA/7/> ;
    rdfs:label "English Language Arts Standards - Anchor Standards - College and Career Readiness Anchor Standards for Reading - 7"^^xsd:string ;
    rdfs:comment "Integrate and evaluate content presented in diverse media and formats, including visually and quantitatively, as well as in words.1"^^xsd:string .

:CCSS.Math.Content.1.OA.D.8 rdf:type owl:Class ;
    rdfs:subClassOf :CCSS.Math.Content.1.OA.D ;
    prov:wasQuotedFrom <http://www.corestandards.org/Math/Content/1/OA/8/> ;
    rdfs:label "English Language Arts Standards - Anchor Standards - College and Career Readiness Anchor Standards for Reading - 8"^^xsd:string ;
    rdfs:comment "Delineate and evaluate the argument and specific claims in a text, including the validity of the reasoning as well as the relevance and sufficiency of the evidence."^^xsd:string .

:CCSS.Math.Content.1.NBT rdf:type owl:Class ;
    rdfs:subClassOf :CCSS.Math.Content.1 ;
    rdfs:label "Number & Operations in Base Ten"^^xsd:string ;
    prov:wasQuotedFrom <http://www.corestandards.org/Math/Content/1/NBT/> .

:CCSS.Math.Content.1.NBT.A rdf:type owl:Class ;
    rdfs:subClassOf :CCSS.Math.Content.1.NBT ;
    rdfs:label "Number & Operations in Base Ten"^^xsd:string ;
    prov:wasQuotedFrom <http://www.corestandards.org/Math/Content/1/NBT/> .

:CCSS.Math.Content.1.NBT.A.1 rdf:type owl:Class ;
    rdfs:subClassOf :CCSS.Math.Content.1.NBT.A ;
    prov:wasQuotedFrom <http://www.corestandards.org/Math/Content/1/NBT/1/> ;
    rdfs:label "English Language Arts Standards - Anchor Standards - College and Career Readiness Anchor Standards for Language - 1"^^xsd:string ;
    rdfs:comment "Demonstrate command of the conventions of standard English grammar and usage when writing or speaking."^^xsd:string .

:CCSS.Math.Content.1.NBT.B rdf:type owl:Class ;
    rdfs:subClassOf :CCSS.Math.Content.1.NBT ;
    rdfs:label "Number & Operations in Base Ten"^^xsd:string ;
    prov:wasQuotedFrom <http://www.corestandards.org/Math/Content/1/NBT/> .

:CCSS.Math.Content.1.NBT.B.2 rdf:type owl:Class ;
    rdfs:subClassOf :CCSS.Math.Content.1.NBT.B ;
    prov:wasQuotedFrom <http://www.corestandards.org/Math/Content/1/NBT/2/> ;
    rdfs:label "English Language Arts Standards - Anchor Standards - College and Career Readiness Anchor Standards for Language - 2"^^xsd:string ;
    rdfs:comment "Demonstrate command of the conventions of standard English capitalization, punctuation, and spelling when writing."^^xsd:string .

:CCSS.Math.Content.1.NBT.B.3 rdf:type owl:Class ;
    rdfs:subClassOf :CCSS.Math.Content.1.NBT.B ;
    prov:wasQuotedFrom <http://www.corestandards.org/Math/Content/1/NBT/3/> ;
    rdfs:label "English Language Arts Standards - Anchor Standards - College and Career Readiness Anchor Standards for Language - 3"^^xsd:string ;
    rdfs:comment "Apply knowledge of language to understand how language functions in different contexts, to make effective choices for meaning or style, and to comprehend more fully when reading or listening. "^^xsd:string .

:CCSS.Math.Content.1.NBT.C rdf:type owl:Class ;
    rdfs:subClassOf :CCSS.Math.Content.1.NBT ;
    rdfs:label "Number & Operations in Base Ten"^^xsd:string ;
    prov:wasQuotedFrom <http://www.corestandards.org/Math/Content/1/NBT/> .

:CCSS.Math.Content.1.NBT.C.4 rdf:type owl:Class ;
    rdfs:subClassOf :CCSS.Math.Content.1.NBT.C ;
    prov:wasQuotedFrom <http://www.corestandards.org/Math/Content/1/NBT/4/> ;
    rdfs:label "English Language Arts Standards - Anchor Standards - College and Career Readiness Anchor Standards for Language - 4"^^xsd:string ;
    rdfs:comment "Determine or clarify the meaning of unknown and multiple-meaning words and phrases by using context clues, analyzing meaningful word parts, and consulting general and specialized reference materials, as appropriate."^^xsd:string .

:CCSS.Math.Content.1.NBT.C.5 rdf:type owl:Class ;
    rdfs:subClassOf :CCSS.Math.Content.1.NBT.C ;
    prov:wasQuotedFrom <http://www.corestandards.org/Math/Content/1/NBT/5/> ;
    rdfs:label "English Language Arts Standards - Anchor Standards - College and Career Readiness Anchor Standards for Language - 5"^^xsd:string ;
    rdfs:comment "Demonstrate understanding of figurative language, word relationships, and nuances in word meanings."^^xsd:string .

:CCSS.Math.Content.1.NBT.C.6 rdf:type owl:Class ;
    rdfs:subClassOf :CCSS.Math.Content.1.NBT.C ;
    prov:wasQuotedFrom <http://www.corestandards.org/Math/Content/1/NBT/6/> ;
    rdfs:label "English Language Arts Standards - Anchor Standards - College and Career Readiness Anchor Standards for Language - 6"^^xsd:string ;
    rdfs:comment "Acquire and use accurately a range of general academic and domain-specific words and phrases sufficient for reading, writing, speaking, and listening at the college and career readiness level; demonstrate independence in gathering vocabulary knowledge when encountering an unknown term important to comprehension or expression."^^xsd:string .

:CCSS.Math.Content.1.NBT.B.2.a rdf:type owl:Class ;
    rdfs:subClassOf :CCSS.Math.Content.1.NBT.B.2 ;
    prov:wasQuotedFrom <http://www.corestandards.org/Math/Content/1/NBT/a/> .

:CCSS.Math.Content.1.NBT.B.2.b rdf:type owl:Class ;
    rdfs:subClassOf :CCSS.Math.Content.1.NBT.B.2 ;
    prov:wasQuotedFrom <http://www.corestandards.org/Math/Content/1/NBT/b/> .

:CCSS.Math.Content.1.NBT.B.2.c rdf:type owl:Class ;
    rdfs:subClassOf :CCSS.Math.Content.1.NBT.B.2 ;
    prov:wasQuotedFrom <http://www.corestandards.org/Math/Content/1/NBT/c/> .

:CCSS.Math.Content.1.MD rdf:type owl:Class ;
    rdfs:subClassOf :CCSS.Math.Content.1 ;
    rdfs:label "Measurement & Data"^^xsd:string ;
    prov:wasQuotedFrom <http://www.corestandards.org/Math/Content/1/MD/> .

:CCSS.Math.Content.1.MD.A rdf:type owl:Class ;
    rdfs:subClassOf :CCSS.Math.Content.1.MD ;
    rdfs:label "Measurement & Data"^^xsd:string ;
    prov:wasQuotedFrom <http://www.corestandards.org/Math/Content/1/MD/> .

:CCSS.Math.Content.1.MD.A.1 rdf:type owl:Class ;
    rdfs:subClassOf :CCSS.Math.Content.1.MD.A ;
    prov:wasQuotedFrom <http://www.corestandards.org/Math/Content/1/MD/1/> ;
    rdfs:label "English Language Arts Standards - Anchor Standards - College and Career Readiness Anchor Standards for Language - 1"^^xsd:string ;
    rdfs:comment "Demonstrate command of the conventions of standard English grammar and usage when writing or speaking."^^xsd:string .

:CCSS.Math.Content.1.MD.A.2 rdf:type owl:Class ;
    rdfs:subClassOf :CCSS.Math.Content.1.MD.A ;
    prov:wasQuotedFrom <http://www.corestandards.org/Math/Content/1/MD/2/> ;
    rdfs:label "English Language Arts Standards - Anchor Standards - College and Career Readiness Anchor Standards for Language - 2"^^xsd:string ;
    rdfs:comment "Demonstrate command of the conventions of standard English capitalization, punctuation, and spelling when writing."^^xsd:string .

:CCSS.Math.Content.1.MD.B rdf:type owl:Class ;
    rdfs:subClassOf :CCSS.Math.Content.1.MD ;
    rdfs:label "Measurement & Data"^^xsd:string ;
    prov:wasQuotedFrom <http://www.corestandards.org/Math/Content/1/MD/> .

:CCSS.Math.Content.1.MD.B.3 rdf:type owl:Class ;
    rdfs:subClassOf :CCSS.Math.Content.1.MD.B ;
    prov:wasQuotedFrom <http://www.corestandards.org/Math/Content/1/MD/3/> ;
    rdfs:label "English Language Arts Standards - Anchor Standards - College and Career Readiness Anchor Standards for Language - 3"^^xsd:string ;
    rdfs:comment "Apply knowledge of language to understand how language functions in different contexts, to make effective choices for meaning or style, and to comprehend more fully when reading or listening. "^^xsd:string .

:CCSS.Math.Content.1.MD.C rdf:type owl:Class ;
    rdfs:subClassOf :CCSS.Math.Content.1.MD ;
    rdfs:label "Measurement & Data"^^xsd:string ;
    prov:wasQuotedFrom <http://www.corestandards.org/Math/Content/1/MD/> .

:CCSS.Math.Content.1.MD.C.4 rdf:type owl:Class ;
    rdfs:subClassOf :CCSS.Math.Content.1.MD.C ;
    prov:wasQuotedFrom <http://www.corestandards.org/Math/Content/1/MD/4/> ;
    rdfs:label "English Language Arts Standards - Anchor Standards - College and Career Readiness Anchor Standards for Language - 4"^^xsd:string ;
    rdfs:comment "Determine or clarify the meaning of unknown and multiple-meaning words and phrases by using context clues, analyzing meaningful word parts, and consulting general and specialized reference materials, as appropriate."^^xsd:string .

:CCSS.Math.Content.1.G rdf:type owl:Class ;
    rdfs:subClassOf :CCSS.Math.Content.1 ;
    rdfs:label "Geometry"^^xsd:string ;
    prov:wasQuotedFrom <http://www.corestandards.org/Math/Content/1/G/> .

:CCSS.Math.Content.1.G.A rdf:type owl:Class ;
    rdfs:subClassOf :CCSS.Math.Content.1.G ;
    rdfs:label "Geometry"^^xsd:string ;
    prov:wasQuotedFrom <http://www.corestandards.org/Math/Content/1/G/> .

:CCSS.Math.Content.1.G.A.1 rdf:type owl:Class ;
    rdfs:subClassOf :CCSS.Math.Content.1.G.A ;
    prov:wasQuotedFrom <http://www.corestandards.org/Math/Content/1/G/1/> ;
    rdfs:label "English Language Arts Standards - Anchor Standards - College and Career Readiness Anchor Standards for Language - 1"^^xsd:string ;
    rdfs:comment "Demonstrate command of the conventions of standard English grammar and usage when writing or speaking."^^xsd:string .

:CCSS.Math.Content.1.G.A.2 rdf:type owl:Class ;
    rdfs:subClassOf :CCSS.Math.Content.1.G.A ;
    prov:wasQuotedFrom <http://www.corestandards.org/Math/Content/1/G/2/> ;
    rdfs:label "English Language Arts Standards - Anchor Standards - College and Career Readiness Anchor Standards for Language - 2"^^xsd:string ;
    rdfs:comment "Demonstrate command of the conventions of standard English capitalization, punctuation, and spelling when writing."^^xsd:string .

:CCSS.Math.Content.1.G.A.3 rdf:type owl:Class ;
    rdfs:subClassOf :CCSS.Math.Content.1.G.A ;
    prov:wasQuotedFrom <http://www.corestandards.org/Math/Content/1/G/3/> ;
    rdfs:label "English Language Arts Standards - Anchor Standards - College and Career Readiness Anchor Standards for Language - 3"^^xsd:string ;
    rdfs:comment "Apply knowledge of language to understand how language functions in different contexts, to make effective choices for meaning or style, and to comprehend more fully when reading or listening. "^^xsd:string .

:CCSS.Math.Content.2 rdf:type owl:Class ;
    rdfs:subClassOf :CCSS.Math.Content ;
    prov:wasQuotedFrom <http://www.corestandards.org/Math/Content/2/> .

:CCSS.Math.Content.2.OA rdf:type owl:Class ;
    rdfs:subClassOf :CCSS.Math.Content.2 ;
    rdfs:label "Operations & Algebraic Thinking"^^xsd:string ;
    prov:wasQuotedFrom <http://www.corestandards.org/Math/Content/2/OA/> .

:CCSS.Math.Content.2.OA.A rdf:type owl:Class ;
    rdfs:subClassOf :CCSS.Math.Content.2.OA ;
    rdfs:label "Operations & Algebraic Thinking"^^xsd:string ;
    prov:wasQuotedFrom <http://www.corestandards.org/Math/Content/2/OA/> .

:CCSS.Math.Content.2.OA.A.1 rdf:type owl:Class ;
    rdfs:subClassOf :CCSS.Math.Content.2.OA.A ;
    prov:wasQuotedFrom <http://www.corestandards.org/Math/Content/2/OA/1/> ;
    rdfs:label "English Language Arts Standards - Anchor Standards - College and Career Readiness Anchor Standards for Language - 1"^^xsd:string ;
    rdfs:comment "Demonstrate command of the conventions of standard English grammar and usage when writing or speaking."^^xsd:string .

:CCSS.Math.Content.2.OA.B rdf:type owl:Class ;
    rdfs:subClassOf :CCSS.Math.Content.2.OA ;
    rdfs:label "Operations & Algebraic Thinking"^^xsd:string ;
    prov:wasQuotedFrom <http://www.corestandards.org/Math/Content/2/OA/> .

:CCSS.Math.Content.2.OA.B.2 rdf:type owl:Class ;
    rdfs:subClassOf :CCSS.Math.Content.2.OA.B ;
    prov:wasQuotedFrom <http://www.corestandards.org/Math/Content/2/OA/2/> ;
    rdfs:label "English Language Arts Standards - Anchor Standards - College and Career Readiness Anchor Standards for Language - 2"^^xsd:string ;
    rdfs:comment "Demonstrate command of the conventions of standard English capitalization, punctuation, and spelling when writing."^^xsd:string .

:CCSS.Math.Content.2.OA.C rdf:type owl:Class ;
    rdfs:subClassOf :CCSS.Math.Content.2.OA ;
    rdfs:label "Operations & Algebraic Thinking"^^xsd:string ;
    prov:wasQuotedFrom <http://www.corestandards.org/Math/Content/2/OA/> .

:CCSS.Math.Content.2.OA.C.3 rdf:type owl:Class ;
    rdfs:subClassOf :CCSS.Math.Content.2.OA.C ;
    prov:wasQuotedFrom <http://www.corestandards.org/Math/Content/2/OA/3/> ;
    rdfs:label "English Language Arts Standards - Anchor Standards - College and Career Readiness Anchor Standards for Language - 3"^^xsd:string ;
    rdfs:comment "Apply knowledge of language to understand how language functions in different contexts, to make effective choices for meaning or style, and to comprehend more fully when reading or listening. "^^xsd:string .

:CCSS.Math.Content.2.OA.C.4 rdf:type owl:Class ;
    rdfs:subClassOf :CCSS.Math.Content.2.OA.C ;
    prov:wasQuotedFrom <http://www.corestandards.org/Math/Content/2/OA/4/> ;
    rdfs:label "English Language Arts Standards - Anchor Standards - College and Career Readiness Anchor Standards for Language - 4"^^xsd:string ;
    rdfs:comment "Determine or clarify the meaning of unknown and multiple-meaning words and phrases by using context clues, analyzing meaningful word parts, and consulting general and specialized reference materials, as appropriate."^^xsd:string .

:CCSS.Math.Content.2.NBT rdf:type owl:Class ;
    rdfs:subClassOf :CCSS.Math.Content.2 ;
    rdfs:label "Number & Operations in Base Ten"^^xsd:string ;
    prov:wasQuotedFrom <http://www.corestandards.org/Math/Content/2/NBT/> .

:CCSS.Math.Content.2.NBT.A rdf:type owl:Class ;
    rdfs:subClassOf :CCSS.Math.Content.2.NBT ;
    rdfs:label "Number & Operations in Base Ten"^^xsd:string ;
    prov:wasQuotedFrom <http://www.corestandards.org/Math/Content/2/NBT/> .

:CCSS.Math.Content.2.NBT.A.1 rdf:type owl:Class ;
    rdfs:subClassOf :CCSS.Math.Content.2.NBT.A ;
    prov:wasQuotedFrom <http://www.corestandards.org/Math/Content/2/NBT/1/> ;
    rdfs:label "English Language Arts Standards - Anchor Standards - College and Career Readiness Anchor Standards for Language - 1"^^xsd:string ;
    rdfs:comment "Demonstrate command of the conventions of standard English grammar and usage when writing or speaking."^^xsd:string .

:CCSS.Math.Content.2.NBT.A.2 rdf:type owl:Class ;
    rdfs:subClassOf :CCSS.Math.Content.2.NBT.A ;
    prov:wasQuotedFrom <http://www.corestandards.org/Math/Content/2/NBT/2/> ;
    rdfs:label "English Language Arts Standards - Anchor Standards - College and Career Readiness Anchor Standards for Language - 2"^^xsd:string ;
    rdfs:comment "Demonstrate command of the conventions of standard English capitalization, punctuation, and spelling when writing."^^xsd:string .

:CCSS.Math.Content.2.NBT.A.3 rdf:type owl:Class ;
    rdfs:subClassOf :CCSS.Math.Content.2.NBT.A ;
    prov:wasQuotedFrom <http://www.corestandards.org/Math/Content/2/NBT/3/> ;
    rdfs:label "English Language Arts Standards - Anchor Standards - College and Career Readiness Anchor Standards for Language - 3"^^xsd:string ;
    rdfs:comment "Apply knowledge of language to understand how language functions in different contexts, to make effective choices for meaning or style, and to comprehend more fully when reading or listening. "^^xsd:string .

:CCSS.Math.Content.2.NBT.A.4 rdf:type owl:Class ;
    rdfs:subClassOf :CCSS.Math.Content.2.NBT.A ;
    prov:wasQuotedFrom <http://www.corestandards.org/Math/Content/2/NBT/4/> ;
    rdfs:label "English Language Arts Standards - Anchor Standards - College and Career Readiness Anchor Standards for Language - 4"^^xsd:string ;
    rdfs:comment "Determine or clarify the meaning of unknown and multiple-meaning words and phrases by using context clues, analyzing meaningful word parts, and consulting general and specialized reference materials, as appropriate."^^xsd:string .

:CCSS.Math.Content.2.NBT.B rdf:type owl:Class ;
    rdfs:subClassOf :CCSS.Math.Content.2.NBT ;
    rdfs:label "Number & Operations in Base Ten"^^xsd:string ;
    prov:wasQuotedFrom <http://www.corestandards.org/Math/Content/2/NBT/> .

:CCSS.Math.Content.2.NBT.B.5 rdf:type owl:Class ;
    rdfs:subClassOf :CCSS.Math.Content.2.NBT.B ;
    prov:wasQuotedFrom <http://www.corestandards.org/Math/Content/2/NBT/5/> ;
    rdfs:label "English Language Arts Standards - Anchor Standards - College and Career Readiness Anchor Standards for Language - 5"^^xsd:string ;
    rdfs:comment "Demonstrate understanding of figurative language, word relationships, and nuances in word meanings."^^xsd:string .

:CCSS.Math.Content.2.NBT.B.6 rdf:type owl:Class ;
    rdfs:subClassOf :CCSS.Math.Content.2.NBT.B ;
    prov:wasQuotedFrom <http://www.corestandards.org/Math/Content/2/NBT/6/> ;
    rdfs:label "English Language Arts Standards - Anchor Standards - College and Career Readiness Anchor Standards for Language - 6"^^xsd:string ;
    rdfs:comment "Acquire and use accurately a range of general academic and domain-specific words and phrases sufficient for reading, writing, speaking, and listening at the college and career readiness level; demonstrate independence in gathering vocabulary knowledge when encountering an unknown term important to comprehension or expression."^^xsd:string .

:CCSS.Math.Content.2.NBT.B.7 rdf:type owl:Class ;
    rdfs:subClassOf :CCSS.Math.Content.2.NBT.B ;
    prov:wasQuotedFrom <http://www.corestandards.org/Math/Content/2/NBT/7/> ;
    rdfs:label "English Language Arts Standards - Anchor Standards - College and Career Readiness Anchor Standards for Reading - 7"^^xsd:string ;
    rdfs:comment "Integrate and evaluate content presented in diverse media and formats, including visually and quantitatively, as well as in words.1"^^xsd:string .

:CCSS.Math.Content.2.NBT.B.8 rdf:type owl:Class ;
    rdfs:subClassOf :CCSS.Math.Content.2.NBT.B ;
    prov:wasQuotedFrom <http://www.corestandards.org/Math/Content/2/NBT/8/> ;
    rdfs:label "English Language Arts Standards - Anchor Standards - College and Career Readiness Anchor Standards for Reading - 8"^^xsd:string ;
    rdfs:comment "Delineate and evaluate the argument and specific claims in a text, including the validity of the reasoning as well as the relevance and sufficiency of the evidence."^^xsd:string .

:CCSS.Math.Content.2.NBT.B.9 rdf:type owl:Class ;
    rdfs:subClassOf :CCSS.Math.Content.2.NBT.B ;
    prov:wasQuotedFrom <http://www.corestandards.org/Math/Content/2/NBT/9/> ;
    rdfs:label "English Language Arts Standards - Anchor Standards - College and Career Readiness Anchor Standards for Reading - 9"^^xsd:string ;
    rdfs:comment "Analyze how two or more texts address similar themes or topics in order to build knowledge or to compare the approaches the authors take."^^xsd:string .

:CCSS.Math.Content.2.NBT.A.1.a rdf:type owl:Class ;
    rdfs:subClassOf :CCSS.Math.Content.2.NBT.A.1 ;
    prov:wasQuotedFrom <http://www.corestandards.org/Math/Content/2/NBT/a/> .

:CCSS.Math.Content.2.NBT.A.1.b rdf:type owl:Class ;
    rdfs:subClassOf :CCSS.Math.Content.2.NBT.A.1 ;
    prov:wasQuotedFrom <http://www.corestandards.org/Math/Content/2/NBT/b/> .

:CCSS.Math.Content.2.MD rdf:type owl:Class ;
    rdfs:subClassOf :CCSS.Math.Content.2 ;
    rdfs:label "Measurement & Data"^^xsd:string ;
    prov:wasQuotedFrom <http://www.corestandards.org/Math/Content/2/MD/> .

:CCSS.Math.Content.2.MD.A rdf:type owl:Class ;
    rdfs:subClassOf :CCSS.Math.Content.2.MD ;
    rdfs:label "Measurement & Data"^^xsd:string ;
    prov:wasQuotedFrom <http://www.corestandards.org/Math/Content/2/MD/> .

:CCSS.Math.Content.2.MD.A.1 rdf:type owl:Class ;
    rdfs:subClassOf :CCSS.Math.Content.2.MD.A ;
    prov:wasQuotedFrom <http://www.corestandards.org/Math/Content/2/MD/1/> ;
    rdfs:label "English Language Arts Standards - Anchor Standards - College and Career Readiness Anchor Standards for Language - 1"^^xsd:string ;
    rdfs:comment "Demonstrate command of the conventions of standard English grammar and usage when writing or speaking."^^xsd:string .

:CCSS.Math.Content.2.MD.A.2 rdf:type owl:Class ;
    rdfs:subClassOf :CCSS.Math.Content.2.MD.A ;
    prov:wasQuotedFrom <http://www.corestandards.org/Math/Content/2/MD/2/> ;
    rdfs:label "English Language Arts Standards - Anchor Standards - College and Career Readiness Anchor Standards for Language - 2"^^xsd:string ;
    rdfs:comment "Demonstrate command of the conventions of standard English capitalization, punctuation, and spelling when writing."^^xsd:string .

:CCSS.Math.Content.2.MD.A.3 rdf:type owl:Class ;
    rdfs:subClassOf :CCSS.Math.Content.2.MD.A ;
    prov:wasQuotedFrom <http://www.corestandards.org/Math/Content/2/MD/3/> ;
    rdfs:label "English Language Arts Standards - Anchor Standards - College and Career Readiness Anchor Standards for Language - 3"^^xsd:string ;
    rdfs:comment "Apply knowledge of language to understand how language functions in different contexts, to make effective choices for meaning or style, and to comprehend more fully when reading or listening. "^^xsd:string .

:CCSS.Math.Content.2.MD.A.4 rdf:type owl:Class ;
    rdfs:subClassOf :CCSS.Math.Content.2.MD.A ;
    prov:wasQuotedFrom <http://www.corestandards.org/Math/Content/2/MD/4/> ;
    rdfs:label "English Language Arts Standards - Anchor Standards - College and Career Readiness Anchor Standards for Language - 4"^^xsd:string ;
    rdfs:comment "Determine or clarify the meaning of unknown and multiple-meaning words and phrases by using context clues, analyzing meaningful word parts, and consulting general and specialized reference materials, as appropriate."^^xsd:string .

:CCSS.Math.Content.2.MD.B rdf:type owl:Class ;
    rdfs:subClassOf :CCSS.Math.Content.2.MD ;
    rdfs:label "Measurement & Data"^^xsd:string ;
    prov:wasQuotedFrom <http://www.corestandards.org/Math/Content/2/MD/> .

:CCSS.Math.Content.2.MD.B.5 rdf:type owl:Class ;
    rdfs:subClassOf :CCSS.Math.Content.2.MD.B ;
    prov:wasQuotedFrom <http://www.corestandards.org/Math/Content/2/MD/5/> ;
    rdfs:label "English Language Arts Standards - Anchor Standards - College and Career Readiness Anchor Standards for Language - 5"^^xsd:string ;
    rdfs:comment "Demonstrate understanding of figurative language, word relationships, and nuances in word meanings."^^xsd:string .

:CCSS.Math.Content.2.MD.B.6 rdf:type owl:Class ;
    rdfs:subClassOf :CCSS.Math.Content.2.MD.B ;
    prov:wasQuotedFrom <http://www.corestandards.org/Math/Content/2/MD/6/> ;
    rdfs:label "English Language Arts Standards - Anchor Standards - College and Career Readiness Anchor Standards for Language - 6"^^xsd:string ;
    rdfs:comment "Acquire and use accurately a range of general academic and domain-specific words and phrases sufficient for reading, writing, speaking, and listening at the college and career readiness level; demonstrate independence in gathering vocabulary knowledge when encountering an unknown term important to comprehension or expression."^^xsd:string .

:CCSS.Math.Content.2.MD.C rdf:type owl:Class ;
    rdfs:subClassOf :CCSS.Math.Content.2.MD ;
    rdfs:label "Measurement & Data"^^xsd:string ;
    prov:wasQuotedFrom <http://www.corestandards.org/Math/Content/2/MD/> .

:CCSS.Math.Content.2.MD.C.7 rdf:type owl:Class ;
    rdfs:subClassOf :CCSS.Math.Content.2.MD.C ;
    prov:wasQuotedFrom <http://www.corestandards.org/Math/Content/2/MD/7/> ;
    rdfs:label "English Language Arts Standards - Anchor Standards - College and Career Readiness Anchor Standards for Reading - 7"^^xsd:string ;
    rdfs:comment "Integrate and evaluate content presented in diverse media and formats, including visually and quantitatively, as well as in words.1"^^xsd:string .

:CCSS.Math.Content.2.MD.C.8 rdf:type owl:Class ;
    rdfs:subClassOf :CCSS.Math.Content.2.MD.C ;
    prov:wasQuotedFrom <http://www.corestandards.org/Math/Content/2/MD/8/> ;
    rdfs:label "English Language Arts Standards - Anchor Standards - College and Career Readiness Anchor Standards for Reading - 8"^^xsd:string ;
    rdfs:comment "Delineate and evaluate the argument and specific claims in a text, including the validity of the reasoning as well as the relevance and sufficiency of the evidence."^^xsd:string .

:CCSS.Math.Content.2.MD.D rdf:type owl:Class ;
    rdfs:subClassOf :CCSS.Math.Content.2.MD ;
    rdfs:label "Measurement & Data"^^xsd:string ;
    prov:wasQuotedFrom <http://www.corestandards.org/Math/Content/2/MD/> .

:CCSS.Math.Content.2.MD.D.9 rdf:type owl:Class ;
    rdfs:subClassOf :CCSS.Math.Content.2.MD.D ;
    prov:wasQuotedFrom <http://www.corestandards.org/Math/Content/2/MD/9/> ;
    rdfs:label "English Language Arts Standards - Anchor Standards - College and Career Readiness Anchor Standards for Reading - 9"^^xsd:string ;
    rdfs:comment "Analyze how two or more texts address similar themes or topics in order to build knowledge or to compare the approaches the authors take."^^xsd:string .

:CCSS.Math.Content.2.MD.D.10 rdf:type owl:Class ;
    rdfs:subClassOf :CCSS.Math.Content.2.MD.D ;
    prov:wasQuotedFrom <http://www.corestandards.org/Math/Content/2/MD/10/> ;
    rdfs:label "English Language Arts Standards - Anchor Standards - College and Career Readiness Anchor Standards for Reading - 10"^^xsd:string ;
    rdfs:comment "Read and comprehend complex literary and informational texts independently and proficiently."^^xsd:string .

:CCSS.Math.Content.2.G rdf:type owl:Class ;
    rdfs:subClassOf :CCSS.Math.Content.2 ;
    rdfs:label "Geometry"^^xsd:string ;
    prov:wasQuotedFrom <http://www.corestandards.org/Math/Content/2/G/> .

:CCSS.Math.Content.2.G.A rdf:type owl:Class ;
    rdfs:subClassOf :CCSS.Math.Content.2.G ;
    rdfs:label "Geometry"^^xsd:string ;
    prov:wasQuotedFrom <http://www.corestandards.org/Math/Content/2/G/> .

:CCSS.Math.Content.2.G.A.1 rdf:type owl:Class ;
    rdfs:subClassOf :CCSS.Math.Content.2.G.A ;
    prov:wasQuotedFrom <http://www.corestandards.org/Math/Content/2/G/1/> ;
    rdfs:label "English Language Arts Standards - Anchor Standards - College and Career Readiness Anchor Standards for Language - 1"^^xsd:string ;
    rdfs:comment "Demonstrate command of the conventions of standard English grammar and usage when writing or speaking."^^xsd:string .

:CCSS.Math.Content.2.G.A.2 rdf:type owl:Class ;
    rdfs:subClassOf :CCSS.Math.Content.2.G.A ;
    prov:wasQuotedFrom <http://www.corestandards.org/Math/Content/2/G/2/> ;
    rdfs:label "English Language Arts Standards - Anchor Standards - College and Career Readiness Anchor Standards for Language - 2"^^xsd:string ;
    rdfs:comment "Demonstrate command of the conventions of standard English capitalization, punctuation, and spelling when writing."^^xsd:string .

:CCSS.Math.Content.2.G.A.3 rdf:type owl:Class ;
    rdfs:subClassOf :CCSS.Math.Content.2.G.A ;
    prov:wasQuotedFrom <http://www.corestandards.org/Math/Content/2/G/3/> ;
    rdfs:label "English Language Arts Standards - Anchor Standards - College and Career Readiness Anchor Standards for Language - 3"^^xsd:string ;
    rdfs:comment "Apply knowledge of language to understand how language functions in different contexts, to make effective choices for meaning or style, and to comprehend more fully when reading or listening. "^^xsd:string .

:CCSS.Math.Content.3 rdf:type owl:Class ;
    rdfs:subClassOf :CCSS.Math.Content ;
    prov:wasQuotedFrom <http://www.corestandards.org/Math/Content/3/> .

:CCSS.Math.Content.3.OA rdf:type owl:Class ;
    rdfs:subClassOf :CCSS.Math.Content.3 ;
    rdfs:label "Operations & Algebraic Thinking"^^xsd:string ;
    prov:wasQuotedFrom <http://www.corestandards.org/Math/Content/3/OA/> .

:CCSS.Math.Content.3.OA.A rdf:type owl:Class ;
    rdfs:subClassOf :CCSS.Math.Content.3.OA ;
    rdfs:label "Operations & Algebraic Thinking"^^xsd:string ;
    prov:wasQuotedFrom <http://www.corestandards.org/Math/Content/3/OA/> .

:CCSS.Math.Content.3.OA.A.1 rdf:type owl:Class ;
    rdfs:subClassOf :CCSS.Math.Content.3.OA.A ;
    prov:wasQuotedFrom <http://www.corestandards.org/Math/Content/3/OA/1/> ;
    rdfs:label "English Language Arts Standards - Anchor Standards - College and Career Readiness Anchor Standards for Language - 1"^^xsd:string ;
    rdfs:comment "Demonstrate command of the conventions of standard English grammar and usage when writing or speaking."^^xsd:string .

:CCSS.Math.Content.3.OA.A.2 rdf:type owl:Class ;
    rdfs:subClassOf :CCSS.Math.Content.3.OA.A ;
    prov:wasQuotedFrom <http://www.corestandards.org/Math/Content/3/OA/2/> ;
    rdfs:label "English Language Arts Standards - Anchor Standards - College and Career Readiness Anchor Standards for Language - 2"^^xsd:string ;
    rdfs:comment "Demonstrate command of the conventions of standard English capitalization, punctuation, and spelling when writing."^^xsd:string .

:CCSS.Math.Content.3.OA.A.3 rdf:type owl:Class ;
    rdfs:subClassOf :CCSS.Math.Content.3.OA.A ;
    prov:wasQuotedFrom <http://www.corestandards.org/Math/Content/3/OA/3/> ;
    rdfs:label "English Language Arts Standards - Anchor Standards - College and Career Readiness Anchor Standards for Language - 3"^^xsd:string ;
    rdfs:comment "Apply knowledge of language to understand how language functions in different contexts, to make effective choices for meaning or style, and to comprehend more fully when reading or listening. "^^xsd:string .

:CCSS.Math.Content.3.OA.A.4 rdf:type owl:Class ;
    rdfs:subClassOf :CCSS.Math.Content.3.OA.A ;
    prov:wasQuotedFrom <http://www.corestandards.org/Math/Content/3/OA/4/> ;
    rdfs:label "English Language Arts Standards - Anchor Standards - College and Career Readiness Anchor Standards for Language - 4"^^xsd:string ;
    rdfs:comment "Determine or clarify the meaning of unknown and multiple-meaning words and phrases by using context clues, analyzing meaningful word parts, and consulting general and specialized reference materials, as appropriate."^^xsd:string .

:CCSS.Math.Content.3.OA.B rdf:type owl:Class ;
    rdfs:subClassOf :CCSS.Math.Content.3.OA ;
    rdfs:label "Operations & Algebraic Thinking"^^xsd:string ;
    prov:wasQuotedFrom <http://www.corestandards.org/Math/Content/3/OA/> .

:CCSS.Math.Content.3.OA.B.5 rdf:type owl:Class ;
    rdfs:subClassOf :CCSS.Math.Content.3.OA.B ;
    prov:wasQuotedFrom <http://www.corestandards.org/Math/Content/3/OA/5/> ;
    rdfs:label "English Language Arts Standards - Anchor Standards - College and Career Readiness Anchor Standards for Language - 5"^^xsd:string ;
    rdfs:comment "Demonstrate understanding of figurative language, word relationships, and nuances in word meanings."^^xsd:string .

:CCSS.Math.Content.3.OA.B.6 rdf:type owl:Class ;
    rdfs:subClassOf :CCSS.Math.Content.3.OA.B ;
    prov:wasQuotedFrom <http://www.corestandards.org/Math/Content/3/OA/6/> ;
    rdfs:label "English Language Arts Standards - Anchor Standards - College and Career Readiness Anchor Standards for Language - 6"^^xsd:string ;
    rdfs:comment "Acquire and use accurately a range of general academic and domain-specific words and phrases sufficient for reading, writing, speaking, and listening at the college and career readiness level; demonstrate independence in gathering vocabulary knowledge when encountering an unknown term important to comprehension or expression."^^xsd:string .

:CCSS.Math.Content.3.OA.C rdf:type owl:Class ;
    rdfs:subClassOf :CCSS.Math.Content.3.OA ;
    rdfs:label "Operations & Algebraic Thinking"^^xsd:string ;
    prov:wasQuotedFrom <http://www.corestandards.org/Math/Content/3/OA/> .

:CCSS.Math.Content.3.OA.C.7 rdf:type owl:Class ;
    rdfs:subClassOf :CCSS.Math.Content.3.OA.C ;
    prov:wasQuotedFrom <http://www.corestandards.org/Math/Content/3/OA/7/> ;
    rdfs:label "English Language Arts Standards - Anchor Standards - College and Career Readiness Anchor Standards for Reading - 7"^^xsd:string ;
    rdfs:comment "Integrate and evaluate content presented in diverse media and formats, including visually and quantitatively, as well as in words.1"^^xsd:string .

:CCSS.Math.Content.3.OA.D rdf:type owl:Class ;
    rdfs:subClassOf :CCSS.Math.Content.3.OA ;
    rdfs:label "Operations & Algebraic Thinking"^^xsd:string ;
    prov:wasQuotedFrom <http://www.corestandards.org/Math/Content/3/OA/> .

:CCSS.Math.Content.3.OA.D.8 rdf:type owl:Class ;
    rdfs:subClassOf :CCSS.Math.Content.3.OA.D ;
    prov:wasQuotedFrom <http://www.corestandards.org/Math/Content/3/OA/8/> ;
    rdfs:label "English Language Arts Standards - Anchor Standards - College and Career Readiness Anchor Standards for Reading - 8"^^xsd:string ;
    rdfs:comment "Delineate and evaluate the argument and specific claims in a text, including the validity of the reasoning as well as the relevance and sufficiency of the evidence."^^xsd:string .

:CCSS.Math.Content.3.OA.D.9 rdf:type owl:Class ;
    rdfs:subClassOf :CCSS.Math.Content.3.OA.D ;
    prov:wasQuotedFrom <http://www.corestandards.org/Math/Content/3/OA/9/> ;
    rdfs:label "English Language Arts Standards - Anchor Standards - College and Career Readiness Anchor Standards for Reading - 9"^^xsd:string ;
    rdfs:comment "Analyze how two or more texts address similar themes or topics in order to build knowledge or to compare the approaches the authors take."^^xsd:string .

:CCSS.Math.Content.3.NBT rdf:type owl:Class ;
    rdfs:subClassOf :CCSS.Math.Content.3 ;
    rdfs:label "Number & Operations in Base Ten"^^xsd:string ;
    prov:wasQuotedFrom <http://www.corestandards.org/Math/Content/3/NBT/> .

:CCSS.Math.Content.3.NBT.A rdf:type owl:Class ;
    rdfs:subClassOf :CCSS.Math.Content.3.NBT ;
    rdfs:label "Number & Operations in Base Ten"^^xsd:string ;
    prov:wasQuotedFrom <http://www.corestandards.org/Math/Content/3/NBT/> .

:CCSS.Math.Content.3.NBT.A.1 rdf:type owl:Class ;
    rdfs:subClassOf :CCSS.Math.Content.3.NBT.A ;
    prov:wasQuotedFrom <http://www.corestandards.org/Math/Content/3/NBT/1/> ;
    rdfs:label "English Language Arts Standards - Anchor Standards - College and Career Readiness Anchor Standards for Language - 1"^^xsd:string ;
    rdfs:comment "Demonstrate command of the conventions of standard English grammar and usage when writing or speaking."^^xsd:string .

:CCSS.Math.Content.3.NBT.A.2 rdf:type owl:Class ;
    rdfs:subClassOf :CCSS.Math.Content.3.NBT.A ;
    prov:wasQuotedFrom <http://www.corestandards.org/Math/Content/3/NBT/2/> ;
    rdfs:label "English Language Arts Standards - Anchor Standards - College and Career Readiness Anchor Standards for Language - 2"^^xsd:string ;
    rdfs:comment "Demonstrate command of the conventions of standard English capitalization, punctuation, and spelling when writing."^^xsd:string .

:CCSS.Math.Content.3.NBT.A.3 rdf:type owl:Class ;
    rdfs:subClassOf :CCSS.Math.Content.3.NBT.A ;
    prov:wasQuotedFrom <http://www.corestandards.org/Math/Content/3/NBT/3/> ;
    rdfs:label "English Language Arts Standards - Anchor Standards - College and Career Readiness Anchor Standards for Language - 3"^^xsd:string ;
    rdfs:comment "Apply knowledge of language to understand how language functions in different contexts, to make effective choices for meaning or style, and to comprehend more fully when reading or listening. "^^xsd:string .

:CCSS.Math.Content.3.NF rdf:type owl:Class ;
    rdfs:subClassOf :CCSS.Math.Content.3 ;
    rdfs:label "Number & Operations - Fractions"^^xsd:string ;
    prov:wasQuotedFrom <http://www.corestandards.org/Math/Content/3/NF/> .

:CCSS.Math.Content.3.NF.A rdf:type owl:Class ;
    rdfs:subClassOf :CCSS.Math.Content.3.NF ;
    rdfs:label "Number & Operations - Fractions"^^xsd:string ;
    prov:wasQuotedFrom <http://www.corestandards.org/Math/Content/3/NF/> .

:CCSS.Math.Content.3.NF.A.1 rdf:type owl:Class ;
    rdfs:subClassOf :CCSS.Math.Content.3.NF.A ;
    prov:wasQuotedFrom <http://www.corestandards.org/Math/Content/3/NF/1/> ;
    rdfs:label "English Language Arts Standards - Anchor Standards - College and Career Readiness Anchor Standards for Language - 1"^^xsd:string ;
    rdfs:comment "Demonstrate command of the conventions of standard English grammar and usage when writing or speaking."^^xsd:string .

:CCSS.Math.Content.3.NF.A.2 rdf:type owl:Class ;
    rdfs:subClassOf :CCSS.Math.Content.3.NF.A ;
    prov:wasQuotedFrom <http://www.corestandards.org/Math/Content/3/NF/2/> ;
    rdfs:label "English Language Arts Standards - Anchor Standards - College and Career Readiness Anchor Standards for Language - 2"^^xsd:string ;
    rdfs:comment "Demonstrate command of the conventions of standard English capitalization, punctuation, and spelling when writing."^^xsd:string .

:CCSS.Math.Content.3.NF.A.3 rdf:type owl:Class ;
    rdfs:subClassOf :CCSS.Math.Content.3.NF.A ;
    prov:wasQuotedFrom <http://www.corestandards.org/Math/Content/3/NF/3/> ;
    rdfs:label "English Language Arts Standards - Anchor Standards - College and Career Readiness Anchor Standards for Language - 3"^^xsd:string ;
    rdfs:comment "Apply knowledge of language to understand how language functions in different contexts, to make effective choices for meaning or style, and to comprehend more fully when reading or listening. "^^xsd:string .

:CCSS.Math.Content.3.NF.A.2.a rdf:type owl:Class ;
    rdfs:subClassOf :CCSS.Math.Content.3.NF.A.2 ;
    prov:wasQuotedFrom <http://www.corestandards.org/Math/Content/3/NF/a/> .

:CCSS.Math.Content.3.NF.A.2.b rdf:type owl:Class ;
    rdfs:subClassOf :CCSS.Math.Content.3.NF.A.2 ;
    prov:wasQuotedFrom <http://www.corestandards.org/Math/Content/3/NF/b/> .

:CCSS.Math.Content.3.NF.A.3.a rdf:type owl:Class ;
    rdfs:subClassOf :CCSS.Math.Content.3.NF.A.3 ;
    prov:wasQuotedFrom <http://www.corestandards.org/Math/Content/3/NF/a/> .

:CCSS.Math.Content.3.NF.A.3.b rdf:type owl:Class ;
    rdfs:subClassOf :CCSS.Math.Content.3.NF.A.3 ;
    prov:wasQuotedFrom <http://www.corestandards.org/Math/Content/3/NF/b/> .

:CCSS.Math.Content.3.NF.A.3.c rdf:type owl:Class ;
    rdfs:subClassOf :CCSS.Math.Content.3.NF.A.3 ;
    prov:wasQuotedFrom <http://www.corestandards.org/Math/Content/3/NF/c/> .

:CCSS.Math.Content.3.NF.A.3.d rdf:type owl:Class ;
    rdfs:subClassOf :CCSS.Math.Content.3.NF.A.3 ;
    prov:wasQuotedFrom <http://www.corestandards.org/Math/Content/3/NF/d/> .

:CCSS.Math.Content.3.MD rdf:type owl:Class ;
    rdfs:subClassOf :CCSS.Math.Content.3 ;
    rdfs:label "Measurement & Data"^^xsd:string ;
    prov:wasQuotedFrom <http://www.corestandards.org/Math/Content/3/MD/> .

:CCSS.Math.Content.3.MD.A rdf:type owl:Class ;
    rdfs:subClassOf :CCSS.Math.Content.3.MD ;
    rdfs:label "Measurement & Data"^^xsd:string ;
    prov:wasQuotedFrom <http://www.corestandards.org/Math/Content/3/MD/> .

:CCSS.Math.Content.3.MD.A.1 rdf:type owl:Class ;
    rdfs:subClassOf :CCSS.Math.Content.3.MD.A ;
    prov:wasQuotedFrom <http://www.corestandards.org/Math/Content/3/MD/1/> ;
    rdfs:label "English Language Arts Standards - Anchor Standards - College and Career Readiness Anchor Standards for Language - 1"^^xsd:string ;
    rdfs:comment "Demonstrate command of the conventions of standard English grammar and usage when writing or speaking."^^xsd:string .

:CCSS.Math.Content.3.MD.A.2 rdf:type owl:Class ;
    rdfs:subClassOf :CCSS.Math.Content.3.MD.A ;
    prov:wasQuotedFrom <http://www.corestandards.org/Math/Content/3/MD/2/> ;
    rdfs:label "English Language Arts Standards - Anchor Standards - College and Career Readiness Anchor Standards for Language - 2"^^xsd:string ;
    rdfs:comment "Demonstrate command of the conventions of standard English capitalization, punctuation, and spelling when writing."^^xsd:string .

:CCSS.Math.Content.3.MD.B rdf:type owl:Class ;
    rdfs:subClassOf :CCSS.Math.Content.3.MD ;
    rdfs:label "Measurement & Data"^^xsd:string ;
    prov:wasQuotedFrom <http://www.corestandards.org/Math/Content/3/MD/> .

:CCSS.Math.Content.3.MD.B.3 rdf:type owl:Class ;
    rdfs:subClassOf :CCSS.Math.Content.3.MD.B ;
    prov:wasQuotedFrom <http://www.corestandards.org/Math/Content/3/MD/3/> ;
    rdfs:label "English Language Arts Standards - Anchor Standards - College and Career Readiness Anchor Standards for Language - 3"^^xsd:string ;
    rdfs:comment "Apply knowledge of language to understand how language functions in different contexts, to make effective choices for meaning or style, and to comprehend more fully when reading or listening. "^^xsd:string .

:CCSS.Math.Content.3.MD.B.4 rdf:type owl:Class ;
    rdfs:subClassOf :CCSS.Math.Content.3.MD.B ;
    prov:wasQuotedFrom <http://www.corestandards.org/Math/Content/3/MD/4/> ;
    rdfs:label "English Language Arts Standards - Anchor Standards - College and Career Readiness Anchor Standards for Language - 4"^^xsd:string ;
    rdfs:comment "Determine or clarify the meaning of unknown and multiple-meaning words and phrases by using context clues, analyzing meaningful word parts, and consulting general and specialized reference materials, as appropriate."^^xsd:string .

:CCSS.Math.Content.3.MD.C rdf:type owl:Class ;
    rdfs:subClassOf :CCSS.Math.Content.3.MD ;
    rdfs:label "Measurement & Data"^^xsd:string ;
    prov:wasQuotedFrom <http://www.corestandards.org/Math/Content/3/MD/> .

:CCSS.Math.Content.3.MD.C.5 rdf:type owl:Class ;
    rdfs:subClassOf :CCSS.Math.Content.3.MD.C ;
    prov:wasQuotedFrom <http://www.corestandards.org/Math/Content/3/MD/5/> ;
    rdfs:label "English Language Arts Standards - Anchor Standards - College and Career Readiness Anchor Standards for Language - 5"^^xsd:string ;
    rdfs:comment "Demonstrate understanding of figurative language, word relationships, and nuances in word meanings."^^xsd:string .

:CCSS.Math.Content.3.MD.C.6 rdf:type owl:Class ;
    rdfs:subClassOf :CCSS.Math.Content.3.MD.C ;
    prov:wasQuotedFrom <http://www.corestandards.org/Math/Content/3/MD/6/> ;
    rdfs:label "English Language Arts Standards - Anchor Standards - College and Career Readiness Anchor Standards for Language - 6"^^xsd:string ;
    rdfs:comment "Acquire and use accurately a range of general academic and domain-specific words and phrases sufficient for reading, writing, speaking, and listening at the college and career readiness level; demonstrate independence in gathering vocabulary knowledge when encountering an unknown term important to comprehension or expression."^^xsd:string .

:CCSS.Math.Content.3.MD.C.7 rdf:type owl:Class ;
    rdfs:subClassOf :CCSS.Math.Content.3.MD.C ;
    prov:wasQuotedFrom <http://www.corestandards.org/Math/Content/3/MD/7/> ;
    rdfs:label "English Language Arts Standards - Anchor Standards - College and Career Readiness Anchor Standards for Reading - 7"^^xsd:string ;
    rdfs:comment "Integrate and evaluate content presented in diverse media and formats, including visually and quantitatively, as well as in words.1"^^xsd:string .

:CCSS.Math.Content.3.MD.D rdf:type owl:Class ;
    rdfs:subClassOf :CCSS.Math.Content.3.MD ;
    rdfs:label "Measurement & Data"^^xsd:string ;
    prov:wasQuotedFrom <http://www.corestandards.org/Math/Content/3/MD/> .

:CCSS.Math.Content.3.MD.D.8 rdf:type owl:Class ;
    rdfs:subClassOf :CCSS.Math.Content.3.MD.D ;
    prov:wasQuotedFrom <http://www.corestandards.org/Math/Content/3/MD/8/> ;
    rdfs:label "English Language Arts Standards - Anchor Standards - College and Career Readiness Anchor Standards for Reading - 8"^^xsd:string ;
    rdfs:comment "Delineate and evaluate the argument and specific claims in a text, including the validity of the reasoning as well as the relevance and sufficiency of the evidence."^^xsd:string .

:CCSS.Math.Content.3.MD.C.5.a rdf:type owl:Class ;
    rdfs:subClassOf :CCSS.Math.Content.3.MD.C.5 ;
    prov:wasQuotedFrom <http://www.corestandards.org/Math/Content/3/MD/a/> .

:CCSS.Math.Content.3.MD.C.5.b rdf:type owl:Class ;
    rdfs:subClassOf :CCSS.Math.Content.3.MD.C.5 ;
    prov:wasQuotedFrom <http://www.corestandards.org/Math/Content/3/MD/b/> .

:CCSS.Math.Content.3.MD.C.7.a rdf:type owl:Class ;
    rdfs:subClassOf :CCSS.Math.Content.3.MD.C.7 ;
    prov:wasQuotedFrom <http://www.corestandards.org/Math/Content/3/MD/a/> .

:CCSS.Math.Content.3.MD.C.7.b rdf:type owl:Class ;
    rdfs:subClassOf :CCSS.Math.Content.3.MD.C.7 ;
    prov:wasQuotedFrom <http://www.corestandards.org/Math/Content/3/MD/b/> .

:CCSS.Math.Content.3.MD.C.7.c rdf:type owl:Class ;
    rdfs:subClassOf :CCSS.Math.Content.3.MD.C.7 ;
    prov:wasQuotedFrom <http://www.corestandards.org/Math/Content/3/MD/c/> .

:CCSS.Math.Content.3.MD.C.7.d rdf:type owl:Class ;
    rdfs:subClassOf :CCSS.Math.Content.3.MD.C.7 ;
    prov:wasQuotedFrom <http://www.corestandards.org/Math/Content/3/MD/d/> .

:CCSS.Math.Content.3.G rdf:type owl:Class ;
    rdfs:subClassOf :CCSS.Math.Content.3 ;
    rdfs:label "Geometry"^^xsd:string ;
    prov:wasQuotedFrom <http://www.corestandards.org/Math/Content/3/G/> .

:CCSS.Math.Content.3.G.A rdf:type owl:Class ;
    rdfs:subClassOf :CCSS.Math.Content.3.G ;
    rdfs:label "Geometry"^^xsd:string ;
    prov:wasQuotedFrom <http://www.corestandards.org/Math/Content/3/G/> .

:CCSS.Math.Content.3.G.A.1 rdf:type owl:Class ;
    rdfs:subClassOf :CCSS.Math.Content.3.G.A ;
    prov:wasQuotedFrom <http://www.corestandards.org/Math/Content/3/G/1/> ;
    rdfs:label "English Language Arts Standards - Anchor Standards - College and Career Readiness Anchor Standards for Language - 1"^^xsd:string ;
    rdfs:comment "Demonstrate command of the conventions of standard English grammar and usage when writing or speaking."^^xsd:string .

:CCSS.Math.Content.3.G.A.2 rdf:type owl:Class ;
    rdfs:subClassOf :CCSS.Math.Content.3.G.A ;
    prov:wasQuotedFrom <http://www.corestandards.org/Math/Content/3/G/2/> ;
    rdfs:label "English Language Arts Standards - Anchor Standards - College and Career Readiness Anchor Standards for Language - 2"^^xsd:string ;
    rdfs:comment "Demonstrate command of the conventions of standard English capitalization, punctuation, and spelling when writing."^^xsd:string .

:CCSS.Math.Content.4 rdf:type owl:Class ;
    rdfs:subClassOf :CCSS.Math.Content ;
    prov:wasQuotedFrom <http://www.corestandards.org/Math/Content/4/> .

:CCSS.Math.Content.4.OA rdf:type owl:Class ;
    rdfs:subClassOf :CCSS.Math.Content.4 ;
    rdfs:label "Operations & Algebraic Thinking"^^xsd:string ;
    prov:wasQuotedFrom <http://www.corestandards.org/Math/Content/4/OA/> .

:CCSS.Math.Content.4.OA.A rdf:type owl:Class ;
    rdfs:subClassOf :CCSS.Math.Content.4.OA ;
    rdfs:label "Operations & Algebraic Thinking"^^xsd:string ;
    prov:wasQuotedFrom <http://www.corestandards.org/Math/Content/4/OA/> .

:CCSS.Math.Content.4.OA.A.1 rdf:type owl:Class ;
    rdfs:subClassOf :CCSS.Math.Content.4.OA.A ;
    prov:wasQuotedFrom <http://www.corestandards.org/Math/Content/4/OA/1/> ;
    rdfs:label "English Language Arts Standards - Anchor Standards - College and Career Readiness Anchor Standards for Language - 1"^^xsd:string ;
    rdfs:comment "Demonstrate command of the conventions of standard English grammar and usage when writing or speaking."^^xsd:string .

:CCSS.Math.Content.4.OA.A.2 rdf:type owl:Class ;
    rdfs:subClassOf :CCSS.Math.Content.4.OA.A ;
    prov:wasQuotedFrom <http://www.corestandards.org/Math/Content/4/OA/2/> ;
    rdfs:label "English Language Arts Standards - Anchor Standards - College and Career Readiness Anchor Standards for Language - 2"^^xsd:string ;
    rdfs:comment "Demonstrate command of the conventions of standard English capitalization, punctuation, and spelling when writing."^^xsd:string .

:CCSS.Math.Content.4.OA.A.3 rdf:type owl:Class ;
    rdfs:subClassOf :CCSS.Math.Content.4.OA.A ;
    prov:wasQuotedFrom <http://www.corestandards.org/Math/Content/4/OA/3/> ;
    rdfs:label "English Language Arts Standards - Anchor Standards - College and Career Readiness Anchor Standards for Language - 3"^^xsd:string ;
    rdfs:comment "Apply knowledge of language to understand how language functions in different contexts, to make effective choices for meaning or style, and to comprehend more fully when reading or listening. "^^xsd:string .

:CCSS.Math.Content.4.OA.B rdf:type owl:Class ;
    rdfs:subClassOf :CCSS.Math.Content.4.OA ;
    rdfs:label "Operations & Algebraic Thinking"^^xsd:string ;
    prov:wasQuotedFrom <http://www.corestandards.org/Math/Content/4/OA/> .

:CCSS.Math.Content.4.OA.B.4 rdf:type owl:Class ;
    rdfs:subClassOf :CCSS.Math.Content.4.OA.B ;
    prov:wasQuotedFrom <http://www.corestandards.org/Math/Content/4/OA/4/> ;
    rdfs:label "English Language Arts Standards - Anchor Standards - College and Career Readiness Anchor Standards for Language - 4"^^xsd:string ;
    rdfs:comment "Determine or clarify the meaning of unknown and multiple-meaning words and phrases by using context clues, analyzing meaningful word parts, and consulting general and specialized reference materials, as appropriate."^^xsd:string .

:CCSS.Math.Content.4.OA.C rdf:type owl:Class ;
    rdfs:subClassOf :CCSS.Math.Content.4.OA ;
    rdfs:label "Operations & Algebraic Thinking"^^xsd:string ;
    prov:wasQuotedFrom <http://www.corestandards.org/Math/Content/4/OA/> .

:CCSS.Math.Content.4.OA.C.5 rdf:type owl:Class ;
    rdfs:subClassOf :CCSS.Math.Content.4.OA.C ;
    prov:wasQuotedFrom <http://www.corestandards.org/Math/Content/4/OA/5/> ;
    rdfs:label "English Language Arts Standards - Anchor Standards - College and Career Readiness Anchor Standards for Language - 5"^^xsd:string ;
    rdfs:comment "Demonstrate understanding of figurative language, word relationships, and nuances in word meanings."^^xsd:string .

:CCSS.Math.Content.4.NBT rdf:type owl:Class ;
    rdfs:subClassOf :CCSS.Math.Content.4 ;
    rdfs:label "Number & Operations in Base Ten"^^xsd:string ;
    prov:wasQuotedFrom <http://www.corestandards.org/Math/Content/4/NBT/> .

:CCSS.Math.Content.4.NBT.A rdf:type owl:Class ;
    rdfs:subClassOf :CCSS.Math.Content.4.NBT ;
    rdfs:label "Number & Operations in Base Ten"^^xsd:string ;
    prov:wasQuotedFrom <http://www.corestandards.org/Math/Content/4/NBT/> .

:CCSS.Math.Content.4.NBT.A.1 rdf:type owl:Class ;
    rdfs:subClassOf :CCSS.Math.Content.4.NBT.A ;
    prov:wasQuotedFrom <http://www.corestandards.org/Math/Content/4/NBT/1/> ;
    rdfs:label "English Language Arts Standards - Anchor Standards - College and Career Readiness Anchor Standards for Language - 1"^^xsd:string ;
    rdfs:comment "Demonstrate command of the conventions of standard English grammar and usage when writing or speaking."^^xsd:string .

:CCSS.Math.Content.4.NBT.A.2 rdf:type owl:Class ;
    rdfs:subClassOf :CCSS.Math.Content.4.NBT.A ;
    prov:wasQuotedFrom <http://www.corestandards.org/Math/Content/4/NBT/2/> ;
    rdfs:label "English Language Arts Standards - Anchor Standards - College and Career Readiness Anchor Standards for Language - 2"^^xsd:string ;
    rdfs:comment "Demonstrate command of the conventions of standard English capitalization, punctuation, and spelling when writing."^^xsd:string .

:CCSS.Math.Content.4.NBT.A.3 rdf:type owl:Class ;
    rdfs:subClassOf :CCSS.Math.Content.4.NBT.A ;
    prov:wasQuotedFrom <http://www.corestandards.org/Math/Content/4/NBT/3/> ;
    rdfs:label "English Language Arts Standards - Anchor Standards - College and Career Readiness Anchor Standards for Language - 3"^^xsd:string ;
    rdfs:comment "Apply knowledge of language to understand how language functions in different contexts, to make effective choices for meaning or style, and to comprehend more fully when reading or listening. "^^xsd:string .

:CCSS.Math.Content.4.NBT.B rdf:type owl:Class ;
    rdfs:subClassOf :CCSS.Math.Content.4.NBT ;
    rdfs:label "Number & Operations in Base Ten"^^xsd:string ;
    prov:wasQuotedFrom <http://www.corestandards.org/Math/Content/4/NBT/> .

:CCSS.Math.Content.4.NBT.B.4 rdf:type owl:Class ;
    rdfs:subClassOf :CCSS.Math.Content.4.NBT.B ;
    prov:wasQuotedFrom <http://www.corestandards.org/Math/Content/4/NBT/4/> ;
    rdfs:label "English Language Arts Standards - Anchor Standards - College and Career Readiness Anchor Standards for Language - 4"^^xsd:string ;
    rdfs:comment "Determine or clarify the meaning of unknown and multiple-meaning words and phrases by using context clues, analyzing meaningful word parts, and consulting general and specialized reference materials, as appropriate."^^xsd:string .

:CCSS.Math.Content.4.NBT.B.5 rdf:type owl:Class ;
    rdfs:subClassOf :CCSS.Math.Content.4.NBT.B ;
    prov:wasQuotedFrom <http://www.corestandards.org/Math/Content/4/NBT/5/> ;
    rdfs:label "English Language Arts Standards - Anchor Standards - College and Career Readiness Anchor Standards for Language - 5"^^xsd:string ;
    rdfs:comment "Demonstrate understanding of figurative language, word relationships, and nuances in word meanings."^^xsd:string .

:CCSS.Math.Content.4.NBT.B.6 rdf:type owl:Class ;
    rdfs:subClassOf :CCSS.Math.Content.4.NBT.B ;
    prov:wasQuotedFrom <http://www.corestandards.org/Math/Content/4/NBT/6/> ;
    rdfs:label "English Language Arts Standards - Anchor Standards - College and Career Readiness Anchor Standards for Language - 6"^^xsd:string ;
    rdfs:comment "Acquire and use accurately a range of general academic and domain-specific words and phrases sufficient for reading, writing, speaking, and listening at the college and career readiness level; demonstrate independence in gathering vocabulary knowledge when encountering an unknown term important to comprehension or expression."^^xsd:string .

:CCSS.Math.Content.4.NF rdf:type owl:Class ;
    rdfs:subClassOf :CCSS.Math.Content.4 ;
    rdfs:label "Number & OperationsFractions"^^xsd:string ;
    prov:wasQuotedFrom <http://www.corestandards.org/Math/Content/4/NF/> .

:CCSS.Math.Content.4.NF.A rdf:type owl:Class ;
    rdfs:subClassOf :CCSS.Math.Content.4.NF ;
    rdfs:label "Number & OperationsFractions"^^xsd:string ;
    prov:wasQuotedFrom <http://www.corestandards.org/Math/Content/4/NF/> .

:CCSS.Math.Content.4.NF.A.1 rdf:type owl:Class ;
    rdfs:subClassOf :CCSS.Math.Content.4.NF.A ;
    prov:wasQuotedFrom <http://www.corestandards.org/Math/Content/4/NF/1/> ;
    rdfs:label "English Language Arts Standards - Anchor Standards - College and Career Readiness Anchor Standards for Language - 1"^^xsd:string ;
    rdfs:comment "Demonstrate command of the conventions of standard English grammar and usage when writing or speaking."^^xsd:string .

:CCSS.Math.Content.4.NF.A.2 rdf:type owl:Class ;
    rdfs:subClassOf :CCSS.Math.Content.4.NF.A ;
    prov:wasQuotedFrom <http://www.corestandards.org/Math/Content/4/NF/2/> ;
    rdfs:label "English Language Arts Standards - Anchor Standards - College and Career Readiness Anchor Standards for Language - 2"^^xsd:string ;
    rdfs:comment "Demonstrate command of the conventions of standard English capitalization, punctuation, and spelling when writing."^^xsd:string .

:CCSS.Math.Content.4.NF.B rdf:type owl:Class ;
    rdfs:subClassOf :CCSS.Math.Content.4.NF ;
    rdfs:label "Number & OperationsFractions"^^xsd:string ;
    prov:wasQuotedFrom <http://www.corestandards.org/Math/Content/4/NF/> .

:CCSS.Math.Content.4.NF.B.3 rdf:type owl:Class ;
    rdfs:subClassOf :CCSS.Math.Content.4.NF.B ;
    prov:wasQuotedFrom <http://www.corestandards.org/Math/Content/4/NF/3/> ;
    rdfs:label "English Language Arts Standards - Anchor Standards - College and Career Readiness Anchor Standards for Language - 3"^^xsd:string ;
    rdfs:comment "Apply knowledge of language to understand how language functions in different contexts, to make effective choices for meaning or style, and to comprehend more fully when reading or listening. "^^xsd:string .

:CCSS.Math.Content.4.NF.B.4 rdf:type owl:Class ;
    rdfs:subClassOf :CCSS.Math.Content.4.NF.B ;
    prov:wasQuotedFrom <http://www.corestandards.org/Math/Content/4/NF/4/> ;
    rdfs:label "English Language Arts Standards - Anchor Standards - College and Career Readiness Anchor Standards for Language - 4"^^xsd:string ;
    rdfs:comment "Determine or clarify the meaning of unknown and multiple-meaning words and phrases by using context clues, analyzing meaningful word parts, and consulting general and specialized reference materials, as appropriate."^^xsd:string .

:CCSS.Math.Content.4.NF.C rdf:type owl:Class ;
    rdfs:subClassOf :CCSS.Math.Content.4.NF ;
    rdfs:label "Number & OperationsFractions"^^xsd:string ;
    prov:wasQuotedFrom <http://www.corestandards.org/Math/Content/4/NF/> .

:CCSS.Math.Content.4.NF.C.5 rdf:type owl:Class ;
    rdfs:subClassOf :CCSS.Math.Content.4.NF.C ;
    prov:wasQuotedFrom <http://www.corestandards.org/Math/Content/4/NF/5/> ;
    rdfs:label "English Language Arts Standards - Anchor Standards - College and Career Readiness Anchor Standards for Language - 5"^^xsd:string ;
    rdfs:comment "Demonstrate understanding of figurative language, word relationships, and nuances in word meanings."^^xsd:string .

:CCSS.Math.Content.4.NF.C.6 rdf:type owl:Class ;
    rdfs:subClassOf :CCSS.Math.Content.4.NF.C ;
    prov:wasQuotedFrom <http://www.corestandards.org/Math/Content/4/NF/6/> ;
    rdfs:label "English Language Arts Standards - Anchor Standards - College and Career Readiness Anchor Standards for Language - 6"^^xsd:string ;
    rdfs:comment "Acquire and use accurately a range of general academic and domain-specific words and phrases sufficient for reading, writing, speaking, and listening at the college and career readiness level; demonstrate independence in gathering vocabulary knowledge when encountering an unknown term important to comprehension or expression."^^xsd:string .

:CCSS.Math.Content.4.NF.C.7 rdf:type owl:Class ;
    rdfs:subClassOf :CCSS.Math.Content.4.NF.C ;
    prov:wasQuotedFrom <http://www.corestandards.org/Math/Content/4/NF/7/> ;
    rdfs:label "English Language Arts Standards - Anchor Standards - College and Career Readiness Anchor Standards for Reading - 7"^^xsd:string ;
    rdfs:comment "Integrate and evaluate content presented in diverse media and formats, including visually and quantitatively, as well as in words.1"^^xsd:string .

:CCSS.Math.Content.4.NF.B.3.a rdf:type owl:Class ;
    rdfs:subClassOf :CCSS.Math.Content.4.NF.B.3 ;
    prov:wasQuotedFrom <http://www.corestandards.org/Math/Content/4/NF/a/> .

:CCSS.Math.Content.4.NF.B.3.b rdf:type owl:Class ;
    rdfs:subClassOf :CCSS.Math.Content.4.NF.B.3 ;
    prov:wasQuotedFrom <http://www.corestandards.org/Math/Content/4/NF/b/> .

:CCSS.Math.Content.4.NF.B.3.c rdf:type owl:Class ;
    rdfs:subClassOf :CCSS.Math.Content.4.NF.B.3 ;
    prov:wasQuotedFrom <http://www.corestandards.org/Math/Content/4/NF/c/> .

:CCSS.Math.Content.4.NF.B.3.d rdf:type owl:Class ;
    rdfs:subClassOf :CCSS.Math.Content.4.NF.B.3 ;
    prov:wasQuotedFrom <http://www.corestandards.org/Math/Content/4/NF/d/> .

:CCSS.Math.Content.4.NF.B.4.a rdf:type owl:Class ;
    rdfs:subClassOf :CCSS.Math.Content.4.NF.B.4 ;
    prov:wasQuotedFrom <http://www.corestandards.org/Math/Content/4/NF/a/> .

:CCSS.Math.Content.4.NF.B.4.b rdf:type owl:Class ;
    rdfs:subClassOf :CCSS.Math.Content.4.NF.B.4 ;
    prov:wasQuotedFrom <http://www.corestandards.org/Math/Content/4/NF/b/> .

:CCSS.Math.Content.4.NF.B.4.c rdf:type owl:Class ;
    rdfs:subClassOf :CCSS.Math.Content.4.NF.B.4 ;
    prov:wasQuotedFrom <http://www.corestandards.org/Math/Content/4/NF/c/> .

:CCSS.Math.Content.4.MD rdf:type owl:Class ;
    rdfs:subClassOf :CCSS.Math.Content.4 ;
    rdfs:label "Measurement & Data"^^xsd:string ;
    prov:wasQuotedFrom <http://www.corestandards.org/Math/Content/4/MD/> .

:CCSS.Math.Content.4.MD.A rdf:type owl:Class ;
    rdfs:subClassOf :CCSS.Math.Content.4.MD ;
    rdfs:label "Measurement & Data"^^xsd:string ;
    prov:wasQuotedFrom <http://www.corestandards.org/Math/Content/4/MD/> .

:CCSS.Math.Content.4.MD.A.1 rdf:type owl:Class ;
    rdfs:subClassOf :CCSS.Math.Content.4.MD.A ;
    prov:wasQuotedFrom <http://www.corestandards.org/Math/Content/4/MD/1/> ;
    rdfs:label "English Language Arts Standards - Anchor Standards - College and Career Readiness Anchor Standards for Language - 1"^^xsd:string ;
    rdfs:comment "Demonstrate command of the conventions of standard English grammar and usage when writing or speaking."^^xsd:string .

:CCSS.Math.Content.4.MD.A.2 rdf:type owl:Class ;
    rdfs:subClassOf :CCSS.Math.Content.4.MD.A ;
    prov:wasQuotedFrom <http://www.corestandards.org/Math/Content/4/MD/2/> ;
    rdfs:label "English Language Arts Standards - Anchor Standards - College and Career Readiness Anchor Standards for Language - 2"^^xsd:string ;
    rdfs:comment "Demonstrate command of the conventions of standard English capitalization, punctuation, and spelling when writing."^^xsd:string .

:CCSS.Math.Content.4.MD.A.3 rdf:type owl:Class ;
    rdfs:subClassOf :CCSS.Math.Content.4.MD.A ;
    prov:wasQuotedFrom <http://www.corestandards.org/Math/Content/4/MD/3/> ;
    rdfs:label "English Language Arts Standards - Anchor Standards - College and Career Readiness Anchor Standards for Language - 3"^^xsd:string ;
    rdfs:comment "Apply knowledge of language to understand how language functions in different contexts, to make effective choices for meaning or style, and to comprehend more fully when reading or listening. "^^xsd:string .

:CCSS.Math.Content.4.MD.B rdf:type owl:Class ;
    rdfs:subClassOf :CCSS.Math.Content.4.MD ;
    rdfs:label "Measurement & Data"^^xsd:string ;
    prov:wasQuotedFrom <http://www.corestandards.org/Math/Content/4/MD/> .

:CCSS.Math.Content.4.MD.B.4 rdf:type owl:Class ;
    rdfs:subClassOf :CCSS.Math.Content.4.MD.B ;
    prov:wasQuotedFrom <http://www.corestandards.org/Math/Content/4/MD/4/> ;
    rdfs:label "English Language Arts Standards - Anchor Standards - College and Career Readiness Anchor Standards for Language - 4"^^xsd:string ;
    rdfs:comment "Determine or clarify the meaning of unknown and multiple-meaning words and phrases by using context clues, analyzing meaningful word parts, and consulting general and specialized reference materials, as appropriate."^^xsd:string .

:CCSS.Math.Content.4.MD.C rdf:type owl:Class ;
    rdfs:subClassOf :CCSS.Math.Content.4.MD ;
    rdfs:label "Measurement & Data"^^xsd:string ;
    prov:wasQuotedFrom <http://www.corestandards.org/Math/Content/4/MD/> .

:CCSS.Math.Content.4.MD.C.5 rdf:type owl:Class ;
    rdfs:subClassOf :CCSS.Math.Content.4.MD.C ;
    prov:wasQuotedFrom <http://www.corestandards.org/Math/Content/4/MD/5/> ;
    rdfs:label "English Language Arts Standards - Anchor Standards - College and Career Readiness Anchor Standards for Language - 5"^^xsd:string ;
    rdfs:comment "Demonstrate understanding of figurative language, word relationships, and nuances in word meanings."^^xsd:string .

:CCSS.Math.Content.4.MD.C.6 rdf:type owl:Class ;
    rdfs:subClassOf :CCSS.Math.Content.4.MD.C ;
    prov:wasQuotedFrom <http://www.corestandards.org/Math/Content/4/MD/6/> ;
    rdfs:label "English Language Arts Standards - Anchor Standards - College and Career Readiness Anchor Standards for Language - 6"^^xsd:string ;
    rdfs:comment "Acquire and use accurately a range of general academic and domain-specific words and phrases sufficient for reading, writing, speaking, and listening at the college and career readiness level; demonstrate independence in gathering vocabulary knowledge when encountering an unknown term important to comprehension or expression."^^xsd:string .

:CCSS.Math.Content.4.MD.C.7 rdf:type owl:Class ;
    rdfs:subClassOf :CCSS.Math.Content.4.MD.C ;
    prov:wasQuotedFrom <http://www.corestandards.org/Math/Content/4/MD/7/> ;
    rdfs:label "English Language Arts Standards - Anchor Standards - College and Career Readiness Anchor Standards for Reading - 7"^^xsd:string ;
    rdfs:comment "Integrate and evaluate content presented in diverse media and formats, including visually and quantitatively, as well as in words.1"^^xsd:string .

:CCSS.Math.Content.4.MD.C.5.a rdf:type owl:Class ;
    rdfs:subClassOf :CCSS.Math.Content.4.MD.C.5 ;
    prov:wasQuotedFrom <http://www.corestandards.org/Math/Content/4/MD/a/> .

:CCSS.Math.Content.4.MD.C.5.b rdf:type owl:Class ;
    rdfs:subClassOf :CCSS.Math.Content.4.MD.C.5 ;
    prov:wasQuotedFrom <http://www.corestandards.org/Math/Content/4/MD/b/> .

:CCSS.Math.Content.4.G rdf:type owl:Class ;
    rdfs:subClassOf :CCSS.Math.Content.4 ;
    rdfs:label "Geometry"^^xsd:string ;
    prov:wasQuotedFrom <http://www.corestandards.org/Math/Content/4/G/> .

:CCSS.Math.Content.4.G.A rdf:type owl:Class ;
    rdfs:subClassOf :CCSS.Math.Content.4.G ;
    rdfs:label "Geometry"^^xsd:string ;
    prov:wasQuotedFrom <http://www.corestandards.org/Math/Content/4/G/> .

:CCSS.Math.Content.4.G.A.1 rdf:type owl:Class ;
    rdfs:subClassOf :CCSS.Math.Content.4.G.A ;
    prov:wasQuotedFrom <http://www.corestandards.org/Math/Content/4/G/1/> ;
    rdfs:label "English Language Arts Standards - Anchor Standards - College and Career Readiness Anchor Standards for Language - 1"^^xsd:string ;
    rdfs:comment "Demonstrate command of the conventions of standard English grammar and usage when writing or speaking."^^xsd:string .

:CCSS.Math.Content.4.G.A.2 rdf:type owl:Class ;
    rdfs:subClassOf :CCSS.Math.Content.4.G.A ;
    prov:wasQuotedFrom <http://www.corestandards.org/Math/Content/4/G/2/> ;
    rdfs:label "English Language Arts Standards - Anchor Standards - College and Career Readiness Anchor Standards for Language - 2"^^xsd:string ;
    rdfs:comment "Demonstrate command of the conventions of standard English capitalization, punctuation, and spelling when writing."^^xsd:string .

:CCSS.Math.Content.4.G.A.3 rdf:type owl:Class ;
    rdfs:subClassOf :CCSS.Math.Content.4.G.A ;
    prov:wasQuotedFrom <http://www.corestandards.org/Math/Content/4/G/3/> ;
    rdfs:label "English Language Arts Standards - Anchor Standards - College and Career Readiness Anchor Standards for Language - 3"^^xsd:string ;
    rdfs:comment "Apply knowledge of language to understand how language functions in different contexts, to make effective choices for meaning or style, and to comprehend more fully when reading or listening. "^^xsd:string .

:CCSS.Math.Content.5 rdf:type owl:Class ;
    rdfs:subClassOf :CCSS.Math.Content ;
    prov:wasQuotedFrom <http://www.corestandards.org/Math/Content/5/> .

:CCSS.Math.Content.5.OA rdf:type owl:Class ;
    rdfs:subClassOf :CCSS.Math.Content.5 ;
    rdfs:label "Operations & Algebraic Thinking"^^xsd:string ;
    prov:wasQuotedFrom <http://www.corestandards.org/Math/Content/5/OA/> .

:CCSS.Math.Content.5.OA.A rdf:type owl:Class ;
    rdfs:subClassOf :CCSS.Math.Content.5.OA ;
    rdfs:label "Operations & Algebraic Thinking"^^xsd:string ;
    prov:wasQuotedFrom <http://www.corestandards.org/Math/Content/5/OA/> .

:CCSS.Math.Content.5.OA.A.1 rdf:type owl:Class ;
    rdfs:subClassOf :CCSS.Math.Content.5.OA.A ;
    prov:wasQuotedFrom <http://www.corestandards.org/Math/Content/5/OA/1/> ;
    rdfs:label "English Language Arts Standards - Anchor Standards - College and Career Readiness Anchor Standards for Language - 1"^^xsd:string ;
    rdfs:comment "Demonstrate command of the conventions of standard English grammar and usage when writing or speaking."^^xsd:string .

:CCSS.Math.Content.5.OA.A.2 rdf:type owl:Class ;
    rdfs:subClassOf :CCSS.Math.Content.5.OA.A ;
    prov:wasQuotedFrom <http://www.corestandards.org/Math/Content/5/OA/2/> ;
    rdfs:label "English Language Arts Standards - Anchor Standards - College and Career Readiness Anchor Standards for Language - 2"^^xsd:string ;
    rdfs:comment "Demonstrate command of the conventions of standard English capitalization, punctuation, and spelling when writing."^^xsd:string .

:CCSS.Math.Content.5.OA.B rdf:type owl:Class ;
    rdfs:subClassOf :CCSS.Math.Content.5.OA ;
    rdfs:label "Operations & Algebraic Thinking"^^xsd:string ;
    prov:wasQuotedFrom <http://www.corestandards.org/Math/Content/5/OA/> .

:CCSS.Math.Content.5.OA.B.3 rdf:type owl:Class ;
    rdfs:subClassOf :CCSS.Math.Content.5.OA.B ;
    prov:wasQuotedFrom <http://www.corestandards.org/Math/Content/5/OA/3/> ;
    rdfs:label "English Language Arts Standards - Anchor Standards - College and Career Readiness Anchor Standards for Language - 3"^^xsd:string ;
    rdfs:comment "Apply knowledge of language to understand how language functions in different contexts, to make effective choices for meaning or style, and to comprehend more fully when reading or listening. "^^xsd:string .

:CCSS.Math.Content.5.NBT rdf:type owl:Class ;
    rdfs:subClassOf :CCSS.Math.Content.5 ;
    rdfs:label "Number & Operations in Base Ten"^^xsd:string ;
    prov:wasQuotedFrom <http://www.corestandards.org/Math/Content/5/NBT/> .

:CCSS.Math.Content.5.NBT.A rdf:type owl:Class ;
    rdfs:subClassOf :CCSS.Math.Content.5.NBT ;
    rdfs:label "Number & Operations in Base Ten"^^xsd:string ;
    prov:wasQuotedFrom <http://www.corestandards.org/Math/Content/5/NBT/> .

:CCSS.Math.Content.5.NBT.A.1 rdf:type owl:Class ;
    rdfs:subClassOf :CCSS.Math.Content.5.NBT.A ;
    prov:wasQuotedFrom <http://www.corestandards.org/Math/Content/5/NBT/1/> ;
    rdfs:label "English Language Arts Standards - Anchor Standards - College and Career Readiness Anchor Standards for Language - 1"^^xsd:string ;
    rdfs:comment "Demonstrate command of the conventions of standard English grammar and usage when writing or speaking."^^xsd:string .

:CCSS.Math.Content.5.NBT.A.2 rdf:type owl:Class ;
    rdfs:subClassOf :CCSS.Math.Content.5.NBT.A ;
    prov:wasQuotedFrom <http://www.corestandards.org/Math/Content/5/NBT/2/> ;
    rdfs:label "English Language Arts Standards - Anchor Standards - College and Career Readiness Anchor Standards for Language - 2"^^xsd:string ;
    rdfs:comment "Demonstrate command of the conventions of standard English capitalization, punctuation, and spelling when writing."^^xsd:string .

:CCSS.Math.Content.5.NBT.A.3 rdf:type owl:Class ;
    rdfs:subClassOf :CCSS.Math.Content.5.NBT.A ;
    prov:wasQuotedFrom <http://www.corestandards.org/Math/Content/5/NBT/3/> ;
    rdfs:label "English Language Arts Standards - Anchor Standards - College and Career Readiness Anchor Standards for Language - 3"^^xsd:string ;
    rdfs:comment "Apply knowledge of language to understand how language functions in different contexts, to make effective choices for meaning or style, and to comprehend more fully when reading or listening. "^^xsd:string .

:CCSS.Math.Content.5.NBT.A.4 rdf:type owl:Class ;
    rdfs:subClassOf :CCSS.Math.Content.5.NBT.A ;
    prov:wasQuotedFrom <http://www.corestandards.org/Math/Content/5/NBT/4/> ;
    rdfs:label "English Language Arts Standards - Anchor Standards - College and Career Readiness Anchor Standards for Language - 4"^^xsd:string ;
    rdfs:comment "Determine or clarify the meaning of unknown and multiple-meaning words and phrases by using context clues, analyzing meaningful word parts, and consulting general and specialized reference materials, as appropriate."^^xsd:string .

:CCSS.Math.Content.5.NBT.B rdf:type owl:Class ;
    rdfs:subClassOf :CCSS.Math.Content.5.NBT ;
    rdfs:label "Number & Operations in Base Ten"^^xsd:string ;
    prov:wasQuotedFrom <http://www.corestandards.org/Math/Content/5/NBT/> .

:CCSS.Math.Content.5.NBT.B.5 rdf:type owl:Class ;
    rdfs:subClassOf :CCSS.Math.Content.5.NBT.B ;
    prov:wasQuotedFrom <http://www.corestandards.org/Math/Content/5/NBT/5/> ;
    rdfs:label "English Language Arts Standards - Anchor Standards - College and Career Readiness Anchor Standards for Language - 5"^^xsd:string ;
    rdfs:comment "Demonstrate understanding of figurative language, word relationships, and nuances in word meanings."^^xsd:string .

:CCSS.Math.Content.5.NBT.B.6 rdf:type owl:Class ;
    rdfs:subClassOf :CCSS.Math.Content.5.NBT.B ;
    prov:wasQuotedFrom <http://www.corestandards.org/Math/Content/5/NBT/6/> ;
    rdfs:label "English Language Arts Standards - Anchor Standards - College and Career Readiness Anchor Standards for Language - 6"^^xsd:string ;
    rdfs:comment "Acquire and use accurately a range of general academic and domain-specific words and phrases sufficient for reading, writing, speaking, and listening at the college and career readiness level; demonstrate independence in gathering vocabulary knowledge when encountering an unknown term important to comprehension or expression."^^xsd:string .

:CCSS.Math.Content.5.NBT.B.7 rdf:type owl:Class ;
    rdfs:subClassOf :CCSS.Math.Content.5.NBT.B ;
    prov:wasQuotedFrom <http://www.corestandards.org/Math/Content/5/NBT/7/> ;
    rdfs:label "English Language Arts Standards - Anchor Standards - College and Career Readiness Anchor Standards for Reading - 7"^^xsd:string ;
    rdfs:comment "Integrate and evaluate content presented in diverse media and formats, including visually and quantitatively, as well as in words.1"^^xsd:string .

:CCSS.Math.Content.5.NBT.A.3.a rdf:type owl:Class ;
    rdfs:subClassOf :CCSS.Math.Content.5.NBT.A.3 ;
    prov:wasQuotedFrom <http://www.corestandards.org/Math/Content/5/NBT/a/> .

:CCSS.Math.Content.5.NBT.A.3.b rdf:type owl:Class ;
    rdfs:subClassOf :CCSS.Math.Content.5.NBT.A.3 ;
    prov:wasQuotedFrom <http://www.corestandards.org/Math/Content/5/NBT/b/> .

:CCSS.Math.Content.5.NF rdf:type owl:Class ;
    rdfs:subClassOf :CCSS.Math.Content.5 ;
    rdfs:label "Number & Operations-Fractions"^^xsd:string ;
    prov:wasQuotedFrom <http://www.corestandards.org/Math/Content/5/NF/> .

:CCSS.Math.Content.5.NF.A rdf:type owl:Class ;
    rdfs:subClassOf :CCSS.Math.Content.5.NF ;
    rdfs:label "Number & Operations-Fractions"^^xsd:string ;
    prov:wasQuotedFrom <http://www.corestandards.org/Math/Content/5/NF/> .

:CCSS.Math.Content.5.NF.A.1 rdf:type owl:Class ;
    rdfs:subClassOf :CCSS.Math.Content.5.NF.A ;
    prov:wasQuotedFrom <http://www.corestandards.org/Math/Content/5/NF/1/> ;
    rdfs:label "English Language Arts Standards - Anchor Standards - College and Career Readiness Anchor Standards for Language - 1"^^xsd:string ;
    rdfs:comment "Demonstrate command of the conventions of standard English grammar and usage when writing or speaking."^^xsd:string .

:CCSS.Math.Content.5.NF.A.2 rdf:type owl:Class ;
    rdfs:subClassOf :CCSS.Math.Content.5.NF.A ;
    prov:wasQuotedFrom <http://www.corestandards.org/Math/Content/5/NF/2/> ;
    rdfs:label "English Language Arts Standards - Anchor Standards - College and Career Readiness Anchor Standards for Language - 2"^^xsd:string ;
    rdfs:comment "Demonstrate command of the conventions of standard English capitalization, punctuation, and spelling when writing."^^xsd:string .

:CCSS.Math.Content.5.NF.B rdf:type owl:Class ;
    rdfs:subClassOf :CCSS.Math.Content.5.NF ;
    rdfs:label "Number & OperationsFractions"^^xsd:string ;
    prov:wasQuotedFrom <http://www.corestandards.org/Math/Content/5/NF/> .

:CCSS.Math.Content.5.NF.B.3 rdf:type owl:Class ;
    rdfs:subClassOf :CCSS.Math.Content.5.NF.B ;
    prov:wasQuotedFrom <http://www.corestandards.org/Math/Content/5/NF/3/> ;
    rdfs:label "English Language Arts Standards - Anchor Standards - College and Career Readiness Anchor Standards for Language - 3"^^xsd:string ;
    rdfs:comment "Apply knowledge of language to understand how language functions in different contexts, to make effective choices for meaning or style, and to comprehend more fully when reading or listening. "^^xsd:string .

:CCSS.Math.Content.5.NF.B.4 rdf:type owl:Class ;
    rdfs:subClassOf :CCSS.Math.Content.5.NF.B ;
    prov:wasQuotedFrom <http://www.corestandards.org/Math/Content/5/NF/4/> ;
    rdfs:label "English Language Arts Standards - Anchor Standards - College and Career Readiness Anchor Standards for Language - 4"^^xsd:string ;
    rdfs:comment "Determine or clarify the meaning of unknown and multiple-meaning words and phrases by using context clues, analyzing meaningful word parts, and consulting general and specialized reference materials, as appropriate."^^xsd:string .

:CCSS.Math.Content.5.NF.B.5 rdf:type owl:Class ;
    rdfs:subClassOf :CCSS.Math.Content.5.NF.B ;
    prov:wasQuotedFrom <http://www.corestandards.org/Math/Content/5/NF/5/> ;
    rdfs:label "English Language Arts Standards - Anchor Standards - College and Career Readiness Anchor Standards for Language - 5"^^xsd:string ;
    rdfs:comment "Demonstrate understanding of figurative language, word relationships, and nuances in word meanings."^^xsd:string .

:CCSS.Math.Content.5.NF.B.6 rdf:type owl:Class ;
    rdfs:subClassOf :CCSS.Math.Content.5.NF.B ;
    prov:wasQuotedFrom <http://www.corestandards.org/Math/Content/5/NF/6/> ;
    rdfs:label "English Language Arts Standards - Anchor Standards - College and Career Readiness Anchor Standards for Language - 6"^^xsd:string ;
    rdfs:comment "Acquire and use accurately a range of general academic and domain-specific words and phrases sufficient for reading, writing, speaking, and listening at the college and career readiness level; demonstrate independence in gathering vocabulary knowledge when encountering an unknown term important to comprehension or expression."^^xsd:string .

:CCSS.Math.Content.5.NF.B.7 rdf:type owl:Class ;
    rdfs:subClassOf :CCSS.Math.Content.5.NF.B ;
    prov:wasQuotedFrom <http://www.corestandards.org/Math/Content/5/NF/7/> ;
    rdfs:label "English Language Arts Standards - Anchor Standards - College and Career Readiness Anchor Standards for Reading - 7"^^xsd:string ;
    rdfs:comment "Integrate and evaluate content presented in diverse media and formats, including visually and quantitatively, as well as in words.1"^^xsd:string .

:CCSS.Math.Content.5.NF.B.4.a rdf:type owl:Class ;
    rdfs:subClassOf :CCSS.Math.Content.5.NF.B.4 ;
    prov:wasQuotedFrom <http://www.corestandards.org/Math/Content/5/NF/a/> .

:CCSS.Math.Content.5.NF.B.4.b rdf:type owl:Class ;
    rdfs:subClassOf :CCSS.Math.Content.5.NF.B.4 ;
    prov:wasQuotedFrom <http://www.corestandards.org/Math/Content/5/NF/b/> .

:CCSS.Math.Content.5.NF.B.5.a rdf:type owl:Class ;
    rdfs:subClassOf :CCSS.Math.Content.5.NF.B.5 ;
    prov:wasQuotedFrom <http://www.corestandards.org/Math/Content/5/NF/a/> .

:CCSS.Math.Content.5.NF.B.5.b rdf:type owl:Class ;
    rdfs:subClassOf :CCSS.Math.Content.5.NF.B.5 ;
    prov:wasQuotedFrom <http://www.corestandards.org/Math/Content/5/NF/b/> .

:CCSS.Math.Content.5.NF.B.7.a rdf:type owl:Class ;
    rdfs:subClassOf :CCSS.Math.Content.5.NF.B.7 ;
    prov:wasQuotedFrom <http://www.corestandards.org/Math/Content/5/NF/a/> .

:CCSS.Math.Content.5.NF.B.7.b rdf:type owl:Class ;
    rdfs:subClassOf :CCSS.Math.Content.5.NF.B.7 ;
    prov:wasQuotedFrom <http://www.corestandards.org/Math/Content/5/NF/b/> .

:CCSS.Math.Content.5.NF.B.7.c rdf:type owl:Class ;
    rdfs:subClassOf :CCSS.Math.Content.5.NF.B.7 ;
    prov:wasQuotedFrom <http://www.corestandards.org/Math/Content/5/NF/c/> .

:CCSS.Math.Content.5.MD rdf:type owl:Class ;
    rdfs:subClassOf :CCSS.Math.Content.5 ;
    rdfs:label "Measurement & Data"^^xsd:string ;
    prov:wasQuotedFrom <http://www.corestandards.org/Math/Content/5/MD/> .

:CCSS.Math.Content.5.MD.A rdf:type owl:Class ;
    rdfs:subClassOf :CCSS.Math.Content.5.MD ;
    rdfs:label "Measurement & Data"^^xsd:string ;
    prov:wasQuotedFrom <http://www.corestandards.org/Math/Content/5/MD/> .

:CCSS.Math.Content.5.MD.A.1 rdf:type owl:Class ;
    rdfs:subClassOf :CCSS.Math.Content.5.MD.A ;
    prov:wasQuotedFrom <http://www.corestandards.org/Math/Content/5/MD/1/> ;
    rdfs:label "English Language Arts Standards - Anchor Standards - College and Career Readiness Anchor Standards for Language - 1"^^xsd:string ;
    rdfs:comment "Demonstrate command of the conventions of standard English grammar and usage when writing or speaking."^^xsd:string .

:CCSS.Math.Content.5.MD.B rdf:type owl:Class ;
    rdfs:subClassOf :CCSS.Math.Content.5.MD ;
    rdfs:label "Measurement & Data"^^xsd:string ;
    prov:wasQuotedFrom <http://www.corestandards.org/Math/Content/5/MD/> .

:CCSS.Math.Content.5.MD.B.2 rdf:type owl:Class ;
    rdfs:subClassOf :CCSS.Math.Content.5.MD.B ;
    prov:wasQuotedFrom <http://www.corestandards.org/Math/Content/5/MD/2/> ;
    rdfs:label "English Language Arts Standards - Anchor Standards - College and Career Readiness Anchor Standards for Language - 2"^^xsd:string ;
    rdfs:comment "Demonstrate command of the conventions of standard English capitalization, punctuation, and spelling when writing."^^xsd:string .

:CCSS.Math.Content.5.MD.C rdf:type owl:Class ;
    rdfs:subClassOf :CCSS.Math.Content.5.MD ;
    rdfs:label "Measurement & Data"^^xsd:string ;
    prov:wasQuotedFrom <http://www.corestandards.org/Math/Content/5/MD/> .

:CCSS.Math.Content.5.MD.C.3 rdf:type owl:Class ;
    rdfs:subClassOf :CCSS.Math.Content.5.MD.C ;
    prov:wasQuotedFrom <http://www.corestandards.org/Math/Content/5/MD/3/> ;
    rdfs:label "English Language Arts Standards - Anchor Standards - College and Career Readiness Anchor Standards for Language - 3"^^xsd:string ;
    rdfs:comment "Apply knowledge of language to understand how language functions in different contexts, to make effective choices for meaning or style, and to comprehend more fully when reading or listening. "^^xsd:string .

:CCSS.Math.Content.5.MD.C.4 rdf:type owl:Class ;
    rdfs:subClassOf :CCSS.Math.Content.5.MD.C ;
    prov:wasQuotedFrom <http://www.corestandards.org/Math/Content/5/MD/4/> ;
    rdfs:label "English Language Arts Standards - Anchor Standards - College and Career Readiness Anchor Standards for Language - 4"^^xsd:string ;
    rdfs:comment "Determine or clarify the meaning of unknown and multiple-meaning words and phrases by using context clues, analyzing meaningful word parts, and consulting general and specialized reference materials, as appropriate."^^xsd:string .

:CCSS.Math.Content.5.MD.C.5 rdf:type owl:Class ;
    rdfs:subClassOf :CCSS.Math.Content.5.MD.C ;
    prov:wasQuotedFrom <http://www.corestandards.org/Math/Content/5/MD/5/> ;
    rdfs:label "English Language Arts Standards - Anchor Standards - College and Career Readiness Anchor Standards for Language - 5"^^xsd:string ;
    rdfs:comment "Demonstrate understanding of figurative language, word relationships, and nuances in word meanings."^^xsd:string .

:CCSS.Math.Content.5.MD.C.3.a rdf:type owl:Class ;
    rdfs:subClassOf :CCSS.Math.Content.5.MD.C.3 ;
    prov:wasQuotedFrom <http://www.corestandards.org/Math/Content/5/MD/a/> .

:CCSS.Math.Content.5.MD.C.3.b rdf:type owl:Class ;
    rdfs:subClassOf :CCSS.Math.Content.5.MD.C.3 ;
    prov:wasQuotedFrom <http://www.corestandards.org/Math/Content/5/MD/b/> .

:CCSS.Math.Content.5.MD.C.5.a rdf:type owl:Class ;
    rdfs:subClassOf :CCSS.Math.Content.5.MD.C.5 ;
    prov:wasQuotedFrom <http://www.corestandards.org/Math/Content/5/MD/a/> .

:CCSS.Math.Content.5.MD.C.5.b rdf:type owl:Class ;
    rdfs:subClassOf :CCSS.Math.Content.5.MD.C.5 ;
    prov:wasQuotedFrom <http://www.corestandards.org/Math/Content/5/MD/b/> .

:CCSS.Math.Content.5.MD.C.5.c rdf:type owl:Class ;
    rdfs:subClassOf :CCSS.Math.Content.5.MD.C.5 ;
    prov:wasQuotedFrom <http://www.corestandards.org/Math/Content/5/MD/c/> .

:CCSS.Math.Content.5.G rdf:type owl:Class ;
    rdfs:subClassOf :CCSS.Math.Content.5 ;
    rdfs:label "Geometry"^^xsd:string ;
    prov:wasQuotedFrom <http://www.corestandards.org/Math/Content/5/G/> .

:CCSS.Math.Content.5.G.A rdf:type owl:Class ;
    rdfs:subClassOf :CCSS.Math.Content.5.G ;
    rdfs:label "Geometry"^^xsd:string ;
    prov:wasQuotedFrom <http://www.corestandards.org/Math/Content/5/G/> .

:CCSS.Math.Content.5.G.A.1 rdf:type owl:Class ;
    rdfs:subClassOf :CCSS.Math.Content.5.G.A ;
    prov:wasQuotedFrom <http://www.corestandards.org/Math/Content/5/G/1/> ;
    rdfs:label "English Language Arts Standards - Anchor Standards - College and Career Readiness Anchor Standards for Language - 1"^^xsd:string ;
    rdfs:comment "Demonstrate command of the conventions of standard English grammar and usage when writing or speaking."^^xsd:string .

:CCSS.Math.Content.5.G.A.2 rdf:type owl:Class ;
    rdfs:subClassOf :CCSS.Math.Content.5.G.A ;
    prov:wasQuotedFrom <http://www.corestandards.org/Math/Content/5/G/2/> ;
    rdfs:label "English Language Arts Standards - Anchor Standards - College and Career Readiness Anchor Standards for Language - 2"^^xsd:string ;
    rdfs:comment "Demonstrate command of the conventions of standard English capitalization, punctuation, and spelling when writing."^^xsd:string .

:CCSS.Math.Content.5.G.B rdf:type owl:Class ;
    rdfs:subClassOf :CCSS.Math.Content.5.G ;
    rdfs:label "Geometry"^^xsd:string ;
    prov:wasQuotedFrom <http://www.corestandards.org/Math/Content/5/G/> .

:CCSS.Math.Content.5.G.B.3 rdf:type owl:Class ;
    rdfs:subClassOf :CCSS.Math.Content.5.G.B ;
    prov:wasQuotedFrom <http://www.corestandards.org/Math/Content/5/G/3/> ;
    rdfs:label "English Language Arts Standards - Anchor Standards - College and Career Readiness Anchor Standards for Language - 3"^^xsd:string ;
    rdfs:comment "Apply knowledge of language to understand how language functions in different contexts, to make effective choices for meaning or style, and to comprehend more fully when reading or listening. "^^xsd:string .

:CCSS.Math.Content.5.G.B.4 rdf:type owl:Class ;
    rdfs:subClassOf :CCSS.Math.Content.5.G.B ;
    prov:wasQuotedFrom <http://www.corestandards.org/Math/Content/5/G/4/> ;
    rdfs:label "English Language Arts Standards - Anchor Standards - College and Career Readiness Anchor Standards for Language - 4"^^xsd:string ;
    rdfs:comment "Determine or clarify the meaning of unknown and multiple-meaning words and phrases by using context clues, analyzing meaningful word parts, and consulting general and specialized reference materials, as appropriate."^^xsd:string .

:CCSS.Math.Content.6 rdf:type owl:Class ;
    rdfs:subClassOf :CCSS.Math.Content ;
    prov:wasQuotedFrom <http://www.corestandards.org/Math/Content/1/> .

:CCSS.Math.Content.6.RP rdf:type owl:Class ;
    rdfs:subClassOf :CCSS.Math.Content.6 ;
    rdfs:label "Ratios & Proportional Relationships"^^xsd:string ;
    prov:wasQuotedFrom <http://www.corestandards.org/Math/Content/6/RP/> .

:CCSS.Math.Content.6.RP.A rdf:type owl:Class ;
    rdfs:subClassOf :CCSS.Math.Content.6.RP ;
    rdfs:label "Ratios & Proportional Relationships"^^xsd:string ;
    prov:wasQuotedFrom <http://www.corestandards.org/Math/Content/6/RP/> .

:CCSS.Math.Content.6.RP.A.1 rdf:type owl:Class ;
    rdfs:subClassOf :CCSS.Math.Content.6.RP.A ;
    prov:wasQuotedFrom <http://www.corestandards.org/Math/Content/6/RP/1/> ;
    rdfs:label "English Language Arts Standards - Anchor Standards - College and Career Readiness Anchor Standards for Language - 1"^^xsd:string ;
    rdfs:comment "Demonstrate command of the conventions of standard English grammar and usage when writing or speaking."^^xsd:string .

:CCSS.Math.Content.6.RP.A.2 rdf:type owl:Class ;
    rdfs:subClassOf :CCSS.Math.Content.6.RP.A ;
    prov:wasQuotedFrom <http://www.corestandards.org/Math/Content/6/RP/2/> ;
    rdfs:label "English Language Arts Standards - Anchor Standards - College and Career Readiness Anchor Standards for Language - 2"^^xsd:string ;
    rdfs:comment "Demonstrate command of the conventions of standard English capitalization, punctuation, and spelling when writing."^^xsd:string .

:CCSS.Math.Content.6.RP.A.3 rdf:type owl:Class ;
    rdfs:subClassOf :CCSS.Math.Content.6.RP.A ;
    prov:wasQuotedFrom <http://www.corestandards.org/Math/Content/6/RP/3/> ;
    rdfs:label "English Language Arts Standards - Anchor Standards - College and Career Readiness Anchor Standards for Language - 3"^^xsd:string ;
    rdfs:comment "Apply knowledge of language to understand how language functions in different contexts, to make effective choices for meaning or style, and to comprehend more fully when reading or listening. "^^xsd:string .

:CCSS.Math.Content.6.RP.A.3.a rdf:type owl:Class ;
    rdfs:subClassOf :CCSS.Math.Content.6.RP.A.3 ;
    prov:wasQuotedFrom <http://www.corestandards.org/Math/Content/6/RP/a/> .

:CCSS.Math.Content.6.RP.A.3.b rdf:type owl:Class ;
    rdfs:subClassOf :CCSS.Math.Content.6.RP.A.3 ;
    prov:wasQuotedFrom <http://www.corestandards.org/Math/Content/6/RP/b/> .

:CCSS.Math.Content.6.RP.A.3.c rdf:type owl:Class ;
    rdfs:subClassOf :CCSS.Math.Content.6.RP.A.3 ;
    prov:wasQuotedFrom <http://www.corestandards.org/Math/Content/6/RP/c/> .

:CCSS.Math.Content.6.RP.A.3.d rdf:type owl:Class ;
    rdfs:subClassOf :CCSS.Math.Content.6.RP.A.3 ;
    prov:wasQuotedFrom <http://www.corestandards.org/Math/Content/6/RP/d/> .

:CCSS.Math.Content.6.NS rdf:type owl:Class ;
    rdfs:subClassOf :CCSS.Math.Content.6 ;
    rdfs:label "The Number System"^^xsd:string ;
    prov:wasQuotedFrom <http://www.corestandards.org/Math/Content/6/NS/> .

:CCSS.Math.Content.6.NS.A rdf:type owl:Class ;
    rdfs:subClassOf :CCSS.Math.Content.6.NS ;
    rdfs:label "The Number System"^^xsd:string ;
    prov:wasQuotedFrom <http://www.corestandards.org/Math/Content/6/NS/> .

:CCSS.Math.Content.6.NS.A.1 rdf:type owl:Class ;
    rdfs:subClassOf :CCSS.Math.Content.6.NS.A ;
    prov:wasQuotedFrom <http://www.corestandards.org/Math/Content/6/NS/1/> ;
    rdfs:label "English Language Arts Standards - Anchor Standards - College and Career Readiness Anchor Standards for Language - 1"^^xsd:string ;
    rdfs:comment "Demonstrate command of the conventions of standard English grammar and usage when writing or speaking."^^xsd:string .

:CCSS.Math.Content.6.NS.B rdf:type owl:Class ;
    rdfs:subClassOf :CCSS.Math.Content.6.NS ;
    rdfs:label "The Number System"^^xsd:string ;
    prov:wasQuotedFrom <http://www.corestandards.org/Math/Content/6/NS/> .

:CCSS.Math.Content.6.NS.B.2 rdf:type owl:Class ;
    rdfs:subClassOf :CCSS.Math.Content.6.NS.B ;
    prov:wasQuotedFrom <http://www.corestandards.org/Math/Content/6/NS/2/> ;
    rdfs:label "English Language Arts Standards - Anchor Standards - College and Career Readiness Anchor Standards for Language - 2"^^xsd:string ;
    rdfs:comment "Demonstrate command of the conventions of standard English capitalization, punctuation, and spelling when writing."^^xsd:string .

:CCSS.Math.Content.6.NS.B.3 rdf:type owl:Class ;
    rdfs:subClassOf :CCSS.Math.Content.6.NS.B ;
    prov:wasQuotedFrom <http://www.corestandards.org/Math/Content/6/NS/3/> ;
    rdfs:label "English Language Arts Standards - Anchor Standards - College and Career Readiness Anchor Standards for Language - 3"^^xsd:string ;
    rdfs:comment "Apply knowledge of language to understand how language functions in different contexts, to make effective choices for meaning or style, and to comprehend more fully when reading or listening. "^^xsd:string .

:CCSS.Math.Content.6.NS.B.4 rdf:type owl:Class ;
    rdfs:subClassOf :CCSS.Math.Content.6.NS.B ;
    prov:wasQuotedFrom <http://www.corestandards.org/Math/Content/6/NS/4/> ;
    rdfs:label "English Language Arts Standards - Anchor Standards - College and Career Readiness Anchor Standards for Language - 4"^^xsd:string ;
    rdfs:comment "Determine or clarify the meaning of unknown and multiple-meaning words and phrases by using context clues, analyzing meaningful word parts, and consulting general and specialized reference materials, as appropriate."^^xsd:string .

:CCSS.Math.Content.6.NS.C rdf:type owl:Class ;
    rdfs:subClassOf :CCSS.Math.Content.6.NS ;
    rdfs:label "The Number System"^^xsd:string ;
    prov:wasQuotedFrom <http://www.corestandards.org/Math/Content/6/NS/> .

:CCSS.Math.Content.6.NS.C.5 rdf:type owl:Class ;
    rdfs:subClassOf :CCSS.Math.Content.6.NS.C ;
    prov:wasQuotedFrom <http://www.corestandards.org/Math/Content/6/NS/5/> ;
    rdfs:label "English Language Arts Standards - Anchor Standards - College and Career Readiness Anchor Standards for Language - 5"^^xsd:string ;
    rdfs:comment "Demonstrate understanding of figurative language, word relationships, and nuances in word meanings."^^xsd:string .

:CCSS.Math.Content.6.NS.C.6 rdf:type owl:Class ;
    rdfs:subClassOf :CCSS.Math.Content.6.NS.C ;
    prov:wasQuotedFrom <http://www.corestandards.org/Math/Content/6/NS/6/> ;
    rdfs:label "English Language Arts Standards - Anchor Standards - College and Career Readiness Anchor Standards for Language - 6"^^xsd:string ;
    rdfs:comment "Acquire and use accurately a range of general academic and domain-specific words and phrases sufficient for reading, writing, speaking, and listening at the college and career readiness level; demonstrate independence in gathering vocabulary knowledge when encountering an unknown term important to comprehension or expression."^^xsd:string .

:CCSS.Math.Content.6.NS.C.7 rdf:type owl:Class ;
    rdfs:subClassOf :CCSS.Math.Content.6.NS.C ;
    prov:wasQuotedFrom <http://www.corestandards.org/Math/Content/6/NS/7/> ;
    rdfs:label "English Language Arts Standards - Anchor Standards - College and Career Readiness Anchor Standards for Reading - 7"^^xsd:string ;
    rdfs:comment "Integrate and evaluate content presented in diverse media and formats, including visually and quantitatively, as well as in words.1"^^xsd:string .

:CCSS.Math.Content.6.NS.C.8 rdf:type owl:Class ;
    rdfs:subClassOf :CCSS.Math.Content.6.NS.C ;
    prov:wasQuotedFrom <http://www.corestandards.org/Math/Content/6/NS/8/> ;
    rdfs:label "English Language Arts Standards - Anchor Standards - College and Career Readiness Anchor Standards for Reading - 8"^^xsd:string ;
    rdfs:comment "Delineate and evaluate the argument and specific claims in a text, including the validity of the reasoning as well as the relevance and sufficiency of the evidence."^^xsd:string .

:CCSS.Math.Content.6.NS.C.6.a rdf:type owl:Class ;
    rdfs:subClassOf :CCSS.Math.Content.6.NS.C.6 ;
    prov:wasQuotedFrom <http://www.corestandards.org/Math/Content/6/NS/a/> .

:CCSS.Math.Content.6.NS.C.6.b rdf:type owl:Class ;
    rdfs:subClassOf :CCSS.Math.Content.6.NS.C.6 ;
    prov:wasQuotedFrom <http://www.corestandards.org/Math/Content/6/NS/b/> .

:CCSS.Math.Content.6.NS.C.6.c rdf:type owl:Class ;
    rdfs:subClassOf :CCSS.Math.Content.6.NS.C.6 ;
    prov:wasQuotedFrom <http://www.corestandards.org/Math/Content/6/NS/c/> .

:CCSS.Math.Content.6.NS.C.7.a rdf:type owl:Class ;
    rdfs:subClassOf :CCSS.Math.Content.6.NS.C.7 ;
    prov:wasQuotedFrom <http://www.corestandards.org/Math/Content/6/NS/a/> .

:CCSS.Math.Content.6.NS.C.7.b rdf:type owl:Class ;
    rdfs:subClassOf :CCSS.Math.Content.6.NS.C.7 ;
    prov:wasQuotedFrom <http://www.corestandards.org/Math/Content/6/NS/b/> .

:CCSS.Math.Content.6.NS.C.7.c rdf:type owl:Class ;
    rdfs:subClassOf :CCSS.Math.Content.6.NS.C.7 ;
    prov:wasQuotedFrom <http://www.corestandards.org/Math/Content/6/NS/c/> .

:CCSS.Math.Content.6.NS.C.7.d rdf:type owl:Class ;
    rdfs:subClassOf :CCSS.Math.Content.6.NS.C.7 ;
    prov:wasQuotedFrom <http://www.corestandards.org/Math/Content/6/NS/d/> .

:CCSS.Math.Content.6.EE rdf:type owl:Class ;
    rdfs:subClassOf :CCSS.Math.Content.6 ;
    rdfs:label "Expressions & Equations"^^xsd:string ;
    prov:wasQuotedFrom <http://www.corestandards.org/Math/Content/6/EE/> .

:CCSS.Math.Content.6.EE.A rdf:type owl:Class ;
    rdfs:subClassOf :CCSS.Math.Content.6.EE ;
    rdfs:label "Expressions & Equations"^^xsd:string ;
    prov:wasQuotedFrom <http://www.corestandards.org/Math/Content/6/EE/> .

:CCSS.Math.Content.6.EE.A.1 rdf:type owl:Class ;
    rdfs:subClassOf :CCSS.Math.Content.6.EE.A ;
    prov:wasQuotedFrom <http://www.corestandards.org/Math/Content/6/EE/1/> ;
    rdfs:label "English Language Arts Standards - Anchor Standards - College and Career Readiness Anchor Standards for Language - 1"^^xsd:string ;
    rdfs:comment "Demonstrate command of the conventions of standard English grammar and usage when writing or speaking."^^xsd:string .

:CCSS.Math.Content.6.EE.A.2 rdf:type owl:Class ;
    rdfs:subClassOf :CCSS.Math.Content.6.EE.A ;
    prov:wasQuotedFrom <http://www.corestandards.org/Math/Content/6/EE/2/> ;
    rdfs:label "English Language Arts Standards - Anchor Standards - College and Career Readiness Anchor Standards for Language - 2"^^xsd:string ;
    rdfs:comment "Demonstrate command of the conventions of standard English capitalization, punctuation, and spelling when writing."^^xsd:string .

:CCSS.Math.Content.6.EE.A.3 rdf:type owl:Class ;
    rdfs:subClassOf :CCSS.Math.Content.6.EE.A ;
    prov:wasQuotedFrom <http://www.corestandards.org/Math/Content/6/EE/3/> ;
    rdfs:label "English Language Arts Standards - Anchor Standards - College and Career Readiness Anchor Standards for Language - 3"^^xsd:string ;
    rdfs:comment "Apply knowledge of language to understand how language functions in different contexts, to make effective choices for meaning or style, and to comprehend more fully when reading or listening. "^^xsd:string .

:CCSS.Math.Content.6.EE.A.4 rdf:type owl:Class ;
    rdfs:subClassOf :CCSS.Math.Content.6.EE.A ;
    prov:wasQuotedFrom <http://www.corestandards.org/Math/Content/6/EE/4/> ;
    rdfs:label "English Language Arts Standards - Anchor Standards - College and Career Readiness Anchor Standards for Language - 4"^^xsd:string ;
    rdfs:comment "Determine or clarify the meaning of unknown and multiple-meaning words and phrases by using context clues, analyzing meaningful word parts, and consulting general and specialized reference materials, as appropriate."^^xsd:string .

:CCSS.Math.Content.6.EE.B rdf:type owl:Class ;
    rdfs:subClassOf :CCSS.Math.Content.6.EE ;
    rdfs:label "Expressions & Equations"^^xsd:string ;
    prov:wasQuotedFrom <http://www.corestandards.org/Math/Content/6/EE/> .

:CCSS.Math.Content.6.EE.B.5 rdf:type owl:Class ;
    rdfs:subClassOf :CCSS.Math.Content.6.EE.B ;
    prov:wasQuotedFrom <http://www.corestandards.org/Math/Content/6/EE/5/> ;
    rdfs:label "English Language Arts Standards - Anchor Standards - College and Career Readiness Anchor Standards for Language - 5"^^xsd:string ;
    rdfs:comment "Demonstrate understanding of figurative language, word relationships, and nuances in word meanings."^^xsd:string .

:CCSS.Math.Content.6.EE.B.6 rdf:type owl:Class ;
    rdfs:subClassOf :CCSS.Math.Content.6.EE.B ;
    prov:wasQuotedFrom <http://www.corestandards.org/Math/Content/6/EE/6/> ;
    rdfs:label "English Language Arts Standards - Anchor Standards - College and Career Readiness Anchor Standards for Language - 6"^^xsd:string ;
    rdfs:comment "Acquire and use accurately a range of general academic and domain-specific words and phrases sufficient for reading, writing, speaking, and listening at the college and career readiness level; demonstrate independence in gathering vocabulary knowledge when encountering an unknown term important to comprehension or expression."^^xsd:string .

:CCSS.Math.Content.6.EE.B.7 rdf:type owl:Class ;
    rdfs:subClassOf :CCSS.Math.Content.6.EE.B ;
    prov:wasQuotedFrom <http://www.corestandards.org/Math/Content/6/EE/7/> ;
    rdfs:label "English Language Arts Standards - Anchor Standards - College and Career Readiness Anchor Standards for Reading - 7"^^xsd:string ;
    rdfs:comment "Integrate and evaluate content presented in diverse media and formats, including visually and quantitatively, as well as in words.1"^^xsd:string .

:CCSS.Math.Content.6.EE.B.8 rdf:type owl:Class ;
    rdfs:subClassOf :CCSS.Math.Content.6.EE.B ;
    prov:wasQuotedFrom <http://www.corestandards.org/Math/Content/6/EE/8/> ;
    rdfs:label "English Language Arts Standards - Anchor Standards - College and Career Readiness Anchor Standards for Reading - 8"^^xsd:string ;
    rdfs:comment "Delineate and evaluate the argument and specific claims in a text, including the validity of the reasoning as well as the relevance and sufficiency of the evidence."^^xsd:string .

:CCSS.Math.Content.6.EE.C rdf:type owl:Class ;
    rdfs:subClassOf :CCSS.Math.Content.6.EE ;
    rdfs:label "Expressions & Equations"^^xsd:string ;
    prov:wasQuotedFrom <http://www.corestandards.org/Math/Content/6/EE/> .

:CCSS.Math.Content.6.EE.C.9 rdf:type owl:Class ;
    rdfs:subClassOf :CCSS.Math.Content.6.EE.C ;
    prov:wasQuotedFrom <http://www.corestandards.org/Math/Content/6/EE/9/> ;
    rdfs:label "English Language Arts Standards - Anchor Standards - College and Career Readiness Anchor Standards for Reading - 9"^^xsd:string ;
    rdfs:comment "Analyze how two or more texts address similar themes or topics in order to build knowledge or to compare the approaches the authors take."^^xsd:string .

:CCSS.Math.Content.6.EE.A.2.a rdf:type owl:Class ;
    rdfs:subClassOf :CCSS.Math.Content.6.EE.A.2 ;
    prov:wasQuotedFrom <http://www.corestandards.org/Math/Content/6/EE/a/> .

:CCSS.Math.Content.6.EE.A.2.b rdf:type owl:Class ;
    rdfs:subClassOf :CCSS.Math.Content.6.EE.A.2 ;
    prov:wasQuotedFrom <http://www.corestandards.org/Math/Content/6/EE/b/> .

:CCSS.Math.Content.6.EE.A.2.c rdf:type owl:Class ;
    rdfs:subClassOf :CCSS.Math.Content.6.EE.A.2 ;
    prov:wasQuotedFrom <http://www.corestandards.org/Math/Content/6/EE/c/> .

:CCSS.Math.Content.6.G rdf:type owl:Class ;
    rdfs:subClassOf :CCSS.Math.Content.6 ;
    rdfs:label "Geometry"^^xsd:string ;
    prov:wasQuotedFrom <http://www.corestandards.org/Math/Content/6/G/> .

:CCSS.Math.Content.6.G.A rdf:type owl:Class ;
    rdfs:subClassOf :CCSS.Math.Content.6.G ;
    rdfs:label "Geometry"^^xsd:string ;
    prov:wasQuotedFrom <http://www.corestandards.org/Math/Content/6/G/> .

:CCSS.Math.Content.6.G.A.1 rdf:type owl:Class ;
    rdfs:subClassOf :CCSS.Math.Content.6.G.A ;
    prov:wasQuotedFrom <http://www.corestandards.org/Math/Content/6/G/1/> ;
    rdfs:label "English Language Arts Standards - Anchor Standards - College and Career Readiness Anchor Standards for Language - 1"^^xsd:string ;
    rdfs:comment "Demonstrate command of the conventions of standard English grammar and usage when writing or speaking."^^xsd:string .

:CCSS.Math.Content.6.G.A.2 rdf:type owl:Class ;
    rdfs:subClassOf :CCSS.Math.Content.6.G.A ;
    prov:wasQuotedFrom <http://www.corestandards.org/Math/Content/6/G/2/> ;
    rdfs:label "English Language Arts Standards - Anchor Standards - College and Career Readiness Anchor Standards for Language - 2"^^xsd:string ;
    rdfs:comment "Demonstrate command of the conventions of standard English capitalization, punctuation, and spelling when writing."^^xsd:string .

:CCSS.Math.Content.6.G.A.3 rdf:type owl:Class ;
    rdfs:subClassOf :CCSS.Math.Content.6.G.A ;
    prov:wasQuotedFrom <http://www.corestandards.org/Math/Content/6/G/3/> ;
    rdfs:label "English Language Arts Standards - Anchor Standards - College and Career Readiness Anchor Standards for Language - 3"^^xsd:string ;
    rdfs:comment "Apply knowledge of language to understand how language functions in different contexts, to make effective choices for meaning or style, and to comprehend more fully when reading or listening. "^^xsd:string .

:CCSS.Math.Content.6.G.A.4 rdf:type owl:Class ;
    rdfs:subClassOf :CCSS.Math.Content.6.G.A ;
    prov:wasQuotedFrom <http://www.corestandards.org/Math/Content/6/G/4/> ;
    rdfs:label "English Language Arts Standards - Anchor Standards - College and Career Readiness Anchor Standards for Language - 4"^^xsd:string ;
    rdfs:comment "Determine or clarify the meaning of unknown and multiple-meaning words and phrases by using context clues, analyzing meaningful word parts, and consulting general and specialized reference materials, as appropriate."^^xsd:string .

:CCSS.Math.Content.6.SP rdf:type owl:Class ;
    rdfs:subClassOf :CCSS.Math.Content.6 ;
    rdfs:label "Statistics & Probability"^^xsd:string ;
    prov:wasQuotedFrom <http://www.corestandards.org/Math/Content/6/SP/> .

:CCSS.Math.Content.6.SP.A rdf:type owl:Class ;
    rdfs:subClassOf :CCSS.Math.Content.6.SP ;
    rdfs:label "Statistics & Probability"^^xsd:string ;
    prov:wasQuotedFrom <http://www.corestandards.org/Math/Content/6/SP/> .

:CCSS.Math.Content.6.SP.A.1 rdf:type owl:Class ;
    rdfs:subClassOf :CCSS.Math.Content.6.SP.A ;
    prov:wasQuotedFrom <http://www.corestandards.org/Math/Content/6/SP/1/> ;
    rdfs:label "English Language Arts Standards - Anchor Standards - College and Career Readiness Anchor Standards for Language - 1"^^xsd:string ;
    rdfs:comment "Demonstrate command of the conventions of standard English grammar and usage when writing or speaking."^^xsd:string .

:CCSS.Math.Content.6.SP.A.2 rdf:type owl:Class ;
    rdfs:subClassOf :CCSS.Math.Content.6.SP.A ;
    prov:wasQuotedFrom <http://www.corestandards.org/Math/Content/6/SP/2/> ;
    rdfs:label "English Language Arts Standards - Anchor Standards - College and Career Readiness Anchor Standards for Language - 2"^^xsd:string ;
    rdfs:comment "Demonstrate command of the conventions of standard English capitalization, punctuation, and spelling when writing."^^xsd:string .

:CCSS.Math.Content.6.SP.A.3 rdf:type owl:Class ;
    rdfs:subClassOf :CCSS.Math.Content.6.SP.A ;
    prov:wasQuotedFrom <http://www.corestandards.org/Math/Content/6/SP/3/> ;
    rdfs:label "English Language Arts Standards - Anchor Standards - College and Career Readiness Anchor Standards for Language - 3"^^xsd:string ;
    rdfs:comment "Apply knowledge of language to understand how language functions in different contexts, to make effective choices for meaning or style, and to comprehend more fully when reading or listening. "^^xsd:string .

:CCSS.Math.Content.6.SP.B rdf:type owl:Class ;
    rdfs:subClassOf :CCSS.Math.Content.6.SP ;
    rdfs:label "Statistics & Probability"^^xsd:string ;
    prov:wasQuotedFrom <http://www.corestandards.org/Math/Content/6/SP/> .

:CCSS.Math.Content.6.SP.B.4 rdf:type owl:Class ;
    rdfs:subClassOf :CCSS.Math.Content.6.SP.B ;
    prov:wasQuotedFrom <http://www.corestandards.org/Math/Content/6/SP/4/> ;
    rdfs:label "English Language Arts Standards - Anchor Standards - College and Career Readiness Anchor Standards for Language - 4"^^xsd:string ;
    rdfs:comment "Determine or clarify the meaning of unknown and multiple-meaning words and phrases by using context clues, analyzing meaningful word parts, and consulting general and specialized reference materials, as appropriate."^^xsd:string .

:CCSS.Math.Content.6.SP.B.5 rdf:type owl:Class ;
    rdfs:subClassOf :CCSS.Math.Content.6.SP.B ;
    prov:wasQuotedFrom <http://www.corestandards.org/Math/Content/6/SP/5/> ;
    rdfs:label "English Language Arts Standards - Anchor Standards - College and Career Readiness Anchor Standards for Language - 5"^^xsd:string ;
    rdfs:comment "Demonstrate understanding of figurative language, word relationships, and nuances in word meanings."^^xsd:string .

:CCSS.Math.Content.6.SP.B.5.a rdf:type owl:Class ;
    rdfs:subClassOf :CCSS.Math.Content.6.SP.B.5 ;
    prov:wasQuotedFrom <http://www.corestandards.org/Math/Content/6/SP/a/> .

:CCSS.Math.Content.6.SP.B.5.b rdf:type owl:Class ;
    rdfs:subClassOf :CCSS.Math.Content.6.SP.B.5 ;
    prov:wasQuotedFrom <http://www.corestandards.org/Math/Content/6/SP/b/> .

:CCSS.Math.Content.6.SP.B.5.c rdf:type owl:Class ;
    rdfs:subClassOf :CCSS.Math.Content.6.SP.B.5 ;
    prov:wasQuotedFrom <http://www.corestandards.org/Math/Content/6/SP/c/> .

:CCSS.Math.Content.6.SP.B.5.d rdf:type owl:Class ;
    rdfs:subClassOf :CCSS.Math.Content.6.SP.B.5 ;
    prov:wasQuotedFrom <http://www.corestandards.org/Math/Content/6/SP/d/> .

:CCSS.Math.Content.7 rdf:type owl:Class ;
    rdfs:subClassOf :CCSS.Math.Content ;
    prov:wasQuotedFrom <http://www.corestandards.org/Math/Content/7/> .

:CCSS.Math.Content.7.RP rdf:type owl:Class ;
    rdfs:subClassOf :CCSS.Math.Content.7 ;
    rdfs:label "Ratios & Proportional Relationships"^^xsd:string ;
    prov:wasQuotedFrom <http://www.corestandards.org/Math/Content/7/RP/> .

:CCSS.Math.Content.7.RP.A rdf:type owl:Class ;
    rdfs:subClassOf :CCSS.Math.Content.7.RP ;
    rdfs:label "Ratios & Proportional Relationships"^^xsd:string ;
    prov:wasQuotedFrom <http://www.corestandards.org/Math/Content/7/RP/> .

:CCSS.Math.Content.7.RP.A.1 rdf:type owl:Class ;
    rdfs:subClassOf :CCSS.Math.Content.7.RP.A ;
    prov:wasQuotedFrom <http://www.corestandards.org/Math/Content/7/RP/1/> ;
    rdfs:label "English Language Arts Standards - Anchor Standards - College and Career Readiness Anchor Standards for Language - 1"^^xsd:string ;
    rdfs:comment "Demonstrate command of the conventions of standard English grammar and usage when writing or speaking."^^xsd:string .

:CCSS.Math.Content.7.RP.A.2 rdf:type owl:Class ;
    rdfs:subClassOf :CCSS.Math.Content.7.RP.A ;
    prov:wasQuotedFrom <http://www.corestandards.org/Math/Content/7/RP/2/> ;
    rdfs:label "English Language Arts Standards - Anchor Standards - College and Career Readiness Anchor Standards for Language - 2"^^xsd:string ;
    rdfs:comment "Demonstrate command of the conventions of standard English capitalization, punctuation, and spelling when writing."^^xsd:string .

:CCSS.Math.Content.7.RP.A.3 rdf:type owl:Class ;
    rdfs:subClassOf :CCSS.Math.Content.7.RP.A ;
    prov:wasQuotedFrom <http://www.corestandards.org/Math/Content/7/RP/3/> ;
    rdfs:label "English Language Arts Standards - Anchor Standards - College and Career Readiness Anchor Standards for Language - 3"^^xsd:string ;
    rdfs:comment "Apply knowledge of language to understand how language functions in different contexts, to make effective choices for meaning or style, and to comprehend more fully when reading or listening. "^^xsd:string .

:CCSS.Math.Content.7.RP.A.2.a rdf:type owl:Class ;
    rdfs:subClassOf :CCSS.Math.Content.7.RP.A.2 ;
    prov:wasQuotedFrom <http://www.corestandards.org/Math/Content/7/RP/a/> .

:CCSS.Math.Content.7.RP.A.2.b rdf:type owl:Class ;
    rdfs:subClassOf :CCSS.Math.Content.7.RP.A.2 ;
    prov:wasQuotedFrom <http://www.corestandards.org/Math/Content/7/RP/b/> .

:CCSS.Math.Content.7.RP.A.2.c rdf:type owl:Class ;
    rdfs:subClassOf :CCSS.Math.Content.7.RP.A.2 ;
    prov:wasQuotedFrom <http://www.corestandards.org/Math/Content/7/RP/c/> .

:CCSS.Math.Content.7.RP.A.2.d rdf:type owl:Class ;
    rdfs:subClassOf :CCSS.Math.Content.7.RP.A.2 ;
    prov:wasQuotedFrom <http://www.corestandards.org/Math/Content/7/RP/d/> .

:CCSS.Math.Content.7.NS rdf:type owl:Class ;
    rdfs:subClassOf :CCSS.Math.Content.7 ;
    rdfs:label "The Number System"^^xsd:string ;
    prov:wasQuotedFrom <http://www.corestandards.org/Math/Content/7/NS/> .

:CCSS.Math.Content.7.NS.A rdf:type owl:Class ;
    rdfs:subClassOf :CCSS.Math.Content.7.NS ;
    rdfs:label "The Number System"^^xsd:string ;
    prov:wasQuotedFrom <http://www.corestandards.org/Math/Content/7/NS/> .

:CCSS.Math.Content.7.NS.A.1 rdf:type owl:Class ;
    rdfs:subClassOf :CCSS.Math.Content.7.NS.A ;
    prov:wasQuotedFrom <http://www.corestandards.org/Math/Content/7/NS/1/> ;
    rdfs:label "English Language Arts Standards - Anchor Standards - College and Career Readiness Anchor Standards for Language - 1"^^xsd:string ;
    rdfs:comment "Demonstrate command of the conventions of standard English grammar and usage when writing or speaking."^^xsd:string .

:CCSS.Math.Content.7.NS.A.2 rdf:type owl:Class ;
    rdfs:subClassOf :CCSS.Math.Content.7.NS.A ;
    prov:wasQuotedFrom <http://www.corestandards.org/Math/Content/7/NS/2/> ;
    rdfs:label "English Language Arts Standards - Anchor Standards - College and Career Readiness Anchor Standards for Language - 2"^^xsd:string ;
    rdfs:comment "Demonstrate command of the conventions of standard English capitalization, punctuation, and spelling when writing."^^xsd:string .

:CCSS.Math.Content.7.NS.A.3 rdf:type owl:Class ;
    rdfs:subClassOf :CCSS.Math.Content.7.NS.A ;
    prov:wasQuotedFrom <http://www.corestandards.org/Math/Content/7/NS/3/> ;
    rdfs:label "English Language Arts Standards - Anchor Standards - College and Career Readiness Anchor Standards for Language - 3"^^xsd:string ;
    rdfs:comment "Apply knowledge of language to understand how language functions in different contexts, to make effective choices for meaning or style, and to comprehend more fully when reading or listening. "^^xsd:string .

:CCSS.Math.Content.7.NS.A.1.a rdf:type owl:Class ;
    rdfs:subClassOf :CCSS.Math.Content.7.NS.A.1 ;
    prov:wasQuotedFrom <http://www.corestandards.org/Math/Content/7/NS/a/> .

:CCSS.Math.Content.7.NS.A.1.b rdf:type owl:Class ;
    rdfs:subClassOf :CCSS.Math.Content.7.NS.A.1 ;
    prov:wasQuotedFrom <http://www.corestandards.org/Math/Content/7/NS/b/> .

:CCSS.Math.Content.7.NS.A.1.c rdf:type owl:Class ;
    rdfs:subClassOf :CCSS.Math.Content.7.NS.A.1 ;
    prov:wasQuotedFrom <http://www.corestandards.org/Math/Content/7/NS/c/> .

:CCSS.Math.Content.7.NS.A.1.d rdf:type owl:Class ;
    rdfs:subClassOf :CCSS.Math.Content.7.NS.A.1 ;
    prov:wasQuotedFrom <http://www.corestandards.org/Math/Content/7/NS/d/> .

:CCSS.Math.Content.7.NS.A.2.a rdf:type owl:Class ;
    rdfs:subClassOf :CCSS.Math.Content.7.NS.A.2 ;
    prov:wasQuotedFrom <http://www.corestandards.org/Math/Content/7/NS/a/> .

:CCSS.Math.Content.7.NS.A.2.b rdf:type owl:Class ;
    rdfs:subClassOf :CCSS.Math.Content.7.NS.A.2 ;
    prov:wasQuotedFrom <http://www.corestandards.org/Math/Content/7/NS/b/> .

:CCSS.Math.Content.7.NS.A.2.c rdf:type owl:Class ;
    rdfs:subClassOf :CCSS.Math.Content.7.NS.A.2 ;
    prov:wasQuotedFrom <http://www.corestandards.org/Math/Content/7/NS/c/> .

:CCSS.Math.Content.7.NS.A.2.d rdf:type owl:Class ;
    rdfs:subClassOf :CCSS.Math.Content.7.NS.A.2 ;
    prov:wasQuotedFrom <http://www.corestandards.org/Math/Content/7/NS/d/> .

:CCSS.Math.Content.7.EE rdf:type owl:Class ;
    rdfs:subClassOf :CCSS.Math.Content.7 ;
    rdfs:label "Expressions & Equations"^^xsd:string ;
    prov:wasQuotedFrom <http://www.corestandards.org/Math/Content/7/EE/> .

:CCSS.Math.Content.7.EE.A rdf:type owl:Class ;
    rdfs:subClassOf :CCSS.Math.Content.7.EE ;
    rdfs:label "Expressions & Equations"^^xsd:string ;
    prov:wasQuotedFrom <http://www.corestandards.org/Math/Content/7/EE/> .

:CCSS.Math.Content.7.EE.A.1 rdf:type owl:Class ;
    rdfs:subClassOf :CCSS.Math.Content.7.EE.A ;
    prov:wasQuotedFrom <http://www.corestandards.org/Math/Content/7/EE/1/> ;
    rdfs:label "English Language Arts Standards - Anchor Standards - College and Career Readiness Anchor Standards for Language - 1"^^xsd:string ;
    rdfs:comment "Demonstrate command of the conventions of standard English grammar and usage when writing or speaking."^^xsd:string .

:CCSS.Math.Content.7.EE.A.2 rdf:type owl:Class ;
    rdfs:subClassOf :CCSS.Math.Content.7.EE.A ;
    prov:wasQuotedFrom <http://www.corestandards.org/Math/Content/7/EE/2/> ;
    rdfs:label "English Language Arts Standards - Anchor Standards - College and Career Readiness Anchor Standards for Language - 2"^^xsd:string ;
    rdfs:comment "Demonstrate command of the conventions of standard English capitalization, punctuation, and spelling when writing."^^xsd:string .

:CCSS.Math.Content.7.EE.B rdf:type owl:Class ;
    rdfs:subClassOf :CCSS.Math.Content.7.EE ;
    rdfs:label "Expressions & Equations"^^xsd:string ;
    prov:wasQuotedFrom <http://www.corestandards.org/Math/Content/7/EE/> .

:CCSS.Math.Content.7.EE.B.3 rdf:type owl:Class ;
    rdfs:subClassOf :CCSS.Math.Content.7.EE.B ;
    prov:wasQuotedFrom <http://www.corestandards.org/Math/Content/7/EE/3/> ;
    rdfs:label "English Language Arts Standards - Anchor Standards - College and Career Readiness Anchor Standards for Language - 3"^^xsd:string ;
    rdfs:comment "Apply knowledge of language to understand how language functions in different contexts, to make effective choices for meaning or style, and to comprehend more fully when reading or listening. "^^xsd:string .

:CCSS.Math.Content.7.EE.B.4 rdf:type owl:Class ;
    rdfs:subClassOf :CCSS.Math.Content.7.EE.B ;
    prov:wasQuotedFrom <http://www.corestandards.org/Math/Content/7/EE/4/> ;
    rdfs:label "English Language Arts Standards - Anchor Standards - College and Career Readiness Anchor Standards for Language - 4"^^xsd:string ;
    rdfs:comment "Determine or clarify the meaning of unknown and multiple-meaning words and phrases by using context clues, analyzing meaningful word parts, and consulting general and specialized reference materials, as appropriate."^^xsd:string .

:CCSS.Math.Content.7.EE.B.4.a rdf:type owl:Class ;
    rdfs:subClassOf :CCSS.Math.Content.7.EE.B.4 ;
    prov:wasQuotedFrom <http://www.corestandards.org/Math/Content/7/EE/a/> .

:CCSS.Math.Content.7.EE.B.4.b rdf:type owl:Class ;
    rdfs:subClassOf :CCSS.Math.Content.7.EE.B.4 ;
    prov:wasQuotedFrom <http://www.corestandards.org/Math/Content/7/EE/b/> .

:CCSS.Math.Content.7.G rdf:type owl:Class ;
    rdfs:subClassOf :CCSS.Math.Content.7 ;
    rdfs:label "Geometry"^^xsd:string ;
    prov:wasQuotedFrom <http://www.corestandards.org/Math/Content/7/G/> .

:CCSS.Math.Content.7.G.A rdf:type owl:Class ;
    rdfs:subClassOf :CCSS.Math.Content.7.G ;
    rdfs:label "Geometry"^^xsd:string ;
    prov:wasQuotedFrom <http://www.corestandards.org/Math/Content/7/G/> .

:CCSS.Math.Content.7.G.A.1 rdf:type owl:Class ;
    rdfs:subClassOf :CCSS.Math.Content.7.G.A ;
    prov:wasQuotedFrom <http://www.corestandards.org/Math/Content/7/G/1/> ;
    rdfs:label "English Language Arts Standards - Anchor Standards - College and Career Readiness Anchor Standards for Language - 1"^^xsd:string ;
    rdfs:comment "Demonstrate command of the conventions of standard English grammar and usage when writing or speaking."^^xsd:string .

:CCSS.Math.Content.7.G.A.2 rdf:type owl:Class ;
    rdfs:subClassOf :CCSS.Math.Content.7.G.A ;
    prov:wasQuotedFrom <http://www.corestandards.org/Math/Content/7/G/2/> ;
    rdfs:label "English Language Arts Standards - Anchor Standards - College and Career Readiness Anchor Standards for Language - 2"^^xsd:string ;
    rdfs:comment "Demonstrate command of the conventions of standard English capitalization, punctuation, and spelling when writing."^^xsd:string .

:CCSS.Math.Content.7.G.A.3 rdf:type owl:Class ;
    rdfs:subClassOf :CCSS.Math.Content.7.G.A ;
    prov:wasQuotedFrom <http://www.corestandards.org/Math/Content/7/G/3/> ;
    rdfs:label "English Language Arts Standards - Anchor Standards - College and Career Readiness Anchor Standards for Language - 3"^^xsd:string ;
    rdfs:comment "Apply knowledge of language to understand how language functions in different contexts, to make effective choices for meaning or style, and to comprehend more fully when reading or listening. "^^xsd:string .

:CCSS.Math.Content.7.G.B rdf:type owl:Class ;
    rdfs:subClassOf :CCSS.Math.Content.7.G ;
    rdfs:label "Geometry"^^xsd:string ;
    prov:wasQuotedFrom <http://www.corestandards.org/Math/Content/7/G/> .

:CCSS.Math.Content.7.G.B.4 rdf:type owl:Class ;
    rdfs:subClassOf :CCSS.Math.Content.7.G.B ;
    prov:wasQuotedFrom <http://www.corestandards.org/Math/Content/7/G/4/> ;
    rdfs:label "English Language Arts Standards - Anchor Standards - College and Career Readiness Anchor Standards for Language - 4"^^xsd:string ;
    rdfs:comment "Determine or clarify the meaning of unknown and multiple-meaning words and phrases by using context clues, analyzing meaningful word parts, and consulting general and specialized reference materials, as appropriate."^^xsd:string .

:CCSS.Math.Content.7.G.B.5 rdf:type owl:Class ;
    rdfs:subClassOf :CCSS.Math.Content.7.G.B ;
    prov:wasQuotedFrom <http://www.corestandards.org/Math/Content/7/G/5/> ;
    rdfs:label "English Language Arts Standards - Anchor Standards - College and Career Readiness Anchor Standards for Language - 5"^^xsd:string ;
    rdfs:comment "Demonstrate understanding of figurative language, word relationships, and nuances in word meanings."^^xsd:string .

:CCSS.Math.Content.7.G.B.6 rdf:type owl:Class ;
    rdfs:subClassOf :CCSS.Math.Content.7.G.B ;
    prov:wasQuotedFrom <http://www.corestandards.org/Math/Content/7/G/6/> ;
    rdfs:label "English Language Arts Standards - Anchor Standards - College and Career Readiness Anchor Standards for Language - 6"^^xsd:string ;
    rdfs:comment "Acquire and use accurately a range of general academic and domain-specific words and phrases sufficient for reading, writing, speaking, and listening at the college and career readiness level; demonstrate independence in gathering vocabulary knowledge when encountering an unknown term important to comprehension or expression."^^xsd:string .

:CCSS.Math.Content.7.SP rdf:type owl:Class ;
    rdfs:subClassOf :CCSS.Math.Content.7 ;
    rdfs:label "Statistics & Probability"^^xsd:string ;
    prov:wasQuotedFrom <http://www.corestandards.org/Math/Content/7/SP/> .

:CCSS.Math.Content.7.SP.A rdf:type owl:Class ;
    rdfs:subClassOf :CCSS.Math.Content.7.SP ;
    rdfs:label "Statistics & Probability"^^xsd:string ;
    prov:wasQuotedFrom <http://www.corestandards.org/Math/Content/7/SP/> .

:CCSS.Math.Content.7.SP.A rdf:type owl:Class ;
    rdfs:label "Statistics & Probability"^^xsd:string ;
    prov:wasQuotedFrom <http://www.corestandards.org/Math/Content/7/SP/> .

:CCSS.Math.Content.7.SP.A.1 rdf:type owl:Class ;
    rdfs:subClassOf :CCSS.Math.Content.7.SP.A ;
    prov:wasQuotedFrom <http://www.corestandards.org/Math/Content/7/SP/1/> ;
    rdfs:label "English Language Arts Standards - Anchor Standards - College and Career Readiness Anchor Standards for Language - 1"^^xsd:string ;
    rdfs:comment "Demonstrate command of the conventions of standard English grammar and usage when writing or speaking."^^xsd:string .

:CCSS.Math.Content.7.SP.A.2 rdf:type owl:Class ;
    rdfs:subClassOf :CCSS.Math.Content.7.SP.A ;
    prov:wasQuotedFrom <http://www.corestandards.org/Math/Content/7/SP/2/> ;
    rdfs:label "English Language Arts Standards - Anchor Standards - College and Career Readiness Anchor Standards for Language - 2"^^xsd:string ;
    rdfs:comment "Demonstrate command of the conventions of standard English capitalization, punctuation, and spelling when writing."^^xsd:string .

:CCSS.Math.Content.7.SP.B rdf:type owl:Class ;
    rdfs:subClassOf :CCSS.Math.Content.7.SP ;
    rdfs:label "Statistics & Probability"^^xsd:string ;
    prov:wasQuotedFrom <http://www.corestandards.org/Math/Content/7/SP/> .

:CCSS.Math.Content.7.SP.B.3 rdf:type owl:Class ;
    rdfs:subClassOf :CCSS.Math.Content.7.SP.B ;
    prov:wasQuotedFrom <http://www.corestandards.org/Math/Content/7/SP/3/> ;
    rdfs:label "English Language Arts Standards - Anchor Standards - College and Career Readiness Anchor Standards for Language - 3"^^xsd:string ;
    rdfs:comment "Apply knowledge of language to understand how language functions in different contexts, to make effective choices for meaning or style, and to comprehend more fully when reading or listening. "^^xsd:string .

:CCSS.Math.Content.7.SP.B.4 rdf:type owl:Class ;
    rdfs:subClassOf :CCSS.Math.Content.7.SP.B ;
    prov:wasQuotedFrom <http://www.corestandards.org/Math/Content/7/SP/4/> ;
    rdfs:label "English Language Arts Standards - Anchor Standards - College and Career Readiness Anchor Standards for Language - 4"^^xsd:string ;
    rdfs:comment "Determine or clarify the meaning of unknown and multiple-meaning words and phrases by using context clues, analyzing meaningful word parts, and consulting general and specialized reference materials, as appropriate."^^xsd:string .

:CCSS.Math.Content.7.SP.C rdf:type owl:Class ;
    rdfs:subClassOf :CCSS.Math.Content.7.SP ;
    rdfs:label "Statistics & Probability"^^xsd:string ;
    prov:wasQuotedFrom <http://www.corestandards.org/Math/Content/7/SP/> .

:CCSS.Math.Content.7.SP.C.5 rdf:type owl:Class ;
    rdfs:subClassOf :CCSS.Math.Content.7.SP.C ;
    prov:wasQuotedFrom <http://www.corestandards.org/Math/Content/7/SP/5/> ;
    rdfs:label "English Language Arts Standards - Anchor Standards - College and Career Readiness Anchor Standards for Language - 5"^^xsd:string ;
    rdfs:comment "Demonstrate understanding of figurative language, word relationships, and nuances in word meanings."^^xsd:string .

:CCSS.Math.Content.7.SP.C.6 rdf:type owl:Class ;
    rdfs:subClassOf :CCSS.Math.Content.7.SP.C ;
    prov:wasQuotedFrom <http://www.corestandards.org/Math/Content/7/SP/6/> ;
    rdfs:label "English Language Arts Standards - Anchor Standards - College and Career Readiness Anchor Standards for Language - 6"^^xsd:string ;
    rdfs:comment "Acquire and use accurately a range of general academic and domain-specific words and phrases sufficient for reading, writing, speaking, and listening at the college and career readiness level; demonstrate independence in gathering vocabulary knowledge when encountering an unknown term important to comprehension or expression."^^xsd:string .

:CCSS.Math.Content.7.SP.C.7 rdf:type owl:Class ;
    rdfs:subClassOf :CCSS.Math.Content.7.SP.C ;
    prov:wasQuotedFrom <http://www.corestandards.org/Math/Content/7/SP/7/> ;
    rdfs:label "English Language Arts Standards - Anchor Standards - College and Career Readiness Anchor Standards for Reading - 7"^^xsd:string ;
    rdfs:comment "Integrate and evaluate content presented in diverse media and formats, including visually and quantitatively, as well as in words.1"^^xsd:string .

:CCSS.Math.Content.7.SP.C.8 rdf:type owl:Class ;
    rdfs:subClassOf :CCSS.Math.Content.7.SP.C ;
    prov:wasQuotedFrom <http://www.corestandards.org/Math/Content/7/SP/8/> ;
    rdfs:label "English Language Arts Standards - Anchor Standards - College and Career Readiness Anchor Standards for Reading - 8"^^xsd:string ;
    rdfs:comment "Delineate and evaluate the argument and specific claims in a text, including the validity of the reasoning as well as the relevance and sufficiency of the evidence."^^xsd:string .

:CCSS.Math.Content.7.SP.C.7.a rdf:type owl:Class ;
    rdfs:subClassOf :CCSS.Math.Content.7.SP.C.7 ;
    prov:wasQuotedFrom <http://www.corestandards.org/Math/Content/7/SP/a/> .

:CCSS.Math.Content.7.SP.C.7.b rdf:type owl:Class ;
    rdfs:subClassOf :CCSS.Math.Content.7.SP.C.7 ;
    prov:wasQuotedFrom <http://www.corestandards.org/Math/Content/7/SP/b/> .

:CCSS.Math.Content.7.SP.C.8.a rdf:type owl:Class ;
    rdfs:subClassOf :CCSS.Math.Content.7.SP.C.8 ;
    prov:wasQuotedFrom <http://www.corestandards.org/Math/Content/7/SP/a/> .

:CCSS.Math.Content.7.SP.C.8.b rdf:type owl:Class ;
    rdfs:subClassOf :CCSS.Math.Content.7.SP.C.8 ;
    prov:wasQuotedFrom <http://www.corestandards.org/Math/Content/7/SP/b/> .

:CCSS.Math.Content.7.SP.C.8.c rdf:type owl:Class ;
    rdfs:subClassOf :CCSS.Math.Content.7.SP.C.8 ;
    prov:wasQuotedFrom <http://www.corestandards.org/Math/Content/7/SP/c/> .

:CCSS.Math.Content.8 rdf:type owl:Class ;
    rdfs:subClassOf :CCSS.Math.Content ;
    prov:wasQuotedFrom <http://www.corestandards.org/Math/Content/8/> .

:CCSS.Math.Content.8.NS rdf:type owl:Class ;
    rdfs:subClassOf :CCSS.Math.Content.8 ;
    rdfs:label "The Number System"^^xsd:string ;
    prov:wasQuotedFrom <http://www.corestandards.org/Math/Content/8/NS/> .

:CCSS.Math.Content.8.NS.A rdf:type owl:Class ;
    rdfs:subClassOf :CCSS.Math.Content.8.NS ;
    rdfs:label "The Number System"^^xsd:string ;
    prov:wasQuotedFrom <http://www.corestandards.org/Math/Content/8/NS/> .

:CCSS.Math.Content.8.NS.A.1 rdf:type owl:Class ;
    rdfs:subClassOf :CCSS.Math.Content.8.NS.A ;
    prov:wasQuotedFrom <http://www.corestandards.org/Math/Content/8/NS/1/> ;
    rdfs:label "English Language Arts Standards - Anchor Standards - College and Career Readiness Anchor Standards for Language - 1"^^xsd:string ;
    rdfs:comment "Demonstrate command of the conventions of standard English grammar and usage when writing or speaking."^^xsd:string .

:CCSS.Math.Content.8.NS.A.2 rdf:type owl:Class ;
    rdfs:subClassOf :CCSS.Math.Content.8.NS.A ;
    prov:wasQuotedFrom <http://www.corestandards.org/Math/Content/8/NS/2/> ;
    rdfs:label "English Language Arts Standards - Anchor Standards - College and Career Readiness Anchor Standards for Language - 2"^^xsd:string ;
    rdfs:comment "Demonstrate command of the conventions of standard English capitalization, punctuation, and spelling when writing."^^xsd:string .

:CCSS.Math.Content.8.EE rdf:type owl:Class ;
    rdfs:subClassOf :CCSS.Math.Content.8 ;
    rdfs:label "Expressions & Equations"^^xsd:string ;
    prov:wasQuotedFrom <http://www.corestandards.org/Math/Content/8/EE/> .

:CCSS.Math.Content.8.EE.A rdf:type owl:Class ;
    rdfs:subClassOf :CCSS.Math.Content.8.EE ;
    rdfs:label "Expressions & Equations"^^xsd:string ;
    prov:wasQuotedFrom <http://www.corestandards.org/Math/Content/8/EE/> .

:CCSS.Math.Content.8.EE.A.1 rdf:type owl:Class ;
    rdfs:subClassOf :CCSS.Math.Content.8.EE.A ;
    prov:wasQuotedFrom <http://www.corestandards.org/Math/Content/8/EE/1/> ;
    rdfs:label "English Language Arts Standards - Anchor Standards - College and Career Readiness Anchor Standards for Language - 1"^^xsd:string ;
    rdfs:comment "Demonstrate command of the conventions of standard English grammar and usage when writing or speaking."^^xsd:string .

:CCSS.Math.Content.8.EE.A.2 rdf:type owl:Class ;
    rdfs:subClassOf :CCSS.Math.Content.8.EE.A ;
    prov:wasQuotedFrom <http://www.corestandards.org/Math/Content/8/EE/2/> ;
    rdfs:label "English Language Arts Standards - Anchor Standards - College and Career Readiness Anchor Standards for Language - 2"^^xsd:string ;
    rdfs:comment "Demonstrate command of the conventions of standard English capitalization, punctuation, and spelling when writing."^^xsd:string .

:CCSS.Math.Content.8.EE.A.3 rdf:type owl:Class ;
    rdfs:subClassOf :CCSS.Math.Content.8.EE.A ;
    prov:wasQuotedFrom <http://www.corestandards.org/Math/Content/8/EE/3/> ;
    rdfs:label "English Language Arts Standards - Anchor Standards - College and Career Readiness Anchor Standards for Language - 3"^^xsd:string ;
    rdfs:comment "Apply knowledge of language to understand how language functions in different contexts, to make effective choices for meaning or style, and to comprehend more fully when reading or listening. "^^xsd:string .

:CCSS.Math.Content.8.EE.A.4 rdf:type owl:Class ;
    rdfs:subClassOf :CCSS.Math.Content.8.EE.A ;
    prov:wasQuotedFrom <http://www.corestandards.org/Math/Content/8/EE/4/> ;
    rdfs:label "English Language Arts Standards - Anchor Standards - College and Career Readiness Anchor Standards for Language - 4"^^xsd:string ;
    rdfs:comment "Determine or clarify the meaning of unknown and multiple-meaning words and phrases by using context clues, analyzing meaningful word parts, and consulting general and specialized reference materials, as appropriate."^^xsd:string .

:CCSS.Math.Content.8.EE.B rdf:type owl:Class ;
    rdfs:subClassOf :CCSS.Math.Content.8.EE ;
    rdfs:label "Expressions & Equations"^^xsd:string ;
    prov:wasQuotedFrom <http://www.corestandards.org/Math/Content/8/EE/> .

:CCSS.Math.Content.8.EE.B.5 rdf:type owl:Class ;
    rdfs:subClassOf :CCSS.Math.Content.8.EE.B ;
    prov:wasQuotedFrom <http://www.corestandards.org/Math/Content/8/EE/5/> ;
    rdfs:label "English Language Arts Standards - Anchor Standards - College and Career Readiness Anchor Standards for Language - 5"^^xsd:string ;
    rdfs:comment "Demonstrate understanding of figurative language, word relationships, and nuances in word meanings."^^xsd:string .

:CCSS.Math.Content.8.EE.B.6 rdf:type owl:Class ;
    rdfs:subClassOf :CCSS.Math.Content.8.EE.B ;
    prov:wasQuotedFrom <http://www.corestandards.org/Math/Content/8/EE/6/> ;
    rdfs:label "English Language Arts Standards - Anchor Standards - College and Career Readiness Anchor Standards for Language - 6"^^xsd:string ;
    rdfs:comment "Acquire and use accurately a range of general academic and domain-specific words and phrases sufficient for reading, writing, speaking, and listening at the college and career readiness level; demonstrate independence in gathering vocabulary knowledge when encountering an unknown term important to comprehension or expression."^^xsd:string .

:CCSS.Math.Content.8.EE.C rdf:type owl:Class ;
    rdfs:subClassOf :CCSS.Math.Content.8.EE ;
    rdfs:label "Expressions & Equations"^^xsd:string ;
    prov:wasQuotedFrom <http://www.corestandards.org/Math/Content/8/EE/> .

:CCSS.Math.Content.8.EE.C.7 rdf:type owl:Class ;
    rdfs:subClassOf :CCSS.Math.Content.8.EE.C ;
    prov:wasQuotedFrom <http://www.corestandards.org/Math/Content/8/EE/7/> ;
    rdfs:label "English Language Arts Standards - Anchor Standards - College and Career Readiness Anchor Standards for Reading - 7"^^xsd:string ;
    rdfs:comment "Integrate and evaluate content presented in diverse media and formats, including visually and quantitatively, as well as in words.1"^^xsd:string .

:CCSS.Math.Content.8.EE.C.8 rdf:type owl:Class ;
    rdfs:subClassOf :CCSS.Math.Content.8.EE.C ;
    prov:wasQuotedFrom <http://www.corestandards.org/Math/Content/8/EE/8/> ;
    rdfs:label "English Language Arts Standards - Anchor Standards - College and Career Readiness Anchor Standards for Reading - 8"^^xsd:string ;
    rdfs:comment "Delineate and evaluate the argument and specific claims in a text, including the validity of the reasoning as well as the relevance and sufficiency of the evidence."^^xsd:string .

:CCSS.Math.Content.8.EE.C.7.a rdf:type owl:Class ;
    rdfs:subClassOf :CCSS.Math.Content.8.EE.C.7 ;
    prov:wasQuotedFrom <http://www.corestandards.org/Math/Content/8/EE/a/> .

:CCSS.Math.Content.8.EE.C.7.b rdf:type owl:Class ;
    rdfs:subClassOf :CCSS.Math.Content.8.EE.C.7 ;
    prov:wasQuotedFrom <http://www.corestandards.org/Math/Content/8/EE/b/> .

:CCSS.Math.Content.8.EE.C.8.a rdf:type owl:Class ;
    rdfs:subClassOf :CCSS.Math.Content.8.EE.C.8 ;
    prov:wasQuotedFrom <http://www.corestandards.org/Math/Content/8/EE/a/> .

:CCSS.Math.Content.8.EE.C.8.b rdf:type owl:Class ;
    rdfs:subClassOf :CCSS.Math.Content.8.EE.C.8 ;
    prov:wasQuotedFrom <http://www.corestandards.org/Math/Content/8/EE/b/> .

:CCSS.Math.Content.8.EE.C.8.c rdf:type owl:Class ;
    rdfs:subClassOf :CCSS.Math.Content.8.EE.C.8 ;
    prov:wasQuotedFrom <http://www.corestandards.org/Math/Content/8/EE/c/> .

:CCSS.Math.Content.8.F rdf:type owl:Class ;
    rdfs:subClassOf :CCSS.Math.Content.8 ;
    rdfs:label "Functions"^^xsd:string ;
    prov:wasQuotedFrom <http://www.corestandards.org/Math/Content/8/F/> .

:CCSS.Math.Content.8.F.A rdf:type owl:Class ;
    rdfs:subClassOf :CCSS.Math.Content.8.F ;
    rdfs:label "Functions"^^xsd:string ;
    prov:wasQuotedFrom <http://www.corestandards.org/Math/Content/8/F/> .

:CCSS.Math.Content.8.F.A.1 rdf:type owl:Class ;
    rdfs:subClassOf :CCSS.Math.Content.8.F.A ;
    prov:wasQuotedFrom <http://www.corestandards.org/Math/Content/8/F/1/> ;
    rdfs:label "English Language Arts Standards - Anchor Standards - College and Career Readiness Anchor Standards for Language - 1"^^xsd:string ;
    rdfs:comment "Demonstrate command of the conventions of standard English grammar and usage when writing or speaking."^^xsd:string .

:CCSS.Math.Content.8.F.A.2 rdf:type owl:Class ;
    rdfs:subClassOf :CCSS.Math.Content.8.F.A ;
    prov:wasQuotedFrom <http://www.corestandards.org/Math/Content/8/F/2/> ;
    rdfs:label "English Language Arts Standards - Anchor Standards - College and Career Readiness Anchor Standards for Language - 2"^^xsd:string ;
    rdfs:comment "Demonstrate command of the conventions of standard English capitalization, punctuation, and spelling when writing."^^xsd:string .

:CCSS.Math.Content.8.F.A.3 rdf:type owl:Class ;
    rdfs:subClassOf :CCSS.Math.Content.8.F.A ;
    prov:wasQuotedFrom <http://www.corestandards.org/Math/Content/8/F/3/> ;
    rdfs:label "English Language Arts Standards - Anchor Standards - College and Career Readiness Anchor Standards for Language - 3"^^xsd:string ;
    rdfs:comment "Apply knowledge of language to understand how language functions in different contexts, to make effective choices for meaning or style, and to comprehend more fully when reading or listening. "^^xsd:string .

:CCSS.Math.Content.8.F.B rdf:type owl:Class ;
    rdfs:subClassOf :CCSS.Math.Content.8.F ;
    rdfs:label "Functions"^^xsd:string ;
    prov:wasQuotedFrom <http://www.corestandards.org/Math/Content/8/F/> .

:CCSS.Math.Content.8.F.B.4 rdf:type owl:Class ;
    rdfs:subClassOf :CCSS.Math.Content.8.F.B ;
    prov:wasQuotedFrom <http://www.corestandards.org/Math/Content/8/F/4/> ;
    rdfs:label "English Language Arts Standards - Anchor Standards - College and Career Readiness Anchor Standards for Language - 4"^^xsd:string ;
    rdfs:comment "Determine or clarify the meaning of unknown and multiple-meaning words and phrases by using context clues, analyzing meaningful word parts, and consulting general and specialized reference materials, as appropriate."^^xsd:string .

:CCSS.Math.Content.8.F.B.5 rdf:type owl:Class ;
    rdfs:subClassOf :CCSS.Math.Content.8.F.B ;
    prov:wasQuotedFrom <http://www.corestandards.org/Math/Content/8/F/5/> ;
    rdfs:label "English Language Arts Standards - Anchor Standards - College and Career Readiness Anchor Standards for Language - 5"^^xsd:string ;
    rdfs:comment "Demonstrate understanding of figurative language, word relationships, and nuances in word meanings."^^xsd:string .

:CCSS.Math.Content.8.G rdf:type owl:Class ;
    rdfs:subClassOf :CCSS.Math.Content.8 ;
    rdfs:label "Geometry"^^xsd:string ;
    prov:wasQuotedFrom <http://www.corestandards.org/Math/Content/8/G/> .

:CCSS.Math.Content.8.G.A rdf:type owl:Class ;
    rdfs:subClassOf :CCSS.Math.Content.8.G ;
    rdfs:label "Geometry"^^xsd:string ;
    prov:wasQuotedFrom <http://www.corestandards.org/Math/Content/8/G/> .

:CCSS.Math.Content.8.G.A.1 rdf:type owl:Class ;
    rdfs:subClassOf :CCSS.Math.Content.8.G.A ;
    prov:wasQuotedFrom <http://www.corestandards.org/Math/Content/8/G/1/> ;
    rdfs:label "English Language Arts Standards - Anchor Standards - College and Career Readiness Anchor Standards for Language - 1"^^xsd:string ;
    rdfs:comment "Demonstrate command of the conventions of standard English grammar and usage when writing or speaking."^^xsd:string .

:CCSS.Math.Content.8.G.A.2 rdf:type owl:Class ;
    rdfs:subClassOf :CCSS.Math.Content.8.G.A ;
    prov:wasQuotedFrom <http://www.corestandards.org/Math/Content/8/G/2/> ;
    rdfs:label "English Language Arts Standards - Anchor Standards - College and Career Readiness Anchor Standards for Language - 2"^^xsd:string ;
    rdfs:comment "Demonstrate command of the conventions of standard English capitalization, punctuation, and spelling when writing."^^xsd:string .

:CCSS.Math.Content.8.G.A.3 rdf:type owl:Class ;
    rdfs:subClassOf :CCSS.Math.Content.8.G.A ;
    prov:wasQuotedFrom <http://www.corestandards.org/Math/Content/8/G/3/> ;
    rdfs:label "English Language Arts Standards - Anchor Standards - College and Career Readiness Anchor Standards for Language - 3"^^xsd:string ;
    rdfs:comment "Apply knowledge of language to understand how language functions in different contexts, to make effective choices for meaning or style, and to comprehend more fully when reading or listening. "^^xsd:string .

:CCSS.Math.Content.8.G.A.4 rdf:type owl:Class ;
    rdfs:subClassOf :CCSS.Math.Content.8.G.A ;
    prov:wasQuotedFrom <http://www.corestandards.org/Math/Content/8/G/4/> ;
    rdfs:label "English Language Arts Standards - Anchor Standards - College and Career Readiness Anchor Standards for Language - 4"^^xsd:string ;
    rdfs:comment "Determine or clarify the meaning of unknown and multiple-meaning words and phrases by using context clues, analyzing meaningful word parts, and consulting general and specialized reference materials, as appropriate."^^xsd:string .

:CCSS.Math.Content.8.G.A.5 rdf:type owl:Class ;
    rdfs:subClassOf :CCSS.Math.Content.8.G.A ;
    prov:wasQuotedFrom <http://www.corestandards.org/Math/Content/8/G/5/> ;
    rdfs:label "English Language Arts Standards - Anchor Standards - College and Career Readiness Anchor Standards for Language - 5"^^xsd:string ;
    rdfs:comment "Demonstrate understanding of figurative language, word relationships, and nuances in word meanings."^^xsd:string .

:CCSS.Math.Content.8.G.B rdf:type owl:Class ;
    rdfs:subClassOf :CCSS.Math.Content.8.G ;
    rdfs:label "Geometry"^^xsd:string ;
    prov:wasQuotedFrom <http://www.corestandards.org/Math/Content/8/G/> .

:CCSS.Math.Content.8.G.B.6 rdf:type owl:Class ;
    rdfs:subClassOf :CCSS.Math.Content.8.G.B ;
    prov:wasQuotedFrom <http://www.corestandards.org/Math/Content/8/G/6/> ;
    rdfs:label "English Language Arts Standards - Anchor Standards - College and Career Readiness Anchor Standards for Language - 6"^^xsd:string ;
    rdfs:comment "Acquire and use accurately a range of general academic and domain-specific words and phrases sufficient for reading, writing, speaking, and listening at the college and career readiness level; demonstrate independence in gathering vocabulary knowledge when encountering an unknown term important to comprehension or expression."^^xsd:string .

:CCSS.Math.Content.8.G.B.7 rdf:type owl:Class ;
    rdfs:subClassOf :CCSS.Math.Content.8.G.B ;
    prov:wasQuotedFrom <http://www.corestandards.org/Math/Content/8/G/7/> ;
    rdfs:label "English Language Arts Standards - Anchor Standards - College and Career Readiness Anchor Standards for Reading - 7"^^xsd:string ;
    rdfs:comment "Integrate and evaluate content presented in diverse media and formats, including visually and quantitatively, as well as in words.1"^^xsd:string .

:CCSS.Math.Content.8.G.B.8 rdf:type owl:Class ;
    rdfs:subClassOf :CCSS.Math.Content.8.G.B ;
    prov:wasQuotedFrom <http://www.corestandards.org/Math/Content/8/G/8/> ;
    rdfs:label "English Language Arts Standards - Anchor Standards - College and Career Readiness Anchor Standards for Reading - 8"^^xsd:string ;
    rdfs:comment "Delineate and evaluate the argument and specific claims in a text, including the validity of the reasoning as well as the relevance and sufficiency of the evidence."^^xsd:string .

:CCSS.Math.Content.8.G.C rdf:type owl:Class ;
    rdfs:subClassOf :CCSS.Math.Content.8.G ;
    rdfs:label "Geometry"^^xsd:string ;
    prov:wasQuotedFrom <http://www.corestandards.org/Math/Content/8/G/> .

:CCSS.Math.Content.8.G.C.9 rdf:type owl:Class ;
    rdfs:subClassOf :CCSS.Math.Content.8.G.C ;
    prov:wasQuotedFrom <http://www.corestandards.org/Math/Content/8/G/9/> ;
    rdfs:label "English Language Arts Standards - Anchor Standards - College and Career Readiness Anchor Standards for Reading - 9"^^xsd:string ;
    rdfs:comment "Analyze how two or more texts address similar themes or topics in order to build knowledge or to compare the approaches the authors take."^^xsd:string .

:CCSS.Math.Content.8.G.A.1.a rdf:type owl:Class ;
    rdfs:subClassOf :CCSS.Math.Content.8.G.A.1 ;
    prov:wasQuotedFrom <http://www.corestandards.org/Math/Content/8/G/a/> .

:CCSS.Math.Content.8.G.A.1.b rdf:type owl:Class ;
    rdfs:subClassOf :CCSS.Math.Content.8.G.A.1 ;
    prov:wasQuotedFrom <http://www.corestandards.org/Math/Content/8/G/b/> .

:CCSS.Math.Content.8.G.A.1.c rdf:type owl:Class ;
    rdfs:subClassOf :CCSS.Math.Content.8.G.A.1 ;
    prov:wasQuotedFrom <http://www.corestandards.org/Math/Content/8/G/c/> .

:CCSS.Math.Content.8.SP rdf:type owl:Class ;
    rdfs:subClassOf :CCSS.Math.Content.8 ;
    rdfs:label "Statistics & Probability"^^xsd:string ;
    prov:wasQuotedFrom <http://www.corestandards.org/Math/Content/8/SP/> .

:CCSS.Math.Content.8.SP.A rdf:type owl:Class ;
    rdfs:subClassOf :CCSS.Math.Content.8.SP ;
    rdfs:label "Statistics & Probability"^^xsd:string ;
    prov:wasQuotedFrom <http://www.corestandards.org/Math/Content/8/SP/> .

:CCSS.Math.Content.8.SP.A.1 rdf:type owl:Class ;
    rdfs:subClassOf :CCSS.Math.Content.8.SP.A ;
    prov:wasQuotedFrom <http://www.corestandards.org/Math/Content/8/SP/1/> ;
    rdfs:label "English Language Arts Standards - Anchor Standards - College and Career Readiness Anchor Standards for Language - 1"^^xsd:string ;
    rdfs:comment "Demonstrate command of the conventions of standard English grammar and usage when writing or speaking."^^xsd:string .

:CCSS.Math.Content.8.SP.A.2 rdf:type owl:Class ;
    rdfs:subClassOf :CCSS.Math.Content.8.SP.A ;
    prov:wasQuotedFrom <http://www.corestandards.org/Math/Content/8/SP/2/> ;
    rdfs:label "English Language Arts Standards - Anchor Standards - College and Career Readiness Anchor Standards for Language - 2"^^xsd:string ;
    rdfs:comment "Demonstrate command of the conventions of standard English capitalization, punctuation, and spelling when writing."^^xsd:string .

:CCSS.Math.Content.8.SP.A.3 rdf:type owl:Class ;
    rdfs:subClassOf :CCSS.Math.Content.8.SP.A ;
    prov:wasQuotedFrom <http://www.corestandards.org/Math/Content/8/SP/3/> ;
    rdfs:label "English Language Arts Standards - Anchor Standards - College and Career Readiness Anchor Standards for Language - 3"^^xsd:string ;
    rdfs:comment "Apply knowledge of language to understand how language functions in different contexts, to make effective choices for meaning or style, and to comprehend more fully when reading or listening. "^^xsd:string .

:CCSS.Math.Content.8.SP.A.4 rdf:type owl:Class ;
    rdfs:subClassOf :CCSS.Math.Content.8.SP.A ;
    prov:wasQuotedFrom <http://www.corestandards.org/Math/Content/8/SP/4/> ;
    rdfs:label "English Language Arts Standards - Anchor Standards - College and Career Readiness Anchor Standards for Language - 4"^^xsd:string ;
    rdfs:comment "Determine or clarify the meaning of unknown and multiple-meaning words and phrases by using context clues, analyzing meaningful word parts, and consulting general and specialized reference materials, as appropriate."^^xsd:string .

:CCSS.Math.Content.HSN rdf:type owl:Class ;
    rdfs:subClassOf :CCSS.Math.Content ;
    rdfs:label "High School: Number and Quantity"^^xsd:string ;
    prov:wasQuotedFrom <http://www.corestandards.org/Math/Content/HSN/> .

:CCSS.Math.Content.HSN.introduction rdf:type owl:Class ;
    rdfs:subClassOf :CCSS.Math.Content.HSN ;
    prov:wasQuotedFrom <http://www.corestandards.org/Math/Content/HSN/introduction/> ;
    rdfs:label "High School: Number and Quantity - Introduction"^^xsd:string ;
    rdfs:comment "During the years from kindergarten to eighth grade, students must repeatedly extend their conception of number. At first, -number- means -counting number-: 1, 2, 3, - Soon after that, 0 is used to represent -none- and the whole numbers are formed by the counting numbers together with zero. The next extension is fractions. At first, fractions are barely numbers and tied strongly to pictorial representations. Yet by the time students understand division of fractions, they have a strong concept of fractions as numbers and have connected them, via their decimal representations, with the base-ten system used to represent the whole numbers. During middle school, fractions are augmented by negative fractions to form the rational numbers. In Grade 8, students extend this system once more, augmenting the rational numbers with the irrational numbers to form the real numbers. In high school, students will be exposed to yet another extension of number, when the real numbers are augmented by the imaginary numbers to form the complex numbers."^^xsd:string .

:CCSS.Math.Content.HSN.CN rdf:type owl:Class ;
    rdfs:subClassOf :CCSS.Math.Content.HSN ;
    rdfs:label "High School: Number and Quantity"^^xsd:string ;
    prov:wasQuotedFrom <http://www.corestandards.org/Math/Content/HSN/> .

:CCSS.Math.Content.HSN.CN.A rdf:type owl:Class ;
    rdfs:subClassOf :CCSS.Math.Content.HSN.CN ;
    prov:wasQuotedFrom <http://www.corestandards.org/Math/Content/HSN/A/> .

:CCSS.Math.Content.HSN.CN.B rdf:type owl:Class ;
    rdfs:subClassOf :CCSS.Math.Content.HSN.CN ;
    prov:wasQuotedFrom <http://www.corestandards.org/Math/Content/HSN/B/> .

:CCSS.Math.Content.HSN.CN.C rdf:type owl:Class ;
    rdfs:subClassOf :CCSS.Math.Content.HSN.CN ;
    prov:wasQuotedFrom <http://www.corestandards.org/Math/Content/HSN/C/> .

:CCSS.Math.Content.HSN.Q rdf:type owl:Class ;
    rdfs:subClassOf :CCSS.Math.Content.HSN ;
    rdfs:label "High School: Number and Quantity"^^xsd:string ;
    prov:wasQuotedFrom <http://www.corestandards.org/Math/Content/HSN/> .

:CCSS.Math.Content.HSN.Q.A rdf:type owl:Class ;
    rdfs:subClassOf :CCSS.Math.Content.HSN.Q ;
    prov:wasQuotedFrom <http://www.corestandards.org/Math/Content/HSN/A/> .

:CCSS.Math.Content.HSN.RN rdf:type owl:Class ;
    rdfs:subClassOf :CCSS.Math.Content.HSN ;
    rdfs:label "High School: Number and Quantity"^^xsd:string ;
    prov:wasQuotedFrom <http://www.corestandards.org/Math/Content/HSN/> .

:CCSS.Math.Content.HSN.RN.A rdf:type owl:Class ;
    rdfs:subClassOf :CCSS.Math.Content.HSN.RN ;
    prov:wasQuotedFrom <http://www.corestandards.org/Math/Content/HSN/A/> .

:CCSS.Math.Content.HSN.RN.B rdf:type owl:Class ;
    rdfs:subClassOf :CCSS.Math.Content.HSN.RN ;
    prov:wasQuotedFrom <http://www.corestandards.org/Math/Content/HSN/B/> .

:CCSS.Math.Content.HSN.VM rdf:type owl:Class ;
    rdfs:subClassOf :CCSS.Math.Content.HSN ;
    rdfs:label "High School: Number and Quantity"^^xsd:string ;
    prov:wasQuotedFrom <http://www.corestandards.org/Math/Content/HSN/> .

:CCSS.Math.Content.HSN.VM.A rdf:type owl:Class ;
    rdfs:subClassOf :CCSS.Math.Content.HSN.VM ;
    prov:wasQuotedFrom <http://www.corestandards.org/Math/Content/HSN/A/> .

:CCSS.Math.Content.HSN.VM.B rdf:type owl:Class ;
    rdfs:subClassOf :CCSS.Math.Content.HSN.VM ;
    prov:wasQuotedFrom <http://www.corestandards.org/Math/Content/HSN/B/> .

:CCSS.Math.Content.HSN.VM.C rdf:type owl:Class ;
    rdfs:subClassOf :CCSS.Math.Content.HSN.VM ;
    prov:wasQuotedFrom <http://www.corestandards.org/Math/Content/HSN/C/> .

:CCSS.Math.Content.HSN.CN rdf:type owl:Class ;
    rdfs:subClassOf :CCSS.Math.Content.HSN .

:CCSS.Math.Content.HSN.CN.A rdf:type owl:Class ;
    rdfs:subClassOf :CCSS.Math.Content.HSN.CN .

:CCSS.Math.Content.HSN.CN.A.1 rdf:type owl:Class ;
    rdfs:subClassOf :CCSS.Math.Content.HSN.CN.A ;
    prov:wasQuotedFrom <http://www.corestandards.org/Math/Content/HSN/1/> ;
    rdfs:label "English Language Arts Standards - Anchor Standards - College and Career Readiness Anchor Standards for Language - 1"^^xsd:string ;
    rdfs:comment "Demonstrate command of the conventions of standard English grammar and usage when writing or speaking."^^xsd:string .

:CCSS.Math.Content.HSN.CN.A.2 rdf:type owl:Class ;
    rdfs:subClassOf :CCSS.Math.Content.HSN.CN.A ;
    prov:wasQuotedFrom <http://www.corestandards.org/Math/Content/HSN/2/> ;
    rdfs:label "English Language Arts Standards - Anchor Standards - College and Career Readiness Anchor Standards for Language - 2"^^xsd:string ;
    rdfs:comment "Demonstrate command of the conventions of standard English capitalization, punctuation, and spelling when writing."^^xsd:string .

:CCSS.Math.Content.HSN.CN.A.3 rdf:type owl:Class ;
    rdfs:subClassOf :CCSS.Math.Content.HSN.CN.A ;
    prov:wasQuotedFrom <http://www.corestandards.org/Math/Content/HSN/3/> ;
    rdfs:label "English Language Arts Standards - Anchor Standards - College and Career Readiness Anchor Standards for Language - 3"^^xsd:string ;
    rdfs:comment "Apply knowledge of language to understand how language functions in different contexts, to make effective choices for meaning or style, and to comprehend more fully when reading or listening. "^^xsd:string .

:CCSS.Math.Content.HSN.CN.B rdf:type owl:Class ;
    rdfs:subClassOf :CCSS.Math.Content.HSN.CN .

:CCSS.Math.Content.HSN.CN.B.4 rdf:type owl:Class ;
    rdfs:subClassOf :CCSS.Math.Content.HSN.CN.B ;
    prov:wasQuotedFrom <http://www.corestandards.org/Math/Content/HSN/4/> ;
    rdfs:label "English Language Arts Standards - Anchor Standards - College and Career Readiness Anchor Standards for Language - 4"^^xsd:string ;
    rdfs:comment "Determine or clarify the meaning of unknown and multiple-meaning words and phrases by using context clues, analyzing meaningful word parts, and consulting general and specialized reference materials, as appropriate."^^xsd:string .

:CCSS.Math.Content.HSN.CN.B.5 rdf:type owl:Class ;
    rdfs:subClassOf :CCSS.Math.Content.HSN.CN.B ;
    prov:wasQuotedFrom <http://www.corestandards.org/Math/Content/HSN/5/> ;
    rdfs:label "English Language Arts Standards - Anchor Standards - College and Career Readiness Anchor Standards for Language - 5"^^xsd:string ;
    rdfs:comment "Demonstrate understanding of figurative language, word relationships, and nuances in word meanings."^^xsd:string .

:CCSS.Math.Content.HSN.CN.B.6 rdf:type owl:Class ;
    rdfs:subClassOf :CCSS.Math.Content.HSN.CN.B ;
    prov:wasQuotedFrom <http://www.corestandards.org/Math/Content/HSN/6/> ;
    rdfs:label "English Language Arts Standards - Anchor Standards - College and Career Readiness Anchor Standards for Language - 6"^^xsd:string ;
    rdfs:comment "Acquire and use accurately a range of general academic and domain-specific words and phrases sufficient for reading, writing, speaking, and listening at the college and career readiness level; demonstrate independence in gathering vocabulary knowledge when encountering an unknown term important to comprehension or expression."^^xsd:string .

:CCSS.Math.Content.HSN.CN.C rdf:type owl:Class ;
    rdfs:subClassOf :CCSS.Math.Content.HSN.CN .

:CCSS.Math.Content.HSN.CN.C.7 rdf:type owl:Class ;
    rdfs:subClassOf :CCSS.Math.Content.HSN.CN.C ;
    prov:wasQuotedFrom <http://www.corestandards.org/Math/Content/HSN/7/> ;
    rdfs:label "English Language Arts Standards - Anchor Standards - College and Career Readiness Anchor Standards for Reading - 7"^^xsd:string ;
    rdfs:comment "Integrate and evaluate content presented in diverse media and formats, including visually and quantitatively, as well as in words.1"^^xsd:string .

:CCSS.Math.Content.HSN.CN.C.8 rdf:type owl:Class ;
    rdfs:subClassOf :CCSS.Math.Content.HSN.CN.C ;
    prov:wasQuotedFrom <http://www.corestandards.org/Math/Content/HSN/8/> ;
    rdfs:label "English Language Arts Standards - Anchor Standards - College and Career Readiness Anchor Standards for Reading - 8"^^xsd:string ;
    rdfs:comment "Delineate and evaluate the argument and specific claims in a text, including the validity of the reasoning as well as the relevance and sufficiency of the evidence."^^xsd:string .

:CCSS.Math.Content.HSN.CN.C.9 rdf:type owl:Class ;
    rdfs:subClassOf :CCSS.Math.Content.HSN.CN.C ;
    prov:wasQuotedFrom <http://www.corestandards.org/Math/Content/HSN/9/> ;
    rdfs:label "English Language Arts Standards - Anchor Standards - College and Career Readiness Anchor Standards for Reading - 9"^^xsd:string ;
    rdfs:comment "Analyze how two or more texts address similar themes or topics in order to build knowledge or to compare the approaches the authors take."^^xsd:string .

:CCSS.Math.Content.HSN.Q rdf:type owl:Class ;
    rdfs:subClassOf :CCSS.Math.Content.HSN .

:CCSS.Math.Content.HSN.Q.A rdf:type owl:Class ;
    rdfs:subClassOf :CCSS.Math.Content.HSN.Q .

:CCSS.Math.Content.HSN.Q.A.1 rdf:type owl:Class ;
    rdfs:subClassOf :CCSS.Math.Content.HSN.Q.A ;
    prov:wasQuotedFrom <http://www.corestandards.org/Math/Content/HSN/1/> ;
    rdfs:label "English Language Arts Standards - Anchor Standards - College and Career Readiness Anchor Standards for Language - 1"^^xsd:string ;
    rdfs:comment "Demonstrate command of the conventions of standard English grammar and usage when writing or speaking."^^xsd:string .

:CCSS.Math.Content.HSN.Q.A.2 rdf:type owl:Class ;
    rdfs:subClassOf :CCSS.Math.Content.HSN.Q.A ;
    prov:wasQuotedFrom <http://www.corestandards.org/Math/Content/HSN/2/> ;
    rdfs:label "English Language Arts Standards - Anchor Standards - College and Career Readiness Anchor Standards for Language - 2"^^xsd:string ;
    rdfs:comment "Demonstrate command of the conventions of standard English capitalization, punctuation, and spelling when writing."^^xsd:string .

:CCSS.Math.Content.HSN.Q.A.3 rdf:type owl:Class ;
    rdfs:subClassOf :CCSS.Math.Content.HSN.Q.A ;
    prov:wasQuotedFrom <http://www.corestandards.org/Math/Content/HSN/3/> ;
    rdfs:label "English Language Arts Standards - Anchor Standards - College and Career Readiness Anchor Standards for Language - 3"^^xsd:string ;
    rdfs:comment "Apply knowledge of language to understand how language functions in different contexts, to make effective choices for meaning or style, and to comprehend more fully when reading or listening. "^^xsd:string .

:CCSS.Math.Content.HSN.RN rdf:type owl:Class ;
    rdfs:subClassOf :CCSS.Math.Content.HSN .

:CCSS.Math.Content.HSN.RN.A rdf:type owl:Class ;
    rdfs:subClassOf :CCSS.Math.Content.HSN.RN .

:CCSS.Math.Content.HSN.RN.A.1 rdf:type owl:Class ;
    rdfs:subClassOf :CCSS.Math.Content.HSN.RN.A ;
    prov:wasQuotedFrom <http://www.corestandards.org/Math/Content/HSN/1/> ;
    rdfs:label "English Language Arts Standards - Anchor Standards - College and Career Readiness Anchor Standards for Language - 1"^^xsd:string ;
    rdfs:comment "Demonstrate command of the conventions of standard English grammar and usage when writing or speaking."^^xsd:string .

:CCSS.Math.Content.HSN.RN.A.2 rdf:type owl:Class ;
    rdfs:subClassOf :CCSS.Math.Content.HSN.RN.A ;
    prov:wasQuotedFrom <http://www.corestandards.org/Math/Content/HSN/2/> ;
    rdfs:label "English Language Arts Standards - Anchor Standards - College and Career Readiness Anchor Standards for Language - 2"^^xsd:string ;
    rdfs:comment "Demonstrate command of the conventions of standard English capitalization, punctuation, and spelling when writing."^^xsd:string .

:CCSS.Math.Content.HSN.RN.B rdf:type owl:Class ;
    rdfs:subClassOf :CCSS.Math.Content.HSN.RN .

:CCSS.Math.Content.HSN.RN.B.3 rdf:type owl:Class ;
    rdfs:subClassOf :CCSS.Math.Content.HSN.RN.B ;
    prov:wasQuotedFrom <http://www.corestandards.org/Math/Content/HSN/3/> ;
    rdfs:label "English Language Arts Standards - Anchor Standards - College and Career Readiness Anchor Standards for Language - 3"^^xsd:string ;
    rdfs:comment "Apply knowledge of language to understand how language functions in different contexts, to make effective choices for meaning or style, and to comprehend more fully when reading or listening. "^^xsd:string .

:CCSS.Math.Content.HSN.VM rdf:type owl:Class ;
    rdfs:subClassOf :CCSS.Math.Content.HSN .

:CCSS.Math.Content.HSN.VM.A rdf:type owl:Class ;
    rdfs:subClassOf :CCSS.Math.Content.HSN.VM .

:CCSS.Math.Content.HSN.VM.A.1 rdf:type owl:Class ;
    rdfs:subClassOf :CCSS.Math.Content.HSN.VM.A ;
    prov:wasQuotedFrom <http://www.corestandards.org/Math/Content/HSN/1/> ;
    rdfs:label "English Language Arts Standards - Anchor Standards - College and Career Readiness Anchor Standards for Language - 1"^^xsd:string ;
    rdfs:comment "Demonstrate command of the conventions of standard English grammar and usage when writing or speaking."^^xsd:string .

:CCSS.Math.Content.HSN.VM.A.2 rdf:type owl:Class ;
    rdfs:subClassOf :CCSS.Math.Content.HSN.VM.A ;
    prov:wasQuotedFrom <http://www.corestandards.org/Math/Content/HSN/2/> ;
    rdfs:label "English Language Arts Standards - Anchor Standards - College and Career Readiness Anchor Standards for Language - 2"^^xsd:string ;
    rdfs:comment "Demonstrate command of the conventions of standard English capitalization, punctuation, and spelling when writing."^^xsd:string .

:CCSS.Math.Content.HSN.VM.A.3 rdf:type owl:Class ;
    rdfs:subClassOf :CCSS.Math.Content.HSN.VM.A ;
    prov:wasQuotedFrom <http://www.corestandards.org/Math/Content/HSN/3/> ;
    rdfs:label "English Language Arts Standards - Anchor Standards - College and Career Readiness Anchor Standards for Language - 3"^^xsd:string ;
    rdfs:comment "Apply knowledge of language to understand how language functions in different contexts, to make effective choices for meaning or style, and to comprehend more fully when reading or listening. "^^xsd:string .

:CCSS.Math.Content.HSN.VM.B rdf:type owl:Class ;
    rdfs:subClassOf :CCSS.Math.Content.HSN.VM .

:CCSS.Math.Content.HSN.VM.B.4 rdf:type owl:Class ;
    rdfs:subClassOf :CCSS.Math.Content.HSN.VM.B ;
    prov:wasQuotedFrom <http://www.corestandards.org/Math/Content/HSN/4/> ;
    rdfs:label "English Language Arts Standards - Anchor Standards - College and Career Readiness Anchor Standards for Language - 4"^^xsd:string ;
    rdfs:comment "Determine or clarify the meaning of unknown and multiple-meaning words and phrases by using context clues, analyzing meaningful word parts, and consulting general and specialized reference materials, as appropriate."^^xsd:string .

:CCSS.Math.Content.HSN.VM.B.5 rdf:type owl:Class ;
    rdfs:subClassOf :CCSS.Math.Content.HSN.VM.B ;
    prov:wasQuotedFrom <http://www.corestandards.org/Math/Content/HSN/5/> ;
    rdfs:label "English Language Arts Standards - Anchor Standards - College and Career Readiness Anchor Standards for Language - 5"^^xsd:string ;
    rdfs:comment "Demonstrate understanding of figurative language, word relationships, and nuances in word meanings."^^xsd:string .

:CCSS.Math.Content.HSN.VM.C rdf:type owl:Class ;
    rdfs:subClassOf :CCSS.Math.Content.HSN.VM .

:CCSS.Math.Content.HSN.VM.C.6 rdf:type owl:Class ;
    rdfs:subClassOf :CCSS.Math.Content.HSN.VM.C ;
    prov:wasQuotedFrom <http://www.corestandards.org/Math/Content/HSN/6/> ;
    rdfs:label "English Language Arts Standards - Anchor Standards - College and Career Readiness Anchor Standards for Language - 6"^^xsd:string ;
    rdfs:comment "Acquire and use accurately a range of general academic and domain-specific words and phrases sufficient for reading, writing, speaking, and listening at the college and career readiness level; demonstrate independence in gathering vocabulary knowledge when encountering an unknown term important to comprehension or expression."^^xsd:string .

:CCSS.Math.Content.HSN.VM.C.7 rdf:type owl:Class ;
    rdfs:subClassOf :CCSS.Math.Content.HSN.VM.C ;
    prov:wasQuotedFrom <http://www.corestandards.org/Math/Content/HSN/7/> ;
    rdfs:label "English Language Arts Standards - Anchor Standards - College and Career Readiness Anchor Standards for Reading - 7"^^xsd:string ;
    rdfs:comment "Integrate and evaluate content presented in diverse media and formats, including visually and quantitatively, as well as in words.1"^^xsd:string .

:CCSS.Math.Content.HSN.VM.C.8 rdf:type owl:Class ;
    rdfs:subClassOf :CCSS.Math.Content.HSN.VM.C ;
    prov:wasQuotedFrom <http://www.corestandards.org/Math/Content/HSN/8/> ;
    rdfs:label "English Language Arts Standards - Anchor Standards - College and Career Readiness Anchor Standards for Reading - 8"^^xsd:string ;
    rdfs:comment "Delineate and evaluate the argument and specific claims in a text, including the validity of the reasoning as well as the relevance and sufficiency of the evidence."^^xsd:string .

:CCSS.Math.Content.HSN.VM.C.9 rdf:type owl:Class ;
    rdfs:subClassOf :CCSS.Math.Content.HSN.VM.C ;
    prov:wasQuotedFrom <http://www.corestandards.org/Math/Content/HSN/9/> ;
    rdfs:label "English Language Arts Standards - Anchor Standards - College and Career Readiness Anchor Standards for Reading - 9"^^xsd:string ;
    rdfs:comment "Analyze how two or more texts address similar themes or topics in order to build knowledge or to compare the approaches the authors take."^^xsd:string .

:CCSS.Math.Content.HSN.VM.C.10 rdf:type owl:Class ;
    rdfs:subClassOf :CCSS.Math.Content.HSN.VM.C ;
    prov:wasQuotedFrom <http://www.corestandards.org/Math/Content/HSN/10/> ;
    rdfs:label "English Language Arts Standards - Anchor Standards - College and Career Readiness Anchor Standards for Reading - 10"^^xsd:string ;
    rdfs:comment "Read and comprehend complex literary and informational texts independently and proficiently."^^xsd:string .

:CCSS.Math.Content.HSN.VM.C.11 rdf:type owl:Class ;
    rdfs:subClassOf :CCSS.Math.Content.HSN.VM.C ;
    prov:wasQuotedFrom <http://www.corestandards.org/Math/Content/HSN/11/> ;
    rdfs:label "High School: Algebra - Reasoning with Equations & Inequalities - Represent and solve equations and inequalities graphically.   - 11"^^xsd:string ;
    rdfs:comment "Explain why the x-coordinates of the points where the graphs of the equations y = f(x) and y = g(x) intersect are the solutions of the equation f(x) = g(x); find the solutions approximately, e.g., using technology to graph the functions, make tables of values, or find successive approximations. Include cases where f(x) and/or g(x) are linear, polynomial, rational, absolute value, exponential, and logarithmic functions.*"^^xsd:string .

:CCSS.Math.Content.HSN.VM.C.12 rdf:type owl:Class ;
    rdfs:subClassOf :CCSS.Math.Content.HSN.VM.C ;
    prov:wasQuotedFrom <http://www.corestandards.org/Math/Content/HSN/12/> ;
    rdfs:label "High School: Algebra - Reasoning with Equations & Inequalities - Represent and solve equations and inequalities graphically.   - 12"^^xsd:string ;
    rdfs:comment "Graph the solutions to a linear inequality in two variables as a half-plane (excluding the boundary in the case of a strict inequality), and graph the solution set to a system of linear inequalities in two variables as the intersection of the corresponding half-planes."^^xsd:string .

:CCSS.Math.Content.HSN.VM.B.4.a rdf:type owl:Class ;
    rdfs:subClassOf :CCSS.Math.Content.HSN.VM.B.4 ;
    prov:wasQuotedFrom <http://www.corestandards.org/Math/Content/HSN/VM/a/> .

:CCSS.Math.Content.HSN.VM.B.4.b rdf:type owl:Class ;
    rdfs:subClassOf :CCSS.Math.Content.HSN.VM.B.4 ;
    prov:wasQuotedFrom <http://www.corestandards.org/Math/Content/HSN/VM/b/> .

:CCSS.Math.Content.HSN.VM.B.4.c rdf:type owl:Class ;
    rdfs:subClassOf :CCSS.Math.Content.HSN.VM.B.4 ;
    prov:wasQuotedFrom <http://www.corestandards.org/Math/Content/HSN/VM/c/> .

:CCSS.Math.Content.HSN.VM.B.5.a rdf:type owl:Class ;
    rdfs:subClassOf :CCSS.Math.Content.HSN.VM.B.5 ;
    prov:wasQuotedFrom <http://www.corestandards.org/Math/Content/HSN/VM/a/> .

:CCSS.Math.Content.HSN.VM.B.5.b rdf:type owl:Class ;
    rdfs:subClassOf :CCSS.Math.Content.HSN.VM.B.5 ;
    prov:wasQuotedFrom <http://www.corestandards.org/Math/Content/HSN/VM/b/> .

:CCSS.Math.Content.HSA rdf:type owl:Class ;
    rdfs:subClassOf :CCSS.Math.Content ;
    rdfs:label "High School: Algebra"^^xsd:string ;
    prov:wasQuotedFrom <http://www.corestandards.org/Math/Content/HSA/> .

:CCSS.Math.Content.HSA.introduction rdf:type owl:Class ;
    rdfs:subClassOf :CCSS.Math.Content.HSA ;
    prov:wasQuotedFrom <http://www.corestandards.org/Math/Content/HSA/introduction/> ;
    rdfs:label "High School: Algebra - Introduction"^^xsd:string ;
    rdfs:comment "An expression is a record of a computation with numbers, symbols that represent numbers, arithmetic operations, exponentiation, and, at more advanced levels, the operation of evaluating a function. Conventions about the use of parentheses and the order of operations assure that each expression is unambiguous. Creating an expression that describes a computation involving a general quantity requires the ability to express the computation in general terms, abstracting from specific instances."^^xsd:string .

:CCSS.Math.Content.HSA.APR rdf:type owl:Class ;
    rdfs:subClassOf :CCSS.Math.Content.HSA ;
    rdfs:label "High School: Algebra"^^xsd:string ;
    prov:wasQuotedFrom <http://www.corestandards.org/Math/Content/HSA/> .

:CCSS.Math.Content.HSA.APR.A rdf:type owl:Class ;
    rdfs:subClassOf :CCSS.Math.Content.HSA.APR ;
    prov:wasQuotedFrom <http://www.corestandards.org/Math/Content/HSA/A/> .

:CCSS.Math.Content.HSA.APR.B rdf:type owl:Class ;
    rdfs:subClassOf :CCSS.Math.Content.HSA.APR ;
    prov:wasQuotedFrom <http://www.corestandards.org/Math/Content/HSA/B/> .

:CCSS.Math.Content.HSA.APR.C rdf:type owl:Class ;
    rdfs:subClassOf :CCSS.Math.Content.HSA.APR ;
    prov:wasQuotedFrom <http://www.corestandards.org/Math/Content/HSA/C/> .

:CCSS.Math.Content.HSA.APR.D rdf:type owl:Class ;
    rdfs:subClassOf :CCSS.Math.Content.HSA.APR ;
    prov:wasQuotedFrom <http://www.corestandards.org/Math/Content/HSA/D/> .

:CCSS.Math.Content.HSA.CED rdf:type owl:Class ;
    rdfs:subClassOf :CCSS.Math.Content.HSA ;
    rdfs:label "High School: Algebra"^^xsd:string ;
    prov:wasQuotedFrom <http://www.corestandards.org/Math/Content/HSA/> .

:CCSS.Math.Content.HSA.CED.A rdf:type owl:Class ;
    rdfs:subClassOf :CCSS.Math.Content.HSA.CED ;
    prov:wasQuotedFrom <http://www.corestandards.org/Math/Content/HSA/A/> .

:CCSS.Math.Content.HSA.REI rdf:type owl:Class ;
    rdfs:subClassOf :CCSS.Math.Content.HSA ;
    rdfs:label "High School: Algebra"^^xsd:string ;
    prov:wasQuotedFrom <http://www.corestandards.org/Math/Content/HSA/> .

:CCSS.Math.Content.HSA.REI.A rdf:type owl:Class ;
    rdfs:subClassOf :CCSS.Math.Content.HSA.REI ;
    prov:wasQuotedFrom <http://www.corestandards.org/Math/Content/HSA/A/> .

:CCSS.Math.Content.HSA.REI.B rdf:type owl:Class ;
    rdfs:subClassOf :CCSS.Math.Content.HSA.REI ;
    prov:wasQuotedFrom <http://www.corestandards.org/Math/Content/HSA/B/> .

:CCSS.Math.Content.HSA.REI.C rdf:type owl:Class ;
    rdfs:subClassOf :CCSS.Math.Content.HSA.REI ;
    prov:wasQuotedFrom <http://www.corestandards.org/Math/Content/HSA/C/> .

:CCSS.Math.Content.HSA.REI.D rdf:type owl:Class ;
    rdfs:subClassOf :CCSS.Math.Content.HSA.REI ;
    prov:wasQuotedFrom <http://www.corestandards.org/Math/Content/HSA/D/> .

:CCSS.Math.Content.HSA.SSE rdf:type owl:Class ;
    rdfs:subClassOf :CCSS.Math.Content.HSA ;
    rdfs:label "High School: Algebra"^^xsd:string ;
    prov:wasQuotedFrom <http://www.corestandards.org/Math/Content/HSA/> .

:CCSS.Math.Content.HSA.SSE.A rdf:type owl:Class ;
    rdfs:subClassOf :CCSS.Math.Content.HSA.SSE ;
    prov:wasQuotedFrom <http://www.corestandards.org/Math/Content/HSA/A/> .

:CCSS.Math.Content.HSA.SSE.B rdf:type owl:Class ;
    rdfs:subClassOf :CCSS.Math.Content.HSA.SSE ;
    prov:wasQuotedFrom <http://www.corestandards.org/Math/Content/HSA/B/> .

:CCSS.Math.Content.HSA.APR.A.1 rdf:type owl:Class ;
    rdfs:subClassOf :CCSS.Math.Content.HSA.APR.A ;
    prov:wasQuotedFrom <http://www.corestandards.org/Math/Content/HSA/1/> ;
    rdfs:label "English Language Arts Standards - Anchor Standards - College and Career Readiness Anchor Standards for Language - 1"^^xsd:string ;
    rdfs:comment "Demonstrate command of the conventions of standard English grammar and usage when writing or speaking."^^xsd:string .

:CCSS.Math.Content.HSA.APR.B.2 rdf:type owl:Class ;
    rdfs:subClassOf :CCSS.Math.Content.HSA.APR.B ;
    prov:wasQuotedFrom <http://www.corestandards.org/Math/Content/HSA/2/> ;
    rdfs:label "English Language Arts Standards - Anchor Standards - College and Career Readiness Anchor Standards for Language - 2"^^xsd:string ;
    rdfs:comment "Demonstrate command of the conventions of standard English capitalization, punctuation, and spelling when writing."^^xsd:string .

:CCSS.Math.Content.HSA.APR.B.3 rdf:type owl:Class ;
    rdfs:subClassOf :CCSS.Math.Content.HSA.APR.B ;
    prov:wasQuotedFrom <http://www.corestandards.org/Math/Content/HSA/3/> ;
    rdfs:label "English Language Arts Standards - Anchor Standards - College and Career Readiness Anchor Standards for Language - 3"^^xsd:string ;
    rdfs:comment "Apply knowledge of language to understand how language functions in different contexts, to make effective choices for meaning or style, and to comprehend more fully when reading or listening. "^^xsd:string .

:CCSS.Math.Content.HSA.APR.C.4 rdf:type owl:Class ;
    rdfs:subClassOf :CCSS.Math.Content.HSA.APR.C ;
    prov:wasQuotedFrom <http://www.corestandards.org/Math/Content/HSA/4/> ;
    rdfs:label "English Language Arts Standards - Anchor Standards - College and Career Readiness Anchor Standards for Language - 4"^^xsd:string ;
    rdfs:comment "Determine or clarify the meaning of unknown and multiple-meaning words and phrases by using context clues, analyzing meaningful word parts, and consulting general and specialized reference materials, as appropriate."^^xsd:string .

:CCSS.Math.Content.HSA.APR.C.5 rdf:type owl:Class ;
    rdfs:subClassOf :CCSS.Math.Content.HSA.APR.C ;
    prov:wasQuotedFrom <http://www.corestandards.org/Math/Content/HSA/5/> ;
    rdfs:label "English Language Arts Standards - Anchor Standards - College and Career Readiness Anchor Standards for Language - 5"^^xsd:string ;
    rdfs:comment "Demonstrate understanding of figurative language, word relationships, and nuances in word meanings."^^xsd:string .

:CCSS.Math.Content.HSA.APR.D.6 rdf:type owl:Class ;
    rdfs:subClassOf :CCSS.Math.Content.HSA.APR.D ;
    prov:wasQuotedFrom <http://www.corestandards.org/Math/Content/HSA/6/> ;
    rdfs:label "English Language Arts Standards - Anchor Standards - College and Career Readiness Anchor Standards for Language - 6"^^xsd:string ;
    rdfs:comment "Acquire and use accurately a range of general academic and domain-specific words and phrases sufficient for reading, writing, speaking, and listening at the college and career readiness level; demonstrate independence in gathering vocabulary knowledge when encountering an unknown term important to comprehension or expression."^^xsd:string .

:CCSS.Math.Content.HSA.APR.D.7 rdf:type owl:Class ;
    rdfs:subClassOf :CCSS.Math.Content.HSA.APR.D ;
    prov:wasQuotedFrom <http://www.corestandards.org/Math/Content/HSA/7/> ;
    rdfs:label "English Language Arts Standards - Anchor Standards - College and Career Readiness Anchor Standards for Reading - 7"^^xsd:string ;
    rdfs:comment "Integrate and evaluate content presented in diverse media and formats, including visually and quantitatively, as well as in words.1"^^xsd:string .

:CCSS.Math.Content.HSA.CED.A.1 rdf:type owl:Class ;
    rdfs:subClassOf :CCSS.Math.Content.HSA.CED.A ;
    prov:wasQuotedFrom <http://www.corestandards.org/Math/Content/HSA/1/> ;
    rdfs:label "English Language Arts Standards - Anchor Standards - College and Career Readiness Anchor Standards for Language - 1"^^xsd:string ;
    rdfs:comment "Demonstrate command of the conventions of standard English grammar and usage when writing or speaking."^^xsd:string .

:CCSS.Math.Content.HSA.CED.A.2 rdf:type owl:Class ;
    rdfs:subClassOf :CCSS.Math.Content.HSA.CED.A ;
    prov:wasQuotedFrom <http://www.corestandards.org/Math/Content/HSA/2/> ;
    rdfs:label "English Language Arts Standards - Anchor Standards - College and Career Readiness Anchor Standards for Language - 2"^^xsd:string ;
    rdfs:comment "Demonstrate command of the conventions of standard English capitalization, punctuation, and spelling when writing."^^xsd:string .

:CCSS.Math.Content.HSA.CED.A.3 rdf:type owl:Class ;
    rdfs:subClassOf :CCSS.Math.Content.HSA.CED.A ;
    prov:wasQuotedFrom <http://www.corestandards.org/Math/Content/HSA/3/> ;
    rdfs:label "English Language Arts Standards - Anchor Standards - College and Career Readiness Anchor Standards for Language - 3"^^xsd:string ;
    rdfs:comment "Apply knowledge of language to understand how language functions in different contexts, to make effective choices for meaning or style, and to comprehend more fully when reading or listening. "^^xsd:string .

:CCSS.Math.Content.HSA.CED.A.4 rdf:type owl:Class ;
    rdfs:subClassOf :CCSS.Math.Content.HSA.CED.A ;
    prov:wasQuotedFrom <http://www.corestandards.org/Math/Content/HSA/4/> ;
    rdfs:label "English Language Arts Standards - Anchor Standards - College and Career Readiness Anchor Standards for Language - 4"^^xsd:string ;
    rdfs:comment "Determine or clarify the meaning of unknown and multiple-meaning words and phrases by using context clues, analyzing meaningful word parts, and consulting general and specialized reference materials, as appropriate."^^xsd:string .

:CCSS.Math.Content.HSA.REI.A.1 rdf:type owl:Class ;
    rdfs:subClassOf :CCSS.Math.Content.HSA.REI.A ;
    prov:wasQuotedFrom <http://www.corestandards.org/Math/Content/HSA/1/> ;
    rdfs:label "English Language Arts Standards - Anchor Standards - College and Career Readiness Anchor Standards for Language - 1"^^xsd:string ;
    rdfs:comment "Demonstrate command of the conventions of standard English grammar and usage when writing or speaking."^^xsd:string .

:CCSS.Math.Content.HSA.REI.A.2 rdf:type owl:Class ;
    rdfs:subClassOf :CCSS.Math.Content.HSA.REI.A ;
    prov:wasQuotedFrom <http://www.corestandards.org/Math/Content/HSA/2/> ;
    rdfs:label "English Language Arts Standards - Anchor Standards - College and Career Readiness Anchor Standards for Language - 2"^^xsd:string ;
    rdfs:comment "Demonstrate command of the conventions of standard English capitalization, punctuation, and spelling when writing."^^xsd:string .

:CCSS.Math.Content.HSA.REI.B.3 rdf:type owl:Class ;
    rdfs:subClassOf :CCSS.Math.Content.HSA.REI.B ;
    prov:wasQuotedFrom <http://www.corestandards.org/Math/Content/HSA/3/> ;
    rdfs:label "English Language Arts Standards - Anchor Standards - College and Career Readiness Anchor Standards for Language - 3"^^xsd:string ;
    rdfs:comment "Apply knowledge of language to understand how language functions in different contexts, to make effective choices for meaning or style, and to comprehend more fully when reading or listening. "^^xsd:string .

:CCSS.Math.Content.HSA.REI.B.4 rdf:type owl:Class ;
    rdfs:subClassOf :CCSS.Math.Content.HSA.REI.B ;
    prov:wasQuotedFrom <http://www.corestandards.org/Math/Content/HSA/4/> ;
    rdfs:label "English Language Arts Standards - Anchor Standards - College and Career Readiness Anchor Standards for Language - 4"^^xsd:string ;
    rdfs:comment "Determine or clarify the meaning of unknown and multiple-meaning words and phrases by using context clues, analyzing meaningful word parts, and consulting general and specialized reference materials, as appropriate."^^xsd:string .

:CCSS.Math.Content.HSA.REI.C.5 rdf:type owl:Class ;
    rdfs:subClassOf :CCSS.Math.Content.HSA.REI.C ;
    prov:wasQuotedFrom <http://www.corestandards.org/Math/Content/HSA/5/> ;
    rdfs:label "English Language Arts Standards - Anchor Standards - College and Career Readiness Anchor Standards for Language - 5"^^xsd:string ;
    rdfs:comment "Demonstrate understanding of figurative language, word relationships, and nuances in word meanings."^^xsd:string .

:CCSS.Math.Content.HSA.REI.C.6 rdf:type owl:Class ;
    rdfs:subClassOf :CCSS.Math.Content.HSA.REI.C ;
    prov:wasQuotedFrom <http://www.corestandards.org/Math/Content/HSA/6/> ;
    rdfs:label "English Language Arts Standards - Anchor Standards - College and Career Readiness Anchor Standards for Language - 6"^^xsd:string ;
    rdfs:comment "Acquire and use accurately a range of general academic and domain-specific words and phrases sufficient for reading, writing, speaking, and listening at the college and career readiness level; demonstrate independence in gathering vocabulary knowledge when encountering an unknown term important to comprehension or expression."^^xsd:string .

:CCSS.Math.Content.HSA.REI.C.7 rdf:type owl:Class ;
    rdfs:subClassOf :CCSS.Math.Content.HSA.REI.C ;
    prov:wasQuotedFrom <http://www.corestandards.org/Math/Content/HSA/7/> ;
    rdfs:label "English Language Arts Standards - Anchor Standards - College and Career Readiness Anchor Standards for Reading - 7"^^xsd:string ;
    rdfs:comment "Integrate and evaluate content presented in diverse media and formats, including visually and quantitatively, as well as in words.1"^^xsd:string .

:CCSS.Math.Content.HSA.REI.C.8 rdf:type owl:Class ;
    rdfs:subClassOf :CCSS.Math.Content.HSA.REI.C ;
    prov:wasQuotedFrom <http://www.corestandards.org/Math/Content/HSA/8/> ;
    rdfs:label "English Language Arts Standards - Anchor Standards - College and Career Readiness Anchor Standards for Reading - 8"^^xsd:string ;
    rdfs:comment "Delineate and evaluate the argument and specific claims in a text, including the validity of the reasoning as well as the relevance and sufficiency of the evidence."^^xsd:string .

:CCSS.Math.Content.HSA.REI.C.9 rdf:type owl:Class ;
    rdfs:subClassOf :CCSS.Math.Content.HSA.REI.C ;
    prov:wasQuotedFrom <http://www.corestandards.org/Math/Content/HSA/9/> ;
    rdfs:label "English Language Arts Standards - Anchor Standards - College and Career Readiness Anchor Standards for Reading - 9"^^xsd:string ;
    rdfs:comment "Analyze how two or more texts address similar themes or topics in order to build knowledge or to compare the approaches the authors take."^^xsd:string .

:CCSS.Math.Content.HSA.REI.D.10 rdf:type owl:Class ;
    rdfs:subClassOf :CCSS.Math.Content.HSA.REI.D ;
    prov:wasQuotedFrom <http://www.corestandards.org/Math/Content/HSA/10/> ;
    rdfs:label "English Language Arts Standards - Anchor Standards - College and Career Readiness Anchor Standards for Reading - 10"^^xsd:string ;
    rdfs:comment "Read and comprehend complex literary and informational texts independently and proficiently."^^xsd:string .

:CCSS.Math.Content.HSA.REI.D.11 rdf:type owl:Class ;
    rdfs:subClassOf :CCSS.Math.Content.HSA.REI.D ;
    prov:wasQuotedFrom <http://www.corestandards.org/Math/Content/HSA/11/> ;
    rdfs:label "High School: Algebra - Reasoning with Equations & Inequalities - Represent and solve equations and inequalities graphically.   - 11"^^xsd:string ;
    rdfs:comment "Explain why the x-coordinates of the points where the graphs of the equations y = f(x) and y = g(x) intersect are the solutions of the equation f(x) = g(x); find the solutions approximately, e.g., using technology to graph the functions, make tables of values, or find successive approximations. Include cases where f(x) and/or g(x) are linear, polynomial, rational, absolute value, exponential, and logarithmic functions.*"^^xsd:string .

:CCSS.Math.Content.HSA.REI.D.12 rdf:type owl:Class ;
    rdfs:subClassOf :CCSS.Math.Content.HSA.REI.D ;
    prov:wasQuotedFrom <http://www.corestandards.org/Math/Content/HSA/12/> ;
    rdfs:label "High School: Algebra - Reasoning with Equations & Inequalities - Represent and solve equations and inequalities graphically.   - 12"^^xsd:string ;
    rdfs:comment "Graph the solutions to a linear inequality in two variables as a half-plane (excluding the boundary in the case of a strict inequality), and graph the solution set to a system of linear inequalities in two variables as the intersection of the corresponding half-planes."^^xsd:string .

:CCSS.Math.Content.HSA.SSE.A.1 rdf:type owl:Class ;
    rdfs:subClassOf :CCSS.Math.Content.HSA.SSE.A ;
    prov:wasQuotedFrom <http://www.corestandards.org/Math/Content/HSA/1/> ;
    rdfs:label "English Language Arts Standards - Anchor Standards - College and Career Readiness Anchor Standards for Language - 1"^^xsd:string ;
    rdfs:comment "Demonstrate command of the conventions of standard English grammar and usage when writing or speaking."^^xsd:string .

:CCSS.Math.Content.HSA.SSE.A.2 rdf:type owl:Class ;
    rdfs:subClassOf :CCSS.Math.Content.HSA.SSE.A ;
    prov:wasQuotedFrom <http://www.corestandards.org/Math/Content/HSA/2/> ;
    rdfs:label "English Language Arts Standards - Anchor Standards - College and Career Readiness Anchor Standards for Language - 2"^^xsd:string ;
    rdfs:comment "Demonstrate command of the conventions of standard English capitalization, punctuation, and spelling when writing."^^xsd:string .

:CCSS.Math.Content.HSA.SSE.B.3 rdf:type owl:Class ;
    rdfs:subClassOf :CCSS.Math.Content.HSA.SSE.B ;
    prov:wasQuotedFrom <http://www.corestandards.org/Math/Content/HSA/3/> ;
    rdfs:label "English Language Arts Standards - Anchor Standards - College and Career Readiness Anchor Standards for Language - 3"^^xsd:string ;
    rdfs:comment "Apply knowledge of language to understand how language functions in different contexts, to make effective choices for meaning or style, and to comprehend more fully when reading or listening. "^^xsd:string .

:CCSS.Math.Content.HSA.SSE.B.4 rdf:type owl:Class ;
    rdfs:subClassOf :CCSS.Math.Content.HSA.SSE.B ;
    prov:wasQuotedFrom <http://www.corestandards.org/Math/Content/HSA/4/> ;
    rdfs:label "English Language Arts Standards - Anchor Standards - College and Career Readiness Anchor Standards for Language - 4"^^xsd:string ;
    rdfs:comment "Determine or clarify the meaning of unknown and multiple-meaning words and phrases by using context clues, analyzing meaningful word parts, and consulting general and specialized reference materials, as appropriate."^^xsd:string .

:CCSS.Math.Content.HSA.SSE.A.1.a rdf:type owl:Class ;
    rdfs:subClassOf :CCSS.Math.Content.HSA.SSE.A.1 ;
    prov:wasQuotedFrom <http://www.corestandards.org/Math/Content/HSA/SSE/a/> .

:CCSS.Math.Content.HSA.SSE.A.1.b rdf:type owl:Class ;
    rdfs:subClassOf :CCSS.Math.Content.HSA.SSE.A.1 ;
    prov:wasQuotedFrom <http://www.corestandards.org/Math/Content/HSA/SSE/b/> .

:CCSS.Math.Content.HSA.SSE.B.3.a rdf:type owl:Class ;
    rdfs:subClassOf :CCSS.Math.Content.HSA.SSE.B.3 ;
    prov:wasQuotedFrom <http://www.corestandards.org/Math/Content/HSA/SSE/a/> .

:CCSS.Math.Content.HSA.SSE.B.3.b rdf:type owl:Class ;
    rdfs:subClassOf :CCSS.Math.Content.HSA.SSE.B.3 ;
    prov:wasQuotedFrom <http://www.corestandards.org/Math/Content/HSA/SSE/b/> .

:CCSS.Math.Content.HSA.SSE.B.3.c rdf:type owl:Class ;
    rdfs:subClassOf :CCSS.Math.Content.HSA.SSE.B.3 ;
    prov:wasQuotedFrom <http://www.corestandards.org/Math/Content/HSA/SSE/c/> .

:CCSS.Math.Content.HSA.REI.B.4.a rdf:type owl:Class ;
    rdfs:subClassOf :CCSS.Math.Content.HSA.REI.B.4 ;
    prov:wasQuotedFrom <http://www.corestandards.org/Math/Content/HSA/REI/a/> .

:CCSS.Math.Content.HSA.REI.B.4.b rdf:type owl:Class ;
    rdfs:subClassOf :CCSS.Math.Content.HSA.REI.B.4 ;
    prov:wasQuotedFrom <http://www.corestandards.org/Math/Content/HSA/REI/b/> .

:CCSS.Math.Content.HSF rdf:type owl:Class ;
    rdfs:subClassOf :CCSS.Math.Content ;
    rdfs:label "High School: Functions"^^xsd:string ;
    prov:wasQuotedFrom <http://www.corestandards.org/Math/Content/HSF/> .

:CCSS.Math.Content.HSF.introduction rdf:type owl:Class ;
    rdfs:subClassOf :CCSS.Math.Content.HSF ;
    prov:wasQuotedFrom <http://www.corestandards.org/Math/Content/HSF/introduction/> ;
    rdfs:label "High School: Functions - Introduction"^^xsd:string ;
    rdfs:comment "Functions describe situations where one quantity determines another. For example, the return on $10,000 invested at an annualized percentage rate of 4.25% is a function of the length of time the money is invested. Because we continually make theories about dependencies between quantities in nature and society, functions are important tools in the construction of mathematical models."^^xsd:string .

:CCSS.Math.Content.HSF.BF rdf:type owl:Class ;
    rdfs:subClassOf :CCSS.Math.Content.HSF ;
    rdfs:label "High School: Functions"^^xsd:string ;
    prov:wasQuotedFrom <http://www.corestandards.org/Math/Content/HSF/> .

:CCSS.Math.Content.HSF.BF.A rdf:type owl:Class ;
    rdfs:subClassOf :CCSS.Math.Content.HSF.BF ;
    prov:wasQuotedFrom <http://www.corestandards.org/Math/Content/HSF/A/> .

:CCSS.Math.Content.HSF.BF.B rdf:type owl:Class ;
    rdfs:subClassOf :CCSS.Math.Content.HSF.BF ;
    prov:wasQuotedFrom <http://www.corestandards.org/Math/Content/HSF/B/> .

:CCSS.Math.Content.HSF.IF rdf:type owl:Class ;
    rdfs:subClassOf :CCSS.Math.Content.HSF ;
    rdfs:label "High School: Functions"^^xsd:string ;
    prov:wasQuotedFrom <http://www.corestandards.org/Math/Content/HSF/> .

:CCSS.Math.Content.HSF.IF.A rdf:type owl:Class ;
    rdfs:subClassOf :CCSS.Math.Content.HSF.IF ;
    prov:wasQuotedFrom <http://www.corestandards.org/Math/Content/HSF/A/> .

:CCSS.Math.Content.HSF.IF.B rdf:type owl:Class ;
    rdfs:subClassOf :CCSS.Math.Content.HSF.IF ;
    prov:wasQuotedFrom <http://www.corestandards.org/Math/Content/HSF/B/> .

:CCSS.Math.Content.HSF.IF.C rdf:type owl:Class ;
    rdfs:subClassOf :CCSS.Math.Content.HSF.IF ;
    prov:wasQuotedFrom <http://www.corestandards.org/Math/Content/HSF/C/> .

:CCSS.Math.Content.HSF.LE rdf:type owl:Class ;
    rdfs:subClassOf :CCSS.Math.Content.HSF ;
    rdfs:label "High School: Functions"^^xsd:string ;
    prov:wasQuotedFrom <http://www.corestandards.org/Math/Content/HSF/> .

:CCSS.Math.Content.HSF.LE.A rdf:type owl:Class ;
    rdfs:subClassOf :CCSS.Math.Content.HSF.LE ;
    prov:wasQuotedFrom <http://www.corestandards.org/Math/Content/HSF/A/> .

:CCSS.Math.Content.HSF.LE.B rdf:type owl:Class ;
    rdfs:subClassOf :CCSS.Math.Content.HSF.LE ;
    prov:wasQuotedFrom <http://www.corestandards.org/Math/Content/HSF/B/> .

:CCSS.Math.Content.HSF.TF rdf:type owl:Class ;
    rdfs:subClassOf :CCSS.Math.Content.HSF ;
    rdfs:label "High School: Functions"^^xsd:string ;
    prov:wasQuotedFrom <http://www.corestandards.org/Math/Content/HSF/> .

:CCSS.Math.Content.HSF.TF.A rdf:type owl:Class ;
    rdfs:subClassOf :CCSS.Math.Content.HSF.TF ;
    prov:wasQuotedFrom <http://www.corestandards.org/Math/Content/HSF/A/> .

:CCSS.Math.Content.HSF.TF.B rdf:type owl:Class ;
    rdfs:subClassOf :CCSS.Math.Content.HSF.TF ;
    prov:wasQuotedFrom <http://www.corestandards.org/Math/Content/HSF/B/> .

:CCSS.Math.Content.HSF.TF.C rdf:type owl:Class ;
    rdfs:subClassOf :CCSS.Math.Content.HSF.TF ;
    prov:wasQuotedFrom <http://www.corestandards.org/Math/Content/HSF/C/> .

:CCSS.Math.Content.HSF.BF.A.1 rdf:type owl:Class ;
    rdfs:subClassOf :CCSS.Math.Content.HSF.BF.A ;
    prov:wasQuotedFrom <http://www.corestandards.org/Math/Content/HSF/1/> ;
    rdfs:label "English Language Arts Standards - Anchor Standards - College and Career Readiness Anchor Standards for Language - 1"^^xsd:string ;
    rdfs:comment "Demonstrate command of the conventions of standard English grammar and usage when writing or speaking."^^xsd:string .

:CCSS.Math.Content.HSF.BF.A.2 rdf:type owl:Class ;
    rdfs:subClassOf :CCSS.Math.Content.HSF.BF.A ;
    prov:wasQuotedFrom <http://www.corestandards.org/Math/Content/HSF/2/> ;
    rdfs:label "English Language Arts Standards - Anchor Standards - College and Career Readiness Anchor Standards for Language - 2"^^xsd:string ;
    rdfs:comment "Demonstrate command of the conventions of standard English capitalization, punctuation, and spelling when writing."^^xsd:string .

:CCSS.Math.Content.HSF.BF.B.3 rdf:type owl:Class ;
    rdfs:subClassOf :CCSS.Math.Content.HSF.BF.B ;
    prov:wasQuotedFrom <http://www.corestandards.org/Math/Content/HSF/3/> ;
    rdfs:label "English Language Arts Standards - Anchor Standards - College and Career Readiness Anchor Standards for Language - 3"^^xsd:string ;
    rdfs:comment "Apply knowledge of language to understand how language functions in different contexts, to make effective choices for meaning or style, and to comprehend more fully when reading or listening. "^^xsd:string .

:CCSS.Math.Content.HSF.BF.B.4 rdf:type owl:Class ;
    rdfs:subClassOf :CCSS.Math.Content.HSF.BF.B ;
    prov:wasQuotedFrom <http://www.corestandards.org/Math/Content/HSF/4/> ;
    rdfs:label "English Language Arts Standards - Anchor Standards - College and Career Readiness Anchor Standards for Language - 4"^^xsd:string ;
    rdfs:comment "Determine or clarify the meaning of unknown and multiple-meaning words and phrases by using context clues, analyzing meaningful word parts, and consulting general and specialized reference materials, as appropriate."^^xsd:string .

:CCSS.Math.Content.HSF.BF.B.5 rdf:type owl:Class ;
    rdfs:subClassOf :CCSS.Math.Content.HSF.BF.B ;
    prov:wasQuotedFrom <http://www.corestandards.org/Math/Content/HSF/5/> ;
    rdfs:label "English Language Arts Standards - Anchor Standards - College and Career Readiness Anchor Standards for Language - 5"^^xsd:string ;
    rdfs:comment "Demonstrate understanding of figurative language, word relationships, and nuances in word meanings."^^xsd:string .

:CCSS.Math.Content.HSF.IF.A.1 rdf:type owl:Class ;
    rdfs:subClassOf :CCSS.Math.Content.HSF.IF.A ;
    prov:wasQuotedFrom <http://www.corestandards.org/Math/Content/HSF/1/> ;
    rdfs:label "English Language Arts Standards - Anchor Standards - College and Career Readiness Anchor Standards for Language - 1"^^xsd:string ;
    rdfs:comment "Demonstrate command of the conventions of standard English grammar and usage when writing or speaking."^^xsd:string .

:CCSS.Math.Content.HSF.IF.A.2 rdf:type owl:Class ;
    rdfs:subClassOf :CCSS.Math.Content.HSF.IF.A ;
    prov:wasQuotedFrom <http://www.corestandards.org/Math/Content/HSF/2/> ;
    rdfs:label "English Language Arts Standards - Anchor Standards - College and Career Readiness Anchor Standards for Language - 2"^^xsd:string ;
    rdfs:comment "Demonstrate command of the conventions of standard English capitalization, punctuation, and spelling when writing."^^xsd:string .

:CCSS.Math.Content.HSF.IF.A.3 rdf:type owl:Class ;
    rdfs:subClassOf :CCSS.Math.Content.HSF.IF.A ;
    prov:wasQuotedFrom <http://www.corestandards.org/Math/Content/HSF/3/> ;
    rdfs:label "English Language Arts Standards - Anchor Standards - College and Career Readiness Anchor Standards for Language - 3"^^xsd:string ;
    rdfs:comment "Apply knowledge of language to understand how language functions in different contexts, to make effective choices for meaning or style, and to comprehend more fully when reading or listening. "^^xsd:string .

:CCSS.Math.Content.HSF.IF.B.4 rdf:type owl:Class ;
    rdfs:subClassOf :CCSS.Math.Content.HSF.IF.B ;
    prov:wasQuotedFrom <http://www.corestandards.org/Math/Content/HSF/4/> ;
    rdfs:label "English Language Arts Standards - Anchor Standards - College and Career Readiness Anchor Standards for Language - 4"^^xsd:string ;
    rdfs:comment "Determine or clarify the meaning of unknown and multiple-meaning words and phrases by using context clues, analyzing meaningful word parts, and consulting general and specialized reference materials, as appropriate."^^xsd:string .

:CCSS.Math.Content.HSF.IF.B.5 rdf:type owl:Class ;
    rdfs:subClassOf :CCSS.Math.Content.HSF.IF.B ;
    prov:wasQuotedFrom <http://www.corestandards.org/Math/Content/HSF/5/> ;
    rdfs:label "English Language Arts Standards - Anchor Standards - College and Career Readiness Anchor Standards for Language - 5"^^xsd:string ;
    rdfs:comment "Demonstrate understanding of figurative language, word relationships, and nuances in word meanings."^^xsd:string .

:CCSS.Math.Content.HSF.IF.B.6 rdf:type owl:Class ;
    rdfs:subClassOf :CCSS.Math.Content.HSF.IF.B ;
    prov:wasQuotedFrom <http://www.corestandards.org/Math/Content/HSF/6/> ;
    rdfs:label "English Language Arts Standards - Anchor Standards - College and Career Readiness Anchor Standards for Language - 6"^^xsd:string ;
    rdfs:comment "Acquire and use accurately a range of general academic and domain-specific words and phrases sufficient for reading, writing, speaking, and listening at the college and career readiness level; demonstrate independence in gathering vocabulary knowledge when encountering an unknown term important to comprehension or expression."^^xsd:string .

:CCSS.Math.Content.HSF.IF.C.7 rdf:type owl:Class ;
    rdfs:subClassOf :CCSS.Math.Content.HSF.IF.C ;
    prov:wasQuotedFrom <http://www.corestandards.org/Math/Content/HSF/7/> ;
    rdfs:label "English Language Arts Standards - Anchor Standards - College and Career Readiness Anchor Standards for Reading - 7"^^xsd:string ;
    rdfs:comment "Integrate and evaluate content presented in diverse media and formats, including visually and quantitatively, as well as in words.1"^^xsd:string .

:CCSS.Math.Content.HSF.IF.C.8 rdf:type owl:Class ;
    rdfs:subClassOf :CCSS.Math.Content.HSF.IF.C ;
    prov:wasQuotedFrom <http://www.corestandards.org/Math/Content/HSF/8/> ;
    rdfs:label "English Language Arts Standards - Anchor Standards - College and Career Readiness Anchor Standards for Reading - 8"^^xsd:string ;
    rdfs:comment "Delineate and evaluate the argument and specific claims in a text, including the validity of the reasoning as well as the relevance and sufficiency of the evidence."^^xsd:string .

:CCSS.Math.Content.HSF.IF.C.9 rdf:type owl:Class ;
    rdfs:subClassOf :CCSS.Math.Content.HSF.IF.C ;
    prov:wasQuotedFrom <http://www.corestandards.org/Math/Content/HSF/9/> ;
    rdfs:label "English Language Arts Standards - Anchor Standards - College and Career Readiness Anchor Standards for Reading - 9"^^xsd:string ;
    rdfs:comment "Analyze how two or more texts address similar themes or topics in order to build knowledge or to compare the approaches the authors take."^^xsd:string .

:CCSS.Math.Content.HSF.LE.A.1 rdf:type owl:Class ;
    rdfs:subClassOf :CCSS.Math.Content.HSF.LE.A ;
    prov:wasQuotedFrom <http://www.corestandards.org/Math/Content/HSF/1/> ;
    rdfs:label "English Language Arts Standards - Anchor Standards - College and Career Readiness Anchor Standards for Language - 1"^^xsd:string ;
    rdfs:comment "Demonstrate command of the conventions of standard English grammar and usage when writing or speaking."^^xsd:string .

:CCSS.Math.Content.HSF.LE.A.2 rdf:type owl:Class ;
    rdfs:subClassOf :CCSS.Math.Content.HSF.LE.A ;
    prov:wasQuotedFrom <http://www.corestandards.org/Math/Content/HSF/2/> ;
    rdfs:label "English Language Arts Standards - Anchor Standards - College and Career Readiness Anchor Standards for Language - 2"^^xsd:string ;
    rdfs:comment "Demonstrate command of the conventions of standard English capitalization, punctuation, and spelling when writing."^^xsd:string .

:CCSS.Math.Content.HSF.LE.A.3 rdf:type owl:Class ;
    rdfs:subClassOf :CCSS.Math.Content.HSF.LE.A ;
    prov:wasQuotedFrom <http://www.corestandards.org/Math/Content/HSF/3/> ;
    rdfs:label "English Language Arts Standards - Anchor Standards - College and Career Readiness Anchor Standards for Language - 3"^^xsd:string ;
    rdfs:comment "Apply knowledge of language to understand how language functions in different contexts, to make effective choices for meaning or style, and to comprehend more fully when reading or listening. "^^xsd:string .

:CCSS.Math.Content.HSF.LE.A.4 rdf:type owl:Class ;
    rdfs:subClassOf :CCSS.Math.Content.HSF.LE.A ;
    prov:wasQuotedFrom <http://www.corestandards.org/Math/Content/HSF/4/> ;
    rdfs:label "English Language Arts Standards - Anchor Standards - College and Career Readiness Anchor Standards for Language - 4"^^xsd:string ;
    rdfs:comment "Determine or clarify the meaning of unknown and multiple-meaning words and phrases by using context clues, analyzing meaningful word parts, and consulting general and specialized reference materials, as appropriate."^^xsd:string .

:CCSS.Math.Content.HSF.LE.B.5 rdf:type owl:Class ;
    rdfs:subClassOf :CCSS.Math.Content.HSF.LE.B ;
    prov:wasQuotedFrom <http://www.corestandards.org/Math/Content/HSF/5/> ;
    rdfs:label "English Language Arts Standards - Anchor Standards - College and Career Readiness Anchor Standards for Language - 5"^^xsd:string ;
    rdfs:comment "Demonstrate understanding of figurative language, word relationships, and nuances in word meanings."^^xsd:string .

:CCSS.Math.Content.HSF.TF.A.1 rdf:type owl:Class ;
    rdfs:subClassOf :CCSS.Math.Content.HSF.TF.A ;
    prov:wasQuotedFrom <http://www.corestandards.org/Math/Content/HSF/1/> ;
    rdfs:label "English Language Arts Standards - Anchor Standards - College and Career Readiness Anchor Standards for Language - 1"^^xsd:string ;
    rdfs:comment "Demonstrate command of the conventions of standard English grammar and usage when writing or speaking."^^xsd:string .

:CCSS.Math.Content.HSF.TF.A.2 rdf:type owl:Class ;
    rdfs:subClassOf :CCSS.Math.Content.HSF.TF.A ;
    prov:wasQuotedFrom <http://www.corestandards.org/Math/Content/HSF/2/> ;
    rdfs:label "English Language Arts Standards - Anchor Standards - College and Career Readiness Anchor Standards for Language - 2"^^xsd:string ;
    rdfs:comment "Demonstrate command of the conventions of standard English capitalization, punctuation, and spelling when writing."^^xsd:string .

:CCSS.Math.Content.HSF.TF.A.3 rdf:type owl:Class ;
    rdfs:subClassOf :CCSS.Math.Content.HSF.TF.A ;
    prov:wasQuotedFrom <http://www.corestandards.org/Math/Content/HSF/3/> ;
    rdfs:label "English Language Arts Standards - Anchor Standards - College and Career Readiness Anchor Standards for Language - 3"^^xsd:string ;
    rdfs:comment "Apply knowledge of language to understand how language functions in different contexts, to make effective choices for meaning or style, and to comprehend more fully when reading or listening. "^^xsd:string .

:CCSS.Math.Content.HSF.TF.A.4 rdf:type owl:Class ;
    rdfs:subClassOf :CCSS.Math.Content.HSF.TF.A ;
    prov:wasQuotedFrom <http://www.corestandards.org/Math/Content/HSF/4/> ;
    rdfs:label "English Language Arts Standards - Anchor Standards - College and Career Readiness Anchor Standards for Language - 4"^^xsd:string ;
    rdfs:comment "Determine or clarify the meaning of unknown and multiple-meaning words and phrases by using context clues, analyzing meaningful word parts, and consulting general and specialized reference materials, as appropriate."^^xsd:string .

:CCSS.Math.Content.HSF.TF.B.5 rdf:type owl:Class ;
    rdfs:subClassOf :CCSS.Math.Content.HSF.TF.B ;
    prov:wasQuotedFrom <http://www.corestandards.org/Math/Content/HSF/5/> ;
    rdfs:label "English Language Arts Standards - Anchor Standards - College and Career Readiness Anchor Standards for Language - 5"^^xsd:string ;
    rdfs:comment "Demonstrate understanding of figurative language, word relationships, and nuances in word meanings."^^xsd:string .

:CCSS.Math.Content.HSF.TF.B.6 rdf:type owl:Class ;
    rdfs:subClassOf :CCSS.Math.Content.HSF.TF.B ;
    prov:wasQuotedFrom <http://www.corestandards.org/Math/Content/HSF/6/> ;
    rdfs:label "English Language Arts Standards - Anchor Standards - College and Career Readiness Anchor Standards for Language - 6"^^xsd:string ;
    rdfs:comment "Acquire and use accurately a range of general academic and domain-specific words and phrases sufficient for reading, writing, speaking, and listening at the college and career readiness level; demonstrate independence in gathering vocabulary knowledge when encountering an unknown term important to comprehension or expression."^^xsd:string .

:CCSS.Math.Content.HSF.TF.B.7 rdf:type owl:Class ;
    rdfs:subClassOf :CCSS.Math.Content.HSF.TF.B ;
    prov:wasQuotedFrom <http://www.corestandards.org/Math/Content/HSF/7/> ;
    rdfs:label "English Language Arts Standards - Anchor Standards - College and Career Readiness Anchor Standards for Reading - 7"^^xsd:string ;
    rdfs:comment "Integrate and evaluate content presented in diverse media and formats, including visually and quantitatively, as well as in words.1"^^xsd:string .

:CCSS.Math.Content.HSF.TF.C.8 rdf:type owl:Class ;
    rdfs:subClassOf :CCSS.Math.Content.HSF.TF.C ;
    prov:wasQuotedFrom <http://www.corestandards.org/Math/Content/HSF/8/> ;
    rdfs:label "English Language Arts Standards - Anchor Standards - College and Career Readiness Anchor Standards for Reading - 8"^^xsd:string ;
    rdfs:comment "Delineate and evaluate the argument and specific claims in a text, including the validity of the reasoning as well as the relevance and sufficiency of the evidence."^^xsd:string .

:CCSS.Math.Content.HSF.TF.C.9 rdf:type owl:Class ;
    rdfs:subClassOf :CCSS.Math.Content.HSF.TF.C ;
    prov:wasQuotedFrom <http://www.corestandards.org/Math/Content/HSF/9/> ;
    rdfs:label "English Language Arts Standards - Anchor Standards - College and Career Readiness Anchor Standards for Reading - 9"^^xsd:string ;
    rdfs:comment "Analyze how two or more texts address similar themes or topics in order to build knowledge or to compare the approaches the authors take."^^xsd:string .

:CCSS.Math.Content.HSF.IF.C.7.a rdf:type owl:Class ;
    rdfs:subClassOf :CCSS.Math.Content.HSF.IF.C.7 ;
    prov:wasQuotedFrom <http://www.corestandards.org/Math/Content/HSF/IF/a/> .

:CCSS.Math.Content.HSF.IF.C.7.b rdf:type owl:Class ;
    rdfs:subClassOf :CCSS.Math.Content.HSF.IF.C.7 ;
    prov:wasQuotedFrom <http://www.corestandards.org/Math/Content/HSF/IF/b/> .

:CCSS.Math.Content.HSF.IF.C.7.c rdf:type owl:Class ;
    rdfs:subClassOf :CCSS.Math.Content.HSF.IF.C.7 ;
    prov:wasQuotedFrom <http://www.corestandards.org/Math/Content/HSF/IF/c/> .

:CCSS.Math.Content.HSF.IF.C.7.d rdf:type owl:Class ;
    rdfs:subClassOf :CCSS.Math.Content.HSF.IF.C.7 ;
    prov:wasQuotedFrom <http://www.corestandards.org/Math/Content/HSF/IF/d/> .

:CCSS.Math.Content.HSF.IF.C.7.e rdf:type owl:Class ;
    rdfs:subClassOf :CCSS.Math.Content.HSF.IF.C.7 ;
    prov:wasQuotedFrom <http://www.corestandards.org/Math/Content/HSF/IF/e/> .

:CCSS.Math.Content.HSF.IF.C.8.a rdf:type owl:Class ;
    rdfs:subClassOf :CCSS.Math.Content.HSF.IF.C.8 ;
    prov:wasQuotedFrom <http://www.corestandards.org/Math/Content/HSF/IF/a/> .

:CCSS.Math.Content.HSF.IF.C.8.b rdf:type owl:Class ;
    rdfs:subClassOf :CCSS.Math.Content.HSF.IF.C.8 ;
    prov:wasQuotedFrom <http://www.corestandards.org/Math/Content/HSF/IF/b/> .

:CCSS.Math.Content.HSF.BF.A.1.a rdf:type owl:Class ;
    rdfs:subClassOf :CCSS.Math.Content.HSF.BF.A.1 ;
    prov:wasQuotedFrom <http://www.corestandards.org/Math/Content/HSF/BF/a/> .

:CCSS.Math.Content.HSF.BF.A.1.b rdf:type owl:Class ;
    rdfs:subClassOf :CCSS.Math.Content.HSF.BF.A.1 ;
    prov:wasQuotedFrom <http://www.corestandards.org/Math/Content/HSF/BF/b/> .

:CCSS.Math.Content.HSF.BF.A.1.c rdf:type owl:Class ;
    rdfs:subClassOf :CCSS.Math.Content.HSF.BF.A.1 ;
    prov:wasQuotedFrom <http://www.corestandards.org/Math/Content/HSF/BF/c/> .

:CCSS.Math.Content.HSF.BF.B.4.a rdf:type owl:Class ;
    rdfs:subClassOf :CCSS.Math.Content.HSF.BF.B.4 ;
    prov:wasQuotedFrom <http://www.corestandards.org/Math/Content/HSF/BF/a/> .

:CCSS.Math.Content.HSF.BF.B.4.b rdf:type owl:Class ;
    rdfs:subClassOf :CCSS.Math.Content.HSF.BF.B.4 ;
    prov:wasQuotedFrom <http://www.corestandards.org/Math/Content/HSF/BF/b/> .

:CCSS.Math.Content.HSF.BF.B.4.c rdf:type owl:Class ;
    rdfs:subClassOf :CCSS.Math.Content.HSF.BF.B.4 ;
    prov:wasQuotedFrom <http://www.corestandards.org/Math/Content/HSF/BF/c/> .

:CCSS.Math.Content.HSF.BF.B.4.d rdf:type owl:Class ;
    rdfs:subClassOf :CCSS.Math.Content.HSF.BF.B.4 ;
    prov:wasQuotedFrom <http://www.corestandards.org/Math/Content/HSF/BF/d/> .

:CCSS.Math.Content.HSF.LE.A.1.a rdf:type owl:Class ;
    rdfs:subClassOf :CCSS.Math.Content.HSF.LE.A.1 ;
    prov:wasQuotedFrom <http://www.corestandards.org/Math/Content/HSF/LE/a/> .

:CCSS.Math.Content.HSF.LE.A.1.b rdf:type owl:Class ;
    rdfs:subClassOf :CCSS.Math.Content.HSF.LE.A.1 ;
    prov:wasQuotedFrom <http://www.corestandards.org/Math/Content/HSF/LE/b/> .

:CCSS.Math.Content.HSF.LE.A.1.c rdf:type owl:Class ;
    rdfs:subClassOf :CCSS.Math.Content.HSF.LE.A.1 ;
    prov:wasQuotedFrom <http://www.corestandards.org/Math/Content/HSF/LE/c/> .

:CCSS.Math.Content.HSG rdf:type owl:Class ;
    rdfs:subClassOf :CCSS.Math.Content ;
    rdfs:label "High School: Geometry"^^xsd:string ;
    prov:wasQuotedFrom <http://www.corestandards.org/Math/Content/HSG/> .

:CCSS.Math.Content.HSG.introduction rdf:type owl:Class ;
    rdfs:subClassOf :CCSS.Math.Content.HSG ;
    prov:wasQuotedFrom <http://www.corestandards.org/Math/Content/HSG/introduction/> ;
    rdfs:label "High School: Geometry - Introduction"^^xsd:string ;
    rdfs:comment "An understanding of the attributes and relationships of geometric objects can be applied in diverse contexts-interpreting a schematic drawing, estimating the amount of wood needed to frame a sloping roof, rendering computer graphics, or designing a sewing pattern for the most efficient use of material."^^xsd:string .

:CCSS.Math.Content.HSG.C rdf:type owl:Class ;
    rdfs:subClassOf :CCSS.Math.Content.HSG ;
    rdfs:label "High School: Geometry"^^xsd:string ;
    prov:wasQuotedFrom <http://www.corestandards.org/Math/Content/HSG/> .

:CCSS.Math.Content.HSG.C.A rdf:type owl:Class ;
    rdfs:subClassOf :CCSS.Math.Content.HSG.C ;
    prov:wasQuotedFrom <http://www.corestandards.org/Math/Content/HSG/A/> .

:CCSS.Math.Content.HSG.C.B rdf:type owl:Class ;
    rdfs:subClassOf :CCSS.Math.Content.HSG.C ;
    prov:wasQuotedFrom <http://www.corestandards.org/Math/Content/HSG/B/> .

:CCSS.Math.Content.HSG.CO rdf:type owl:Class ;
    rdfs:subClassOf :CCSS.Math.Content.HSG ;
    rdfs:label "High School: Geometry"^^xsd:string ;
    prov:wasQuotedFrom <http://www.corestandards.org/Math/Content/HSG/> .

:CCSS.Math.Content.HSG.CO.A rdf:type owl:Class ;
    rdfs:subClassOf :CCSS.Math.Content.HSG.CO ;
    prov:wasQuotedFrom <http://www.corestandards.org/Math/Content/HSG/A/> .

:CCSS.Math.Content.HSG.CO.B rdf:type owl:Class ;
    rdfs:subClassOf :CCSS.Math.Content.HSG.CO ;
    prov:wasQuotedFrom <http://www.corestandards.org/Math/Content/HSG/B/> .

:CCSS.Math.Content.HSG.CO.C rdf:type owl:Class ;
    rdfs:subClassOf :CCSS.Math.Content.HSG.CO ;
    prov:wasQuotedFrom <http://www.corestandards.org/Math/Content/HSG/C/> ;
    rdfs:label "High School: Geometry - Circles"^^xsd:string .

:CCSS.Math.Content.HSG.CO.D rdf:type owl:Class ;
    rdfs:subClassOf :CCSS.Math.Content.HSG.CO ;
    prov:wasQuotedFrom <http://www.corestandards.org/Math/Content/HSG/D/> .

:CCSS.Math.Content.HSG.GMD rdf:type owl:Class ;
    rdfs:subClassOf :CCSS.Math.Content.HSG ;
    rdfs:label "High School: Geometry"^^xsd:string ;
    prov:wasQuotedFrom <http://www.corestandards.org/Math/Content/HSG/> .

:CCSS.Math.Content.HSG.GMD.A rdf:type owl:Class ;
    rdfs:subClassOf :CCSS.Math.Content.HSG.GMD ;
    prov:wasQuotedFrom <http://www.corestandards.org/Math/Content/HSG/A/> .

:CCSS.Math.Content.HSG.GMD.B rdf:type owl:Class ;
    rdfs:subClassOf :CCSS.Math.Content.HSG.GMD ;
    prov:wasQuotedFrom <http://www.corestandards.org/Math/Content/HSG/B/> .

:CCSS.Math.Content.HSG.GPE rdf:type owl:Class ;
    rdfs:subClassOf :CCSS.Math.Content.HSG ;
    rdfs:label "High School: Geometry"^^xsd:string ;
    prov:wasQuotedFrom <http://www.corestandards.org/Math/Content/HSG/> .

:CCSS.Math.Content.HSG.GPE.A rdf:type owl:Class ;
    rdfs:subClassOf :CCSS.Math.Content.HSG.GPE ;
    prov:wasQuotedFrom <http://www.corestandards.org/Math/Content/HSG/A/> .

:CCSS.Math.Content.HSG.GPE.B rdf:type owl:Class ;
    rdfs:subClassOf :CCSS.Math.Content.HSG.GPE ;
    prov:wasQuotedFrom <http://www.corestandards.org/Math/Content/HSG/B/> .

:CCSS.Math.Content.HSG.MG rdf:type owl:Class ;
    rdfs:subClassOf :CCSS.Math.Content.HSG ;
    rdfs:label "High School: Geometry"^^xsd:string ;
    prov:wasQuotedFrom <http://www.corestandards.org/Math/Content/HSG/> .

:CCSS.Math.Content.HSG.MG.A rdf:type owl:Class ;
    rdfs:subClassOf :CCSS.Math.Content.HSG.MG ;
    prov:wasQuotedFrom <http://www.corestandards.org/Math/Content/HSG/A/> .

:CCSS.Math.Content.HSG.SRT rdf:type owl:Class ;
    rdfs:subClassOf :CCSS.Math.Content.HSG ;
    rdfs:label "High School: Geometry"^^xsd:string ;
    prov:wasQuotedFrom <http://www.corestandards.org/Math/Content/HSG/> .

:CCSS.Math.Content.HSG.SRT.A rdf:type owl:Class ;
    rdfs:subClassOf :CCSS.Math.Content.HSG.SRT ;
    prov:wasQuotedFrom <http://www.corestandards.org/Math/Content/HSG/A/> .

:CCSS.Math.Content.HSG.SRT.B rdf:type owl:Class ;
    rdfs:subClassOf :CCSS.Math.Content.HSG.SRT ;
    prov:wasQuotedFrom <http://www.corestandards.org/Math/Content/HSG/B/> .

:CCSS.Math.Content.HSG.SRT.C rdf:type owl:Class ;
    rdfs:subClassOf :CCSS.Math.Content.HSG.SRT ;
    prov:wasQuotedFrom <http://www.corestandards.org/Math/Content/HSG/C/> ;
    rdfs:label "High School: Geometry - Circles"^^xsd:string .

:CCSS.Math.Content.HSG.SRT.D rdf:type owl:Class ;
    rdfs:subClassOf :CCSS.Math.Content.HSG.SRT ;
    prov:wasQuotedFrom <http://www.corestandards.org/Math/Content/HSG/D/> .

:CCSS.Math.Content.HSG.C.A.1 rdf:type owl:Class ;
    rdfs:subClassOf :CCSS.Math.Content.HSG.C.A ;
    prov:wasQuotedFrom <http://www.corestandards.org/Math/Content/HSG/1/> ;
    rdfs:label "English Language Arts Standards - Anchor Standards - College and Career Readiness Anchor Standards for Language - 1"^^xsd:string ;
    rdfs:comment "Demonstrate command of the conventions of standard English grammar and usage when writing or speaking."^^xsd:string .

:CCSS.Math.Content.HSG.C.A.2 rdf:type owl:Class ;
    rdfs:subClassOf :CCSS.Math.Content.HSG.C.A ;
    prov:wasQuotedFrom <http://www.corestandards.org/Math/Content/HSG/2/> ;
    rdfs:label "English Language Arts Standards - Anchor Standards - College and Career Readiness Anchor Standards for Language - 2"^^xsd:string ;
    rdfs:comment "Demonstrate command of the conventions of standard English capitalization, punctuation, and spelling when writing."^^xsd:string .

:CCSS.Math.Content.HSG.C.A.3 rdf:type owl:Class ;
    rdfs:subClassOf :CCSS.Math.Content.HSG.C.A ;
    prov:wasQuotedFrom <http://www.corestandards.org/Math/Content/HSG/3/> ;
    rdfs:label "English Language Arts Standards - Anchor Standards - College and Career Readiness Anchor Standards for Language - 3"^^xsd:string ;
    rdfs:comment "Apply knowledge of language to understand how language functions in different contexts, to make effective choices for meaning or style, and to comprehend more fully when reading or listening. "^^xsd:string .

:CCSS.Math.Content.HSG.C.A.4 rdf:type owl:Class ;
    rdfs:subClassOf :CCSS.Math.Content.HSG.C.A ;
    prov:wasQuotedFrom <http://www.corestandards.org/Math/Content/HSG/4/> ;
    rdfs:label "English Language Arts Standards - Anchor Standards - College and Career Readiness Anchor Standards for Language - 4"^^xsd:string ;
    rdfs:comment "Determine or clarify the meaning of unknown and multiple-meaning words and phrases by using context clues, analyzing meaningful word parts, and consulting general and specialized reference materials, as appropriate."^^xsd:string .

:CCSS.Math.Content.HSG.C.B.5 rdf:type owl:Class ;
    rdfs:subClassOf :CCSS.Math.Content.HSG.C.B ;
    prov:wasQuotedFrom <http://www.corestandards.org/Math/Content/HSG/5/> ;
    rdfs:label "English Language Arts Standards - Anchor Standards - College and Career Readiness Anchor Standards for Language - 5"^^xsd:string ;
    rdfs:comment "Demonstrate understanding of figurative language, word relationships, and nuances in word meanings."^^xsd:string .

:CCSS.Math.Content.HSG.CO.A.1 rdf:type owl:Class ;
    rdfs:subClassOf :CCSS.Math.Content.HSG.CO.A ;
    prov:wasQuotedFrom <http://www.corestandards.org/Math/Content/HSG/1/> ;
    rdfs:label "English Language Arts Standards - Anchor Standards - College and Career Readiness Anchor Standards for Language - 1"^^xsd:string ;
    rdfs:comment "Demonstrate command of the conventions of standard English grammar and usage when writing or speaking."^^xsd:string .

:CCSS.Math.Content.HSG.CO.A.2 rdf:type owl:Class ;
    rdfs:subClassOf :CCSS.Math.Content.HSG.CO.A ;
    prov:wasQuotedFrom <http://www.corestandards.org/Math/Content/HSG/2/> ;
    rdfs:label "English Language Arts Standards - Anchor Standards - College and Career Readiness Anchor Standards for Language - 2"^^xsd:string ;
    rdfs:comment "Demonstrate command of the conventions of standard English capitalization, punctuation, and spelling when writing."^^xsd:string .

:CCSS.Math.Content.HSG.CO.A.3 rdf:type owl:Class ;
    rdfs:subClassOf :CCSS.Math.Content.HSG.CO.A ;
    prov:wasQuotedFrom <http://www.corestandards.org/Math/Content/HSG/3/> ;
    rdfs:label "English Language Arts Standards - Anchor Standards - College and Career Readiness Anchor Standards for Language - 3"^^xsd:string ;
    rdfs:comment "Apply knowledge of language to understand how language functions in different contexts, to make effective choices for meaning or style, and to comprehend more fully when reading or listening. "^^xsd:string .

:CCSS.Math.Content.HSG.CO.A.4 rdf:type owl:Class ;
    rdfs:subClassOf :CCSS.Math.Content.HSG.CO.A ;
    prov:wasQuotedFrom <http://www.corestandards.org/Math/Content/HSG/4/> ;
    rdfs:label "English Language Arts Standards - Anchor Standards - College and Career Readiness Anchor Standards for Language - 4"^^xsd:string ;
    rdfs:comment "Determine or clarify the meaning of unknown and multiple-meaning words and phrases by using context clues, analyzing meaningful word parts, and consulting general and specialized reference materials, as appropriate."^^xsd:string .

:CCSS.Math.Content.HSG.CO.A.5 rdf:type owl:Class ;
    rdfs:subClassOf :CCSS.Math.Content.HSG.CO.A ;
    prov:wasQuotedFrom <http://www.corestandards.org/Math/Content/HSG/5/> ;
    rdfs:label "English Language Arts Standards - Anchor Standards - College and Career Readiness Anchor Standards for Language - 5"^^xsd:string ;
    rdfs:comment "Demonstrate understanding of figurative language, word relationships, and nuances in word meanings."^^xsd:string .

:CCSS.Math.Content.HSG.CO.B.6 rdf:type owl:Class ;
    rdfs:subClassOf :CCSS.Math.Content.HSG.CO.B ;
    prov:wasQuotedFrom <http://www.corestandards.org/Math/Content/HSG/6/> ;
    rdfs:label "English Language Arts Standards - Anchor Standards - College and Career Readiness Anchor Standards for Language - 6"^^xsd:string ;
    rdfs:comment "Acquire and use accurately a range of general academic and domain-specific words and phrases sufficient for reading, writing, speaking, and listening at the college and career readiness level; demonstrate independence in gathering vocabulary knowledge when encountering an unknown term important to comprehension or expression."^^xsd:string .

:CCSS.Math.Content.HSG.CO.B.7 rdf:type owl:Class ;
    rdfs:subClassOf :CCSS.Math.Content.HSG.CO.B ;
    prov:wasQuotedFrom <http://www.corestandards.org/Math/Content/HSG/7/> ;
    rdfs:label "English Language Arts Standards - Anchor Standards - College and Career Readiness Anchor Standards for Reading - 7"^^xsd:string ;
    rdfs:comment "Integrate and evaluate content presented in diverse media and formats, including visually and quantitatively, as well as in words.1"^^xsd:string .

:CCSS.Math.Content.HSG.CO.B.8 rdf:type owl:Class ;
    rdfs:subClassOf :CCSS.Math.Content.HSG.CO.B ;
    prov:wasQuotedFrom <http://www.corestandards.org/Math/Content/HSG/8/> ;
    rdfs:label "English Language Arts Standards - Anchor Standards - College and Career Readiness Anchor Standards for Reading - 8"^^xsd:string ;
    rdfs:comment "Delineate and evaluate the argument and specific claims in a text, including the validity of the reasoning as well as the relevance and sufficiency of the evidence."^^xsd:string .

:CCSS.Math.Content.HSG.CO.C.9 rdf:type owl:Class ;
    rdfs:subClassOf :CCSS.Math.Content.HSG.CO.C ;
    prov:wasQuotedFrom <http://www.corestandards.org/Math/Content/HSG/9/> ;
    rdfs:label "English Language Arts Standards - Anchor Standards - College and Career Readiness Anchor Standards for Reading - 9"^^xsd:string ;
    rdfs:comment "Analyze how two or more texts address similar themes or topics in order to build knowledge or to compare the approaches the authors take."^^xsd:string .

:CCSS.Math.Content.HSG.CO.C.10 rdf:type owl:Class ;
    rdfs:subClassOf :CCSS.Math.Content.HSG.CO.C ;
    prov:wasQuotedFrom <http://www.corestandards.org/Math/Content/HSG/10/> ;
    rdfs:label "English Language Arts Standards - Anchor Standards - College and Career Readiness Anchor Standards for Reading - 10"^^xsd:string ;
    rdfs:comment "Read and comprehend complex literary and informational texts independently and proficiently."^^xsd:string .

:CCSS.Math.Content.HSG.CO.C.11 rdf:type owl:Class ;
    rdfs:subClassOf :CCSS.Math.Content.HSG.CO.C ;
    prov:wasQuotedFrom <http://www.corestandards.org/Math/Content/HSG/11/> ;
    rdfs:label "High School: Algebra - Reasoning with Equations & Inequalities - Represent and solve equations and inequalities graphically.   - 11"^^xsd:string ;
    rdfs:comment "Explain why the x-coordinates of the points where the graphs of the equations y = f(x) and y = g(x) intersect are the solutions of the equation f(x) = g(x); find the solutions approximately, e.g., using technology to graph the functions, make tables of values, or find successive approximations. Include cases where f(x) and/or g(x) are linear, polynomial, rational, absolute value, exponential, and logarithmic functions.*"^^xsd:string .

:CCSS.Math.Content.HSG.CO.D.12 rdf:type owl:Class ;
    rdfs:subClassOf :CCSS.Math.Content.HSG.CO.D ;
    prov:wasQuotedFrom <http://www.corestandards.org/Math/Content/HSG/12/> ;
    rdfs:label "High School: Algebra - Reasoning with Equations & Inequalities - Represent and solve equations and inequalities graphically.   - 12"^^xsd:string ;
    rdfs:comment "Graph the solutions to a linear inequality in two variables as a half-plane (excluding the boundary in the case of a strict inequality), and graph the solution set to a system of linear inequalities in two variables as the intersection of the corresponding half-planes."^^xsd:string .

:CCSS.Math.Content.HSG.CO.D.13 rdf:type owl:Class ;
    rdfs:subClassOf :CCSS.Math.Content.HSG.CO.D ;
    prov:wasQuotedFrom <http://www.corestandards.org/Math/Content/HSG/13/> ;
    rdfs:label "High School: Geometry - Congruence - Make geometric constructions   - 13"^^xsd:string ;
    rdfs:comment "Construct an equilateral triangle, a square, and a regular hexagon inscribed in a circle."^^xsd:string .

:CCSS.Math.Content.HSG.GMD.A.1 rdf:type owl:Class ;
    rdfs:subClassOf :CCSS.Math.Content.HSG.GMD.A ;
    prov:wasQuotedFrom <http://www.corestandards.org/Math/Content/HSG/1/> ;
    rdfs:label "English Language Arts Standards - Anchor Standards - College and Career Readiness Anchor Standards for Language - 1"^^xsd:string ;
    rdfs:comment "Demonstrate command of the conventions of standard English grammar and usage when writing or speaking."^^xsd:string .

:CCSS.Math.Content.HSG.GMD.A.2 rdf:type owl:Class ;
    rdfs:subClassOf :CCSS.Math.Content.HSG.GMD.A ;
    prov:wasQuotedFrom <http://www.corestandards.org/Math/Content/HSG/2/> ;
    rdfs:label "English Language Arts Standards - Anchor Standards - College and Career Readiness Anchor Standards for Language - 2"^^xsd:string ;
    rdfs:comment "Demonstrate command of the conventions of standard English capitalization, punctuation, and spelling when writing."^^xsd:string .

:CCSS.Math.Content.HSG.GMD.A.3 rdf:type owl:Class ;
    rdfs:subClassOf :CCSS.Math.Content.HSG.GMD.A ;
    prov:wasQuotedFrom <http://www.corestandards.org/Math/Content/HSG/3/> ;
    rdfs:label "English Language Arts Standards - Anchor Standards - College and Career Readiness Anchor Standards for Language - 3"^^xsd:string ;
    rdfs:comment "Apply knowledge of language to understand how language functions in different contexts, to make effective choices for meaning or style, and to comprehend more fully when reading or listening. "^^xsd:string .

:CCSS.Math.Content.HSG.GMD.B.4 rdf:type owl:Class ;
    rdfs:subClassOf :CCSS.Math.Content.HSG.GMD.B ;
    prov:wasQuotedFrom <http://www.corestandards.org/Math/Content/HSG/4/> ;
    rdfs:label "English Language Arts Standards - Anchor Standards - College and Career Readiness Anchor Standards for Language - 4"^^xsd:string ;
    rdfs:comment "Determine or clarify the meaning of unknown and multiple-meaning words and phrases by using context clues, analyzing meaningful word parts, and consulting general and specialized reference materials, as appropriate."^^xsd:string .

:CCSS.Math.Content.HSG.GPE.A.1 rdf:type owl:Class ;
    rdfs:subClassOf :CCSS.Math.Content.HSG.GPE.A ;
    prov:wasQuotedFrom <http://www.corestandards.org/Math/Content/HSG/1/> ;
    rdfs:label "English Language Arts Standards - Anchor Standards - College and Career Readiness Anchor Standards for Language - 1"^^xsd:string ;
    rdfs:comment "Demonstrate command of the conventions of standard English grammar and usage when writing or speaking."^^xsd:string .

:CCSS.Math.Content.HSG.GPE.A.2 rdf:type owl:Class ;
    rdfs:subClassOf :CCSS.Math.Content.HSG.GPE.A ;
    prov:wasQuotedFrom <http://www.corestandards.org/Math/Content/HSG/2/> ;
    rdfs:label "English Language Arts Standards - Anchor Standards - College and Career Readiness Anchor Standards for Language - 2"^^xsd:string ;
    rdfs:comment "Demonstrate command of the conventions of standard English capitalization, punctuation, and spelling when writing."^^xsd:string .

:CCSS.Math.Content.HSG.GPE.A.3 rdf:type owl:Class ;
    rdfs:subClassOf :CCSS.Math.Content.HSG.GPE.A ;
    prov:wasQuotedFrom <http://www.corestandards.org/Math/Content/HSG/3/> ;
    rdfs:label "English Language Arts Standards - Anchor Standards - College and Career Readiness Anchor Standards for Language - 3"^^xsd:string ;
    rdfs:comment "Apply knowledge of language to understand how language functions in different contexts, to make effective choices for meaning or style, and to comprehend more fully when reading or listening. "^^xsd:string .

:CCSS.Math.Content.HSG.GPE.B.4 rdf:type owl:Class ;
    rdfs:subClassOf :CCSS.Math.Content.HSG.GPE.B ;
    prov:wasQuotedFrom <http://www.corestandards.org/Math/Content/HSG/4/> ;
    rdfs:label "English Language Arts Standards - Anchor Standards - College and Career Readiness Anchor Standards for Language - 4"^^xsd:string ;
    rdfs:comment "Determine or clarify the meaning of unknown and multiple-meaning words and phrases by using context clues, analyzing meaningful word parts, and consulting general and specialized reference materials, as appropriate."^^xsd:string .

:CCSS.Math.Content.HSG.GPE.B.5 rdf:type owl:Class ;
    rdfs:subClassOf :CCSS.Math.Content.HSG.GPE.B ;
    prov:wasQuotedFrom <http://www.corestandards.org/Math/Content/HSG/5/> ;
    rdfs:label "English Language Arts Standards - Anchor Standards - College and Career Readiness Anchor Standards for Language - 5"^^xsd:string ;
    rdfs:comment "Demonstrate understanding of figurative language, word relationships, and nuances in word meanings."^^xsd:string .

:CCSS.Math.Content.HSG.GPE.B.6 rdf:type owl:Class ;
    rdfs:subClassOf :CCSS.Math.Content.HSG.GPE.B ;
    prov:wasQuotedFrom <http://www.corestandards.org/Math/Content/HSG/6/> ;
    rdfs:label "English Language Arts Standards - Anchor Standards - College and Career Readiness Anchor Standards for Language - 6"^^xsd:string ;
    rdfs:comment "Acquire and use accurately a range of general academic and domain-specific words and phrases sufficient for reading, writing, speaking, and listening at the college and career readiness level; demonstrate independence in gathering vocabulary knowledge when encountering an unknown term important to comprehension or expression."^^xsd:string .

:CCSS.Math.Content.HSG.GPE.B.7 rdf:type owl:Class ;
    rdfs:subClassOf :CCSS.Math.Content.HSG.GPE.B ;
    prov:wasQuotedFrom <http://www.corestandards.org/Math/Content/HSG/7/> ;
    rdfs:label "English Language Arts Standards - Anchor Standards - College and Career Readiness Anchor Standards for Reading - 7"^^xsd:string ;
    rdfs:comment "Integrate and evaluate content presented in diverse media and formats, including visually and quantitatively, as well as in words.1"^^xsd:string .

:CCSS.Math.Content.HSG.MG.A.1 rdf:type owl:Class ;
    rdfs:subClassOf :CCSS.Math.Content.HSG.MG.A ;
    prov:wasQuotedFrom <http://www.corestandards.org/Math/Content/HSG/1/> ;
    rdfs:label "English Language Arts Standards - Anchor Standards - College and Career Readiness Anchor Standards for Language - 1"^^xsd:string ;
    rdfs:comment "Demonstrate command of the conventions of standard English grammar and usage when writing or speaking."^^xsd:string .

:CCSS.Math.Content.HSG.MG.A.2 rdf:type owl:Class ;
    rdfs:subClassOf :CCSS.Math.Content.HSG.MG.A ;
    prov:wasQuotedFrom <http://www.corestandards.org/Math/Content/HSG/2/> ;
    rdfs:label "English Language Arts Standards - Anchor Standards - College and Career Readiness Anchor Standards for Language - 2"^^xsd:string ;
    rdfs:comment "Demonstrate command of the conventions of standard English capitalization, punctuation, and spelling when writing."^^xsd:string .

:CCSS.Math.Content.HSG.MG.A.3 rdf:type owl:Class ;
    rdfs:subClassOf :CCSS.Math.Content.HSG.MG.A ;
    prov:wasQuotedFrom <http://www.corestandards.org/Math/Content/HSG/3/> ;
    rdfs:label "English Language Arts Standards - Anchor Standards - College and Career Readiness Anchor Standards for Language - 3"^^xsd:string ;
    rdfs:comment "Apply knowledge of language to understand how language functions in different contexts, to make effective choices for meaning or style, and to comprehend more fully when reading or listening. "^^xsd:string .

:CCSS.Math.Content.HSG.SRT.A.1 rdf:type owl:Class ;
    rdfs:subClassOf :CCSS.Math.Content.HSG.SRT.A ;
    prov:wasQuotedFrom <http://www.corestandards.org/Math/Content/HSG/1/> ;
    rdfs:label "English Language Arts Standards - Anchor Standards - College and Career Readiness Anchor Standards for Language - 1"^^xsd:string ;
    rdfs:comment "Demonstrate command of the conventions of standard English grammar and usage when writing or speaking."^^xsd:string .

:CCSS.Math.Content.HSG.SRT.A.2 rdf:type owl:Class ;
    rdfs:subClassOf :CCSS.Math.Content.HSG.SRT.A ;
    prov:wasQuotedFrom <http://www.corestandards.org/Math/Content/HSG/2/> ;
    rdfs:label "English Language Arts Standards - Anchor Standards - College and Career Readiness Anchor Standards for Language - 2"^^xsd:string ;
    rdfs:comment "Demonstrate command of the conventions of standard English capitalization, punctuation, and spelling when writing."^^xsd:string .

:CCSS.Math.Content.HSG.SRT.A.3 rdf:type owl:Class ;
    rdfs:subClassOf :CCSS.Math.Content.HSG.SRT.A ;
    prov:wasQuotedFrom <http://www.corestandards.org/Math/Content/HSG/3/> ;
    rdfs:label "English Language Arts Standards - Anchor Standards - College and Career Readiness Anchor Standards for Language - 3"^^xsd:string ;
    rdfs:comment "Apply knowledge of language to understand how language functions in different contexts, to make effective choices for meaning or style, and to comprehend more fully when reading or listening. "^^xsd:string .

:CCSS.Math.Content.HSG.SRT.B.4 rdf:type owl:Class ;
    rdfs:subClassOf :CCSS.Math.Content.HSG.SRT.B ;
    prov:wasQuotedFrom <http://www.corestandards.org/Math/Content/HSG/4/> ;
    rdfs:label "English Language Arts Standards - Anchor Standards - College and Career Readiness Anchor Standards for Language - 4"^^xsd:string ;
    rdfs:comment "Determine or clarify the meaning of unknown and multiple-meaning words and phrases by using context clues, analyzing meaningful word parts, and consulting general and specialized reference materials, as appropriate."^^xsd:string .

:CCSS.Math.Content.HSG.SRT.B.5 rdf:type owl:Class ;
    rdfs:subClassOf :CCSS.Math.Content.HSG.SRT.B ;
    prov:wasQuotedFrom <http://www.corestandards.org/Math/Content/HSG/5/> ;
    rdfs:label "English Language Arts Standards - Anchor Standards - College and Career Readiness Anchor Standards for Language - 5"^^xsd:string ;
    rdfs:comment "Demonstrate understanding of figurative language, word relationships, and nuances in word meanings."^^xsd:string .

:CCSS.Math.Content.HSG.SRT.C.6 rdf:type owl:Class ;
    rdfs:subClassOf :CCSS.Math.Content.HSG.SRT.C ;
    prov:wasQuotedFrom <http://www.corestandards.org/Math/Content/HSG/6/> ;
    rdfs:label "English Language Arts Standards - Anchor Standards - College and Career Readiness Anchor Standards for Language - 6"^^xsd:string ;
    rdfs:comment "Acquire and use accurately a range of general academic and domain-specific words and phrases sufficient for reading, writing, speaking, and listening at the college and career readiness level; demonstrate independence in gathering vocabulary knowledge when encountering an unknown term important to comprehension or expression."^^xsd:string .

:CCSS.Math.Content.HSG.SRT.C.7 rdf:type owl:Class ;
    rdfs:subClassOf :CCSS.Math.Content.HSG.SRT.C ;
    prov:wasQuotedFrom <http://www.corestandards.org/Math/Content/HSG/7/> ;
    rdfs:label "English Language Arts Standards - Anchor Standards - College and Career Readiness Anchor Standards for Reading - 7"^^xsd:string ;
    rdfs:comment "Integrate and evaluate content presented in diverse media and formats, including visually and quantitatively, as well as in words.1"^^xsd:string .

:CCSS.Math.Content.HSG.SRT.C.8 rdf:type owl:Class ;
    rdfs:subClassOf :CCSS.Math.Content.HSG.SRT.C ;
    prov:wasQuotedFrom <http://www.corestandards.org/Math/Content/HSG/8/> ;
    rdfs:label "English Language Arts Standards - Anchor Standards - College and Career Readiness Anchor Standards for Reading - 8"^^xsd:string ;
    rdfs:comment "Delineate and evaluate the argument and specific claims in a text, including the validity of the reasoning as well as the relevance and sufficiency of the evidence."^^xsd:string .

:CCSS.Math.Content.HSG.SRT.D.9 rdf:type owl:Class ;
    rdfs:subClassOf :CCSS.Math.Content.HSG.SRT.D ;
    prov:wasQuotedFrom <http://www.corestandards.org/Math/Content/HSG/9/> ;
    rdfs:label "English Language Arts Standards - Anchor Standards - College and Career Readiness Anchor Standards for Reading - 9"^^xsd:string ;
    rdfs:comment "Analyze how two or more texts address similar themes or topics in order to build knowledge or to compare the approaches the authors take."^^xsd:string .

:CCSS.Math.Content.HSG.SRT.D.10 rdf:type owl:Class ;
    rdfs:subClassOf :CCSS.Math.Content.HSG.SRT.D ;
    prov:wasQuotedFrom <http://www.corestandards.org/Math/Content/HSG/10/> ;
    rdfs:label "English Language Arts Standards - Anchor Standards - College and Career Readiness Anchor Standards for Reading - 10"^^xsd:string ;
    rdfs:comment "Read and comprehend complex literary and informational texts independently and proficiently."^^xsd:string .

:CCSS.Math.Content.HSG.SRT.D.11 rdf:type owl:Class ;
    rdfs:subClassOf :CCSS.Math.Content.HSG.SRT.D ;
    prov:wasQuotedFrom <http://www.corestandards.org/Math/Content/HSG/11/> ;
    rdfs:label "High School: Algebra - Reasoning with Equations & Inequalities - Represent and solve equations and inequalities graphically.   - 11"^^xsd:string ;
    rdfs:comment "Explain why the x-coordinates of the points where the graphs of the equations y = f(x) and y = g(x) intersect are the solutions of the equation f(x) = g(x); find the solutions approximately, e.g., using technology to graph the functions, make tables of values, or find successive approximations. Include cases where f(x) and/or g(x) are linear, polynomial, rational, absolute value, exponential, and logarithmic functions.*"^^xsd:string .

:CCSS.Math.Content.HSG.SRT.A.1.a rdf:type owl:Class ;
    rdfs:subClassOf :CCSS.Math.Content.HSG.SRT.A.1 ;
    prov:wasQuotedFrom <http://www.corestandards.org/Math/Content/HSG/SRT/a/> .

:CCSS.Math.Content.HSG.SRT.A.1.b rdf:type owl:Class ;
    rdfs:subClassOf :CCSS.Math.Content.HSG.SRT.A.1 ;
    prov:wasQuotedFrom <http://www.corestandards.org/Math/Content/HSG/SRT/b/> .

:CCSS.Math.Content.HSS rdf:type owl:Class ;
    rdfs:subClassOf :CCSS.Math.Content ;
    rdfs:label "High School: Statistics & Probability"^^xsd:string ;
    prov:wasQuotedFrom <http://www.corestandards.org/Math/Content/HSS/> .

:CCSS.Math.Content.HSS.introduction rdf:type owl:Class ;
    rdfs:subClassOf :CCSS.Math.Content.HSS ;
    prov:wasQuotedFrom <http://www.corestandards.org/Math/Content/HSS/introduction/> ;
    rdfs:label "High School: Statistics & Probability - Introduction"^^xsd:string ;
    rdfs:comment "Decisions or predictions are often based on data-numbers in context. These decisions or predictions would be easy if the data always sent a clear message, but the message is often obscured by variability. Statistics provides tools for describing variability in data and for making informed decisions that take it into account."^^xsd:string .

:CCSS.Math.Content.HSS.CP rdf:type owl:Class ;
    rdfs:subClassOf :CCSS.Math.Content.HSS ;
    rdfs:label "High School: Statistics & Probability"^^xsd:string ;
    prov:wasQuotedFrom <http://www.corestandards.org/Math/Content/HSS/> .

:CCSS.Math.Content.HSS.CP.A rdf:type owl:Class ;
    rdfs:subClassOf :CCSS.Math.Content.HSS.CP ;
    prov:wasQuotedFrom <http://www.corestandards.org/Math/Content/HSS/A/> .

:CCSS.Math.Content.HSS.CP.B rdf:type owl:Class ;
    rdfs:subClassOf :CCSS.Math.Content.HSS.CP ;
    prov:wasQuotedFrom <http://www.corestandards.org/Math/Content/HSS/B/> .

:CCSS.Math.Content.HSS.IC rdf:type owl:Class ;
    rdfs:subClassOf :CCSS.Math.Content.HSS ;
    rdfs:label "High School: Statistics & Probability"^^xsd:string ;
    prov:wasQuotedFrom <http://www.corestandards.org/Math/Content/HSS/> .

:CCSS.Math.Content.HSS.IC.A rdf:type owl:Class ;
    rdfs:subClassOf :CCSS.Math.Content.HSS.IC ;
    prov:wasQuotedFrom <http://www.corestandards.org/Math/Content/HSS/A/> .

:CCSS.Math.Content.HSS.IC.B rdf:type owl:Class ;
    rdfs:subClassOf :CCSS.Math.Content.HSS.IC ;
    prov:wasQuotedFrom <http://www.corestandards.org/Math/Content/HSS/B/> .

:CCSS.Math.Content.HSS.ID rdf:type owl:Class ;
    rdfs:subClassOf :CCSS.Math.Content.HSS ;
    rdfs:label "High School: Statistics & Probability"^^xsd:string ;
    prov:wasQuotedFrom <http://www.corestandards.org/Math/Content/HSS/> .

:CCSS.Math.Content.HSS.ID.A rdf:type owl:Class ;
    rdfs:subClassOf :CCSS.Math.Content.HSS.ID ;
    prov:wasQuotedFrom <http://www.corestandards.org/Math/Content/HSS/A/> .

:CCSS.Math.Content.HSS.ID.B rdf:type owl:Class ;
    rdfs:subClassOf :CCSS.Math.Content.HSS.ID ;
    prov:wasQuotedFrom <http://www.corestandards.org/Math/Content/HSS/B/> .

:CCSS.Math.Content.HSS.ID.C rdf:type owl:Class ;
    rdfs:subClassOf :CCSS.Math.Content.HSS.ID ;
    prov:wasQuotedFrom <http://www.corestandards.org/Math/Content/HSS/C/> .

:CCSS.Math.Content.HSS.MD rdf:type owl:Class ;
    rdfs:subClassOf :CCSS.Math.Content.HSS ;
    rdfs:label "High School: Statistics & Probability"^^xsd:string ;
    prov:wasQuotedFrom <http://www.corestandards.org/Math/Content/HSS/> .

:CCSS.Math.Content.HSS.MD.A rdf:type owl:Class ;
    rdfs:subClassOf :CCSS.Math.Content.HSS.MD ;
    prov:wasQuotedFrom <http://www.corestandards.org/Math/Content/HSS/A/> .

:CCSS.Math.Content.HSS.MD.B rdf:type owl:Class ;
    rdfs:subClassOf :CCSS.Math.Content.HSS.MD ;
    prov:wasQuotedFrom <http://www.corestandards.org/Math/Content/HSS/B/> .

:CCSS.Math.Content.HSS.CP.A.1 rdf:type owl:Class ;
    rdfs:subClassOf :CCSS.Math.Content.HSS.CP.A ;
    prov:wasQuotedFrom <http://www.corestandards.org/Math/Content/HSS/1/> ;
    rdfs:label "English Language Arts Standards - Anchor Standards - College and Career Readiness Anchor Standards for Language - 1"^^xsd:string ;
    rdfs:comment "Demonstrate command of the conventions of standard English grammar and usage when writing or speaking."^^xsd:string .

:CCSS.Math.Content.HSS.CP.A.2 rdf:type owl:Class ;
    rdfs:subClassOf :CCSS.Math.Content.HSS.CP.A ;
    prov:wasQuotedFrom <http://www.corestandards.org/Math/Content/HSS/2/> ;
    rdfs:label "English Language Arts Standards - Anchor Standards - College and Career Readiness Anchor Standards for Language - 2"^^xsd:string ;
    rdfs:comment "Demonstrate command of the conventions of standard English capitalization, punctuation, and spelling when writing."^^xsd:string .

:CCSS.Math.Content.HSS.CP.A.3 rdf:type owl:Class ;
    rdfs:subClassOf :CCSS.Math.Content.HSS.CP.A ;
    prov:wasQuotedFrom <http://www.corestandards.org/Math/Content/HSS/3/> ;
    rdfs:label "English Language Arts Standards - Anchor Standards - College and Career Readiness Anchor Standards for Language - 3"^^xsd:string ;
    rdfs:comment "Apply knowledge of language to understand how language functions in different contexts, to make effective choices for meaning or style, and to comprehend more fully when reading or listening. "^^xsd:string .

:CCSS.Math.Content.HSS.CP.A.4 rdf:type owl:Class ;
    rdfs:subClassOf :CCSS.Math.Content.HSS.CP.A ;
    prov:wasQuotedFrom <http://www.corestandards.org/Math/Content/HSS/4/> ;
    rdfs:label "English Language Arts Standards - Anchor Standards - College and Career Readiness Anchor Standards for Language - 4"^^xsd:string ;
    rdfs:comment "Determine or clarify the meaning of unknown and multiple-meaning words and phrases by using context clues, analyzing meaningful word parts, and consulting general and specialized reference materials, as appropriate."^^xsd:string .

:CCSS.Math.Content.HSS.CP.A.5 rdf:type owl:Class ;
    rdfs:subClassOf :CCSS.Math.Content.HSS.CP.A ;
    prov:wasQuotedFrom <http://www.corestandards.org/Math/Content/HSS/5/> ;
    rdfs:label "English Language Arts Standards - Anchor Standards - College and Career Readiness Anchor Standards for Language - 5"^^xsd:string ;
    rdfs:comment "Demonstrate understanding of figurative language, word relationships, and nuances in word meanings."^^xsd:string .

:CCSS.Math.Content.HSS.CP.B.6 rdf:type owl:Class ;
    rdfs:subClassOf :CCSS.Math.Content.HSS.CP.B ;
    prov:wasQuotedFrom <http://www.corestandards.org/Math/Content/HSS/6/> ;
    rdfs:label "English Language Arts Standards - Anchor Standards - College and Career Readiness Anchor Standards for Language - 6"^^xsd:string ;
    rdfs:comment "Acquire and use accurately a range of general academic and domain-specific words and phrases sufficient for reading, writing, speaking, and listening at the college and career readiness level; demonstrate independence in gathering vocabulary knowledge when encountering an unknown term important to comprehension or expression."^^xsd:string .

:CCSS.Math.Content.HSS.CP.B.7 rdf:type owl:Class ;
    rdfs:subClassOf :CCSS.Math.Content.HSS.CP.B ;
    prov:wasQuotedFrom <http://www.corestandards.org/Math/Content/HSS/7/> ;
    rdfs:label "English Language Arts Standards - Anchor Standards - College and Career Readiness Anchor Standards for Reading - 7"^^xsd:string ;
    rdfs:comment "Integrate and evaluate content presented in diverse media and formats, including visually and quantitatively, as well as in words.1"^^xsd:string .

:CCSS.Math.Content.HSS.CP.B.8 rdf:type owl:Class ;
    rdfs:subClassOf :CCSS.Math.Content.HSS.CP.B ;
    prov:wasQuotedFrom <http://www.corestandards.org/Math/Content/HSS/8/> ;
    rdfs:label "English Language Arts Standards - Anchor Standards - College and Career Readiness Anchor Standards for Reading - 8"^^xsd:string ;
    rdfs:comment "Delineate and evaluate the argument and specific claims in a text, including the validity of the reasoning as well as the relevance and sufficiency of the evidence."^^xsd:string .

:CCSS.Math.Content.HSS.CP.B.9 rdf:type owl:Class ;
    rdfs:subClassOf :CCSS.Math.Content.HSS.CP.B ;
    prov:wasQuotedFrom <http://www.corestandards.org/Math/Content/HSS/9/> ;
    rdfs:label "English Language Arts Standards - Anchor Standards - College and Career Readiness Anchor Standards for Reading - 9"^^xsd:string ;
    rdfs:comment "Analyze how two or more texts address similar themes or topics in order to build knowledge or to compare the approaches the authors take."^^xsd:string .

:CCSS.Math.Content.HSS.IC.A.1 rdf:type owl:Class ;
    rdfs:subClassOf :CCSS.Math.Content.HSS.IC.A ;
    prov:wasQuotedFrom <http://www.corestandards.org/Math/Content/HSS/1/> ;
    rdfs:label "English Language Arts Standards - Anchor Standards - College and Career Readiness Anchor Standards for Language - 1"^^xsd:string ;
    rdfs:comment "Demonstrate command of the conventions of standard English grammar and usage when writing or speaking."^^xsd:string .

:CCSS.Math.Content.HSS.IC.A.2 rdf:type owl:Class ;
    rdfs:subClassOf :CCSS.Math.Content.HSS.IC.A ;
    prov:wasQuotedFrom <http://www.corestandards.org/Math/Content/HSS/2/> ;
    rdfs:label "English Language Arts Standards - Anchor Standards - College and Career Readiness Anchor Standards for Language - 2"^^xsd:string ;
    rdfs:comment "Demonstrate command of the conventions of standard English capitalization, punctuation, and spelling when writing."^^xsd:string .

:CCSS.Math.Content.HSS.IC.B.3 rdf:type owl:Class ;
    rdfs:subClassOf :CCSS.Math.Content.HSS.IC.B ;
    prov:wasQuotedFrom <http://www.corestandards.org/Math/Content/HSS/3/> ;
    rdfs:label "English Language Arts Standards - Anchor Standards - College and Career Readiness Anchor Standards for Language - 3"^^xsd:string ;
    rdfs:comment "Apply knowledge of language to understand how language functions in different contexts, to make effective choices for meaning or style, and to comprehend more fully when reading or listening. "^^xsd:string .

:CCSS.Math.Content.HSS.IC.B.4 rdf:type owl:Class ;
    rdfs:subClassOf :CCSS.Math.Content.HSS.IC.B ;
    prov:wasQuotedFrom <http://www.corestandards.org/Math/Content/HSS/4/> ;
    rdfs:label "English Language Arts Standards - Anchor Standards - College and Career Readiness Anchor Standards for Language - 4"^^xsd:string ;
    rdfs:comment "Determine or clarify the meaning of unknown and multiple-meaning words and phrases by using context clues, analyzing meaningful word parts, and consulting general and specialized reference materials, as appropriate."^^xsd:string .

:CCSS.Math.Content.HSS.IC.B.5 rdf:type owl:Class ;
    rdfs:subClassOf :CCSS.Math.Content.HSS.IC.B ;
    prov:wasQuotedFrom <http://www.corestandards.org/Math/Content/HSS/5/> ;
    rdfs:label "English Language Arts Standards - Anchor Standards - College and Career Readiness Anchor Standards for Language - 5"^^xsd:string ;
    rdfs:comment "Demonstrate understanding of figurative language, word relationships, and nuances in word meanings."^^xsd:string .

:CCSS.Math.Content.HSS.IC.B.6 rdf:type owl:Class ;
    rdfs:subClassOf :CCSS.Math.Content.HSS.IC.B ;
    prov:wasQuotedFrom <http://www.corestandards.org/Math/Content/HSS/6/> ;
    rdfs:label "English Language Arts Standards - Anchor Standards - College and Career Readiness Anchor Standards for Language - 6"^^xsd:string ;
    rdfs:comment "Acquire and use accurately a range of general academic and domain-specific words and phrases sufficient for reading, writing, speaking, and listening at the college and career readiness level; demonstrate independence in gathering vocabulary knowledge when encountering an unknown term important to comprehension or expression."^^xsd:string .

:CCSS.Math.Content.HSS.ID.A.1 rdf:type owl:Class ;
    rdfs:subClassOf :CCSS.Math.Content.HSS.ID.A ;
    prov:wasQuotedFrom <http://www.corestandards.org/Math/Content/HSS/1/> ;
    rdfs:label "English Language Arts Standards - Anchor Standards - College and Career Readiness Anchor Standards for Language - 1"^^xsd:string ;
    rdfs:comment "Demonstrate command of the conventions of standard English grammar and usage when writing or speaking."^^xsd:string .

:CCSS.Math.Content.HSS.ID.A.2 rdf:type owl:Class ;
    rdfs:subClassOf :CCSS.Math.Content.HSS.ID.A ;
    prov:wasQuotedFrom <http://www.corestandards.org/Math/Content/HSS/2/> ;
    rdfs:label "English Language Arts Standards - Anchor Standards - College and Career Readiness Anchor Standards for Language - 2"^^xsd:string ;
    rdfs:comment "Demonstrate command of the conventions of standard English capitalization, punctuation, and spelling when writing."^^xsd:string .

:CCSS.Math.Content.HSS.ID.A.3 rdf:type owl:Class ;
    rdfs:subClassOf :CCSS.Math.Content.HSS.ID.A ;
    prov:wasQuotedFrom <http://www.corestandards.org/Math/Content/HSS/3/> ;
    rdfs:label "English Language Arts Standards - Anchor Standards - College and Career Readiness Anchor Standards for Language - 3"^^xsd:string ;
    rdfs:comment "Apply knowledge of language to understand how language functions in different contexts, to make effective choices for meaning or style, and to comprehend more fully when reading or listening. "^^xsd:string .

:CCSS.Math.Content.HSS.ID.A.4 rdf:type owl:Class ;
    rdfs:subClassOf :CCSS.Math.Content.HSS.ID.A ;
    prov:wasQuotedFrom <http://www.corestandards.org/Math/Content/HSS/4/> ;
    rdfs:label "English Language Arts Standards - Anchor Standards - College and Career Readiness Anchor Standards for Language - 4"^^xsd:string ;
    rdfs:comment "Determine or clarify the meaning of unknown and multiple-meaning words and phrases by using context clues, analyzing meaningful word parts, and consulting general and specialized reference materials, as appropriate."^^xsd:string .

:CCSS.Math.Content.HSS.ID.B.5 rdf:type owl:Class ;
    rdfs:subClassOf :CCSS.Math.Content.HSS.ID.B ;
    prov:wasQuotedFrom <http://www.corestandards.org/Math/Content/HSS/5/> ;
    rdfs:label "English Language Arts Standards - Anchor Standards - College and Career Readiness Anchor Standards for Language - 5"^^xsd:string ;
    rdfs:comment "Demonstrate understanding of figurative language, word relationships, and nuances in word meanings."^^xsd:string .

:CCSS.Math.Content.HSS.ID.B.6 rdf:type owl:Class ;
    rdfs:subClassOf :CCSS.Math.Content.HSS.ID.B ;
    prov:wasQuotedFrom <http://www.corestandards.org/Math/Content/HSS/6/> ;
    rdfs:label "English Language Arts Standards - Anchor Standards - College and Career Readiness Anchor Standards for Language - 6"^^xsd:string ;
    rdfs:comment "Acquire and use accurately a range of general academic and domain-specific words and phrases sufficient for reading, writing, speaking, and listening at the college and career readiness level; demonstrate independence in gathering vocabulary knowledge when encountering an unknown term important to comprehension or expression."^^xsd:string .

:CCSS.Math.Content.HSS.ID.C.7 rdf:type owl:Class ;
    rdfs:subClassOf :CCSS.Math.Content.HSS.ID.C ;
    prov:wasQuotedFrom <http://www.corestandards.org/Math/Content/HSS/7/> ;
    rdfs:label "English Language Arts Standards - Anchor Standards - College and Career Readiness Anchor Standards for Reading - 7"^^xsd:string ;
    rdfs:comment "Integrate and evaluate content presented in diverse media and formats, including visually and quantitatively, as well as in words.1"^^xsd:string .

:CCSS.Math.Content.HSS.ID.C.8 rdf:type owl:Class ;
    rdfs:subClassOf :CCSS.Math.Content.HSS.ID.C ;
    prov:wasQuotedFrom <http://www.corestandards.org/Math/Content/HSS/8/> ;
    rdfs:label "English Language Arts Standards - Anchor Standards - College and Career Readiness Anchor Standards for Reading - 8"^^xsd:string ;
    rdfs:comment "Delineate and evaluate the argument and specific claims in a text, including the validity of the reasoning as well as the relevance and sufficiency of the evidence."^^xsd:string .

:CCSS.Math.Content.HSS.ID.C.9 rdf:type owl:Class ;
    rdfs:subClassOf :CCSS.Math.Content.HSS.ID.C ;
    prov:wasQuotedFrom <http://www.corestandards.org/Math/Content/HSS/9/> ;
    rdfs:label "English Language Arts Standards - Anchor Standards - College and Career Readiness Anchor Standards for Reading - 9"^^xsd:string ;
    rdfs:comment "Analyze how two or more texts address similar themes or topics in order to build knowledge or to compare the approaches the authors take."^^xsd:string .

:CCSS.Math.Content.HSS.MD.A.1 rdf:type owl:Class ;
    rdfs:subClassOf :CCSS.Math.Content.HSS.MD.A ;
    prov:wasQuotedFrom <http://www.corestandards.org/Math/Content/HSS/1/> ;
    rdfs:label "English Language Arts Standards - Anchor Standards - College and Career Readiness Anchor Standards for Language - 1"^^xsd:string ;
    rdfs:comment "Demonstrate command of the conventions of standard English grammar and usage when writing or speaking."^^xsd:string .

:CCSS.Math.Content.HSS.MD.A.2 rdf:type owl:Class ;
    rdfs:subClassOf :CCSS.Math.Content.HSS.MD.A ;
    prov:wasQuotedFrom <http://www.corestandards.org/Math/Content/HSS/2/> ;
    rdfs:label "English Language Arts Standards - Anchor Standards - College and Career Readiness Anchor Standards for Language - 2"^^xsd:string ;
    rdfs:comment "Demonstrate command of the conventions of standard English capitalization, punctuation, and spelling when writing."^^xsd:string .

:CCSS.Math.Content.HSS.MD.A.3 rdf:type owl:Class ;
    rdfs:subClassOf :CCSS.Math.Content.HSS.MD.A ;
    prov:wasQuotedFrom <http://www.corestandards.org/Math/Content/HSS/3/> ;
    rdfs:label "English Language Arts Standards - Anchor Standards - College and Career Readiness Anchor Standards for Language - 3"^^xsd:string ;
    rdfs:comment "Apply knowledge of language to understand how language functions in different contexts, to make effective choices for meaning or style, and to comprehend more fully when reading or listening. "^^xsd:string .

:CCSS.Math.Content.HSS.MD.A.4 rdf:type owl:Class ;
    rdfs:subClassOf :CCSS.Math.Content.HSS.MD.A ;
    prov:wasQuotedFrom <http://www.corestandards.org/Math/Content/HSS/4/> ;
    rdfs:label "English Language Arts Standards - Anchor Standards - College and Career Readiness Anchor Standards for Language - 4"^^xsd:string ;
    rdfs:comment "Determine or clarify the meaning of unknown and multiple-meaning words and phrases by using context clues, analyzing meaningful word parts, and consulting general and specialized reference materials, as appropriate."^^xsd:string .

:CCSS.Math.Content.HSS.MD.B.5 rdf:type owl:Class ;
    rdfs:subClassOf :CCSS.Math.Content.HSS.MD.B ;
    prov:wasQuotedFrom <http://www.corestandards.org/Math/Content/HSS/5/> ;
    rdfs:label "English Language Arts Standards - Anchor Standards - College and Career Readiness Anchor Standards for Language - 5"^^xsd:string ;
    rdfs:comment "Demonstrate understanding of figurative language, word relationships, and nuances in word meanings."^^xsd:string .

:CCSS.Math.Content.HSS.MD.B.6 rdf:type owl:Class ;
    rdfs:subClassOf :CCSS.Math.Content.HSS.MD.B ;
    prov:wasQuotedFrom <http://www.corestandards.org/Math/Content/HSS/6/> ;
    rdfs:label "English Language Arts Standards - Anchor Standards - College and Career Readiness Anchor Standards for Language - 6"^^xsd:string ;
    rdfs:comment "Acquire and use accurately a range of general academic and domain-specific words and phrases sufficient for reading, writing, speaking, and listening at the college and career readiness level; demonstrate independence in gathering vocabulary knowledge when encountering an unknown term important to comprehension or expression."^^xsd:string .

:CCSS.Math.Content.HSS.MD.B.7 rdf:type owl:Class ;
    rdfs:subClassOf :CCSS.Math.Content.HSS.MD.B ;
    prov:wasQuotedFrom <http://www.corestandards.org/Math/Content/HSS/7/> ;
    rdfs:label "English Language Arts Standards - Anchor Standards - College and Career Readiness Anchor Standards for Reading - 7"^^xsd:string ;
    rdfs:comment "Integrate and evaluate content presented in diverse media and formats, including visually and quantitatively, as well as in words.1"^^xsd:string .

:CCSS.Math.Content.HSS.ID.B.6.a rdf:type owl:Class ;
    rdfs:subClassOf :CCSS.Math.Content.HSS.ID.B.6 ;
    prov:wasQuotedFrom <http://www.corestandards.org/Math/Content/HSS/ID/a/> .

:CCSS.Math.Content.HSS.ID.B.6.b rdf:type owl:Class ;
    rdfs:subClassOf :CCSS.Math.Content.HSS.ID.B.6 ;
    prov:wasQuotedFrom <http://www.corestandards.org/Math/Content/HSS/ID/b/> .

:CCSS.Math.Content.HSS.ID.B.6.c rdf:type owl:Class ;
    rdfs:subClassOf :CCSS.Math.Content.HSS.ID.B.6 ;
    prov:wasQuotedFrom <http://www.corestandards.org/Math/Content/HSS/ID/c/> .

:CCSS.Math.Content.HSS.MD.B.5.a rdf:type owl:Class ;
    rdfs:subClassOf :CCSS.Math.Content.HSS.MD.B.5 ;
    prov:wasQuotedFrom <http://www.corestandards.org/Math/Content/HSS/MD/a/> .

:CCSS.Math.Content.HSS.MD.B.5.b rdf:type owl:Class ;
    rdfs:subClassOf :CCSS.Math.Content.HSS.MD.B.5 ;
    prov:wasQuotedFrom <http://www.corestandards.org/Math/Content/HSS/MD/b/> .

:CCSS.Math.Content.note-on-courses-transitions rdf:type owl:Class ;
    rdfs:subClassOf :CCSS.Math.Content ;
    rdfs:label "Note on courses & transitions"^^xsd:string ;
    prov:wasQuotedFrom <http://www.corestandards.org/Math/Content/note-on-courses-transitions/> .

:CCSS.Math.Content.note-on-courses-transitions.courses-transitions rdf:type owl:Class ;
    rdfs:subClassOf :CCSS.Math.Content.note-on-courses-transitions ;
    prov:wasQuotedFrom <http://www.corestandards.org/Math/Content/note-on-courses-transitions/courses-transitions/> ;
    rdfs:label "Note on courses & transitions - Courses & Transitions"^^xsd:string ;
    rdfs:comment "The high school portion of the Standards for Mathematical Content specifies the mathematics all students should study for college and career readiness. These standards do not mandate the sequence of high school courses. However, the organization of high school courses is a critical component to implementation of the standards. To that end, sample high school pathways for mathematics - in both a traditional course sequence (Algebra I, Geometry, and Algebra II) as well as an integrated course sequence (Mathematics 1, Mathematics 2, Mathematics 3) - will be made available shortly after the release of the final Common Core State Standards. It is expected that additional model pathways based on these standards will become available as well."^^xsd:string .

